PREFIX cs: <http://resource.geosciml.org/vocabulary/timescale/skos-demo>
PREFIX dcterms: <http://purl.org/dc/terms/>
PREFIX isc: <http://resource.geosciml.org/classifier/ics/ischart/>
PREFIX prov: <http://www.w3.org/ns/prov#>
PREFIX rdfs: <http://www.w3.org/2000/01/rdf-schema#>
PREFIX skos: <http://www.w3.org/2004/02/skos/core#>
PREFIX ts: <http://resource.geosciml.org/vocabulary/timescale/>
PREFIX xsd: <http://www.w3.org/2001/XMLSchema#>

isc:BaseAeronianSP
    dcterms:identifier "BaseAeronianSP" ;
    a skos:Concept ;
    rdfs:isDefinedBy ts:gts2020 ;
    skos:definition "A time period with the following approximated bounds: Trefawr Track Section, Wales, UK" ;
    skos:inScheme cs: ;
    skos:prefLabel "Stratotype Point Base of Aeronian"@en ;
    prov:wasDerivedFrom ts:gts2020 ;
.

isc:BaseAlbianSP
    dcterms:identifier "BaseAlbianSP" ;
    a skos:Concept ;
    rdfs:isDefinedBy ts:gts2020 ;
    skos:definition "A time period with the following approximated bounds: Southeastern France" ;
    skos:inScheme cs: ;
    skos:prefLabel "Stratotype Point Base of Albian"@en ;
    prov:wasDerivedFrom ts:gts2020 ;
.

isc:BaseAptianSP
    dcterms:identifier "BaseAptianSP" ;
    a skos:Concept ;
    rdfs:isDefinedBy ts:gts2020 ;
    skos:definition "A time period with the following approximated bounds: candidate is Gorgo a Cerbara, Piobbico, Umbria-Marche, central Italy" ;
    skos:inScheme cs: ;
    skos:prefLabel "Stratotype Point Base of Aptian"@en ;
    prov:wasDerivedFrom ts:gts2020 ;
.

isc:BaseArtinskianSP
    dcterms:identifier "BaseArtinskianSP" ;
    a skos:Concept ;
    rdfs:isDefinedBy ts:gts2020 ;
    skos:definition "A time period with the following approximated bounds: candidate is Usolka section, Russia" ;
    skos:inScheme cs: ;
    skos:prefLabel "Stratotype Point Base of Artinskian"@en ;
    prov:wasDerivedFrom ts:gts2020 ;
.

isc:BaseBajocianSP
    dcterms:identifier "BaseBajocianSP" ;
    a skos:Concept ;
    rdfs:isDefinedBy ts:gts2020 ;
    skos:definition "A time period with the following approximated bounds: Murtinheira Section, Cabo Mondego, Portugal " ;
    skos:inScheme cs: ;
    skos:prefLabel "Stratotype Point Base of Bajocian"@en ;
    prov:wasDerivedFrom ts:gts2020 ;
.

isc:BaseBarremianSP
    dcterms:identifier "BaseBarremianSP" ;
    a skos:Concept ;
    rdfs:isDefinedBy ts:gts2020 ;
    skos:definition "A time period with the following approximated bounds: candidate is Río Argos near Caravaca, Murcia Province, Spain" ;
    skos:inScheme cs: ;
    skos:prefLabel "Stratotype Point Base of Barremian"@en ;
    prov:wasDerivedFrom ts:gts2020 ;
.

isc:BaseBartonianSP
    dcterms:identifier "BaseBartonianSP" ;
    a skos:Concept ;
    rdfs:isDefinedBy ts:gts2020 ;
    skos:definition "A time period with the following approximated bounds: Contessa highway section near Gubio, Central Apennines, Italy" ;
    skos:inScheme cs: ;
    skos:prefLabel "Stratotype Point Base of Bartonian"@en ;
    prov:wasDerivedFrom ts:gts2020 ;
.

isc:BaseBathonianSP
    dcterms:identifier "BaseBathonianSP" ;
    a skos:Concept ;
    rdfs:isDefinedBy ts:gts2020 ;
    skos:definition "A time period with the following approximated bounds: Ravin du Bes, Bas Auran area, Alpes de Haute Provence, France  " ;
    skos:inScheme cs: ;
    skos:prefLabel "Stratotype Point Base of Bathonian"@en ;
    prov:wasDerivedFrom ts:gts2020 ;
.

isc:BaseBurdigalianSP
    dcterms:identifier "BaseBurdigalianSP" ;
    a skos:Concept ;
    rdfs:isDefinedBy ts:gts2020 ;
    skos:definition "A time period with the following approximated bounds: Potentially in astronomically tuned ODP core" ;
    skos:inScheme cs: ;
    skos:prefLabel "Stratotype Point Base of Burdigalian"@en ;
    prov:wasDerivedFrom ts:gts2020 ;
.

isc:BaseCalabrianSP
    dcterms:identifier "BaseCalabrianSP" ;
    a skos:Concept ;
    rdfs:isDefinedBy ts:gts2020 ;
    skos:definition "A time period with the following approximated bounds: Vrica, Italy" ;
    skos:inScheme cs: ;
    skos:prefLabel "Stratotype Point Base of Calabrian"@en ;
    prov:wasDerivedFrom ts:gts2020 ;
.

isc:BaseCallovianSP
    dcterms:identifier "BaseCallovianSP" ;
    a skos:Concept ;
    rdfs:isDefinedBy ts:gts2020 ;
    skos:definition "A time period with the following approximated bounds: candidates are Pfeffingen (Swabian Alb, SW Germany) and in Russia" ;
    skos:inScheme cs: ;
    skos:prefLabel "Stratotype Point Base of Callovian"@en ;
    prov:wasDerivedFrom ts:gts2020 ;
.

isc:BaseCambrianStage10SP
    dcterms:identifier "BaseCambrianStage10SP" ;
    a skos:Concept ;
    rdfs:isDefinedBy ts:gts2020 ;
    skos:definition "A time period with the following approximated bounds: candidate section is Duibian (Zhejiang province, China)" ;
    skos:inScheme cs: ;
    skos:prefLabel "Stratotype Point Base of Cambrian Stage 10"@en ;
    prov:wasDerivedFrom ts:gts2020 ;
.

isc:BaseCampanianSP
    dcterms:identifier "BaseCampanianSP" ;
    a skos:Concept ;
    rdfs:isDefinedBy ts:gts2020 ;
    skos:definition "A time period with the following approximated bounds: candidates are in Italy and in Texas" ;
    skos:inScheme cs: ;
    skos:prefLabel "Stratotype Point Base of Campanian"@en ;
    prov:wasDerivedFrom ts:gts2020 ;
.

isc:BaseCapitanianSP
    dcterms:identifier "BaseCapitanianSP" ;
    a skos:Concept ;
    rdfs:isDefinedBy ts:gts2020 ;
    skos:definition "A time period with the following approximated bounds: Nipple Hill, SE Guadalupe Mountains, Texas, U.S.A" ;
    skos:inScheme cs: ;
    skos:prefLabel "Stratotype Point Base of Capitanian"@en ;
    prov:wasDerivedFrom ts:gts2020 ;
.

isc:BaseCarboniferousSP
    dcterms:identifier "BaseCarboniferousSP" ;
    a skos:Concept ;
    rdfs:isDefinedBy ts:gts2020 ;
    skos:definition "A time period with the following approximated bounds: La Serre, France" ;
    skos:inScheme cs: ;
    skos:prefLabel "Stratotype Point Base of Tournaisian"@en ;
    prov:wasDerivedFrom ts:gts2020 ;
.

isc:BaseCenozoicSP
    dcterms:identifier "BaseCenozoicSP" ;
    a skos:Concept ;
    rdfs:isDefinedBy ts:gts2020 ;
    skos:definition "A time period with the following approximated bounds: Oued Djerfane, west of El Kef, Tunisia" ;
    skos:inScheme cs: ;
    skos:prefLabel "Stratotype Point Base of Danian"@en ;
    prov:wasDerivedFrom ts:gts2020 ;
.

isc:BaseChanghsingianSP
    dcterms:identifier "BaseChanghsingianSP" ;
    a skos:Concept ;
    rdfs:isDefinedBy ts:gts2020 ;
    skos:definition "A time period with the following approximated bounds: Meishan, Zhejiang Province, China" ;
    skos:inScheme cs: ;
    skos:prefLabel "Stratotype Point Base of Changhsingian"@en ;
    prov:wasDerivedFrom ts:gts2020 ;
.

isc:BaseChattianSP
    dcterms:identifier "BaseChattianSP" ;
    a skos:Concept ;
    rdfs:isDefinedBy ts:gts2020 ;
    skos:definition "A time period with the following approximated bounds: Monte Cagnero, Umbria-Marche region, Italy" ;
    skos:inScheme cs: ;
    skos:prefLabel "Stratotype Point Base of Chattian"@en ;
    prov:wasDerivedFrom ts:gts2020 ;
.

isc:BaseConiacianSP
    dcterms:identifier "BaseConiacianSP" ;
    a skos:Concept ;
    rdfs:isDefinedBy ts:gts2020 ;
    skos:definition "A time period with the following approximated bounds: candidates are in Poland (Slupia Nadbrzena), USA (Pueblo, Colorado), and Germany (Salzgitter-Salder Quarry)" ;
    skos:inScheme cs: ;
    skos:prefLabel "Stratotype Point Base of Coniaician"@en ;
    prov:wasDerivedFrom ts:gts2020 ;
.

isc:BaseCryogenianSP
    dcterms:identifier "BaseCryogenianSP" ;
    a skos:Concept ;
    rdfs:isDefinedBy ts:gts2020 ;
    skos:definition "A time period with the following approximated bounds: Onset of the first global glaciation. First glacial episode occurred after 750 Ma" ;
    skos:inScheme cs: ;
    skos:prefLabel "Stratotype Point Base of Cryogenian"@en ;
    prov:wasDerivedFrom ts:gts2020 ;
.

isc:BaseDarriwilianSP
    dcterms:identifier "BaseDarriwilianSP" ;
    a skos:Concept ;
    rdfs:isDefinedBy ts:gts2020 ;
    skos:definition "A time period with the following approximated bounds: Huangnitang section, Changshan, Zhejiang Province, SE China" ;
    skos:inScheme cs: ;
    skos:prefLabel "Stratotype Point Base of Darriwilian"@en ;
    prov:wasDerivedFrom ts:gts2020 ;
.

isc:BaseDevonianSP
    dcterms:identifier "BaseDevonianSP" ;
    a skos:Concept ;
    rdfs:isDefinedBy ts:gts2020 ;
    skos:definition "A time period with the following approximated bounds: Klonk, near Prague, Czech Republic" ;
    skos:inScheme cs: ;
    skos:prefLabel "Stratotype Point Base of Lochkovian"@en ;
    prov:wasDerivedFrom ts:gts2020 ;
.

isc:BaseDrumianSP
    dcterms:identifier "BaseDrumianSP" ;
    a skos:Concept ;
    rdfs:isDefinedBy ts:gts2020 ;
    skos:definition "A time period with the following approximated bounds: Drum Mountains, Millard County, Utah, USA" ;
    skos:inScheme cs: ;
    skos:prefLabel "Stratotype Point Base of Drumian"@en ;
    prov:wasDerivedFrom ts:gts2020 ;
.

isc:BaseEdiacaranSP
    dcterms:identifier "BaseEdiacaranSP" ;
    a skos:Concept ;
    rdfs:isDefinedBy ts:gts2020 ;
    skos:definition "A time period with the following approximated bounds: Enorama Creek, Flinders Ranges, South Australia" ;
    skos:inScheme cs: ;
    skos:prefLabel "Stratotype Point Base of Ediacaran"@en ;
    prov:wasDerivedFrom ts:gts2020 ;
.

isc:BaseEmsianSP
    dcterms:identifier "BaseEmsianSP" ;
    a skos:Concept ;
    rdfs:isDefinedBy ts:gts2020 ;
    skos:definition "A time period with the following approximated bounds: Zinzil'ban Gorge in the Kitab State Geological Reserve, Uzbekistan" ;
    skos:inScheme cs: ;
    skos:prefLabel "Stratotype Point Base of Emsian"@en ;
    prov:wasDerivedFrom ts:gts2020 ;
.

isc:BaseEoceneSP
    dcterms:identifier "BaseEoceneSP" ;
    a skos:Concept ;
    rdfs:isDefinedBy ts:gts2020 ;
    skos:definition "A time period with the following approximated bounds: Dababiya, near Luxor, Egypt" ;
    skos:inScheme cs: ;
    skos:prefLabel "Stratotype Point Base of Ypresian"@en ;
    prov:wasDerivedFrom ts:gts2020 ;
.

isc:BaseFamennianSP
    dcterms:identifier "BaseFamennianSP" ;
    a skos:Concept ;
    rdfs:isDefinedBy ts:gts2020 ;
    skos:definition "A time period with the following approximated bounds: Coumiac Quarry, near Cessenon, Montagne Noire, France" ;
    skos:inScheme cs: ;
    skos:prefLabel "Stratotype Point Base of Famennian"@en ;
    prov:wasDerivedFrom ts:gts2020 ;
.

isc:BaseFloianSP
    dcterms:identifier "BaseFloianSP" ;
    a skos:Concept ;
    rdfs:isDefinedBy ts:gts2020 ;
    skos:definition "A time period with the following approximated bounds: Diabasbrottet, Hunneberg, Sweden" ;
    skos:inScheme cs: ;
    skos:prefLabel "Stratotype Point Base of Floian"@en ;
    prov:wasDerivedFrom ts:gts2020 ;
.

isc:BaseFurongianSP
    dcterms:identifier "BaseFurongianSP" ;
    a skos:Concept ;
    rdfs:isDefinedBy ts:gts2020 ;
    skos:definition "A time period with the following approximated bounds: Wuling Mountains, Huayuan County, NW Hunan Province, China" ;
    skos:inScheme cs: ;
    skos:prefLabel "Stratotype Point Base of Paibian"@en ;
    prov:wasDerivedFrom ts:gts2020 ;
.

isc:BaseGivetianSP
    dcterms:identifier "BaseGivetianSP" ;
    a skos:Concept ;
    rdfs:isDefinedBy ts:gts2020 ;
    skos:definition "A time period with the following approximated bounds: Jebel Mech Irdane, Morocco" ;
    skos:inScheme cs: ;
    skos:prefLabel "Stratotype Point Base of Givetian"@en ;
    prov:wasDerivedFrom ts:gts2020 ;
.

isc:BaseGuadalupianSP
    dcterms:identifier "BaseGuadalupianSP" ;
    a skos:Concept ;
    rdfs:isDefinedBy ts:gts2020 ;
    skos:definition "A time period with the following approximated bounds: Stratotype Canyon, Texas, U.S.A" ;
    skos:inScheme cs: ;
    skos:prefLabel "Stratotype Point Base of Guadalupian"@en ;
    prov:wasDerivedFrom ts:gts2020 ;
.

isc:BaseGuzhangianSP
    dcterms:identifier "BaseGuzhangianSP" ;
    a skos:Concept ;
    rdfs:isDefinedBy ts:gts2020 ;
    skos:definition "A time period with the following approximated bounds: Louyixi, Guzhang County, NW Hunan Province, S. China" ;
    skos:inScheme cs: ;
    skos:prefLabel "Stratotype Point Base of Guzhangian "@en ;
    prov:wasDerivedFrom ts:gts2020 ;
.

isc:BaseGzhelianSP
    dcterms:identifier "BaseGzhelianSP" ;
    a skos:Concept ;
    rdfs:isDefinedBy ts:gts2020 ;
    skos:definition "A time period with the following approximated bounds: candidates are in southern Urals or Nashui (south China)." ;
    skos:inScheme cs: ;
    skos:prefLabel "Stratotype Point Base of Gzhelian"@en ;
    prov:wasDerivedFrom ts:gts2020 ;
.

isc:BaseHauterivianSP
    dcterms:identifier "BaseHauterivianSP" ;
    a skos:Concept ;
    rdfs:isDefinedBy ts:gts2020 ;
    skos:definition "A time period with the following approximated bounds: La Charce village, Drôme Province, southeast France" ;
    skos:inScheme cs: ;
    skos:prefLabel "Stratotype Point Base of Hauterivian"@en ;
    prov:wasDerivedFrom ts:gts2020 ;
.

isc:BaseHirnantianSP
    dcterms:identifier "BaseHirnantianSP" ;
    a skos:Concept ;
    rdfs:isDefinedBy ts:gts2020 ;
    skos:definition "A time period with the following approximated bounds: Wangjiawan North section, N of Yichang city, Western Hubei Province, China" ;
    skos:inScheme cs: ;
    skos:prefLabel "Stratotype Point Base of Hirnantian"@en ;
    prov:wasDerivedFrom ts:gts2020 ;
.

isc:BaseHoloceneSP
    dcterms:identifier "BaseHoloceneSP" ;
    a skos:Concept ;
    rdfs:isDefinedBy ts:gts2020 ;
    skos:definition "A time period with the following approximated bounds: NorthGRIP2 ice core, central Greenland" ;
    skos:inScheme cs: ;
    skos:prefLabel "Stratotype Point Base of Greenlandian"@en ;
    prov:wasDerivedFrom ts:gts2020 ;
.

isc:BaseHomerianSP
    dcterms:identifier "BaseHomerianSP" ;
    a skos:Concept ;
    rdfs:isDefinedBy ts:gts2020 ;
    skos:definition "A time period with the following approximated bounds: Sheinton Brook, Homer, UK" ;
    skos:inScheme cs: ;
    skos:prefLabel "Stratotype Point Base of Homerian"@en ;
    prov:wasDerivedFrom ts:gts2020 ;
.

isc:BaseJiangshanianSP
    dcterms:identifier "BaseJiangshanianSP" ;
    a skos:Concept ;
    rdfs:isDefinedBy ts:gts2020 ;
    skos:definition "A time period with the following approximated bounds: Duibian B section, Zhejiang province, China" ;
    skos:inScheme cs: ;
    skos:prefLabel "Stratotype Point Base of Jiangshanian"@en ;
    prov:wasDerivedFrom ts:gts2020 ;
.

isc:BaseJurassicSP
    dcterms:identifier "BaseJurassicSP" ;
    a skos:Concept ;
    rdfs:isDefinedBy ts:gts2020 ;
    skos:definition "A time period with the following approximated bounds: Kuhjoch section,Tyrol, Austria " ;
    skos:inScheme cs: ;
    skos:prefLabel "Stratotype Point Base of Hettangian"@en ;
    prov:wasDerivedFrom ts:gts2020 ;
.

isc:BaseKatianSP
    dcterms:identifier "BaseKatianSP" ;
    a skos:Concept ;
    rdfs:isDefinedBy ts:gts2020 ;
    skos:definition "A time period with the following approximated bounds: Black Knob Ridge Section, Atoka, Oklahoma (USA)" ;
    skos:inScheme cs: ;
    skos:prefLabel "Stratotype Point Base of Katian"@en ;
    prov:wasDerivedFrom ts:gts2020 ;
.

isc:BaseKimmeridgianSP
    dcterms:identifier "BaseKimmeridgianSP" ;
    a skos:Concept ;
    rdfs:isDefinedBy ts:gts2020 ;
    skos:definition "A time period with the following approximated bounds: candidate is Flodigarry (Isle of Skye, NW Scotland)" ;
    skos:inScheme cs: ;
    skos:prefLabel "Stratotype Point Base of Kimmeridgian"@en ;
    prov:wasDerivedFrom ts:gts2020 ;
.

isc:BaseKungurianSP
    dcterms:identifier "BaseKungurianSP" ;
    a skos:Concept ;
    rdfs:isDefinedBy ts:gts2020 ;
    skos:definition "A time period with the following approximated bounds: candidate Pequob Mtns., Nevada, USA." ;
    skos:inScheme cs: ;
    skos:prefLabel "Stratotype Point Base of Kungurian"@en ;
    prov:wasDerivedFrom ts:gts2020 ;
.

isc:BaseLadinianSP
    dcterms:identifier "BaseLadinianSP" ;
    a skos:Concept ;
    rdfs:isDefinedBy ts:gts2020 ;
    skos:definition "A time period with the following approximated bounds: Bagolino, Province of Brescia, Northern Italy" ;
    skos:inScheme cs: ;
    skos:prefLabel "Stratotype Point Base of Ladinian"@en ;
    prov:wasDerivedFrom ts:gts2020 ;
.

isc:BaseLanghianSP
    dcterms:identifier "BaseLanghianSP" ;
    a skos:Concept ;
    rdfs:isDefinedBy ts:gts2020 ;
    skos:definition "A time period with the following approximated bounds: Potentially in astronomically tuned ODP core (Leg 154) or in Italy (Moria or La Vedova), St. Peter's Pool, Malta or La Vedova,Italy" ;
    skos:inScheme cs: ;
    skos:prefLabel "Stratotype Point Base of Langhian"@en ;
    prov:wasDerivedFrom ts:gts2020 ;
.

isc:BaseLatePleistocene
    dcterms:identifier "BaseLatePleistocene" ;
    a skos:Concept ;
    rdfs:isDefinedBy ts:gts2020 ;
    skos:definition "A time period with the following approximated bounds: The age sought is near the mid-point of Termination II in the marine isotope stratigraphy." ;
    skos:inScheme cs: ;
    skos:prefLabel "Base of Late Pleistocene"@en ;
    prov:wasDerivedFrom ts:gts2020 ;
.

isc:BaseLopingianSP
    dcterms:identifier "BaseLopingianSP" ;
    a skos:Concept ;
    rdfs:isDefinedBy ts:gts2020 ;
    skos:definition "A time period with the following approximated bounds: Penglaitan, Guanxi Province, South China" ;
    skos:inScheme cs: ;
    skos:prefLabel "Stratotype Point Base of Wuchiapingian"@en ;
    prov:wasDerivedFrom ts:gts2020 ;
.

isc:BaseLudfordianSP
    dcterms:identifier "BaseLudfordianSP" ;
    a skos:Concept ;
    rdfs:isDefinedBy ts:gts2020 ;
    skos:definition "A time period with the following approximated bounds: near Ludlow, UK" ;
    skos:inScheme cs: ;
    skos:prefLabel "Stratotype Point Base of Ludfordian"@en ;
    prov:wasDerivedFrom ts:gts2020 ;
.

isc:BaseLudlowSP
    dcterms:identifier "BaseLudlowSP" ;
    a skos:Concept ;
    rdfs:isDefinedBy ts:gts2020 ;
    skos:definition "A time period with the following approximated bounds: near Ludlow, UK" ;
    skos:inScheme cs: ;
    skos:prefLabel "Stratotype Point Base of Gorstian"@en ;
    prov:wasDerivedFrom ts:gts2020 ;
.

isc:BaseLutetianSP
    dcterms:identifier "BaseLutetianSP" ;
    a skos:Concept ;
    rdfs:isDefinedBy ts:gts2020 ;
    skos:definition "A time period with the following approximated bounds: Gorrondatxe sea-cliff section,Basque Country, northern Spain" ;
    skos:inScheme cs: ;
    skos:prefLabel "Stratotype Point Base of Lutetian"@en ;
    prov:wasDerivedFrom ts:gts2020 ;
.

isc:BaseMaastrichtianSP
    dcterms:identifier "BaseMaastrichtianSP" ;
    a skos:Concept ;
    rdfs:isDefinedBy ts:gts2020 ;
    skos:definition "A time period with the following approximated bounds: Tercis les Bains, Landes, France" ;
    skos:inScheme cs: ;
    skos:prefLabel "Stratotype Point Base of Maastrichtian"@en ;
    prov:wasDerivedFrom ts:gts2020 ;
.

isc:BaseMeghalayanAuxSP
    dcterms:identifier "BaseMeghalayanAuxSP" ;
    a skos:Concept ;
    rdfs:isDefinedBy ts:gts2020 ;
    skos:definition "A time period with the following approximated bounds: Global Auxiliary Stratotype, Mount Logan ice core, Canada" ;
    skos:inScheme cs: ;
    skos:prefLabel "Auxiliary Stratotype Point Base of Meghalayan"@en ;
    prov:wasDerivedFrom ts:gts2020 ;
.

isc:BaseMeghalayanSP
    dcterms:identifier "BaseMeghalayanSP" ;
    a skos:Concept ;
    rdfs:isDefinedBy ts:gts2020 ;
    skos:definition "A time period with the following approximated bounds: Mawmluh Cave, Meghalaya,India" ;
    skos:inScheme cs: ;
    skos:prefLabel "Stratotype Point Base of Meghalayan"@en ;
    prov:wasDerivedFrom ts:gts2020 ;
.

isc:BaseMesozoicSP
    dcterms:identifier "BaseMesozoicSP" ;
    a skos:Concept ;
    rdfs:isDefinedBy ts:gts2020 ;
    skos:definition "A time period with the following approximated bounds: Meishan, Zhejiang Province, China" ;
    skos:inScheme cs: ;
    skos:prefLabel "Stratotype Point Base of Induan"@en ;
    prov:wasDerivedFrom ts:gts2020 ;
.

isc:BaseMessinianSP
    dcterms:identifier "BaseMessinianSP" ;
    a skos:Concept ;
    rdfs:isDefinedBy ts:gts2020 ;
    skos:definition "A time period with the following approximated bounds: Oued Akrech, Morocco" ;
    skos:inScheme cs: ;
    skos:prefLabel "Stratotype Point Base of Messinian"@en ;
    prov:wasDerivedFrom ts:gts2020 ;
.

isc:BaseMiaolingianSP
    dcterms:identifier "BaseMiaolingianSP" ;
    a skos:Concept ;
    rdfs:isDefinedBy ts:gts2020 ;
    skos:definition "A time period with the following approximated bounds: Wuliu-Zengjiayan (east Guizhou, China)" ;
    skos:inScheme cs: ;
    skos:prefLabel "Stratotype Point Base of Wuliuan"@en ;
    prov:wasDerivedFrom ts:gts2020 ;
.

isc:BaseMiddleDevonianSP
    dcterms:identifier "BaseMiddleDevonianSP" ;
    a skos:Concept ;
    rdfs:isDefinedBy ts:gts2020 ;
    skos:definition "A time period with the following approximated bounds: Wetteldorf, Eifel Hills, Germany" ;
    skos:inScheme cs: ;
    skos:prefLabel "Stratotype Point Base of Eifelian"@en ;
    prov:wasDerivedFrom ts:gts2020 ;
.

isc:BaseMiddleJurassicSP
    dcterms:identifier "BaseMiddleJurassicSP" ;
    a skos:Concept ;
    rdfs:isDefinedBy ts:gts2020 ;
    skos:definition "A time period with the following approximated bounds: Fuentelsaz, Spain " ;
    skos:inScheme cs: ;
    skos:prefLabel "Stratotype Point Base of Aalenian"@en ;
    prov:wasDerivedFrom ts:gts2020 ;
.

isc:BaseMiddleMississippianSP
    dcterms:identifier "BaseMiddleMississippianSP" ;
    a skos:Concept ;
    rdfs:isDefinedBy ts:gts2020 ;
    skos:definition "A time period with the following approximated bounds: Pengchong, south China" ;
    skos:inScheme cs: ;
    skos:prefLabel "Stratotype Point Base of Visean"@en ;
    prov:wasDerivedFrom ts:gts2020 ;
.

isc:BaseMiddleOrdovicianSP
    dcterms:identifier "BaseMiddleOrdovicianSP" ;
    a skos:Concept ;
    rdfs:isDefinedBy ts:gts2020 ;
    skos:definition "A time period with the following approximated bounds: Huanghuachang Section, NE of Yichang city, Hubei Province, S. China" ;
    skos:inScheme cs: ;
    skos:prefLabel "Stratotype Point Base of Dapingian"@en ;
    prov:wasDerivedFrom ts:gts2020 ;
.

isc:BaseMiddlePennsylvanianSP
    dcterms:identifier "BaseMiddlePennsylvanianSP" ;
    a skos:Concept ;
    rdfs:isDefinedBy ts:gts2020 ;
    skos:definition "A time period with the following approximated bounds: candidates are in southern Urals or Nashui (south China)." ;
    skos:inScheme cs: ;
    skos:prefLabel "Stratotype Point Base of Moscovian"@en ;
    prov:wasDerivedFrom ts:gts2020 ;
.

isc:BaseMiddleTriassicSP
    dcterms:identifier "BaseMiddleTriassicSP" ;
    a skos:Concept ;
    rdfs:isDefinedBy ts:gts2020 ;
    skos:definition "A time period with the following approximated bounds: Candidate section at Desli Caira (Dobrogea, Romania); significant sections in Guizhou Province (China) and South Primorye (Russia)" ;
    skos:inScheme cs: ;
    skos:prefLabel "Stratotype Point Base of Anisian"@en ;
    prov:wasDerivedFrom ts:gts2020 ;
.

isc:BaseNeogeneSP
    dcterms:identifier "BaseNeogeneSP" ;
    a skos:Concept ;
    rdfs:isDefinedBy ts:gts2020 ;
    skos:definition "A time period with the following approximated bounds: Lemme Carrioso Section, Allessandria Province, Italy" ;
    skos:inScheme cs: ;
    skos:prefLabel "Stratotype Point Base of Aquitainian"@en ;
    prov:wasDerivedFrom ts:gts2020 ;
.

isc:BaseNorianSP
    dcterms:identifier "BaseNorianSP" ;
    a skos:Concept ;
    rdfs:isDefinedBy ts:gts2020 ;
    skos:definition "A time period with the following approximated bounds: Candidates are Black Bear Ridge in British Columbia (Canada) and Pizzo Mondello, Sicily (Italy)" ;
    skos:inScheme cs: ;
    skos:prefLabel "Stratotype Point Base of Norian"@en ;
    prov:wasDerivedFrom ts:gts2020 ;
.

isc:BaseNorthgrippianAuxSP
    dcterms:identifier "BaseNorthgrippianAuxSP" ;
    a skos:Concept ;
    rdfs:isDefinedBy ts:gts2020 ;
    skos:definition "A time period with the following approximated bounds: Global AuxiliaryStratotype: Gruta do Padre Cave speleothem, Brazil" ;
    skos:inScheme cs: ;
    skos:prefLabel "Auxiliary Stratotype Point Base of Northgrippian"@en ;
    prov:wasDerivedFrom ts:gts2020 ;
.

isc:BaseNorthgrippianSP
    dcterms:identifier "BaseNorthgrippianSP" ;
    a skos:Concept ;
    rdfs:isDefinedBy ts:gts2020 ;
    skos:definition "A time period with the following approximated bounds: Global AuxiliaryStratotype: Gruta do Padre Cave speleothem, Brazil, NorthGRIP1 ice core, Greenland, NorthGRIP1 ice core, Greenland." ;
    skos:inScheme cs: ;
    skos:prefLabel "Stratotype Point Base of Northgrippian"@en ;
    prov:wasDerivedFrom ts:gts2020 ;
.

isc:BaseOlenekianSP
    dcterms:identifier "BaseOlenekianSP" ;
    a skos:Concept ;
    rdfs:isDefinedBy ts:gts2020 ;
    skos:definition "A time period with the following approximated bounds: Candidate Stratotype Point Mud (Muth) village, Spiti valley, northwest India" ;
    skos:inScheme cs: ;
    skos:prefLabel "Stratotype Point Base of Olenekian"@en ;
    prov:wasDerivedFrom ts:gts2020 ;
.

isc:BaseOligoceneSP
    dcterms:identifier "BaseOligoceneSP" ;
    a skos:Concept ;
    rdfs:isDefinedBy ts:gts2020 ;
    skos:definition "A time period with the following approximated bounds: Massignano, near Ancona, Italy" ;
    skos:inScheme cs: ;
    skos:prefLabel "Stratotype Point Base of Rupelian"@en ;
    prov:wasDerivedFrom ts:gts2020 ;
.

isc:BaseOrdovicianSP
    dcterms:identifier "BaseOrdovicianSP" ;
    a skos:Concept ;
    rdfs:isDefinedBy ts:gts2020 ;
    skos:definition "A time period with the following approximated bounds: Green Point Section, western Newfoundland" ;
    skos:inScheme cs: ;
    skos:prefLabel "Stratotype Point Base of Tremadocian"@en ;
    prov:wasDerivedFrom ts:gts2020 ;
.

isc:BasePennsylvanianSP
    dcterms:identifier "BasePennsylvanianSP" ;
    a skos:Concept ;
    rdfs:isDefinedBy ts:gts2020 ;
    skos:definition "A time period with the following approximated bounds: Arrow Canyon, Nevada" ;
    skos:inScheme cs: ;
    skos:prefLabel "Stratotype Point Base of Bashkirian"@en ;
    prov:wasDerivedFrom ts:gts2020 ;
.

isc:BasePermianSP
    dcterms:identifier "BasePermianSP" ;
    a skos:Concept ;
    rdfs:isDefinedBy ts:gts2020 ;
    skos:definition "A time period with the following approximated bounds: Aidaralash Creek, Kazakhstan" ;
    skos:inScheme cs: ;
    skos:prefLabel "Stratotype Point Base of Asselian"@en ;
    prov:wasDerivedFrom ts:gts2020 ;
.

isc:BasePhanerozoicSP
    dcterms:identifier "BasePhanerozoicSP" ;
    a skos:Concept ;
    rdfs:isDefinedBy ts:gts2020 ;
    skos:definition "A time period with the following approximated bounds: Fortune Head, SE Newfoundland, Canada" ;
    skos:inScheme cs: ;
    skos:prefLabel "Stratotype Point Base of Fortunian"@en ;
    prov:wasDerivedFrom ts:gts2020 ;
.

isc:BasePiacenzianSP
    dcterms:identifier "BasePiacenzianSP" ;
    a skos:Concept ;
    rdfs:isDefinedBy ts:gts2020 ;
    skos:definition "A time period with the following approximated bounds: Punta Piccola, Sicily, Italy" ;
    skos:inScheme cs: ;
    skos:prefLabel "Stratotype Point Base of Piacenzian"@en ;
    prov:wasDerivedFrom ts:gts2020 ;
.

isc:BasePliensbachianSP
    dcterms:identifier "BasePliensbachianSP" ;
    a skos:Concept ;
    rdfs:isDefinedBy ts:gts2020 ;
    skos:definition "A time period with the following approximated bounds: Wine Haven, Robin Hoods Bay, Yorkshire Coast, England " ;
    skos:inScheme cs: ;
    skos:prefLabel "Stratotype Point Base of Pliensbachian"@en ;
    prov:wasDerivedFrom ts:gts2020 ;
.

isc:BasePlioceneSP
    dcterms:identifier "BasePlioceneSP" ;
    a skos:Concept ;
    rdfs:isDefinedBy ts:gts2020 ;
    skos:definition "A time period with the following approximated bounds: Eraclea Minoa, Sicily, Italy" ;
    skos:inScheme cs: ;
    skos:prefLabel "Stratotype Point Base of Zanclean"@en ;
    prov:wasDerivedFrom ts:gts2020 ;
.

isc:BasePragianSP
    dcterms:identifier "BasePragianSP" ;
    a skos:Concept ;
    rdfs:isDefinedBy ts:gts2020 ;
    skos:definition "A time period with the following approximated bounds: Velka Chuchle, Prague, Czech Republic" ;
    skos:inScheme cs: ;
    skos:prefLabel "Stratotype Point Base of Pragian"@en ;
    prov:wasDerivedFrom ts:gts2020 ;
.

isc:BasePriabonianSP
    dcterms:identifier "BasePriabonianSP" ;
    a skos:Concept ;
    rdfs:isDefinedBy ts:gts2020 ;
    skos:definition "A time period with the following approximated bounds: Alano section, Piave River; Veneto Prealps, Belluno province, N. Italy" ;
    skos:inScheme cs: ;
    skos:prefLabel "Stratotype Point Base of Priabonian"@en ;
    prov:wasDerivedFrom ts:gts2020 ;
.

isc:BasePridoliSP
    dcterms:identifier "BasePridoliSP" ;
    a skos:Concept ;
    rdfs:isDefinedBy ts:gts2020 ;
    skos:definition "A time period with the following approximated bounds: Požáry Section, Reporyje, Prague, Czech Republic" ;
    skos:inScheme cs: ;
    skos:prefLabel "Stratotype Point Base of Přídolí"@en ;
    prov:wasDerivedFrom ts:gts2020 ;
.

isc:BaseQuaternarySP
    dcterms:identifier "BaseQuaternarySP" ;
    a skos:Concept ;
    rdfs:isDefinedBy ts:gts2020 ;
    skos:definition "A time period with the following approximated bounds: Definition as base of Quaternary and Pleistocene ratified 2009, Monte San Nicola, Sicily, Italy" ;
    skos:inScheme cs: ;
    skos:prefLabel "Stratotype Point Base of Gelasian"@en ;
    prov:wasDerivedFrom ts:gts2020 ;
.

isc:BaseRhaetianSP
    dcterms:identifier "BaseRhaetianSP" ;
    a skos:Concept ;
    rdfs:isDefinedBy ts:gts2020 ;
    skos:definition "A time period with the following approximated bounds: Candidates are Pizzo Mondello, Sicily (Italy) and Steinbergkogel, Austria" ;
    skos:inScheme cs: ;
    skos:prefLabel "Stratotype Point Base of Rhaetian"@en ;
    prov:wasDerivedFrom ts:gts2020 ;
.

isc:BaseSakmarianSP
    dcterms:identifier "BaseSakmarianSP" ;
    a skos:Concept ;
    rdfs:isDefinedBy ts:gts2020 ;
    skos:definition "A time period with the following approximated bounds: Kondurovsky, Orenburg Province, Russia." ;
    skos:inScheme cs: ;
    skos:prefLabel "Stratotype Point Base of Sakmarian"@en ;
    prov:wasDerivedFrom ts:gts2020 ;
.

isc:BaseSantonianSP
    dcterms:identifier "BaseSantonianSP" ;
    a skos:Concept ;
    rdfs:isDefinedBy ts:gts2020 ;
    skos:definition "A time period with the following approximated bounds: Olazagutia, Navarra, Spain" ;
    skos:inScheme cs: ;
    skos:prefLabel "Stratotype Point Base of Santonian"@en ;
    prov:wasDerivedFrom ts:gts2020 ;
.

isc:BaseSelandianSP
    dcterms:identifier "BaseSelandianSP" ;
    a skos:Concept ;
    rdfs:isDefinedBy ts:gts2020 ;
    skos:definition "A time period with the following approximated bounds: Zumaia section, northern Spain" ;
    skos:inScheme cs: ;
    skos:prefLabel "Stratotype Point Base of Selandian"@en ;
    prov:wasDerivedFrom ts:gts2020 ;
.

isc:BaseSerravallianSP
    dcterms:identifier "BaseSerravallianSP" ;
    a skos:Concept ;
    rdfs:isDefinedBy ts:gts2020 ;
    skos:definition "A time period with the following approximated bounds: Ras il Pellegrin section, Fomm Ir- Rih Bay, west coast of Malta" ;
    skos:inScheme cs: ;
    skos:prefLabel "Stratotype Point Base of Serravallian"@en ;
    prov:wasDerivedFrom ts:gts2020 ;
.

isc:BaseSilurianSP
    dcterms:identifier "BaseSilurianSP" ;
    a skos:Concept ;
    rdfs:isDefinedBy ts:gts2020 ;
    skos:definition "A time period with the following approximated bounds: Dobs Linn, Scotland" ;
    skos:inScheme cs: ;
    skos:prefLabel "Stratotype Point Base of Rhuddanian"@en ;
    prov:wasDerivedFrom ts:gts2020 ;
.

isc:BaseSinemurianSP
    dcterms:identifier "BaseSinemurianSP" ;
    a skos:Concept ;
    rdfs:isDefinedBy ts:gts2020 ;
    skos:definition "A time period with the following approximated bounds: East Quantoxhead, SW England " ;
    skos:inScheme cs: ;
    skos:prefLabel "Stratotype Point Base of Sinemurian"@en ;
    prov:wasDerivedFrom ts:gts2020 ;
.

isc:BaseTelychianSP
    dcterms:identifier "BaseTelychianSP" ;
    a skos:Concept ;
    rdfs:isDefinedBy ts:gts2020 ;
    skos:definition "A time period with the following approximated bounds: Cefn-cerig Road Section, Wales, UK" ;
    skos:inScheme cs: ;
    skos:prefLabel "Stratotype Point Base of Telychian"@en ;
    prov:wasDerivedFrom ts:gts2020 ;
.

isc:BaseThanetianSP
    dcterms:identifier "BaseThanetianSP" ;
    a skos:Concept ;
    rdfs:isDefinedBy ts:gts2020 ;
    skos:definition "A time period with the following approximated bounds: Zumaia section, northern Spain" ;
    skos:inScheme cs: ;
    skos:prefLabel "Stratotype Point Base of Thanetian"@en ;
    prov:wasDerivedFrom ts:gts2020 ;
.

isc:BaseTithonianSP
    dcterms:identifier "BaseTithonianSP" ;
    a skos:Concept ;
    rdfs:isDefinedBy ts:gts2020 ;
    skos:definition "A time period with the following approximated bounds: candidates are Mt. Crussol or Canjuers (SE France) and Fornazzo (Sicily, S. Italy)" ;
    skos:inScheme cs: ;
    skos:prefLabel "Stratotype Point Base of Tithonian"@en ;
    prov:wasDerivedFrom ts:gts2020 ;
.

isc:BaseToarcianSP
    dcterms:identifier "BaseToarcianSP" ;
    a skos:Concept ;
    rdfs:isDefinedBy ts:gts2020 ;
    skos:definition "A time period with the following approximated bounds: Ponta do Trovao, Peniche (Portugal)" ;
    skos:inScheme cs: ;
    skos:prefLabel "Stratotype Point Base of Toarcian"@en ;
    prov:wasDerivedFrom ts:gts2020 ;
.

isc:BaseTortonianSP
    dcterms:identifier "BaseTortonianSP" ;
    a skos:Concept ;
    rdfs:isDefinedBy ts:gts2020 ;
    skos:definition "A time period with the following approximated bounds: Monte dei Corvi Beach, near Ancona, Italy" ;
    skos:inScheme cs: ;
    skos:prefLabel "Stratotype Point Base of Tortonian"@en ;
    prov:wasDerivedFrom ts:gts2020 ;
.

isc:BaseTuronianSP
    dcterms:identifier "BaseTuronianSP" ;
    a skos:Concept ;
    rdfs:isDefinedBy ts:gts2020 ;
    skos:definition "A time period with the following approximated bounds: Pueblo, Colorado, USA" ;
    skos:inScheme cs: ;
    skos:prefLabel "Stratotype Point Base of Turonian"@en ;
    prov:wasDerivedFrom ts:gts2020 ;
.

isc:BaseUpperCretaceousSP
    dcterms:identifier "BaseUpperCretaceousSP" ;
    a skos:Concept ;
    rdfs:isDefinedBy ts:gts2020 ;
    skos:definition "A time period with the following approximated bounds: Mount Risou, Hautes Alpes, France" ;
    skos:inScheme cs: ;
    skos:prefLabel "Stratotype Point Base of Cenomanian"@en ;
    prov:wasDerivedFrom ts:gts2020 ;
.

isc:BaseUpperDevonianSP
    dcterms:identifier "BaseUpperDevonianSP" ;
    a skos:Concept ;
    rdfs:isDefinedBy ts:gts2020 ;
    skos:definition "A time period with the following approximated bounds: Col du Puech de la Suque, Montage Noire, France" ;
    skos:inScheme cs: ;
    skos:prefLabel "Stratotype Point Base of Frasnian"@en ;
    prov:wasDerivedFrom ts:gts2020 ;
.

isc:BaseUpperJurassicSP
    dcterms:identifier "BaseUpperJurassicSP" ;
    a skos:Concept ;
    rdfs:isDefinedBy ts:gts2020 ;
    skos:definition "A time period with the following approximated bounds: Thuoux Section, SE France" ;
    skos:inScheme cs: ;
    skos:prefLabel "Stratotype Point Base of Oxfordian"@en ;
    prov:wasDerivedFrom ts:gts2020 ;
.

isc:BaseUpperMississippianSP
    dcterms:identifier "BaseUpperMississippianSP" ;
    a skos:Concept ;
    rdfs:isDefinedBy ts:gts2020 ;
    skos:definition "A time period with the following approximated bounds: candidates are Verkhnyaya Kardailovka (Urals) or Nashui (China)" ;
    skos:inScheme cs: ;
    skos:prefLabel "Stratotype Point Base of Serpukhovian"@en ;
    prov:wasDerivedFrom ts:gts2020 ;
.

isc:BaseUpperOrdovicianSP
    dcterms:identifier "BaseUpperOrdovicianSP" ;
    a skos:Concept ;
    rdfs:isDefinedBy ts:gts2020 ;
    skos:definition "A time period with the following approximated bounds: Sularp Brook, Fagelsang, Sweden" ;
    skos:inScheme cs: ;
    skos:prefLabel "Stratotype Point Base of Sandbian"@en ;
    prov:wasDerivedFrom ts:gts2020 ;
.

isc:BaseUpperPennsylvanianSP
    dcterms:identifier "BaseUpperPennsylvanianSP" ;
    a skos:Concept ;
    rdfs:isDefinedBy ts:gts2020 ;
    skos:definition "A time period with the following approximated bounds: candidates are in southern Urals, and Nashui (South China)." ;
    skos:inScheme cs: ;
    skos:prefLabel "Stratotype Point Base of Kasimovian"@en ;
    prov:wasDerivedFrom ts:gts2020 ;
.

isc:BaseUpperTriassicSP
    dcterms:identifier "BaseUpperTriassicSP" ;
    a skos:Concept ;
    rdfs:isDefinedBy ts:gts2020 ;
    skos:definition "A time period with the following approximated bounds: Prati di Stuores, Dolomites, Italy" ;
    skos:inScheme cs: ;
    skos:prefLabel "Stratotype Point Base of Carnian"@en ;
    prov:wasDerivedFrom ts:gts2020 ;
.

isc:BaseValanginianSP
    dcterms:identifier "BaseValanginianSP" ;
    a skos:Concept ;
    rdfs:isDefinedBy ts:gts2020 ;
    skos:definition "A time period with the following approximated bounds: candidates are near Montbrunles- Bains (Drôme province, SE France) and Cañada Luenga (Betic Cordillera, S. Spain)" ;
    skos:inScheme cs: ;
    skos:prefLabel "Stratotype Point Base of Valanginian"@en ;
    prov:wasDerivedFrom ts:gts2020 ;
.

isc:BaseWenlockSP
    dcterms:identifier "BaseWenlockSP" ;
    a skos:Concept ;
    rdfs:isDefinedBy ts:gts2020 ;
    skos:definition "A time period with the following approximated bounds: Hughley Brook, UK" ;
    skos:inScheme cs: ;
    skos:prefLabel "Stratotype Point Base of Sheinwoodian"@en ;
    prov:wasDerivedFrom ts:gts2020 ;
.

isc:BaseWordianSP
    dcterms:identifier "BaseWordianSP" ;
    a skos:Concept ;
    rdfs:isDefinedBy ts:gts2020 ;
    skos:definition "A time period with the following approximated bounds: Guadalupe Pass, Texas, U.S.A" ;
    skos:inScheme cs: ;
    skos:prefLabel "Stratotype Point Base of Wordian"@en ;
    prov:wasDerivedFrom ts:gts2020 ;
.

isc:Aalenian
    dcterms:identifier "Aalenian" ;
    a skos:Concept ;
    rdfs:isDefinedBy ts:gts2020 ;
    skos:broader isc:MiddleJurassic ;
    skos:definition "A time period with the following approximated bounds: older bound -174.1 +|-1.0 Ma, younger bound -170.3 +|-1.4 Ma" ;
    skos:inScheme cs: ;
    skos:prefLabel
        "пален"@bg ,
        "Aalen"@cs ,
        "Aalenien"@da ,
        "Aalénium"@de ,
        "Aalenian"@en ,
        "Aaleniense"@es ,
        "Aaleni"@et ,
        "Aalen"@fi ,
        "Aalénien"@fr ,
        "aaleni"@hu ,
        "aaleniano"@it ,
        "アーレニアン期"@ja ,
        "Alenis"@lt ,
        "Aaleniën"@nl ,
        "Aalen"@no ,
        "Aalen"@pl ,
        "Aaleniano"@pt ,
        "álen"@sk ,
        "aalenij"@sl ,
        "aalen"@sv ,
        "阿连期"@zh ;
    prov:wasDerivedFrom ts:gts2020 ;
.

isc:Aeronian
    dcterms:identifier "Aeronian" ;
    a skos:Concept ;
    rdfs:isDefinedBy ts:gts2020 ;
    skos:broader isc:Llandovery ;
    skos:definition "A time period with the following approximated bounds: older bound -440.8 +|-1.2 Ma, younger bound -438.5 +|-1.1 Ma" ;
    skos:inScheme cs: ;
    skos:prefLabel
        "перон"@bg ,
        "Aeron"@cs ,
        "Aeronien"@da ,
        "Aeronium"@de ,
        "Aeronian"@en ,
        "Aeroniense"@es ,
        "Aeroni"@et ,
        "Aeron"@fi ,
        "Aéronien"@fr ,
        "aeroni"@hu ,
        "aeroniano"@it ,
        "アエロニアン期"@ja ,
        "Aeronis"@lt ,
        "Aeroniën"@nl ,
        "Aeronium"@no ,
        "Aeron"@pl ,
        "Aeroniano"@pt ,
        "aerón"@sk ,
        "aeronij"@sl ,
        "aeron"@sv ,
        "埃隆期"@zh ;
    prov:wasDerivedFrom ts:gts2020 ;
.

isc:Albian
    dcterms:identifier "Albian" ;
    a skos:Concept ;
    rdfs:isDefinedBy ts:gts2020 ;
    skos:broader isc:LowerCretaceous ;
    skos:definition "A time period with the following approximated bounds: older bound -113.0 Ma, younger bound -100.5 Ma" ;
    skos:inScheme cs: ;
    skos:prefLabel
        "плб"@bg ,
        "Alb"@cs ,
        "Albien"@da ,
        "Albium"@de ,
        "Albian"@en ,
        "Albiense"@es ,
        "Albi"@et ,
        "Alb"@fi ,
        "Albien"@fr ,
        "albai"@hu ,
        "albiano"@it ,
        "アルビアン期"@ja ,
        "Albis"@lt ,
        "Albiën"@nl ,
        "Alb"@no ,
        "Alb"@pl ,
        "Albiano"@pt ,
        "alb"@sk ,
        "albij"@sl ,
        "alban"@sv ,
        "阿尔布期"@zh ;
    prov:wasDerivedFrom ts:gts2020 ;
.

isc:Anisian
    dcterms:identifier "Anisian" ;
    a skos:Concept ;
    rdfs:isDefinedBy ts:gts2020 ;
    skos:broader isc:MiddleTriassic ;
    skos:definition "A time period with the following approximated bounds: older bound -247.2 Ma, younger bound -242 Ma" ;
    skos:inScheme cs: ;
    skos:prefLabel
        "пниз"@bg ,
        "Anis"@cs ,
        "Anisien"@da ,
        "Anisium"@de ,
        "Anisian"@en ,
        "Anisiense"@es ,
        "Anisi"@et ,
        "Anis"@fi ,
        "Anisien"@fr ,
        "anisusi"@hu ,
        "anisico"@it ,
        "アニシアン期"@ja ,
        "Anizis"@lt ,
        "Anisiën"@nl ,
        "Ansin"@no ,
        "Anizyk"@pl ,
        "Anisiano"@pt ,
        "anis"@sk ,
        "anizij"@sl ,
        "anis"@sv ,
        "安尼期"@zh ;
    prov:wasDerivedFrom ts:gts2020 ;
.

isc:Aptian
    dcterms:identifier "Aptian" ;
    a skos:Concept ;
    rdfs:isDefinedBy ts:gts2020 ;
    skos:broader isc:LowerCretaceous ;
    skos:definition "A time period with the following approximated bounds: older bound -125.0 Ma, younger bound -113.0 Ma" ;
    skos:inScheme cs: ;
    skos:prefLabel
        "ппт"@bg ,
        "Apt"@cs ,
        "Aptien"@da ,
        "Aptium"@de ,
        "Aptian"@en ,
        "Aptiense"@es ,
        "Apti"@et ,
        "Apt"@fi ,
        "Aptien"@fr ,
        "apti"@hu ,
        "aptiano"@it ,
        "アプチアン期"@ja ,
        "Aptis"@lt ,
        "Aptiën"@nl ,
        "Apt"@no ,
        "Apt"@pl ,
        "Aptiano"@pt ,
        "apt"@sk ,
        "aptij"@sl ,
        "apt"@sv ,
        "阿普弟期"@zh ;
    prov:wasDerivedFrom ts:gts2020 ;
.

isc:Aquitanian
    dcterms:identifier "Aquitanian" ;
    a skos:Concept ;
    rdfs:isDefinedBy ts:gts2020 ;
    skos:broader isc:Miocene ;
    skos:definition "A time period with the following approximated bounds: older bound -23.03 Ma, younger bound -20.44 Ma" ;
    skos:inScheme cs: ;
    skos:prefLabel
        "пквитан"@bg ,
        "Aquitan"@cs ,
        "Aquitanien"@da ,
        "Aquitanium"@de ,
        "Aquitanian"@en ,
        "Aquitaninse"@es ,
        "Aquitani"@et ,
        "Aquitan"@fi ,
        "Aquitanien"@fr ,
        "aquitaniai"@hu ,
        "aquitaniano"@it ,
        "アキタニアン期"@ja ,
        "Akvitanis"@lt ,
        "Aquitaniën-Vierland"@nl ,
        "Aquitanium"@no ,
        "Akwitan"@pl ,
        "Aquitaniano"@pt ,
        "akvitán"@sk ,
        "akvitanij"@sl ,
        "aquitan"@sv ,
        "阿启坦期"@zh ;
    prov:wasDerivedFrom ts:gts2020 ;
.

isc:Artinskian
    dcterms:identifier "Artinskian" ;
    a skos:Concept ;
    rdfs:isDefinedBy ts:gts2020 ;
    skos:broader isc:Cisuralian ;
    skos:definition "A time period with the following approximated bounds: older bound -290.1 +|-0.26 Ma, younger bound -283.5 +|-0.6 Ma" ;
    skos:inScheme cs: ;
    skos:prefLabel
        "пртин"@bg ,
        "Artinsk"@cs ,
        "Artinskien"@da ,
        "Artinskium"@de ,
        "Artinskian"@en ,
        "Artinskiense"@es ,
        "Artinski"@et ,
        "Artinsk"@fi ,
        "Artinskien"@fr ,
        "artyinszki"@hu ,
        "artinskiano"@it ,
        "アルティンスキアン期"@ja ,
        "Artinskis"@lt ,
        "Artinskiën"@nl ,
        "Artiskium"@no ,
        "Artinsk"@pl ,
        "Artinskiano"@pt ,
        "artinsk"@sk ,
        "artinskij"@sl ,
        "artinsk"@sv ,
        "亚丁斯克期"@zh ;
    prov:wasDerivedFrom ts:gts2020 ;
.

isc:Asselian
    dcterms:identifier "Asselian" ;
    a skos:Concept ;
    rdfs:isDefinedBy ts:gts2020 ;
    skos:broader isc:Cisuralian ;
    skos:definition "A time period with the following approximated bounds: older bound -298.9 +|-0.15 Ma, younger bound -295.0 +|-0.18 Ma" ;
    skos:inScheme cs: ;
    skos:prefLabel
        "пѿел"@bg ,
        "Assel"@cs ,
        "Asselien"@da ,
        "Asselium"@de ,
        "Asselian"@en ,
        "Asseliense"@es ,
        "Asseli"@et ,
        "Assel"@fi ,
        "Assélien"@fr ,
        "asszeli"@hu ,
        "asseliano"@it ,
        "アセリアン期"@ja ,
        "Aselis"@lt ,
        "Asseliën"@nl ,
        "Asselium"@no ,
        "Aselsk"@pl ,
        "Asseliano"@pt ,
        "assel"@sk ,
        "asselij"@sl ,
        "assel"@sv ,
        "阿瑟尔期"@zh ;
    prov:wasDerivedFrom ts:gts2020 ;
.

isc:Bajocian
    dcterms:identifier "Bajocian" ;
    a skos:Concept ;
    rdfs:isDefinedBy ts:gts2020 ;
    skos:broader isc:MiddleJurassic ;
    skos:definition "A time period with the following approximated bounds: older bound -170.3 +|-1.4 Ma, younger bound -168.3 +|-1.3 Ma" ;
    skos:inScheme cs: ;
    skos:prefLabel
        "Байоѿ"@bg ,
        "Bajok"@cs ,
        "Bajocien"@da ,
        "Bajocium"@de ,
        "Bajocian"@en ,
        "Bajociense"@es ,
        "Bajoci"@et ,
        "Bajoc"@fi ,
        "Bajocien"@fr ,
        "bajoci"@hu ,
        "bajociano"@it ,
        "バジョシアン期"@ja ,
        "Bajosis"@lt ,
        "Bajociën"@nl ,
        "Bajoc"@no ,
        "Bajos"@pl ,
        "Bajociano"@pt ,
        "bajok"@sk ,
        "bajocij"@sl ,
        "bajoc"@sv ,
        "巴柔期"@zh ;
    prov:wasDerivedFrom ts:gts2020 ;
.

isc:Barremian
    dcterms:identifier "Barremian" ;
    a skos:Concept ;
    rdfs:isDefinedBy ts:gts2020 ;
    skos:broader isc:LowerCretaceous ;
    skos:definition "A time period with the following approximated bounds: older bound -129.4 Ma, younger bound -125.0 Ma" ;
    skos:inScheme cs: ;
    skos:prefLabel
        "Барем"@bg ,
        "Barrem"@cs ,
        "Barremien"@da ,
        "Barrêmium"@de ,
        "Barremian"@en ,
        "Barremiense"@es ,
        "Barremi"@et ,
        "Barrem"@fi ,
        "Barrémien"@fr ,
        "barremi"@hu ,
        "berremiano"@it ,
        "バレミアン期"@ja ,
        "Baremis"@lt ,
        "Barremiën"@nl ,
        "Barremium"@no ,
        "Barrem"@pl ,
        "Barremiano"@pt ,
        "barém"@sk ,
        "barremij"@sl ,
        "barrem"@sv ,
        "巴列姆期"@zh ;
    prov:wasDerivedFrom ts:gts2020 ;
.

isc:Bartonian
    dcterms:identifier "Bartonian" ;
    a skos:Concept ;
    rdfs:isDefinedBy ts:gts2020 ;
    skos:broader isc:Eocene ;
    skos:definition "A time period with the following approximated bounds: older bound -41.2 Ma, younger bound -37.8 Ma" ;
    skos:inScheme cs: ;
    skos:prefLabel
        "Бартон"@bg ,
        "Barton"@cs ,
        "Bartonien"@da ,
        "Bartonium"@de ,
        "Bartonian"@en ,
        "Bartoniense"@es ,
        "Bartoni"@et ,
        "Barton"@fi ,
        "Bartonien"@fr ,
        "bartoni"@hu ,
        "bartoniano"@it ,
        "バートニアン期"@ja ,
        "Bartonis"@lt ,
        "Bartoniën"@nl ,
        "Barton"@no ,
        "Barton"@pl ,
        "Bartoniano"@pt ,
        "bartón"@sk ,
        "bartonij"@sl ,
        "barton"@sv ,
        "巴尔顿期"@zh ;
    prov:wasDerivedFrom ts:gts2020 ;
.

isc:Bashkirian
    dcterms:identifier "Bashkirian" ;
    a skos:Concept ;
    rdfs:isDefinedBy ts:gts2020 ;
    skos:broader isc:LowerPennsylvanian ;
    skos:definition "A time period with the following approximated bounds: older bound -323.2 +|-0.4 Ma, younger bound -315.2 +|-0.2 Ma" ;
    skos:inScheme cs: ;
    skos:prefLabel
        "Башкир"@bg ,
        "Bashkir"@cs ,
        "Bashkirien"@da ,
        "Bashkirium"@de ,
        "Bashkirian"@en ,
        "Bashkiriense"@es ,
        "Baškiiri"@et ,
        "Bashkir"@fi ,
        "Bashkirien"@fr ,
        "baskír"@hu ,
        "bashkiriano"@it ,
        "バシキリアン期"@ja ,
        "Bashkirian"@lt ,
        "Bashkiriën"@nl ,
        "Bashkirium"@no ,
        "Baszkir"@pl ,
        "Bashkiriano"@pt ,
        "baškir"@sk ,
        "baškirij"@sl ,
        "bashkir"@sv ,
        "巴什基尔期"@zh ;
    prov:wasDerivedFrom ts:gts2020 ;
.

isc:Bathonian
    dcterms:identifier "Bathonian" ;
    a skos:Concept ;
    rdfs:isDefinedBy ts:gts2020 ;
    skos:broader isc:MiddleJurassic ;
    skos:definition "A time period with the following approximated bounds: older bound -168.3 +|-1.3 Ma, younger bound -166.1 +|-1.2 Ma" ;
    skos:inScheme cs: ;
    skos:prefLabel
        "Бат"@bg ,
        "Bathon"@cs ,
        "Bathonien"@da ,
        "Bathonium"@de ,
        "Bathonian"@en ,
        "Bathoniense"@es ,
        "Bathoni"@et ,
        "Bathon"@fi ,
        "Bathonien"@fr ,
        "bath"@hu ,
        "bathoniano"@it ,
        "バソニアン期"@ja ,
        "Batonis"@lt ,
        "Barthoniën"@nl ,
        "Bathon"@no ,
        "Baton"@pl ,
        "Batoniano"@pt ,
        "bath"@sk ,
        "bathonij"@sl ,
        "bathon"@sv ,
        "巴通期"@zh ;
    prov:wasDerivedFrom ts:gts2020 ;
.

isc:Berriasian
    dcterms:identifier "Berriasian" ;
    a skos:Concept ;
    rdfs:isDefinedBy ts:gts2020 ;
    skos:broader isc:LowerCretaceous ;
    skos:definition "A time period with the following approximated bounds: older bound -145.0 Ma, younger bound -139.8 Ma" ;
    skos:inScheme cs: ;
    skos:prefLabel
        "Бериаѿ"@bg ,
        "Berrias"@cs ,
        "Berriasien"@da ,
        "Berriasium"@de ,
        "Berriasian"@en ,
        "Berriasiense"@es ,
        "Berriasi"@et ,
        "Berrias"@fi ,
        "Berriasien"@fr ,
        "berriasi"@hu ,
        "berriasiano"@it ,
        "ベリアシアン期"@ja ,
        "Beriasis"@lt ,
        "Berrasiën"@nl ,
        "Berriasium"@no ,
        "Berias"@pl ,
        "Berriasiano"@pt ,
        "berias"@sk ,
        "berriasij"@sl ,
        "berrias"@sv ,
        "贝利亚斯期"@zh ;
    prov:wasDerivedFrom ts:gts2020 ;
.

isc:Burdigalian
    dcterms:identifier "Burdigalian" ;
    a skos:Concept ;
    rdfs:isDefinedBy ts:gts2020 ;
    skos:broader isc:Miocene ;
    skos:definition "A time period with the following approximated bounds: older bound -20.44 Ma, younger bound -15.97 Ma" ;
    skos:inScheme cs: ;
    skos:prefLabel
        "Бурдигал"@bg ,
        "Burdigal"@cs ,
        "Burdigalien"@da ,
        "Burdigalium"@de ,
        "Burdigalian"@en ,
        "Burdigaliense"@es ,
        "Burdigali"@et ,
        "Burdigal"@fi ,
        "Burdigalien"@fr ,
        "burdigaliai"@hu ,
        "burdigaliano"@it ,
        "バーディガリアン期"@ja ,
        "Burdigalis"@lt ,
        "Burdigaliën-Hemmoor"@nl ,
        "Burdigalium"@no ,
        "Burdygał"@pl ,
        "Burdigaliano"@pt ,
        "burdigal"@sk ,
        "burdigalij"@sl ,
        "burdigal"@sv ,
        "布迪加尔期"@zh ;
    prov:wasDerivedFrom ts:gts2020 ;
.

isc:Calabrian
    dcterms:identifier "Calabrian" ;
    a skos:Concept ;
    rdfs:isDefinedBy ts:gts2020 ;
    skos:broader isc:Pleistocene ;
    skos:definition "A time period with the following approximated bounds: older bound -1.80 Ma, younger bound -0.781 Ma" ;
    skos:inScheme cs: ;
    skos:prefLabel
        "Калабрий"@bg ,
        "Calabr"@cs ,
        "Calabrian"@da ,
        "Calabrium"@de ,
        "Calabrian"@en ,
        "Calabriense"@es ,
        "Kalaabria"@et ,
        "Calabria"@fi ,
        "Calabrien"@fr ,
        "kalabriai"@hu ,
        "calabriano"@it ,
        "カラブリア期"@ja ,
        "Kalabris"@lt ,
        "Onder Pleistoceen/ Hoog Terras"@nl ,
        "Calabrium"@no ,
        "Kalambr"@pl ,
        "Calabriano"@pt ,
        "kalábrian"@sk ,
        "calabrij"@sl ,
        "calabr"@sv ,
        "卡拉布里亚期"@zh ;
    prov:wasDerivedFrom ts:gts2020 ;
.

isc:Callovian
    dcterms:identifier "Callovian" ;
    a skos:Concept ;
    rdfs:isDefinedBy ts:gts2020 ;
    skos:broader isc:MiddleJurassic ;
    skos:definition "A time period with the following approximated bounds: older bound -166.1 +|-1.2 Ma, younger bound -163.5 +|-1.0 Ma" ;
    skos:inScheme cs: ;
    skos:prefLabel
        "Калов"@bg ,
        "Callov"@cs ,
        "Callovien"@da ,
        "Callovium"@de ,
        "Callovian"@en ,
        "Calloviense"@es ,
        "Callovi"@et ,
        "Callov"@fi ,
        "Callovien"@fr ,
        "callovi"@hu ,
        "calloviano"@it ,
        "カロビアン期"@ja ,
        "Kelovėjis"@lt ,
        "Calloviën"@nl ,
        "Callove"@no ,
        "Kelowej"@pl ,
        "Caloviano"@pt ,
        "kelovej"@sk ,
        "callovij"@sl ,
        "callov"@sv ,
        "卡洛夫期"@zh ;
    prov:wasDerivedFrom ts:gts2020 ;
.

isc:Calymmian
    dcterms:identifier "Calymmian" ;
    a skos:Concept ;
    rdfs:isDefinedBy ts:gts2020 ;
    skos:broader isc:Mesoproterozoic ;
    skos:definition "A time period with the following approximated bounds: older bound -1600 Ma, younger bound -1400 Ma" ;
    skos:inScheme cs: ;
    skos:prefLabel
        "Калим"@bg ,
        "Calymm"@cs ,
        "Calymmien"@da ,
        "Calymmium"@de ,
        "Calymmian"@en ,
        "Calymmiense"@es ,
        "Calymm"@et ,
        "Calym"@fi ,
        "Calymmien"@fr ,
        "calymmi"@hu ,
        "calymmiano"@it ,
        "カリミアン紀"@ja ,
        "Kalymis"@lt ,
        "Calymmiën"@nl ,
        "Kalymmium"@no ,
        "Kalym"@pl ,
        "Calymiano"@pt ,
        "kalymnium"@sk ,
        "calymmij"@sl ,
        "kalymmium"@sv ,
        "盖层纪"@zh ;
    prov:wasDerivedFrom ts:gts2020 ;
.

isc:CambrianStage10
    dcterms:identifier "CambrianStage10" ;
    a skos:Concept ;
    rdfs:isDefinedBy ts:gts2020 ;
    skos:broader isc:Furongian ;
    skos:definition "A time period with the following approximated bounds: older bound -489.5 Ma, younger bound -485.4 +|-1.9 Ma" ;
    skos:inScheme cs: ;
    skos:prefLabel
        "Камбрий - 10 етаж"@bg ,
        "Kambrium-Stupeň 10"@cs ,
        "Kambrium-Etage 10"@da ,
        "Kambrium-Stufe 10"@de ,
        "Cambrian-Stage 10"@en ,
        "Cámbrico-Piso 10"@es ,
        "Kambrium, Lade 10"@et ,
        "Kambri-vaihe 10"@fi ,
        "Cambrien-Etage 10"@fr ,
        "kambrium 10. emelet"@hu ,
        "cambriano - stage 10"@it ,
        "第10期"@ja ,
        "Kambras-Aukštas 10"@lt ,
        "Cambrium, Zone 10"@nl ,
        "Kambrium-etasje10"@no ,
        "Kambr-Piętro 10"@pl ,
        "Câmbrico-Piso 10"@pt ,
        "kambrium, stupeň 10"@sk ,
        "kambrij-stopnja 10"@sl ,
        "kambrium etage 10"@sv ,
        "第十期"@zh ;
    prov:wasDerivedFrom ts:gts2020 ;
.

isc:CambrianStage2
    dcterms:identifier "CambrianStage2" ;
    a skos:Concept ;
    rdfs:isDefinedBy ts:gts2020 ;
    skos:broader isc:Terreneuvian ;
    skos:definition "A time period with the following approximated bounds: older bound -529 Ma, younger bound -521 Ma" ;
    skos:inScheme cs: ;
    skos:prefLabel
        "Камбрий - 2 етаж"@bg ,
        "Kambrium-Stupeň 2"@cs ,
        "Kambrium-Etage 2"@da ,
        "Kambrium-Stufe 2"@de ,
        "Cambrian-Stage 2"@en ,
        "Cámbrico-Piso 2"@es ,
        "Kambrium, Lade 2"@et ,
        "Kambri-vaihe 2"@fi ,
        "Cambrien-Etage 2"@fr ,
        "kambrium 2. emelet"@hu ,
        "cambriano - stage 2"@it ,
        "第2期"@ja ,
        "Kambras-Aukštas 2"@lt ,
        "Cambrium, Zone 2"@nl ,
        "Kambrium-etasje 2"@no ,
        "Kambr-Piętro 2"@pl ,
        "Câmbrico-Piso 2"@pt ,
        "kambrium, stupeň 2"@sk ,
        "kambrij-stopnja 2"@sl ,
        "kambrium etage 1"@sv ,
        "第二期"@zh ;
    prov:wasDerivedFrom ts:gts2020 ;
.

isc:CambrianStage3
    dcterms:identifier "CambrianStage3" ;
    a skos:Concept ;
    rdfs:isDefinedBy ts:gts2020 ;
    skos:broader isc:CambrianSeries2 ;
    skos:definition "A time period with the following approximated bounds: older bound -521 Ma, younger bound -514 Ma" ;
    skos:inScheme cs: ;
    skos:prefLabel
        "Камбрий - 3 етаж"@bg ,
        "Kambrium-Stupeň 3"@cs ,
        "Kambrium-Etage 3"@da ,
        "Kambrium-Stufe 3"@de ,
        "Cambrian-Stage 3"@en ,
        "Cámbrico-Piso 3"@es ,
        "Kambrium, Lade 3"@et ,
        "Kambri-vaihe 3"@fi ,
        "Cambrien-Etage 3"@fr ,
        "kambrium 3. emelet"@hu ,
        "cambriano - stage 3"@it ,
        "第3期"@ja ,
        "Kambras-Aukštas 3"@lt ,
        "Cambrium, Zone3"@nl ,
        "Kambrium-etasje 3"@no ,
        "Kambr-Piętro 3"@pl ,
        "Câmbrico-Piso 3"@pt ,
        "kambrium, stupeň 3"@sk ,
        "kambrij-stopnja 3"@sl ,
        "kambrium etage 3"@sv ,
        "第三期"@zh ;
    prov:wasDerivedFrom ts:gts2020 ;
.

isc:CambrianStage4
    dcterms:identifier "CambrianStage4" ;
    a skos:Concept ;
    rdfs:isDefinedBy ts:gts2020 ;
    skos:broader isc:CambrianSeries2 ;
    skos:definition "A time period with the following approximated bounds: older bound -514 Ma, younger bound -509 Ma" ;
    skos:inScheme cs: ;
    skos:prefLabel
        "Камбрий - 4 етаж"@bg ,
        "Kambrium-Stupeň 4"@cs ,
        "Kambrium-Etage 4"@da ,
        "Kambrium-Stufe 4"@de ,
        "Cambrian-Stage 4"@en ,
        "Cámbrico-Piso 4"@es ,
        "Kambrium, Lade 4"@et ,
        "Kambri-vaihe 4"@fi ,
        "Cambrien-Etage 4"@fr ,
        "kambrium 4. emelet"@hu ,
        "cambriano - stage 4"@it ,
        "第4期"@ja ,
        "Kambras-Aukšts 4"@lt ,
        "Cambrium, Zone 4"@nl ,
        "Kambrium-etasje 4"@no ,
        "Kambr-Piętro 4"@pl ,
        "Câmbrico-Piso 4"@pt ,
        "kambrium, stupeň 4"@sk ,
        "kambrij stopnja 4"@sl ,
        "kambrium etage 4"@sv ,
        "第四期"@zh ;
    prov:wasDerivedFrom ts:gts2020 ;
.

isc:Campanian
    dcterms:identifier "Campanian" ;
    a skos:Concept ;
    rdfs:isDefinedBy ts:gts2020 ;
    skos:broader isc:UpperCretaceous ;
    skos:definition "A time period with the following approximated bounds: older bound -83.6 +|-0.2 Ma, younger bound -72.1 +|-0.2 Ma" ;
    skos:inScheme cs: ;
    skos:prefLabel
        "Кампан"@bg ,
        "Campan"@cs ,
        "Campanien"@da ,
        "Campanium"@de ,
        "Campanian"@en ,
        "Campaniense"@es ,
        "Campani"@et ,
        "Campan"@fi ,
        "Campanien"@fr ,
        "campaniai"@hu ,
        "campaniano"@it ,
        "カンパニアン期"@ja ,
        "Kampanis"@lt ,
        "Campaniën"@nl ,
        "Campanium"@no ,
        "Kampan"@pl ,
        "Campaniano"@pt ,
        "kampán"@sk ,
        "campanij"@sl ,
        "campan"@sv ,
        "坎佩尼期"@zh ;
    prov:wasDerivedFrom ts:gts2020 ;
.

isc:Capitanian
    dcterms:identifier "Capitanian" ;
    a skos:Concept ;
    rdfs:isDefinedBy ts:gts2020 ;
    skos:broader isc:Guadalupian ;
    skos:definition "A time period with the following approximated bounds: older bound -265.1 +|-0.4 Ma, younger bound -259.1 +|-0.5 Ma" ;
    skos:inScheme cs: ;
    skos:prefLabel
        "Капитан"@bg ,
        "Capitan"@cs ,
        "Capitanien"@da ,
        "Capitanium"@de ,
        "Capitanian"@en ,
        "Capitaniense"@es ,
        "Capitani"@et ,
        "Capitan"@fi ,
        "Capitanien"@fr ,
        "capitani"@hu ,
        "capitaniano"@it ,
        "カピタニアン期"@ja ,
        "Kapitanis"@lt ,
        "Capitaniën"@nl ,
        "Capitanium"@no ,
        "Kapitan"@pl ,
        "Capitaniano"@pt ,
        "capitan"@sk ,
        "capitanij"@sl ,
        "capitan"@sv ,
        "卡匹敦期"@zh ;
    prov:wasDerivedFrom ts:gts2020 ;
.

isc:Carnian
    dcterms:identifier "Carnian" ;
    a skos:Concept ;
    rdfs:isDefinedBy ts:gts2020 ;
    skos:broader isc:UpperTriassic ;
    skos:definition "A time period with the following approximated bounds: older bound -237 Ma, younger bound -227 Ma" ;
    skos:inScheme cs: ;
    skos:prefLabel
        "Карн"@bg ,
        "Carn"@cs ,
        "Carnien"@da ,
        "Karnium"@de ,
        "Carnian"@en ,
        "Carniense"@es ,
        "Carni"@et ,
        "Carn"@fi ,
        "Carnien"@fr ,
        "karni"@hu ,
        "carnico"@it ,
        "カーニアン期"@ja ,
        "Karnis"@lt ,
        "Carniën"@nl ,
        "Carn"@no ,
        "Karnik"@pl ,
        "Carniano"@pt ,
        "karn"@sk ,
        "karnij"@sl ,
        "carn"@sv ,
        "卡尼期"@zh ;
    prov:wasDerivedFrom ts:gts2020 ;
.

isc:Cenomanian
    dcterms:identifier "Cenomanian" ;
    a skos:Concept ;
    rdfs:isDefinedBy ts:gts2020 ;
    skos:broader isc:UpperCretaceous ;
    skos:definition "A time period with the following approximated bounds: older bound -100.5 Ma, younger bound -93.9 Ma" ;
    skos:inScheme cs: ;
    skos:prefLabel
        "Ценоман"@bg ,
        "Cenoman"@cs ,
        "Cenomanien"@da ,
        "Cenomanium"@de ,
        "Cenomanian"@en ,
        "Cenomaniense"@es ,
        "Cenomani"@et ,
        "Cenoman"@fi ,
        "Cénomanien"@fr ,
        "cenoman"@hu ,
        "cenomaniano"@it ,
        "セノマニアン期"@ja ,
        "Cenomanis"@lt ,
        "Laat/Boven Krijt"@nl ,
        "Cenomanium"@no ,
        "Cenoman"@pl ,
        "Cenomaniano"@pt ,
        "cenoman"@sk ,
        "cenomanij"@sl ,
        "cenoman"@sv ,
        "森诺曼期"@zh ;
    prov:wasDerivedFrom ts:gts2020 ;
.

isc:Changhsingian
    dcterms:identifier "Changhsingian" ;
    a skos:Concept ;
    rdfs:isDefinedBy ts:gts2020 ;
    skos:broader isc:Lopingian ;
    skos:definition "A time period with the following approximated bounds: older bound -254.14 +|-0.07 Ma, younger bound -251.902 +|-0.024 Ma" ;
    skos:inScheme cs: ;
    skos:prefLabel
        "Чангшинг"@bg ,
        "Changhsing"@cs ,
        "Changhsingien"@da ,
        "Changhsingium"@de ,
        "Changhsingian"@en ,
        "Changsingiense"@es ,
        "Changhsingi"@et ,
        "Changhsing"@fi ,
        "Changhsingien"@fr ,
        "changhsingi"@hu ,
        "changsingiano"@it ,
        "チャンシンギアン期"@ja ,
        "Čangšinjanis"@lt ,
        "Changhsingiën"@nl ,
        "Changxingium"@no ,
        "Changhsing"@pl ,
        "Changhsingiano"@pt ,
        "Ŀchangsing"@sk ,
        "changhsingij"@sl ,
        "changhsing"@sv ,
        "长兴期"@zh ;
    prov:wasDerivedFrom ts:gts2020 ;
.

isc:Chattian
    dcterms:identifier "Chattian" ;
    a skos:Concept ;
    rdfs:isDefinedBy ts:gts2020 ;
    skos:broader isc:Oligocene ;
    skos:definition "A time period with the following approximated bounds: older bound -27.82 Ma, younger bound -23.03 Ma" ;
    skos:inScheme cs: ;
    skos:prefLabel
        "Хат"@bg ,
        "Chat"@cs ,
        "Chattien"@da ,
        "Chattium"@de ,
        "Chattian"@en ,
        "Chattiense"@es ,
        "Chatti"@et ,
        "Chatt"@fi ,
        "Chattien"@fr ,
        "katti"@hu ,
        "chattiano"@it ,
        "シャティアン期"@ja ,
        "Chatis"@lt ,
        "Chattiën"@nl ,
        "Chattium"@no ,
        "Szat"@pl ,
        "Chatiano"@pt ,
        "chatt"@sk ,
        "chattij"@sl ,
        "chatt"@sv ,
        "恰特期"@zh ;
    prov:wasDerivedFrom ts:gts2020 ;
.

isc:Coniacian
    dcterms:identifier "Coniacian" ;
    a skos:Concept ;
    rdfs:isDefinedBy ts:gts2020 ;
    skos:broader isc:UpperCretaceous ;
    skos:definition "A time period with the following approximated bounds: older bound -89.8 +|-0.3 Ma, younger bound -86.3 +|-0.5 Ma" ;
    skos:inScheme cs: ;
    skos:prefLabel
        "Кониак"@bg ,
        "Coniak"@cs ,
        "Coniacien"@da ,
        "Coniacium"@de ,
        "Coniacian"@en ,
        "Coni"@es ,
        "Coniaci"@et ,
        "Coniac"@fi ,
        "Coniacien"@fr ,
        "coniaci"@hu ,
        "coniaciano"@it ,
        "コニアシアン期"@ja ,
        "Konjakis"@lt ,
        "Conaciën"@nl ,
        "Coniacium"@no ,
        "Koniak"@pl ,
        "Coniaciano"@pt ,
        "koňak"@sk ,
        "coniacij"@sl ,
        "coniac"@sv ,
        "科尼亚克期"@zh ;
    prov:wasDerivedFrom ts:gts2020 ;
.

isc:Cryogenian
    dcterms:identifier "Cryogenian" ;
    a skos:Concept ;
    rdfs:isDefinedBy ts:gts2020 ;
    skos:broader isc:Neoproterozoic ;
    skos:definition "A time period with the following approximated bounds: older bound -720 Ma, younger bound -635 Ma" ;
    skos:inScheme cs: ;
    skos:prefLabel
        "Криоген"@bg ,
        "Cryogen"@cs ,
        "Cryogenien"@da ,
        "Kryogenium"@de ,
        "Cryogenian"@en ,
        "Criogeniense"@es ,
        "Krüogeen"@et ,
        "Cryogen"@fi ,
        "Cryogénien"@fr ,
        "cryogeni"@hu ,
        "cryogeniano"@it ,
        "クリオジェニアン紀"@ja ,
        "Kriogenis"@lt ,
        "Cryogeniën"@nl ,
        "Kryogenium"@no ,
        "Kriogen"@pl ,
        "Criogeniano"@pt ,
        "kryogén"@sk ,
        "cryogenij"@sl ,
        "kryogenium"@sv ,
        "成冰纪"@zh ;
    prov:wasDerivedFrom ts:gts2020 ;
.

isc:Danian
    dcterms:identifier "Danian" ;
    a skos:Concept ;
    rdfs:isDefinedBy ts:gts2020 ;
    skos:broader isc:Paleocene ;
    skos:definition "A time period with the following approximated bounds: older bound -66.0 Ma, younger bound -61.6 Ma" ;
    skos:inScheme cs: ;
    skos:prefLabel
        "Дан"@bg ,
        "Dan"@cs ,
        "Danien"@da ,
        "Danium"@de ,
        "Danian"@en ,
        "Daninese"@es ,
        "Taani"@et ,
        "Dan"@fi ,
        "Danien"@fr ,
        "dániai"@hu ,
        "daniano"@it ,
        "ダニアン期"@ja ,
        "Danis"@lt ,
        "Daniën"@nl ,
        "Danium"@no ,
        "Dan"@pl ,
        "Daniano"@pt ,
        "dán"@sk ,
        "danij"@sl ,
        "dan"@sv ,
        "丹麦期"@zh ;
    prov:wasDerivedFrom ts:gts2020 ;
.

isc:Dapingian
    dcterms:identifier "Dapingian" ;
    a skos:Concept ;
    rdfs:isDefinedBy ts:gts2020 ;
    skos:broader isc:MiddleOrdovician ;
    skos:definition "A time period with the following approximated bounds: older bound -470.0 +|-1.4 Ma, younger bound -467.3 +|-1.1 Ma" ;
    skos:inScheme cs: ;
    skos:prefLabel
        "Дапинг"@bg ,
        "Daping"@cs ,
        "Dapingien"@da ,
        "Dapingium"@de ,
        "Dapingian"@en ,
        "Dapingiense"@es ,
        "Dapingi"@et ,
        "Daping"@fi ,
        "Dapingien"@fr ,
        "dapingi"@hu ,
        "dapingiano"@it ,
        "ダピンギアン期"@ja ,
        "Dapingis"@lt ,
        "Dapingiën"@nl ,
        "Dapingium"@no ,
        "Daping"@pl ,
        "Dapingiano"@pt ,
        "daping"@sk ,
        "dapingij"@sl ,
        "daping"@sv ,
        "大坪期"@zh ;
    prov:wasDerivedFrom ts:gts2020 ;
.

isc:Darriwilian
    dcterms:identifier "Darriwilian" ;
    a skos:Concept ;
    rdfs:isDefinedBy ts:gts2020 ;
    skos:broader isc:MiddleOrdovician ;
    skos:definition "A time period with the following approximated bounds: older bound -467.3 +|-1.1 Ma, younger bound -458.4 +|-0.9 Ma" ;
    skos:inScheme cs: ;
    skos:prefLabel
        "Даривил"@bg ,
        "Darriwil"@cs ,
        "Darriwilien"@da ,
        "Darriwilium"@de ,
        "Darriwilian"@en ,
        "Darriwiliense"@es ,
        "Darriwili"@et ,
        "Darriwil"@fi ,
        "Darriwilien"@fr ,
        "darriwili"@hu ,
        "darriwilliano"@it ,
        "ダーリウィリアン期"@ja ,
        "Darivilis"@lt ,
        "Darriwiliën"@nl ,
        "Daewillium"@no ,
        "Darriwil"@pl ,
        "Darriwiliano"@pt ,
        "darriwil"@sk ,
        "darriwilij"@sl ,
        "darriwil"@sv ,
        "达瑞威尔期"@zh ;
    prov:wasDerivedFrom ts:gts2020 ;
.

isc:Drumian
    dcterms:identifier "Drumian" ;
    a skos:Concept ;
    rdfs:isDefinedBy ts:gts2020 ;
    skos:broader isc:Miaolingian ;
    skos:definition "A time period with the following approximated bounds: older bound -504.5 Ma, younger bound -500.5 Ma" ;
    skos:inScheme cs: ;
    skos:prefLabel
        "Друм"@bg ,
        "Drum"@cs ,
        "Drumien"@da ,
        "Drumium"@de ,
        "Drumian"@en ,
        "Drumiense"@es ,
        "Drumi"@et ,
        "Drum"@fi ,
        "Drumien"@fr ,
        "drumi"@hu ,
        "drumiano"@it ,
        "ドルミアン期"@ja ,
        "Drumis"@lt ,
        "Drumiën"@nl ,
        "Drumium"@no ,
        "Drum"@pl ,
        "Drumiano"@pt ,
        "drum"@sk ,
        "drumij"@sl ,
        "drum"@sv ,
        "鼓山期"@zh ;
    prov:wasDerivedFrom ts:gts2020 ;
.

isc:Ectasian
    dcterms:identifier "Ectasian" ;
    a skos:Concept ;
    rdfs:isDefinedBy ts:gts2020 ;
    skos:broader isc:Mesoproterozoic ;
    skos:definition "A time period with the following approximated bounds: older bound -1400 Ma, younger bound -1200 Ma" ;
    skos:inScheme cs: ;
    skos:prefLabel
        "Ектаз"@bg ,
        "Ectas"@cs ,
        "Ectasien"@da ,
        "Ectasium"@de ,
        "Ectasian"@en ,
        "Ectasiense"@es ,
        "Ectas"@et ,
        "Ectas"@fi ,
        "Ectasien"@fr ,
        "ectasi"@hu ,
        "ectasiano"@it ,
        "エクタシアン紀"@ja ,
        "Ektasis"@lt ,
        "Ectasiën"@nl ,
        "Ektasium"@no ,
        "Ektas"@pl ,
        "Ectasiano"@pt ,
        "ektazium"@sk ,
        "ectasij"@sl ,
        "ectasium"@sv ,
        "延展纪"@zh ;
    prov:wasDerivedFrom ts:gts2020 ;
.

isc:Ediacaran
    dcterms:identifier "Ediacaran" ;
    a skos:Concept ;
    rdfs:isDefinedBy ts:gts2020 ;
    skos:broader isc:Neoproterozoic ;
    skos:definition "A time period with the following approximated bounds: older bound -635 Ma, younger bound -541.0 +|-1.0 Ma" ;
    skos:inScheme cs: ;
    skos:prefLabel
        "Едиакар"@bg ,
        "Ediacar"@cs ,
        "Ediacara"@da ,
        "Ediacarium"@de ,
        "Ediacaran"@en ,
        "Ediacariense"@es ,
        "Ediacara"@et ,
        "Ediacar"@fi ,
        "Ediacarien"@fr ,
        "ediacaranum"@hu ,
        "ediacariano"@it ,
        "エディアカラ紀"@ja ,
        "Ediakaras"@lt ,
        "Ediacaran"@nl ,
        "Ediacara"@no ,
        "Ediakar"@pl ,
        "Ediacariano"@pt ,
        "ediakarium"@sk ,
        "ediacarij"@sl ,
        "ediacara"@sv ,
        "埃迪卡拉纪"@zh ;
    prov:wasDerivedFrom ts:gts2020 ;
.

isc:Eifelian
    dcterms:identifier "Eifelian" ;
    a skos:Concept ;
    rdfs:isDefinedBy ts:gts2020 ;
    skos:broader isc:MiddleDevonian ;
    skos:definition "A time period with the following approximated bounds: older bound -393.3 +|-1.2 Ma, younger bound -387.7 +|-0.8 Ma" ;
    skos:inScheme cs: ;
    skos:prefLabel
        "пйфел"@bg ,
        "Eifel"@cs ,
        "Eifelien"@da ,
        "Eifelium"@de ,
        "Eifelian"@en ,
        "Eifeliense"@es ,
        "Eifeli"@et ,
        "Eifel"@fi ,
        "Eifélien"@fr ,
        "eifeli"@hu ,
        "eifeliano"@it ,
        "アイフェリアン期"@ja ,
        "Eifelis"@lt ,
        "Eifeliën"@nl ,
        "Eifelium"@no ,
        "Eifel"@pl ,
        "Eifeliano"@pt ,
        "eifel"@sk ,
        "eifelij"@sl ,
        "eifel"@sv ,
        "艾菲尔期"@zh ;
    prov:wasDerivedFrom ts:gts2020 ;
.

isc:Emsian
    dcterms:identifier "Emsian" ;
    a skos:Concept ;
    rdfs:isDefinedBy ts:gts2020 ;
    skos:broader isc:LowerDevonian ;
    skos:definition "A time period with the following approximated bounds: older bound -407.6 +|-2.6 Ma, younger bound -393.3 +|-1.2 Ma" ;
    skos:inScheme cs: ;
    skos:prefLabel
        "Емѿ"@bg ,
        "Ems"@cs ,
        "Emsien"@da ,
        "Emsium"@de ,
        "Emsian"@en ,
        "Emsiense"@es ,
        "Emsi"@et ,
        "Ems"@fi ,
        "Emsien"@fr ,
        "emsi"@hu ,
        "emsiano"@it ,
        "エムシアン期"@ja ,
        "Emsis"@lt ,
        "Emsiën"@nl ,
        "Emsium"@no ,
        "Ems"@pl ,
        "Emsiano"@pt ,
        "ems"@sk ,
        "emsij"@sl ,
        "ems"@sv ,
        "艾姆斯期"@zh ;
    prov:wasDerivedFrom ts:gts2020 ;
.

isc:Eoarchean
    dcterms:identifier "Eoarchean" ;
    a skos:Concept ;
    rdfs:isDefinedBy ts:gts2020 ;
    skos:broader isc:Archean ;
    skos:definition "A time period with the following approximated bounds: older bound -4000 Ma, younger bound -3600 Ma" ;
    skos:inScheme cs: ;
    skos:prefLabel
        "Еоархай"@bg ,
        "Eoarchaikum"@cs ,
        "Eoarkæisk"@da ,
        "Eoarchaikum"@de ,
        "Eoarchean"@en ,
        "Eoarchaean"@en-gb ,
        "Eoarchean"@en-us ,
        "Eoarcaico"@es ,
        "Eoarhaikum"@et ,
        "Eoarkeikum"@fi ,
        "Eoarchéen"@fr ,
        "eoarchaikum"@hu ,
        "eoarcheano"@it ,
        "暁始生代"@ja ,
        "Eoarchejus"@lt ,
        "Eo-archaicum"@nl ,
        "Eoarkeikum"@no ,
        "Eoarchaik"@pl ,
        "Eoarcaico"@pt ,
        "eoarchaikum"@sk ,
        "eoarhaik"@sl ,
        "eoarkeikum"@sv ,
        "始太古代"@zh ;
    prov:wasDerivedFrom ts:gts2020 ;
.

isc:Famennian
    dcterms:identifier "Famennian" ;
    a skos:Concept ;
    rdfs:isDefinedBy ts:gts2020 ;
    skos:broader isc:UpperDevonian ;
    skos:definition "A time period with the following approximated bounds: older bound -372.2 +|-1.6 Ma, younger bound -358.9 +|-0.4 Ma" ;
    skos:inScheme cs: ;
    skos:prefLabel
        "Фамен"@bg ,
        "Famen"@cs ,
        "Famennien"@da ,
        "Fammennium"@de ,
        "Famennian"@en ,
        "Fameniense"@es ,
        "Famenne"@et ,
        "Fammenn"@fi ,
        "Famennien"@fr ,
        "famenni"@hu ,
        "famenniano"@it ,
        "ファメニアン期"@ja ,
        "Famenis"@lt ,
        "Famenniën"@nl ,
        "Famennium"@no ,
        "Famen"@pl ,
        "Fameniano"@pt ,
        "famen"@sk ,
        "fammenij"@sl ,
        "famenn"@sv ,
        "法门期"@zh ;
    prov:wasDerivedFrom ts:gts2020 ;
.

isc:Floian
    dcterms:identifier "Floian" ;
    a skos:Concept ;
    rdfs:isDefinedBy ts:gts2020 ;
    skos:broader isc:LowerOrdovician ;
    skos:definition "A time period with the following approximated bounds: older bound -477.7 +|-1.4 Ma, younger bound -470.0 +|-1.4 Ma" ;
    skos:inScheme cs: ;
    skos:prefLabel
        "Flo"@cs ,
        "Floian"@da ,
        "Floium"@de ,
        "Floian"@en ,
        "Floiense"@es ,
        "Floi"@et ,
        "Flo"@fi ,
        "Floien"@fr ,
        "floi"@hu ,
        "floiano"@it ,
        "フロイアン期"@ja ,
        "Flois"@lt ,
        "Floiën"@nl ,
        "Floium"@no ,
        "Flo"@pl ,
        "Floiano"@pt ,
        "flo"@sk ,
        "floij"@sl ,
        "flo"@sv ,
        "弗洛期"@zh ;
    prov:wasDerivedFrom ts:gts2020 ;
.

isc:Fortunian
    dcterms:identifier "Fortunian" ;
    a skos:Concept ;
    rdfs:isDefinedBy ts:gts2020 ;
    skos:broader isc:Terreneuvian ;
    skos:definition "A time period with the following approximated bounds: older bound -541.0 +|-1.0 Ma, younger bound -529 Ma" ;
    skos:inScheme cs: ;
    skos:prefLabel
        "Фортун"@bg ,
        "Fortun"@cs ,
        "Fortunien"@da ,
        "Fortunium"@de ,
        "Fortunian"@en ,
        "Fortuniense"@es ,
        "Fortune"@et ,
        "Fortun"@fi ,
        "Fortunien"@fr ,
        "fortuni"@hu ,
        "fortuniano"@it ,
        "フォルツニアン期"@ja ,
        "Fortunis"@lt ,
        "Fortuniën"@nl ,
        "Fortunium"@no ,
        "Fortun"@pl ,
        "Fortuniano"@pt ,
        "fortun"@sk ,
        "fortunij"@sl ,
        "fortun"@sv ,
        "好运期"@zh ;
    prov:wasDerivedFrom ts:gts2020 ;
.

isc:Frasnian
    dcterms:identifier "Frasnian" ;
    a skos:Concept ;
    rdfs:isDefinedBy ts:gts2020 ;
    skos:broader isc:UpperDevonian ;
    skos:definition "A time period with the following approximated bounds: older bound -382.7 +|-1.6 Ma, younger bound -372.2 +|-1.6 Ma" ;
    skos:inScheme cs: ;
    skos:prefLabel
        "Фран"@bg ,
        "Frasn"@cs ,
        "Frasnien"@da ,
        "Frasnium"@de ,
        "Frasnian"@en ,
        "Frasniense"@es ,
        "Frasne"@et ,
        "Frasn"@fi ,
        "Frasnien"@fr ,
        "frasni"@hu ,
        "frasniano"@it ,
        "フラスニアン期"@ja ,
        "Franis"@lt ,
        "Frasniën"@nl ,
        "Frasneium"@no ,
        "Fran"@pl ,
        "Frasniano"@pt ,
        "frasn"@sk ,
        "frasnij"@sl ,
        "frasn"@sv ,
        "弗拉斯期"@zh ;
    prov:wasDerivedFrom ts:gts2020 ;
.

isc:Gelasian
    dcterms:identifier "Gelasian" ;
    a skos:Concept ;
    rdfs:isDefinedBy ts:gts2020 ;
    skos:broader isc:Pleistocene ;
    skos:definition "A time period with the following approximated bounds: older bound -2.58 Ma, younger bound -1.80 Ma" ;
    skos:inScheme cs: ;
    skos:prefLabel
        "Gelas"@cs ,
        "Gelasian"@da ,
        "Gelasium"@de ,
        "Gelasian"@en ,
        "Gelasiense"@es ,
        "Gelasi"@et ,
        "Gelas"@fi ,
        "Gelasien"@fr ,
        "gelasi"@hu ,
        "gelasiano"@it ,
        "ゲラシアン期"@ja ,
        "Gelasis"@lt ,
        "Pretigliën + Tigliën"@nl ,
        "Gelasium"@no ,
        "Gelas"@pl ,
        "Gelasiano"@pt ,
        "gelas"@sk ,
        "gelasij"@sl ,
        "gelas"@sv ,
        "格拉斯期"@zh ;
    prov:wasDerivedFrom ts:gts2020 ;
.

isc:Givetian
    dcterms:identifier "Givetian" ;
    a skos:Concept ;
    rdfs:isDefinedBy ts:gts2020 ;
    skos:broader isc:MiddleDevonian ;
    skos:definition "A time period with the following approximated bounds: older bound -387.7 +|-0.8 Ma, younger bound -382.7 +|-1.6 Ma" ;
    skos:inScheme cs: ;
    skos:prefLabel
        "Живет"@bg ,
        "Givet"@cs ,
        "Givetien"@da ,
        "Givetium"@de ,
        "Givetian"@en ,
        "Givetiense"@es ,
        "Givet"@et ,
        "Givet"@fi ,
        "Givétien"@fr ,
        "giveti"@hu ,
        "givetiano"@it ,
        "ジベーチアン期"@ja ,
        "Živetis"@lt ,
        "Givetiën"@nl ,
        "Givetium"@no ,
        "Żywet"@pl ,
        "Givetiano"@pt ,
        "givet"@sk ,
        "givetij"@sl ,
        "givet"@sv ,
        "吉维特期"@zh ;
    prov:wasDerivedFrom ts:gts2020 ;
.

isc:Gorstian
    dcterms:identifier "Gorstian" ;
    a skos:Concept ;
    rdfs:isDefinedBy ts:gts2020 ;
    skos:broader isc:Ludlow ;
    skos:definition "A time period with the following approximated bounds: older bound -427.4 +|-0.5 Ma, younger bound -425.6 +|-0.9 Ma" ;
    skos:inScheme cs: ;
    skos:prefLabel
        "Горѿт"@bg ,
        "Gorst"@cs ,
        "Gorstien"@da ,
        "Gorstium"@de ,
        "Gorstian"@en ,
        "Gorstiense"@es ,
        "Gorsti"@et ,
        "Gorst"@fi ,
        "Gorstien"@fr ,
        "gorsti"@hu ,
        "gorstiano"@it ,
        "ゴースティアン期"@ja ,
        "Gorstis"@lt ,
        "Gorstiën"@nl ,
        "Gorstium"@no ,
        "Gorst"@pl ,
        "Gorstiano"@pt ,
        "gorst"@sk ,
        "gorstij"@sl ,
        "gorst"@sv ,
        "格斯特期"@zh ;
    prov:wasDerivedFrom ts:gts2020 ;
.

isc:Greenlandian
    dcterms:identifier "Greenlandian" ;
    a skos:Concept ;
    rdfs:isDefinedBy ts:gts2020 ;
    skos:broader isc:Holocene ;
    skos:definition "A time period with the following approximated bounds: older bound -0.0117 Ma, younger bound -0.0082 Ma" ;
    skos:inScheme cs: ;
    skos:prefLabel "Greenlandian"@en ;
    prov:wasDerivedFrom ts:gts2020 ;
.

isc:Guzhangian
    dcterms:identifier "Guzhangian" ;
    a skos:Concept ;
    rdfs:isDefinedBy ts:gts2020 ;
    skos:broader isc:Miaolingian ;
    skos:definition "A time period with the following approximated bounds: older bound -500.5 Ma, younger bound -497 Ma" ;
    skos:inScheme cs: ;
    skos:prefLabel
        "Жужанг"@bg ,
        "Guzhang"@cs ,
        "Guzhangien"@da ,
        "Guzhangium"@de ,
        "Guzhangian"@en ,
        "Guzhangiense"@es ,
        "Guzhangi"@et ,
        "Guzhang"@fi ,
        "Guzhangien"@fr ,
        "guzhangi"@hu ,
        "guzhangiano"@it ,
        "グザンギアン期"@ja ,
        "Gužangis"@lt ,
        "Guzhangiën"@nl ,
        "Guzhangium"@no ,
        "Gużang"@pl ,
        "Guzhangiano"@pt ,
        "gužang"@sk ,
        "guzhangij"@sl ,
        "guzhang"@sv ,
        "古丈期"@zh ;
    prov:wasDerivedFrom ts:gts2020 ;
.

isc:Gzhelian
    dcterms:identifier "Gzhelian" ;
    a skos:Concept ;
    rdfs:isDefinedBy ts:gts2020 ;
    skos:broader isc:UpperPennsylvanian ;
    skos:definition "A time period with the following approximated bounds: older bound -303.7 +|-0.1 Ma, younger bound -298.9 +|-0.15 Ma" ;
    skos:inScheme cs: ;
    skos:prefLabel
        "Гжел"@bg ,
        "Gzhel"@cs ,
        "Gzhelien"@da ,
        "Gzhelium"@de ,
        "Gzhelian"@en ,
        "Gzeliense"@es ,
        "Gzheli"@et ,
        "Gzhel"@fi ,
        "Gzhélien"@fr ,
        "gzseli"@hu ,
        "gzheliano"@it ,
        "グゼリアン期"@ja ,
        "Gželis"@lt ,
        "Gzheliën"@nl ,
        "Gzhelium"@no ,
        "Gżel"@pl ,
        "Gzeliano"@pt ,
        "gžel"@sk ,
        "gželij"@sl ,
        "gzhel"@sv ,
        "格热尔期"@zh ;
    prov:wasDerivedFrom ts:gts2020 ;
.

isc:Hadean
    dcterms:identifier "Hadean" ;
    a skos:Concept ;
    rdfs:isDefinedBy ts:gts2020 ;
    skos:broader isc:Precambrian ;
    skos:definition "A time period with the following approximated bounds: older bound -4567 +|-1 Ma, younger bound -4000 Ma" ;
    skos:inScheme cs: ;
    skos:prefLabel
        "Hád (spodní hranice není definována)"@cs ,
        "Hadean"@da ,
        "Hadaikum"@de ,
        "Hadean"@en ,
        "Hadeánico"@es ,
        "Hadesi??"@et ,
        "Hadea"@fi ,
        "Hadéen"@fr ,
        "hadei"@hu ,
        "adeano"@it ,
        "冥王代（非公式の）"@ja ,
        "Hadejus (neoficialus)"@lt ,
        "Hadeïcum"@nl ,
        "Hadeikum"@no ,
        "Hadean (Nieformalny)"@pl ,
        "Hadeano"@pt ,
        "hadaikum"@sk ,
        "hadej (neformalno)"@sl ,
        "hadeikum"@sv ,
        "冥古宙（非正式）"@zh ;
    prov:wasDerivedFrom ts:gts2020 ;
.

isc:Hauterivian
    dcterms:identifier "Hauterivian" ;
    a skos:Concept ;
    rdfs:isDefinedBy ts:gts2020 ;
    skos:broader isc:LowerCretaceous ;
    skos:definition "A time period with the following approximated bounds: older bound -132.9 Ma, younger bound -129.4 Ma" ;
    skos:inScheme cs: ;
    skos:prefLabel
        "Хотрив"@bg ,
        "Hauteriv"@cs ,
        "Hauterivien"@da ,
        "Hauterivium"@de ,
        "Hauterivian"@en ,
        "Hauteviriense"@es ,
        "Hauterivi"@et ,
        "Hauteriv"@fi ,
        "Hauterivien"@fr ,
        "hauterivi"@hu ,
        "hauteriviano"@it ,
        "オーテリビアン期"@ja ,
        "Hoterivis"@lt ,
        "Hauteriviën"@nl ,
        "Hauterivium"@no ,
        "Hoteryw"@pl ,
        "Hauteriviano"@pt ,
        "hauteriv"@sk ,
        "hauterivij"@sl ,
        "hauteriv"@sv ,
        "豪特里维期"@zh ;
    prov:wasDerivedFrom ts:gts2020 ;
.

isc:Hettangian
    dcterms:identifier "Hettangian" ;
    a skos:Concept ;
    rdfs:isDefinedBy ts:gts2020 ;
    skos:broader isc:LowerJurassic ;
    skos:definition "A time period with the following approximated bounds: older bound -201.3 +|-0.2 Ma, younger bound -199.3 +|-0.3 Ma" ;
    skos:inScheme cs: ;
    skos:prefLabel
        "Хетанж"@bg ,
        "Hettang"@cs ,
        "Hettangien"@da ,
        "Hettangium"@de ,
        "Hettangian"@en ,
        "Hettagiense"@es ,
        "Hettangi"@et ,
        "Hettang"@fi ,
        "Hettangien"@fr ,
        "hettangi"@hu ,
        "hettangiano"@it ,
        "ヘッタンギアン期"@ja ,
        "Hetangis"@lt ,
        "Hettangiën"@nl ,
        "Hettang"@no ,
        "Hetang"@pl ,
        "Hetangiano"@pt ,
        "hetanž"@sk ,
        "hettangij"@sl ,
        "hettang"@sv ,
        "赫唐期"@zh ;
    prov:wasDerivedFrom ts:gts2020 ;
.

isc:Hirnantian
    dcterms:identifier "Hirnantian" ;
    a skos:Concept ;
    rdfs:isDefinedBy ts:gts2020 ;
    skos:broader isc:UpperOrdovician ;
    skos:definition "A time period with the following approximated bounds: older bound -445.2 +|-1.4 Ma, younger bound -443.8 +|-1.5 Ma" ;
    skos:inScheme cs: ;
    skos:prefLabel
        "Хирнант"@bg ,
        "Hirnant"@cs ,
        "Hirnantien"@da ,
        "Hirnantium"@de ,
        "Hirnantian"@en ,
        "Hirnantiense"@es ,
        "Hirnantia"@et ,
        "Hirnant"@fi ,
        "Hirnantien"@fr ,
        "hirnanti"@hu ,
        "hirnantiano"@it ,
        "ヒルナンティアン期"@ja ,
        "Hirnantis"@lt ,
        "Hirnantiën"@nl ,
        "Hirnatium"@no ,
        "Hirnant"@pl ,
        "Hirnantiano"@pt ,
        "hirnant"@sk ,
        "hirnantij"@sl ,
        "hirnant"@sv ,
        "赫南特期"@zh ;
    prov:wasDerivedFrom ts:gts2020 ;
.

isc:Homerian
    dcterms:identifier "Homerian" ;
    a skos:Concept ;
    rdfs:isDefinedBy ts:gts2020 ;
    skos:broader isc:Wenlock ;
    skos:definition "A time period with the following approximated bounds: older bound -430.5 +|-0.7 Ma, younger bound -427.4 +|-0.5 Ma" ;
    skos:inScheme cs: ;
    skos:prefLabel
        "Хомер"@bg ,
        "Homer"@cs ,
        "Homerien"@da ,
        "Homerium"@de ,
        "Homerian"@en ,
        "Homeriense"@es ,
        "Homeri"@et ,
        "Homer"@fi ,
        "Homérien"@fr ,
        "homeri"@hu ,
        "homeriano"@it ,
        "ホメリアン期"@ja ,
        "Homeris"@lt ,
        "Homeriën"@nl ,
        "Homer"@no ,
        "Homer"@pl ,
        "Homeriano"@pt ,
        "homer"@sk ,
        "homerij"@sl ,
        "homer"@sv ,
        "侯默期"@zh ;
    prov:wasDerivedFrom ts:gts2020 ;
.

isc:Induan
    dcterms:identifier "Induan" ;
    a skos:Concept ;
    rdfs:isDefinedBy ts:gts2020 ;
    skos:broader isc:LowerTriassic ;
    skos:definition "A time period with the following approximated bounds: older bound -251.902 +|-0.024 Ma, younger bound -251.2 Ma" ;
    skos:inScheme cs: ;
    skos:prefLabel
        "Инд"@bg ,
        "Indu"@cs ,
        "Induen"@da ,
        "Indusium"@de ,
        "Induan"@en ,
        "Induense"@es ,
        "Indu"@et ,
        "Indus"@fi ,
        "Induen"@fr ,
        "indusi"@hu ,
        "induano"@it ,
        "インドゥアン期"@ja ,
        "Indis"@lt ,
        "Induiën"@nl ,
        "Indu"@no ,
        "Ind"@pl ,
        "Induano"@pt ,
        "indu"@sk ,
        "indij"@sl ,
        "indu"@sv ,
        "印度期"@zh ;
    prov:wasDerivedFrom ts:gts2020 ;
.

isc:Jiangshanian
    dcterms:identifier "Jiangshanian" ;
    a skos:Concept ;
    rdfs:isDefinedBy ts:gts2020 ;
    skos:broader isc:Furongian ;
    skos:definition "A time period with the following approximated bounds: older bound -494 Ma, younger bound -489.5 Ma" ;
    skos:inScheme cs: ;
    skos:prefLabel
        "Jiangshanian"@en ,
        "江山期"@zh ;
    prov:wasDerivedFrom ts:gts2020 ;
.

isc:Kasimovian
    dcterms:identifier "Kasimovian" ;
    a skos:Concept ;
    rdfs:isDefinedBy ts:gts2020 ;
    skos:broader isc:UpperPennsylvanian ;
    skos:definition "A time period with the following approximated bounds: older bound -307 +|-0.1 Ma, younger bound -303.7 +|-0.1 Ma" ;
    skos:inScheme cs: ;
    skos:prefLabel
        "Каѿимов"@bg ,
        "Kasimov"@cs ,
        "Kasimovien"@da ,
        "Kasimovium"@de ,
        "Kasimovian"@en ,
        "Kasimoviense"@es ,
        "Kasimovi"@et ,
        "Kasimov"@fi ,
        "Kasimovien"@fr ,
        "kaszimovi"@hu ,
        "kasimoviano"@it ,
        "カシモビアン期"@ja ,
        "Kasimovis"@lt ,
        "Kasimoviën"@nl ,
        "Kasimovium"@no ,
        "Kasimow"@pl ,
        "Kasimoviano"@pt ,
        "kasimov"@sk ,
        "kasimovij"@sl ,
        "kasimov"@sv ,
        "卡西莫夫期"@zh ;
    prov:wasDerivedFrom ts:gts2020 ;
.

isc:Katian
    dcterms:identifier "Katian" ;
    a skos:Concept ;
    rdfs:isDefinedBy ts:gts2020 ;
    skos:broader isc:UpperOrdovician ;
    skos:definition "A time period with the following approximated bounds: older bound -453 +|-0.7 Ma, younger bound -445.2 +|-1.4 Ma" ;
    skos:inScheme cs: ;
    skos:prefLabel
        "Кат"@bg ,
        "Kat"@cs ,
        "Katien"@da ,
        "Katium"@de ,
        "Katian"@en ,
        "Katiense"@es ,
        "Kati"@et ,
        "Kat"@fi ,
        "Katien"@fr ,
        "kati"@hu ,
        "katiano"@it ,
        "カティアン期"@ja ,
        "Katis"@lt ,
        "Katiën"@nl ,
        "Katium"@no ,
        "Kat"@pl ,
        "Katiano"@pt ,
        "kat"@sk ,
        "katij"@sl ,
        "kat"@sv ,
        "凯迪期"@zh ;
    prov:wasDerivedFrom ts:gts2020 ;
.

isc:Kimmeridgian
    dcterms:identifier "Kimmeridgian" ;
    a skos:Concept ;
    rdfs:isDefinedBy ts:gts2020 ;
    skos:broader isc:UpperJurassic ;
    skos:definition "A time period with the following approximated bounds: older bound -157.3 +|-1.0 Ma, younger bound -152.1 +|-0.9 Ma" ;
    skos:inScheme cs: ;
    skos:prefLabel
        "Кимеридж"@bg ,
        "Kimmeridž"@cs ,
        "Kimmeridgien"@da ,
        "Kimmeridgium"@de ,
        "Kimmeridgian"@en ,
        "Kimmeridgiense"@es ,
        "Kimmeridge"@et ,
        "Kimmeridge"@fi ,
        "Kimméridgien"@fr ,
        "kimmeridgei"@hu ,
        "kimmeridgiano"@it ,
        "キンメリッジアン期"@ja ,
        "Kimeridis"@lt ,
        "Kimmeridgiën"@nl ,
        "Kimmeridge"@no ,
        "Kimeryd"@pl ,
        "Kimeridgiano"@pt ,
        "kimeridž"@sk ,
        "kimmeridgij"@sl ,
        "kimmeridge"@sv ,
        "启莫里支期"@zh ;
    prov:wasDerivedFrom ts:gts2020 ;
.

isc:Kungurian
    dcterms:identifier "Kungurian" ;
    a skos:Concept ;
    rdfs:isDefinedBy ts:gts2020 ;
    skos:broader isc:Cisuralian ;
    skos:definition "A time period with the following approximated bounds: older bound -283.5 +|-0.6 Ma, younger bound -272.95 +|-0.11 Ma" ;
    skos:inScheme cs: ;
    skos:prefLabel
        "Кунгур"@bg ,
        "Kungur"@cs ,
        "Kungurien"@da ,
        "Kungurium"@de ,
        "Kungurian"@en ,
        "Kunguriense"@es ,
        "Kunguri"@et ,
        "Kungur"@fi ,
        "Kungurien"@fr ,
        "kunguri"@hu ,
        "kungurianno"@it ,
        "クングリアン期"@ja ,
        "Kunguris"@lt ,
        "Kunguriën"@nl ,
        "Kungurium"@no ,
        "Kungur"@pl ,
        "Kunguriano"@pt ,
        "kungur"@sk ,
        "kungurij"@sl ,
        "kungur"@sv ,
        "孔古尔期"@zh ;
    prov:wasDerivedFrom ts:gts2020 ;
.

isc:Ladinian
    dcterms:identifier "Ladinian" ;
    a skos:Concept ;
    rdfs:isDefinedBy ts:gts2020 ;
    skos:broader isc:MiddleTriassic ;
    skos:definition "A time period with the following approximated bounds: older bound -242 Ma, younger bound -237 Ma" ;
    skos:inScheme cs: ;
    skos:prefLabel
        "Ладин"@bg ,
        "Ladin"@cs ,
        "Ladinien"@da ,
        "Ladinium"@de ,
        "Ladinian"@en ,
        "Ladiniense"@es ,
        "Ladini"@et ,
        "Ladin"@fi ,
        "Ladinien"@fr ,
        "ladin"@hu ,
        "ladinico"@it ,
        "ラディニアン期"@ja ,
        "Ladinis"@lt ,
        "Ladiniën"@nl ,
        "Ladin"@no ,
        "Ladyn"@pl ,
        "Ladiniano"@pt ,
        "ladin"@sk ,
        "ladinij"@sl ,
        "ladin"@sv ,
        "拉迪尼亚期"@zh ;
    prov:wasDerivedFrom ts:gts2020 ;
.

isc:Langhian
    dcterms:identifier "Langhian" ;
    a skos:Concept ;
    rdfs:isDefinedBy ts:gts2020 ;
    skos:broader isc:Miocene ;
    skos:definition "A time period with the following approximated bounds: older bound -15.97 Ma, younger bound -13.82 Ma" ;
    skos:inScheme cs: ;
    skos:prefLabel
        "Ланг"@bg ,
        "Langh"@cs ,
        "Langhien"@da ,
        "Langhium"@de ,
        "Langhian"@en ,
        "Langhiense"@es ,
        "Langhi"@et ,
        "Langh"@fi ,
        "Langhien"@fr ,
        "langhei"@hu ,
        "langhiano"@it ,
        "ランギアン期"@ja ,
        "Langis"@lt ,
        "Langhiën-Reinbek"@nl ,
        "Langhium"@no ,
        "Lang"@pl ,
        "Langhiano"@pt ,
        "langh"@sk ,
        "langhij"@sl ,
        "langh"@sv ,
        "兰海期"@zh ;
    prov:wasDerivedFrom ts:gts2020 ;
.

isc:Lochkovian
    dcterms:identifier "Lochkovian" ;
    a skos:Concept ;
    rdfs:isDefinedBy ts:gts2020 ;
    skos:broader isc:LowerDevonian ;
    skos:definition "A time period with the following approximated bounds: older bound -419.2 +|-3.2 Ma, younger bound -410.8 +|-2.8 Ma" ;
    skos:inScheme cs: ;
    skos:prefLabel
        "Ложков"@bg ,
        "Lochkov"@cs ,
        "Lochkovien"@da ,
        "Lochkovium"@de ,
        "Lochkovian"@en ,
        "Lochkoviense"@es ,
        "Lochkovi"@et ,
        "Lochkov"@fi ,
        "Lochkovien"@fr ,
        "lochkovi"@hu ,
        "lochkoviano"@it ,
        "ロッコビアン期"@ja ,
        "Lochkovis"@lt ,
        "Lochkoviën"@nl ,
        "Lochkovium"@no ,
        "Lochkow"@pl ,
        "Lochkoviano"@pt ,
        "lochkov"@sk ,
        "lochkovij"@sl ,
        "lochkov"@sv ,
        "洛赫科夫期"@zh ;
    prov:wasDerivedFrom ts:gts2020 ;
.

isc:Ludfordian
    dcterms:identifier "Ludfordian" ;
    a skos:Concept ;
    rdfs:isDefinedBy ts:gts2020 ;
    skos:broader isc:Ludlow ;
    skos:definition "A time period with the following approximated bounds: older bound -425.6 +|-0.9 Ma, younger bound -423 +|-2.3 Ma" ;
    skos:inScheme cs: ;
    skos:prefLabel
        "Лудфорд"@bg ,
        "Ludford"@cs ,
        "Ludfordien"@da ,
        "Ludfordium"@de ,
        "Ludfordian"@en ,
        "Ludfordiense"@es ,
        "Ludfordi"@et ,
        "Ludford"@fi ,
        "Ludfordien"@fr ,
        "ludfordi"@hu ,
        "ludfordiano"@it ,
        "ルドフォーディアン期"@ja ,
        "Lutfordis"@lt ,
        "Ludfordiën"@nl ,
        "Ludford"@no ,
        "Ludford"@pl ,
        "Ludfordiano"@pt ,
        "ludford"@sk ,
        "ludfordij"@sl ,
        "ludford"@sv ,
        "卢德福德期"@zh ;
    prov:wasDerivedFrom ts:gts2020 ;
.

isc:Lutetian
    dcterms:identifier "Lutetian" ;
    a skos:Concept ;
    rdfs:isDefinedBy ts:gts2020 ;
    skos:broader isc:Eocene ;
    skos:definition "A time period with the following approximated bounds: older bound -47.8 Ma, younger bound -41.2 Ma" ;
    skos:inScheme cs: ;
    skos:prefLabel
        "Лютеѿ"@bg ,
        "Lutet"@cs ,
        "Lutetien"@da ,
        "Lutetium"@de ,
        "Lutetian"@en ,
        "Luteciense"@es ,
        "Luteti"@et ,
        "Lutet"@fi ,
        "Lutétien"@fr ,
        "lutetiai"@hu ,
        "leteziano"@it ,
        "ルテシアン期"@ja ,
        "Liutetis"@lt ,
        "Lutetiën"@nl ,
        "Litetium"@no ,
        "Lutet"@pl ,
        "Luteciano"@pt ,
        "lutét"@sk ,
        "lutecij"@sl ,
        "lutet"@sv ,
        "卢台特期"@zh ;
    prov:wasDerivedFrom ts:gts2020 ;
.

isc:Maastrichtian
    dcterms:identifier "Maastrichtian" ;
    a skos:Concept ;
    rdfs:isDefinedBy ts:gts2020 ;
    skos:broader isc:UpperCretaceous ;
    skos:definition "A time period with the following approximated bounds: older bound -72.1 +|-0.2 Ma, younger bound -66.0 Ma" ;
    skos:inScheme cs: ;
    skos:prefLabel
        "Маѿтрихт"@bg ,
        "Maastricht"@cs ,
        "Maastrichtien"@da ,
        "Maastrichtium"@de ,
        "Maastrichtian"@en ,
        "Maastrichtiense"@es ,
        "Maastrichti"@et ,
        "Maastricht"@fi ,
        "Maastrichtien"@fr ,
        "maastrichti"@hu ,
        "maastrichtiano"@it ,
        "マーストリヒシアン期"@ja ,
        "Mastrichtis"@lt ,
        "Maastrichtiën"@nl ,
        "Maastricht"@no ,
        "Mastrycht"@pl ,
        "Maestrichtiano"@pt ,
        "mástricht"@sk ,
        "maastrichtij"@sl ,
        "maastricht"@sv ,
        "马斯特里赫特期"@zh ;
    prov:wasDerivedFrom ts:gts2020 ;
.

isc:Meghalayan
    dcterms:identifier "Meghalayan" ;
    a skos:Concept ;
    rdfs:isDefinedBy ts:gts2020 ;
    skos:broader isc:Holocene ;
    skos:definition "A time period with the following approximated bounds: older bound -0.0042 Ma, younger bound 0 Ma" ;
    skos:inScheme cs: ;
    skos:prefLabel "Meghalayan"@en ;
    prov:wasDerivedFrom ts:gts2020 ;
.

isc:Mesoarchean
    dcterms:identifier "Mesoarchean" ;
    a skos:Concept ;
    rdfs:isDefinedBy ts:gts2020 ;
    skos:broader isc:Archean ;
    skos:definition "A time period with the following approximated bounds: older bound -3200 Ma, younger bound -2800 Ma" ;
    skos:inScheme cs: ;
    skos:prefLabel
        "Мезоархай"@bg ,
        "Mezoarchaikum"@cs ,
        "Mesoarkæisk"@da ,
        "Mesoarchaikum"@de ,
        "Mesoarchean"@en ,
        "Mesoarchaean"@en-gb ,
        "Mesoarchean"@en-us ,
        "Mesoarcaico"@es ,
        "Mesoarhaikum"@et ,
        "Mesoarkeikum"@fi ,
        "Mésoarchéen"@fr ,
        "mezoarchai"@hu ,
        "mesoarcheano"@it ,
        "中始生代"@ja ,
        "Mezoarchejus"@lt ,
        "Meso-archaicum"@nl ,
        "Mesoarkeikum"@no ,
        "Mezoarchaik"@pl ,
        "Mesoarcaico"@pt ,
        "mezoarchaikum"@sk ,
        "mezoarhaik"@sl ,
        "mesoarkeikum"@sv ,
        "中太古代"@zh ;
    prov:wasDerivedFrom ts:gts2020 ;
.

isc:Messinian
    dcterms:identifier "Messinian" ;
    a skos:Concept ;
    rdfs:isDefinedBy ts:gts2020 ;
    skos:broader isc:Miocene ;
    skos:definition "A time period with the following approximated bounds: older bound -7.246 Ma, younger bound -5.333 Ma" ;
    skos:inScheme cs: ;
    skos:prefLabel
        "Меѿин"@bg ,
        "Messin"@cs ,
        "Messinien"@da ,
        "Messinium"@de ,
        "Messinian"@en ,
        "Messiniense"@es ,
        "Messini"@et ,
        "Messina"@fi ,
        "Messinien"@fr ,
        "messinai"@hu ,
        "messiniano"@it ,
        "メッシニアン期"@ja ,
        "Mesinis"@lt ,
        "Susteriën"@nl ,
        "Messinium"@no ,
        "Messyn"@pl ,
        "Messiniano"@pt ,
        "messin"@sk ,
        "messinij"@sl ,
        "messin"@sv ,
        "墨西拿期"@zh ;
    prov:wasDerivedFrom ts:gts2020 ;
.

isc:MiddlePleistocene
    dcterms:identifier "MiddlePleistocene" ;
    a skos:Concept ;
    rdfs:isDefinedBy ts:gts2020 ;
    skos:broader isc:Pleistocene ;
    skos:definition "A time period with the following approximated bounds: older bound -0.781 Ma, younger bound -0.126 Ma" ;
    skos:inScheme cs: ;
    skos:prefLabel "Chibanian"@en ;
    prov:wasDerivedFrom ts:gts2020 ;
.

isc:Moscovian
    dcterms:identifier "Moscovian" ;
    a skos:Concept ;
    rdfs:isDefinedBy ts:gts2020 ;
    skos:broader isc:MiddlePennsylvanian ;
    skos:definition "A time period with the following approximated bounds: older bound -315.2 +|-0.2 Ma, younger bound -307 +|-0.1 Ma" ;
    skos:inScheme cs: ;
    skos:prefLabel
        "Моѿков"@bg ,
        "Moscov"@cs ,
        "Moscovien"@da ,
        "Moskovium"@de ,
        "Moscovian"@en ,
        "Moscoviense"@es ,
        "Moskva"@et ,
        "Moskova"@fi ,
        "Moscovien"@fr ,
        "moszkvai"@hu ,
        "moscoviano"@it ,
        "モスコビアン期"@ja ,
        "Moskovis"@lt ,
        "Moscoviën"@nl ,
        "Moskovium"@no ,
        "Moskow"@pl ,
        "Moscoviano"@pt ,
        "moskov"@sk ,
        "moskovij"@sl ,
        "moscov"@sv ,
        "莫斯科期"@zh ;
    prov:wasDerivedFrom ts:gts2020 ;
.

isc:Neoarchean
    dcterms:identifier "Neoarchean" ;
    a skos:Concept ;
    rdfs:isDefinedBy ts:gts2020 ;
    skos:broader isc:Archean ;
    skos:definition "A time period with the following approximated bounds: older bound -2800 Ma, younger bound -2500 Ma" ;
    skos:inScheme cs: ;
    skos:prefLabel
        "пеоархай"@bg ,
        "Neoarchaikum"@cs ,
        "Neoarkæisk"@da ,
        "Neoarchaikum"@de ,
        "Neoarchean"@en ,
        "Neoarchaean"@en-gb ,
        "Neoarchean"@en-us ,
        "Neoarcaico"@es ,
        "Neoarhaikum"@et ,
        "Neoarkeikum"@fi ,
        "Néoarchéen"@fr ,
        "neoarchaikum"@hu ,
        "neoarcheano"@it ,
        "新始生代"@ja ,
        "Neoarchejus"@lt ,
        "Neo-archaicum"@nl ,
        "Neoarkeikum"@no ,
        "Neoarchaik"@pl ,
        "Neoarcaico"@pt ,
        "neoarchaikum"@sk ,
        "neoarhaik"@sl ,
        "neoarkeikum"@sv ,
        "新太古代"@zh ;
    prov:wasDerivedFrom ts:gts2020 ;
.

isc:Norian
    dcterms:identifier "Norian" ;
    a skos:Concept ;
    rdfs:isDefinedBy ts:gts2020 ;
    skos:broader isc:UpperTriassic ;
    skos:definition "A time period with the following approximated bounds: older bound -227 Ma, younger bound -208.5 Ma" ;
    skos:inScheme cs: ;
    skos:prefLabel
        "пор"@bg ,
        "Nor"@cs ,
        "Norien"@da ,
        "Norium"@de ,
        "Norian"@en ,
        "Noriense"@es ,
        "Nori"@et ,
        "Nor"@fi ,
        "Norien"@fr ,
        "nori"@hu ,
        "norico"@it ,
        "ノーリアン期"@ja ,
        "Noris"@lt ,
        "Noriën"@nl ,
        "Nor"@no ,
        "Noryk"@pl ,
        "Noriano"@pt ,
        "norik"@sk ,
        "norij"@sl ,
        "nor"@sv ,
        "诺利克期"@zh ;
    prov:wasDerivedFrom ts:gts2020 ;
.

isc:Northgrippian
    dcterms:identifier "Northgrippian" ;
    a skos:Concept ;
    rdfs:isDefinedBy ts:gts2020 ;
    skos:broader isc:Holocene ;
    skos:definition "A time period with the following approximated bounds: older bound -0.0082 Ma, younger bound -0.0042 Ma" ;
    skos:inScheme cs: ;
    skos:prefLabel "Northgrippian"@en ;
    prov:wasDerivedFrom ts:gts2020 ;
.

isc:Olenekian
    dcterms:identifier "Olenekian" ;
    a skos:Concept ;
    rdfs:isDefinedBy ts:gts2020 ;
    skos:broader isc:LowerTriassic ;
    skos:definition "A time period with the following approximated bounds: older bound -251.2 Ma, younger bound -247.2 Ma" ;
    skos:inScheme cs: ;
    skos:prefLabel
        "Оленек"@bg ,
        "Olenek"@cs ,
        "Olenekien"@da ,
        "Olenekium"@de ,
        "Olenekian"@en ,
        "Olenekiense"@es ,
        "Oleneki"@et ,
        "Olenek"@fi ,
        "Olénekien"@fr ,
        "olenyoki"@hu ,
        "olenekiano"@it ,
        "オレネキアン期"@ja ,
        "Olenekis"@lt ,
        "Olenekiën"@nl ,
        "Olenek"@no ,
        "Olenek"@pl ,
        "Olenekiano"@pt ,
        "olenek"@sk ,
        "olenekij"@sl ,
        "olenek"@sv ,
        "奥伦尼克期"@zh ;
    prov:wasDerivedFrom ts:gts2020 ;
.

isc:Orosirian
    dcterms:identifier "Orosirian" ;
    a skos:Concept ;
    rdfs:isDefinedBy ts:gts2020 ;
    skos:broader isc:Paleoproterozoic ;
    skos:definition "A time period with the following approximated bounds: older bound -2050 Ma, younger bound -1800 Ma" ;
    skos:inScheme cs: ;
    skos:prefLabel
        "Ороѿир"@bg ,
        "Orosir"@cs ,
        "Orosirien"@da ,
        "Orosirium"@de ,
        "Orosirian"@en ,
        "Orosiriense"@es ,
        "Orosir"@et ,
        "Orosir"@fi ,
        "Orosirien"@fr ,
        "orosiri"@hu ,
        "orosiriano"@it ,
        "オロシリアン紀"@ja ,
        "Orosiris"@lt ,
        "Orosiriën"@nl ,
        "Orosirium"@no ,
        "Orosir"@pl ,
        "Orosiriano"@pt ,
        "orosirium"@sk ,
        "orosijrij"@sl ,
        "orosirium"@sv ,
        "造山纪"@zh ;
    prov:wasDerivedFrom ts:gts2020 ;
.

isc:Oxfordian
    dcterms:identifier "Oxfordian" ;
    a skos:Concept ;
    rdfs:isDefinedBy ts:gts2020 ;
    skos:broader isc:UpperJurassic ;
    skos:definition "A time period with the following approximated bounds: older bound -163.5 +|-1.0 Ma, younger bound -157.3 +|-1.0 Ma" ;
    skos:inScheme cs: ;
    skos:prefLabel
        "Окѿфорд"@bg ,
        "Oxford"@cs ,
        "Oxfordien"@da ,
        "Oxfordium"@de ,
        "Oxfordian"@en ,
        "Oxfordiense"@es ,
        "Oxfordi"@et ,
        "Oxford"@fi ,
        "Oxfordien"@fr ,
        "oxfordi"@hu ,
        "oxfordiano"@it ,
        "オックスフォーディアン期"@ja ,
        "Oksfordis"@lt ,
        "Oxfordiën"@nl ,
        "Oxford"@no ,
        "Oksford"@pl ,
        "Oxfordiano"@pt ,
        "oxford"@sk ,
        "oxfordij"@sl ,
        "oxford"@sv ,
        "牛津期"@zh ;
    prov:wasDerivedFrom ts:gts2020 ;
.

isc:Paibian
    dcterms:identifier "Paibian" ;
    a skos:Concept ;
    rdfs:isDefinedBy ts:gts2020 ;
    skos:broader isc:Furongian ;
    skos:definition "A time period with the following approximated bounds: older bound -497 Ma, younger bound -494 Ma" ;
    skos:inScheme cs: ;
    skos:prefLabel
        "Паиб"@bg ,
        "Paib"@cs ,
        "Paibien"@da ,
        "Paibium"@de ,
        "Paibian"@en ,
        "Paibiense"@es ,
        "Paibi"@et ,
        "Paib"@fi ,
        "Paibien"@fr ,
        "paibi"@hu ,
        "paibiano"@it ,
        "パイビアン期"@ja ,
        "Paibis"@lt ,
        "Paibiën"@nl ,
        "Paibium"@no ,
        "Paib"@pl ,
        "Paibiano"@pt ,
        "pajb"@sk ,
        "paibij"@sl ,
        "paib"@sv ,
        "排碧期"@zh ;
    prov:wasDerivedFrom ts:gts2020 ;
.

isc:Paleoarchean
    dcterms:identifier "Paleoarchean" ;
    a skos:Concept ;
    rdfs:isDefinedBy ts:gts2020 ;
    skos:broader isc:Archean ;
    skos:definition "A time period with the following approximated bounds: older bound -3600 Ma, younger bound -3200 Ma" ;
    skos:inScheme cs: ;
    skos:prefLabel
        "Палеоархай"@bg ,
        "Paleoarchaikum"@cs ,
        "Palæoarkæisk"@da ,
        "Paläoarchaikum"@de ,
        "Paleoarchean"@en ,
        "Palaeoarchaean"@en-gb ,
        "Paleoarchean"@en-us ,
        "Paleoarcaico"@es ,
        "Paleoarhaikum"@et ,
        "Paleoarkeikum"@fi ,
        "Paléoarchéen"@fr ,
        "paleoarchai"@hu ,
        "paleoarcheano"@it ,
        "古始生代"@ja ,
        "Paleoarchejus"@lt ,
        "Paleo-archaicum"@nl ,
        "Paleoarkeikum"@no ,
        "Paleoarchaik"@pl ,
        "Paleoarcaico"@pt ,
        "paleoarchaikum"@sk ,
        "paleoarhaik"@sl ,
        "paleoarkeikum"@sv ,
        "古太古代"@zh ;
    prov:wasDerivedFrom ts:gts2020 ;
.

isc:Piacenzian
    dcterms:identifier "Piacenzian" ;
    a skos:Concept ;
    rdfs:isDefinedBy ts:gts2020 ;
    skos:broader isc:Pliocene ;
    skos:definition "A time period with the following approximated bounds: older bound -3.6 Ma, younger bound -2.58 Ma" ;
    skos:inScheme cs: ;
    skos:prefLabel
        "Пиачен"@bg ,
        "Piacenz"@cs ,
        "Piacenzien"@da ,
        "Piacenzium"@de ,
        "Piacenzian"@en ,
        "Plazenciense"@es ,
        "Piacenzi"@et ,
        "Piacenz"@fi ,
        "Piacenzien"@fr ,
        "piacenzai"@hu ,
        "piacenziano"@it ,
        "ﾋﾟｱｾﾝｼﾞｱﾝ期"@ja ,
        "PiaĿenzis"@lt ,
        "Reuveriën"@nl ,
        "Piecenzium"@no ,
        "Piacenz"@pl ,
        "Placenciano"@pt ,
        "piaĿenz"@sk ,
        "piacenzij"@sl ,
        "piacenz"@sv ,
        "皮亚琴期"@zh ;
    prov:wasDerivedFrom ts:gts2020 ;
.

isc:Pliensbachian
    dcterms:identifier "Pliensbachian" ;
    a skos:Concept ;
    rdfs:isDefinedBy ts:gts2020 ;
    skos:broader isc:LowerJurassic ;
    skos:definition "A time period with the following approximated bounds: older bound -190.8 +|-1.0 Ma, younger bound -182.7 +|-0.7 Ma" ;
    skos:inScheme cs: ;
    skos:prefLabel
        "Плиинѿбах"@bg ,
        "Pliensbach"@cs ,
        "Pliensbachien"@da ,
        "Pliensbachium"@de ,
        "Pliensbachian"@en ,
        "Pliensbachiense"@es ,
        "Pliensbachi"@et ,
        "Plienbach"@fi ,
        "Pliensbachien"@fr ,
        "pliensbachi"@hu ,
        "pliensbachiano"@it ,
        "プリンスバッキアン期"@ja ,
        "Plynsbachis"@lt ,
        "Pliënsbachiën"@nl ,
        "Pliensbach"@no ,
        "Pliensbach"@pl ,
        "Pliensbaquiano"@pt ,
        "pliensbach"@sk ,
        "pleinsbachij"@sl ,
        "pliensbach"@sv ,
        "普连斯巴奇期"@zh ;
    prov:wasDerivedFrom ts:gts2020 ;
.

isc:Pragian
    dcterms:identifier "Pragian" ;
    a skos:Concept ;
    rdfs:isDefinedBy ts:gts2020 ;
    skos:broader isc:LowerDevonian ;
    skos:definition "A time period with the following approximated bounds: older bound -410.8 +|-2.8 Ma, younger bound -407.6 +|-2.6 Ma" ;
    skos:inScheme cs: ;
    skos:prefLabel
        "Праг"@bg ,
        "Prag"@cs ,
        "Pragien"@da ,
        "Pragium"@de ,
        "Pragian"@en ,
        "Praguiense"@es ,
        "Praha"@et ,
        "Praha"@fi ,
        "Praguien"@fr ,
        "prágai"@hu ,
        "pragiano"@it ,
        "プラギアン期"@ja ,
        "Pragis"@lt ,
        "Pragiën"@nl ,
        "Pragium"@no ,
        "Prag"@pl ,
        "Pragiano"@pt ,
        "prág"@sk ,
        "pragij"@sl ,
        "prag"@sv ,
        "布拉格期"@zh ;
    prov:wasDerivedFrom ts:gts2020 ;
.

isc:Priabonian
    dcterms:identifier "Priabonian" ;
    a skos:Concept ;
    rdfs:isDefinedBy ts:gts2020 ;
    skos:broader isc:Eocene ;
    skos:definition "A time period with the following approximated bounds: older bound -37.8 Ma, younger bound -33.9 Ma" ;
    skos:inScheme cs: ;
    skos:prefLabel
        "Приабон"@bg ,
        "Priabon"@cs ,
        "Priabonien"@da ,
        "Priabonium"@de ,
        "Priabonian"@en ,
        "Priaboniense"@es ,
        "Priaboni"@et ,
        "Priabon"@fi ,
        "Priabonien"@fr ,
        "priabonai"@hu ,
        "priaboniano"@it ,
        "プリアボニアン期"@ja ,
        "Priabonis"@lt ,
        "Priaboniën"@nl ,
        "Priabon"@no ,
        "Priabon"@pl ,
        "Priaboniano"@pt ,
        "priabón"@sk ,
        "priabonij"@sl ,
        "priabon"@sv ,
        "普里阿邦期"@zh ;
    prov:wasDerivedFrom ts:gts2020 ;
.

isc:Pridoli
    dcterms:identifier "Pridoli" ;
    a skos:Concept ;
    rdfs:isDefinedBy ts:gts2020 ;
    skos:broader isc:Silurian ;
    skos:definition "A time period with the following approximated bounds: older bound -423 +|-2.3 Ma, younger bound -419.2 +|-3.2 Ma" ;
    skos:inScheme cs: ;
    skos:prefLabel
        "Пржидол"@bg ,
        "Přídolí"@cs ,
        "Pridoli"@da ,
        "Pridoli"@de ,
        "Pridoli"@en ,
        "Prídoli"@es ,
        "Pridoli"@et ,
        "Pridoli"@fi ,
        "Pridoli"@fr ,
        "pridoli"@hu ,
        "pridoli"@it ,
        "プリドリアン世"@ja ,
        "Pržidolis"@lt ,
        "Pridoli"@nl ,
        "Pridoli"@no ,
        "Przydol"@pl ,
        "Pridoli"@pt ,
        "přídol"@sk ,
        "pridolij"@sl ,
        "pridoli"@sv ,
        "普里多利世"@zh ;
    prov:wasDerivedFrom ts:gts2020 ;
.

isc:Rhaetian
    dcterms:identifier "Rhaetian" ;
    a skos:Concept ;
    rdfs:isDefinedBy ts:gts2020 ;
    skos:broader isc:UpperTriassic ;
    skos:definition "A time period with the following approximated bounds: older bound -208.5 Ma, younger bound -201.3 +|-0.2 Ma" ;
    skos:inScheme cs: ;
    skos:prefLabel
        "Рет"@bg ,
        "Rhaet"@cs ,
        "Rhaetien"@da ,
        "Rhätium"@de ,
        "Rhaetian"@en ,
        "Rhetiense"@es ,
        "Rhaeti"@et ,
        "Rhaet"@fi ,
        "Rhétien"@fr ,
        "rhaeti"@hu ,
        "retico"@it ,
        "レーティアン期"@ja ,
        "Retis"@lt ,
        "Rhaetiën"@nl ,
        "Ræt"@no ,
        "Retyk"@pl ,
        "Reciano"@pt ,
        "rét"@sk ,
        "retij"@sl ,
        "rät"@sv ,
        "瑞替期"@zh ;
    prov:wasDerivedFrom ts:gts2020 ;
.

isc:Rhuddanian
    dcterms:identifier "Rhuddanian" ;
    a skos:Concept ;
    rdfs:isDefinedBy ts:gts2020 ;
    skos:broader isc:Llandovery ;
    skos:definition "A time period with the following approximated bounds: older bound -443.8 +|-1.5 Ma, younger bound -440.8 +|-1.2 Ma" ;
    skos:inScheme cs: ;
    skos:prefLabel
        "Рудан"@bg ,
        "Rhuddan"@cs ,
        "Rhuddanien"@da ,
        "Rhuddanium"@de ,
        "Rhuddanian"@en ,
        "Rhuddaniense"@es ,
        "Rhuddani"@et ,
        "Rhuddan"@fi ,
        "Rhuddanien"@fr ,
        "rhuddani"@hu ,
        "rhuddaniano"@it ,
        "ルダニアン期"@ja ,
        "Rudanis"@lt ,
        "Rhuddaniën"@nl ,
        "Rhuddanium"@no ,
        "Rhuddan"@pl ,
        "Rudaniano"@pt ,
        "rhuddan"@sk ,
        "rhuddanij"@sl ,
        "rhuddan"@sv ,
        "鲁丹期"@zh ;
    prov:wasDerivedFrom ts:gts2020 ;
.

isc:Rhyacian
    dcterms:identifier "Rhyacian" ;
    a skos:Concept ;
    rdfs:isDefinedBy ts:gts2020 ;
    skos:broader isc:Paleoproterozoic ;
    skos:definition "A time period with the following approximated bounds: older bound -2300 Ma, younger bound -2050 Ma" ;
    skos:inScheme cs: ;
    skos:prefLabel
        "Риац"@bg ,
        "Rhyak"@cs ,
        "Rhyacien"@da ,
        "Rhyacium"@de ,
        "Rhyacian"@en ,
        "Ryaciense"@es ,
        "Rhyac"@et ,
        "Ryak"@fi ,
        "Rhyacien"@fr ,
        "rhyaci"@hu ,
        "rhyaciano"@it ,
        "リヤシアン紀"@ja ,
        "Riacis"@lt ,
        "Rhyaciën"@nl ,
        "Ryasium"@no ,
        "Riak"@pl ,
        "Riaciano"@pt ,
        "rhyacium"@sk ,
        "rhyacij"@sl ,
        "ryacium"@sv ,
        "层侵纪"@zh ;
    prov:wasDerivedFrom ts:gts2020 ;
.

isc:Roadian
    dcterms:identifier "Roadian" ;
    a skos:Concept ;
    rdfs:isDefinedBy ts:gts2020 ;
    skos:broader isc:Guadalupian ;
    skos:definition "A time period with the following approximated bounds: older bound -272.95 +|-0.11 Ma, younger bound -268.8 +|-0.5 Ma" ;
    skos:inScheme cs: ;
    skos:prefLabel
        "Роад"@bg ,
        "Road"@cs ,
        "Roadien"@da ,
        "Roadium"@de ,
        "Roadian"@en ,
        "Roadiense"@es ,
        "Roadi"@et ,
        "Road"@fi ,
        "Roadien"@fr ,
        "roadi"@hu ,
        "roadiano"@it ,
        "ローディアン期"@ja ,
        "Roadis"@lt ,
        "Roadiën"@nl ,
        "Roadium"@no ,
        "Road"@pl ,
        "Roadiano"@pt ,
        "road"@sk ,
        "roadij"@sl ,
        "road"@sv ,
        "罗德期"@zh ;
    prov:wasDerivedFrom ts:gts2020 ;
.

isc:Rupelian
    dcterms:identifier "Rupelian" ;
    a skos:Concept ;
    rdfs:isDefinedBy ts:gts2020 ;
    skos:broader isc:Oligocene ;
    skos:definition "A time period with the following approximated bounds: older bound -33.9 Ma, younger bound -28.1 Ma" ;
    skos:inScheme cs: ;
    skos:prefLabel
        "Рупел"@bg ,
        "Rupel"@cs ,
        "Rupelien"@da ,
        "Rupelium"@de ,
        "Rupelian"@en ,
        "Rupeliense"@es ,
        "Rupeli"@et ,
        "Rupel"@fi ,
        "Rupélien"@fr ,
        "rupeli"@hu ,
        "rupeliano"@it ,
        "ルペル期"@ja ,
        "Rupelis"@lt ,
        "Rupeliën"@nl ,
        "Rupel"@no ,
        "Rupel"@pl ,
        "Rupeliano"@pt ,
        "rupel"@sk ,
        "rupelij"@sl ,
        "rupel"@sv ,
        "鲁珀利期"@zh ;
    prov:wasDerivedFrom ts:gts2020 ;
.

isc:Sakmarian
    dcterms:identifier "Sakmarian" ;
    a skos:Concept ;
    rdfs:isDefinedBy ts:gts2020 ;
    skos:broader isc:Cisuralian ;
    skos:definition "A time period with the following approximated bounds: older bound -295.0 +|-0.18 Ma, younger bound -290.1 +|-0.26 Ma" ;
    skos:inScheme cs: ;
    skos:prefLabel
        "Сакмар"@bg ,
        "Sakmar"@cs ,
        "Sakmarien"@da ,
        "Sakmarium"@de ,
        "Sakmarian"@en ,
        "Sakmariense"@es ,
        "Sakmaria"@et ,
        "Sakmar"@fi ,
        "Sakmarien"@fr ,
        "szakmarai"@hu ,
        "sakmariano"@it ,
        "サクマリアン期"@ja ,
        "Sakmaris"@lt ,
        "Sakmariën"@nl ,
        "Samarkium"@no ,
        "Sakmar"@pl ,
        "Sakmariano"@pt ,
        "sakmar"@sk ,
        "sakmarij"@sl ,
        "sakmar"@sv ,
        "萨克马尔期"@zh ;
    prov:wasDerivedFrom ts:gts2020 ;
.

isc:Sandbian
    dcterms:identifier "Sandbian" ;
    a skos:Concept ;
    rdfs:isDefinedBy ts:gts2020 ;
    skos:broader isc:UpperOrdovician ;
    skos:definition "A time period with the following approximated bounds: older bound -458.4 +|-0.9 Ma, younger bound -453.0 +|-0.7 Ma" ;
    skos:inScheme cs: ;
    skos:prefLabel
        "Сандб"@bg ,
        "Sandby"@cs ,
        "Sandbien"@da ,
        "Sandbium"@de ,
        "Sandbian"@en ,
        "Sandbiense"@es ,
        "Sandbi"@et ,
        "Sandb"@fi ,
        "Sandbien"@fr ,
        "sandbi"@hu ,
        "sandbiano"@it ,
        "サンドビアン期"@ja ,
        "Sandbis"@lt ,
        "Sandbiën"@nl ,
        "Sandbyium"@no ,
        "Sandb"@pl ,
        "Sandbiano"@pt ,
        "sandb"@sk ,
        "sandbij"@sl ,
        "sandby"@sv ,
        "桑比期"@zh ;
    prov:wasDerivedFrom ts:gts2020 ;
.

isc:Santonian
    dcterms:identifier "Santonian" ;
    a skos:Concept ;
    rdfs:isDefinedBy ts:gts2020 ;
    skos:broader isc:UpperCretaceous ;
    skos:definition "A time period with the following approximated bounds: older bound -86.3 +|-0.5 Ma, younger bound -83.6 +|-0.2 Ma" ;
    skos:inScheme cs: ;
    skos:prefLabel
        "Сантон"@bg ,
        "Santon"@cs ,
        "Santonien"@da ,
        "Santonium"@de ,
        "Santonian"@en ,
        "Santoniense"@es ,
        "Santoni"@et ,
        "Santon"@fi ,
        "Santonien"@fr ,
        "santoni"@hu ,
        "santoniano"@it ,
        "サントニアン期"@ja ,
        "Santonis"@lt ,
        "Santoniën"@nl ,
        "Santonium"@no ,
        "Santon"@pl ,
        "Santoniano"@pt ,
        "santón"@sk ,
        "santonij"@sl ,
        "santon"@sv ,
        "桑托期"@zh ;
    prov:wasDerivedFrom ts:gts2020 ;
.

isc:Selandian
    dcterms:identifier "Selandian" ;
    a skos:Concept ;
    rdfs:isDefinedBy ts:gts2020 ;
    skos:broader isc:Paleocene ;
    skos:definition "A time period with the following approximated bounds: older bound -61.6 Ma, younger bound -59.2 Ma" ;
    skos:inScheme cs: ;
    skos:prefLabel
        "Селанд"@bg ,
        "Seland"@cs ,
        "Selandien"@da ,
        "Selandium"@de ,
        "Selandian"@en ,
        "Selandiense"@es ,
        "Selandi"@et ,
        "Seland"@fi ,
        "Sélandien"@fr ,
        "selandi"@hu ,
        "selandiano"@it ,
        "セランディアン期"@ja ,
        "Selandis"@lt ,
        "Selandiën"@nl ,
        "Selandium"@no ,
        "Zeland"@pl ,
        "Selandiano"@pt ,
        "seland"@sk ,
        "selandij"@sl ,
        "seland"@sv ,
        "塞兰特期"@zh ;
    prov:wasDerivedFrom ts:gts2020 ;
.

isc:Serpukhovian
    dcterms:identifier "Serpukhovian" ;
    a skos:Concept ;
    rdfs:isDefinedBy ts:gts2020 ;
    skos:broader isc:UpperMississippian ;
    skos:definition "A time period with the following approximated bounds: older bound -330.9 +|-0.2 Ma, younger bound -323.2 +|-0.4 Ma" ;
    skos:inScheme cs: ;
    skos:prefLabel
        "Серпухов"@bg ,
        "Serpukhov"@cs ,
        "Serpukhovien"@da ,
        "Serpukhovium"@de ,
        "Serpukhovian"@en ,
        "Serpulkhoviense"@es ,
        "Serpuhhovi"@et ,
        "Serpukhov"@fi ,
        "Serpukhovien"@fr ,
        "szerpuhovi"@hu ,
        "serpukhoviano"@it ,
        "サプコビアン期"@ja ,
        "Serpuchovis"@lt ,
        "Serpukhoviën"@nl ,
        "Serpukovium"@no ,
        "Serpuchow"@pl ,
        "Serpukoviano"@pt ,
        "serpuchov"@sk ,
        "serpukhovij"@sl ,
        "serpukhov"@sv ,
        "谢尔普霍夫期"@zh ;
    prov:wasDerivedFrom ts:gts2020 ;
.

isc:Serravallian
    dcterms:identifier "Serravallian" ;
    a skos:Concept ;
    rdfs:isDefinedBy ts:gts2020 ;
    skos:broader isc:Miocene ;
    skos:definition "A time period with the following approximated bounds: older bound -13.82 Ma, younger bound -11.63 Ma" ;
    skos:inScheme cs: ;
    skos:prefLabel
        "Саравал"@bg ,
        "Serraval"@cs ,
        "Serravallien"@da ,
        "Serravallium"@de ,
        "Serravallian"@en ,
        "Serravalliense"@es ,
        "Serravalli"@et ,
        "Serravall"@fi ,
        "Serravallien"@fr ,
        "serravallei"@hu ,
        "serravaliano"@it ,
        "サーラバリアン期"@ja ,
        "Seravalis"@lt ,
        "Serravalliën - Langeveld"@nl ,
        "Servallium"@no ,
        "Serrawal"@pl ,
        "Serravaliano"@pt ,
        "serravall"@sk ,
        "serravallij"@sl ,
        "serravall"@sv ,
        "塞拉瓦尔期"@zh ;
    prov:wasDerivedFrom ts:gts2020 ;
.

isc:Sheinwoodian
    dcterms:identifier "Sheinwoodian" ;
    a skos:Concept ;
    rdfs:isDefinedBy ts:gts2020 ;
    skos:broader isc:Wenlock ;
    skos:definition "A time period with the following approximated bounds: older bound -433.4 +|-0.8 Ma, younger bound -430.5 +|-0.7 Ma" ;
    skos:inScheme cs: ;
    skos:prefLabel
        "Шейнуд"@bg ,
        "Sheinwood"@cs ,
        "Sheinwoodien"@da ,
        "Sheinwoodium"@de ,
        "Sheinwoodian"@en ,
        "Sheinwoodiense"@es ,
        "Sheinwoodi"@et ,
        "Sheinwood"@fi ,
        "Sheinwoodien"@fr ,
        "sheinwoodi"@hu ,
        "sheinwoodiano"@it ,
        "シェインウッディアン期"@ja ,
        "Šeinvudis"@lt ,
        "Sheinwoodiën"@nl ,
        "Sheinwood"@no ,
        "Sheinwood"@pl ,
        "Sheinwoodiano"@pt ,
        "sheinwood"@sk ,
        "sheinwodij"@sl ,
        "sheinwood"@sv ,
        "申伍德期"@zh ;
    prov:wasDerivedFrom ts:gts2020 ;
.

isc:Siderian
    dcterms:identifier "Siderian" ;
    a skos:Concept ;
    rdfs:isDefinedBy ts:gts2020 ;
    skos:broader isc:Paleoproterozoic ;
    skos:definition "A time period with the following approximated bounds: older bound -2500 Ma, younger bound -2300 Ma" ;
    skos:inScheme cs: ;
    skos:prefLabel
        "Сидер"@bg ,
        "Sider"@cs ,
        "Siderien"@da ,
        "Siderium"@de ,
        "Siderian"@en ,
        "Sideriense"@es ,
        "Sider"@et ,
        "Sider"@fi ,
        "Sidérien"@fr ,
        "sideri"@hu ,
        "sideriano"@it ,
        "シデリアン紀"@ja ,
        "Sideris"@lt ,
        "Sideriën"@nl ,
        "Siderium"@no ,
        "Sider"@pl ,
        "Sideriano"@pt ,
        "siderium"@sk ,
        "siderij"@sl ,
        "siderium"@sv ,
        "成铁纪"@zh ;
    prov:wasDerivedFrom ts:gts2020 ;
.

isc:Sinemurian
    dcterms:identifier "Sinemurian" ;
    a skos:Concept ;
    rdfs:isDefinedBy ts:gts2020 ;
    skos:broader isc:LowerJurassic ;
    skos:definition "A time period with the following approximated bounds: older bound -199.3 +|-0.3 Ma, younger bound -190.8 +|-1.0 Ma" ;
    skos:inScheme cs: ;
    skos:prefLabel
        "Синемур"@bg ,
        "Sinemur"@cs ,
        "Sinemurien"@da ,
        "Sinémurium"@de ,
        "Sinemurian"@en ,
        "Sinemuriense"@es ,
        "Sinemuri"@et ,
        "Sinemur"@fi ,
        "Sinémurien"@fr ,
        "sinemuri"@hu ,
        "sinemuriano"@it ,
        "シネムール期"@ja ,
        "Sinemiūris"@lt ,
        "Sinemuriën"@nl ,
        "Sinemur"@no ,
        "Synemur"@pl ,
        "Sinemuriano"@pt ,
        "sinemúr"@sk ,
        "sinemurij"@sl ,
        "sinemur"@sv ,
        "辛涅穆尔期"@zh ;
    prov:wasDerivedFrom ts:gts2020 ;
.

isc:Statherian
    dcterms:identifier "Statherian" ;
    a skos:Concept ;
    rdfs:isDefinedBy ts:gts2020 ;
    skos:broader isc:Paleoproterozoic ;
    skos:definition "A time period with the following approximated bounds: older bound -1800 Ma, younger bound -1600 Ma" ;
    skos:inScheme cs: ;
    skos:prefLabel
        "Статер"@bg ,
        "Stather"@cs ,
        "Statherien"@da ,
        "Statherium"@de ,
        "Statherian"@en ,
        "Statheriense"@es ,
        "Stather"@et ,
        "Stather"@fi ,
        "Stathérien"@fr ,
        "statheri"@hu ,
        "statheriano"@it ,
        "スタテリアン紀"@ja ,
        "Stateris"@lt ,
        "Statheriën"@nl ,
        "Staterium"@no ,
        "Stater"@pl ,
        "Stateriano"@pt ,
        "staterium"@sk ,
        "statherij"@sl ,
        "staterium"@sv ,
        "固结纪"@zh ;
    prov:wasDerivedFrom ts:gts2020 ;
.

isc:Stenian
    dcterms:identifier "Stenian" ;
    a skos:Concept ;
    rdfs:isDefinedBy ts:gts2020 ;
    skos:broader isc:Mesoproterozoic ;
    skos:definition "A time period with the following approximated bounds: older bound -1200 Ma, younger bound -1000 Ma" ;
    skos:inScheme cs: ;
    skos:prefLabel
        "Стен"@bg ,
        "Sten"@cs ,
        "Stenien"@da ,
        "Stenium"@de ,
        "Stenian"@en ,
        "Esteniense"@es ,
        "Sten"@et ,
        "Sten"@fi ,
        "Sténien"@fr ,
        "steni"@hu ,
        "steniano"@it ,
        "ステニアン紀"@ja ,
        "Stenis"@lt ,
        "Steniën"@nl ,
        "Stenium"@no ,
        "Sten"@pl ,
        "Steniano"@pt ,
        "stenium"@sk ,
        "stenij"@sl ,
        "stenium"@sv ,
        "狭带纪"@zh ;
    prov:wasDerivedFrom ts:gts2020 ;
.

isc:Telychian
    dcterms:identifier "Telychian" ;
    a skos:Concept ;
    rdfs:isDefinedBy ts:gts2020 ;
    skos:broader isc:Llandovery ;
    skos:definition "A time period with the following approximated bounds: older bound -438.5 +|-1.1 Ma, younger bound -433.4 +|-0.8 Ma" ;
    skos:inScheme cs: ;
    skos:prefLabel
        "Телич"@bg ,
        "Telych"@cs ,
        "Telychien"@da ,
        "Telychium"@de ,
        "Telychian"@en ,
        "Telychiense"@es ,
        "Telychi"@et ,
        "Telych"@fi ,
        "Télychien"@fr ,
        "telychi"@hu ,
        "telychiano"@it ,
        "テリチアン期"@ja ,
        "TelyĿis"@lt ,
        "Telychiën"@nl ,
        "Telychium"@no ,
        "Telych"@pl ,
        "Telychiano"@pt ,
        "telych"@sk ,
        "telychij"@sl ,
        "telych"@sv ,
        "特列奇期"@zh ;
    prov:wasDerivedFrom ts:gts2020 ;
.

isc:Thanetian
    dcterms:identifier "Thanetian" ;
    a skos:Concept ;
    rdfs:isDefinedBy ts:gts2020 ;
    skos:broader isc:Paleocene ;
    skos:definition "A time period with the following approximated bounds: older bound -59.2 Ma, younger bound -56 Ma" ;
    skos:inScheme cs: ;
    skos:prefLabel
        "Танет"@bg ,
        "Thanet"@cs ,
        "Thanetien"@da ,
        "Thanetium"@de ,
        "Thanetian"@en ,
        "Thanetiense"@es ,
        "Thaneti"@et ,
        "Thanet"@fi ,
        "Thanétien"@fr ,
        "thaneti"@hu ,
        "thanetiano"@it ,
        "サネティアン期"@ja ,
        "Tanetis"@lt ,
        "Thanetiën"@nl ,
        "Thanetium"@no ,
        "Tanet"@pl ,
        "Tanetiano"@pt ,
        "tanet"@sk ,
        "thanetij"@sl ,
        "thanet"@sv ,
        "塔内提期"@zh ;
    prov:wasDerivedFrom ts:gts2020 ;
.

isc:Tithonian
    dcterms:identifier "Tithonian" ;
    a skos:Concept ;
    rdfs:isDefinedBy ts:gts2020 ;
    skos:broader isc:UpperJurassic ;
    skos:definition "A time period with the following approximated bounds: older bound -152.1 +|-0.9 Ma, younger bound -145.0 Ma" ;
    skos:inScheme cs: ;
    skos:prefLabel
        "Титон"@bg ,
        "Tithon"@cs ,
        "Tithonien"@da ,
        "Tithonium"@de ,
        "Tithonian"@en ,
        "Tithoniense"@es ,
        "Tithoni"@et ,
        "Tithon"@fi ,
        "Tithonien"@fr ,
        "tithon"@hu ,
        "titoniano"@it ,
        "チトニアン期"@ja ,
        "Titonis"@lt ,
        "Tithoniën"@nl ,
        "Tithonium"@no ,
        "Tyton"@pl ,
        "Titoniano"@pt ,
        "titón"@sk ,
        "tithonij"@sl ,
        "tithon"@sv ,
        "提通期"@zh ;
    prov:wasDerivedFrom ts:gts2020 ;
.

isc:Toarcian
    dcterms:identifier "Toarcian" ;
    a skos:Concept ;
    rdfs:isDefinedBy ts:gts2020 ;
    skos:broader isc:LowerJurassic ;
    skos:definition "A time period with the following approximated bounds: older bound -182.7 +|-0.7 Ma, younger bound -174.1 +|-1.0 Ma" ;
    skos:inScheme cs: ;
    skos:prefLabel
        "Тоар"@bg ,
        "Toark"@cs ,
        "Toarcien"@da ,
        "Toarcium"@de ,
        "Toarcian"@en ,
        "Toarciense"@es ,
        "Toarci"@et ,
        "Toarc"@fi ,
        "Toarcien"@fr ,
        "toarci"@hu ,
        "toarciano"@it ,
        "トアルシアン期"@ja ,
        "Toaris"@lt ,
        "Toarciën"@nl ,
        "Toarc"@no ,
        "Toark"@pl ,
        "Toarciano"@pt ,
        "toark"@sk ,
        "toarcij"@sl ,
        "toarc"@sv ,
        "托阿尔期"@zh ;
    prov:wasDerivedFrom ts:gts2020 ;
.

isc:Tonian
    dcterms:identifier "Tonian" ;
    a skos:Concept ;
    rdfs:isDefinedBy ts:gts2020 ;
    skos:broader isc:Neoproterozoic ;
    skos:definition "A time period with the following approximated bounds: older bound -1000 Ma, younger bound -720 Ma" ;
    skos:inScheme cs: ;
    skos:prefLabel
        "Тон"@bg ,
        "Ton"@cs ,
        "Tonien"@da ,
        "Tonium"@de ,
        "Tonian"@en ,
        "Toniense"@es ,
        "Ton"@et ,
        "Ton"@fi ,
        "Tonien"@fr ,
        "toni"@hu ,
        "toniano"@it ,
        "トニアン紀"@ja ,
        "Tonis"@lt ,
        "Toniën"@nl ,
        "Tonium"@no ,
        "Ton"@pl ,
        "Toniano"@pt ,
        "tonium"@sk ,
        "tonij"@sl ,
        "tonium"@sv ,
        "拉伸纪"@zh ;
    prov:wasDerivedFrom ts:gts2020 ;
.

isc:Tortonian
    dcterms:identifier "Tortonian" ;
    a skos:Concept ;
    rdfs:isDefinedBy ts:gts2020 ;
    skos:broader isc:Miocene ;
    skos:definition "A time period with the following approximated bounds: older bound -11.63 Ma, younger bound -7.246 Ma" ;
    skos:inScheme cs: ;
    skos:prefLabel
        "Тортон"@bg ,
        "Torton"@cs ,
        "Tortonien"@da ,
        "Tortonium"@de ,
        "Tortonian"@en ,
        "Tortoniense"@es ,
        "Tortoni"@et ,
        "Torton"@fi ,
        "Tortonien"@fr ,
        "tortonai"@hu ,
        "toroniano"@it ,
        "トートニアン期"@ja ,
        "Tortonis"@lt ,
        "Tortoniën - Linne"@nl ,
        "Tortonium"@no ,
        "Torton"@pl ,
        "Tortoniano"@pt ,
        "tortón"@sk ,
        "tortonij"@sl ,
        "torton"@sv ,
        "托尔顿期"@zh ;
    prov:wasDerivedFrom ts:gts2020 ;
.

isc:Tournaisian
    dcterms:identifier "Tournaisian" ;
    a skos:Concept ;
    rdfs:isDefinedBy ts:gts2020 ;
    skos:broader isc:LowerMississippian ;
    skos:definition "A time period with the following approximated bounds: older bound -358.9 +|-0.4 Ma, younger bound -346.7 +|-0.4 Ma" ;
    skos:inScheme cs: ;
    skos:prefLabel
        "Турней"@bg ,
        "Tournai"@cs ,
        "Tournaisien"@da ,
        "Tournaisium"@de ,
        "Tournaisian"@en ,
        "Tournaisiense"@es ,
        "Tournais"@et ,
        "Tournais"@fi ,
        "Tournaisien"@fr ,
        "tournaisi"@hu ,
        "tournasiano"@it ,
        "トルネージアン期"@ja ,
        "Turnėjis"@lt ,
        "Tournaisiën"@nl ,
        "Tournasium"@no ,
        "Turnej"@pl ,
        "Turnaisiano"@pt ,
        "turnén"@sk ,
        "tournaisij"@sl ,
        "tournas"@sv ,
        "杜内期"@zh ;
    prov:wasDerivedFrom ts:gts2020 ;
.

isc:Tremadocian
    dcterms:identifier "Tremadocian" ;
    a skos:Concept ;
    rdfs:isDefinedBy ts:gts2020 ;
    skos:broader isc:LowerOrdovician ;
    skos:definition "A time period with the following approximated bounds: older bound -485.4 +|-1.9 Ma, younger bound -477.7 +|-1.4 Ma" ;
    skos:inScheme cs: ;
    skos:prefLabel
        "Тремадок"@bg ,
        "Tremadok"@cs ,
        "Tremadocien"@da ,
        "Tremadocium"@de ,
        "Tremadocian"@en ,
        "Tremadociense"@es ,
        "Tremadoci"@et ,
        "Tremadoc"@fi ,
        "Trémadocien"@fr ,
        "tremadoci"@hu ,
        "tremadociano"@it ,
        "トレマドキアン期"@ja ,
        "Tremadokis"@lt ,
        "Tremadociën"@nl ,
        "Tremadoc"@no ,
        "Tremadok"@pl ,
        "Tremadociano"@pt ,
        "tremadok"@sk ,
        "tremadocij"@sl ,
        "tremadoc"@sv ,
        "特马豆克期"@zh ;
    prov:wasDerivedFrom ts:gts2020 ;
.

isc:Turonian
    dcterms:identifier "Turonian" ;
    a skos:Concept ;
    rdfs:isDefinedBy ts:gts2020 ;
    skos:broader isc:UpperCretaceous ;
    skos:definition "A time period with the following approximated bounds: older bound -93.9 Ma, younger bound -89.8 +|-0.3 Ma" ;
    skos:inScheme cs: ;
    skos:prefLabel
        "Турон"@bg ,
        "Turon"@cs ,
        "Turonien"@da ,
        "Turonium"@de ,
        "Turonian"@en ,
        "Turoniense"@es ,
        "Turoni"@et ,
        "Turon"@fi ,
        "Turonien"@fr ,
        "turon"@hu ,
        "turoniano"@it ,
        "チュロニアン期"@ja ,
        "Turonis"@lt ,
        "Tuironiën"@nl ,
        "Turonium"@no ,
        "Turon"@pl ,
        "Turoniano"@pt ,
        "turón"@sk ,
        "turonij"@sl ,
        "turon"@sv ,
        "土仑期"@zh ;
    prov:wasDerivedFrom ts:gts2020 ;
.

isc:UpperPleistocene
    dcterms:identifier "UpperPleistocene" ;
    a skos:Concept ;
    rdfs:isDefinedBy ts:gts2020 ;
    skos:broader isc:Pleistocene ;
    skos:definition "A time period with the following approximated bounds: older bound -0.126 Ma, younger bound -0.0117 Ma" ;
    skos:inScheme cs: ;
    skos:prefLabel
        "Къѿен плейѿтоцен"@bg ,
        "Pozdní pleistocén"@cs ,
        "Sen Pleistocæn"@da ,
        "Spätes Pleistozän"@de ,
        "Late Pleistocene"@en ,
        "Hiline pleistotseen"@et ,
        "Myöhäis-Pleistoseeni"@fi ,
        "késő pleisztocén"@hu ,
        "後期更新世"@ja ,
        "Apatinis Pleistocenas"@lt ,
        "Laat Pleistoceen"@nl ,
        "Yngre pleistocen"@no ,
        "Późny Plejstocen"@pl ,
        "mladší pleistocén"@sk ,
        "pozni pleistocen"@sl ,
        "yngre pleistocen"@sv ,
        "晚更新世"@zh ;
    prov:wasDerivedFrom ts:gts2020 ;
.

isc:Valanginian
    dcterms:identifier "Valanginian" ;
    a skos:Concept ;
    rdfs:isDefinedBy ts:gts2020 ;
    skos:broader isc:LowerCretaceous ;
    skos:definition "A time period with the following approximated bounds: older bound -139.8 Ma, younger bound -132.9 Ma" ;
    skos:inScheme cs: ;
    skos:prefLabel
        "Валанжин"@bg ,
        "Valangin"@cs ,
        "Valanginien"@da ,
        "Valanginium"@de ,
        "Valanginian"@en ,
        "Valanginiense"@es ,
        "Valangini"@et ,
        "Valangin"@fi ,
        "Valanginien"@fr ,
        "valangini"@hu ,
        "valanginiano"@it ,
        "バランギニアン期"@ja ,
        "Valendis"@lt ,
        "Vanlangiën"@nl ,
        "Valanginium"@no ,
        "Walanżyn"@pl ,
        "Valanginiano"@pt ,
        "valanžin"@sk ,
        "valanginij"@sl ,
        "valangin"@sv ,
        "凡兰吟期"@zh ;
    prov:wasDerivedFrom ts:gts2020 ;
.

isc:Visean
    dcterms:identifier "Visean" ;
    a skos:Concept ;
    rdfs:isDefinedBy ts:gts2020 ;
    skos:broader isc:MiddleMississippian ;
    skos:definition "A time period with the following approximated bounds: older bound -346.7 +|-0.4 Ma, younger bound -330.9 +|-0.2 Ma" ;
    skos:inScheme cs: ;
    skos:prefLabel
        "Визей"@bg ,
        "Visé"@cs ,
        "Viseen"@da ,
        "Viseum"@de ,
        "Visean"@en ,
        "Viseense"@es ,
        "Vise"@et ,
        "Vis"@fi ,
        "Viséen"@fr ,
        "viséi"@hu ,
        "viseano"@it ,
        "ビゼアン期"@ja ,
        "Vizejis"@lt ,
        "Vise-iën"@nl ,
        "Viseium"@no ,
        "Wizen"@pl ,
        "Viseano"@pt ,
        "visén"@sk ,
        "viseij"@sl ,
        "vis"@sv ,
        "韦宪期"@zh ;
    prov:wasDerivedFrom ts:gts2020 ;
.

isc:Wordian
    dcterms:identifier "Wordian" ;
    a skos:Concept ;
    rdfs:isDefinedBy ts:gts2020 ;
    skos:broader isc:Guadalupian ;
    skos:definition "A time period with the following approximated bounds: older bound -268.8 +|-0.5 Ma, younger bound -265.1 +|-0.4 Ma" ;
    skos:inScheme cs: ;
    skos:prefLabel
        "Уорд"@bg ,
        "Word"@cs ,
        "Wordien"@da ,
        "Wordium"@de ,
        "Wordian"@en ,
        "Wordiense"@es ,
        "Wordi"@et ,
        "Word"@fi ,
        "Wordien"@fr ,
        "wordi"@hu ,
        "wordiano"@it ,
        "ワーディアン期"@ja ,
        "Vordis"@lt ,
        "Wordiën"@nl ,
        "Wordium"@no ,
        "Word"@pl ,
        "Wordiano"@pt ,
        "word"@sk ,
        "wordij"@sl ,
        "word"@sv ,
        "沃德期"@zh ;
    prov:wasDerivedFrom ts:gts2020 ;
.

isc:Wuchiapingian
    dcterms:identifier "Wuchiapingian" ;
    a skos:Concept ;
    rdfs:isDefinedBy ts:gts2020 ;
    skos:broader isc:Lopingian ;
    skos:definition "A time period with the following approximated bounds: older bound -259.1 +|-0.5 Ma, younger bound -254.14 +|-0.07 Ma" ;
    skos:inScheme cs: ;
    skos:prefLabel
        "Вучиапинг"@bg ,
        "Wuchiaping"@cs ,
        "Wuchiapingien"@da ,
        "Wuchiapingium"@de ,
        "Wuchiapingian"@en ,
        "Wuchiapingiense"@es ,
        "Wuchiapingi"@et ,
        "Wuchiaiping"@fi ,
        "Wuchiapingien"@fr ,
        "wuchiapingi"@hu ,
        "wuchiapingiano"@it ,
        "ウキアピンギアン期"@ja ,
        "VuĿiapingis"@lt ,
        "Wuchiapingiën"@nl ,
        "Wuchianpingum"@no ,
        "Wuchiaping"@pl ,
        "Wuchiapingiano"@pt ,
        "wuťiapching"@sk ,
        "wuchiapingij"@sl ,
        "wuchiaping"@sv ,
        "吴家坪期"@zh ;
    prov:wasDerivedFrom ts:gts2020 ;
.

isc:Wuliuan
    dcterms:identifier "Wuliuan" ;
    a skos:Concept ;
    rdfs:isDefinedBy ts:gts2020 ;
    skos:broader isc:Miaolingian ;
    skos:definition "A time period with the following approximated bounds: older bound -509 Ma, younger bound -504.5 Ma" ;
    skos:inScheme cs: ;
    skos:prefLabel "Wuliuan"@en ;
    prov:wasDerivedFrom ts:gts2020 ;
.

isc:Ypresian
    dcterms:identifier "Ypresian" ;
    a skos:Concept ;
    rdfs:isDefinedBy ts:gts2020 ;
    skos:broader isc:Eocene ;
    skos:definition "A time period with the following approximated bounds: older bound -56 Ma, younger bound -47.8 Ma" ;
    skos:inScheme cs: ;
    skos:prefLabel
        "Ипреѿ"@bg ,
        "Ypres"@cs ,
        "Ypresien"@da ,
        "Ypersium"@de ,
        "Ypresian"@en ,
        "Ypresiense"@es ,
        "Ypresi"@et ,
        "Ypres"@fi ,
        "Yprésien"@fr ,
        "ypresi"@hu ,
        "ypresiano"@it ,
        "イプレシアン期"@ja ,
        "Ypris"@lt ,
        "Ypresiën"@nl ,
        "Ypres"@no ,
        "Ipr"@pl ,
        "Ipresiano"@pt ,
        "ypres"@sk ,
        "ypresij"@sl ,
        "ypres"@sv ,
        "伊普雷斯期"@zh ;
    prov:wasDerivedFrom ts:gts2020 ;
.

isc:Zanclean
    dcterms:identifier "Zanclean" ;
    a skos:Concept ;
    rdfs:isDefinedBy ts:gts2020 ;
    skos:broader isc:Pliocene ;
    skos:definition "A time period with the following approximated bounds: older bound -5.333 Ma, younger bound -3.6 Ma" ;
    skos:inScheme cs: ;
    skos:prefLabel
        "Занклѿки"@bg ,
        "Zancl"@cs ,
        "Zanclien"@da ,
        "Zanclium"@de ,
        "Zanclean"@en ,
        "Zanclayense"@es ,
        "Zancle"@et ,
        "Zancl"@fi ,
        "Zancléen"@fr ,
        "zanclai"@hu ,
        "zancleano"@it ,
        "ザンクレアン期"@ja ,
        "Zanklis"@lt ,
        "Brunssummiën"@nl ,
        "Zancleium"@no ,
        "Zankl"@pl ,
        "Zancleano"@pt ,
        "zanclean"@sk ,
        "zanclij"@sl ,
        "zancl"@sv ,
        "赞克勒期"@zh ;
    prov:wasDerivedFrom ts:gts2020 ;
.

isc:LowerMississippian
    dcterms:identifier "LowerMississippian" ;
    a skos:Concept ;
    rdfs:isDefinedBy ts:gts2020 ;
    skos:broader isc:Mississippian ;
    skos:definition "A time period with the following approximated bounds: older bound -358.9 +|-0.4 Ma, younger bound -346.7 +|-0.4 Ma" ;
    skos:inScheme cs: ;
    skos:narrower isc:Tournaisian ;
    skos:prefLabel
        "Early Mississippian"@en ,
        "前期ミシシッピアン紀"@ja ,
        "早密西西比世"@zh ;
    prov:wasDerivedFrom ts:gts2020 ;
.

isc:LowerPennsylvanian
    dcterms:identifier "LowerPennsylvanian" ;
    a skos:Concept ;
    rdfs:isDefinedBy ts:gts2020 ;
    skos:broader isc:Pennsylvanian ;
    skos:definition "A time period with the following approximated bounds: older bound -323.2 +|-0.4 Ma, younger bound -315.2 +|-0.2 Ma" ;
    skos:inScheme cs: ;
    skos:narrower isc:Bashkirian ;
    skos:prefLabel
        "Early Pennsylvanian"@en ,
        "前期ペンシルバニア紀"@ja ,
        "早宾夕法尼亚世"@zh ;
    prov:wasDerivedFrom ts:gts2020 ;
.

isc:MiddleMississippian
    dcterms:identifier "MiddleMississippian" ;
    a skos:Concept ;
    rdfs:isDefinedBy ts:gts2020 ;
    skos:broader isc:Mississippian ;
    skos:definition "A time period with the following approximated bounds: older bound -346.7 +|-0.4 Ma, younger bound -330.9 +|-0.2 Ma" ;
    skos:inScheme cs: ;
    skos:narrower isc:Visean ;
    skos:prefLabel
        "Middle Mississippian"@en ,
        "中期ミシシッピアン紀"@ja ,
        "中密西西比世"@zh ;
    prov:wasDerivedFrom ts:gts2020 ;
.

isc:MiddlePennsylvanian
    dcterms:identifier "MiddlePennsylvanian" ;
    a skos:Concept ;
    rdfs:isDefinedBy ts:gts2020 ;
    skos:broader isc:Pennsylvanian ;
    skos:definition "A time period with the following approximated bounds: older bound -315.2 +|-0.2 Ma, younger bound -307 +|-0.1 Ma" ;
    skos:inScheme cs: ;
    skos:narrower isc:Moscovian ;
    skos:prefLabel
        "Middle Pennsylvanian"@en ,
        "中期ペンシルバニア紀"@ja ,
        "中宾夕法尼亚世"@zh ;
    prov:wasDerivedFrom ts:gts2020 ;
.

isc:UpperMississippian
    dcterms:identifier "UpperMississippian" ;
    a skos:Concept ;
    rdfs:isDefinedBy ts:gts2020 ;
    skos:broader isc:Mississippian ;
    skos:definition "A time period with the following approximated bounds: older bound -330.9 +|-0.2 Ma, younger bound -298.9 +|-0.15 Ma" ;
    skos:inScheme cs: ;
    skos:narrower isc:Serpukhovian ;
    skos:prefLabel
        "Late Mississippian"@en ,
        "後期ミシシッピアン紀"@ja ,
        "晚密西西比世"@zh ;
    prov:wasDerivedFrom ts:gts2020 ;
.

isc:CambrianSeries2
    dcterms:identifier "CambrianSeries2" ;
    a skos:Concept ;
    rdfs:isDefinedBy ts:gts2020 ;
    skos:broader isc:Cambrian ;
    skos:definition "A time period with the following approximated bounds: older bound -521 Ma, younger bound -509 Ma" ;
    skos:inScheme cs: ;
    skos:narrower
        isc:CambrianStage3 ,
        isc:CambrianStage4 ;
    skos:prefLabel
        "Камбрий - 2 ѿериѿ"@bg ,
        "Kambrium-Oddělení 2"@cs ,
        "Kambrium-Serie 2"@da ,
        "Kambrium-Serie 2"@de ,
        "Cambrian Series 2"@en ,
        "Cámbrico-Serie 2"@es ,
        "Kambrium, Ladestik 2"@et ,
        "Kambri-sarja 2"@fi ,
        "Cambrien-Séries 2"@fr ,
        "kambrium 2. sorozat"@hu ,
        "cambriano - serie 2"@it ,
        "第2世"@ja ,
        "Kambras-Serija 2"@lt ,
        "Cambrium, Zone 2"@nl ,
        "Kambrium -serie 2"@no ,
        "Kambr-Oddział 2"@pl ,
        "Câmbrico-Série 2"@pt ,
        "kambrium - séria 2"@sk ,
        "kambrij-serija 2"@sl ,
        "kambrium serie 2"@sv ,
        "第二世"@zh ;
    prov:wasDerivedFrom ts:gts2020 ;
.

isc:Carboniferous
    dcterms:identifier "Carboniferous" ;
    a skos:Concept ;
    rdfs:isDefinedBy ts:gts2020 ;
    skos:broader isc:Paleozoic ;
    skos:definition "A time period with the following approximated bounds: older bound -358.9 +|-0.4 Ma, younger bound -298.9 +|-0.15 Ma" ;
    skos:inScheme cs: ;
    skos:narrower
        isc:Mississippian ,
        isc:Pennsylvanian ;
    skos:prefLabel
        "Карбон"@bg ,
        "Karbon"@cs ,
        "Karbon"@da ,
        "Karbon"@de ,
        "Carboniferous"@en ,
        "Carbonífero"@es ,
        "Karbon"@et ,
        "Kivihiili"@fi ,
        "Carbonifère"@fr ,
        "karbon"@hu ,
        "carbonifero"@it ,
        "石炭紀"@ja ,
        "Karbonas"@lt ,
        "Carboon"@nl ,
        "Karbon"@no ,
        "Karbon"@pl ,
        "Carbónico"@pt ,
        "karbón"@sk ,
        "karbon"@sl ,
        "karbon"@sv ,
        "石炭纪"@zh ;
    prov:wasDerivedFrom ts:gts2020 ;
.

isc:Cretaceous
    dcterms:identifier "Cretaceous" ;
    a skos:Concept ;
    rdfs:isDefinedBy ts:gts2020 ;
    skos:broader isc:Mesozoic ;
    skos:definition "A time period with the following approximated bounds: older bound -145.0 Ma, younger bound -66.0 Ma" ;
    skos:inScheme cs: ;
    skos:narrower
        isc:LowerCretaceous ,
        isc:UpperCretaceous ;
    skos:prefLabel
        "Креда"@bg ,
        "Křída"@cs ,
        "Kridt"@da ,
        "Kreide"@de ,
        "Cretaceous"@en ,
        "Cretácico"@es ,
        "Kriit"@et ,
        "Liitu"@fi ,
        "Crétacé"@fr ,
        "kréta"@hu ,
        "cretacico"@it ,
        "白亜紀"@ja ,
        "Kreida"@lt ,
        "Krijt"@nl ,
        "Kritt"@no ,
        "Kreda"@pl ,
        "Cretácico"@pt ,
        "krieda"@sk ,
        "kreda"@sl ,
        "krita"@sv ,
        "白垩纪"@zh ;
    prov:wasDerivedFrom ts:gts2020 ;
.

isc:Lopingian
    dcterms:identifier "Lopingian" ;
    a skos:Concept ;
    rdfs:isDefinedBy ts:gts2020 ;
    skos:broader isc:Permian ;
    skos:definition "A time period with the following approximated bounds: older bound -259.1 +|-0.5 Ma, younger bound -251.902 +|-0.024 Ma" ;
    skos:inScheme cs: ;
    skos:narrower
        isc:Changhsingian ,
        isc:Wuchiapingian ;
    skos:prefLabel
        "Лопинг"@bg ,
        "Loping"@cs ,
        "Lopingien"@da ,
        "Lopingium"@de ,
        "Lopingian"@en ,
        "Lopingiense"@es ,
        "Loping"@et ,
        "Loping"@fi ,
        "Lopingien"@fr ,
        "lopingi"@hu ,
        "lopingiano"@it ,
        "ロピンギアン世"@ja ,
        "Lopingis"@lt ,
        "Lopingiën"@nl ,
        "Lopingium"@no ,
        "Loping"@pl ,
        "Lopingiano"@pt ,
        "loping"@sk ,
        "lopingij"@sl ,
        "loping"@sv ,
        "乐平世"@zh ;
    prov:wasDerivedFrom ts:gts2020 ;
.

isc:LowerOrdovician
    dcterms:identifier "LowerOrdovician" ;
    a skos:Concept ;
    rdfs:isDefinedBy ts:gts2020 ;
    skos:broader isc:Ordovician ;
    skos:definition "A time period with the following approximated bounds: older bound -485.4 +|-1.9 Ma, younger bound -470.0 +|-1.4 Ma" ;
    skos:inScheme cs: ;
    skos:narrower
        isc:Floian ,
        isc:Tremadocian ;
    skos:prefLabel
        "Ранен Ордовик"@bg ,
        "brzy ordovik"@cs ,
        "Tidlig Ordovicium"@da ,
        "Fühes Ordovizium"@de ,
        "Early Ordovician"@en ,
        "Ordovícico temprano"@es ,
        "Vara-Ordoviitsium"@et ,
        "Varhais-Ordoviikki"@fi ,
        "Ordovicien précoce"@fr ,
        "kora-ordovícium"@hu ,
        "ordoviciano precoce"@it ,
        "オルドビス紀前期"@ja ,
        "Ankstyvasis Ordovikas"@lt ,
        "Vroeg Ordovicium"@nl ,
        "Tidlig ordovicium"@no ,
        "Wczesny Ordowik"@pl ,
        "Ordovícista adiantado"@pt ,
        "raný ordovik"@sk ,
        "zgodnji ordovicij"@sl ,
        "äldre ordovicium"@sv ,
        "早奥陶世"@zh ;
    prov:wasDerivedFrom ts:gts2020 ;
.

isc:LowerTriassic
    dcterms:identifier "LowerTriassic" ;
    a skos:Concept ;
    rdfs:isDefinedBy ts:gts2020 ;
    skos:broader isc:Triassic ;
    skos:definition "A time period with the following approximated bounds: older bound -251.902 +|-0.024 Ma, younger bound -247.2 Ma" ;
    skos:inScheme cs: ;
    skos:narrower
        isc:Induan ,
        isc:Olenekian ;
    skos:prefLabel
        "Раннен Триаѿ"@bg ,
        "brzy trias"@cs ,
        "Tidlig Triassisk"@da ,
        "Frühe Trias (Buntsandstein)"@de ,
        "Early Triassic"@en ,
        "Triásico temprano"@es ,
        "Vara-Triias"@et ,
        "Varhais-Trias"@fi ,
        "Trias précoce"@fr ,
        "kora-triász"@hu ,
        "triassico precoce"@it ,
        "三畳紀前期"@ja ,
        "Ankstyvasis Triasas"@lt ,
        "Vroeg Trias"@nl ,
        "Tidlig trias"@no ,
        "Wczesny Trias"@pl ,
        "Triássico primitivo"@pt ,
        "raný trias"@sk ,
        "zgodnji trias"@sl ,
        "äldre trias"@sv ,
        "早三叠世"@zh ;
    prov:wasDerivedFrom ts:gts2020 ;
.

isc:Ludlow
    dcterms:identifier "Ludlow" ;
    a skos:Concept ;
    rdfs:isDefinedBy ts:gts2020 ;
    skos:broader isc:Silurian ;
    skos:definition "A time period with the following approximated bounds: older bound -427.4 +|-0.5 Ma, younger bound -423 +|-2.3 Ma" ;
    skos:inScheme cs: ;
    skos:narrower
        isc:Gorstian ,
        isc:Ludfordian ;
    skos:prefLabel
        "Лудлоу"@bg ,
        "Ludlow"@cs ,
        "Ludlow"@da ,
        "Ludlow"@de ,
        "Ludlow"@en ,
        "Ludlow"@es ,
        "Ludlow"@et ,
        "Ludlow"@fi ,
        "Ludlow"@fr ,
        "ludlowi"@hu ,
        "ludlow"@it ,
        "ルーロビアン世"@ja ,
        "Ludlovis"@lt ,
        "Ludlow"@nl ,
        "Ludlow"@no ,
        "Ludlow"@pl ,
        "Ludlow"@pt ,
        "ludlow"@sk ,
        "ludlowij"@sl ,
        "ludlow"@sv ,
        "卢德洛世"@zh ;
    prov:wasDerivedFrom ts:gts2020 ;
.

isc:MiddleDevonian
    dcterms:identifier "MiddleDevonian" ;
    a skos:Concept ;
    rdfs:isDefinedBy ts:gts2020 ;
    skos:broader isc:Devonian ;
    skos:definition "A time period with the following approximated bounds: older bound -393.3 +|-1.2 Ma, younger bound -382.7 +|-1.6 Ma" ;
    skos:inScheme cs: ;
    skos:narrower
        isc:Eifelian ,
        isc:Givetian ;
    skos:prefLabel
        "Среден Девон"@bg ,
        "Střední devon"@cs ,
        "Mellem Devon"@da ,
        "Mitteldevon"@de ,
        "Middle Devonian"@en ,
        "Devónico Medio"@es ,
        "Kesk-Devon"@et ,
        "Keski-Devoni"@fi ,
        "Dévonien moyen"@fr ,
        "középső-devon"@hu ,
        "devoniano medio"@it ,
        "中期デボン紀"@ja ,
        "Vidurinis Devonas"@lt ,
        "Midden Devoon"@nl ,
        "Midtre devon"@no ,
        "Środkowy Dewon"@pl ,
        "Devónico Médio"@pt ,
        "stredný devón"@sk ,
        "srednji devon"@sl ,
        "mellersta devon"@sv ,
        "中泥盆世"@zh ;
    prov:wasDerivedFrom ts:gts2020 ;
.

isc:MiddleOrdovician
    dcterms:identifier "MiddleOrdovician" ;
    a skos:Concept ;
    rdfs:isDefinedBy ts:gts2020 ;
    skos:broader isc:Ordovician ;
    skos:definition "A time period with the following approximated bounds: older bound -470.0 +|-1.4 Ma, younger bound -458.4 +|-0.9 Ma" ;
    skos:inScheme cs: ;
    skos:narrower
        isc:Dapingian ,
        isc:Darriwilian ;
    skos:prefLabel
        "Среден Ордовик"@bg ,
        "Střední ordovik"@cs ,
        "Mellem Ordovicium"@da ,
        "Mittleres Ordovizium"@de ,
        "Middle Ordovician"@en ,
        "Ordovícico Medio"@es ,
        "Kesk-Ordoviitsium"@et ,
        "Keski-Ordoviikki"@fi ,
        "Ordovicien moyen"@fr ,
        "középső-ordovícium"@hu ,
        "ordoviciano medio"@it ,
        "中期オルドビス紀"@ja ,
        "Vidurinis Ordovikas"@lt ,
        "Midden Ordovicium"@nl ,
        "Midtre ordovicium"@no ,
        "Środkowy Ordowik"@pl ,
        "Ordovícico Médio"@pt ,
        "stredný ordovik"@sk ,
        "srednji ordovicij"@sl ,
        "mellersta ordovicium"@sv ,
        "中奥陶世"@zh ;
    prov:wasDerivedFrom ts:gts2020 ;
.

isc:MiddleTriassic
    dcterms:identifier "MiddleTriassic" ;
    a skos:Concept ;
    rdfs:isDefinedBy ts:gts2020 ;
    skos:broader isc:Triassic ;
    skos:definition "A time period with the following approximated bounds: older bound -247.2 Ma, younger bound -237 Ma" ;
    skos:inScheme cs: ;
    skos:narrower
        isc:Anisian ,
        isc:Ladinian ;
    skos:prefLabel
        "Среден Триаѿ"@bg ,
        "Střední trias"@cs ,
        "Mellem Triassisk"@da ,
        "Mittlere Trias"@de ,
        "Middle Triassic"@en ,
        "Triásico Medio"@es ,
        "Kesk-Triias"@et ,
        "Keski-Trias"@fi ,
        "Trias moyen"@fr ,
        "középső-triász"@hu ,
        "triassico medio"@it ,
        "中期三畳紀"@ja ,
        "Vidurinis Triasas"@lt ,
        "Midden Trias"@nl ,
        "Midtre trias"@no ,
        "Środkowy Trias"@pl ,
        "Triásico Médio"@pt ,
        "stredný trias"@sk ,
        "srednji trias"@sl ,
        "mellersta trias"@sv ,
        "中三叠世"@zh ;
    prov:wasDerivedFrom ts:gts2020 ;
.

isc:Neogene
    dcterms:identifier "Neogene" ;
    a skos:Concept ;
    rdfs:isDefinedBy ts:gts2020 ;
    skos:broader isc:Cenozoic ;
    skos:definition "A time period with the following approximated bounds: older bound -23.03 Ma, younger bound -2.58 Ma" ;
    skos:inScheme cs: ;
    skos:narrower
        isc:Miocene ,
        isc:Pliocene ;
    skos:prefLabel
        "пеоген"@bg ,
        "Neogén"@cs ,
        "Neogen"@da ,
        "Neogen"@de ,
        "Neogene"@en ,
        "Neógeno"@es ,
        "Neogeen"@et ,
        "Neogeeni"@fi ,
        "Néogène"@fr ,
        "neogén"@hu ,
        "neogene"@it ,
        "新第三紀"@ja ,
        "Neogenas"@lt ,
        "Neogeen"@nl ,
        "Neogen"@no ,
        "Neogen"@pl ,
        "Neogénico"@pt ,
        "neogén"@sk ,
        "neogen"@sl ,
        "neogen"@sv ,
        "晚第三纪"@zh ;
    prov:wasDerivedFrom ts:gts2020 ;
.

isc:Oligocene
    dcterms:identifier "Oligocene" ;
    a skos:Concept ;
    rdfs:isDefinedBy ts:gts2020 ;
    skos:broader isc:Paleogene ;
    skos:definition "A time period with the following approximated bounds: older bound -33.9 Ma, younger bound -23.03 Ma" ;
    skos:inScheme cs: ;
    skos:narrower
        isc:Chattian ,
        isc:Rupelian ;
    skos:prefLabel
        "Олигоцен"@bg ,
        "Oligocén"@cs ,
        "Oligocæn"@da ,
        "Oligozän"@de ,
        "Oligocene"@en ,
        "Oligoceno"@es ,
        "Oligotseen"@et ,
        "Oligoseeni"@fi ,
        "Oligocène"@fr ,
        "oligocén"@hu ,
        "oligocene"@it ,
        "漸新世"@ja ,
        "Oligocenas"@lt ,
        "Oliogoceen"@nl ,
        "Oligocen"@no ,
        "Oligocen"@pl ,
        "Oligocénico"@pt ,
        "oligocén"@sk ,
        "oligocen"@sl ,
        "oligocen"@sv ,
        "渐新世"@zh ;
    prov:wasDerivedFrom ts:gts2020 ;
.

isc:Pliocene
    dcterms:identifier "Pliocene" ;
    a skos:Concept ;
    rdfs:isDefinedBy ts:gts2020 ;
    skos:broader isc:Neogene ;
    skos:definition "A time period with the following approximated bounds: older bound -5.333 Ma, younger bound -2.58 Ma" ;
    skos:inScheme cs: ;
    skos:narrower
        isc:Piacenzian ,
        isc:Zanclean ;
    skos:prefLabel
        "Плиоцен"@bg ,
        "Pliocén"@cs ,
        "Pliocæn"@da ,
        "Pliozän"@de ,
        "Pliocene"@en ,
        "Ploceno"@es ,
        "Pliotseen"@et ,
        "Plioseeni"@fi ,
        "Pliocène"@fr ,
        "pliocén"@hu ,
        "pliocene"@it ,
        "鮮新世"@ja ,
        "Pliocenas"@lt ,
        "Plioceen"@nl ,
        "Pliocen"@no ,
        "Pliocen"@pl ,
        "Pliocénico"@pt ,
        "pliocén"@sk ,
        "pliocen"@sl ,
        "pliocen"@sv ,
        "上新世"@zh ;
    prov:wasDerivedFrom ts:gts2020 ;
.

isc:Quaternary
    dcterms:identifier "Quaternary" ;
    a skos:Concept ;
    rdfs:isDefinedBy ts:gts2020 ;
    skos:broader isc:Cenozoic ;
    skos:definition "A time period with the following approximated bounds: older bound -2.58 Ma, younger bound -0.0 Ma" ;
    skos:inScheme cs: ;
    skos:narrower
        isc:Holocene ,
        isc:Pleistocene ;
    skos:prefLabel
        "Кватернер"@bg ,
        "Kvartér"@cs ,
        "Kvartær"@da ,
        "Quartär"@de ,
        "Quaternary"@en ,
        "Cuaternario"@es ,
        "Kvaternaar"@et ,
        "Kvartääri"@fi ,
        "Quaternaire"@fr ,
        "negyedidőszak"@hu ,
        "quaternario"@it ,
        "第四紀"@ja ,
        "Kvarteras"@lt ,
        "Kwartair"@nl ,
        "Kvartær"@no ,
        "Czwartorzęd"@pl ,
        "Quaternário"@pt ,
        "kvartér"@sk ,
        "kvartar"@sl ,
        "kvartär"@sv ,
        "第四纪"@zh ;
    prov:wasDerivedFrom ts:gts2020 ;
.

isc:Terreneuvian
    dcterms:identifier "Terreneuvian" ;
    a skos:Concept ;
    rdfs:isDefinedBy ts:gts2020 ;
    skos:broader isc:Cambrian ;
    skos:definition "A time period with the following approximated bounds: older bound -541.0 +|-1.0 Ma, younger bound -521 Ma" ;
    skos:inScheme cs: ;
    skos:narrower
        isc:CambrianStage2 ,
        isc:Fortunian ;
    skos:prefLabel
        "Теренеув"@bg ,
        "Terreneuv"@cs ,
        "Terreneuvien"@da ,
        "Terreneuvium"@de ,
        "Terreneuvian"@en ,
        "Terreneuviense"@es ,
        "Terreneuvi"@et ,
        "Terreneuv"@fi ,
        "Terreneuvien"@fr ,
        "terreneuvi"@hu ,
        "terreneuviano"@it ,
        "テレニュービアン世"@ja ,
        "Tereniuvis"@lt ,
        "Terreneuviën"@nl ,
        "Terreneuvium"@no ,
        "Terenew"@pl ,
        "Terreneuviano"@pt ,
        "terreneuv"@sk ,
        "terreneuvij"@sl ,
        "terreneuv"@sv ,
        "纽芬兰世"@zh ;
    prov:wasDerivedFrom ts:gts2020 ;
.

isc:UpperDevonian
    dcterms:identifier "UpperDevonian" ;
    a skos:Concept ;
    rdfs:isDefinedBy ts:gts2020 ;
    skos:broader isc:Devonian ;
    skos:definition "A time period with the following approximated bounds: older bound -382.7 +|-1.6 Ma, younger bound -358.9 +|-0.4 Ma" ;
    skos:inScheme cs: ;
    skos:narrower
        isc:Famennian ,
        isc:Frasnian ;
    skos:prefLabel
        "Къѿен Девон"@bg ,
        "Svrchní devon"@cs ,
        "Sen Devon"@da ,
        "Spätes Devon"@de ,
        "Late Devonian"@en ,
        "Hilis-Devon"@et ,
        "Myöhäis-Devoni"@fi ,
        "késő-devon"@hu ,
        "後期デボン紀"@ja ,
        "Vėlyvasis Devonas"@lt ,
        "Laat Devoon"@nl ,
        "Sen devon"@no ,
        "Późny Dewon"@pl ,
        "mladší devón"@sk ,
        "pozni devon"@sl ,
        "yngre devon"@sv ,
        "晚泥盆世"@zh ;
    prov:wasDerivedFrom ts:gts2020 ;
.

isc:UpperPennsylvanian
    dcterms:identifier "UpperPennsylvanian" ;
    a skos:Concept ;
    rdfs:isDefinedBy ts:gts2020 ;
    skos:broader isc:Pennsylvanian ;
    skos:definition "A time period with the following approximated bounds: older bound -307 +|-0.1 Ma, younger bound -298.9 +|-0.15 Ma" ;
    skos:inScheme cs: ;
    skos:narrower
        isc:Gzhelian ,
        isc:Kasimovian ;
    skos:prefLabel
        "Къѿен Пенѿилван"@bg ,
        "Pozdní pennsylván"@cs ,
        "Sen Pennsylvanien"@da ,
        "Spätes Pennsylvanium"@de ,
        "Late Pennsylvanian"@en ,
        "Hilis-Pennsylvania"@et ,
        "Myöhäis-Pennsylvania"@fi ,
        "késő-pennsylvaniai"@hu ,
        "後期ペンシルバニア紀"@ja ,
        "Vėlyvasis Pensilvanis"@lt ,
        "Laat Pennsylvaniën"@nl ,
        "Sen pennsylvanium"@no ,
        "Późny Pensylwan"@pl ,
        "mladší penssylván"@sk ,
        "pozni pennsylvanij"@sl ,
        "yngre pennsylvan"@sv ,
        "晚宾夕法尼亚世"@zh ;
    prov:wasDerivedFrom ts:gts2020 ;
.

isc:Wenlock
    dcterms:identifier "Wenlock" ;
    a skos:Concept ;
    rdfs:isDefinedBy ts:gts2020 ;
    skos:broader isc:Silurian ;
    skos:definition "A time period with the following approximated bounds: older bound -433.4 +|-0.8 Ma, younger bound -427.4 +|-0.5 Ma" ;
    skos:inScheme cs: ;
    skos:narrower
        isc:Homerian ,
        isc:Sheinwoodian ;
    skos:prefLabel
        "Венлок"@bg ,
        "Wenlock"@cs ,
        "Wenlock"@da ,
        "Wenlock"@de ,
        "Wenlock"@en ,
        "Wenlock"@es ,
        "Wenlock"@et ,
        "Wenlock"@fi ,
        "Wenlock"@fr ,
        "wenlocki"@hu ,
        "wenlockiano"@it ,
        "ウェンロッキアン世"@ja ,
        "Uenlokis"@lt ,
        "Wenlock"@nl ,
        "Welnlock"@no ,
        "Wenlok"@pl ,
        "Wenlock"@pt ,
        "wenlock"@sk ,
        "wenlockij"@sl ,
        "wenlock"@sv ,
        "温洛克世"@zh ;
    prov:wasDerivedFrom ts:gts2020 ;
.

isc:Cenozoic
    dcterms:identifier "Cenozoic" ;
    a skos:Concept ;
    rdfs:isDefinedBy ts:gts2020 ;
    skos:broader isc:Phanerozoic ;
    skos:definition "A time period with the following approximated bounds: older bound -66.0 Ma, younger bound -0.0 Ma" ;
    skos:inScheme cs: ;
    skos:narrower
        isc:Neogene ,
        isc:Paleogene ,
        isc:Quaternary ;
    skos:prefLabel
        "пеозой"@bg ,
        "Kenozoikum"@cs ,
        "Kænozoisk"@da ,
        "Känozoikum"@de ,
        "Cenozoic"@en ,
        "Cainozoic"@en-gb ,
        "Cenozoic"@en-us ,
        "Cenozoico"@es ,
        "Kainosoikum"@et ,
        "Kenotsoikum"@fi ,
        "Cénozoïque"@fr ,
        "kainozoikum"@hu ,
        "cenozoico"@it ,
        "新生代"@ja ,
        "Cenozojus"@lt ,
        "Kaenozoïcum"@nl ,
        "Kenozoikum"@no ,
        "Kenozoik"@pl ,
        "Cenozóico"@pt ,
        "kenozoikum"@sk ,
        "kenozoik"@sl ,
        "kenozoikum"@sv ,
        "新生代"@zh ;
    prov:wasDerivedFrom ts:gts2020 ;
.

isc:Devonian
    dcterms:identifier "Devonian" ;
    a skos:Concept ;
    rdfs:isDefinedBy ts:gts2020 ;
    skos:broader isc:Paleozoic ;
    skos:definition "A time period with the following approximated bounds: older bound -419.2 +|-3.2 Ma, younger bound -358.9 +|-0.4 Ma" ;
    skos:inScheme cs: ;
    skos:narrower
        isc:LowerDevonian ,
        isc:MiddleDevonian ,
        isc:UpperDevonian ;
    skos:prefLabel
        "Девон"@bg ,
        "Devon"@cs ,
        "Devon"@da ,
        "Devon"@de ,
        "Devonian"@en ,
        "Devónico"@es ,
        "Devon"@et ,
        "Devoni"@fi ,
        "Dévonien"@fr ,
        "devon"@hu ,
        "devoniano"@it ,
        "デボン紀"@ja ,
        "Devonas"@lt ,
        "Devoon"@nl ,
        "Devon"@no ,
        "Dewon"@pl ,
        "Devónico"@pt ,
        "devón"@sk ,
        "devon"@sl ,
        "devon"@sv ,
        "泥盆纪"@zh ;
    prov:wasDerivedFrom ts:gts2020 ;
.

isc:Furongian
    dcterms:identifier "Furongian" ;
    a skos:Concept ;
    rdfs:isDefinedBy ts:gts2020 ;
    skos:broader isc:Cambrian ;
    skos:definition "A time period with the following approximated bounds: older bound -497 Ma, younger bound -485.4 +|-1.9 Ma" ;
    skos:inScheme cs: ;
    skos:narrower
        isc:CambrianStage10 ,
        isc:Jiangshanian ,
        isc:Paibian ;
    skos:prefLabel
        "Фуронг"@bg ,
        "Furong"@cs ,
        "Furongien"@da ,
        "Furongium"@de ,
        "Furongian"@en ,
        "Furogiense"@es ,
        "Furong"@et ,
        "Furong"@fi ,
        "Furongien"@fr ,
        "furongi"@hu ,
        "furongiano"@it ,
        "フロンギアン世"@ja ,
        "Furongis"@lt ,
        "Furongiën"@nl ,
        "Furongium"@no ,
        "Furong"@pl ,
        "Furongiano"@pt ,
        "furong"@sk ,
        "furongij"@sl ,
        "furong"@sv ,
        "芙蓉世"@zh ;
    prov:wasDerivedFrom ts:gts2020 ;
.

isc:Guadalupian
    dcterms:identifier "Guadalupian" ;
    a skos:Concept ;
    rdfs:isDefinedBy ts:gts2020 ;
    skos:broader isc:Permian ;
    skos:definition "A time period with the following approximated bounds: older bound -272.95 +|-0.11 Ma, younger bound -259.1 +|-0.5 Ma" ;
    skos:inScheme cs: ;
    skos:narrower
        isc:Capitanian ,
        isc:Roadian ,
        isc:Wordian ;
    skos:prefLabel
        "Гуадалуп"@bg ,
        "Guadalup"@cs ,
        "Guadalupien"@da ,
        "Guadalupium"@de ,
        "Guadalupian"@en ,
        "Guadalupiense"@es ,
        "Guadalup"@et ,
        "Guadalup"@fi ,
        "Guadalupéen"@fr ,
        "guadalupei"@hu ,
        "guadalupiano"@it ,
        "ガダリューピアン世"@ja ,
        "Gvadalupis"@lt ,
        "Guadalupiën"@nl ,
        "Guadalupium"@no ,
        "Gwadelup"@pl ,
        "Guadalupiano"@pt ,
        "guadalup"@sk ,
        "guadalupij"@sl ,
        "guadalup"@sv ,
        "瓜德鲁普世"@zh ;
    prov:wasDerivedFrom ts:gts2020 ;
.

isc:Holocene
    dcterms:identifier "Holocene" ;
    a skos:Concept ;
    rdfs:isDefinedBy ts:gts2020 ;
    skos:broader isc:Quaternary ;
    skos:definition "A time period with the following approximated bounds: older bound -0.0117 Ma, younger bound -0.0 Ma" ;
    skos:inScheme cs: ;
    skos:narrower
        isc:Greenlandian ,
        isc:Meghalayan ,
        isc:Northgrippian ;
    skos:prefLabel
        "Холоцен"@bg ,
        "Holocén"@cs ,
        "Holocæn"@da ,
        "Holozän"@de ,
        "Holocene"@en ,
        "Holoceno"@es ,
        "Holotseen"@et ,
        "Holoseeni"@fi ,
        "Holocène"@fr ,
        "holocén"@hu ,
        "olocene"@it ,
        "完新世"@ja ,
        "Holocenas"@lt ,
        "Holoceen"@nl ,
        "Holocen"@no ,
        "Holocen"@pl ,
        "Holocénico"@pt ,
        "holocén"@sk ,
        "holocen"@sl ,
        "holocen"@sv ,
        "全新世"@zh ;
    prov:wasDerivedFrom ts:gts2020 ;
.

isc:Jurassic
    dcterms:identifier "Jurassic" ;
    a skos:Concept ;
    rdfs:isDefinedBy ts:gts2020 ;
    skos:broader isc:Mesozoic ;
    skos:definition "A time period with the following approximated bounds: older bound -201.3 +|-0.2 Ma, younger bound -145.0 Ma" ;
    skos:inScheme cs: ;
    skos:narrower
        isc:LowerJurassic ,
        isc:MiddleJurassic ,
        isc:UpperJurassic ;
    skos:prefLabel
        "Юра"@bg ,
        "Jura"@cs ,
        "Jurassisk"@da ,
        "Jura"@de ,
        "Jurassic"@en ,
        "Jurásico"@es ,
        "Juura"@et ,
        "Jura"@fi ,
        "Jurassique"@fr ,
        "jura"@hu ,
        "giurassico"@it ,
        "ジュラ紀"@ja ,
        "Jura"@lt ,
        "Jura"@nl ,
        "Jura"@no ,
        "Jura"@pl ,
        "Jurássico"@pt ,
        "jura, jurský"@sk ,
        "jura"@sl ,
        "jura"@sv ,
        "侏罗纪"@zh ;
    prov:wasDerivedFrom ts:gts2020 ;
.

isc:Llandovery
    dcterms:identifier "Llandovery" ;
    a skos:Concept ;
    rdfs:isDefinedBy ts:gts2020 ;
    skos:broader isc:Silurian ;
    skos:definition "A time period with the following approximated bounds: older bound -443.8 +|-1.5 Ma, younger bound -433.4 +|-0.8 Ma" ;
    skos:inScheme cs: ;
    skos:narrower
        isc:Aeronian ,
        isc:Rhuddanian ,
        isc:Telychian ;
    skos:prefLabel
        "Лиандовери"@bg ,
        "Llandovery"@cs ,
        "Llandovery"@da ,
        "Llandovery"@de ,
        "Llandovery"@en ,
        "Llandovery"@es ,
        "Llandovery"@et ,
        "Llandovery"@fi ,
        "Llandovery"@fr ,
        "llandoveryi"@hu ,
        "llandovery"@it ,
        "ランドベリアン世"@ja ,
        "Landoveris"@lt ,
        "Llandovery"@nl ,
        "Llandovery"@no ,
        "Landower"@pl ,
        "Llandovery"@pt ,
        "llandover"@sk ,
        "llandoverij"@sl ,
        "llandovery"@sv ,
        "兰多维列世"@zh ;
    prov:wasDerivedFrom ts:gts2020 ;
.

isc:LowerDevonian
    dcterms:identifier "LowerDevonian" ;
    a skos:Concept ;
    rdfs:isDefinedBy ts:gts2020 ;
    skos:broader isc:Devonian ;
    skos:definition "A time period with the following approximated bounds: older bound -419.2 +|-3.2 Ma, younger bound -393.3 +|-1.2 Ma" ;
    skos:inScheme cs: ;
    skos:narrower
        isc:Emsian ,
        isc:Lochkovian ,
        isc:Pragian ;
    skos:prefLabel
        "Ранен Девон"@bg ,
        "brzy devon"@cs ,
        "Tidlig Devon"@da ,
        "Frühes Devon"@de ,
        "Early Devonian"@en ,
        "Devónico temprano"@es ,
        "Vara-Devon"@et ,
        "Varhais-Devoni"@fi ,
        "Dévonien précoce"@fr ,
        "kora-devon"@hu ,
        "devoniano precoce"@it ,
        "デボン紀前期"@ja ,
        "Ankstyvasis Devonas"@lt ,
        "Vroeg Devoon"@nl ,
        "Tidlig devon"@no ,
        "Wczesny Dewon"@pl ,
        "Devoniano primitivo"@pt ,
        "raný devón"@sk ,
        "zgodnji devon"@sl ,
        "äldre devon"@sv ,
        "早泥盆世"@zh ;
    prov:wasDerivedFrom ts:gts2020 ;
.

isc:Mesoproterozoic
    dcterms:identifier "Mesoproterozoic" ;
    a skos:Concept ;
    rdfs:isDefinedBy ts:gts2020 ;
    skos:broader isc:Proterozoic ;
    skos:definition "A time period with the following approximated bounds: older bound -1600 Ma, younger bound -1000 Ma" ;
    skos:inScheme cs: ;
    skos:narrower
        isc:Calymmian ,
        isc:Ectasian ,
        isc:Stenian ;
    skos:prefLabel
        "Мезопротерозой"@bg ,
        "Mezoproterozoikum"@cs ,
        "Mesoproterozoisk"@da ,
        "Mesoproterozoikum"@de ,
        "Mesoproterozoic"@en ,
        "Mesoproterozoico"@es ,
        "Mesoproterosoikum"@et ,
        "Mesoproterotsoikum"@fi ,
        "Mésoprotérozoïque"@fr ,
        "mezoproterozoikum"@hu ,
        "mesoproterozoico"@it ,
        "原生代中期"@ja ,
        "Mezoproterozojus"@lt ,
        "Mesoproterozoïcum"@nl ,
        "Mesoproterozoikum"@no ,
        "Mezoproterozoik"@pl ,
        "Mesoproterozóico"@pt ,
        "mezoproterozoikum"@sk ,
        "mezoproterozoik"@sl ,
        "mesoproterozoikum"@sv ,
        "中元古代"@zh ;
    prov:wasDerivedFrom ts:gts2020 ;
.

isc:Mesozoic
    dcterms:identifier "Mesozoic" ;
    a skos:Concept ;
    rdfs:isDefinedBy ts:gts2020 ;
    skos:broader isc:Phanerozoic ;
    skos:definition "A time period with the following approximated bounds: older bound -251.902 +|-0.024 Ma, younger bound -66.0 Ma" ;
    skos:inScheme cs: ;
    skos:narrower
        isc:Cretaceous ,
        isc:Jurassic ,
        isc:Triassic ;
    skos:prefLabel
        "Мезозой"@bg ,
        "Mezozoikum"@cs ,
        "Mesozoisk"@da ,
        "Mesozoikum"@de ,
        "Mesozoic"@en ,
        "Mesozoico"@es ,
        "Mesosoikum"@et ,
        "Mesotsoikum"@fi ,
        "Mésozoïque"@fr ,
        "mezozoikum"@hu ,
        "mesozoico"@it ,
        "中生代"@ja ,
        "Mezozojus"@lt ,
        "Mesozoïcum"@nl ,
        "Mesozoikum"@no ,
        "Mezozoik"@pl ,
        "Mesozóico"@pt ,
        "mezozoikum"@sk ,
        "mezozoik"@sl ,
        "mesozoikum"@sv ,
        "中生代"@zh ;
    prov:wasDerivedFrom ts:gts2020 ;
.

isc:Miaolingian
    dcterms:identifier "Miaolingian" ;
    a skos:Concept ;
    rdfs:isDefinedBy ts:gts2020 ;
    skos:broader isc:Cambrian ;
    skos:definition "A time period with the following approximated bounds: older bound -509 Ma, younger bound -497 Ma" ;
    skos:inScheme cs: ;
    skos:narrower
        isc:Drumian ,
        isc:Guzhangian ,
        isc:Wuliuan ;
    skos:prefLabel "Miaolingian"@en ;
    prov:wasDerivedFrom ts:gts2020 ;
.

isc:Mississippian
    dcterms:identifier "Mississippian" ;
    a skos:Concept ;
    rdfs:isDefinedBy ts:gts2020 ;
    skos:broader isc:Carboniferous ;
    skos:definition "A time period with the following approximated bounds: older bound -358.9 +|-0.4 Ma, younger bound -323.2 +|-0.4 Ma" ;
    skos:inScheme cs: ;
    skos:narrower
        isc:LowerMississippian ,
        isc:MiddleMississippian ,
        isc:UpperMississippian ;
    skos:prefLabel
        "Миѿиѿип"@bg ,
        "Mississip"@cs ,
        "Mississippien"@da ,
        "Mississippium"@de ,
        "Mississippian"@en ,
        "Mississippiense"@es ,
        "Mississippi"@et ,
        "Mississippi"@fi ,
        "Mississippien"@fr ,
        "mississippi"@hu ,
        "mississippiano"@it ,
        "ミシシッピアン紀"@ja ,
        "Misisipis"@lt ,
        "Mississippiën"@nl ,
        "Mississippium"@no ,
        "Missisip"@pl ,
        "Mississipiano"@pt ,
        "mississip"@sk ,
        "mississippij"@sl ,
        "mississippi"@sv ,
        "密西西比亚纪"@zh ;
    prov:wasDerivedFrom ts:gts2020 ;
.

isc:Neoproterozoic
    dcterms:identifier "Neoproterozoic" ;
    a skos:Concept ;
    rdfs:isDefinedBy ts:gts2020 ;
    skos:broader isc:Proterozoic ;
    skos:definition "A time period with the following approximated bounds: older bound -1000 Ma, younger bound -541.0 +|-1.0 Ma" ;
    skos:inScheme cs: ;
    skos:narrower
        isc:Cryogenian ,
        isc:Ediacaran ,
        isc:Tonian ;
    skos:prefLabel
        "пеопротерозой"@bg ,
        "Neoproterozoikum"@cs ,
        "Neoproterozoisk"@da ,
        "Neoproterozoikum"@de ,
        "Neoproterozoic"@en ,
        "Neoproerozoico"@es ,
        "Neoproterosoikum"@et ,
        "Neoproterotsoikum"@fi ,
        "Néoprotérozoïque"@fr ,
        "neoproterozoikum"@hu ,
        "neoproterozoico"@it ,
        "原生代後期"@ja ,
        "Neoproterozojus"@lt ,
        "Neoproterozoïcum"@nl ,
        "Neoproterozoikum"@no ,
        "Neoproterozoik"@pl ,
        "Neoproterozóico"@pt ,
        "neoproterozoikum"@sk ,
        "neoproterozoik"@sl ,
        "neoproterozoikum"@sv ,
        "新元古代"@zh ;
    prov:wasDerivedFrom ts:gts2020 ;
.

isc:Ordovician
    dcterms:identifier "Ordovician" ;
    a skos:Concept ;
    rdfs:isDefinedBy ts:gts2020 ;
    skos:broader isc:Paleozoic ;
    skos:definition "A time period with the following approximated bounds: older bound -485.4 +|-1.9 Ma, younger bound -443.8 +|-1.5 Ma" ;
    skos:inScheme cs: ;
    skos:narrower
        isc:LowerOrdovician ,
        isc:MiddleOrdovician ,
        isc:UpperOrdovician ;
    skos:prefLabel
        "Ордовик"@bg ,
        "Ordovik"@cs ,
        "Ordovicium"@da ,
        "Ordovizium"@de ,
        "Ordovician"@en ,
        "Ordovícico"@es ,
        "Ordoviitsium"@et ,
        "Ordoviikki"@fi ,
        "Ordovicien"@fr ,
        "ordovícium"@hu ,
        "ordoviciano"@it ,
        "オルドビス紀"@ja ,
        "Ordovikas"@lt ,
        "Ordovicium"@nl ,
        "Ordovicium"@no ,
        "Ordowik"@pl ,
        "Ordovícico"@pt ,
        "ordovik"@sk ,
        "ordovicij"@sl ,
        "ordovicium"@sv ,
        "奥陶纪"@zh ;
    prov:wasDerivedFrom ts:gts2020 ;
.

isc:Paleocene
    dcterms:identifier "Paleocene" ;
    a skos:Concept ;
    rdfs:isDefinedBy ts:gts2020 ;
    skos:broader isc:Paleogene ;
    skos:definition "A time period with the following approximated bounds: older bound -66.0 Ma, younger bound -56 Ma" ;
    skos:inScheme cs: ;
    skos:narrower
        isc:Danian ,
        isc:Selandian ,
        isc:Thanetian ;
    skos:prefLabel
        "Палеоцен"@bg ,
        "Paleocén"@cs ,
        "Paleocæn"@da ,
        "Paläozän"@de ,
        "Paleocene"@en ,
        "Palaeocene"@en-gb ,
        "Paleocene"@en-us ,
        "Paleoceno"@es ,
        "Paleotseen"@et ,
        "Paleoseeni"@fi ,
        "Paléocène"@fr ,
        "paleocén"@hu ,
        "paleocene"@it ,
        "暁新世"@ja ,
        "Paleocenas"@lt ,
        "Paleoceen"@nl ,
        "Paleocen"@no ,
        "Paleocen"@pl ,
        "Paleocénico"@pt ,
        "paleocén"@sk ,
        "paleocen"@sl ,
        "paleocen"@sv ,
        "古新世"@zh ;
    prov:wasDerivedFrom ts:gts2020 ;
.

isc:Paleogene
    dcterms:identifier "Paleogene" ;
    a skos:Concept ;
    rdfs:isDefinedBy ts:gts2020 ;
    skos:broader isc:Cenozoic ;
    skos:definition "A time period with the following approximated bounds: older bound -66.0 Ma, younger bound -23.03 Ma" ;
    skos:inScheme cs: ;
    skos:narrower
        isc:Eocene ,
        isc:Oligocene ,
        isc:Paleocene ;
    skos:prefLabel
        "Палеоген"@bg ,
        "Paleogén"@cs ,
        "Palæogen"@da ,
        "Paläogen"@de ,
        "Paleogene"@en ,
        "Palaeogene"@en-gb ,
        "Paleogene"@en-us ,
        "Paleógeno"@es ,
        "Paleogeen"@et ,
        "Paleogeeni"@fi ,
        "Paléogène"@fr ,
        "paleogén"@hu ,
        "paleogene"@it ,
        "古第三紀"@ja ,
        "Paleogenas"@lt ,
        "Paleogeen"@nl ,
        "Paleogen"@no ,
        "Paleogen"@pl ,
        "Paleogénico"@pt ,
        "paleogén"@sk ,
        "paleogen"@sl ,
        "paleogen"@sv ,
        "早第三纪"@zh ;
    prov:wasDerivedFrom ts:gts2020 ;
.

isc:Pennsylvanian
    dcterms:identifier "Pennsylvanian" ;
    a skos:Concept ;
    rdfs:isDefinedBy ts:gts2020 ;
    skos:broader isc:Carboniferous ;
    skos:definition "A time period with the following approximated bounds: older bound -323.2 +|-0.4 Ma, younger bound -298.9 +|-0.15 Ma" ;
    skos:inScheme cs: ;
    skos:narrower
        isc:LowerPennsylvanian ,
        isc:MiddlePennsylvanian ,
        isc:UpperPennsylvanian ;
    skos:prefLabel
        "Пенѿилван"@bg ,
        "Pennsylván"@cs ,
        "Pennsylvanien"@da ,
        "Pennsylvanium"@de ,
        "Pennsylvanian"@en ,
        "Pennsylvaniense"@es ,
        "Pennsylvania"@et ,
        "Pennsylvania"@fi ,
        "Pennsylvanien"@fr ,
        "pennsylvaniai"@hu ,
        "pennsylvaniano"@it ,
        "ペンシルバニア紀"@ja ,
        "Pensilvanis"@lt ,
        "Pennsylvaniën"@nl ,
        "Pennsylvanium"@no ,
        "Pensylwan"@pl ,
        "Pensilvaniano"@pt ,
        "penssylván"@sk ,
        "pennsylvanij"@sl ,
        "pennsylvan"@sv ,
        "宾夕法尼亚亚纪"@zh ;
    prov:wasDerivedFrom ts:gts2020 ;
.

isc:Permian
    dcterms:identifier "Permian" ;
    a skos:Concept ;
    rdfs:isDefinedBy ts:gts2020 ;
    skos:broader isc:Paleozoic ;
    skos:definition "A time period with the following approximated bounds: older bound -298.9 +|-0.15 Ma, younger bound -251.902 +|-0.024 Ma" ;
    skos:inScheme cs: ;
    skos:narrower
        isc:Cisuralian ,
        isc:Guadalupian ,
        isc:Lopingian ;
    skos:prefLabel
        "Перм"@bg ,
        "Perm"@cs ,
        "Perm"@da ,
        "Perm"@de ,
        "Permian"@en ,
        "Pérmico"@es ,
        "Perm"@et ,
        "Permi"@fi ,
        "Permien"@fr ,
        "perm"@hu ,
        "permiano"@it ,
        "ペルム紀"@ja ,
        "Permas"@lt ,
        "Perm"@nl ,
        "Perm"@no ,
        "Perm"@pl ,
        "Pérmico"@pt ,
        "perm"@sk ,
        "perm"@sl ,
        "perm"@sv ,
        "二叠纪"@zh ;
    prov:wasDerivedFrom ts:gts2020 ;
.

isc:Phanerozoic
    dcterms:identifier "Phanerozoic" ;
    a skos:Concept ;
    rdfs:isDefinedBy ts:gts2020 ;
    skos:definition "A time period with the following approximated bounds: older bound -541.0 +|-1.0 Ma, younger bound -0.0 Ma" ;
    skos:inScheme cs: ;
    skos:narrower
        isc:Cenozoic ,
        isc:Mesozoic ,
        isc:Paleozoic ;
    skos:prefLabel
        "Фанерозой"@bg ,
        "Fanerozoikum"@cs ,
        "Phanerozoisk"@da ,
        "Phanerozoikum"@de ,
        "Phanerozoic"@en ,
        "Fanerozoico"@es ,
        "Fanerosoikum"@et ,
        "Fanerotsoikum"@fi ,
        "Phanérozoïque"@fr ,
        "fanerozoikum"@hu ,
        "fanerozoico"@it ,
        "顕生代"@ja ,
        "Fanerozojus"@lt ,
        "Phanerozoïcum"@nl ,
        "Fanerozoikum"@no ,
        "Fanerozoik"@pl ,
        "Fanerozóico"@pt ,
        "fanerozoikum"@sk ,
        "fanerozoik"@sl ,
        "fanerozoikum"@sv ,
        "显生宙"@zh ;
    prov:wasDerivedFrom ts:gts2020 ;
.

isc:Precambrian
    dcterms:identifier "Precambrian" ;
    a skos:Concept ;
    rdfs:isDefinedBy ts:gts2020 ;
    skos:definition "A time period with the following approximated bounds: older bound -4567 +|-1 Ma, younger bound -541.0 +|-1.0 Ma" ;
    skos:inScheme cs: ;
    skos:narrower
        isc:Archean ,
        isc:Hadean ,
        isc:Proterozoic ;
    skos:prefLabel
        "Прекамбрий"@bg ,
        "Prekambrium"@cs ,
        "Prækambrium"@da ,
        "Präkambrium"@de ,
        "Precambrian"@en ,
        "Precámbrico"@es ,
        "Prekambrium"@et ,
        "Prekambri"@fi ,
        "Précambrien"@fr ,
        "prekambrium"@hu ,
        "precambriano"@it ,
        "先カンブリア時代"@ja ,
        "Prekambras"@lt ,
        "Precambrium"@nl ,
        "Prekambrium"@no ,
        "Prekambr"@pl ,
        "Precâmbrico"@pt ,
        "prekambrium"@sk ,
        "predkambrij"@sl ,
        "prekambrium"@sv ,
        "前寒武纪"@zh ;
    prov:wasDerivedFrom ts:gts2020 ;
.

isc:Proterozoic
    dcterms:identifier "Proterozoic" ;
    a skos:Concept ;
    rdfs:isDefinedBy ts:gts2020 ;
    skos:broader isc:Precambrian ;
    skos:definition "A time period with the following approximated bounds: older bound -2500 Ma, younger bound -541.0 +|-1.0 Ma" ;
    skos:inScheme cs: ;
    skos:narrower
        isc:Mesoproterozoic ,
        isc:Neoproterozoic ,
        isc:Paleoproterozoic ;
    skos:prefLabel
        "Протерозой"@bg ,
        "Proterozoikum"@cs ,
        "Proterozoikum"@da ,
        "Proterozoikum"@de ,
        "Proterozoic"@en ,
        "Proterozoico"@es ,
        "Proterosoikum"@et ,
        "Proterotsoikum"@fi ,
        "Protérozoïque"@fr ,
        "proterozoos"@hu ,
        "proterozoico"@it ,
        "原生代"@ja ,
        "Proterozojus"@lt ,
        "Proterozoïcum"@nl ,
        "Proterozoisk"@no ,
        "Proterozoik"@pl ,
        "Proterozóico"@pt ,
        "proterozoikum"@sk ,
        "proterozoik"@sl ,
        "proterozoikum"@sv ,
        "元古宙"@zh ;
    prov:wasDerivedFrom ts:gts2020 ;
.

isc:Triassic
    dcterms:identifier "Triassic" ;
    a skos:Concept ;
    rdfs:isDefinedBy ts:gts2020 ;
    skos:broader isc:Mesozoic ;
    skos:definition "A time period with the following approximated bounds: older bound -251.902 +|-0.024 Ma, younger bound -201.3 +|-0.2 Ma" ;
    skos:inScheme cs: ;
    skos:narrower
        isc:LowerTriassic ,
        isc:MiddleTriassic ,
        isc:UpperTriassic ;
    skos:prefLabel
        "Триаѿ"@bg ,
        "Trias"@cs ,
        "Triassisk"@da ,
        "Trias"@de ,
        "Triassic"@en ,
        "Triásico"@es ,
        "Triias"@et ,
        "Trias"@fi ,
        "Trias"@fr ,
        "triász"@hu ,
        "triassico"@it ,
        "三畳紀"@ja ,
        "Triasas"@lt ,
        "Trias"@nl ,
        "Trias"@no ,
        "Trias"@pl ,
        "Triásico"@pt ,
        "trias"@sk ,
        "trias"@sl ,
        "trias"@sv ,
        "三叠纪"@zh ;
    prov:wasDerivedFrom ts:gts2020 ;
.

isc:UpperJurassic
    dcterms:identifier "UpperJurassic" ;
    a skos:Concept ;
    rdfs:isDefinedBy ts:gts2020 ;
    skos:broader isc:Jurassic ;
    skos:definition "A time period with the following approximated bounds: older bound -163.5 +|-1.0 Ma, younger bound -145.0 Ma" ;
    skos:inScheme cs: ;
    skos:narrower
        isc:Kimmeridgian ,
        isc:Oxfordian ,
        isc:Tithonian ;
    skos:prefLabel
        "Къѿна Юра"@bg ,
        "Pozdní jura"@cs ,
        "Sen Jurassisk"@da ,
        "Später Jura"@de ,
        "Late Jurassic"@en ,
        "Hilis-Juura"@et ,
        "Myöhäis-Jura"@fi ,
        "késő-jura"@hu ,
        "後期ジュラ紀"@ja ,
        "Vėlyvoji Jura"@lt ,
        "Laat Jura"@nl ,
        "Sen jura"@no ,
        "Późna Jura"@pl ,
        "mladšia jura"@sk ,
        "pozna jura"@sl ,
        "yngre jura"@sv ,
        "晚侏罗世"@zh ;
    prov:wasDerivedFrom ts:gts2020 ;
.

isc:UpperOrdovician
    dcterms:identifier "UpperOrdovician" ;
    a skos:Concept ;
    rdfs:isDefinedBy ts:gts2020 ;
    skos:broader isc:Ordovician ;
    skos:definition "A time period with the following approximated bounds: older bound -458.4 +|-0.9 Ma, younger bound -443.8 +|-1.5 Ma" ;
    skos:inScheme cs: ;
    skos:narrower
        isc:Hirnantian ,
        isc:Katian ,
        isc:Sandbian ;
    skos:prefLabel
        "Къѿен Ордовик"@bg ,
        "Pozdní ordovik"@cs ,
        "Sen Ordovicium"@da ,
        "Spätes Ordovizium"@de ,
        "Late Ordovician"@en ,
        "Hilis-Ordoviitsium"@et ,
        "Myöhäis-Ordoviikki"@fi ,
        "késő-ordovícium"@hu ,
        "後期オルドビス紀"@ja ,
        "Vėlyvasis Ordovikas"@lt ,
        "Laat Ordovicium"@nl ,
        "Sen ordovicium"@no ,
        "Późny Ordowik"@pl ,
        "mladší ordovik"@sk ,
        "starejši ordovicij"@sl ,
        "yngre ordovicium"@sv ,
        "晚奥陶世"@zh ;
    prov:wasDerivedFrom ts:gts2020 ;
.

isc:UpperTriassic
    dcterms:identifier "UpperTriassic" ;
    a skos:Concept ;
    rdfs:isDefinedBy ts:gts2020 ;
    skos:broader isc:Triassic ;
    skos:definition "A time period with the following approximated bounds: older bound -237 Ma, younger bound -201.3 +|-0.2 Ma" ;
    skos:inScheme cs: ;
    skos:narrower
        isc:Carnian ,
        isc:Norian ,
        isc:Rhaetian ;
    skos:prefLabel
        "Къѿен Триаѿ"@bg ,
        "Pozdní trias"@cs ,
        "Sen Triassisk"@da ,
        "Späte Trias"@de ,
        "Late Triassic"@en ,
        "Hilis-Triias"@et ,
        "Myöhäis-Trias"@fi ,
        "késő-triász"@hu ,
        "後期三畳紀"@ja ,
        "Vėlyvasis Triasas"@lt ,
        "Laat Trias"@nl ,
        "Sen trias"@no ,
        "Późny Trias"@pl ,
        "mladší trias"@sk ,
        "pozni trias"@sl ,
        "yngre trias"@sv ,
        "晚三叠世"@zh ;
    prov:wasDerivedFrom ts:gts2020 ;
.

isc:Archean
    dcterms:identifier "Archean" ;
    a skos:Concept ;
    rdfs:isDefinedBy ts:gts2020 ;
    skos:broader isc:Precambrian ;
    skos:definition "A time period with the following approximated bounds: older bound -4000 Ma, younger bound -2500 Ma" ;
    skos:inScheme cs: ;
    skos:narrower
        isc:Eoarchean ,
        isc:Mesoarchean ,
        isc:Neoarchean ,
        isc:Paleoarchean ;
    skos:prefLabel
        "прхай"@bg ,
        "Archaikum"@cs ,
        "Arkæisk"@da ,
        "Archaikum"@de ,
        "Archean"@en ,
        "Archaean"@en-gb ,
        "Archean"@en-us ,
        "Arcaico"@es ,
        "Arhaikum"@et ,
        "Arkeikum"@fi ,
        "Archéen"@fr ,
        "archaikum"@hu ,
        "archeano"@it ,
        "始生代"@ja ,
        "Archejus"@lt ,
        "Archaïcum"@nl ,
        "Arkeikum"@no ,
        "Archaik"@pl ,
        "Arcaico"@pt ,
        "archaikum, prahory"@sk ,
        "arhaik"@sl ,
        "arkeikum"@sv ,
        "太古宙"@zh ;
    prov:wasDerivedFrom ts:gts2020 ;
.

isc:Cambrian
    dcterms:identifier "Cambrian" ;
    a skos:Concept ;
    rdfs:isDefinedBy ts:gts2020 ;
    skos:broader isc:Paleozoic ;
    skos:definition "A time period with the following approximated bounds: older bound -541.0 +|-1.0 Ma, younger bound -485.4 +|-1.9 Ma" ;
    skos:inScheme cs: ;
    skos:narrower
        isc:CambrianSeries2 ,
        isc:Furongian ,
        isc:Miaolingian ,
        isc:Terreneuvian ;
    skos:prefLabel
        "Камбрий"@bg ,
        "Kambrium"@cs ,
        "Kambrium"@da ,
        "Kambrium"@de ,
        "Cambrian"@en ,
        "Cámbrico"@es ,
        "Kambrium"@et ,
        "Kambri"@fi ,
        "Cambrien"@fr ,
        "kambriumi"@hu ,
        "cambriano"@it ,
        "カンブリア紀"@ja ,
        "Kambras"@lt ,
        "Cambrium"@nl ,
        "Cambrium"@no ,
        "Kambr"@pl ,
        "Câmbrico"@pt ,
        "kambrium"@sk ,
        "kambrij"@sl ,
        "kambrium"@sv ,
        "寒武纪"@zh ;
    prov:wasDerivedFrom ts:gts2020 ;
.

isc:Cisuralian
    dcterms:identifier "Cisuralian" ;
    a skos:Concept ;
    rdfs:isDefinedBy ts:gts2020 ;
    skos:broader isc:Permian ;
    skos:definition "A time period with the following approximated bounds: older bound -298.9 +|-0.15 Ma, younger bound -272.95 +|-0.11 Ma" ;
    skos:inScheme cs: ;
    skos:narrower
        isc:Artinskian ,
        isc:Asselian ,
        isc:Kungurian ,
        isc:Sakmarian ;
    skos:prefLabel
        "Циѿурал"@bg ,
        "Cisural"@cs ,
        "Cisuralien"@da ,
        "Cisuralium"@de ,
        "Cisuralian"@en ,
        "Cisuraliense"@es ,
        "Cisural"@et ,
        "Cisural"@fi ,
        "Cisuralien"@fr ,
        "ciszurali"@hu ,
        "cisuraliano"@it ,
        "キスラリアン世"@ja ,
        "Kisuralis"@lt ,
        "Cisuraliën"@nl ,
        "Cisuralium"@no ,
        "Cisural"@pl ,
        "Cisuraliano"@pt ,
        "cisural"@sk ,
        "cisuralij"@sl ,
        "cisural"@sv ,
        "乌拉尔世"@zh ;
    prov:wasDerivedFrom ts:gts2020 ;
.

isc:Eocene
    dcterms:identifier "Eocene" ;
    a skos:Concept ;
    rdfs:isDefinedBy ts:gts2020 ;
    skos:broader isc:Paleogene ;
    skos:definition "A time period with the following approximated bounds: older bound -56 Ma, younger bound -33.9 Ma" ;
    skos:inScheme cs: ;
    skos:narrower
        isc:Bartonian ,
        isc:Lutetian ,
        isc:Priabonian ,
        isc:Ypresian ;
    skos:prefLabel
        "Еоцен"@bg ,
        "Eocén"@cs ,
        "Eocæn"@da ,
        "Eozän"@de ,
        "Eocene"@en ,
        "Eoceno"@es ,
        "Eotseen"@et ,
        "Eoseeni"@fi ,
        "Eocène"@fr ,
        "eocén"@hu ,
        "eocene"@it ,
        "始新世"@ja ,
        "Eocenas"@lt ,
        "Eoceen"@nl ,
        "Eocen"@no ,
        "Eocen"@pl ,
        "Eocénico"@pt ,
        "eocén"@sk ,
        "eocen"@sl ,
        "eocen"@sv ,
        "始新世"@zh ;
    prov:wasDerivedFrom ts:gts2020 ;
.

isc:LowerJurassic
    dcterms:identifier "LowerJurassic" ;
    a skos:Concept ;
    rdfs:isDefinedBy ts:gts2020 ;
    skos:broader isc:Jurassic ;
    skos:definition "A time period with the following approximated bounds: older bound -201.3 +|-0.2 Ma, younger bound -174.1 +|-1.0 Ma" ;
    skos:inScheme cs: ;
    skos:narrower
        isc:Hettangian ,
        isc:Pliensbachian ,
        isc:Sinemurian ,
        isc:Toarcian ;
    skos:prefLabel
        "Ранна Юра"@bg ,
        "brzy jura"@cs ,
        "Tidlig Jurassisk"@da ,
        "Früher Jura"@de ,
        "Early Jurassic"@en ,
        "Jurásico temprano"@es ,
        "Vara-Juura"@et ,
        "Varhais-Jura"@fi ,
        "Jurassique précoce"@fr ,
        "kora-jura"@hu ,
        "giurassico precoce"@it ,
        "ジュラ紀前期"@ja ,
        "Ankstyvoji Jura"@lt ,
        "Vroeg Jura"@nl ,
        "Tidlig jura"@no ,
        "Wczesna Jura"@pl ,
        "Jurássico primitivo"@pt ,
        "raná jura"@sk ,
        "zgodnja jura"@sl ,
        "äldre jura"@sv ,
        "早侏罗世"@zh ;
    prov:wasDerivedFrom ts:gts2020 ;
.

isc:MiddleJurassic
    dcterms:identifier "MiddleJurassic" ;
    a skos:Concept ;
    rdfs:isDefinedBy ts:gts2020 ;
    skos:broader isc:Jurassic ;
    skos:definition "A time period with the following approximated bounds: older bound -174.1 +|-1.0 Ma, younger bound -163.5 +|-1.0 Ma" ;
    skos:inScheme cs: ;
    skos:narrower
        isc:Aalenian ,
        isc:Bajocian ,
        isc:Bathonian ,
        isc:Callovian ;
    skos:prefLabel
        "Средна Юра"@bg ,
        "Střední jura"@cs ,
        "Mellem Jurassisk"@da ,
        "Mittlerer Jura"@de ,
        "Middle Jurassic"@en ,
        "Jurásico Medio"@es ,
        "Kesk-Juura"@et ,
        "Keski-Jura"@fi ,
        "Jurassique moyen"@fr ,
        "középső-jura"@hu ,
        "giurassico medio"@it ,
        "中期ジュラ紀"@ja ,
        "Vidurinė Jura"@lt ,
        "Midden Jura"@nl ,
        "Midtre jura"@no ,
        "Środkowa Jura"@pl ,
        "Jurássico Médio"@pt ,
        "stredná jura"@sk ,
        "srednja jura"@sl ,
        "mellersta jura"@sv ,
        "中侏罗世"@zh ;
    prov:wasDerivedFrom ts:gts2020 ;
.

isc:Paleoproterozoic
    dcterms:identifier "Paleoproterozoic" ;
    a skos:Concept ;
    rdfs:isDefinedBy ts:gts2020 ;
    skos:broader isc:Proterozoic ;
    skos:definition "A time period with the following approximated bounds: older bound -2500 Ma, younger bound -1600 Ma" ;
    skos:inScheme cs: ;
    skos:narrower
        isc:Orosirian ,
        isc:Rhyacian ,
        isc:Siderian ,
        isc:Statherian ;
    skos:prefLabel
        "Палеопротерозой"@bg ,
        "Paleoproterozoikum"@cs ,
        "Palæoproterozoisk"@da ,
        "Paläoproteroizoikum"@de ,
        "Paleoproterozoic"@en ,
        "Palaeoproterozoic"@en-gb ,
        "Paleoproterozoic"@en-us ,
        "Paleoproterozoico"@es ,
        "Paleoproterosoikum"@et ,
        "Paleoproterotsoikum"@fi ,
        "Paléoprotérozoïque"@fr ,
        "paleoproterozikum"@hu ,
        "paleoproterozoico"@it ,
        "原生代前期"@ja ,
        "Paleoproterozojus"@lt ,
        "paleoproterozoïcum"@nl ,
        "Paleoproterozoikum"@no ,
        "Paleoproterozoik"@pl ,
        "Paleoproterozóico"@pt ,
        "paleoproterozoikum"@sk ,
        "paleoproterozoik"@sl ,
        "paleoproterozoikum"@sv ,
        "古元古代"@zh ;
    prov:wasDerivedFrom ts:gts2020 ;
.

isc:Pleistocene
    dcterms:identifier "Pleistocene" ;
    a skos:Concept ;
    rdfs:isDefinedBy ts:gts2020 ;
    skos:broader isc:Quaternary ;
    skos:definition "A time period with the following approximated bounds: older bound -2.58 Ma, younger bound -0.0117 Ma" ;
    skos:inScheme cs: ;
    skos:narrower
        isc:Calabrian ,
        isc:Gelasian ,
        isc:MiddlePleistocene ,
        isc:UpperPleistocene ;
    skos:prefLabel
        "Плейѿтоцен"@bg ,
        "Pleistocén"@cs ,
        "Pleistocæn"@da ,
        "Pleistozän"@de ,
        "Pleistocene"@en ,
        "Pleistoceno"@es ,
        "Pleistotseen"@et ,
        "Pleistoseeni"@fi ,
        "Pléistocène"@fr ,
        "pleisztocén"@hu ,
        "pleistocene"@it ,
        "更新世"@ja ,
        "Pleistocenas"@lt ,
        "Pleistoceen"@nl ,
        "Pleistocen"@no ,
        "Plejstocen"@pl ,
        "Plistocénico"@pt ,
        "pleistocén"@sk ,
        "pleistocen"@sl ,
        "pleistocen"@sv ,
        "更新世"@zh ;
    prov:wasDerivedFrom ts:gts2020 ;
.

isc:Silurian
    dcterms:identifier "Silurian" ;
    a skos:Concept ;
    rdfs:isDefinedBy ts:gts2020 ;
    skos:broader isc:Paleozoic ;
    skos:definition "A time period with the following approximated bounds: older bound -443.8 +|-1.5 Ma, younger bound -419.2 +|-3.2 Ma" ;
    skos:inScheme cs: ;
    skos:narrower
        isc:Llandovery ,
        isc:Ludlow ,
        isc:Pridoli ,
        isc:Wenlock ;
    skos:prefLabel
        "Силур"@bg ,
        "Silur"@cs ,
        "Silur"@da ,
        "Silur"@de ,
        "Silurian"@en ,
        "Silúrcio"@es ,
        "Silur"@et ,
        "Siluuri"@fi ,
        "Silurien"@fr ,
        "szilur"@hu ,
        "siluriano"@it ,
        "シルル紀"@ja ,
        "Silūras"@lt ,
        "Siluur"@nl ,
        "Silur"@no ,
        "Sylur"@pl ,
        "Silúrico"@pt ,
        "silúr"@sk ,
        "silur"@sl ,
        "silur"@sv ,
        "志留纪"@zh ;
    prov:wasDerivedFrom ts:gts2020 ;
.

isc:LowerCretaceous
    dcterms:identifier "LowerCretaceous" ;
    a skos:Concept ;
    rdfs:isDefinedBy ts:gts2020 ;
    skos:broader isc:Cretaceous ;
    skos:definition "A time period with the following approximated bounds: older bound -145.0 Ma, younger bound -100.5 Ma" ;
    skos:inScheme cs: ;
    skos:narrower
        isc:Albian ,
        isc:Aptian ,
        isc:Barremian ,
        isc:Berriasian ,
        isc:Hauterivian ,
        isc:Valanginian ;
    skos:prefLabel
        "Ранна Креда"@bg ,
        "Tidlig Kridt"@da ,
        "Frühe Kreide"@de ,
        "Early Cretaceous"@en ,
        "Cretácico temprano"@es ,
        "Varajane kriit"@et ,
        "Varhais-Liitu"@fi ,
        "Crétacé précoce"@fr ,
        "kora-kréta"@hu ,
        "Cretaceo precoce"@it ,
        "白亜紀前期"@ja ,
        "Ankstyvoji Kreida"@lt ,
        "Vroeg Krijt"@nl ,
        "Wczesna Kreda"@pl ,
        "Cretáceo Primitivo"@pt ,
        "raná  krieda"@sk ,
        "zgodnja kreda"@sl ,
        "äldre krita"@sv ,
        "早白垩世"@zh ;
    prov:wasDerivedFrom ts:gts2020 ;
.

isc:Miocene
    dcterms:identifier "Miocene" ;
    a skos:Concept ;
    rdfs:isDefinedBy ts:gts2020 ;
    skos:broader isc:Neogene ;
    skos:definition "A time period with the following approximated bounds: older bound -23.03 Ma, younger bound -5.333 Ma" ;
    skos:inScheme cs: ;
    skos:narrower
        isc:Aquitanian ,
        isc:Burdigalian ,
        isc:Langhian ,
        isc:Messinian ,
        isc:Serravallian ,
        isc:Tortonian ;
    skos:prefLabel
        "Миоцен"@bg ,
        "Miocén"@cs ,
        "Miocæn"@da ,
        "Miozän"@de ,
        "Miocene"@en ,
        "Mioceno"@es ,
        "Miotseen"@et ,
        "Mioseeni"@fi ,
        "Miocène"@fr ,
        "miocén"@hu ,
        "miocene"@it ,
        "中新世"@ja ,
        "Miocenas"@lt ,
        "Mioceen"@nl ,
        "Miocen"@no ,
        "Miocen"@pl ,
        "Miocénico"@pt ,
        "miocén"@sk ,
        "miocen"@sl ,
        "miocen"@sv ,
        "中新世"@zh ;
    prov:wasDerivedFrom ts:gts2020 ;
.

isc:Paleozoic
    dcterms:identifier "Paleozoic" ;
    a skos:Concept ;
    rdfs:isDefinedBy ts:gts2020 ;
    skos:broader isc:Phanerozoic ;
    skos:definition "A time period with the following approximated bounds: older bound -541.0 +|-1.0 Ma, younger bound -251.902 +|-0.024 Ma" ;
    skos:inScheme cs: ;
    skos:narrower
        isc:Cambrian ,
        isc:Carboniferous ,
        isc:Devonian ,
        isc:Ordovician ,
        isc:Permian ,
        isc:Silurian ;
    skos:prefLabel
        "Палеозой"@bg ,
        "Paleozoikum"@cs ,
        "Palæozoisk"@da ,
        "Paläozoikum"@de ,
        "Paleozoic"@en ,
        "Palaeozoic"@en-gb ,
        "Paleozoic"@en-us ,
        "Palozoico"@es ,
        "Paleosoikum"@et ,
        "Paleotsoikum"@fi ,
        "Paléozoïque"@fr ,
        "paleozoikum"@hu ,
        "paleozoico"@it ,
        "古生代"@ja ,
        "Paleozojus"@lt ,
        "Paleozoïcum"@nl ,
        "Paleozoikum"@no ,
        "Paleozoik"@pl ,
        "Paleozóico"@pt ,
        "paleozoikum"@sk ,
        "paleozoik"@sl ,
        "paleozoikum"@sv ,
        "古生代"@zh ;
    prov:wasDerivedFrom ts:gts2020 ;
.

isc:UpperCretaceous
    dcterms:identifier "UpperCretaceous" ;
    a skos:Concept ;
    rdfs:isDefinedBy ts:gts2020 ;
    skos:broader isc:Cretaceous ;
    skos:definition "A time period with the following approximated bounds: older bound -100.5 Ma, younger bound -66.0 Ma" ;
    skos:inScheme cs: ;
    skos:narrower
        isc:Campanian ,
        isc:Cenomanian ,
        isc:Coniacian ,
        isc:Maastrichtian ,
        isc:Santonian ,
        isc:Turonian ;
    skos:prefLabel
        "Къѿна Креда"@bg ,
        "Pozdní křída"@cs ,
        "Sen Kridt"@da ,
        "Späte Kreide"@de ,
        "Late Cretaceous"@en ,
        "Hilis-Kriit"@et ,
        "Myöhäis-Liitu"@fi ,
        "késő-kréta"@hu ,
        "後期白亜紀"@ja ,
        "Vėlyva kreida"@lt ,
        "Laat Krijt"@nl ,
        "Sen kritt"@no ,
        "Późna Kreda"@pl ,
        "mladšia krieda"@sk ,
        "pozna kreda"@sl ,
        "yngre krita"@sv ,
        "晚白垩世"@zh ;
    prov:wasDerivedFrom ts:gts2020 ;
.

cs:
    a skos:ConceptScheme ;
    dcterms:identifier "chart" ;
    dcterms:created "2020-06-05"^^xsd:date ;
    dcterms:issued "2022-02-25"^^xsd:date ;
    dcterms:license <https://creativecommons.org/licenses/by/4.0/> ;
    dcterms:modified "2022-02-25"^^xsd:date ;
    dcterms:rights "Original version Copyright © 2020 International Commission on Stratigraphy"@en ;
    dcterms:source "https://stratigraphy.org/chart"^^xsd:anyURI ;
    skos:definition "SKOS representation of the Geologic Time Scale, as defined in the International Chronostratigraphic Chart (ICC) from the International Commission on Stratigraphy (ICS). The ICC embraces both chronostratigraphic (time-rock) units and their equivalent geochronologic (geologic-time) units, the former being related to the ‘Stratigraphic points’ referred to below, and the latter (geochronologic units) being employed in this SKOS representation."@en ;
    skos:hasTopConcept
        isc:Phanerozoic ,
        isc:Precambrian ;
    skos:prefLabel "Geologic Time Scale (2020)"@en ;
.
