@prefix gsqi: <http://linked.data.gov.au/def/gsq-initiatives/> .

@prefix dcterms: <http://purl.org/dc/terms/> .
@prefix owl: <http://www.w3.org/2002/07/owl#> .
@prefix sdo: <https://schema.org/> .
@prefix skos: <http://www.w3.org/2004/02/skos/core#> .
@prefix xsd: <http://www.w3.org/2001/XMLSchema#> .

<http://linked.data.gov.au/def/gsq-initiatives> a owl:Ontology,
        skos:ConceptScheme ;
    dcterms:created "2020-11-27"^^xsd:date ;
    dcterms:creator <http://linked.data.gov.au/org/gsq> ;
    dcterms:modified "2020-11-27"^^xsd:date ;
    dcterms:publisher <http://linked.data.gov.au/org/gsq> ;
    skos:definition "Projects and initiatives undertaken or supported by the Geological Survey of Queensland."@en ;
    skos:prefLabel "GSQ Initiatives"@en .
    
<http://linked.data.gov.au/org/gsq> a sdo:Organization ;
    sdo:name "Geological Survey of Queensland" ;
    sdo:url <https://www.business.qld.gov.au/industries/mining-energy-water/resources/geoscience-information/gsq> .

gsqi:cdi a skos:Concept ;
    skos:prefLabel "Collaborative Drilling Initiative"@en ;
    skos:definition "The Collaborative Drilling Initiative (CEI) provides industry grants to encourage exploration drilling programs, particularly in frontier areas;  "@en ;
    skos:inScheme <http://linked.data.gov.au/def/gsq-initiatives> ;
    skos:notation "CDI" ;
    skos:altLabel "CDI"@en ;
    skos:topConceptOf <http://linked.data.gov.au/def/gsq-initiatives> .

gsqi:cei a skos:Concept ;
    skos:prefLabel "Collaborative Exploration Initiative"@en ;
    skos:definition """The Collaborative Exploration Initiative (CEI) provides industry grants to: encourage exploration, particularly in frontier areas; support innovative exploration techniques, including machine learning; promote the discovery and development of 'new economy' minerals."""@en ;
    skos:inScheme <http://linked.data.gov.au/def/gsq-initiatives> ;
    skos:notation "CEI" ;
    skos:altLabel "CEI"@en ;
    skos:topConceptOf <http://linked.data.gov.au/def/gsq-initiatives> .

gsqi:cemts a skos:Concept ;
    skos:prefLabel "Cloncurry extension magnetotelluric survey"@en ;
    skos:definition "The Cloncurry extension survey began in 2019 and is being conducted as part of the Queensland Government's Strategic Resources Exploration Program in collaboration with Geoscience Australia. The project aims to build on the success of the 2016 Cloncurry magnetotelluric survey by extending coverage to prospective undercover sequences to the north-west."@en ;
    skos:inScheme <http://linked.data.gov.au/def/gsq-initiatives> ;
    skos:notation "CEMTS" ;
    skos:altLabel "CEMTS"@en ;
    skos:topConceptOf <http://linked.data.gov.au/def/gsq-initiatives> .

gsqi:cgei a skos:Concept ;
    skos:prefLabel "Coastal Geothermal energy Initiative"@en ;
    skos:definition "The Coastal Geothermal energy Initiative (CGEI) is a Queensland Government project designed to investigate potential for geothermal energy close to existing power networks and population centres. The CGEI program is a co-operative undertaking between the Office of Clean energy and the Geological Survey of Queensland (GSQ). The CGEI aims to gather thermal data through a structured drilling program to support the State's growing geothermal explorers."@en ;
    skos:inScheme <http://linked.data.gov.au/def/gsq-initiatives> ;
    skos:notation "CGEI" ;
    skos:altLabel "CGEI"@en ;
    skos:topConceptOf <http://linked.data.gov.au/def/gsq-initiatives> .

gsqi:css a skos:Concept ;
    skos:prefLabel "Camooweal seismic survey"@en ;
    skos:definition "The Camooweal 2D seismic survey was conducted in 2019 by the Geological Survey of Queensland (GSQ). This survey was funded by the Queensland Government's Strategic Resources Exploration Program. The survey's primary aim was to improve understanding of basin architecture underlying the Camooweal area  the Isa Superbasin, South Nicholson Basin and Georgina Basin  and to provide data in an area with limited exploration."@en ;
    skos:inScheme <http://linked.data.gov.au/def/gsq-initiatives> ;
    skos:notation "CSS" ;
    skos:altLabel "CSS"@en ;
    skos:topConceptOf <http://linked.data.gov.au/def/gsq-initiatives> .

gsqi:dcss a skos:Concept ;
    skos:prefLabel "Deep Crustal Seismic Surveys 2014-15"@en ;
    skos:definition "Completed in December 2010, the North West Queensland Mineral and energy Province study has improved geological understanding through geological mapping and geophysical data acquisition programs."@en ;
    skos:inScheme <http://linked.data.gov.au/def/gsq-initiatives> ;
    skos:notation "DCSS" ;
    skos:altLabel "DCSS"@en ;
    skos:topConceptOf <http://linked.data.gov.au/def/gsq-initiatives> .

gsqi:gdmp a skos:Concept ;
    skos:prefLabel "Geoscience Data Modernisation Project"@en ;
    skos:definition "The Geoscience Data Modernisation Project (GDMP) aims to transform Queenslands geoscience data ecosystem and enable data-driven exploration, discovery and success for industry."@en ;
    skos:inScheme <http://linked.data.gov.au/def/gsq-initiatives> ;
    skos:notation "GDMP" ;
    skos:altLabel "GDMP"@en ;
    skos:topConceptOf <http://linked.data.gov.au/def/gsq-initiatives> .

gsqi:mkdg a skos:Concept ;
    skos:prefLabel "Mary Kathleen Domain geology"@en ;
    skos:definition "The Mary Kathleen Domain geology project is a collaboration between the Geological Survey of Queensland, James Cook University researchers and Geoscience Australia. Its aim is to establish a geochemical and geochronological framework for magmatic rocks of the Mary Kathleen Domain. Sampling and local geological mapping will be followed by geochemistry and geochronology analyses. The Mary Kathleen Domain is the western part of the highly prospective eastern succession of the Mount Isa inlier (see map below). It hosts significant copper, zinc, uranium and rare earth element deposits."@en ;
    skos:inScheme <http://linked.data.gov.au/def/gsq-initiatives> ;
    skos:notation "MKDG" ;
    skos:altLabel "MKDG"@en ;
    skos:topConceptOf <http://linked.data.gov.au/def/gsq-initiatives> .

gsqi:nemi a skos:Concept ;
    skos:prefLabel "New Economy Minerals Initiative"@en ;
    skos:definition "In order to develop a sustainable pipeline of new economy minerals projects into the future, the Queensland Government is investing in exploration activities to improve scientific understanding and supply the valuable geoscience data needed by industry to help locate and define deposits for future production. New economy minerals is an umbrella term for a range of metals and mineral elements used in many emerging technologies including electric vehicles, renewable energy products, low-emission power sources, consumer devices, and products for the medical, defence and scientific research sectors."@en ;
    skos:inScheme <http://linked.data.gov.au/def/gsq-initiatives> ;
    skos:notation "NEMI" ;
    skos:altLabel "NEMI"@en ;
    skos:topConceptOf <http://linked.data.gov.au/def/gsq-initiatives> .

gsqi:ngsa a skos:Concept ;
    skos:prefLabel "National Geochemical Survey of Australia"@en ;
    skos:definition "Completed in June 2011, GSQ collaborated with Geoscience Australia and geoscience agencies throughout Australia to conduct a survey of Australia's background geochemical concentration levels and patterns."@en ;
    skos:inScheme <http://linked.data.gov.au/def/gsq-initiatives> ;
    skos:notation "NGSA" ;
    skos:altLabel "NGSA"@en ;
    skos:topConceptOf <http://linked.data.gov.au/def/gsq-initiatives> .

gsqi:nwqmep a skos:Concept ;
    skos:prefLabel "North West Queensland Mineral and energy Province"@en ;
    skos:definition "Completed in December 2010, the North West Queensland Mineral and energy Province study has improved geological understanding through geological mapping and geophysical data acquisition programs."@en ;
    skos:inScheme <http://linked.data.gov.au/def/gsq-initiatives> ;
    skos:notation "NWQMEP" ;
    skos:altLabel "NWQMEP"@en ;
    skos:topConceptOf <http://linked.data.gov.au/def/gsq-initiatives> .

gsqi:seebase a skos:Concept ;
    skos:prefLabel "SEEBASE study and GIS data package"@en ;
    skos:definition "In 2018, under the Queensland Government's Strategic Resources Exploration Program, the Geological Survey of Queensland conducted a study using the SEEBASE methodology.The aim was to enhance the subsurface knowledge of frontier basins covering about 400,000km2 in north-west and central Queensland."@en ;
    skos:inScheme <http://linked.data.gov.au/def/gsq-initiatives> ;
    skos:notation "SEEBASE" ;
    skos:altLabel "SEEBASE"@en ;
    skos:topConceptOf <http://linked.data.gov.au/def/gsq-initiatives> .

gsqi:srep a skos:Concept ;
    skos:prefLabel "Strategic Resources Exploration Program"@en ;
    skos:definition """The 4-year Strategic Resources Exploration Program is a $27.125 million project to boost exploration and support for resource development projects. The program funding is helping to expand resource exploration and development for gas and minerals in North West Queensland. Initiatives funded under the program include: $3.6 million to drive exploration for gas in the Georgina, South Nicholson and Isa Super Basins. $4.275 million for mineral geophysics to pinpoint the locations of potential new mineral prospects over wide areas. $1.45 million for mineral geochemistry programs to identify the type of potential mineral deposits (e.g. copper, lead, zinc) identified from geophysical programs using surface samples. $4.95 million for mineral synthesis to develop a comprehensive and integrated understanding of the geology of the North West Minerals Province $925,000 to support national research into advanced techniques used in the discovery of mineral deposits in frontier regions. $7.125 million for the Geoscience Data Modernisation Program, to modernise legacy systems and enable data driven exploration and resource development opportunities for Queensland"""@en ;
    skos:inScheme <http://linked.data.gov.au/def/gsq-initiatives> ;
    skos:notation "SREP" ;
    skos:altLabel "SREP"@en ;
    skos:topConceptOf <http://linked.data.gov.au/def/gsq-initiatives> .
