PREFIX : <https://linked.data.gov.au/def/addr-part-types/>
PREFIX agldwgstatus: <https://linked.data.gov.au/def/reg-statuses/>
PREFIX dcterms: <http://purl.org/dc/terms/>
PREFIX droles: <https://linked.data.gov.au/def/data-roles/>
PREFIX owl: <http://www.w3.org/2002/07/owl#>
PREFIX prov: <http://www.w3.org/ns/prov#>
PREFIX rdfs: <http://www.w3.org/2000/01/rdf-schema#>
PREFIX reg: <http://purl.org/linked-data/registry#>
PREFIX sdo: <https://schema.org/>
PREFIX skos: <http://www.w3.org/2004/02/skos/core#>
PREFIX themes: <https://linked.data.gov.au/def/fsdf/themes/>
PREFIX xsd: <http://www.w3.org/2001/XMLSchema#>
PREFIX apt: <https://linked.data.gov.au/def/addr-part-types/>
PREFIX cs: <https://linked.data.gov.au/def/addr-part-types>
PREFIX dcat: <http://www.w3.org/ns/dcat#>
PREFIX isoroles: <https://linked.data.gov.au/def/data-roles/>
PREFIX schema: <https://schema.org/>


apt:addressNumberFirst
    a skos:Concept ;
    rdfs:isDefinedBy cs: ;
    skos:definition "Either the house number, or the lowest in a range where the Address Site has a range of numbers. Usually, street numbers are odd on the left side of the road, and even on the right."@en ;
    skos:historyNote "From Queensland address data." ;
    skos:inScheme cs: ;
    skos:prefLabel "Address Number First"@en ;
    skos:topConceptOf cs: ;
.

apt:addressNumberFirstSuffix
    a skos:Concept ;
    rdfs:isDefinedBy cs: ;
    skos:definition "Alphabetical suffix to streetNumberFirst. Requires streetNumberFirst to have a value."@en ;
    skos:historyNote "From Queensland address data." ;
    skos:inScheme cs: ;
    skos:prefLabel "Address Number First Suffix"@en ;
    skos:topConceptOf cs: ;
.

apt:addressNumberLast
    a skos:Concept ;
    rdfs:isDefinedBy cs: ;
    skos:definition "This is the upper number range if an Address Site has a range of numbers. Requires streetNumberFirst to have a value."@en ;
    skos:historyNote "From Queensland address data." ;
    skos:inScheme cs: ;
    skos:prefLabel "Address Number Last"@en ;
    skos:topConceptOf cs: ;
.

apt:addressNumberLastSuffix
    a skos:Concept ;
    rdfs:isDefinedBy cs: ;
    skos:definition "Alphabetical suffix to streetNumberLast. Requires streetNumberLast to have a value."@en ;
    skos:historyNote "From Queensland address data." ;
    skos:inScheme cs: ;
    skos:prefLabel "Address Number Last Suffix"@en ;
    skos:topConceptOf cs: ;
.

apt:buildingLevelNumber
    a skos:Concept ;
    rdfs:isDefinedBy cs: ;
    skos:definition "The number assigned to the floor of type specified in buildingLevelType."@en ;
    skos:historyNote "From Queensland address data." ;
    skos:inScheme cs: ;
    skos:prefLabel "Building Level Number"@en ;
    skos:topConceptOf cs: ;
.

apt:buildingLevelNumberSuffix
    a skos:Concept ;
    rdfs:isDefinedBy cs: ;
    skos:definition "Alphabetical suffix to buildingLevelNumber. Requires buildingLevelNumber to have a value."@en ;
    skos:historyNote "From Queensland address data." ;
    skos:inScheme cs: ;
    skos:prefLabel "Building Level Number Suffix"@en ;
    skos:topConceptOf cs: ;
.

apt:buildingLevelType
    a skos:Concept ;
    rdfs:isDefinedBy cs: ;
    skos:definition "The type of floor or level, within a multi-storey building. One of the concepts from https://linked.data.gov.au/def/building-level-types."@en ;
    skos:historyNote "From Queensland address data." ;
    skos:inScheme cs: ;
    skos:prefLabel "Building Level Type"@en ;
    skos:topConceptOf cs: ;
.

apt:countryName
    a skos:Concept ;
    rdfs:isDefinedBy cs: ;
    skos:definition "The country name from ISO-3166. One of the concepts from http://linked.data.gov.au/def/countries."@en ;
    skos:historyNote "Original concept of country name from ISO19160-1." ;
    skos:inScheme cs: ;
    skos:prefLabel "Country"@en ;
    skos:topConceptOf cs: ;
.

apt:geographicName
    a skos:Concept ;
    rdfs:isDefinedBy cs: ;
    skos:definition "An official geographic name or culturally accepted common usage name for an addressable object of a suitable type from https://linked.data.gov.au/def/address-geographic-name-types."@en ;
    skos:historyNote "From Queensland address data. This replaces several ISO19160-1 & GNAF values as this reference can be used to any category of Geographical Object with the name for the object used within the address this part is part of. Geographical Object categories are assgned to the Geographical Object, not any part of this address part or the address it is part of." ;
    skos:inScheme cs: ;
    skos:prefLabel "Geographic Name"@en ;
    skos:topConceptOf cs: ;
.

apt:buildingName
    a skos:Concept ;
    rdfs:isDefinedBy cs: ;
    skos:definition "The official name or culturally accepted common usage name for a building as defined by https://linked.data.gov.au/def/go-categories/building."@en ;
    skos:historyNote "From Queensland address data." ;
    skos:inScheme cs: ;
    skos:prefLabel "Building Name"@en ;
    skos:topConceptOf cs: ;
.

apt:indigenousCountryName
    a skos:Concept ;
    rdfs:isDefinedBy cs: ;
    skos:definition "A name used in association with traditional lands or water to which Aboriginal peoples are ancestrally and spiritually connected."@en ;
    skos:historyNote "From Queensland address data." ;
    skos:inScheme cs: ;
    skos:prefLabel "Indigenous Country Name"@en ;
    skos:topConceptOf cs: ;
.

apt:locality
    a skos:Concept ;
    rdfs:isDefinedBy cs: ;
    skos:definition "A reference to a Locality object. A bounded area distinguished for its community and/or landscape characteristics: in metropolitan areas it is commonly referred to as a ‘suburb’; it provides an official reference point for addressing purposes. Defined by https://linked.data.gov.au/def/go-categories/locality."@en ;
    skos:historyNote "Original concept of locality name from ISO19160-1." ;
    skos:inScheme cs: ;
    skos:prefLabel "Locality"@en ;
    skos:topConceptOf cs: ;
.

apt:postcode
    a skos:Concept ;
    rdfs:isDefinedBy cs: ;
    skos:definition "The relevant postcode allocated by Australia Post to the locality utilised in the address."@en ;
    skos:historyNote "Original concept of postcode from ISO19160-1." ;
    skos:inScheme cs: ;
    skos:prefLabel "Postcode"@en ;
    skos:topConceptOf cs: ;
.

apt:propertyName
    a skos:Concept ;
    rdfs:isDefinedBy cs: ;
    skos:definition "The official name or culturally accepted common usage name for a property, including a rural or agricultural property, as defined by https://linked.data.gov.au/def/go-categories/property."@en ;
    skos:historyNote "From Queensland address data." ;
    skos:inScheme cs: ;
    skos:prefLabel "Property Name"@en ;
    skos:topConceptOf cs: ;
.

apt:road
    a skos:Concept ;
    rdfs:isDefinedBy cs: ;
    skos:altLabel "Street"@en ;
    skos:broader apt:thoroughfareName ;
    skos:definition "The name of the road from which the address site is accessed. A reference to a road object."@en ;
    skos:historyNote "From Queensland address data." ;
    skos:inScheme cs: ;
    skos:prefLabel "Road"@en ;
.

apt:stateOrTerritory
    a skos:Concept ;
    rdfs:isDefinedBy cs: ;
    skos:altLabel
        "State"@en ,
        "Territory"@en ;
    skos:definition "Any of the sixteen major divisions which contribute to the federated Commonwealth of Australia. One of the concepts from https://linked.data.gov.au/dataset/asgsed3/STE that indicates the state or territory in which the address site is located."@en ;
    skos:historyNote "Original concept of administrative area name from ISO19160-1." ;
    skos:inScheme cs: ;
    skos:prefLabel "State Or Territory"@en ;
    skos:topConceptOf cs: ;
.

apt:subaddressNumber
    a skos:Concept ;
    rdfs:isDefinedBy cs: ;
    skos:definition "The number assigned to a subaddress of that of type specified in subaddressType."@en ;
    skos:historyNote "Replaces GNAF’s flatNumber." ;
    skos:inScheme cs: ;
    skos:prefLabel "Subaddress Number"@en ;
    skos:topConceptOf cs: ;
.

apt:subaddressNumberSuffix
    a skos:Concept ;
    rdfs:isDefinedBy cs: ;
    skos:definition "Alphabetical suffix to subaddressNumber. Requires subaddressNumber to have a value."@en ;
    skos:historyNote "Replaces GNAF’s flatNumberSuffix." ;
    skos:inScheme cs: ;
    skos:prefLabel "Subaddress Number Suffix"@en ;
    skos:topConceptOf cs: ;
.

apt:subaddressType
    a skos:Concept ;
    rdfs:isDefinedBy cs: ;
    skos:definition "The type that distinguishes the separately identifiable portion of the address within a building, complex or marina. One of the concepts from https://linked.data.gov.au/def/subaddress-types."@en ;
    skos:historyNote "Replaces GNAF’s flatTypeCode." ;
    skos:inScheme cs: ;
    skos:prefLabel "Subaddress Type"@en ;
    skos:topConceptOf cs: ;
.

apt:waterFeature
    a skos:Concept ;
    rdfs:isDefinedBy cs: ;
    skos:broader apt:thoroughfareName ;
    skos:definition "The name of the water feature from which the address site is accessed. A reference to  Water Feature object."@en ;
    skos:historyNote "From Queensland address data." ;
    skos:inScheme cs: ;
    skos:prefLabel "Water Feature Name"@en ;
.

apt:thoroughfareName
    a skos:Concept ;
    rdfs:isDefinedBy cs: ;
    skos:definition "The name of the thoroughfare from which the address site is accessed."@en ;
    skos:historyNote "Original concept of thoroughfare name from ISO19160-1." ;
    skos:inScheme cs: ;
    skos:narrower
        apt:road ,
        apt:waterFeature ;
    skos:prefLabel "Thoroughfare Name"@en ;
    skos:topConceptOf cs: ;
.

cs:
    a skos:ConceptScheme ;
    owl:versionIRI apt:None ;
    skos:definition "This vocabulary describes the components for addresses. It is an extended version of ISO19160-1's Address Component Type vocabulary. "@en ;
    skos:hasTopConcept
        apt:addressNumberFirst ,
        apt:addressNumberFirstSuffix ,
        apt:addressNumberLast ,
        apt:addressNumberLastSuffix ,
        apt:buildingLevelNumber ,
        apt:buildingLevelNumberSuffix ,
        apt:buildingLevelType ,
        apt:countryName ,
        apt:geographicName ,
        apt:buildingName ,
        apt:indigenousCountryName ,
        apt:locality ,
        apt:postcode ,
        apt:propertyName ,
        apt:stateOrTerritory ,
        apt:subaddressNumber ,
        apt:subaddressNumberSuffix ,
        apt:subaddressType ,
        apt:thoroughfareName ;
    skos:historyNote "This vocabulary is an extended version of ISO19160-1's Address Component Type vocabulary, with additional components provided by Queensland."@en ;
    skos:prefLabel "Address Part Types"@en ;
    prov:qualifiedAttribution
        [
            dcat:hadRole isoroles:custodian ;
            prov:agent
                [
                    a schema:Person ;
                    schema:email ""^^xsd:anyURI ;
                    schema:name "Icsm" ;
                ] ;
        ] ;
    schema:creator
        [
            a schema:Organization ;
            schema:name "Department Of Resources" ;
            schema:url ""^^xsd:anyURI ;
        ] ;
    dcterms:created "2024-09-18"^^xsd:date ;
	dcterms:modified "2024-09-18"^^xsd:date ;
    schema:keywords "Address" ;
    schema:publisher
        [
            a schema:Organization ;
            schema:name "Icsm" ;
            schema:url ""^^xsd:anyURI ;
        ] ;
    schema:version "None" ;
.

