PREFIX : <https://linked.data.gov.au/def/fsdf/themes/>
PREFIX agldwgstatus: <https://linked.data.gov.au/def/reg-statuses/>
PREFIX cs: <https://linked.data.gov.au/def/fsdf/themes>
PREFIX dcterms: <http://purl.org/dc/terms/>
PREFIX droles: <https://linked.data.gov.au/def/data-roles/>
PREFIX fsdf: <https://linked.data.gov.au/def/fsdf/>
PREFIX owl: <http://www.w3.org/2002/07/owl#>
PREFIX prov: <http://www.w3.org/ns/prov#>
PREFIX reg: <http://purl.org/linked-data/registry#>
PREFIX rdfs: <http://www.w3.org/2000/01/rdf-schema#>
PREFIX sdo: <https://schema.org/>
PREFIX skos: <http://www.w3.org/2004/02/skos/core#>
PREFIX xsd: <http://www.w3.org/2001/XMLSchema#>

:airports-and-airfields
    a
        skos:Concept ,
        fsdf:Theme ;
    rdfs:isDefinedBy cs: ;
    skos:broader :transport ;
    skos:definition "Airports and airfields are defined by the International Civil Aviation Organisation as defined points or areas on land or water intended to be used either wholly or in part for the arrival, departure and surface movement of aircraft. ICAO uses the term aerodromes. Airports are generally facilities that have commercial passenger and cargo facilities."@en ;
    skos:inScheme cs: ;
    skos:prefLabel "Airports and Airfields"@en ;
.

:australian-collaborative-land-use-and-management-program
    a
        skos:Concept ,
        fsdf:Theme ;
    rdfs:isDefinedBy cs: ;
    skos:broader :land-cover-and-land-use ;
    skos:definition """Land use mapping in Australia is coordinated by the Australian Collaborative Land Use and Management Program (ACLUMP), a consortium of state and national agencies. Mapping is conducted at two scales: national scale and catchment scale. Land use is mapped according to the nationally agreed Australian Land Use and Management (ALUM) Classification, a three-tier hierarchical structure.

* National scale land use mapping is produced by ABARES using coarse-scale satellite data (pixel size of 1.1 square kilometres), ABS agricultural statistics and ground control point data for the agricultural land uses and various other digital maps, including the finer resolution catchment scale land use data, for the non-agricultural land uses. National scale (1:2 500 000) land use datasets have been compiled for 1992-93, 1993-94, 1996-97, 1998-99, 2000-01, 2001-02, 2005-06, 2010-11.
* Catchment scale land use mapping is produced by the state and territory agencies using land tenure and other types of land use data, fine-scale satellite data and information collected in the field. The operational scale of catchment scale land use mapping varies according to the intensity of land-use activities and landscape context. Mapping ranges from fine scale (1:10 000 to 1:25 000) for irrigated and peri-urban areas to coarser scales for cropping regions (1:100 000) and for the semi-arid and arid pastoral zone (1:250 000). Catchment scale mapping is compiled into a national raster (50m) dataset by ABARES as new datasets are available from the jurisdictions.
"""@en ;
    skos:inScheme cs: ;
    skos:prefLabel "Australian Collaborative Land Use and Management Program"@en ;
.

:australian-electoral-boundaries
    a
        skos:Concept ,
        fsdf:Theme ;
    rdfs:isDefinedBy cs: ;
    skos:broader :administrative-boundaries ;
    skos:definition """The geographical boundaries that divide the area of interest for the purposes of an election or referendum held under the Commonwealth Electoral Act, 1918.

Australian Electoral boundaries are a collection of legislative, political boundaries sourced from Federal, State and Territory authorities:

* Federal electoral boundaries
* State electoral boundaries
* Local government wards"""@en ;
    skos:inScheme cs: ;
    skos:prefLabel "Australian Electoral Boundaries"@en ;
.

:australian-statistical-geographical-standard-boundaries
    a
        skos:Concept ,
        fsdf:Theme ;
    rdfs:isDefinedBy cs: ;
    skos:broader :administrative-boundaries ;
    skos:definition """The geographical boundaries that divide the area of interest on which the statistics are collected for purposes under the Australian Bureau of Statistics Act, 1975.

The Australian Statistical Geography Standard (ASGS) is the Australian Bureau of Statistics' geographical framework.

The ASGS brings all the regions used by the ABS to output data under the one umbrella. They are divided into two broad categories:

    ABS Structures, those regions which are defined and maintained by the ABS.
    Non-ABS Structures, those regions defined and maintained by other organisations, but for which the ABS supplies data.

The ABS Structures are a hierarchy of regions developed for the release of ABS statistical information. Their main components are listed below:

    Australia
    State/Territory
    Statistical Areas Level 4
    Statistical Areas Level 3
    Statistical Areas Level 2
    Statistical Areas Level 1
    Mesh blocks"""@en ;
    skos:inScheme cs: ;
    skos:prefLabel "Australian Statistical Geographical Standard Boundaries"@en ;
.

:catchment-boundaries
    a
        skos:Concept ,
        fsdf:Theme ;
    rdfs:isDefinedBy cs: ;
    skos:broader :water ;
    skos:definition "The National Catchments is a topologically consistent and hierologically enforced stream flow aggregation of boundaries"@en ;
    skos:inScheme cs: ;
    skos:prefLabel "Catchment Boundaries"@en ;
.

:dynamic-land-cover
    a
        skos:Concept ,
        fsdf:Theme ;
    rdfs:isDefinedBy cs: ;
    skos:broader :land-cover-and-land-use ;
    skos:definition "The Dynamic Land Cover Dataset is a nationally consistent and thematically comprehensive land cover reference for Australia. Dynamic Land Cover Dataset provides an 8 year synoptic overview of land cover at 250 metre resolution for the Australian continent between April 2000 and April 2008."@en ;
    skos:inScheme cs: ;
    skos:prefLabel "Dynamic Land Cover"@en ;
.

:flow-direction-grid
    a
        skos:Concept ,
        fsdf:Theme ;
    rdfs:isDefinedBy cs: ;
    skos:broader :water ;
    skos:definition "The Flow Direction Grid is a regular grid of surface flow directions accompanying the GEODATA 9 Second Digital Elevation Model (DEM) Version 3. It ascribes to each DEM point one of eight cardinal directions (E, SE, S, SW, W, NW, N, NE) denoting the direction of surface flow from each grid point to one of its eight immediate neighbours."@en ;
    skos:inScheme cs: ;
    skos:prefLabel "Flow Direction Grid"@en ;
.

:forests-of-australia
    a
        skos:Concept ,
        fsdf:Theme ;
    rdfs:isDefinedBy cs: ;
    skos:broader :land-cover-and-land-use ;
    skos:definition """Forests of Australia (2018) is a continental spatial ​dataset of forest extent, by national forest categories and types, assembled for [Australia's State of the Forests Report 2018](http://www.agriculture.gov.au/abares/forestsaustralia/Pages/SOFR2018/sofr-2018.aspx). It was developed from multiple forest, vegetation and land cover data inputs, including contributions from Australian, state and territory government agencies and external sources.
​
A forest is defined in this dataset as _"An area, incorporating all living and non-living components, that is dominated by trees having usually a single stem and a mature or potentially mature stand height exceeding two metres and with existing or potential crown cover of overstorey​ strata about equal to or greater than 20 per cent. This includes Australia's diverse native forests and commercial plantations, regardless of age. It is also sufficiently broad to encompass areas of trees that are sometimes described as woodlands"_.

The dataset was compiled by the Australian Bureau of Agricultural and Resource Economics and Sciences (ABARES) for the [National Forest Inventory](http://www.agriculture.gov.au/abares/forestsaustralia/Pages/Australia%27s-National-Forest-Inventory.aspx) (NFI), a collaborative partnership between the Australian and state and territory governments. The role of the NFI is to collate, integrate and communicate information on Australia's forests. States and territories agencies collect forest data using independent methods and at varying scales or resolutions. The NFI applies a national classification to state and territory data to allow seamless integration of these datasets. Multiple independent ​sources of external data are used to fill data gaps and improve the quality of the final data​set.

The NFI classifies forests into three national forest categories (Native forest, Commercial plantation, and Other forest) and then into various forest types. Commercial plantations presented in this dataset were sourced from the [National Plantation Inventory](http://www.agriculture.gov.au/abares/forestsaustralia/plantation-inventory-and-statistics) (NPI) spatial dataset (2016), also produced by ABARES. Another dataset produced by ABARES, the [Catchment scale Land Use and Management](http://www.agriculture.gov.au/abares/aclump/Pages/land-use/data-download.aspx) (CLUM) dataset (2016) was used to identify ​and mask out land uses that are inappropriate to map as forest.​"""@en ;
    skos:inScheme cs: ;
    skos:prefLabel "Forests of Australia"@en ;
.

:fractional-ground-cover
    a
        skos:Concept ,
        fsdf:Theme ;
    rdfs:isDefinedBy cs: ;
    skos:broader :land-cover-and-land-use ;
    skos:definition "The data represent the fractional cover of Photosynthetic Vegetation (PV), Non-Photosynthetic Vegetation (NPV) and Bare Soil (BS)."@en ;
    skos:inScheme cs: ;
    skos:prefLabel "Fractional Ground Cover"@en ;
.

:gazetteer-of-australia
    a
        skos:Concept ,
        fsdf:Theme ;
    rdfs:isDefinedBy cs: ;
    skos:broader :place-names ;
    skos:definition """A geographical index or dictionary of the names of cultural and physical features and their associated location in Australia.

These names can include approved, unapproved, commonly used, alternate and historical place names."""@en ;
    skos:inScheme cs: ;
    skos:prefLabel "Gazetteer of Australia"@en ;
.

:groundwater
    a
        skos:Concept ,
        fsdf:Theme ;
    rdfs:isDefinedBy cs: ;
    skos:broader :water ;
    skos:definition "Nationally consistent set of groundwater boundaries and properties including aquifer boundaries, geometry, salinity, yield and hydraulic conductivity. The Interim Aquifer Framework has been used to standardise the hydrogeological unit terminology for this dataset."@en ;
    skos:inScheme cs: ;
    skos:prefLabel "Groundwater"@en ;
.

:groundwater-bores
    a
        skos:Concept ,
        fsdf:Theme ;
    rdfs:isDefinedBy cs: ;
    skos:broader :water ;
    skos:definition "Nationally consistent set of groundwater bores (including monitoring, irrigation and commercial bores) and associated lithology, construction and hydrostratigraphy logs. The National Aquifer Framework has been used to standardise the hydrogeological unit terminology for this dataset."@en ;
    skos:inScheme cs: ;
    skos:prefLabel "Groundwater Bores"@en ;
.

:groundwater-dependent-ecosystems
    a
        skos:Concept ,
        fsdf:Theme ;
    rdfs:isDefinedBy cs: ;
    skos:broader :water ;
    skos:definition "Groundwater Dependent Ecosystems (GDE) is ecological and hydrogeological information on known groundwater dependent ecosystems and ecosystems that potentially use groundwater."@en ;
    skos:inScheme cs: ;
    skos:prefLabel "Groundwater Dependent Ecosystems (GDE)"@en ;
.

:high-spatial-resolution-low-temporal-coverage
    a
        skos:Concept ,
        fsdf:Theme ;
    rdfs:isDefinedBy cs: ;
    skos:broader :imagery ;
    skos:definition """These data sets have a spatial resolution of between 2.5-10 m and provide national coverage every quarter. They are primarily operated by Jurisdictions and/or commercial enterprises.

There are an increasing number of these sensors available for both satellite and airborne platforms and an ever-expanding range of applications that use them. The data derived from SPOT from 2005 to Present and ALOS from 2009/2010 is identified as the primary data within this data set."""@en ;
    skos:inScheme cs: ;
    skos:prefLabel "High Spatial Resolution (>2.5-10m) Low Temporal Coverage (>Quarterly)"@en ;
.

:hydrological-obstructions
    a
        skos:Concept ,
        fsdf:Theme ;
    rdfs:isDefinedBy cs: ;
    skos:broader :water ;
    skos:definition "Hydrological obstructions are man-made features that impact the water network either by obstruction, diversion or storage of water"@en ;
    skos:inScheme cs: ;
    skos:prefLabel "Hydrological Obstructions"@en ;
.

:jurisdictional-boundaries
    a
        skos:Concept ,
        fsdf:Theme ;
    rdfs:isDefinedBy cs: ;
    skos:broader :administrative-boundaries ;
    skos:definition """The agreed boundary separating the individual states and territories of Australia and bounded by the maritime boundary.

Jurisdictional boundaries are a collection of legislative, regulatory, political and general administrative boundaries sourced from Federal, State and Territory authorities.

* National boundary
* State/Territory boundary
* Local government areas
* Parishes
* Regions
* Suburbs"""@en ;
    skos:inScheme cs: ;
    skos:prefLabel "Jurisdictional Boundaries"@en ;
.

:land-parcel-boundaries
    a
        skos:Concept ,
        fsdf:Theme ;
    rdfs:isDefinedBy cs: ;
    skos:broader :land-parcel-and-property ;
    skos:definition "The Land Parcel dataset is a data aggregation sourced from the jurisdictions which depicts national and accurate land and strata based information including parcels representing easements, roads, crossing, rail and water."@en ;
    skos:inScheme cs: ;
    skos:prefLabel "Land Parcel Boundaries"@en ;
.

:land-tenure
    a
        skos:Concept ,
        fsdf:Theme ;
    rdfs:isDefinedBy cs: ;
    skos:broader :land-parcel-and-property ;
    skos:definition "Aligns land tenure classifications to cadastral parcel identifiers, requiring the use of the CadLite® dataset to visualise or spatially analyse the Land Tenure dataset."@en ;
    skos:inScheme cs: ;
    skos:prefLabel "Land Tenure"@en ;
.

:low-resolution-high-temporal-coverage
    a
        skos:Concept ,
        fsdf:Theme ;
    rdfs:isDefinedBy cs: ;
    skos:broader :imagery ;
    skos:definition """These data sets have a spatial resolution of no closer than 80 m and are collected on a close to weekly basis.

The AVHRR and MODIS sensors service most Australian needs for low resolution optical data. Data is derived from MODIS, AVHRR, VIIRS missions and includes the following spectral ranges, VIS, NIR, SWIR.
"""@en ;
    skos:inScheme cs: ;
    skos:prefLabel "Low Resolution (>80m) High Temporal Coverage (>weekly)"@en ;
.

:maritime-jurisdiction-boundaries
    a
        skos:Concept ,
        fsdf:Theme ;
    rdfs:isDefinedBy cs: ;
    skos:broader :administrative-boundaries ;
    skos:definition """The delineation of the baseline from which the outer limits of the various maritime zones are measured as set out in the UN Convention of the Law of the Sea (UNCLOS) and Seas and Submerged Lands Act, 1973.

* Territorial Sea Baseline
* Territorial Sea (12 nautical mile limit)
* Contiguous Zone (24 nautical mile limit)
* Exclusive Economic Zone (200 nautical mile limit)
* Australian Fishing Zone"""@en ;
    skos:inScheme cs: ;
    skos:prefLabel "Maritime Jurisdiction Boundaries"@en ;
.

:medium-resolution-medium-temporal
    a
        skos:Concept ,
        fsdf:Theme ;
    rdfs:isDefinedBy cs: ;
    skos:broader :imagery ;
    skos:definition """These data sets have a spatial resolution between 10–80 m and are collected on a weekly to monthly basis. They are the most commonly used category of imagery data.

For several decades the Landsat series of satellites have provided the majority of medium resolution optical imagery for operational programs in Australia. Data is derived from MSS, TM, ETM+, Aster, OLI, Sentinel-2 MSI missions and includes the following spectral ranges, VIS, NIR, SWIR, PAN.

Medium resolution optical sensors have traditionally been operated for public good, although the number of commercial sensors is increasing."""@en ;
    skos:inScheme cs: ;
    skos:prefLabel "Medium Resolution (>10-80m) Medium Temporal"@en ;
.

:national-crossings
    a
        skos:Concept ,
        fsdf:Theme ;
    rdfs:isDefinedBy cs: ;
    skos:broader :transport ;
    skos:definition "Crossings are structures built to facilitate the movement over, under or through another physical feature. In the Transport Theme, crossings include bridges, tunnels, fords, culverts and boardwalks."@en ;
    skos:inScheme cs: ;
    skos:prefLabel "National Crossings"@en ;
.

:national-digital-elevation-and-depth-model
    a
        skos:Concept ,
        fsdf:Theme ;
    rdfs:isDefinedBy cs: ;
    skos:broader :elevation-and-depth ;
    skos:definition """The one arc second (~30m) DEMs provide a nationally consistent, medium resolution dataset essential for national and regional scale analysis using the best available source data. It comprises data derived from the Shuttle Radar Topography Mission (SRTM) and LiDAR where available.

Bathymetry is the study and mapping of sea floor topography. It involves obtaining measurements of the depth of the ocean and is equivalent to mapping the topography on land.
Such measurements can be made using:

* Multibeam (swath) echosounders
* Airborne laser measurements (LADS)
* Derived depths from satellite remote sensing
* Singlebeam echosounders"""@en ;
    skos:inScheme cs: ;
    skos:prefLabel "National Digital Elevation and Depth Model"@en ;
.

:national-geospatial-reference-system
    a
        skos:Concept ,
        fsdf:Theme ;
    rdfs:isDefinedBy cs: ;
    skos:broader :positioning ;
    skos:definition """The CORSnet is a network of permanent global navigation satellite systems (GNSS) continuously operating reference stations (CORS) providing DGPS, RTK and RINEX data 24/7 to enable users to achieve sub-metre positional accuracy.

Expanding the CORSnet network of global navigation satellite systems (GNSS) continuously operating reference stations (CORS) providing DGPS, RTK and RINEX data 24/7 to enable users to achieve sub-metre positional accuracy."""@en ;
    skos:inScheme cs: ;
    skos:prefLabel "National Geospatial Reference System"@en ;
.

:national-topographic-data
    a
        skos:Concept ,
        fsdf:Theme ;
    rdfs:isDefinedBy cs: ;
    skos:broader :land-cover-and-land-use ;
    skos:definition """National Topographic data – principally referred to in this document as Geodata Topo 250K Series 3 – is a nationally consistent representation of natural and built environment features on the earth's surface for Australia excluding external territories. The data is thematically ordered and includes the following datasets containing up to 92 different feature classes:

* Culture
* Drainage
* Elevation
* Framework
* Habitation
* Transport
    Utility
    Vegetation"""@en ;
    skos:inScheme cs: ;
    skos:prefLabel "National Topographic Data"@en ;
.

:national-vegetation-information-system
    a
        skos:Concept ,
        fsdf:Theme ;
    rdfs:isDefinedBy cs: ;
    skos:broader :land-cover-and-land-use ;
    skos:definition "The NVIS framework was developed to enable the compilation of a nationally consistent vegetation dataset from data collected by states and territories. It provides a comprehensive means of describing and representing vegetation information based on establishing relationships between structural and floristic data. The NVIS Information Hierarchy is a system for describing the structural and floristic patterns of groups of plants in the landscape. Collectively, the different levels in the classification provide a description of vegetation that can be directly related to precise spatial areas as a vegetation map."@en ;
    skos:inScheme cs: ;
    skos:prefLabel "National Vegetation Information System"@en ;
.

:native-title-boundaries
    a
        skos:Concept ,
        fsdf:Theme ;
    rdfs:isDefinedBy cs: ;
    skos:broader :administrative-boundaries ;
    skos:definition """Mapping and spatial information play a key role in navigating native title.

Applications, Indigenous land use agreements, and determinations of native title are described geographically and mapped, similar to other interests in land and/or water.

Mapping enables people to gain an understanding of where these matters are in relation to other things, such as towns, roads, farms, mining tenements and local government areas.

Together with other information, maps are also used to notify interested parties about native title matters, enabling them to become involved in the process."""@en ;
    skos:inScheme cs: ;
    skos:prefLabel "Native Title Boundaries"@en ;
.

:navigation-aids-and-obstacles
    a
        skos:Concept ,
        fsdf:Theme ;
    rdfs:isDefinedBy cs: ;
    skos:broader :transport ;
    skos:definition "Location, height and description of infrastructure, markers or other devices on land which may aid travellers in determining their position or safe course."@en ;
    skos:inScheme cs: ;
    skos:prefLabel "Navigation Aids and Obstacles"@en ;
.

:railways-and-railway-stations
    a
        skos:Concept ,
        fsdf:Theme ;
    rdfs:isDefinedBy cs: ;
    skos:broader :transport ;
    skos:definition "Railways are transportation systems using one or more rails to carry freight or passengers. Railway stations are recognised stopping places where goods, vehicles or passengers may be transferred from one form of transport to the rail network, and vice versa. Railway stations can also include what are now called “intermodal transfer stations”."@en ;
    skos:inScheme cs: ;
    skos:prefLabel "Railways and Railway Stations"@en ;
.

:roads
    a
        skos:Concept ,
        fsdf:Theme ;
    rdfs:isDefinedBy cs: ;
    skos:broader :transport ;
    skos:definition "Roads are defined paths for the transfer of goods or movement of vehicles, people or animals. Unlike Railways, Roads do not have fixed tracks. The Roads dataset includes cycleways, foot tracks and ferry routes."@en ;
    skos:inScheme cs: ;
    skos:prefLabel "Roads"@en ;
.

:surface-hydrology
    a
        skos:Concept ,
        fsdf:Theme ;
    rdfs:isDefinedBy cs: ;
    skos:broader :water ;
    skos:definition "The Surface Hydrology dataset provides a set of related feature classes to be used as the basis of the production of consistent hydrological information. This dataset contains a geometric representation of the (major) surface water features of Australia. Primarily, these are natural surface hydrology features, but the dataset also contains some artificial features (notably reservoirs, canals and other hydrographic features)."@en ;
    skos:inScheme cs: ;
    skos:prefLabel "Surface Hydrology"@en ;
.

:the-geocoded-national-address-file
    a
        skos:Concept ,
        fsdf:Theme ;
    rdfs:isDefinedBy cs: ;
    skos:broader :geocoded-addressing ;
    skos:definition "Validates the captured address and makes it possible to verify a physical address and locate its position."@en ;
    skos:inScheme cs: ;
    skos:prefLabel "The Geocoded National Address File"@en ;
.

:traffic-control-devices
    a
        skos:Concept ,
        fsdf:Theme ;
    rdfs:isDefinedBy cs: ;
    skos:broader :transport ;
    skos:definition "Traffic control devices are used to control, calm, slow or impede the movement of traffic. They include roundabouts, gates, stock grids, level crossings, tolls and barriers"@en ;
    skos:inScheme cs: ;
    skos:prefLabel "Traffic Control Devices"@en ;
.

:very-high-resolution-very-low-temporal-coverage
    a
        skos:Concept ,
        fsdf:Theme ;
    rdfs:isDefinedBy cs: ;
    skos:broader :imagery ;
    skos:definition """An orthophoto is an aerial photograph geometrically corrected (“orthorectified”) to ensure the scale is uniform: the photo has the same lack of distortion as a map. Unlike an uncorrected aerial photograph, an orthophotograph can be used to measure true distances, because it is an accurate representation of the Earth’s surface, having been adjusted for topographic relief, lens distortion, and camera tilt. The image has been corrected to ensure that horizontal scale is constant

These data sets have a spatial resolution of 2.5m or closer and are primarily operated by Jurisdictions and/or commercial enterprises.

There are an increasing number of these sensors available for both satellite and airborne platforms and an ever-expanding range of applications that use them."""@en ;
    skos:inScheme cs: ;
    skos:prefLabel "Very High Resolution (<2.5 m) Very Low Temporal Coverage (>annual)"@en ;
.

:buildings-and-settlements
    a
        skos:Concept ,
        fsdf:Theme ;
    dcterms:source "https://ggim.un.org/documents/E-C20-2018-7-Add_1-Global-fundamental-geospatial-data-themes.pdf"^^xsd:anyURI ;
    rdfs:isDefinedBy cs: ;
    skos:definition "A building refers to any roofed structure permanently constructed or erected on its site, for the protection of humans, animals, things, or the production of economic goods. Settlements are collections of buildings and associated features where a community carries out socio-economic activities."@en ;
    skos:inScheme cs: ;
    skos:prefLabel "Buildings and Settlements"@en ;
    skos:topConceptOf cs: ;
.

:geology-and-soils
    a
        skos:Concept ,
        fsdf:Theme ;
    dcterms:source "https://ggim.un.org/documents/E-C20-2018-7-Add_1-Global-fundamental-geospatial-data-themes.pdf"^^xsd:anyURI ;
    rdfs:isDefinedBy cs: ;
    skos:definition "Geology is the composition and properties of geologic materials (rocks and sediments) underground and outcropping at the Earth’s surface. It includes bedrock, aquifers, geomorphology for land and marine environments, mineral resources and overlying soils. Soils are the upper part of the Earth’s crust, formed by mineral particles, organic matter, water, air, and living organisms."@en ;
    skos:inScheme cs: ;
    skos:prefLabel "Geology and Soils"@en ;
    skos:topConceptOf cs: ;
.

:physical-infrastructure
    a
        skos:Concept ,
        fsdf:Theme ;
    dcterms:source "https://ggim.un.org/documents/E-C20-2018-7-Add_1-Global-fundamental-geospatial-data-themes.pdf"^^xsd:anyURI ;
    rdfs:isDefinedBy cs: ;
    skos:definition "The Physical Infrastructure theme includes industrial & utility facilities, and the service delivery facilities associated with administrative & social governmental services such as public administrations, utilities, transport, civil protection, schools and hospitals."@en ;
    skos:inScheme cs: ;
    skos:prefLabel "Physical Infrastructure"@en ;
    skos:topConceptOf cs: ;
.

:population-distributions
    a
        skos:Concept ,
        fsdf:Theme ;
    dcterms:source "https://ggim.un.org/documents/E-C20-2018-7-Add_1-Global-fundamental-geospatial-data-themes.pdf"^^xsd:anyURI ;
    rdfs:isDefinedBy cs: ;
    skos:definition "The Population Distribution theme covers the geographical distribution of people, including population characteristics."@en ;
    skos:inScheme cs: ;
    skos:prefLabel "Population Distributions"@en ;
    skos:topConceptOf cs: ;
.

<https://linked.data.gov.au/org/ga>
    a sdo:Organization ;
    sdo:name "Geoscience Australia" ;
    sdo:url "https://www.ga.gov.au"^^xsd:anyURI ;
.

<https://linked.data.gov.au/org/icsm>
    a sdo:Organization ;
    sdo:name "Intergovernmental Committee on Surveying & Mapping" ;
    sdo:url "https://www.icsm.gov.au/"^^xsd:anyURI ;
.

:elevation-and-depth
    a
        skos:Concept ,
        fsdf:Theme ;
    rdfs:isDefinedBy cs: ;
    skos:definition "The Elevation and Depth theme focusses on foundation datasets which measure the Earth’s surface (wet or dry) above or below a vertical datum to obtain either the height of the land or a bathymetric depth."@en ;
    skos:inScheme cs: ;
    skos:prefLabel "Elevation and Depth"@en ;
    skos:topConceptOf cs: ;
.

:geocoded-addressing
    a
        skos:Concept ,
        fsdf:Theme ;
    rdfs:isDefinedBy cs: ;
    skos:definition "The Geocoded Addressing theme focusses on the connection between a physical address with location information which shows up as a 'place' or 'spot' on the Earth. This makes the information able to be mapped and connected to other location information. An address is a structured label usually containing a property number, a road name and a locality name."@en ;
    skos:inScheme cs: ;
    skos:prefLabel "Geocoded Addressing"@en ;
    skos:topConceptOf cs: ;
.

:place-names
    a
        skos:Concept ,
        fsdf:Theme ;
    rdfs:isDefinedBy cs: ;
    skos:definition "The Place Names theme focuses on foundation datasets for the names of cultural and physical features and their location and extent."@en ;
    skos:inScheme cs: ;
    skos:prefLabel "Place Names"@en ;
    skos:topConceptOf cs: ;
.

:positioning
    a
        skos:Concept ,
        fsdf:Theme ;
    rdfs:isDefinedBy cs: ;
    skos:definition "The positioning theme is Australia's spatial referencing system. The positioning service defined under this theme includes the coordinates and their uncertainty of all location-based data promulgated from or related to, the Australian Fiducial Network (AFN) and the defining Australian Height Datum tide gauge stations."@en ;
    skos:inScheme cs: ;
    skos:prefLabel "Positioning"@en ;
    skos:topConceptOf cs: ;
.

:land-parcel-and-property
    a
        skos:Concept ,
        fsdf:Theme ;
    rdfs:isDefinedBy cs: ;
    skos:definition "The Land Parcel and Property theme focusses on foundation datasets for the land boundary system. The term Land Parcel and Property can be interchangeable with cadastral, land administration and property systems. Land Parcel and Property contains a record of interest in land."@en ;
    skos:inScheme cs: ;
    skos:prefLabel "Land Parcel and Property"@en ;
    skos:topConceptOf cs: ;
.

:imagery
    a
        skos:Concept ,
        fsdf:Theme ;
    rdfs:isDefinedBy cs: ;
    skos:definition "The Imagery theme focuses on foundation data which captures images of the Earths surface, from many different sensors and cameras. This data is often the base layer over which many other datasets are used."@en ;
    skos:inScheme cs: ;
    skos:prefLabel "Imagery"@en ;
    skos:topConceptOf cs: ;
.

:administrative-boundaries
    a
        skos:Concept ,
        fsdf:Theme ;
    rdfs:isDefinedBy cs: ;
    skos:definition "The Administrative Boundaries theme focusses on foundation datasets which define the spatial extent of legislative jurisdictions and regulatory, electoral, statistical and maritime geographic areas"@en ;
    skos:inScheme cs: ;
    skos:prefLabel "Administrative Boundaries"@en ;
    skos:topConceptOf cs: ;
.

:land-cover-and-land-use
    a
        skos:Concept ,
        fsdf:Theme ;
    rdfs:isDefinedBy cs: ;
    skos:definition "The Land cover and Land Use theme focusses on foundation datasets for Land Cover and Land Use. Both land cover/use are often very interrelated datasets. Land cover shows the natural cover on the Earth's surface including trees, shrubs, grasses, soils, exposed rocks and water bodies; as well as human elements such as plantations, crops and built environments; Land Use refers to the ways in which land cover is used by humans (e.g. residential, industrial, commercial, agricultural, forestry, recreational)."@en ;
    skos:inScheme cs: ;
    skos:prefLabel "Land Cover and Land Use"@en ;
    skos:topConceptOf cs: ;
.

:transport
    a
        skos:Concept ,
        fsdf:Theme ;
    rdfs:isDefinedBy cs: ;
    skos:definition "The Transport theme focuses on foundation datasets for moving people, goods and freight, and other services from one location to another."@en ;
    skos:inScheme cs: ;
    skos:prefLabel "Transport"@en ;
    skos:topConceptOf cs: ;
.

:water
    a
        skos:Concept ,
        fsdf:Theme ;
    rdfs:isDefinedBy cs: ;
    skos:definition "The Water theme focuses on foundation datasets for surface and groundwater and excludes atmospheric, industrial or oceanic water processes."@en ;
    skos:inScheme cs: ;
    skos:prefLabel "Water"@en ;
    skos:topConceptOf cs: ;
.

cs:
    a skos:ConceptScheme ;
    dcterms:provenance "This vocabulary was generated from the FSDF LINK website which containes all this information in non-Semantic Web but highly structured, form" ;
    owl:versionInfo "1.0"^^xsd:string ;
    reg:status agldwgstatus:stable ;
    skos:definition "This FSDF Themes vocabulary is the taxonomy of dataset themes implemented by the [ANZLIC - The Spatial  Information Council](https://www.anzlic.gov.au)'s' Foundation Spatial Data Framework (FSDF) project which is \"a common reference for the assembly and maintenance of Australian and New Zealand foundation level spatial data\"" ;
    skos:hasTopConcept
        :administrative-boundaries ,
        :buildings-and-settlements ,
        :elevation-and-depth ,
        :geocoded-addressing ,
        :geology-and-soils ,
        :imagery ,
        :land-cover-and-land-use ,
        :land-parcel-and-property ,
        :physical-infrastructure ,
        :place-names ,
        :population-distributions ,
        :positioning ,
        :transport ,
        :water ;
    skos:historyNote "This vocabulary was developed by Geoscience Australia for ICSM vocabulary testing work in 2021" ;
    skos:prefLabel "FSDF Themes" ;
    dcterms:creator <https://linked.data.gov.au/org/ga> ;
    dcterms:created "2021-04-21"^^xsd:date ;
    dcterms:modified "2021-04-21"^^xsd:date ;
    sdo:license <http://purl.org/NET/rdflicense/cc-by4.0> ;
    dcterms:publisher <https://linked.data.gov.au/org/icsm> ;
    prov:qualifiedAttribution
        [
            prov:hadRole droles:custodian ;
            prov:agent <https://linked.data.gov.au/org/icsm>
        ] ;
.
