PREFIX : <https://linked.data.gov.au/def/gn-statuses/>
PREFIX cs: <https://linked.data.gov.au/def/gn-statuses>
PREFIX agldwgstatus: <https://linked.data.gov.au/def/reg-statuses/>
PREFIX dcat: <http://www.w3.org/ns/dcat#>
PREFIX dcterms: <http://purl.org/dc/terms/>
PREFIX isoroles: <http://def.isotc211.org/iso19115/-1/2018/CitationAndResponsiblePartyInformation/code/CI_RoleCode/>
PREFIX owl: <http://www.w3.org/2002/07/owl#>
PREFIX prov: <http://www.w3.org/ns/prov#>
PREFIX rdfs: <http://www.w3.org/2000/01/rdf-schema#>
PREFIX reg: <http://purl.org/linked-data/registry#>
PREFIX skos: <http://www.w3.org/2004/02/skos/core#>
PREFIX xsd: <http://www.w3.org/2001/XMLSchema#>


:historical
    a skos:Concept ;
    rdfs:isDefinedBy cs: ;
    skos:definition "The name has been used historically and perhaps currently but is not an official name"@en ;
    skos:historyNote "Taken from the Place Names Ontology but with a definition added here" ;
    skos:inScheme cs: ;
    skos:prefLabel "Historical"@en ;
    skos:topConceptOf cs: ;
.

:indigenous
    a skos:Concept ;
    rdfs:isDefinedBy cs: ;
    skos:definition "The name is used by indigenous communities"@en ;
    skos:historyNote "New in this vocabulary" ;
    skos:inScheme cs: ;
    skos:prefLabel "Indigenous"@en ;
    skos:topConceptOf cs: ;
.

:informal
    a skos:Concept ;
    rdfs:isDefinedBy cs: ;
    skos:definition "The name is used but it is not official"@en ;
    skos:historyNote "Taken from the Place Names Ontology but with a definition added here" ;
    skos:inScheme cs: ;
    skos:prefLabel "Informal"@en ;
    skos:topConceptOf cs: ;
.

:official
    a skos:Concept ;
    rdfs:isDefinedBy cs: ;
    skos:definition "The name has been sanctioned by an authoritative institution"@en ;
    skos:historyNote "Taken from the Place Names Ontology but with a definition added here" ;
    skos:inScheme cs: ;
    skos:prefLabel "Official"@en ;
    skos:topConceptOf cs: ;
.

:retired
    a skos:Concept ;
    rdfs:isDefinedBy cs: ;
    skos:definition "The name is official but is now no longer to be used"@en ;
    skos:historyNote "Taken from the Place Names Ontology but with a definition added here" ;
    skos:inScheme cs: ;
    skos:prefLabel "Retired"@en ;
    skos:broader :official ;
.

:released
    a skos:Concept ;
    rdfs:isDefinedBy cs: ;
    skos:definition "The name is official but is no longer to be used and the name is available for other use"@en ;
    skos:historyNote "Taken from the Place Names Ontology but with a definition added here" ;
    skos:inScheme cs: ;
    skos:prefLabel "Released"@en ;
    skos:broader :official ;
.

:published
    a skos:Concept ;
    rdfs:isDefinedBy cs: ;
    skos:definition "The name is official and listed in publications"@en ;
    skos:historyNote "Taken from the Place Names Ontology but with a definition added here" ;
    skos:inScheme cs: ;
    skos:prefLabel "Published"@en ;
    skos:broader :official ;
.

:gazetted
    a skos:Concept ;
    rdfs:isDefinedBy cs: ;
    skos:definition "The name is official and authorised in a jurisdictional gazette"@en ;
    skos:historyNote "Taken from the Place Names Ontology but with a definition added here" ;
    skos:inScheme cs: ;
    skos:prefLabel "Gazetted"@en ;
    skos:broader :official ;
.

<https://linked.data.gov.au/org/qsi>
    a prov:Agent ;
    rdfs:label "Queensland Spatial Information" ;
.

<https://linked.data.gov.au/org/icsm>
    a prov:Agent ;
    rdfs:label "Intergovernmental Committee on Surveying & Mapping" ;
.

cs:
    a skos:ConceptScheme ;
    dcterms:created "2023-06-12"^^xsd:date ;
    dcterms:creator <https://linked.data.gov.au/org/qsi> ;
    dcterms:modified "2023-06-12"^^xsd:date ;
    dcterms:publisher <https://linked.data.gov.au/org/icsm> ;
    owl:versionIRI cs:1.0 ;
    owl:versionInfo "1.0" ;
    skos:definition "This vocabulary contains classifications of how official, or otherwise, a Geographical Name is"@en ;
    skos:hasTopConcept
        :historical ,
        :indigenous ,
        :informal ,
        :official ;
    skos:historyNote "Taken from the Place Names Ontology (https://linked.data.gov.au/def/placenames)"@en ;
    skos:prefLabel "Geographical Name Statuses"@en ;
    skos:scopeNote "These statuses do not indicate whether a Geographical Name is current. Currency of Geographical Names should be indicated by temporal properties" ;
    reg:status agldwgstatus:experimental ;
    prov:qualifiedAttribution [
            dcat:hadRole isoroles:custodian ;
            prov:agent <https://linked.data.gov.au/org/icsm>
        ] ;
.

