PREFIX cs: <https://linked.data.gov.au/def/go-categories>
PREFIX droles: <https://linked.data.gov.au/def/data-roles/>
PREFIX go: <https://linked.data.gov.au/def/go-categories/>
PREFIX owl: <http://www.w3.org/2002/07/owl#>
PREFIX prov: <http://www.w3.org/ns/prov#>
PREFIX rdfs: <http://www.w3.org/2000/01/rdf-schema#>
PREFIX reg: <http://purl.org/linked-data/registry#>
PREFIX schema: <https://schema.org/>
PREFIX skos: <http://www.w3.org/2004/02/skos/core#>
PREFIX xsd: <http://www.w3.org/2001/XMLSchema#>
PREFIX dcterms: <http://purl.org/dc/terms/>

go:abandoned-mine
    a skos:Concept ;
    rdfs:isDefinedBy cs: ;
    skos:definition "An underground site used for the extraction of minerals currently not in use."@en ;
    skos:historyNote "Inherited from ICSM Place Names Working Group's National Feature Catalogue as at 21 December 2023." ;
    skos:inScheme cs: ;
    skos:prefLabel "Abandoned Mine"@en ;
.

go:abandoned-quarry
    a skos:Concept ;
    rdfs:isDefinedBy cs: ;
    skos:definition "An open surface excavation used for the extraction of stone currently not in use."@en ;
    skos:historyNote "Inherited from ICSM Place Names Working Group's National Feature Catalogue as at 21 December 2023." ;
    skos:inScheme cs: ;
    skos:prefLabel "Abandoned Quarry"@en ;
.

go:abattoir
    a skos:Concept ;
    rdfs:isDefinedBy cs: ;
    skos:altLabel
        "Knacker's Yard"@en ,
        "Knackery"@en ,
        "Slaughterhouse"@en ;
    skos:definition "A place where animals are slaughtered."@en ;
    skos:historyNote "Inherited from ICSM Place Names Working Group's National Feature Catalogue as at 21 December 2023." ;
    skos:inScheme cs: ;
    skos:prefLabel "Abattoir"@en ;
.

go:abbey
    a skos:Concept ;
    rdfs:isDefinedBy cs: ;
    skos:altLabel
        "Convent"@en ,
        "Monastery"@en ;
    skos:definition "A building or buildings occupied by monks or nuns under an abbot or abbess."@en ;
    skos:historyNote "Inherited from ICSM Place Names Working Group's National Feature Catalogue as at 21 December 2023." ;
    skos:inScheme cs: ;
    skos:prefLabel "Abbey"@en ;
.

go:abyssal-plain
    a skos:Concept ;
    rdfs:isDefinedBy cs: ;
    skos:definition "An extensive, flat or gently sloping region, usually found at depths greater than 4000 m."@en ;
    skos:historyNote "Inherited from ICSM Place Names Working Group's National Feature Catalogue as at 21 December 2023. Definition from General Bathymetric Chart of the Oceans (GEBCO) Sub-Committee on Undersea Features Names (SCUFN)." ;
    skos:inScheme cs: ;
    skos:prefLabel "Abyssal Plain"@en ;
    schema:citation "https://iho.int/en/basic-documents-1"^^xsd:anyURI ;
.

go:academy
    a skos:Concept ;
    rdfs:isDefinedBy cs: ;
    skos:definition "An educational institution that offers a learning environment for students, often with a focus on a particular field or area of study, and may provide instruction at various levels, from primary to higher education, with some academies having a reputation for academic excellence or specialised programs."@en ;
    skos:historyNote "Created by separating 'Further Education' alternate labels 2024-03-05." ;
    skos:inScheme cs: ;
    skos:prefLabel "Academy"@en ;
.

go:accommodations
    a skos:Concept ;
    rdfs:isDefinedBy cs: ;
    skos:definition "Places primarily used for short term accommodation, usually for recreational purposes."@en ;
    skos:historyNote "Inherited from ICSM Place Names Working Group's National Feature Catalogue as at 21 December 2023, with name label amended 2024-05-04 from 'Accommodation' and definition altered to note recreational purposes 2024-03-05." ;
    skos:inScheme cs: ;
    skos:narrower
        go:camp-ground ,
        go:group-camp ,
        go:holiday-park ,
        go:hut ;
    skos:prefLabel "Accommodations"@en ;
.

go:addressable-property
    a skos:Concept ;
    rdfs:isDefinedBy cs: ;
    skos:definition "A contiguous area of commonly owned land with a single usage by a individual entity."@en ;
    skos:historyNote "Added by Queensland 2024-06-05." ;
    skos:inScheme cs: ;
    skos:prefLabel "Addressable Property"@en ;
.

go:adit
    a skos:Concept ;
    rdfs:isDefinedBy cs: ;
    skos:definition "An almost horizontal shaft into a mine, for access or drainage."@en ;
    skos:historyNote "Inherited from ICSM Place Names Working Group's National Feature Catalogue as at 21 December 2023." ;
    skos:inScheme cs: ;
    skos:prefLabel "Adit"@en ;
.

go:administrative-area
    a skos:Concept ;
    rdfs:isDefinedBy cs: ;
    skos:definition "Places with officially defined boundaries for governance purposes."@en ;
    skos:historyNote "Inherited from ICSM Place Names Working Group's National Feature Catalogue as at 21 December 2023." ;
    skos:inScheme cs: ;
    skos:narrower
        go:agricultural-area ,
        go:antarctic-land ,
        go:catchment-management ,
        go:county ,
        go:federal-electorate ,
        go:land-district ,
        go:local-government-area ,
        go:local-government-area-ward ,
        go:locality ,
        go:mining-centre ,
        go:parish ,
        go:pastoral-district ,
        go:protected-area ,
        go:state-electorate ,
        go:state-territory ,
        go:tourist-region ,
        go:town-site ;
    skos:prefLabel "Administrative Area"@en ;
.

go:administrative-construct
    a skos:Concept ;
    rdfs:isDefinedBy cs: ;
    skos:definition "A virtual delineation object that contributes to or facilitates governance."@en ;
    skos:historyNote "Inherited from ICSM Place Names Working Group's National Feature Catalogue as at 21 December 2023, with name label amended 2024-05-04 from 'Administration' 2024-03-05." ;
    skos:inScheme cs: ;
    skos:narrower
        go:administrative-area ,
        go:populated-place ,
        go:state-border-section ;
    skos:prefLabel "Administrative Construct"@en ;
    skos:topConceptOf cs: ;
.

go:aerodrome
    a skos:Concept ;
    rdfs:isDefinedBy cs: ;
    skos:definition "A landing field for aeroplanes, especially private aeroplanes, having permanent buildings, equipment, hangars, etc., but usually smaller than an airport."@en ;
    skos:historyNote "Created by separating 'Airport' alternate labels 2024-06-10. Definition from Macquarie Dictionary." ;
    skos:inScheme cs: ;
    skos:prefLabel "Aerodrome"@en ;
.

go:aged-care
    a skos:Concept ;
    rdfs:isDefinedBy cs: ;
    skos:definition "A facility that supports the care of the elderly."@en ;
    skos:historyNote "Inherited from ICSM Place Names Working Group's National Feature Catalogue as at 21 December 2023." ;
    skos:inScheme cs: ;
    skos:narrower go:residential-aged-care ;
    skos:prefLabel "Aged Care"@en ;
.

go:agricultural-area
    a skos:Concept ;
    rdfs:isDefinedBy cs: ;
    skos:definition "An area defined for agricultural purposes."@en ;
    skos:historyNote "Inherited from ICSM Place Names Working Group's National Feature Catalogue as at 21 December 2023." ;
    skos:inScheme cs: ;
    skos:prefLabel "Agricultural Area"@en ;
.

go:agriculture
    a skos:Concept ;
    rdfs:isDefinedBy cs: ;
    skos:definition "Places where agricultural activities are undertaken."@en ;
    skos:historyNote "Inherited from ICSM Place Names Working Group's National Feature Catalogue as at 21 December 2023, with name label amended 2024-05-04 from 'Agriculture'." ;
    skos:inScheme cs: ;
    skos:narrower
        go:dairy ,
        go:farm ,
        go:paddock ,
        go:plantation ,
        go:stockyard ,
        go:vineyard ;
    skos:prefLabel "Agricultural Activity Area"@en ;
.

go:aiguille
    a skos:Concept ;
    rdfs:isDefinedBy cs: ;
    skos:altLabel
        "Needle"@en ,
        "Pinnacle"@en ;
    skos:definition "A needle-like rock mass or mountain peak."@en ;
    skos:historyNote "Created by separating 'Peak' alternate labels 2024-06-10. Definition from Macquarie Dictionary." ;
    skos:inScheme cs: ;
    skos:prefLabel "Aiguille"@en ;
.

go:air-force-base
    a skos:Concept ;
    rdfs:isDefinedBy cs: ;
    skos:definition "A facility used by the Air Force for the operation and/or training of personnel and their aircraft."@en ;
    skos:historyNote "Inherited from ICSM Place Names Working Group's National Feature Catalogue as at 21 December 2023." ;
    skos:inScheme cs: ;
    skos:prefLabel "Air Force Base"@en ;
.

go:air-transport-infrastructure
    a skos:Concept ;
    rdfs:isDefinedBy cs: ;
    skos:definition "Facilities and systems necessary for the operation of aircraft and the management of air travel, including airports, runways, air traffic control, navigation aids, and ground support services."@en ;
    skos:historyNote "Inherited from ICSM Place Names Working Group's National Feature Catalogue as at 21 December 2023. with name label amended 2024-05-04 from 'Air'." ;
    skos:inScheme cs: ;
    skos:narrower
        go:air-traffic-control-tower ,
        go:hangar ,
        go:helipad ,
        go:heliport ,
        go:landing-area ,
        go:runway ;
    skos:prefLabel "Air Transport Infrastructure"@en ;
.

go:airfield
    a skos:Concept ;
    rdfs:isDefinedBy cs: ;
    skos:definition "A level area, usually equipped with hard-surfaced runways, buildings, etc., for the operation and maintenance of aircraft."@en ;
    skos:historyNote "Created by separating 'Landing Area' alternate labels 2024-06-10. Definition adapted from Macquarie Dictionary." ;
    skos:inScheme cs: ;
    skos:prefLabel "Airfield"@en ;
.

go:airport
    a skos:Concept ;
    rdfs:isDefinedBy cs: ;
    skos:definition "A regulated landing and taking off area for civil aircraft, usually equipped with runways and aircraft maintenance and passenger facilities."@en ;
    skos:historyNote "Inherited from ICSM Place Names Working Group's National Feature Catalogue as at 21 December 2023." ;
    skos:inScheme cs: ;
    skos:prefLabel "Airport"@en ;
.

go:airstrip
    a skos:Concept ;
    rdfs:isDefinedBy cs: ;
    skos:definition "A runway, especially a single runway forming a landing ground in a remote place. May be unpaved (grass, dirt, or gravel surfaces)."@en ;
    skos:historyNote "Created by separating 'Landing Area' alternate labels 2024-06-10. Definition adapted from Macquarie Dictionary." ;
    skos:inScheme cs: ;
    skos:prefLabel "Airstrip"@en ;
.

go:alluvial-plain
    a skos:Concept ;
    rdfs:isDefinedBy cs: ;
    skos:definition "A river flood plain with a surface covered by alluvial deposits."@en ;
    skos:historyNote "Created by separating 'Plain' alternate labels 2024-06-10. Definition from Macquarie Dictionary." ;
    skos:inScheme cs: ;
    skos:prefLabel "Alluvial Plain"@en ;
.

go:alumina-refinery
    a skos:Concept ;
    rdfs:isDefinedBy cs: ;
    skos:definition "A refinery for extracting Aluminium."@en ;
    skos:historyNote "Inherited from ICSM Place Names Working Group's National Feature Catalogue as at 21 December 2023." ;
    skos:inScheme cs: ;
    skos:prefLabel "Alumina Refinery"@en ;
.

go:ambulance-station
    a skos:Concept ;
    rdfs:isDefinedBy cs: ;
    skos:definition "A structure or other area set aside for storage ofambulance vehicles and medical equipment."@en ;
    skos:historyNote "Inherited from ICSM Place Names Working Group's National Feature Catalogue as at 21 December 2023." ;
    skos:inScheme cs: ;
    skos:prefLabel "Ambulance Station"@en ;
.

go:ampitheatre
    a skos:Concept ;
    rdfs:isDefinedBy cs: ;
    skos:altLabel "Natural Amphitheatre"@en ;
    skos:definition "A circular or oval area of ground, surrounded by tiers of seats on a steep slope, for open-air public performances."@en ;
    skos:historyNote "Inherited from ICSM Place Names Working Group's National Feature Catalogue as at 21 December 2023." ;
    skos:inScheme cs: ;
    skos:prefLabel "Amphitheatre"@en ;
.

go:amusement-centre
    a skos:Concept ;
    rdfs:isDefinedBy cs: ;
    skos:definition "A type of tourist attraction that primarily provides entertainment and recreational activities. It normally includes games, and other forms of amusement, such as arcades."@en ;
    skos:historyNote "Created by separating 'Tourist Attraction' alternate labels 2024-06-10." ;
    skos:inScheme cs: ;
    skos:prefLabel "Amusement Centre"@en ;
.

go:anabranch
    a skos:Concept ;
    rdfs:isDefinedBy cs: ;
    skos:definition "A branch of a river which leaves the main stream and enters it again further on."@en ;
    skos:historyNote "Concept created by separating 'Watercourse' alternate labels 2024-06-10. Definition added from Macquarie Dictionary." ;
    skos:inScheme cs: ;
    skos:prefLabel "Anabranch"@en ;
.

go:anchorage
    a skos:Concept ;
    rdfs:isDefinedBy cs: ;
    skos:altLabel
        "Haven"@en ,
        "Natural Harbour"@en ,
        "Roadstead"@en ;
    skos:definition "A natural area in which vessels anchor or may anchor."@en ;
    skos:historyNote "Inherited from ICSM Place Names Working Group's National Feature Catalogue as at 21 December 2023." ;
    skos:inScheme cs: ;
    skos:prefLabel "Anchorage"@en ;
.

go:antarctic-land
    a skos:Concept ;
    rdfs:isDefinedBy cs: ;
    skos:definition "Large continental area defined by natural boundaries, or partly by natural boundaries and partly by boundaries of political convenience. The term was formally used by explorers for newly discovered lengths of coastline, cf. coast. Outside the area covered by this work the term may be synonymous with territory. The use of land does not refer to the ground, rather it is a generic part of a toponym."@en ;
    skos:historyNote "Inherited from ICSM Place Names Working Group's National Feature Catalogue as at 21 December 2023. Concept and definition from the Australian Antarctic Division." ;
    skos:inScheme cs: ;
    skos:prefLabel "Antarctic Land"@en ;
    schema:citation "https://data.aad.gov.au/aadc/ftc/display_feature_type.cfm?feature_type_code=389"^^xsd:anyURI ;
.

go:antarctic-specially-managed-areas
    a skos:Concept ;
    rdfs:isDefinedBy cs: ;
    skos:altLabel "ASMA"@en ;
    skos:definition "Areas intended to facilitate cooperation between nations operating in close proximity to each other, with a view to minimising environmental impacts. ASMAs may contain zones where various restrictions and permits might apply, and activities within ASMAs are governed by a code of conduct. Designated under the Antarctic Treaty System."@en ;
    skos:historyNote "Inherited from ICSM Place Names Working Group's National Feature Catalogue as at 21 December 2023. Concept and definition from the Australian Antarctic Division." ;
    skos:inScheme cs: ;
    skos:prefLabel "Antarctic Specially Managed Areas"@en ;
.

go:antarctic-specially-protected-areas
    a skos:Concept ;
    rdfs:isDefinedBy cs: ;
    skos:altLabel "ASPA"@en ;
    skos:definition "Areas set aside to protect outstanding environmental, scientific, historic, aesthetic or wilderness values, any combination of those values, or ongoing or planned scientific research. Designated under the Antarctic Treaty System."@en ;
    skos:historyNote "Inherited from ICSM Place Names Working Group's National Feature Catalogue as at 21 December 2023. Concept and definition from the Australian Antarctic Division." ;
    skos:inScheme cs: ;
    skos:prefLabel "Antarctic Specially Protected Areas"@en ;
.

go:aquaculture
    a skos:Concept ;
    rdfs:isDefinedBy cs: ;
    skos:definition "A place for the cultivation of freshwater and marine resources, both plant and animal."@en ;
    skos:historyNote "Inherited from ICSM Place Names Working Group's National Feature Catalogue as at 21 December 2023, with name label amended 2024-05-04 from 'Aquaculture' 2024-03-05." ;
    skos:inScheme cs: ;
    skos:narrower go:hatchery ;
    skos:prefLabel "Aquacultural Activity Area"@en ;
.

go:aquarium
    a skos:Concept ;
    rdfs:isDefinedBy cs: ;
    skos:definition "A facility for the public display of aquatic species."@en ;
    skos:historyNote "Inherited from ICSM Place Names Working Group's National Feature Catalogue as at 21 December 2023." ;
    skos:inScheme cs: ;
    skos:prefLabel "Aquarium"@en ;
.

go:aquatic-passage
    a skos:Concept ;
    rdfs:isDefinedBy cs: ;
    skos:altLabel
        "Narrows"@en ,
        "Rip"@en ,
        "Strait"@en ;
    skos:definition "A navigable route, specifically one through reefs, islands, lands or shallow waters."@en ;
    skos:historyNote "Inherited from ICSM Place Names Working Group's National Feature Catalogue as at 21 December 2023." ;
    skos:inScheme cs: ;
    skos:prefLabel "Aquatic Passage"@en ;
.

go:aquifer
    a skos:Concept ;
    rdfs:isDefinedBy cs: ;
    skos:altLabel "Artesian Basin"@en ;
    skos:definition "An underground waterbody."@en ;
    skos:historyNote "Inherited from ICSM Place Names Working Group's National Feature Catalogue as at 21 December 2023." ;
    skos:inScheme cs: ;
    skos:prefLabel "Aquifer"@en ;
.

go:arboretum
    a skos:Concept ;
    rdfs:isDefinedBy cs: ;
    skos:definition "A place where trees or shrubs are cultivated for their scientific or educational interest."@en ;
    skos:historyNote "Inherited from ICSM Place Names Working Group's National Feature Catalogue as at 21 December 2023." ;
    skos:inScheme cs: ;
    skos:prefLabel "Arboretum"@en ;
.

go:arena
    a skos:Concept ;
    rdfs:isDefinedBy cs: ;
    skos:definition "An enclosure for sports contests, shows, etc."@en ;
    skos:historyNote "Created by separating 'Sports Facility' alternate labels 2024-05-10. Definition from Macquarie Dictionary." ;
    skos:inScheme cs: ;
    skos:prefLabel "Arena"@en ;
.

go:army-base
    a skos:Concept ;
    rdfs:isDefinedBy cs: ;
    skos:definition "A facility used by the army for the operation and/or training of personnel and their vehicles."@en ;
    skos:historyNote "Inherited from ICSM Place Names Working Group's National Feature Catalogue as at 21 December 2023." ;
    skos:inScheme cs: ;
    skos:prefLabel "Army Base"@en ;
.

go:art-gallery
    a skos:Concept ;
    rdfs:isDefinedBy cs: ;
    skos:definition "An area or facility which displays art works."@en ;
    skos:historyNote "Inherited from ICSM Place Names Working Group's National Feature Catalogue as at 21 December 2023." ;
    skos:inScheme cs: ;
    skos:prefLabel "Art Gallery"@en ;
.

go:athletic-field
    a skos:Concept ;
    rdfs:isDefinedBy cs: ;
    skos:altLabel "Athletic Track"@en ;
    skos:definition "A place where training and competitions are held related to athletics."@en ;
    skos:historyNote "Inherited from ICSM Place Names Working Group's National Feature Catalogue as at 21 December 2023. Definition amended 2024-06-10." ;
    skos:inScheme cs: ;
    skos:prefLabel "Athletic Field"@en ;
.

go:atoll
    a skos:Concept ;
    rdfs:isDefinedBy cs: ;
    skos:definition "A coral island consisting of a reef surrounding a lagoon."@en ;
    skos:historyNote "Created by separating 'Island' alternate labels 2024-03-05. Definition adapted from Macquarie Dictionary." ;
    skos:inScheme cs: ;
    skos:prefLabel "Atoll"@en ;
.

go:automatic-weather-station
    a skos:Concept ;
    rdfs:isDefinedBy cs: ;
    skos:definition "A facility that uses sensors and other instruments to collect data on atmospheric conditions and weather parameters without requiring manual intervention by humans."@en ;
    skos:historyNote "Created by separating 'Weather Station' alternate labels 2024-06-10." ;
    skos:inScheme cs: ;
    skos:prefLabel "Automatic Weather Station"@en ;
.

go:backwater
    a skos:Concept ;
    rdfs:isDefinedBy cs: ;
    skos:altLabel "Back Water"@en ;
    skos:definition "A body of stagnant water connected to a river."@en ;
    skos:historyNote "Concept created by separating 'Lake' alternate labels 2024-06-10. Definition added from Macquarie Dictionary." ;
    skos:inScheme cs: ;
    skos:prefLabel "Backwater"@en ;
.

go:bank
    a skos:Concept ;
    rdfs:isDefinedBy cs: ;
    skos:definition "The sloping ground along the edge of water."@en ;
    skos:historyNote "Inherited from ICSM Place Names Working Group's National Feature Catalogue as at 21 December 2023." ;
    skos:inScheme cs: ;
    skos:narrower go:marine-bank ;
    skos:prefLabel "Bank"@en ;
.

go:bar
    a skos:Concept ;
    rdfs:isDefinedBy cs: ;
    skos:definition "A bar of sand, coral, mud formed in a sea or river, exposed at low tide and formed by the action of the tides or currents."@en ;
    skos:historyNote "Inherited from ICSM Place Names Working Group's National Feature Catalogue as at 21 December 2023." ;
    skos:inScheme cs: ;
    skos:narrower go:sandbar ;
    skos:prefLabel "Bar"@en ;
.

go:barracks
    a skos:Concept ;
    rdfs:isDefinedBy cs: ;
    skos:definition "A building or buildings used for the lodgement or residence of defence personnel."@en ;
    skos:historyNote "Inherited from ICSM Place Names Working Group's National Feature Catalogue as at 21 December 2023." ;
    skos:inScheme cs: ;
    skos:prefLabel "Barracks"@en ;
.

go:baseball-field
    a skos:Concept ;
    rdfs:isDefinedBy cs: ;
    skos:definition "A place where baseball is played."@en ;
    skos:historyNote "Inherited from ICSM Place Names Working Group's National Feature Catalogue as at 21 December 2023." ;
    skos:inScheme cs: ;
    skos:prefLabel "Baseball Field"@en ;
.

go:basin
    a skos:Concept ;
    rdfs:isDefinedBy cs: ;
    skos:definition "A hollow or trough in the surface of the land, synonymous with cirque, or an almost landlocked body of water off an inlet or sound; the term may be applied also to submarine features."@en ;
    skos:historyNote "Broader concept introduced 2024-03-05. Concept and definition from the Australian Antarctic Division." ;
    skos:inScheme cs: ;
    skos:narrower
        go:marine-basin ,
        go:subglacial-basin ;
    skos:prefLabel "Basin"@en ;
    schema:citation "https://data.aad.gov.au/aadc/ftc/display_feature_type.cfm?feature_type_code=354"^^xsd:anyURI ;
.

go:basketball-court
    a skos:Concept ;
    rdfs:isDefinedBy cs: ;
    skos:definition "A place where basketball is played."@en ;
    skos:historyNote "Inherited from ICSM Place Names Working Group's National Feature Catalogue as at 21 December 2023." ;
    skos:inScheme cs: ;
    skos:prefLabel "Basketball Court"@en ;
.

go:battery
    a skos:Concept ;
    rdfs:isDefinedBy cs: ;
    skos:definition "A stone crushing works for ore extraction, as used on gold fields."@en ;
    skos:historyNote "Inherited from ICSM Place Names Working Group's National Feature Catalogue as at 21 December 2023." ;
    skos:inScheme cs: ;
    skos:prefLabel "Battery"@en ;
.

go:bay
    a skos:Concept ;
    rdfs:isDefinedBy cs: ;
    skos:altLabel "Cove"@en ;
    skos:definition "A well-marked indentation made by the sea or a lake into its shoreline."@en ;
    skos:historyNote "Inherited from ICSM Place Names Working Group's National Feature Catalogue as at 21 December 2023." ;
    skos:inScheme cs: ;
    skos:prefLabel "Bay"@en ;
.

go:beach
    a skos:Concept ;
    rdfs:isDefinedBy cs: ;
    skos:altLabel "Shore"@en ;
    skos:definition "A sloping shore along water that is periodically washed by waves or tides and is usually covered in sand or gravel."@en ;
    skos:historyNote "Inherited from ICSM Place Names Working Group's National Feature Catalogue as at 21 December 2023." ;
    skos:inScheme cs: ;
    skos:prefLabel "Beach"@en ;
.

go:beacon
    a skos:Concept ;
    rdfs:isDefinedBy cs: ;
    skos:altLabel
        "Buoy"@en ,
        "Navigation Bouy"@en ,
        "Navigation Light"@en ;
    skos:definition "A structure to provide a navigational signal for vessels or aircraft."@en ;
    skos:historyNote "Inherited from ICSM Place Names Working Group's National Feature Catalogue as at 21 December 2023." ;
    skos:inScheme cs: ;
    skos:prefLabel "Beacon"@en ;
.

go:bench
    a skos:Concept ;
    rdfs:isDefinedBy cs: ;
    skos:altLabel
        "Terrace"@en ,
        "Tiers"@en ;
    skos:definition "A flat ledge on sloping ground."@en ;
    skos:historyNote "Inherited from ICSM Place Names Working Group's National Feature Catalogue as at 21 December 2023." ;
    skos:inScheme cs: ;
    skos:prefLabel "Bench"@en ;
.

go:bend
    a skos:Concept ;
    rdfs:isDefinedBy cs: ;
    skos:altLabel
        "Loop"@en ,
        "Meander"@en ,
        "River Bend"@en ;
    skos:definition "A curve in the course of a stream."@en ;
    skos:historyNote "Inherited from ICSM Place Names Working Group's National Feature Catalogue as at 21 December 2023." ;
    skos:inScheme cs: ;
    skos:prefLabel "Bend"@en ;
.

go:bikeway
    a skos:Concept ;
    rdfs:isDefinedBy cs: ;
    skos:altLabel
        "Bike Path"@en ,
        "Cycleway"@en ;
    skos:definition "A designated path primarily for bicycle use. This is not a shared roadway with vehicular traffic."@en ;
    skos:historyNote "Inherited from ICSM Place Names Working Group's National Feature Catalogue as at 21 December 2023, with name label amended 2024-05-04 from 'Bicycle Track' for clarity." ;
    skos:inScheme cs: ;
    skos:prefLabel "Bikeway"@en ;
.

go:billabong
    a skos:Concept ;
    rdfs:isDefinedBy cs: ;
    skos:definition "An anabranch in which the water has stopped flowing and which is characterised by occasional swamps, waterholes and watered patches, the river sometimes flowing again and replenishing the water supply in flood time."@en ;
    skos:historyNote "Concept created by separating 'Lake' alternate labels 2024-06-10. Definition added from Macquarie Dictionary." ;
    skos:inScheme cs: ;
    skos:prefLabel "Billabong"@en ;
.

go:biomass-power-station
    a skos:Concept ;
    rdfs:isDefinedBy cs: ;
    skos:definition "A process plant that creates power from biomass sources."@en ;
    skos:historyNote "Created by separating 'Power Station' alternate labels 2024-03-05." ;
    skos:inScheme cs: ;
    skos:prefLabel "Biomass Power Station"@en ;
.

go:blowhole
    a skos:Concept ;
    rdfs:isDefinedBy cs: ;
    skos:definition "A hole near the seashore that has been formed in the roof of a cave, and through which air and possibly water are forced by the rising tide."@en ;
    skos:historyNote "Inherited from ICSM Place Names Working Group's National Feature Catalogue as at 21 December 2023." ;
    skos:inScheme cs: ;
    skos:prefLabel "Blowhole"@en ;
.

go:bluff
    a skos:Concept ;
    rdfs:isDefinedBy cs: ;
    skos:definition "A rounded cliff, headland, or hill with a broad, steep face."@en ;
    skos:historyNote "Created by separating 'Cliff' alternate labels 2024-05-10. Definition adapted from Macquarie Dictionary." ;
    skos:inScheme cs: ;
    skos:prefLabel "Bluff"@en ;
.

go:bmx-track
    a skos:Concept ;
    rdfs:isDefinedBy cs: ;
    skos:definition "A place where BMX bikes are used for recreation or racing."@en ;
    skos:historyNote "Inherited from ICSM Place Names Working Group's National Feature Catalogue as at 21 December 2023." ;
    skos:inScheme cs: ;
    skos:prefLabel "BMX Track"@en ;
.

go:boardwalk
    a skos:Concept ;
    rdfs:isDefinedBy cs: ;
    skos:definition "A trail made of boarding; a surface of planks or sleepers, usually of wood, between which water can usually drain."@en ;
    skos:historyNote "Created by separating 'Walking Trail' alternate labels 2024-06-10. Definition adapted from Macquarie Dictionary." ;
    skos:inScheme cs: ;
    skos:prefLabel "Boardwalk"@en ;
.

go:boat-ramp
    a skos:Concept ;
    rdfs:isDefinedBy cs: ;
    skos:altLabel
        "Boat Launch"@en ,
        "Landing Ramp"@en ,
        "Launching Ramp"@en ,
        "Slipway"@en ;
    skos:definition "A sloping construction to facilitate launching or retrieving vessels from water."@en ;
    skos:historyNote "Inherited from ICSM Place Names Working Group's National Feature Catalogue as at 21 December 2023." ;
    skos:inScheme cs: ;
    skos:prefLabel "Boat Ramp"@en ;
.

go:boating-club
    a skos:Concept ;
    rdfs:isDefinedBy cs: ;
    skos:definition "A building where boats are stored or from where boating related activities conducted."@en ;
    skos:historyNote "Inherited from ICSM Place Names Working Group's National Feature Catalogue as at 21 December 2023." ;
    skos:inScheme cs: ;
    skos:prefLabel "Boating Club"@en ;
.

go:bombing-range
    a skos:Concept ;
    rdfs:isDefinedBy cs: ;
    skos:altLabel "Rocket Range"@en ;
    skos:definition "A tract of land on which the military conducts bombing practice."@en ;
    skos:historyNote "Inherited from ICSM Place Names Working Group's National Feature Catalogue as at 21 December 2023." ;
    skos:inScheme cs: ;
    skos:prefLabel "Bombing Range"@en ;
.

go:bore
    a skos:Concept ;
    rdfs:isDefinedBy cs: ;
    skos:altLabel "Artesian Well"@en ;
    skos:definition "A deep vertical hole of a small diameter made to obtain water."@en ;
    skos:historyNote "Inherited from ICSM Place Names Working Group's National Feature Catalogue as at 21 December 2023." ;
    skos:inScheme cs: ;
    skos:prefLabel "Bore"@en ;
.

go:botanic-gardens
    a skos:Concept ;
    rdfs:isDefinedBy cs: ;
    skos:definition "A park or reserve which contains specialised collections of plants."@en ;
    skos:historyNote "Inherited from ICSM Place Names Working Group's National Feature Catalogue as at 21 December 2023." ;
    skos:inScheme cs: ;
    skos:prefLabel "Botanic Gardens"@en ;
.

go:boulder
    a skos:Concept ;
    rdfs:isDefinedBy cs: ;
    skos:definition "A detached and rounded or worn rock, especially a large one."@en ;
    skos:historyNote "Created by separating 'Rock' alternate labels 2024-06-10. Definition from Macquarie Dictionary." ;
    skos:inScheme cs: ;
    skos:prefLabel "Boulder"@en ;
.

go:bowling-green
    a skos:Concept ;
    rdfs:isDefinedBy cs: ;
    skos:definition "An area of closely mown turf on which the game of bowls is played."@en ;
    skos:historyNote "Inherited from ICSM Place Names Working Group's National Feature Catalogue as at 21 December 2023." ;
    skos:inScheme cs: ;
    skos:prefLabel "Bowling Green"@en ;
.

go:breakaway
    a skos:Concept ;
    rdfs:isDefinedBy cs: ;
    skos:definition "Steep cliffs connecting the old and new plateaus formed by the collapse of a tabletop, mesa or the like."@en ;
    skos:historyNote "Created by separating 'Cliff' alternate labels 2024-05-10. Definition from Macquarie Dictionary." ;
    skos:inScheme cs: ;
    skos:prefLabel "Breakaway"@en ;
.

go:brewery
    a skos:Concept ;
    rdfs:isDefinedBy cs: ;
    skos:definition "An establishment for brewing beer, ale."@en ;
    skos:historyNote "Inherited from ICSM Place Names Working Group's National Feature Catalogue as at 21 December 2023." ;
    skos:inScheme cs: ;
    skos:prefLabel "Brewery"@en ;
.

go:brickworks
    a skos:Concept ;
    rdfs:isDefinedBy cs: ;
    skos:definition "A place where bricks are made."@en ;
    skos:historyNote "Inherited from ICSM Place Names Working Group's National Feature Catalogue as at 21 December 2023." ;
    skos:inScheme cs: ;
    skos:prefLabel "Brickworks"@en ;
.

go:bridge
    a skos:Concept ;
    rdfs:isDefinedBy cs: ;
    skos:definition "Engineered structures that enable vehicles or people to cross over obstacles like rivers, gorges, railways, or other roadways, facilitating uninterrupted travel."@en ;
    skos:historyNote "Broader concept introduced 2024-03-05." ;
    skos:inScheme cs: ;
    skos:narrower
        go:green-bridge ,
        go:rail-bridge ,
        go:road-bridge ;
    skos:prefLabel "Bridge"@en ;
.

go:broadcasting-tower
    a skos:Concept ;
    rdfs:isDefinedBy cs: ;
    skos:definition "Tower equipped with transmitters and antennas for broadcasting audio (radio) and video (television) signals to the public."@en ;
    skos:historyNote "Created by separating 'Communicatio Tower' alternate labels 2024-06-10." ;
    skos:inScheme cs: ;
    skos:narrower
        go:radio-tower ,
        go:television-tower ;
    skos:prefLabel "Broadcasting Tower"@en ;
.

go:brook
    a skos:Concept ;
    rdfs:isDefinedBy cs: ;
    skos:altLabel
        "Rivulet"@en ,
        "Streamlet"@en ;
    skos:definition "A small, natural stream of fresh water."@en ;
    skos:historyNote "Concept created by separating 'Watercourse' alternate labels 2024-06-10. Definition added from Macquarie Dictionary." ;
    skos:inScheme cs: ;
    skos:prefLabel "Brook"@en ;
.

go:building
    a skos:Concept ;
    rdfs:isDefinedBy cs: ;
    skos:definition "a substantial structure with a roof and walls."@en ;
    skos:historyNote "Added by Queensland 2024-03-05. Definition from Macquarie Dictionary." ;
    skos:inScheme cs: ;
    skos:prefLabel "Building"@en ;
.

go:bus-depot
    a skos:Concept ;
    rdfs:isDefinedBy cs: ;
    skos:definition "An area for storage and maintenance of buses."@en ;
    skos:historyNote "Inherited from ICSM Place Names Working Group's National Feature Catalogue as at 21 December 2023." ;
    skos:inScheme cs: ;
    skos:prefLabel "Bus Depot"@en ;
.

go:bus-lane
    a skos:Concept ;
    rdfs:isDefinedBy cs: ;
    skos:definition "A road lane that is restricted to buses, taxis, motorcycles and bicycles, emergency vehicles, etc."@en ;
    skos:historyNote "Added by Queensland 2024-06-05. Definition from Macquarie Dictionary." ;
    skos:inScheme cs: ;
    skos:prefLabel "Bus Lane"@en ;
.

go:bus-route
    a skos:Concept ;
    rdfs:isDefinedBy cs: ;
    skos:definition "The set route taken by a bus service."@en ;
    skos:historyNote "Inherited from ICSM Place Names Working Group's National Feature Catalogue as at 21 December 2023." ;
    skos:inScheme cs: ;
    skos:prefLabel "Bus Route"@en ;
.

go:bus-stop
    a skos:Concept ;
    rdfs:isDefinedBy cs: ;
    skos:definition "A designated place where buses stop for passengers to board or alight."@en ;
    skos:historyNote "Inherited from ICSM Place Names Working Group's National Feature Catalogue as at 21 December 2023. 2023-09-13" ;
    skos:inScheme cs: ;
    skos:prefLabel "Bus Stop"@en ;
.

go:bus-transport-infrastructure
    a skos:Concept ;
    rdfs:isDefinedBy cs: ;
    skos:definition "Facilities and structures designed and built to support the movement of buses."@en ;
    skos:historyNote "Broader concept introduced 2024-06-05." ;
    skos:inScheme cs: ;
    skos:narrower
        go:bus-depot ,
        go:bus-lane ,
        go:bus-route ,
        go:bus-station ,
        go:bus-stop ,
        go:busway ;
    skos:prefLabel "Bus Transport Infrastructure"@en ;
.

go:bush-nursing-hospital
    a skos:Concept ;
    rdfs:isDefinedBy cs: ;
    skos:definition "A hospital that operates primarily in rural areas."@en ;
    skos:historyNote "Inherited from ICSM Place Names Working Group's National Feature Catalogue as at 21 December 2023." ;
    skos:inScheme cs: ;
    skos:prefLabel "Bush Nursing Hospital"@en ;
.

go:business-college
    a skos:Concept ;
    rdfs:isDefinedBy cs: ;
    skos:definition "An educational institution that specialises in teaching courses and programs related to business disciplines such as accounting, finance, marketing, management, human resources, entrepreneurship, and international business"@en ;
    skos:historyNote "Created by separating 'Further Education' alternate labels 2024-03-05." ;
    skos:inScheme cs: ;
    skos:prefLabel "Business College"@en ;
.

go:busway
    a skos:Concept ;
    rdfs:isDefinedBy cs: ;
    skos:definition "A road which is wholly dedicated as a bus-only transit way. This does not include bus lanes on roads with other trafficability."@en ;
    skos:historyNote "Added by Queensland 2024-06-04 from Queensland Roads and Tracks dataset." ;
    skos:inScheme cs: ;
    skos:prefLabel "Busway"@en ;
.

go:butte
    a skos:Concept ;
    rdfs:isDefinedBy cs: ;
    skos:definition "An isolated hill or mountain rising abruptly above the surrounding land. Similar to a mesa but smaller."@en ;
    skos:historyNote "Created by separating 'Hill' alternate labels 2024-05-10. Definition adapted from Macquarie Dictionary." ;
    skos:inScheme cs: ;
    skos:prefLabel "Butte"@en ;
.

go:buttress
    a skos:Concept ;
    rdfs:isDefinedBy cs: ;
    skos:definition "A prominent support or projection of rock that juts out from a mountain or cliff face."@en ;
    skos:historyNote "Created by separating 'Cliff' alternate labels 2024-05-10. Definition adapted from Macquarie Dictionary." ;
    skos:inScheme cs: ;
    skos:prefLabel "Buttress"@en ;
.

go:cableway
    a skos:Concept ;
    rdfs:isDefinedBy cs: ;
    skos:altLabel
        "Chair Lift"@en ,
        "Gondola Lift"@en ,
        "J-Bar"@en ,
        "Poma Gondola"@en ,
        "Surface Lift"@en ,
        "T-Bar"@en ;
    skos:definition "A series of chairs, bars or cabins attached to a power-driven cable for conveying people."@en ;
    skos:historyNote "Inherited from ICSM Place Names Working Group's National Feature Catalogue as at 21 December 2023." ;
    skos:inScheme cs: ;
    skos:prefLabel "Cableway"@en ;
.

go:cableway-transport-infrastructure
    a skos:Concept ;
    rdfs:isDefinedBy cs: ;
    skos:definition "Installations, systems, and structures that enable the operation of cableways and serve as the foundation for cableway transportation."@en ;
    skos:historyNote "Broader concept introduced 2024-03-05." ;
    skos:inScheme cs: ;
    skos:narrower
        go:cableway ,
        go:cableway-terminal ;
    skos:prefLabel "Cableway Transport Infrastructure"@en ;
.

go:cairn
    a skos:Concept ;
    rdfs:isDefinedBy cs: ;
    skos:definition "A pyramidal heap of stones to mark a summit, track, boundary, historical event, or a memorial to a person."@en ;
    skos:historyNote "Created by separating 'Monument' alternate labels 2024-03-05. Definition from Macquarie Dictionary." ;
    skos:inScheme cs: ;
    skos:prefLabel "Cairn"@en ;
.

go:camp-ground
    a skos:Concept ;
    rdfs:isDefinedBy cs: ;
    skos:altLabel
        "Camp"@en ,
        "Camp Site"@en ;
    skos:definition "An area where a camp has been established or where it would be suitable to establish one; an area, often provided with amenities, where it is permitted to set up a camp."@en ;
    skos:historyNote "Inherited from ICSM Place Names Working Group's National Feature Catalogue as at 21 December 2023." ;
    skos:inScheme cs: ;
    skos:prefLabel "Camp Ground"@en ;
.

go:canal
    a skos:Concept ;
    rdfs:isDefinedBy cs: ;
    skos:definition "An artificial waterway constructed for navigation and/or water power."@en ;
    skos:historyNote "Inherited from ICSM Place Names Working Group's National Feature Catalogue as at 21 December 2023." ;
    skos:inScheme cs: ;
    skos:prefLabel "Canal"@en ;
.

go:cape
    a skos:Concept ;
    rdfs:isDefinedBy cs: ;
    skos:altLabel
        "Head"@en ,
        "Headland"@en ;
    skos:definition "An elevated protrusion of land into the sea, more prominent than a point."@en ;
    skos:historyNote "Inherited from ICSM Place Names Working Group's National Feature Catalogue as at 21 December 2023." ;
    skos:inScheme cs: ;
    skos:prefLabel "Cape"@en ;
.

go:car-park
    a skos:Concept ;
    rdfs:isDefinedBy cs: ;
    skos:altLabel "Parking Station"@en ;
    skos:definition "An area or building which is designed or adapted for the parking of cars."@en ;
    skos:historyNote "Inherited from ICSM Place Names Working Group's National Feature Catalogue as at 21 December 2023." ;
    skos:inScheme cs: ;
    skos:prefLabel "Car Park"@en ;
.

go:caravan-park
    a skos:Concept ;
    rdfs:isDefinedBy cs: ;
    skos:definition "A bounded area in which caravans are, or can be, parked, or where caravan type accommodation can be obtained; domestic facilities may be provided."@en ;
    skos:historyNote "Inherited from ICSM Place Names Working Group's National Feature Catalogue as at 21 December 2023." ;
    skos:inScheme cs: ;
    skos:prefLabel "Caravan Park"@en ;
.

go:care-facility
    a skos:Concept ;
    rdfs:isDefinedBy cs: ;
    skos:definition "Facility to support persons requiring care for reasons not directly related to a medical need."@en ;
    skos:historyNote "Inherited from ICSM Place Names Working Group's National Feature Catalogue as at 21 December 2023, with name label amended 2024-05-04 from 'Care' 2024-03-05." ;
    skos:inScheme cs: ;
    skos:narrower
        go:aged-care ,
        go:child-care ,
        go:disability-support-facility ;
    skos:prefLabel "Care Facility"@en ;
    skos:topConceptOf cs: ;
.

go:cargo-terminal
    a skos:Concept ;
    rdfs:isDefinedBy cs: ;
    skos:altLabel "Container Terminal"@en ;
    skos:definition "A site used to manage and store freight."@en ;
    skos:historyNote "Inherited from ICSM Place Names Working Group's National Feature Catalogue as at 21 December 2023." ;
    skos:inScheme cs: ;
    skos:prefLabel "Cargo Terminal"@en ;
.

go:catchment-management
    a skos:Concept ;
    rdfs:isDefinedBy cs: ;
    skos:definition "An administrative bounded area proclaimed for water catchment protection."@en ;
    skos:historyNote "Inherited from ICSM Place Names Working Group's National Feature Catalogue as at 21 December 2023." ;
    skos:inScheme cs: ;
    skos:prefLabel "Catchment Management"@en ;
.

go:cathedral
    a skos:Concept ;
    rdfs:isDefinedBy cs: ;
    skos:definition "The principal church of a diocese, containing the bishop’s throne."@en ;
    skos:historyNote "Inherited from ICSM Place Names Working Group's National Feature Catalogue as at 21 December 2023. Definition from Macquarie Dictionary." ;
    skos:inScheme cs: ;
    skos:prefLabel "Cathedral"@en ;
.

go:causeway
    a skos:Concept ;
    rdfs:isDefinedBy cs: ;
    skos:definition "A raised road or path, as across low or wet ground."@en ;
    skos:historyNote "Inherited from ICSM Place Names Working Group's National Feature Catalogue as at 21 December 2023. Definition from Macquarie Dictionary." ;
    skos:inScheme cs: ;
    skos:prefLabel "Causeway"@en ;
.

go:cave
    a skos:Concept ;
    rdfs:isDefinedBy cs: ;
    skos:definition "A hollowed-out chamber in the Earth, or in the side of a cliff or hill; especially a larger natural cavity in the earth with an opening to the surface."@en ;
    skos:historyNote "Inherited from ICSM Place Names Working Group's National Feature Catalogue as at 21 December 2023." ;
    skos:inScheme cs: ;
    skos:narrower
        go:cavern ,
        go:grotto ,
        go:lava-tube ;
    skos:prefLabel "Cave"@en ;
.

go:cavern
    a skos:Concept ;
    rdfs:isDefinedBy cs: ;
    skos:definition "A specific type of cave, naturally formed in soluble rock with the ability to grow speleothems. Often implies a larger, more spacious cave or a series of interconnected chambers."@en ;
    skos:historyNote "Created by separating 'Cave' alternate labels 2024-03-05. Definition adapted from Macquarie Dictionary." ;
    skos:inScheme cs: ;
    skos:prefLabel "Cavern"@en ;
.

go:cay
    a skos:Concept ;
    rdfs:isDefinedBy cs: ;
    skos:definition "An area of sand or coral above sea level."@en ;
    skos:historyNote "Created by separating 'Island' alternate labels 2024-03-05." ;
    skos:inScheme cs: ;
    skos:prefLabel "Cay"@en ;
.

go:cement-plant
    a skos:Concept ;
    rdfs:isDefinedBy cs: ;
    skos:definition "A place where cement is manufactured."@en ;
    skos:historyNote "Inherited from ICSM Place Names Working Group's National Feature Catalogue as at 21 December 2023." ;
    skos:inScheme cs: ;
    skos:prefLabel "Cement Plant"@en ;
.

go:cemetery
    a skos:Concept ;
    rdfs:isDefinedBy cs: ;
    skos:altLabel "Burial Site"@en ;
    skos:definition "An operational place/area for burying the dead"@en ;
    skos:historyNote "Inherited from ICSM Place Names Working Group's National Feature Catalogue as at 21 December 2023." ;
    skos:inScheme cs: ;
    skos:prefLabel "Cemetery"@en ;
.

go:chapel
    a skos:Concept ;
    rdfs:isDefinedBy cs: ;
    skos:definition "A place of worship connected with and subsidiary to a church; a place of worship other than a church or cathedral, especially in public institutions."@en ;
    skos:historyNote "Inherited from ICSM Place Names Working Group's National Feature Catalogue as at 21 December 2023." ;
    skos:inScheme cs: ;
    skos:prefLabel "Chapel"@en ;
.

go:child-care
    a skos:Concept ;
    rdfs:isDefinedBy cs: ;
    skos:altLabel
        "Creche"@en ,
        "Nursery"@en ,
        "Play Group"@en ;
    skos:definition "A facility to care for children."@en ;
    skos:historyNote "Inherited from ICSM Place Names Working Group's National Feature Catalogue as at 21 December 2023." ;
    skos:inScheme cs: ;
    skos:prefLabel "Child Care"@en ;
.

go:childrens-hospital
    a skos:Concept ;
    rdfs:isDefinedBy cs: ;
    skos:definition "An institution in which sick or injured young persons are given medical or surgical treatment."@en ;
    skos:historyNote "Created by separating Hospital alternate labels, definition adapted from Hospital Queensland 2024-03-05." ;
    skos:inScheme cs: ;
    skos:prefLabel "Childrens Hospital"@en ;
.

go:church
    a skos:Concept ;
    rdfs:isDefinedBy cs: ;
    skos:definition "A building used for religious worship. Includes all Christian dominations."@en ;
    skos:historyNote "Inherited from ICSM Place Names Working Group's National Feature Catalogue as at 21 December 2023." ;
    skos:inScheme cs: ;
    skos:prefLabel "Church"@en ;
.

go:cinema
    a skos:Concept ;
    rdfs:isDefinedBy cs: ;
    skos:definition "A place designed for the exhibition of films."@en ;
    skos:historyNote "Inherited from ICSM Place Names Working Group's National Feature Catalogue as at 21 December 2023." ;
    skos:inScheme cs: ;
    skos:narrower go:drive-in-theatre ;
    skos:prefLabel "Cinema"@en ;
.

go:cirque
    a skos:Concept ;
    rdfs:isDefinedBy cs: ;
    skos:definition "A deep rounded hollow on a mountain side formed by glacial action and usually occupied by a remnant glacier or neve."@en ;
    skos:historyNote "Inherited from ICSM Place Names Working Group's National Feature Catalogue as at 21 December 2023." ;
    skos:inScheme cs: ;
    skos:prefLabel "Cirque"@en ;
.

go:clay-pan
    a skos:Concept ;
    rdfs:isDefinedBy cs: ;
    skos:definition "A small depression, intermittently containing water, which holds clay deposits."@en ;
    skos:historyNote "Inherited from ICSM Place Names Working Group's National Feature Catalogue as at 21 December 2023." ;
    skos:inScheme cs: ;
    skos:prefLabel "Clay Pan"@en ;
.

go:clearing
    a skos:Concept ;
    rdfs:isDefinedBy cs: ;
    skos:definition "A tract of cleared land, as in a forest."@en ;
    skos:historyNote "Created by separating 'Plain' alternate labels 2024-06-10. Definition from Macquarie Dictionary." ;
    skos:inScheme cs: ;
    skos:prefLabel "Clearing"@en ;
.

go:cliff
    a skos:Concept ;
    rdfs:isDefinedBy cs: ;
    skos:definition "A perpendicular or steep face of rock of considerable height either inland or along the coast."@en ;
    skos:historyNote "Inherited from ICSM Place Names Working Group's National Feature Catalogue as at 21 December 2023." ;
    skos:inScheme cs: ;
    skos:narrower
        go:bluff ,
        go:breakaway ,
        go:buttress ,
        go:crag ,
        go:jump-up ,
        go:precipice ,
        go:rockface ;
    skos:prefLabel "Cliff"@en ;
.

go:clumps
    a skos:Concept ;
    rdfs:isDefinedBy cs: ;
    skos:definition "Clusters or aggregates of coral."@en ;
    skos:historyNote "Created by separating 'Island' alternate labels 2024-03-05." ;
    skos:inScheme cs: ;
    skos:prefLabel "Clumps"@en ;
.

go:coal-field
    a skos:Concept ;
    rdfs:isDefinedBy cs: ;
    skos:definition "An area in which coal resources have been identified."@en ;
    skos:historyNote "Inherited from ICSM Place Names Working Group's National Feature Catalogue as at 21 December 2023." ;
    skos:inScheme cs: ;
    skos:prefLabel "Coal Field"@en ;
.

go:coal-power-station
    a skos:Concept ;
    rdfs:isDefinedBy cs: ;
    skos:definition "A process plant that creates power from coal."@en ;
    skos:historyNote "Created by separating 'Power Station' alternate labels 2024-03-05." ;
    skos:inScheme cs: ;
    skos:prefLabel "Coal Power Station"@en ;
.

go:coast
    a skos:Concept ;
    rdfs:isDefinedBy cs: ;
    skos:altLabel "Coastline"@en ;
    skos:definition "Boundary between land and sea, applied in place-names to lengths of coastline determined partly by the history of their discovery and partly by convenient demarcation points."@en ;
    skos:historyNote "Inherited from ICSM Place Names Working Group's National Feature Catalogue as at 21 December 2023. Concept and definition from the Australian Antarctic Division." ;
    skos:inScheme cs: ;
    skos:prefLabel "Coast"@en ;
    schema:citation "https://data.aad.gov.au/aadc/ftc/display_feature_type.cfm?feature_type_code=366"^^xsd:anyURI ;
.

go:coast-guard-facility
    a skos:Concept ;
    rdfs:isDefinedBy cs: ;
    skos:altLabel
        "Marine Rescue"@en ,
        "Volunteer Marine Rescue"@en ;
    skos:definition "A maritime facility supporting the activities of a coast guard."@en ;
    skos:historyNote "Inherited from ICSM Place Names Working Group's National Feature Catalogue as at 21 December 2023, with name label amended 2024-05-04 from 'Coast Guard' 2024-03-05." ;
    skos:inScheme cs: ;
    skos:prefLabel "Coast Guard Facility"@en ;
.

go:coastal-reserve
    a skos:Concept ;
    rdfs:isDefinedBy cs: ;
    skos:definition "An area of land adjacent to the sea, set apart, as by a state or nation, to be preserved in its natural state for the benefit of the public."@en ;
    skos:historyNote "Inherited from ICSM Place Names Working Group's National Feature Catalogue as at 21 December 2023." ;
    skos:inScheme cs: ;
    skos:prefLabel "Coastal Reserve"@en ;
.

go:colony
    a skos:Concept ;
    rdfs:isDefinedBy cs: ;
    skos:altLabel "Wallow"@en ;
    skos:definition "A place where animals gather."@en ;
    skos:historyNote "Inherited from ICSM Place Names Working Group's National Feature Catalogue as at 21 December 2023." ;
    skos:inScheme cs: ;
    skos:prefLabel "Colony"@en ;
.

go:commemorative-tree
    a skos:Concept ;
    rdfs:isDefinedBy cs: ;
    skos:definition "A tree that may have historical significance, may serve as a momento, or may honor individuals or entities."@en ;
    skos:historyNote "Created by separating 'Monument' alternate labels 2024-03-05. Definition adapted from Macquarie Dictionary." ;
    skos:inScheme cs: ;
    skos:prefLabel "Commemorative Tree"@en ;
.

go:commercial-premises
    a skos:Concept ;
    rdfs:isDefinedBy cs: ;
    skos:definition "Places where the major activity is of a commercial nature."@en ;
    skos:historyNote "New concept to replace part of previous concept 'Business' 2024-06-05." ;
    skos:inScheme cs: ;
    skos:narrower
        go:market ,
        go:post-office ,
        go:shopping-centre ;
    skos:prefLabel "Commercial Premises"@en ;
.

go:commune
    a skos:Concept ;
    rdfs:isDefinedBy cs: ;
    skos:definition "A group of families or individuals living together and sharing possessions, interests and or responsibilities."@en ;
    skos:historyNote "Inherited from ICSM Place Names Working Group's National Feature Catalogue as at 21 December 2023." ;
    skos:inScheme cs: ;
    skos:prefLabel "Commune"@en ;
.

go:communication-infrastructure
    a skos:Concept ;
    rdfs:isDefinedBy cs: ;
    skos:definition "Location or equipment facilitating the transmission of information."@en ;
    skos:historyNote "Inherited from ICSM Place Names Working Group's National Feature Catalogue as at 21 December 2023, with name label amended from 'Communication'." ;
    skos:inScheme cs: ;
    skos:narrower
        go:communication-tower ,
        go:fibre-optic-cable ,
        go:radio-communication-facility ,
        go:radio-station ,
        go:telephone-exchange ,
        go:television-communication-facility ,
        go:television-station ;
    skos:prefLabel "Communication Infrastructure"@en ;
.

go:communication-tower
    a skos:Concept ;
    rdfs:isDefinedBy cs: ;
    skos:definition "A structure that supports communication devices."@en ;
    skos:historyNote "Inherited from ICSM Place Names Working Group's National Feature Catalogue as at 21 December 2023." ;
    skos:inScheme cs: ;
    skos:narrower
        go:broadcasting-tower ,
        go:phone-tower ,
        go:radio-mast ;
    skos:prefLabel "Communication Tower"@en ;
.

go:community-centre
    a skos:Concept ;
    rdfs:isDefinedBy cs: ;
    skos:altLabel
        "Community Home"@en ,
        "Multicultural Centre"@en ;
    skos:definition "A building used by members of the community for social gatherings, educational activities."@en ;
    skos:historyNote "Inherited from ICSM Place Names Working Group's National Feature Catalogue as at 21 December 2023." ;
    skos:inScheme cs: ;
    skos:prefLabel "Community Centre"@en ;
.

go:community-facility
    a skos:Concept ;
    rdfs:isDefinedBy cs: ;
    skos:definition "Places to support specific public activities."@en ;
    skos:historyNote "Inherited from ICSM Place Names Working Group's National Feature Catalogue as at 21 December 2023." ;
    skos:inScheme cs: ;
    skos:narrower
        go:ampitheatre ,
        go:arboretum ,
        go:botanic-gardens ,
        go:cemetery ,
        go:community-centre ,
        go:community-gardens ,
        go:conservatory ,
        go:hall ,
        go:library ,
        go:park ,
        go:picnic-site ,
        go:rotunda ,
        go:showground ;
    skos:prefLabel "Community Facility"@en ;
.

go:community-fire-refuge
    a skos:Concept ;
    rdfs:isDefinedBy cs: ;
    skos:definition "A purpose built or modified structure to provide shelter and supplies to community members in the event of a fire-related emergency."@en ;
    skos:historyNote "Created by separating 'Refuge' alternate labels 2024-06-10. Definition adapted from 'Refuge'." ;
    skos:inScheme cs: ;
    skos:prefLabel "Community Fire Refuge"@en ;
.

go:community-gardens
    a skos:Concept ;
    rdfs:isDefinedBy cs: ;
    skos:definition "A piece of land which is managed and encourages members of the community to cultivate primarily for the production of food and to contribute to sustainability."@en ;
    skos:historyNote "Inherited from ICSM Place Names Working Group's National Feature Catalogue as at 21 December 2023." ;
    skos:inScheme cs: ;
    skos:prefLabel "Community Gardens"@en ;
.

go:community-hall
    a skos:Concept ;
    rdfs:isDefinedBy cs: ;
    skos:definition "A hall provided by a community or local government authority for community use."@en ;
    skos:historyNote "Added by Queensland 2024-06-05. Definition from Macquarie Dictionary." ;
    skos:inScheme cs: ;
    skos:prefLabel "Community Hall"@en ;
.

go:community-health-centre
    a skos:Concept ;
    rdfs:isDefinedBy cs: ;
    skos:definition "A health facility that caters for the community, urban and rural."@en ;
    skos:historyNote "Inherited from ICSM Place Names Working Group's National Feature Catalogue as at 21 December 2023." ;
    skos:inScheme cs: ;
    skos:prefLabel "Community Health Centre"@en ;
.

go:community-living
    a skos:Concept ;
    rdfs:isDefinedBy cs: ;
    skos:definition "Places that provide medium to long term accommodation in a structured environment"@en ;
    skos:historyNote "Inherited from ICSM Place Names Working Group's National Feature Catalogue as at 21 December 2023." ;
    skos:inScheme cs: ;
    skos:narrower
        go:commune ,
        go:residential-aged-care ,
        go:retirement-village ;
    skos:prefLabel "Community Living"@en ;
.

go:composting-facility
    a skos:Concept ;
    rdfs:isDefinedBy cs: ;
    skos:definition "A designated site where organic waste, such as yard debris, food scraps, and agricultural waste, is broken down into compost through the process of biological decomposition."@en ;
    skos:historyNote "Created by separating 'Refuse Transfer Station' alternate labels 2024-06-10." ;
    skos:inScheme cs: ;
    skos:prefLabel "Composting Facility"@en ;
.

go:connector-road
    a skos:Concept ;
    rdfs:isDefinedBy cs: ;
    skos:altLabel "Collector Road"@en ;
    skos:definition "Roads that provide for traffic movement between secondary (sub-arterial) and local roads or to distribute traffic to local street systems. Includes rural roads of local significance. These are sometimes known as collector roads."@en ;
    skos:historyNote "Added by Queensland 2024-06-04 from Queensland Roads and Tracks dataset." ;
    skos:inScheme cs: ;
    skos:prefLabel "Connector Road"@en ;
.

go:conservation-park
    a skos:Concept ;
    rdfs:isDefinedBy cs: ;
    skos:altLabel "Biosphere Reserve"@en ;
    skos:definition "An area of land which is not a National Park but is protected to ensure the cultural heritage and/or natural features are safeguarded."@en ;
    skos:historyNote "Inherited from ICSM Place Names Working Group's National Feature Catalogue as at 21 December 2023." ;
    skos:inScheme cs: ;
    skos:prefLabel "Conservation Park"@en ;
.

go:conservatory
    a skos:Concept ;
    rdfs:isDefinedBy cs: ;
    skos:definition "A public building with a glass roof and walls and used for growing delicate plants."@en ;
    skos:historyNote "Inherited from ICSM Place Names Working Group's National Feature Catalogue as at 21 December 2023." ;
    skos:inScheme cs: ;
    skos:prefLabel "Conservatory"@en ;
.

go:continent
    a skos:Concept ;
    rdfs:isDefinedBy cs: ;
    skos:definition "One of the main continuous bodies of land on the earth's surface."@en ;
    skos:historyNote "Inherited from ICSM Place Names Working Group's National Feature Catalogue as at 21 December 2023. Definition from the Oxford English Dictionary." ;
    skos:inScheme cs: ;
    skos:prefLabel "Continent"@en ;
.

go:control-tower
    a skos:Concept ;
    rdfs:isDefinedBy cs: ;
    skos:definition "A tower-shaped building, as at an airport or harbour, from which instructions to planes or ships arriving and departing can be given."@en ;
    skos:historyNote "Inherited from ICSM Place Names Working Group's National Feature Catalogue as at 21 December 2023. Definition adapted from Macquarie Dictionary." ;
    skos:inScheme cs: ;
    skos:narrower
        go:air-traffic-control-tower ,
        go:harbour-control-tower ,
        go:port-control-tower ;
    skos:prefLabel "Control Tower"@en ;
.

go:copse
    a skos:Concept ;
    rdfs:isDefinedBy cs: ;
    skos:altLabel "Coppice"@en ;
    skos:definition "A wood, thicket, or plantation of small trees or bushes."@en ;
    skos:historyNote "Concept created by separating 'Forest' alternate labels 2024-06-11. Definition from Macquarie Dictionary." ;
    skos:inScheme cs: ;
    skos:prefLabel "Copse"@en ;
.

go:coral-reef
    a skos:Concept ;
    rdfs:isDefinedBy cs: ;
    skos:definition "A reef or bank formed by the growth and deposit of coral polyps."@en ;
    skos:historyNote "Added by Queensland 2024-03-05. Definition from Macquarie Dictionary." ;
    skos:inScheme cs: ;
    skos:prefLabel "Coral Reef"@en ;
.

go:corner
    a skos:Concept ;
    rdfs:isDefinedBy cs: ;
    skos:definition "A place where two boundaries meet; a region; a remote place"@en ;
    skos:historyNote "Inherited from ICSM Place Names Working Group's National Feature Catalogue as at 21 December 2023." ;
    skos:inScheme cs: ;
    skos:prefLabel "Corner"@en ;
.

go:county
    a skos:Concept ;
    rdfs:isDefinedBy cs: ;
    skos:definition "A subdivision of Australia into land units."@en ;
    skos:historyNote "Inherited from ICSM Place Names Working Group's National Feature Catalogue as at 21 December 2023." ;
    skos:inScheme cs: ;
    skos:prefLabel "County"@en ;
	skos:scopeNote "No longer in use; recognised for historically named features only.  " ;
.

go:crag
    a skos:Concept ;
    rdfs:isDefinedBy cs: ;
    skos:definition "A steep, rugged rock; a rough, broken, projecting part of a rock."@en ;
    skos:historyNote "Created by separating 'Cliff' alternate labels 2024-05-10. Definition from Macquarie Dictionary." ;
    skos:inScheme cs: ;
    skos:prefLabel "Crag"@en ;
.

go:crater
    a skos:Concept ;
    rdfs:isDefinedBy cs: ;
    skos:definition "A bowl-shaped hollow in the Earth's surface."@en ;
    skos:historyNote "Inherited from ICSM Place Names Working Group's National Feature Catalogue as at 21 December 2023." ;
    skos:inScheme cs: ;
    skos:narrower
        go:meteorite-crater ,
        go:volcanic-crater ;
    skos:prefLabel "Crater"@en ;
.

go:creek
    a skos:Concept ;
    rdfs:isDefinedBy cs: ;
    skos:definition "A defined watercourse, whether flowing or dry according to the season, and whether a single channel or a number of channels; usually of lesser size and length relative to a river and ultimately flowing into another creek or a river."@en ;
    skos:historyNote "Concept created by separating 'Watercourse' alternate labels 2024-06-10. Definition added from Macquarie Dictionary." ;
    skos:inScheme cs: ;
    skos:prefLabel "Creek"@en ;
.

go:cricket-field
    a skos:Concept ;
    rdfs:isDefinedBy cs: ;
    skos:altLabel
        "Cricket Ground"@en ,
        "Cricket Pitch"@en ;
    skos:definition "A place where cricket is played."@en ;
    skos:historyNote "Added by Queensland 2024-06-05." ;
    skos:inScheme cs: ;
    skos:prefLabel "Cricket Field"@en ;
.

go:croquet-green
    a skos:Concept ;
    rdfs:isDefinedBy cs: ;
    skos:definition "An area of land on which the game of Croquet is played."@en ;
    skos:historyNote "Inherited from ICSM Place Names Working Group's National Feature Catalogue as at 21 December 2023." ;
    skos:inScheme cs: ;
    skos:prefLabel "Croquet Green"@en ;
.

go:crossover
    a skos:Concept ;
    rdfs:isDefinedBy cs: ;
    skos:definition "A short roadway connecting two carriageways of a road, often for emergecny service access."@en ;
    skos:historyNote "Added by Queensland 2024-06-04 from Queensland Roads and Tracks dataset." ;
    skos:inScheme cs: ;
    skos:prefLabel "Crossover"@en ;
.

go:cultural-feature
    a skos:Concept ;
    rdfs:isDefinedBy cs: ;
    skos:definition "Places that support activities and interactions of the community."@en ;
    skos:historyNote "Inherited from ICSM Place Names Working Group's National Feature Catalogue as at 21 December 2023, with name label amended 2024-05-04 from 'Culture' 2024-03-05." ;
    skos:inScheme cs: ;
    skos:narrower
        go:accommodations ,
        go:commercial-premises ,
        go:community-facility ,
        go:community-living ,
        go:entertainment-premises ,
        go:landmark ,
        go:place-of-worship ,
        go:recreational-facility ,
        go:tourist-attraction ;
    skos:prefLabel "Cultural Feature"@en ;
    skos:topConceptOf cs: ;
.

go:cycle-crossing
    a skos:Concept ;
    rdfs:isDefinedBy cs: ;
    skos:definition "A designated point on a road or street where cyclists are permitted, and often encouraged, to cross safely from one side to the other."@en ;
    skos:historyNote "Inherited from ICSM Place Names Working Group's National Feature Catalogue as at 21 December 2023. Definition updated 2024-06-10." ;
    skos:inScheme cs: ;
    skos:prefLabel "Cycle Crossing"@en ;
.

go:cyclone-shelter
    a skos:Concept ;
    rdfs:isDefinedBy cs: ;
    skos:definition "A purpose built or modified structure to provide shelter and supplies to community members in the event of a cyclone."@en ;
    skos:historyNote "Created by separating 'Refuge' alternate labels 2024-06-10. Definition adapted from 'Refuge'." ;
    skos:inScheme cs: ;
    skos:prefLabel "Cyclone Shelter"@en ;
.

go:dairy
    a skos:Concept ;
    rdfs:isDefinedBy cs: ;
    skos:definition "A site that processes milk and or milk related products."@en ;
    skos:historyNote "Inherited from ICSM Place Names Working Group's National Feature Catalogue as at 21 December 2023." ;
    skos:inScheme cs: ;
    skos:prefLabel "Dairy"@en ;
.

go:dam
    a skos:Concept ;
    rdfs:isDefinedBy cs: ;
    skos:altLabel
        "Catch"@en ,
        "Farm Bank"@en ,
        "Farm Dam"@en ;
    skos:definition "A small structure in generally undrained areas, built to contain water for stock purposes."@en ;
    skos:historyNote "Inherited from ICSM Place Names Working Group's National Feature Catalogue as at 21 December 2023." ;
    skos:inScheme cs: ;
    skos:prefLabel "Dam"@en ;
.

go:dam-wall
    a skos:Concept ;
    rdfs:isDefinedBy cs: ;
    skos:definition "A large man-made structure of earth, masonry, built across a stream or river to impound water for any purpose."@en ;
    skos:historyNote "Inherited from ICSM Place Names Working Group's National Feature Catalogue as at 21 December 2023." ;
    skos:inScheme cs: ;
    skos:prefLabel "Dam Wall"@en ;
.

go:day-procedure-centre
    a skos:Concept ;
    rdfs:isDefinedBy cs: ;
    skos:altLabel "Day Surgery Centre"@en ;
    skos:definition "A facility which undertakes minor medical procedures that do not require the patient to stay overnight as part of their recovery."@en ;
    skos:historyNote "Inherited from ICSM Place Names Working Group's National Feature Catalogue as at 21 December 2023." ;
    skos:inScheme cs: ;
    skos:prefLabel "Day Procedure Centre"@en ;
.

go:defence-site
    a skos:Concept ;
    rdfs:isDefinedBy cs: ;
    skos:definition "An area of land or facility used for defence operations and/or training."@en ;
    skos:historyNote "Inherited from ICSM Place Names Working Group's National Feature Catalogue as at 21 December 2023, with name label amended 2024-05-04 from 'Defence' 2024-03-05." ;
    skos:inScheme cs: ;
    skos:narrower
        go:air-force-base ,
        go:army-base ,
        go:barracks ,
        go:bombing-range ,
        go:defence-training-area ,
        go:naval-base ;
    skos:prefLabel "Defence Site"@en ;
    skos:topConceptOf cs: ;
.

go:defence-training-area
    a skos:Concept ;
    rdfs:isDefinedBy cs: ;
    skos:definition "An area of land or facility used for the training of defence personnel."@en ;
    skos:historyNote "Inherited from ICSM Place Names Working Group's National Feature Catalogue as at 21 December 2023, with name label amended 2024-05-04 from 'Defence Site' 2024-03-05." ;
    skos:inScheme cs: ;
    skos:prefLabel "Defence Training Area"@en ;
.

go:dental-hospital
    a skos:Concept ;
    rdfs:isDefinedBy cs: ;
    skos:definition "An institution in which medical services for or relating to teeth are delivered."@en ;
    skos:historyNote "Created by separating Hospital alternate labels, definition adapted from Hospital Queensland 2024-03-05." ;
    skos:inScheme cs: ;
    skos:prefLabel "Dental Hospital"@en ;
.

go:depression
    a skos:Concept ;
    rdfs:isDefinedBy cs: ;
    skos:altLabel "Natural Amphitheater"@en ;
    skos:definition "Any hollow or relatively sunken area, on land."@en ;
    skos:historyNote "Inherited from ICSM Place Names Working Group's National Feature Catalogue as at 21 December 2023." ;
    skos:inScheme cs: ;
    skos:prefLabel "Depression"@en ;
.

go:desert
    a skos:Concept ;
    rdfs:isDefinedBy cs: ;
    skos:definition "An almost barren tract of land on which precipitation is so scant or spasmodic that it will not adequately support vegetation."@en ;
    skos:historyNote "Inherited from ICSM Place Names Working Group's National Feature Catalogue as at 21 December 2023." ;
    skos:inScheme cs: ;
    skos:prefLabel "Desert"@en ;
.

go:diplomatic-mission
    a skos:Concept ;
    rdfs:isDefinedBy cs: ;
    skos:altLabel
        "Consulate"@en ,
        "Embassy"@en ,
        "High Commission"@en ;
    skos:definition "Office of a country's diplomatic representatives."@en ;
    skos:historyNote "Inherited from ICSM Place Names Working Group's National Feature Catalogue as at 21 December 2023." ;
    skos:inScheme cs: ;
    skos:prefLabel "Diplomatic Mission"@en ;
.

go:disability-support-facility
    a skos:Concept ;
    rdfs:isDefinedBy cs: ;
    skos:definition "A facility to support the care of those with disabilities."@en ;
    skos:historyNote "Inherited from ICSM Place Names Working Group's National Feature Catalogue as at 21 December 2023, with name label amended 2024-05-04 from 'Disability Support' 2024-03-05." ;
    skos:inScheme cs: ;
    skos:prefLabel "Disability Support Facility"@en ;
.

go:distance-education
    a skos:Concept ;
    rdfs:isDefinedBy cs: ;
    skos:definition "A school delivering teaching to remote locations, usually online or over the telephone."@en ;
    skos:historyNote "Added by Queensland 2024-06-05." ;
    skos:inScheme cs: ;
    skos:prefLabel "Distance Education"@en ;
.

go:distillery
    a skos:Concept ;
    rdfs:isDefinedBy cs: ;
    skos:definition "A place where spirits are manufactured."@en ;
    skos:historyNote "Inherited from ICSM Place Names Working Group's National Feature Catalogue as at 21 December 2023." ;
    skos:inScheme cs: ;
    skos:prefLabel "Distillery"@en ;
.

go:dock
    a skos:Concept ;
    rdfs:isDefinedBy cs: ;
    skos:definition "A structure where a vessel is constructed or repaired."@en ;
    skos:historyNote "Inherited from ICSM Place Names Working Group's National Feature Catalogue as at 21 December 2023." ;
    skos:inScheme cs: ;
    skos:narrower
        go:dry-dock ,
        go:wet-dock ;
    skos:prefLabel "Dock"@en ;
.

go:downs
    a skos:Concept ;
    rdfs:isDefinedBy cs: ;
    skos:definition "Low rolling, grassy, treeless plains."@en ;
    skos:historyNote "Created by separating 'Plain' alternate labels 2024-06-10." ;
    skos:inScheme cs: ;
    skos:prefLabel "Downs"@en ;
.

go:drain
    a skos:Concept ;
    rdfs:isDefinedBy cs: ;
    skos:altLabel
        "Bore Drain"@en ,
        "Culvert"@en ;
    skos:definition "An artificially constructed watercourse designed for the purpose of removing surplus water from the land surface. Can be open or closed."@en ;
    skos:historyNote "Inherited from ICSM Place Names Working Group's National Feature Catalogue as at 21 December 2023." ;
    skos:inScheme cs: ;
    skos:prefLabel "Drain"@en ;
.

go:drive-in-theatre
    a skos:Concept ;
    rdfs:isDefinedBy cs: ;
    skos:altLabel "Drive-In"@en ;
    skos:definition "A place where people can watch films outdoors while sitting in their vehicle."@en ;
    skos:historyNote "Created by separating 'Cinema' alternate labels 2024-03-05." ;
    skos:inScheme cs: ;
    skos:prefLabel "Drive In Theatre"@en ;
.

go:dry-dock
    a skos:Concept ;
    rdfs:isDefinedBy cs: ;
    skos:definition "A basin-like structure from which the water can be removed after the entrance of a ship, used when making repairs on a ship’s bottom, etc."@en ;
    skos:historyNote "Created by separating 'Dock' alternate labels 2024-06-10. Definition from Macquarie Dictionary." ;
    skos:inScheme cs: ;
    skos:prefLabel "Dry Dock"@en ;
.

go:dune
    a skos:Concept ;
    rdfs:isDefinedBy cs: ;
    skos:altLabel
        "Sandhill"@en ,
        "Sandhills"@en ;
    skos:definition "A mound or ridge of drifted sand, occurring on the sea coast, near inland water bodies and in deserts."@en ;
    skos:historyNote "Inherited from ICSM Place Names Working Group's National Feature Catalogue as at 21 December 2023." ;
    skos:inScheme cs: ;
    skos:prefLabel "Dune"@en ;
.

go:early-education
    a skos:Concept ;
    rdfs:isDefinedBy cs: ;
    skos:altLabel
        "Kindergarten"@en ,
        "Preschool"@en ;
    skos:definition "Pre-school to prepare children for primary education."@en ;
    skos:historyNote "Inherited from ICSM Place Names Working Group's National Feature Catalogue as at 21 December 2023, with name label amended 2024-05-04 from 'Early Education' 2024-03-05." ;
    skos:inScheme cs: ;
    skos:prefLabel "Early Education Facility"@en ;
.

go:education-complex
    a skos:Concept ;
    rdfs:isDefinedBy cs: ;
    skos:altLabel "Education Precinct"@en ;
    skos:definition "Education area containing multiple types of education centres."@en ;
    skos:historyNote "Inherited from ICSM Place Names Working Group's National Feature Catalogue as at 21 December 2023." ;
    skos:inScheme cs: ;
    skos:prefLabel "Education Complex"@en ;
.

go:educational-facility
    a skos:Concept ;
    rdfs:isDefinedBy cs: ;
    skos:definition "Places for the delivery of instruction and training."@en ;
    skos:historyNote "Inherited from ICSM Place Names Working Group's National Feature Catalogue as at 21 December 2023, with name label amended 2024-05-04 from 'Education' 2024-03-05." ;
    skos:inScheme cs: ;
    skos:narrower
        go:academy ,
        go:business-college ,
        go:early-education ,
        go:education-complex ,
        go:further-education ,
        go:oeec ,
        go:school ,
        go:school-camp ;
    skos:prefLabel "Educational Facility"@en ;
    skos:topConceptOf cs: ;
.

go:elevated-water-tank
    a skos:Concept ;
    rdfs:isDefinedBy cs: ;
    skos:definition "A large elevated container for the storage of water."@en ;
    skos:historyNote "Concept created by separating 'Water Tank' alternate labels 2024-06-10. Definition added from Macquarie Dictionary." ;
    skos:inScheme cs: ;
    skos:prefLabel "Elevated Water Tank"@en ;
.

go:emergency-complex
    a skos:Concept ;
    rdfs:isDefinedBy cs: ;
    skos:altLabel "Emergency Precinct"@en ;
    skos:definition "Emergency facility area containing multiple types of emergency facilities; each may have its own name."@en ;
    skos:historyNote "Inherited from ICSM Place Names Working Group's National Feature Catalogue as at 21 December 2023." ;
    skos:inScheme cs: ;
    skos:prefLabel "Emergency Complex"@en ;
.

go:emergency-control-centre
    a skos:Concept ;
    rdfs:isDefinedBy cs: ;
    skos:definition "A facility to coordinate multiple agencies."@en ;
    skos:historyNote "Inherited from ICSM Place Names Working Group's National Feature Catalogue as at 21 December 2023." ;
    skos:inScheme cs: ;
    skos:prefLabel "Emergency Control Centre"@en ;
.

go:emergency-facility
    a skos:Concept ;
    rdfs:isDefinedBy cs: ;
    skos:definition "Places for the governance of emergency services."@en ;
    skos:historyNote "Inherited from ICSM Place Names Working Group's National Feature Catalogue as at 21 December 2023, with name label amended 2024-05-04 from 'Emergency' 2024-03-05." ;
    skos:inScheme cs: ;
    skos:narrower
        go:ambulance-station ,
        go:coast-guard-facility ,
        go:emergency-complex ,
        go:emergency-control-centre ,
        go:fire-lookout ,
        go:fire-station ,
        go:lifesaving-club ,
        go:neighbourhood-safer-place ,
        go:police-station ,
        go:refuge ,
        go:ses-facility ;
    skos:prefLabel "Emergency Facility"@en ;
    skos:topConceptOf cs: ;
.

go:energy-infrastructure
    a skos:Concept ;
    rdfs:isDefinedBy cs: ;
    skos:definition "Facilities related to the generation/transmission/storage of power."@en ;
    skos:historyNote "Inherited from ICSM Place Names Working Group's National Feature Catalogue as at 21 December 2023, with name label amended from 'Energy'." ;
    skos:inScheme cs: ;
    skos:narrower
        go:gas-plant ,
        go:pipeline ,
        go:power-distribution-line ,
        go:power-station ,
        go:power-sub-station ,
        go:power-sub-transmission-line ,
        go:power-terminal-station ,
        go:power-transmission-line ,
        go:wind-turbine ;
    skos:prefLabel "Energy Infrastructure"@en ;
.

go:entertainment-centre
    a skos:Concept ;
    rdfs:isDefinedBy cs: ;
    skos:altLabel
        "Conference Centre"@en ,
        "Exhibition Centre"@en ,
        "Theatre"@en ;
    skos:definition "A place for where the public can be entertained and or be educated."@en ;
    skos:historyNote "Inherited from ICSM Place Names Working Group's National Feature Catalogue as at 21 December 2023." ;
    skos:inScheme cs: ;
    skos:prefLabel "Entertainment Centre"@en ;
.

go:entertainment-premises
    a skos:Concept ;
    rdfs:isDefinedBy cs: ;
    skos:definition "Places where the major activity is provision of entertainment."@en ;
    skos:historyNote "New concept to replace part of previous concept 'Business' 2024-06-05." ;
    skos:inScheme cs: ;
    skos:narrower
        go:cinema ,
        go:entertainment-centre ,
        go:racetrack ;
    skos:prefLabel "Entertainment Premises"@en ;
.

go:entrance
    a skos:Concept ;
    rdfs:isDefinedBy cs: ;
    skos:definition "A passageway into enclosed waters."@en ;
    skos:historyNote "Inherited from ICSM Place Names Working Group's National Feature Catalogue as at 21 December 2023." ;
    skos:inScheme cs: ;
    skos:prefLabel "Entrance"@en ;
.

go:equestrian-centre
    a skos:Concept ;
    rdfs:isDefinedBy cs: ;
    skos:definition "A place related to horses and riding."@en ;
    skos:historyNote "Inherited from ICSM Place Names Working Group's National Feature Catalogue as at 21 December 2023." ;
    skos:inScheme cs: ;
    skos:prefLabel "Equestrian Centre"@en ;
.

go:escarpment
    a skos:Concept ;
    rdfs:isDefinedBy cs: ;
    skos:altLabel "Scarp"@en ;
    skos:definition "The steep slope terminating a plateau or any level or upland surface."@en ;
    skos:historyNote "Inherited from ICSM Place Names Working Group's National Feature Catalogue as at 21 December 2023." ;
    skos:inScheme cs: ;
    skos:narrower go:marine-escarpment ;
    skos:prefLabel "Escarpment"@en ;
.

go:estuary
    a skos:Concept ;
    rdfs:isDefinedBy cs: ;
    skos:definition "The portion of a river where tidal effects are evident and where fresh water and sea water mix; the widening out lower portion of a tidal river."@en ;
    skos:historyNote "Inherited from ICSM Place Names Working Group's National Feature Catalogue as at 21 December 2023." ;
    skos:inScheme cs: ;
    skos:prefLabel "Estuary"@en ;
.

go:eye-and-ear-hospital
    a skos:Concept ;
    rdfs:isDefinedBy cs: ;
    skos:definition "An institution in which medical services for or relating to eyes or ears are delivered."@en ;
    skos:historyNote "Created by separating Hospital alternate labels, definition adapted from Hospital Queensland 2024-03-05." ;
    skos:inScheme cs: ;
    skos:prefLabel "Eye and Ear Hospital"@en ;
.

go:farm
    a skos:Concept ;
    rdfs:isDefinedBy cs: ;
    skos:altLabel
        "Agriculture Establishment"@en ,
        "Research Establishment"@en ,
        "Special Purpose Farm"@en ;
    skos:definition "A tract of land devoted for agricultural or horticultural purposes."@en ;
    skos:historyNote "Inherited from ICSM Place Names Working Group's National Feature Catalogue as at 21 December 2023." ;
    skos:inScheme cs: ;
    skos:prefLabel "Farm"@en ;
.

go:federal-electorate
    a skos:Concept ;
    rdfs:isDefinedBy cs: ;
    skos:definition "An administrative area of Australia represented by a member of Parliament elected at a House of Representatives election."@en ;
    skos:historyNote "Inherited from ICSM Place Names Working Group's National Feature Catalogue as at 21 December 2023." ;
    skos:inScheme cs: ;
    skos:prefLabel "Federal Electorate"@en ;
.

go:fence
    a skos:Concept ;
    rdfs:isDefinedBy cs: ;
    skos:definition "A structure used to enclose an area."@en ;
    skos:historyNote "Inherited from ICSM Place Names Working Group's National Feature Catalogue as at 21 December 2023." ;
    skos:inScheme cs: ;
    skos:prefLabel "Fence"@en ;
.

go:ferry-route
    a skos:Concept ;
    rdfs:isDefinedBy cs: ;
    skos:definition "The set route taken by a ferry service."@en ;
    skos:historyNote "Inherited from ICSM Place Names Working Group's National Feature Catalogue as at 21 December 2023." ;
    skos:inScheme cs: ;
    skos:narrower
        go:passenger-ferry-route ,
        go:vehicular-ferry-route ;
    skos:prefLabel "Ferry Route"@en ;
.

go:ferry-transport-infrastructure
    a skos:Concept ;
    rdfs:isDefinedBy cs: ;
    skos:definition "Physical structures, facilities, and systems that support the operation of ferry services."@en ;
    skos:historyNote "Broader concept introduced 2024-06-04." ;
    skos:inScheme cs: ;
    skos:narrower
        go:ferry-route ,
        go:ferry-station ;
    skos:prefLabel "Ferry Transport Infrastructure"@en ;
.

go:fibre-optic-cable
    a skos:Concept ;
    rdfs:isDefinedBy cs: ;
    skos:definition "A cable used for the distribution of digital communications."@en ;
    skos:historyNote "Inherited from ICSM Place Names Working Group's National Feature Catalogue as at 21 December 2023." ;
    skos:inScheme cs: ;
    skos:prefLabel "Fibre Optic Cable"@en ;
.

go:fire-lookout
    a skos:Concept ;
    rdfs:isDefinedBy cs: ;
    skos:altLabel
        "Fire Tower"@en ,
        "Observation Tower"@en ;
    skos:definition "A high structure used to observe an area for indications of fire."@en ;
    skos:historyNote "Inherited from ICSM Place Names Working Group's National Feature Catalogue as at 21 December 2023." ;
    skos:inScheme cs: ;
    skos:prefLabel "Fire Lookout"@en ;
.

go:fire-station
    a skos:Concept ;
    rdfs:isDefinedBy cs: ;
    skos:definition "A building in which a fire brigade is based, and which houses fire engines and other equipment."@en ;
    skos:historyNote "Inherited from ICSM Place Names Working Group's National Feature Catalogue as at 21 December 2023." ;
    skos:inScheme cs: ;
    skos:narrower
        go:forest-industry-fire-station ,
        go:rural-fire-station ;
    skos:prefLabel "Fire Station"@en ;
.

go:firebreak
    a skos:Concept ;
    rdfs:isDefinedBy cs: ;
    skos:altLabel
        "Fire Break"@en ,
        "Fireguard"@en ;
    skos:definition "A strip of ploughed or cleared land made to check the spread of fire."@en ;
    skos:historyNote "Inherited from ICSM Place Names Working Group's National Feature Catalogue as at 21 December 2023." ;
    skos:inScheme cs: ;
    skos:prefLabel "Firebreak"@en ;
.

go:firing-range
    a skos:Concept ;
    rdfs:isDefinedBy cs: ;
    skos:altLabel
        "Rifle Range"@en ,
        "Shooting Range"@en ;
    skos:definition "An area set aside for shooting practice."@en ;
    skos:historyNote "Inherited from ICSM Place Names Working Group's National Feature Catalogue as at 21 December 2023." ;
    skos:inScheme cs: ;
    skos:prefLabel "Firing Range"@en ;
.

go:fitness-centre
    a skos:Concept ;
    rdfs:isDefinedBy cs: ;
    skos:altLabel "Gym"@en ;
    skos:definition "A gym designed for people who work to maintain a level of fitness."@en ;
    skos:historyNote "Created by separating 'Sports Facility' alternate labels 2024-05-10. Definition from Macquarie Dictionary." ;
    skos:inScheme cs: ;
    skos:prefLabel "Fitness Centre"@en ;
.

go:fjord
    a skos:Concept ;
    rdfs:isDefinedBy cs: ;
    skos:definition "A long narrow inlet of the sea between high steep cliffs."@en ;
    skos:historyNote "Inherited from ICSM Place Names Working Group's National Feature Catalogue as at 21 December 2023." ;
    skos:inScheme cs: ;
    skos:prefLabel "Fjord"@en ;
.

go:football-field
    a skos:Concept ;
    rdfs:isDefinedBy cs: ;
    skos:altLabel
        "Football Ground"@en ,
        "Football Pitch"@en ;
    skos:definition "A place where football is played."@en ;
    skos:historyNote "Added by Queensland 2024-06-05." ;
    skos:inScheme cs: ;
    skos:prefLabel "Football Field"@en ;
.

go:footbridge
    a skos:Concept ;
    rdfs:isDefinedBy cs: ;
    skos:definition "A structure spanning a rail line, river, road or the like affording safe passage for pedestrians."@en ;
    skos:historyNote "Inherited from ICSM Place Names Working Group's National Feature Catalogue as at 21 December 2023." ;
    skos:inScheme cs: ;
    skos:prefLabel "Footbridge"@en ;
.

go:ford
    a skos:Concept ;
    rdfs:isDefinedBy cs: ;
    skos:definition "The shallow part of a river or other body of water which may be crossed by vehicle or by wading."@en ;
    skos:historyNote "Inherited from ICSM Place Names Working Group's National Feature Catalogue as at 21 December 2023." ;
    skos:inScheme cs: ;
    skos:prefLabel "Ford"@en ;
.

go:foreshore
    a skos:Concept ;
    rdfs:isDefinedBy cs: ;
    skos:definition "The part of the shore between the ordinary high-water mark and low-water mark."@en ;
    skos:historyNote "Created by separating 'Coast' alternate labels 2024-03-05. Definition from Macquarie Dictionary." ;
    skos:inScheme cs: ;
    skos:prefLabel "Foreshore"@en ;
.

go:forest
    a skos:Concept ;
    rdfs:isDefinedBy cs: ;
    skos:definition "A large wooded area having a thick growth of trees and plants."@en ;
    skos:historyNote "Inherited from ICSM Place Names Working Group's National Feature Catalogue as at 21 December 2023." ;
    skos:inScheme cs: ;
    skos:prefLabel "Forest"@en ;
.

go:forest-industry-fire-station
    a skos:Concept ;
    rdfs:isDefinedBy cs: ;
    skos:definition "A building related to forestry operations from which forestry fire fighting operations are coordinated, and which houses fire fighting vehicles and related equipment."@en ;
    skos:historyNote "Created by separating 'Fire Station' alternate labels 2024-03-05." ;
    skos:inScheme cs: ;
    skos:prefLabel "Forest Industry Fire Station"@en ;
.

go:fountain
    a skos:Concept ;
    rdfs:isDefinedBy cs: ;
    skos:definition "A structure that incorporates a reservoir to supply liquid gradually or continuously to a number of mechanically created jets or streams which make liquid spout or rise from an opening within the structure. Typically for ornamental purpose but may also provide utility such as supplying water for use or for cooling the air."@en ;
    skos:historyNote "Created by separating 'Monument' alternate labels 2024-03-05. Definition adapted from Macquarie Dictionary." ;
    skos:inScheme cs: ;
    skos:prefLabel "Fountain"@en ;
.

go:freshwater-lagoon
    a skos:Concept ;
    rdfs:isDefinedBy cs: ;
    skos:definition "An enclosed area of fresh water which is partly or completely separated from the sea."@en ;
    skos:historyNote "Created by separating 'Lagoon' alternate labels 2024-05-10." ;
    skos:inScheme cs: ;
    skos:prefLabel "Fresh Water Lagoon"@en ;
.

go:further-education
    a skos:Concept ;
    rdfs:isDefinedBy cs: ;
    skos:altLabel "Further Education Facility"@en ;
    skos:definition "Post secondary education facility."@en ;
    skos:historyNote "Inherited from ICSM Place Names Working Group's National Feature Catalogue as at 21 December 2023, with name label amended 2024-05-04 from 'Further Education' 2024-03-05." ;
    skos:inScheme cs: ;
    skos:narrower
        go:tafe-facility ,
        go:university ;
    skos:prefLabel "Tertiary Education Facility"@en ;
.

go:gas-field
    a skos:Concept ;
    rdfs:isDefinedBy cs: ;
    skos:definition "An area in which gas resources have been identified."@en ;
    skos:historyNote "Created by separating 'Oil and Gas Field' alternate labels 2024-03-05." ;
    skos:inScheme cs: ;
    skos:prefLabel "Gas Field"@en ;
.

go:gas-pipeline
    a skos:Concept ;
    rdfs:isDefinedBy cs: ;
    skos:definition "A long pipe, typically underground, used to transport gas over long distances."@en ;
    skos:historyNote "Inherited from ICSM Place Names Working Group's National Feature Catalogue as at 21 December 2023." ;
    skos:inScheme cs: ;
    skos:prefLabel "Gas Pipeline"@en ;
.

go:gas-plant
    a skos:Concept ;
    rdfs:isDefinedBy cs: ;
    skos:altLabel
        "Gas Conditioning Plant"@en ,
        "Gas Processing Plant"@en ;
    skos:definition "A place where gas is processed and/ or stored ."@en ;
    skos:historyNote "Inherited from ICSM Place Names Working Group's National Feature Catalogue as at 21 December 2023." ;
    skos:inScheme cs: ;
    skos:prefLabel "Gas Plant"@en ;
.

go:gas-platform
    a skos:Concept ;
    rdfs:isDefinedBy cs: ;
    skos:definition "A large structure with facilities to drill wells, to extract and process natural gas."@en ;
    skos:historyNote "Created by separating 'Oil and Gas Platform' alternate labels 2024-03-05." ;
    skos:inScheme cs: ;
    skos:prefLabel "Gas Platform"@en ;
.

go:gas-power-station
    a skos:Concept ;
    rdfs:isDefinedBy cs: ;
    skos:definition "A process plant that creates power from gas."@en ;
    skos:historyNote "Created by separating 'Power Station' alternate labels 2024-03-05." ;
    skos:inScheme cs: ;
    skos:prefLabel "Gas Power Station"@en ;
.

go:gas-well
    a skos:Concept ;
    rdfs:isDefinedBy cs: ;
    skos:definition "A hole drilled into the ground to extract gas."@en ;
    skos:historyNote "Created by separating 'Oil and Gas Well' alternate labels 2024-03-05." ;
    skos:inScheme cs: ;
    skos:prefLabel "Gas Well"@en ;
.

go:gate
    a skos:Concept ;
    rdfs:isDefinedBy cs: ;
    skos:definition "A structure used to regulate movement associated with road or track."@en ;
    skos:historyNote "Inherited from ICSM Place Names Working Group's National Feature Catalogue as at 21 December 2023." ;
    skos:inScheme cs: ;
    skos:prefLabel "Gate"@en ;
.

go:general-hospital
    a skos:Concept ;
    rdfs:isDefinedBy cs: ;
    skos:definition "An institution in which sick or injured persons are given medical or surgical treatment."@en ;
    skos:historyNote "Inherited from ICSM Place Names Working Group's National Feature Catalogue as at 21 December 2023." ;
    skos:inScheme cs: ;
    skos:prefLabel "General Hospital"@en ;
.

go:general-hospital-emergency
    a skos:Concept ;
    rdfs:isDefinedBy cs: ;
    skos:definition "A general hospital with 24-hour emergency service."@en ;
    skos:historyNote "Inherited from ICSM Place Names Working Group's National Feature Catalogue as at 21 December 2023." ;
    skos:inScheme cs: ;
    skos:prefLabel "General Hospital with Emergency"@en ;
.

go:geothermal-power-station
    a skos:Concept ;
    rdfs:isDefinedBy cs: ;
    skos:definition "A process plant that creates power from geothermal sources."@en ;
    skos:historyNote "Created by separating 'Power Station' alternate labels 2024-03-05." ;
    skos:inScheme cs: ;
    skos:prefLabel "Geothermal Power Station"@en ;
.

go:glacier
    a skos:Concept ;
    rdfs:isDefinedBy cs: ;
    skos:definition "A mass of snow and ice continuously moving from higher to lower ground or, if afloat, continuously spreading."@en ;
    skos:historyNote "Inherited from ICSM Place Names Working Group's National Feature Catalogue as at 21 December 2023. Concept and definition from the Australian Antarctic Division." ;
    skos:inScheme cs: ;
    skos:prefLabel "Glacier"@en ;
    schema:citation "https://data.aad.gov.au/aadc/ftc/display_feature_type.cfm?feature_type_code=196"^^xsd:anyURI ;
.

go:glade
    a skos:Concept ;
    rdfs:isDefinedBy cs: ;
    skos:definition "An open space in a forest."@en ;
    skos:historyNote "Concept created by separating 'Forest' alternate labels 2024-06-11. Definition from Macquarie Dictionary." ;
    skos:inScheme cs: ;
    skos:prefLabel "Glade"@en ;
.

go:gnamma-hole
    a skos:Concept ;
    rdfs:isDefinedBy cs: ;
    skos:definition "A depression in rock, especially granite, forming a natural reservoir, specific to Australia. A depression that holds water, often found on top of boulders or rock surfaces."@en ;
    skos:historyNote "Created by separating 'Rockhole' alternate labels 2024-06-10. Definition adapted from Macquarie Dictionary." ;
    skos:inScheme cs: ;
    skos:prefLabel "Gnamma Hole"@en ;
.

go:gold-field
    a skos:Concept ;
    rdfs:isDefinedBy cs: ;
    skos:definition "An area in which gold deposits have been found and where mines have been established."@en ;
    skos:historyNote "Inherited from ICSM Place Names Working Group's National Feature Catalogue as at 21 December 2023." ;
    skos:inScheme cs: ;
    skos:prefLabel "Gold Field"@en ;
.

go:gold-refinery
    a skos:Concept ;
    rdfs:isDefinedBy cs: ;
    skos:definition "A refinery for extracting gold."@en ;
    skos:historyNote "Inherited from ICSM Place Names Working Group's National Feature Catalogue as at 21 December 2023." ;
    skos:inScheme cs: ;
    skos:prefLabel "Gold Refinery"@en ;
.

go:golf-course
    a skos:Concept ;
    rdfs:isDefinedBy cs: ;
    skos:altLabel "Golf Driving Range"@en ;
    skos:definition "A ground or course over which golf is played."@en ;
    skos:historyNote "Inherited from ICSM Place Names Working Group's National Feature Catalogue as at 21 December 2023." ;
    skos:inScheme cs: ;
    skos:prefLabel "Golf Course"@en ;
.

go:gorge
    a skos:Concept ;
    rdfs:isDefinedBy cs: ;
    skos:altLabel
        "Canyon"@en ,
        "Chasm"@en ,
        "Ravine"@en ;
    skos:definition "A valley which is more than usually deep and narrow, with steep walls."@en ;
    skos:historyNote "Inherited from ICSM Place Names Working Group's National Feature Catalogue as at 21 December 2023." ;
    skos:inScheme cs: ;
    skos:prefLabel "Gorge"@en ;
.

go:grandstand
    a skos:Concept ;
    rdfs:isDefinedBy cs: ;
    skos:definition "A terraced block of seats, usually under a roof, commanding the best view."@en ;
    skos:historyNote "Inherited from ICSM Place Names Working Group's National Feature Catalogue as at 21 December 2023." ;
    skos:inScheme cs: ;
    skos:prefLabel "Grandstand"@en ;
.

go:grassland
    a skos:Concept ;
    rdfs:isDefinedBy cs: ;
    skos:definition "An area in which the natural vegetation consists primarily of perennial grasses."@en ;
    skos:historyNote "Inherited from ICSM Place Names Working Group's National Feature Catalogue as at 21 December 2023." ;
    skos:inScheme cs: ;
    skos:prefLabel "Grassland"@en ;
.

go:greyhound-racetrack
    a skos:Concept ;
    rdfs:isDefinedBy cs: ;
    skos:altLabel "Dog Track"@en ;
    skos:definition "A track enclosed by rails with start and finish points over which a specific bread of dog is raced."@en ;
    skos:historyNote "Inherited from ICSM Place Names Working Group's National Feature Catalogue as at 21 December 2023." ;
    skos:inScheme cs: ;
    skos:prefLabel "Greyhound Racetrack"@en ;
.

go:grotto
    a skos:Concept ;
    rdfs:isDefinedBy cs: ;
    skos:definition "A small picturesque cave, often next to water, that's generally associated with an idyllic or tranquil atmosphere."@en ;
    skos:historyNote "Created by separating 'Cave' alternate labels 2024-03-05. Definition adapted from Macquarie Dictionary." ;
    skos:inScheme cs: ;
    skos:prefLabel "Grotto"@en ;
.

go:group-camp
    a skos:Concept ;
    rdfs:isDefinedBy cs: ;
    skos:altLabel "Scout Camp"@en ;
    skos:definition "A place where tents, cabins, or other temporary structures are erected for the use by a particular group."@en ;
    skos:historyNote "Inherited from ICSM Place Names Working Group's National Feature Catalogue as at 21 December 2023." ;
    skos:inScheme cs: ;
    skos:prefLabel "Group Camp"@en ;
.

go:grove
    a skos:Concept ;
    rdfs:isDefinedBy cs: ;
    skos:definition "A small wood or plantation of trees, often found within a park or a garden."@en ;
    skos:historyNote "Concept created by separating 'Forest' alternate labels 2024-06-11. Definition adapted from Macquarie Dictionary." ;
    skos:inScheme cs: ;
    skos:prefLabel "Grove"@en ;
.

go:gulf
    a skos:Concept ;
    rdfs:isDefinedBy cs: ;
    skos:altLabel "Bight"@en ;
    skos:definition "An area of sea partly enclosed by land, taking the form of a long narrow stretch of water larger than a loop."@en ;
    skos:historyNote "Inherited from ICSM Place Names Working Group's National Feature Catalogue as at 21 December 2023." ;
    skos:inScheme cs: ;
    skos:prefLabel "Gulf"@en ;
.

go:gully
    a skos:Concept ;
    rdfs:isDefinedBy cs: ;
    skos:definition "A watercourse in a steep-sided ravine or fissure cut into the side of a mountain by the action of running water."@en ;
    skos:historyNote "Concept created by separating 'Watercourse' alternate labels 2024-06-10. Definition amended from Macquarie Dictionary." ;
    skos:inScheme cs: ;
    skos:prefLabel "Gully"@en ;
.

go:gurdwara
    a skos:Concept ;
    rdfs:isDefinedBy cs: ;
    skos:definition "Sikh place of worship."@en ;
    skos:historyNote "Inherited from ICSM Place Names Working Group's National Feature Catalogue as at 21 December 2023. Definition from Macquarie Dictionary." ;
    skos:inScheme cs: ;
    skos:prefLabel "Gurdwara"@en ;
.

go:hall
    a skos:Concept ;
    rdfs:isDefinedBy cs: ;
    skos:definition "A large building or room for public assembly and other community uses."@en ;
    skos:historyNote "Added by Queensland 2024-06-05. Definition from Macquarie Dictionary." ;
    skos:inScheme cs: ;
    skos:narrower
        go:community-hall ,
        go:town-hall ;
    skos:prefLabel "Hall"@en ;
.

go:hangar
    a skos:Concept ;
    rdfs:isDefinedBy cs: ;
    skos:definition "Facility for housing aircraft and or associated infrastructure."@en ;
    skos:historyNote "Inherited from ICSM Place Names Working Group's National Feature Catalogue as at 21 December 2023." ;
    skos:inScheme cs: ;
    skos:prefLabel "Hangar"@en ;
.

go:harbour
    a skos:Concept ;
    rdfs:isDefinedBy cs: ;
    skos:definition "An artificially improved body of water providing protection for vessels, and often anchorage and docking facilities."@en ;
    skos:historyNote "Inherited from ICSM Place Names Working Group's National Feature Catalogue as at 21 December 2023." ;
    skos:inScheme cs: ;
    skos:prefLabel "Harbour"@en ;
.

go:harness-racetrack
    a skos:Concept ;
    rdfs:isDefinedBy cs: ;
    skos:altLabel "Trotting Track"@en ;
    skos:definition "A track enclosed by rails with start and finish points over which standardbred horses are harnessed to race."@en ;
    skos:historyNote "Inherited from ICSM Place Names Working Group's National Feature Catalogue as at 21 December 2023." ;
    skos:inScheme cs: ;
    skos:prefLabel "Harness Racetrack"@en ;
.

go:hatchery
    a skos:Concept ;
    rdfs:isDefinedBy cs: ;
    skos:definition "A facility for artificially breeding, hatching, and rearing fish and shellfish in their early life stages."@en ;
    skos:historyNote "Created by separating 'Aquaculture' alternate labels 2024-03-05." ;
    skos:inScheme cs: ;
    skos:prefLabel "Hatchery"@en ;
.

go:health-facility
    a skos:Concept ;
    rdfs:isDefinedBy cs: ;
    skos:definition "A facility that supports medical treatment and services."@en ;
    skos:historyNote "Inherited from ICSM Place Names Working Group's National Feature Catalogue as at 21 December 2023, with name label amended 2024-05-04 from 'Health' 2024-03-05." ;
    skos:inScheme cs: ;
    skos:narrower
        go:community-health-centre ,
        go:hospital ,
        go:maternal-and-child-health-centre ,
        go:medical-centre ;
    skos:prefLabel "Health Facility"@en ;
    skos:topConceptOf cs: ;
.

go:helipad
    a skos:Concept ;
    rdfs:isDefinedBy cs: ;
    skos:definition "A place for helicopters to land and take-off, like 'runway' is to 'airport'."@en ;
    skos:historyNote "Inherited from ICSM Place Names Working Group's National Feature Catalogue as at 21 December 2023." ;
    skos:inScheme cs: ;
    skos:prefLabel "Helipad"@en ;
.

go:heliport
    a skos:Concept ;
    rdfs:isDefinedBy cs: ;
    skos:definition "An airport for helicopters."@en ;
    skos:historyNote "Inherited from ICSM Place Names Working Group's National Feature Catalogue as at 21 December 2023." ;
    skos:inScheme cs: ;
    skos:prefLabel "Heliport"@en ;
.

go:highway
    a skos:Concept ;
    rdfs:isDefinedBy cs: ;
    skos:altLabel "Arterial Road"@en ;
    skos:definition "Roads which are of importance in a national sense, and/or are a major interstate through route, and/or are principal connector roads between capitals and/or major regions and or key towns/commercial centres/inter-transport hubs. This category encompasses what are sometimes referred to as arterial roads."@en ;
    skos:historyNote "Added by Queensland 2024-06-04 from Queensland Roads and Tracks dataset." ;
    skos:inScheme cs: ;
    skos:prefLabel "Highway"@en ;
.

go:hill
    a skos:Concept ;
    rdfs:isDefinedBy cs: ;
    skos:definition "A small portion of the Earth's surface elevated above its surroundings. In general, a feature is not considered a mountain unless its elevation, from foot to summit, is well over 300m, but the distinction is arbitrary."@en ;
    skos:historyNote "Inherited from ICSM Place Names Working Group's National Feature Catalogue as at 21 December 2023." ;
    skos:inScheme cs: ;
    skos:narrower
        go:butte ,
        go:knob ,
        go:knoll ,
        go:marine-hill ,
        go:mesa ,
        go:sugarloaf ,
        go:tor ;
    skos:prefLabel "Hill"@en ;
.

go:hillside
    a skos:Concept ;
    rdfs:isDefinedBy cs: ;
    skos:definition "The side or slope of a hill."@en ;
    skos:historyNote "Created by separating 'Slope' alternate labels 2024-06-10. Definition from Macquarie Dictionary." ;
    skos:inScheme cs: ;
    skos:prefLabel "Hillside"@en ;
.

go:historic-site
    a skos:Concept ;
    rdfs:isDefinedBy cs: ;
    skos:altLabel "Ruin"@en ;
    skos:definition "A specific place or site which has at one time been the site of an event or activity which is now remembered or commemorated."@en ;
    skos:historyNote "Inherited from ICSM Place Names Working Group's National Feature Catalogue as at 21 December 2023." ;
    skos:inScheme cs: ;
    skos:prefLabel "Historic Site"@en ;
.

go:hockey-field
    a skos:Concept ;
    rdfs:isDefinedBy cs: ;
    skos:altLabel
        "Hockey Ground"@en ,
        "Hockey Pitch"@en ;
    skos:definition "A place where hockey is played."@en ;
    skos:historyNote "Inherited from ICSM Place Names Working Group's National Feature Catalogue as at 21 December 2023." ;
    skos:inScheme cs: ;
    skos:prefLabel "Hockey Field"@en ;
.

go:holiday-park
    a skos:Concept ;
    rdfs:isDefinedBy cs: ;
    skos:altLabel "Tourist Park"@en ;
    skos:definition "A site for holidaymakers which offers various types of accommodation including caravan or tent sites."@en ;
    skos:historyNote "Created by separating 'Caravan Park' alternate labels 2024-03-05." ;
    skos:inScheme cs: ;
    skos:narrower go:caravan-park ;
    skos:prefLabel "Holiday Park"@en ;
.

go:homestead
    a skos:Concept ;
    rdfs:isDefinedBy cs: ;
    skos:definition "A main residence on a rural property."@en ;
    skos:historyNote "Inherited from ICSM Place Names Working Group's National Feature Catalogue as at 21 December 2023, with 'horticultural or agricultural farm' amended to 'rural property' in description for continuity." ;
    skos:inScheme cs: ;
    skos:prefLabel "Homestead"@en ;
.

go:horse-riding-trail
    a skos:Concept ;
    rdfs:isDefinedBy cs: ;
    skos:altLabel
        "Bridle Path"@en ,
        "Bridleway"@en ;
    skos:definition "A non-vehicular trail designed for horse riding traffic in the main."@en ;
    skos:historyNote "Inherited from ICSM Place Names Working Group's National Feature Catalogue as at 21 December 2023, with 'non vehicular' appended to description 2024-05-04." ;
    skos:inScheme cs: ;
    skos:prefLabel "Horse Riding Trail"@en ;
.

go:hospital
    a skos:Concept ;
    rdfs:isDefinedBy cs: ;
    skos:definition "An institution in which sick or injured persons are given medical or surgical treatment."@en ;
    skos:historyNote "Added by Queensland 2024-03-05. Definition from Macquarie Dictionary." ;
    skos:inScheme cs: ;
    skos:narrower
        go:bush-nursing-hospital ,
        go:day-procedure-centre ,
        go:general-hospital ,
        go:general-hospital-emergency ,
        go:hospital-complex ,
        go:specialised-hospital ;
    skos:prefLabel "Hospital"@en ;
.

go:hospital-complex
    a skos:Concept ;
    rdfs:isDefinedBy cs: ;
    skos:altLabel "Hospital Precinct"@en ;
    skos:definition "An area containing multiple hospitals."@en ;
    skos:historyNote "Inherited from ICSM Place Names Working Group's National Feature Catalogue as at 21 December 2023." ;
    skos:inScheme cs: ;
    skos:prefLabel "Hospital Complex"@en ;
.

go:hot-spring
    a skos:Concept ;
    rdfs:isDefinedBy cs: ;
    skos:definition "A naturally heated spring, often containing mineral substances in solution."@en ;
    skos:historyNote "Concept created by separating 'Spring' alternate labels 2024-06-10. Definition added from Macquarie Dictionary." ;
    skos:inScheme cs: ;
    skos:prefLabel "Hot Spring"@en ;
.

go:hut
    a skos:Concept ;
    rdfs:isDefinedBy cs: ;
    skos:definition "A simple, usually small, building which may be used for temporary accommodation, as for bushwalkers or skiers."@en ;
    skos:historyNote "Inherited from ICSM Place Names Working Group's National Feature Catalogue as at 21 December 2023." ;
    skos:inScheme cs: ;
    skos:prefLabel "Hut"@en ;
.

go:hydroelectric-power-station
    a skos:Concept ;
    rdfs:isDefinedBy cs: ;
    skos:altLabel "Hydro Power Station"@en ;
    skos:definition "A process plant that creates power from gravity induced flow of water."@en ;
    skos:historyNote "Created by separating 'Power Station' alternate labels 2024-03-05." ;
    skos:inScheme cs: ;
    skos:prefLabel "Hydroelectric Power Station"@en ;
.

go:hydrological-feature
    a skos:Concept ;
    rdfs:isDefinedBy cs: ;
    skos:definition "Natural or man-made places which relate to the surface and underground water or marine environments."@en ;
    skos:historyNote "Inherited from ICSM Place Names Working Group's National Feature Catalogue as at 21 December 2023, with name label amended 2024-05-04 from 'Hydrology' 2024-03-05." ;
    skos:inScheme cs: ;
    skos:narrower
        go:anchorage ,
        go:waterbody ,
        go:water-infrastructure ,
        go:water-point ,
        go:waterway ;
    skos:prefLabel "Hydrological Feature"@en ;
    skos:topConceptOf cs: ;
.

go:ice-dome
    a skos:Concept ;
    rdfs:isDefinedBy cs: ;
    skos:definition "A rounded and gently sloping elevation in the surface of an inland ice sheet. Ice domes do not have precisely defined margins and may cover very large areas - more than 100,000km sq."@en ;
    skos:historyNote "Inherited from ICSM Place Names Working Group's National Feature Catalogue as at 21 December 2023. Concept and definition from the Australian Antarctic Division." ;
    skos:inScheme cs: ;
    skos:prefLabel "Ice Dome"@en ;
    schema:citation "https://data.aad.gov.au/aadc/ftc/display_feature_type.cfm?feature_type_code=167"^^xsd:anyURI ;
.

go:ice-feature
    a skos:Concept ;
    rdfs:isDefinedBy cs: ;
    skos:definition "Feature related to ice forms."@en ;
    skos:historyNote "Inherited from ICSM Place Names Working Group's National Feature Catalogue as at 21 December 2023." ;
    skos:inScheme cs: ;
    skos:narrower
        go:glacier ,
        go:ice-dome ,
        go:ice-field ,
        go:ice-massif ,
        go:ice-rise ,
        go:ice-shelf ,
        go:ice-stream ,
        go:ice-tongue ,
        go:ice-wall ,
        go:icefall ,
        go:neve ;
    skos:prefLabel "Ice Feature"@en ;
    skos:topConceptOf cs: ;
.

go:ice-field
    a skos:Concept ;
    rdfs:isDefinedBy cs: ;
    skos:definition "Flat glaciated area, underlying topography is not completely levelled out."@en ;
    skos:historyNote "Inherited from ICSM Place Names Working Group's National Feature Catalogue as at 21 December 2023. Concept and definition from the Australian Antarctic Division." ;
    skos:inScheme cs: ;
    skos:prefLabel "Ice Field"@en ;
    schema:citation "https://data.aad.gov.au/aadc/ftc/display_feature_type.cfm?feature_type_code=210"^^xsd:anyURI ;
.

go:ice-massif
    a skos:Concept ;
    rdfs:isDefinedBy cs: ;
    skos:definition "Compact group of mountain heights, which may be partly or almost entirely ice-covered."@en ;
    skos:historyNote "Inherited from ICSM Place Names Working Group's National Feature Catalogue as at 21 December 2023. Concept and definition from the Australian Antarctic Division." ;
    skos:inScheme cs: ;
    skos:prefLabel "Ice Massif"@en ;
    schema:citation "https://data.aad.gov.au/aadc/ftc/display_feature_type.cfm?feature_type_code=392"^^xsd:anyURI ;
.

go:ice-rise
    a skos:Concept ;
    rdfs:isDefinedBy cs: ;
    skos:definition "A mass of ice resting on rock and surrounded either by an ice shelf, or partly by an ice shelf and partly by sea. No rock is exposed and there may be none above sea level. Ice rises often have a dome-shaped surface. The largest known is about 100km across."@en ;
    skos:historyNote "Inherited from ICSM Place Names Working Group's National Feature Catalogue as at 21 December 2023. Concept and definition from the Australian Antarctic Division." ;
    skos:inScheme cs: ;
    skos:prefLabel "Ice Rise"@en ;
    schema:citation "https://data.aad.gov.au/aadc/ftc/display_feature_type.cfm?feature_type_code=213"^^xsd:anyURI ;
.

go:ice-shelf
    a skos:Concept ;
    rdfs:isDefinedBy cs: ;
    skos:definition "A floating ice sheet of considerable thickness attached to a coast. Ice shelves are usually of great horizontal extent and have a level or gently undulating surface. They are nourished by the accumulation of snow and often by seaward extension of land glaciers. Limited areas may be aground. The seaward edge is termed an ice front."@en ;
    skos:historyNote "Inherited from ICSM Place Names Working Group's National Feature Catalogue as at 21 December 2023. Concept and definition from the Australian Antarctic Division." ;
    skos:inScheme cs: ;
    skos:prefLabel "Ice Shelf"@en ;
    schema:citation "https://data.aad.gov.au/aadc/ftc/display_feature_type.cfm?feature_type_code=298"^^xsd:anyURI ;
.

go:ice-stream
    a skos:Concept ;
    rdfs:isDefinedBy cs: ;
    skos:definition "Part of an ice sheet in which the ice flows more rapidly and not necessarily in the same direction as the surrounding ice. The margins are sometimes clearly marked by a change in direction of the surface slope, but may be indistinct."@en ;
    skos:historyNote "Inherited from ICSM Place Names Working Group's National Feature Catalogue as at 21 December 2023. Concept and definition from the Australian Antarctic Division." ;
    skos:inScheme cs: ;
    skos:prefLabel "Ice Stream"@en ;
    schema:citation "https://data.aad.gov.au/aadc/ftc/display_feature_type.cfm?feature_type_code=215"^^xsd:anyURI ;
.

go:ice-tongue
    a skos:Concept ;
    rdfs:isDefinedBy cs: ;
    skos:definition "A projection of the ice edge up to several km in length caused by wind and current."@en ;
    skos:historyNote "Inherited from ICSM Place Names Working Group's National Feature Catalogue as at 21 December 2023. Concept and definition from the Australian Antarctic Division." ;
    skos:inScheme cs: ;
    skos:prefLabel "Ice Tongue"@en ;
    schema:citation "https://data.aad.gov.au/aadc/ftc/display_feature_type.cfm?feature_type_code=325"^^xsd:anyURI ;
.

go:icefall
    a skos:Concept ;
    rdfs:isDefinedBy cs: ;
    skos:definition "The portion of a glacier at a point of steep descent, segmented by many transverse crevasses into separate blocks."@en ;
    skos:historyNote "Inherited from ICSM Place Names Working Group's National Feature Catalogue as at 21 December 2023. Concept and definition from the Australian Antarctic Division." ;
    skos:inScheme cs: ;
    skos:prefLabel "Icefall"@en ;
    schema:citation "https://data.aad.gov.au/aadc/ftc/display_feature_type.cfm?feature_type_code=218"^^xsd:anyURI ;
.

go:indigenous-protected-area
    a skos:Concept ;
    rdfs:isDefinedBy cs: ;
    skos:altLabel "IPA"@en ;
    skos:definition "An Indigenous Protected Area is an area of Indigenous-owned land or sea where Traditional Owners have entered into an agreement with the Australian Government to promote biodiversity and cultural resource conservation."@en ;
    skos:historyNote "Inherited from ICSM Place Names Working Group's National Feature Catalogue as at 21 December 2023." ;
    skos:inScheme cs: ;
    skos:prefLabel "Indigenous Protected Area"@en ;
.

go:industrial-production-facility
    a skos:Concept ;
    rdfs:isDefinedBy cs: ;
    skos:definition "Places where the major activity is of a manufacturing or processing nature."@en ;
    skos:historyNote "Inherited from ICSM Place Names Working Group's National Feature Catalogue as at 21 December 2023, with name label amended 2024-05-04 from 'Industry' 2024-03-05." ;
    skos:inScheme cs: ;
    skos:narrower
        go:abattoir ,
        go:brewery ,
        go:brickworks ,
        go:cement-plant ,
        go:distillery ,
        go:steel-works ,
        go:sugar-refinery ,
        go:tannery ,
        go:timber-operations ,
        go:winery ;
    skos:prefLabel "Industrial Production Facility"@en ;
.

go:inlet
    a skos:Concept ;
    rdfs:isDefinedBy cs: ;
    skos:altLabel "Arm"@en ;
    skos:definition "A small indentation in a waterline usually tapering towards its head."@en ;
    skos:historyNote "Inherited from ICSM Place Names Working Group's National Feature Catalogue as at 21 December 2023." ;
    skos:inScheme cs: ;
    skos:prefLabel "Inlet"@en ;
.

go:iron-ore-processor
    a skos:Concept ;
    rdfs:isDefinedBy cs: ;
    skos:definition "An iron ore processing plant."@en ;
    skos:historyNote "Inherited from ICSM Place Names Working Group's National Feature Catalogue as at 21 December 2023." ;
    skos:inScheme cs: ;
    skos:prefLabel "Iron Ore Processor"@en ;
.

go:irrigation-channel
    a skos:Concept ;
    rdfs:isDefinedBy cs: ;
    skos:altLabel "Aqueduct"@en ;
    skos:definition "An artificial watercourse used for irrigation. Can be open or closed."@en ;
    skos:historyNote "Inherited from ICSM Place Names Working Group's National Feature Catalogue as at 21 December 2023." ;
    skos:inScheme cs: ;
    skos:prefLabel "Irrigation Channel"@en ;
.

go:island
    a skos:Concept ;
    rdfs:isDefinedBy cs: ;
    skos:definition "A tract of land completely surrounded by water."@en ;
    skos:historyNote "Inherited from ICSM Place Names Working Group's National Feature Catalogue as at 21 December 2023." ;
    skos:inScheme cs: ;
    skos:narrower
        go:atoll ,
        go:cay ,
        go:clumps ,
        go:islet ,
        go:offshore-rock ,
        go:skerry ;
    skos:prefLabel "Island"@en ;
.

go:island-group
    a skos:Concept ;
    rdfs:isDefinedBy cs: ;
    skos:altLabel "Archipelago"@en ;
    skos:definition "A group of islands often with a common name which covers the group. The islands may have their own individual names. The island group can include any combination of rocks, reefs, islets and island names."@en ;
    skos:historyNote "Inherited from ICSM Place Names Working Group's National Feature Catalogue as at 21 December 2023." ;
    skos:inScheme cs: ;
    skos:prefLabel "Island Group"@en ;
.

go:islet
    a skos:Concept ;
    rdfs:isDefinedBy cs: ;
    skos:altLabel "Isle"@en ;
    skos:definition "A small island."@en ;
    skos:historyNote "Created by separating 'Island' alternate labels 2024-03-05. Definition from Macquarie Dictionary." ;
    skos:inScheme cs: ;
    skos:prefLabel "Islet"@en ;
.

go:isthmus
    a skos:Concept ;
    rdfs:isDefinedBy cs: ;
    skos:altLabel "Neck"@en ;
    skos:definition "A narrow portion of land enclosed on each side by water and connecting two larger bodies of land."@en ;
    skos:historyNote "Inherited from ICSM Place Names Working Group's National Feature Catalogue as at 21 December 2023." ;
    skos:inScheme cs: ;
    skos:prefLabel "Isthmus"@en ;
.

go:jetty
    a skos:Concept ;
    rdfs:isDefinedBy cs: ;
    skos:definition "A structure of stone or timber projecting into water, often for private use and significantly smaller than a pier."@en ;
    skos:historyNote "Inherited from ICSM Place Names Working Group's National Feature Catalogue as at 21 December 2023." ;
    skos:inScheme cs: ;
    skos:prefLabel "Jetty"@en ;
.

go:jump-up
    a skos:Concept ;
    rdfs:isDefinedBy cs: ;
    skos:definition "An isolated mesa; a sudden rise in the landscape or a steep section in otherwise relatively flat terrain. Areas where the top layer of earth appears to \"jump up\" to a higher level because of erosion that has removed surrounding material, leaving a distinctive, abrupt elevation in the landscape."@en ;
    skos:historyNote "Created by separating 'Cliff' alternate labels 2024-05-10. Definition adapted from Macquarie Dictionary." ;
    skos:inScheme cs: ;
    skos:prefLabel "Jump Up"@en ;
.

go:junction
    a skos:Concept ;
    rdfs:isDefinedBy cs: ;
    skos:definition "A place where RIVERS, ROADS or RAILWAYS intersect."@en ;
    skos:historyNote "Inherited from ICSM Place Names Working Group's National Feature Catalogue as at 21 December 2023." ;
    skos:inScheme cs: ;
    skos:prefLabel "Junction"@en ;
.

go:knob
    a skos:Concept ;
    rdfs:isDefinedBy cs: ;
    skos:definition "A rounded hill or mountain, especially an isolated one."@en ;
    skos:historyNote "Created by separating 'Hill' alternate labels 2024-05-10. Definition from Macquarie Dictionary." ;
    skos:inScheme cs: ;
    skos:prefLabel "Knob"@en ;
.

go:knoll
    a skos:Concept ;
    rdfs:isDefinedBy cs: ;
    skos:altLabel "Hillock"@en ;
    skos:definition "A small, rounded hill or eminence."@en ;
    skos:historyNote "Created by separating 'Hill' alternate labels 2024-05-10. Definition from Macquarie Dictionary." ;
    skos:inScheme cs: ;
    skos:prefLabel "Knoll"@en ;
.

go:lagoon
    a skos:Concept ;
    rdfs:isDefinedBy cs: ;
    skos:definition "An enclosed area of shallow salt or brackish water which is partly or completely separated from the sea."@en ;
    skos:historyNote "Inherited from ICSM Place Names Working Group's National Feature Catalogue as at 21 December 2023." ;
    skos:inScheme cs: ;
    skos:narrower go:freshwater-lagoon ;
    skos:prefLabel "Lagoon"@en ;
.

go:lake
    a skos:Concept ;
    rdfs:isDefinedBy cs: ;
    skos:definition "A body of fresh or salt water, natural or artificial, enclosed or nearly enclosed by land; it may or may not have in and outflowing water (either permanent, intermittent or largely dry)."@en ;
    skos:historyNote "Inherited from ICSM Place Names Working Group's National Feature Catalogue as at 21 December 2023." ;
    skos:inScheme cs: ;
    skos:narrower
        go:backwater ,
        go:billabong ,
        go:oxbow ;
    skos:prefLabel "Lake"@en ;
.

go:land-district
    a skos:Concept ;
    rdfs:isDefinedBy cs: ;
    skos:altLabel "Land Division"@en ;
    skos:definition "A classification of land to assist in the administration of land."@en ;
    skos:historyNote "Inherited from ICSM Place Names Working Group's National Feature Catalogue as at 21 December 2023." ;
    skos:inScheme cs: ;
    skos:prefLabel "Land District"@en ;
	skos:scopeNote "No longer in use; recognised for historically named features only.  " ;
.

go:landfill
    a skos:Concept ;
    rdfs:isDefinedBy cs: ;
    skos:definition "A site where refuse is dumped and covered with earth."@en ;
    skos:historyNote "Inherited from ICSM Place Names Working Group's National Feature Catalogue as at 21 December 2023." ;
    skos:inScheme cs: ;
    skos:prefLabel "Landfill"@en ;
.

go:landform
    a skos:Concept ;
    rdfs:isDefinedBy cs: ;
    skos:definition "Natural features of the Earth's surface."@en ;
    skos:historyNote "Inherited from ICSM Place Names Working Group's National Feature Catalogue as at 21 December 2023." ;
    skos:inScheme cs: ;
    skos:narrower
        go:bank ,
        go:bar ,
        go:basin ,
        go:beach ,
        go:bench ,
        go:blowhole ,
        go:cape ,
        go:cave ,
        go:cirque ,
        go:cliff ,
        go:coast ,
        go:continent ,
        go:crater ,
        go:depression ,
        go:desert ,
        go:dune ,
        go:escarpment ,
        go:foreshore ,
        go:gorge ,
        go:hill ,
        go:island ,
        go:island-group ,
        go:isthmus ,
        go:ledge ,
        go:moraine ,
        go:mountain ,
        go:nunatak ,
        go:pan ,
        go:pass ,
        go:peak ,
        go:peninsula ,
        go:plain ,
        go:plateau ,
        go:pocket ,
        go:point ,
        go:range ,
        go:ridge ,
        go:rock ,
        go:rockhole ,
        go:slope ,
        go:spit ,
        go:tidal-flat ,
        go:trench ,
        go:valley ,
        go:wall ;
    skos:prefLabel "Landform"@en ;
.

go:landing-area
    a skos:Concept ;
    rdfs:isDefinedBy cs: ;
    skos:definition "An area that is used for the landing and takeoff of aircraft."@en ;
    skos:historyNote "Inherited from ICSM Place Names Working Group's National Feature Catalogue as at 21 December 2023." ;
    skos:inScheme cs: ;
    skos:narrower
        go:aerodrome ,
        go:airfield ,
        go:airport ,
        go:airstrip ,
        go:landing-ground ;
    skos:prefLabel "Landing Area"@en ;
.

go:landing-ground
    a skos:Concept ;
    rdfs:isDefinedBy cs: ;
    skos:definition "A prepared ground on which to land an aeroplane, usually without other facilities. Often used in relation to temporary sites suitable for aircraft to land."@en ;
    skos:historyNote "Created by separating 'Landing Area' alternate labels 2024-06-10. Definition adapted from Macquarie Dictionary." ;
    skos:inScheme cs: ;
    skos:prefLabel "Landing Ground"@en ;
.

go:landing-place
    a skos:Concept ;
    rdfs:isDefinedBy cs: ;
    skos:definition "A place where boats receive or discharge passengers and/or freight."@en ;
    skos:historyNote "Inherited from ICSM Place Names Working Group's National Feature Catalogue as at 21 December 2023." ;
    skos:inScheme cs: ;
    skos:prefLabel "Landing Place"@en ;
.

go:landmark
    a skos:Concept ;
    rdfs:isDefinedBy cs: ;
    skos:definition "Places that are a recognised entity by the community for specific identification purposes."@en ;
    skos:historyNote "Inherited from ICSM Place Names Working Group's National Feature Catalogue as at 21 December 2023." ;
    skos:inScheme cs: ;
    skos:narrower
        go:building ,
        go:colony ,
        go:corner ,
        go:fence ,
        go:historic-site ,
        go:homestead ,
        go:junction ,
        go:lookout ,
        go:monument ,
        go:outstation ,
        go:property ,
        go:ship-wreck ,
        go:survey-marker ;
    skos:prefLabel "Landmark"@en ;
.

go:lava-tube
    a skos:Concept ;
    rdfs:isDefinedBy cs: ;
    skos:definition "A natural conduit in a volcano through which a lava flow travels before being expelled; forming a long channel once the rock has cooled."@en ;
    skos:historyNote "Created by separating 'Cave' alternate labels 2024-03-05. Definition adapted from Macquarie Dictionary." ;
    skos:inScheme cs: ;
    skos:prefLabel "Lava Tube"@en ;
.

go:law-court
    a skos:Concept ;
    rdfs:isDefinedBy cs: ;
    skos:altLabel
        "Court"@en ,
        "Court House"@en ,
        "High Court"@en ,
        "Magistrates Court"@en ,
        "Supreme Court"@en ,
        "Tribunal"@en ;
    skos:definition "A building which houses a tribunal which has power to adjudicate in civil, criminal or military matters."@en ;
    skos:historyNote "Inherited from ICSM Place Names Working Group's National Feature Catalogue as at 21 December 2023." ;
    skos:inScheme cs: ;
    skos:prefLabel "Law Court"@en ;
.

go:ledge
    a skos:Concept ;
    rdfs:isDefinedBy cs: ;
    skos:definition "A narrow shelf-like projection on a cliff or on the side of a hill or mountain."@en ;
    skos:historyNote "Inherited from ICSM Place Names Working Group's National Feature Catalogue as at 21 December 2023." ;
    skos:inScheme cs: ;
    skos:prefLabel "Ledge"@en ;
.

go:legal-institution
    a skos:Concept ;
    rdfs:isDefinedBy cs: ;
    skos:definition "A facility relating to law or justice."@en ;
    skos:historyNote "Inherited from ICSM Place Names Working Group's National Feature Catalogue as at 21 December 2023, with name label amended 2024-05-04 from 'Legal' and definition updated 2024-03-05." ;
    skos:inScheme cs: ;
    skos:narrower
        go:diplomatic-mission ,
        go:law-court ,
        go:prison ;
    skos:prefLabel "Legal Institution"@en ;
    skos:topConceptOf cs: ;
.

go:level-crossing
    a skos:Concept ;
    rdfs:isDefinedBy cs: ;
    skos:definition "A place where a road crosses a railway at the same level."@en ;
    skos:historyNote "Added by Queensland 2024-06-04 from Queensland Roads and Tracks dataset. Definition adapted from Macquarie Dictionary." ;
    skos:inScheme cs: ;
    skos:prefLabel "Level Crossing"@en ;
.

go:library
    a skos:Concept ;
    rdfs:isDefinedBy cs: ;
    skos:definition "A place in which literary materials, such as books, periodicals, newspapers, pamphlets, prints, records, and tapes, are kept for reading, reference, or lending."@en ;
    skos:historyNote "Inherited from ICSM Place Names Working Group's National Feature Catalogue as at 21 December 2023." ;
    skos:inScheme cs: ;
    skos:prefLabel "Library"@en ;
.

go:lifesaving-club
    a skos:Concept ;
    rdfs:isDefinedBy cs: ;
    skos:altLabel "Surf Lifesaving Club"@en ;
    skos:definition "A patrol and response service for those that are in difficulty in the water."@en ;
    skos:historyNote "Inherited from ICSM Place Names Working Group's National Feature Catalogue as at 21 December 2023." ;
    skos:inScheme cs: ;
    skos:prefLabel "Lifesaving Club"@en ;
.

go:light-rail
    a skos:Concept ;
    rdfs:isDefinedBy cs: ;
    skos:altLabel "Light Railway"@en ;
    skos:definition "A track or set of tracks of iron or steel rails used for the passage of light rail."@en ;
    skos:historyNote "Inherited from ICSM Place Names Working Group's National Feature Catalogue as at 21 December 2023." ;
    skos:inScheme cs: ;
    skos:prefLabel "Light Rail"@en ;
.

go:light-rail-transport-infrastructure
    a skos:Concept ;
    rdfs:isDefinedBy cs: ;
    skos:definition "Installations, systems, and structures that enable the operation of light rail trains and serve as the foundation for light rail transportation."@en ;
    skos:historyNote "Broader concept introduced 2024-03-05." ;
    skos:inScheme cs: ;
    skos:narrower
        go:light-rail ,
        go:light-rail-station ,
        go:light-rail-tunnel ;
    skos:prefLabel "Light Rail Transport Infrastructure"@en ;
.

go:lighthouse
    a skos:Concept ;
    rdfs:isDefinedBy cs: ;
    skos:definition "A distinctive structure on or off the coast, exhibiting a major light designed to serve as an aid to navigation."@en ;
    skos:historyNote "Inherited from ICSM Place Names Working Group's National Feature Catalogue as at 21 December 2023." ;
    skos:inScheme cs: ;
    skos:prefLabel "Lighthouse"@en ;
.

go:liquid-waste-disposal-site
    a skos:Concept ;
    rdfs:isDefinedBy cs: ;
    skos:altLabel "Dump Point"@en ;
    skos:definition "A place for the disposal of liquid waste."@en ;
    skos:historyNote "Inherited from ICSM Place Names Working Group's National Feature Catalogue as at 21 December 2023, with 'liquid' added to description 2024-03-05." ;
    skos:inScheme cs: ;
    skos:prefLabel "Liquid Waste Disposal Site"@en ;
.

go:local-government-area
    a skos:Concept ;
    rdfs:isDefinedBy cs: ;
    skos:altLabel
        "LGA"@en ,
        "Municipality"@en ,
        "Shire"@en ;
    skos:definition "A regional division of a State or Territory administered by local government"@en ;
    skos:historyNote "Inherited from ICSM Place Names Working Group's National Feature Catalogue as at 21 December 2023." ;
    skos:inScheme cs: ;
    skos:prefLabel "Local Government Area"@en ;
.

go:local-government-area-ward
    a skos:Concept ;
    rdfs:isDefinedBy cs: ;
    skos:altLabel
        "Division"@en ,
        "Local Government Area Division"@en ,
        "Ward"@en ;
    skos:definition "A division of a local government for electoral purposes."@en ;
    skos:historyNote "Inherited from ICSM Place Names Working Group's National Feature Catalogue as at 21 December 2023." ;
    skos:inScheme cs: ;
    skos:prefLabel "Local Government Area Ward"@en ;
.

go:local-road
    a skos:Concept ;
    rdfs:isDefinedBy cs: ;
    skos:definition "Roads that provide primarily property access. These generally have addresses assigned against them. These roads may be privately owned roads that are connected and open to the public network. Includes service roads that may share the same name as higher order roads."@en ;
    skos:historyNote "Added by Queensland 2024-06-04 from Queensland Roads and Tracks dataset." ;
    skos:inScheme cs: ;
    skos:prefLabel "Local Road"@en ;
.

go:locality
    a skos:Concept ;
    rdfs:isDefinedBy cs: ;
    skos:altLabel
        "Bounded Locality"@en ,
        "Suburb"@en ;
    skos:definition "A bounded area distinguished for its community and/or landscape characteristics: in metropolitan areas it is commonly referred to as a ‘suburb’; it provides an official reference point for addressing purposes."@en ;
    skos:historyNote "Inherited from ICSM Place Names Working Group's National Feature Catalogue as at 21 December 2023." ;
    skos:inScheme cs: ;
    skos:prefLabel "Locality"@en ;
.

go:lock
    a skos:Concept ;
    rdfs:isDefinedBy cs: ;
    skos:definition "A stretch of water in a river or canal enclosed by gates fitted with sluices to enable craft to be raised from one water level to another."@en ;
    skos:historyNote "Inherited from ICSM Place Names Working Group's National Feature Catalogue as at 21 December 2023." ;
    skos:inScheme cs: ;
    skos:prefLabel "Lock"@en ;
.

go:lookout
    a skos:Concept ;
    rdfs:isDefinedBy cs: ;
    skos:altLabel "Viewing Platform"@en ;
    skos:definition "An observation or viewing point often a man-made structure."@en ;
    skos:historyNote "Inherited from ICSM Place Names Working Group's National Feature Catalogue as at 21 December 2023." ;
    skos:inScheme cs: ;
    skos:prefLabel "Lookout"@en ;
.

go:mall
    a skos:Concept ;
    rdfs:isDefinedBy cs: ;
    skos:definition "A road or passage whose main purpose is to provide access to pedestrians but may allow some vehicular access."@en ;
    skos:historyNote "Added by Queensland 2024-06-04 from Queensland Roads and Tracks dataset." ;
    skos:inScheme cs: ;
    skos:prefLabel "Mall"@en ;
.

go:marina
    a skos:Concept ;
    rdfs:isDefinedBy cs: ;
    skos:definition "An area provided with berthing and shore facilities (including toilets, water and rubbish disposal) particularly for yachts and other pleasure craft."@en ;
    skos:historyNote "Inherited from ICSM Place Names Working Group's National Feature Catalogue as at 21 December 2023." ;
    skos:inScheme cs: ;
    skos:prefLabel "Marina"@en ;
.

go:marine-caldera
    a skos:Concept ;
    rdfs:isDefinedBy cs: ;
    skos:definition "A roughly circular, cauldron-like depression generally characterised by steep sides and formed by collapse, or partial collapse, during or following a volcanic eruption."@en ;
    skos:historyNote "Inherited from ICSM Place Names Working Group's National Feature Catalogue as at 21 December 2023. Definition from General Bathymetric Chart of the Oceans (GEBCO) Sub-Committee on Undersea Features Names (SCUFN)." ;
    skos:inScheme cs: ;
    skos:prefLabel "Marine Caldera"@en ;
    schema:citation "https://iho.int/en/basic-documents-1"^^xsd:anyURI ;
.

go:marine-canyon
    a skos:Concept ;
    rdfs:isDefinedBy cs: ;
    skos:definition "An elongated, narrow, steep-sided depression that generally deepens down-slope."@en ;
    skos:historyNote "Inherited from ICSM Place Names Working Group's National Feature Catalogue as at 21 December 2023. Definition from General Bathymetric Chart of the Oceans (GEBCO) Sub-Committee on Undersea Features Names (SCUFN)." ;
    skos:inScheme cs: ;
    skos:prefLabel "Marine Canyon"@en ;
    schema:citation "https://iho.int/en/basic-documents-1"^^xsd:anyURI ;
.

go:marine-continental-margin
    a skos:Concept ;
    rdfs:isDefinedBy cs: ;
    skos:definition "The zone, generally consisting of shelf, slope and continental rise, separating the continent from the deep seafloor or abyssal plain. Occasionally a trench may be present in place of a continental rise."@en ;
    skos:historyNote "Inherited from ICSM Place Names Working Group's National Feature Catalogue as at 21 December 2023. Definition from General Bathymetric Chart of the Oceans (GEBCO) Sub-Committee on Undersea Features Names (SCUFN)." ;
    skos:inScheme cs: ;
    skos:prefLabel "Marine Continental Margin"@en ;
	skos:scopeNote "Recognised for historically named features only. " ;
    schema:citation "https://iho.int/en/basic-documents-1"^^xsd:anyURI ;
.

go:marine-fan
    a skos:Concept ;
    rdfs:isDefinedBy cs: ;
    skos:definition "A relatively smooth depositional feature continuously deepening away from a sediment source commonly located at the lower termination of a canyon or canyon system."@en ;
    skos:historyNote "Inherited from ICSM Place Names Working Group's National Feature Catalogue as at 21 December 2023. Definition from General Bathymetric Chart of the Oceans (GEBCO) Sub-Committee on Undersea Features Names (SCUFN)." ;
    skos:inScheme cs: ;
    skos:prefLabel "Marine Fan"@en ;
    schema:citation "https://iho.int/en/basic-documents-1"^^xsd:anyURI ;
.

go:marine-fracture-zone
    a skos:Concept ;
    rdfs:isDefinedBy cs: ;
    skos:definition "A long narrow zone of irregular topography formed by the movement of tectonic plates associated with an offset of a spreading ridge axis, characterised by steep-sided and/or asymmetrical ridges, troughs or escarpments."@en ;
    skos:historyNote "Inherited from ICSM Place Names Working Group's National Feature Catalogue as at 21 December 2023. Definition from General Bathymetric Chart of the Oceans (GEBCO) Sub-Committee on Undersea Features Names (SCUFN)." ;
    skos:inScheme cs: ;
    skos:prefLabel "Marine Fracture Zone"@en ;
    schema:citation "https://iho.int/en/basic-documents-1"^^xsd:anyURI ;
.

go:marine-hole
    a skos:Concept ;
    rdfs:isDefinedBy cs: ;
    skos:definition "A depression of limited extent with all sides rising steeply from a relatively flat bottom."@en ;
    skos:historyNote "Inherited from ICSM Place Names Working Group's National Feature Catalogue as at 21 December 2023. Definition from General Bathymetric Chart of the Oceans (GEBCO) Sub-Committee on Undersea Features Names (SCUFN)." ;
    skos:inScheme cs: ;
    skos:prefLabel "Marine Hole"@en ;
    schema:citation "https://iho.int/en/basic-documents-1"^^xsd:anyURI ;
.

go:marine-knoll
    a skos:Concept ;
    rdfs:isDefinedBy cs: ;
    skos:definition "A distinct elevation with a rounded profile less than 1000m above the surrounding relief as measured from the deepest isobath that surrounds most of the feature."@en ;
    skos:historyNote "Inherited from ICSM Place Names Working Group's National Feature Catalogue as at 21 December 2023. Definition from General Bathymetric Chart of the Oceans (GEBCO) Sub-Committee on Undersea Features Names (SCUFN)." ;
    skos:inScheme cs: ;
    skos:prefLabel "Marine Knoll"@en ;
    schema:citation "https://iho.int/en/basic-documents-1"^^xsd:anyURI ;
.

go:marine-levee
    a skos:Concept ;
    rdfs:isDefinedBy cs: ;
    skos:definition "A depositional embankment bordering a canyon, valley or sea channel."@en ;
    skos:historyNote "Inherited from ICSM Place Names Working Group's National Feature Catalogue as at 21 December 2023. Definition from General Bathymetric Chart of the Oceans (GEBCO) Sub-Committee on Undersea Features Names (SCUFN)." ;
    skos:inScheme cs: ;
    skos:prefLabel "Marine Levee"@en ;
    schema:citation "https://iho.int/en/basic-documents-1"^^xsd:anyURI ;
.

go:marine-moat
    a skos:Concept ;
    rdfs:isDefinedBy cs: ;
    skos:definition "An annular or partially annular depression commonly located at the base of seamounts, islands and other isolated elevations."@en ;
    skos:historyNote "Inherited from ICSM Place Names Working Group's National Feature Catalogue as at 21 December 2023. Definition from General Bathymetric Chart of the Oceans (GEBCO) Sub-Committee on Undersea Features Names (SCUFN)." ;
    skos:inScheme cs: ;
    skos:prefLabel "Marine Moat"@en ;
    schema:citation "https://iho.int/en/basic-documents-1"^^xsd:anyURI ;
.

go:marine-mound
    a skos:Concept ;
    rdfs:isDefinedBy cs: ;
    skos:definition "A distinct elevation with a rounded profile generally less than 500m above the surrounding relief as measured from the deepest isobath that surrounds most of the feature, commonly formed by the expulsion of fluids or by coral reef development, sedimentation and (bio)erosion."@en ;
    skos:historyNote "Inherited from ICSM Place Names Working Group's National Feature Catalogue as at 21 December 2023. Definition from General Bathymetric Chart of the Oceans (GEBCO) Sub-Committee on Undersea Features Names (SCUFN)." ;
    skos:inScheme cs: ;
    skos:prefLabel "Marine Mound"@en ;
    schema:citation "https://iho.int/en/basic-documents-1"^^xsd:anyURI ;
.

go:marine-mud-volcano
    a skos:Concept ;
    rdfs:isDefinedBy cs: ;
    skos:definition "A mound or cone-shaped elevation formed by the expulsion of non-magmatic liquids and gasses."@en ;
    skos:historyNote "Inherited from ICSM Place Names Working Group's National Feature Catalogue as at 21 December 2023. Definition from General Bathymetric Chart of the Oceans (GEBCO) Sub-Committee on Undersea Features Names (SCUFN)." ;
    skos:inScheme cs: ;
    skos:prefLabel "Marine Mud Volcano"@en ;
    schema:citation "https://iho.int/en/basic-documents-1"^^xsd:anyURI ;
.

go:marine-park
    a skos:Concept ;
    rdfs:isDefinedBy cs: ;
    skos:altLabel "Aquatic Reserve"@en ;
    skos:definition "An area of sea, set apart, as by a state or nation, to be preserved in its natural state for the benefit of the public."@en ;
    skos:historyNote "Inherited from ICSM Place Names Working Group's National Feature Catalogue as at 21 December 2023." ;
    skos:inScheme cs: ;
    skos:prefLabel "Marine Park"@en ;
.

go:marine-peak
    a skos:Concept ;
    rdfs:isDefinedBy cs: ;
    skos:definition "A conical or pointed elevation at the summit of a larger feature."@en ;
    skos:historyNote "Inherited from ICSM Place Names Working Group's National Feature Catalogue as at 21 December 2023. Definition from General Bathymetric Chart of the Oceans (GEBCO) Sub-Committee on Undersea Features Names (SCUFN)." ;
    skos:inScheme cs: ;
    skos:prefLabel "Marine Peak"@en ;
    schema:citation "https://iho.int/en/basic-documents-1"^^xsd:anyURI ;
.

go:marine-pinnacle
    a skos:Concept ;
    rdfs:isDefinedBy cs: ;
    skos:definition "A spire-shaped pillar either isolated or at the summit of a larger feature."@en ;
    skos:historyNote "Inherited from ICSM Place Names Working Group's National Feature Catalogue as at 21 December 2023. Definition from General Bathymetric Chart of the Oceans (GEBCO) Sub-Committee on Undersea Features Names (SCUFN)." ;
    skos:inScheme cs: ;
    skos:prefLabel "Marine Pinnacle"@en ;
    schema:citation "https://iho.int/en/basic-documents-1"^^xsd:anyURI ;
.

go:marine-province
    a skos:Concept ;
    rdfs:isDefinedBy cs: ;
    skos:definition "A geographically distinct region with a number of shared physiographic characteristics that contrast with those in the surrounding areas."@en ;
    skos:historyNote "Inherited from ICSM Place Names Working Group's National Feature Catalogue as at 21 December 2023. Definition from General Bathymetric Chart of the Oceans (GEBCO) Sub-Committee on Undersea Features Names (SCUFN)." ;
    skos:inScheme cs: ;
    skos:prefLabel "Marine Province"@en ;
    schema:citation "https://iho.int/en/basic-documents-1"^^xsd:anyURI ;
.

go:marine-reef
    a skos:Concept ;
    rdfs:isDefinedBy cs: ;
    skos:definition "A shallow elevation composed of consolidated material that may constitute a hazard to surface navigation."@en ;
    skos:historyNote "Inherited from ICSM Place Names Working Group's National Feature Catalogue as at 21 December 2023. Definition from General Bathymetric Chart of the Oceans (GEBCO) Sub-Committee on Undersea Features Names (SCUFN)." ;
    skos:inScheme cs: ;
    skos:narrower go:coral-reef ;
    skos:prefLabel "Marine Reef"@en ;
    schema:citation "https://iho.int/en/basic-documents-1"^^xsd:anyURI ;
.

go:marine-ridge
    a skos:Concept ;
    rdfs:isDefinedBy cs: ;
    skos:altLabel "Undersea Ridge"@en ;
    skos:definition "An elongated elevation of varying complexity, size and gradient."@en ;
    skos:historyNote "Inherited from ICSM Place Names Working Group's National Feature Catalogue as at 21 December 2023. Definition from General Bathymetric Chart of the Oceans (GEBCO) Sub-Committee on Undersea Features Names (SCUFN)." ;
    skos:inScheme cs: ;
    skos:narrower go:mid-ocean-ridge ;
    skos:prefLabel "Marine Ridge"@en ;
    schema:citation "https://iho.int/en/basic-documents-1"^^xsd:anyURI ;
.

go:marine-rift
    a skos:Concept ;
    rdfs:isDefinedBy cs: ;
    skos:definition "An elongated depression bounded by two or more faults formed as a breach or split between two bodies that were once joined."@en ;
    skos:historyNote "Inherited from ICSM Place Names Working Group's National Feature Catalogue as at 21 December 2023. Definition from General Bathymetric Chart of the Oceans (GEBCO) Sub-Committee on Undersea Features Names (SCUFN)." ;
    skos:inScheme cs: ;
    skos:prefLabel "Marine Rift"@en ;
    schema:citation "https://iho.int/en/basic-documents-1"^^xsd:anyURI ;
.

go:marine-rise
    a skos:Concept ;
    rdfs:isDefinedBy cs: ;
    skos:definition "A broad elevation that generally rises gently and smoothly from the surrounding relief."@en ;
    skos:historyNote "Inherited from ICSM Place Names Working Group's National Feature Catalogue as at 21 December 2023. Definition from General Bathymetric Chart of the Oceans (GEBCO) Sub-Committee on Undersea Features Names (SCUFN)." ;
    skos:inScheme cs: ;
    skos:prefLabel "Marine Rise"@en ;
    schema:citation "https://iho.int/en/basic-documents-1"^^xsd:anyURI ;
.

go:marine-saddle
    a skos:Concept ;
    rdfs:isDefinedBy cs: ;
    skos:definition "A broad pass or col in a ridge, rise or other elevation."@en ;
    skos:historyNote "Inherited from ICSM Place Names Working Group's National Feature Catalogue as at 21 December 2023. Definition from General Bathymetric Chart of the Oceans (GEBCO) Sub-Committee on Undersea Features Names (SCUFN)." ;
    skos:inScheme cs: ;
    skos:prefLabel "Marine Saddle"@en ;
    schema:citation "https://iho.int/en/basic-documents-1"^^xsd:anyURI ;
.

go:marine-salt-dome
    a skos:Concept ;
    rdfs:isDefinedBy cs: ;
    skos:definition "A distinct elevation, often with a rounded profile, one km or more in diameter that is the geomorphologic expression of a diapir formed by vertical intrusion of salt. Commonly found in a PROVINCE of similar features."@en ;
    skos:historyNote "Inherited from ICSM Place Names Working Group's National Feature Catalogue as at 21 December 2023. Definition from General Bathymetric Chart of the Oceans (GEBCO) Sub-Committee on Undersea Features Names (SCUFN)." ;
    skos:inScheme cs: ;
    skos:prefLabel "Marine Salt Dome"@en ;
    schema:citation "https://iho.int/en/basic-documents-1"^^xsd:anyURI ;
.

go:marine-sand-ridge
    a skos:Concept ;
    rdfs:isDefinedBy cs: ;
    skos:definition "An elongated feature of unconsolidated sediment of limited vertical relief and sometimes crescent shaped. Commonly found in a PROVINCE of similar features."@en ;
    skos:historyNote "Inherited from ICSM Place Names Working Group's National Feature Catalogue as at 21 December 2023. Definition from General Bathymetric Chart of the Oceans (GEBCO) Sub-Committee on Undersea Features Names (SCUFN)." ;
    skos:inScheme cs: ;
    skos:prefLabel "Marine Sand Ridge"@en ;
    schema:citation "https://iho.int/en/basic-documents-1"^^xsd:anyURI ;
.

go:marine-shelf
    a skos:Concept ;
    rdfs:isDefinedBy cs: ;
    skos:altLabel
        "Borderland"@en ,
        "Continental Shelf"@en ,
        "Shelf Break"@en ,
        "Shelf Edge"@en ;
    skos:definition "The flat or gently sloping region adjacent to a continent or around an island that extends from the low water line to a depth, generally about 200m, where there is a marked increase in downward slope."@en ;
    skos:historyNote "Inherited from ICSM Place Names Working Group's National Feature Catalogue as at 21 December 2023. Definition from General Bathymetric Chart of the Oceans (GEBCO) Sub-Committee on Undersea Features Names (SCUFN)." ;
    skos:inScheme cs: ;
    skos:prefLabel "Marine Shelf"@en ;
	skos:scopeNote "Terms 'Borderland' and 'Continental Shelf' now obsolete and recognised for historically named features only. " ;
    schema:citation "https://iho.int/en/basic-documents-1"^^xsd:anyURI ;
.

go:marine-shoal
    a skos:Concept ;
    rdfs:isDefinedBy cs: ;
    skos:altLabel
        "Patches"@en ,
        "Shallows"@en ;
    skos:definition "A shallow elevation composed of unconsolidated material that may constitute a hazard to surface navigation."@en ;
    skos:historyNote "Inherited from ICSM Place Names Working Group's National Feature Catalogue as at 21 December 2023. Definition from General Bathymetric Chart of the Oceans (GEBCO) Sub-Committee on Undersea Features Names (SCUFN)." ;
    skos:inScheme cs: ;
    skos:prefLabel "Marine Shoal"@en ;
    schema:citation "https://iho.int/en/basic-documents-1"^^xsd:anyURI ;
.

go:marine-sill
    a skos:Concept ;
    rdfs:isDefinedBy cs: ;
    skos:definition "A relatively shallow barrier between basins that may inhibit water movement."@en ;
    skos:historyNote "Inherited from ICSM Place Names Working Group's National Feature Catalogue as at 21 December 2023. Definition from General Bathymetric Chart of the Oceans (GEBCO) Sub-Committee on Undersea Features Names (SCUFN)." ;
    skos:inScheme cs: ;
    skos:prefLabel "Marine Sill"@en ;
    schema:citation "https://iho.int/en/basic-documents-1"^^xsd:anyURI ;
.

go:marine-spur
    a skos:Concept ;
    rdfs:isDefinedBy cs: ;
    skos:altLabel "Marine Promontory"@en ;
    skos:definition "A subordinate ridge protruding from a larger feature."@en ;
    skos:historyNote "Inherited from ICSM Place Names Working Group's National Feature Catalogue as at 21 December 2023. Definition from General Bathymetric Chart of the Oceans (GEBCO) Sub-Committee on Undersea Features Names (SCUFN)." ;
    skos:inScheme cs: ;
    skos:prefLabel "Marine Spur"@en ;
	skos:scopeNote "Term 'Marine Promontory' now obsolete and recognised for historically named features only. " ;
    schema:citation "https://iho.int/en/basic-documents-1"^^xsd:anyURI ;
.

go:marine-terrace
    a skos:Concept ;
    rdfs:isDefinedBy cs: ;
    skos:definition "A flat or gently sloping region, generally long and narrow, bounded along one edge by a steeper descending slope and along the other by a steeper ascending slope."@en ;
    skos:historyNote "Inherited from ICSM Place Names Working Group's National Feature Catalogue as at 21 December 2023. Definition from General Bathymetric Chart of the Oceans (GEBCO) Sub-Committee on Undersea Features Names (SCUFN)." ;
    skos:inScheme cs: ;
    skos:prefLabel "Marine Terrace"@en ;
    schema:citation "https://iho.int/en/basic-documents-1"^^xsd:anyURI ;
.

go:marine-trough
    a skos:Concept ;
    rdfs:isDefinedBy cs: ;
    skos:definition "A long depression, generally wide and flat bottomed with symmetrical and parallel sides."@en ;
    skos:historyNote "Inherited from ICSM Place Names Working Group's National Feature Catalogue as at 21 December 2023. Definition from General Bathymetric Chart of the Oceans (GEBCO) Sub-Committee on Undersea Features Names (SCUFN)." ;
    skos:inScheme cs: ;
    skos:narrower go:deep ;
    skos:prefLabel "Marine Trough"@en ;
    schema:citation "https://iho.int/en/basic-documents-1"^^xsd:anyURI ;
.

go:market
    a skos:Concept ;
    rdfs:isDefinedBy cs: ;
    skos:definition "An open space or covered building(s) in which provisions are exposed for sale."@en ;
    skos:historyNote "Inherited from ICSM Place Names Working Group's National Feature Catalogue as at 21 December 2023." ;
    skos:inScheme cs: ;
    skos:prefLabel "Market"@en ;
.

go:maternal-and-child-health-centre
    a skos:Concept ;
    rdfs:isDefinedBy cs: ;
    skos:altLabel
        "MACH"@en ,
        "MCH"@en ,
        "Maternal Child Health"@en ,
        "Maternal and Child Health"@en ;
    skos:definition "A health facility that caters for the maternal and child health needs of a community."@en ;
    skos:historyNote "Inherited from ICSM Place Names Working Group's National Feature Catalogue as at 21 December 2023." ;
    skos:inScheme cs: ;
    skos:prefLabel "Maternal and Child Health Centre"@en ;
.

go:medical-centre
    a skos:Concept ;
    rdfs:isDefinedBy cs: ;
    skos:altLabel "Doctors Surgery"@en ;
    skos:definition "A healthcare facility that typically offers a range of outpatient services, possibly including diagnostic, treatment, and consultation services provided by various medical professionals such as doctors, nurses, and specialists."@en ;
    skos:historyNote "Inherited from ICSM Place Names Working Group's National Feature Catalogue as at 21 December 2023." ;
    skos:inScheme cs: ;
    skos:prefLabel "Medical Centre"@en ;
.

go:memorial
    a skos:Concept ;
    rdfs:isDefinedBy cs: ;
    skos:definition "Something designed to preserve the memory of a person, event, etc."@en ;
    skos:historyNote "Created by separating 'Monument' alternate labels 2024-03-05. Definition from Macquarie Dictionary." ;
    skos:inScheme cs: ;
    skos:prefLabel "Memorial"@en ;
.

go:mesa
    a skos:Concept ;
    rdfs:isDefinedBy cs: ;
    skos:definition "A landform having a relatively flat top and bounded wholly or in part with steep rock walls, common in arid and semi-arid parts of the south-western US but also occurring in areas of inland Australia."@en ;
    skos:historyNote "Created by separating 'Hill' alternate labels 2024-05-10. Definition from Macquarie Dictionary." ;
    skos:inScheme cs: ;
    skos:prefLabel "Mesa"@en ;
.

go:meteorite-crater
    a skos:Concept ;
    rdfs:isDefinedBy cs: ;
    skos:altLabel "Impact Crater"@en ;
    skos:definition "A hollow caused by the fall of a meteorite on to the Earth's surface."@en ;
    skos:historyNote "Inherited from ICSM Place Names Working Group's National Feature Catalogue as at 21 December 2023." ;
    skos:inScheme cs: ;
    skos:prefLabel "Meteorite Crater"@en ;
.

go:mid-ocean-ridge
    a skos:Concept ;
    rdfs:isDefinedBy cs: ;
    skos:definition "A mountain range on the ocean floor caused by the diverging of two tectonic plates which created a crust of upwelling magma."@en ;
    skos:historyNote "Created by separating 'Marine Ridge' alternate labels 2024-03-05. Definition from Macquarie Dictionary." ;
    skos:inScheme cs: ;
    skos:prefLabel "Mid-Ocean Ridge"@en ;
    schema:citation "https://app.macquariedictionary.com.au/"^^xsd:anyURI ;
.

go:mine
    a skos:Concept ;
    rdfs:isDefinedBy cs: ;
    skos:definition "Places related to the extraction of mined materials."@en ;
    skos:historyNote "Added by Queensland 2024-03-05." ;
    skos:inScheme cs: ;
    skos:narrower
        go:abandoned-mine ,
        go:open-cut-mine ,
        go:underground-mine ;
    skos:prefLabel "Mine"@en ;
.

go:mineral-field
    a skos:Concept ;
    rdfs:isDefinedBy cs: ;
    skos:definition "An area in which mineral resources have been identified."@en ;
    skos:historyNote "Inherited from ICSM Place Names Working Group's National Feature Catalogue as at 21 December 2023." ;
    skos:inScheme cs: ;
    skos:narrower
        go:coal-field ,
        go:gold-field ,
        go:oil-gas-field ,
        go:opal-field ;
    skos:prefLabel "Mineral Field"@en ;
.

go:mineral-sand-processing-plant
    a skos:Concept ;
    rdfs:isDefinedBy cs: ;
    skos:definition "A refinery for extracting rare metals."@en ;
    skos:historyNote "Inherited from ICSM Place Names Working Group's National Feature Catalogue as at 21 December 2023." ;
    skos:inScheme cs: ;
    skos:prefLabel "Mineral Sand Processing Plant"@en ;
.

go:mining-feature
    a skos:Concept ;
    rdfs:isDefinedBy cs: ;
    skos:definition "Place pertaining to the administration, extraction and processing of minerals, rock, gas and oil."@en ;
    skos:historyNote "Inherited from ICSM Place Names Working Group's National Feature Catalogue as at 21 December 2023, with name label amended 2024-05-04 from 'Mining' 2024-03-05." ;
    skos:inScheme cs: ;
    skos:narrower
        go:mineral-field ,
        go:mining-centre ,
        go:resource-extraction-feature ,
        go:resource-processing-facility ;
    skos:prefLabel "Mining Feature"@en ;
.

go:mission
    a skos:Concept ;
    rdfs:isDefinedBy cs: ;
    skos:definition "An establishment administered by a religious community for the spiritual and social welfare of others."@en ;
    skos:historyNote "Inherited from ICSM Place Names Working Group's National Feature Catalogue as at 21 December 2023." ;
    skos:inScheme cs: ;
    skos:prefLabel "Mission"@en ;
.

go:mobile-phone-tower
    a skos:Concept ;
    rdfs:isDefinedBy cs: ;
    skos:altLabel "Cellular Tower"@en ;
    skos:definition "Tower that supports the antennas and transmitters needed for mobile or cellular telephone communication."@en ;
    skos:historyNote "Created by separating 'Communication Tower' alternate labels 2024-06-10." ;
    skos:inScheme cs: ;
    skos:prefLabel "Mobile Phone Tower"@en ;
.

go:mondir
    a skos:Concept ;
    rdfs:isDefinedBy cs: ;
    skos:definition "Hindu place of worship."@en ;
    skos:historyNote "Inherited from ICSM Place Names Working Group's National Feature Catalogue as at 21 December 2023. Definition from Macquarie Dictionary." ;
    skos:inScheme cs: ;
    skos:prefLabel "Mondir"@en ;
.

go:monolith
    a skos:Concept ;
    rdfs:isDefinedBy cs: ;
    skos:definition "A single block or piece of stone of considerable size."@en ;
    skos:historyNote "Created by separating 'Rock' alternate labels 2024-06-10. Definition from Macquarie Dictionary." ;
    skos:inScheme cs: ;
    skos:prefLabel "Monolith"@en ;
.

go:monument
    a skos:Concept ;
    rdfs:isDefinedBy cs: ;
    skos:definition "Anything by which the memory of persons or things are preserved; anything that serves as a memorial to a person, event, or of past times."@en ;
    skos:historyNote "Inherited from ICSM Place Names Working Group's National Feature Catalogue as at 21 December 2023." ;
    skos:inScheme cs: ;
    skos:narrower
        go:cairn ,
        go:commemorative-tree ,
        go:fountain ,
        go:memorial ,
        go:obelisk ,
        go:shrine ;
    skos:prefLabel "Monument"@en ;
.

go:moraine
    a skos:Concept ;
    rdfs:isDefinedBy cs: ;
    skos:definition "A mound, ridge, or other distinct accumulation of unsorted, unstratified glacial drift, predominantly till, deposited primarily by direct action of glacier ice, in a variety of topographic landforms that are independent of control by the surface on which the drift lies."@en ;
    skos:historyNote "Inherited from ICSM Place Names Working Group's National Feature Catalogue as at 21 December 2023. Concept and definition from the Australian Antarctic Division." ;
    skos:inScheme cs: ;
    skos:prefLabel "Moraine"@en ;
    schema:citation "https://data.aad.gov.au/aadc/ftc/display_feature_type.cfm?feature_type_code=245"^^xsd:anyURI ;
.

go:mosque
    a skos:Concept ;
    rdfs:isDefinedBy cs: ;
    skos:definition "Muslim place of worship."@en ;
    skos:historyNote "Inherited from ICSM Place Names Working Group's National Feature Catalogue as at 21 December 2023. Definition from Macquarie Dictionary." ;
    skos:inScheme cs: ;
    skos:prefLabel "Mosque"@en ;
.

go:motor-track
    a skos:Concept ;
    rdfs:isDefinedBy cs: ;
    skos:altLabel "Auto Track"@en ;
    skos:definition "A circuit or course used for racing vehicles."@en ;
    skos:historyNote "Inherited from ICSM Place Names Working Group's National Feature Catalogue as at 21 December 2023." ;
    skos:inScheme cs: ;
    skos:prefLabel "Motor Track"@en ;
.

go:motorway
    a skos:Concept ;
    rdfs:isDefinedBy cs: ;
    skos:definition "Roads which are of importance in a national sense, and/or are a major interstate through route, and/or are principal connector roads between capitals and/or major regions and or key towns/commercial centres/inter-transport hubs. Also exhibit separated carriageways and unhindered, regulated traffic flow through use of grade-separated crossings and entry/exit ramps (e.g. Pacific Motorway)."@en ;
    skos:historyNote "Added by Queensland 2024-06-04 from Queensland Roads and Tracks dataset." ;
    skos:inScheme cs: ;
    skos:prefLabel "Motorway"@en ;
.

go:mountain
    a skos:Concept ;
    rdfs:isDefinedBy cs: ;
    skos:altLabel "Mount"@en ;
    skos:definition "A natural elevation of the Earth's surface rising more or less abruptly from the surrounding level, and attaining an altitude which, relative to adjacent elevations, is impressive or notable. In general the elevation of a mountain is more than 300m from foot to summit, but this distinction is arbitrary."@en ;
    skos:historyNote "Inherited from ICSM Place Names Working Group's National Feature Catalogue as at 21 December 2023." ;
    skos:inScheme cs: ;
    skos:narrower
        go:seamount ,
        go:subglacial-mount ;
    skos:prefLabel "Mountain"@en ;
.

go:mountain-bike-trail
    a skos:Concept ;
    rdfs:isDefinedBy cs: ;
    skos:altLabel "Mountain Bike Track"@en ;
    skos:definition "A non-vehicular trail designed for mountain bike traffic in the main."@en ;
    skos:historyNote "Inherited from ICSM Place Names Working Group's National Feature Catalogue as at 21 December 2023, with name label amended 2024-05-04 from 'Mountain Bike Track' and 'non vehicular' appended to description." ;
    skos:inScheme cs: ;
    skos:prefLabel "Mountain Bike Trail"@en ;
.

go:multiuse-trail
    a skos:Concept ;
    rdfs:isDefinedBy cs: ;
    skos:altLabel
        "Multi Use Trail"@en ,
        "Rail Trail"@en ,
        "Shared Use Trail"@en ;
    skos:definition "A non-vehicular trail designed for shared use access, being walking and bicycle traffic and may also include horse riding or skiing or may be any combination of multiple use. Main uses cycling and walking."@en ;
    skos:historyNote "Inherited from ICSM Place Names Working Group's National Feature Catalogue as at 21 December 2023, with 'non vehicular' appended to description 2024-05-04." ;
    skos:inScheme cs: ;
    skos:prefLabel "Multiuse Trail"@en ;
.

go:museum
    a skos:Concept ;
    rdfs:isDefinedBy cs: ;
    skos:altLabel "Museum Precinct"@en ;
    skos:definition "An institution that cares for (conserves) a collection of artefacts and other objects of scientific, artistic, cultural, or historical importance and makes them available for public viewing."@en ;
    skos:historyNote "Inherited from ICSM Place Names Working Group's National Feature Catalogue as at 21 December 2023." ;
    skos:inScheme cs: ;
    skos:prefLabel "Museum"@en ;
.

go:national-park
    a skos:Concept ;
    rdfs:isDefinedBy cs: ;
    skos:altLabel
        "Wilderness Area"@en ,
        "Wilderness Park"@en ;
    skos:definition "An area of land, set apart, as by a state or nation, to be preserved in its natural state for the benefit of the public."@en ;
    skos:historyNote "Inherited from ICSM Place Names Working Group's National Feature Catalogue as at 21 December 2023." ;
    skos:inScheme cs: ;
    skos:prefLabel "National Park"@en ;
.

go:native-well
    a skos:Concept ;
    rdfs:isDefinedBy cs: ;
    skos:definition "A naturally occurring source of fresh water found in the Australian outback. These wells were identified and used by Aboriginal Australians and may be spring-fed, or they might collect and store groundwater or rainwater seeping into the ground."@en ;
    skos:historyNote "Created by separating 'Rockhole' alternate labels 2024-06-10." ;
    skos:inScheme cs: ;
    skos:prefLabel "Native Well"@en ;
.

go:naval-base
    a skos:Concept ;
    rdfs:isDefinedBy cs: ;
    skos:definition "A facility used by the navy for the operation and/or training of personnel and their vessels."@en ;
    skos:historyNote "Inherited from ICSM Place Names Working Group's National Feature Catalogue as at 21 December 2023." ;
    skos:inScheme cs: ;
    skos:prefLabel "Naval Base"@en ;
.

go:neighbourhood
    a skos:Concept ;
    rdfs:isDefinedBy cs: ;
    skos:altLabel "Unbounded Locality"@en ;
    skos:definition "Does not have officially recognised and registered boundaries hence an unbounded locality. For this reason a neighbourhood name cannot be used for addressing purposes."@en ;
    skos:historyNote "Inherited from ICSM Place Names Working Group's National Feature Catalogue as at 21 December 2023." ;
    skos:inScheme cs: ;
    skos:prefLabel "Neighbourhood"@en ;
.

go:neighbourhood-safer-place
    a skos:Concept ;
    rdfs:isDefinedBy cs: ;
    skos:altLabel
        "BPLR"@en ,
        "Bushfire Place Of Last Resort"@en ,
        "NSP"@en ;
    skos:definition "An area or premises that may as a last resort provide some sanctuary from the life threatening effects of a bushfire. I.e. direct flame contact or radiant heat."@en ;
    skos:historyNote "Inherited from ICSM Place Names Working Group's National Feature Catalogue as at 21 December 2023." ;
    skos:inScheme cs: ;
    skos:prefLabel "Neighbourhood Safer Place"@en ;
.

go:netball-court
    a skos:Concept ;
    rdfs:isDefinedBy cs: ;
    skos:definition "A place where netball is played."@en ;
    skos:historyNote "Inherited from ICSM Place Names Working Group's National Feature Catalogue as at 21 December 2023." ;
    skos:inScheme cs: ;
    skos:prefLabel "Netball Court"@en ;
.

go:neve
    a skos:Concept ;
    rdfs:isDefinedBy cs: ;
    skos:definition "The crystalline or granular snow on the upper part of a glacier, which has not yet been compressed into ice; a field or bed of frozen snow."@en ;
    skos:historyNote "Inherited from ICSM Place Names Working Group's National Feature Catalogue as at 21 December 2023. Concept and definition from the Australian Antarctic Division." ;
    skos:inScheme cs: ;
    skos:prefLabel "Neve"@en ;
    schema:citation "https://data.aad.gov.au/aadc/ftc/display_feature_type.cfm?feature_type_code=396"^^xsd:anyURI ;
.

go:nickel-refinery
    a skos:Concept ;
    rdfs:isDefinedBy cs: ;
    skos:definition "A refinery for extracting nickel."@en ;
    skos:historyNote "Inherited from ICSM Place Names Working Group's National Feature Catalogue as at 21 December 2023." ;
    skos:inScheme cs: ;
    skos:prefLabel "Nickel Refinery"@en ;
.

go:non-vehicular-track
    a skos:Concept ;
    rdfs:isDefinedBy cs: ;
    skos:altLabel "Trail"@en ;
    skos:definition "Track or trail not for vehicle use."@en ;
    skos:historyNote "Inherited from ICSM Place Names Working Group's National Feature Catalogue as at 21 December 2023, with name label amended 2024-05-04 from 'Trail' for clarity." ;
    skos:inScheme cs: ;
    skos:narrower
        go:horse-riding-trail ,
        go:mountain-bike-trail ,
        go:multiuse-trail ,
        go:ski-trail ,
        go:stock-route ,
        go:walking-trail ;
    skos:prefLabel "Non Vehicular Track"@en ;
.

go:nunatak
    a skos:Concept ;
    rdfs:isDefinedBy cs: ;
    skos:definition "A small mountain, rocky crag or outcrop projecting from a glacier, ice shelf or snowfield."@en ;
    skos:historyNote "Inherited from ICSM Place Names Working Group's National Feature Catalogue as at 21 December 2023.Concept and definition from the Australian Antarctic Division." ;
    skos:inScheme cs: ;
    skos:prefLabel "Nunatak"@en ;
    schema:citation "https://data.aad.gov.au/aadc/ftc/display_feature_type.cfm?feature_type_code=397"^^xsd:anyURI ;
.

go:obelisk
    a skos:Concept ;
    rdfs:isDefinedBy cs: ;
    skos:definition "A tapering, four-sided shaft of stone, usually monolithic and having a pyramidal apex."@en ;
    skos:historyNote "Created by separating 'Monument' alternate labels 2024-03-05. Definition from Macquarie Dictionary." ;
    skos:inScheme cs: ;
    skos:prefLabel "Obelisk"@en ;
.

go:observatory
    a skos:Concept ;
    rdfs:isDefinedBy cs: ;
    skos:definition "An institution or building specially designed and equipped for observing meteorological and astronomical phenomena."@en ;
    skos:historyNote "Inherited from ICSM Place Names Working Group's National Feature Catalogue as at 21 December 2023." ;
    skos:inScheme cs: ;
    skos:narrower go:weather-station ;
    skos:prefLabel "Observatory"@en ;
.

go:ocean
    a skos:Concept ;
    rdfs:isDefinedBy cs: ;
    skos:definition "Any of the geographical divisions of the vast body of salt water which covers almost three quarters of the earth’s surface."@en ;
    skos:historyNote "Broader term created by separating 'Sea' alternate labels 2024-03-05. Definition added from Macquarie Dictionary." ;
    skos:inScheme cs: ;
    skos:narrower go:sea ;
    skos:prefLabel "Ocean"@en ;
.

go:oeec
    a skos:Concept ;
    rdfs:isDefinedBy cs: ;
    skos:definition "A facility that promotes and delivers outdoor and environmental education programs for schools and the community."@en ;
    skos:historyNote "Added by Queensland 2024-06-05." ;
    skos:inScheme cs: ;
    skos:prefLabel "Outdoor and Environmental Education Centre"@en ;
.

go:oil-field
    a skos:Concept ;
    rdfs:isDefinedBy cs: ;
    skos:definition "An area in which oil resources have been identified."@en ;
    skos:historyNote "Created by separating 'Oil and Gas Field' alternate labels 2024-03-05." ;
    skos:inScheme cs: ;
    skos:prefLabel "Oil Field"@en ;
.

go:oil-gas-field
    a skos:Concept ;
    rdfs:isDefinedBy cs: ;
    skos:definition "An area in which oil and gas resources have been identified."@en ;
    skos:historyNote "Inherited from ICSM Place Names Working Group's National Feature Catalogue as at 21 December 2023." ;
    skos:inScheme cs: ;
    skos:narrower
        go:gas-field ,
        go:oil-field ;
    skos:prefLabel "Oil and Gas Field"@en ;
.

go:oil-gas-platform
    a skos:Concept ;
    rdfs:isDefinedBy cs: ;
    skos:altLabel
        "Drilling Rig"@en ,
        "Offshore Platform"@en ;
    skos:definition "A large structure with facilities to drill wells, to extract and process oil and natural gas."@en ;
    skos:historyNote "Inherited from ICSM Place Names Working Group's National Feature Catalogue as at 21 December 2023." ;
    skos:inScheme cs: ;
    skos:narrower
        go:gas-platform ,
        go:oil-platform ;
    skos:prefLabel "Oil and Gas Platform"@en ;
.

go:oil-gas-well
    a skos:Concept ;
    rdfs:isDefinedBy cs: ;
    skos:definition "A hole drilled into the ground to extract oil or gas."@en ;
    skos:historyNote "Inherited from ICSM Place Names Working Group's National Feature Catalogue as at 21 December 2023." ;
    skos:inScheme cs: ;
    skos:narrower
        go:gas-well ,
        go:oil-well ;
    skos:prefLabel "Oil and Gas Well"@en ;
.

go:oil-pipeline
    a skos:Concept ;
    rdfs:isDefinedBy cs: ;
    skos:definition "A long pipe, typically underground, used to transport oil over long distances."@en ;
    skos:historyNote "Inherited from ICSM Place Names Working Group's National Feature Catalogue as at 21 December 2023." ;
    skos:inScheme cs: ;
    skos:prefLabel "Oil Pipeline"@en ;
.

go:oil-platform
    a skos:Concept ;
    rdfs:isDefinedBy cs: ;
    skos:altLabel "Oil Rig"@en ;
    skos:definition "A large structure with facilities to drill wells, to extract and process oil."@en ;
    skos:historyNote "Created by separating 'Oil and Gas Platform' alternate labels 2024-03-05." ;
    skos:inScheme cs: ;
    skos:prefLabel "Oil Platform"@en ;
.

go:oil-refinery
    a skos:Concept ;
    rdfs:isDefinedBy cs: ;
    skos:definition "An industrial processing plant where crude oil is refined to produce petroleum product."@en ;
    skos:historyNote "Inherited from ICSM Place Names Working Group's National Feature Catalogue as at 21 December 2023." ;
    skos:inScheme cs: ;
    skos:prefLabel "Oil Refinery"@en ;
.

go:oil-well
    a skos:Concept ;
    rdfs:isDefinedBy cs: ;
    skos:definition "A hole drilled into the ground to extract oil."@en ;
    skos:historyNote "Created by separating 'Oil and Gas Well' alternate labels 2024-03-05." ;
    skos:inScheme cs: ;
    skos:prefLabel "Oil Well"@en ;
.

go:opal-field
    a skos:Concept ;
    rdfs:isDefinedBy cs: ;
    skos:definition "An area in which opals have been found and where mines have been established."@en ;
    skos:historyNote "Inherited from ICSM Place Names Working Group's National Feature Catalogue as at 21 December 2023." ;
    skos:inScheme cs: ;
    skos:prefLabel "Opal Field"@en ;
.

go:open-cut-mine
    a skos:Concept ;
    rdfs:isDefinedBy cs: ;
    skos:altLabel
        "Open Pit Mine"@en ,
        "Open Surface Mine"@en ,
        "Strip Mine"@en ;
    skos:definition "A place or area from which commercial minerals are removed from the Earth."@en ;
    skos:historyNote "Inherited from ICSM Place Names Working Group's National Feature Catalogue as at 21 December 2023." ;
    skos:inScheme cs: ;
    skos:prefLabel "Open Cut Mine"@en ;
.

go:outcamp
    a skos:Concept ;
    rdfs:isDefinedBy cs: ;
    skos:altLabel
        "Aboriginal Location"@en ,
        "Homelands"@en ;
    skos:definition "Small Aboriginal community outside of the main community."@en ;
    skos:historyNote "Inherited from ICSM Place Names Working Group's National Feature Catalogue as at 21 December 2023." ;
    skos:inScheme cs: ;
    skos:prefLabel "Outcamp"@en ;
.

go:outcrop
    a skos:Concept ;
    rdfs:isDefinedBy cs: ;
    skos:definition "A visible exposure of bedrock; a cropping out, as of a stratum or vein at the surface of the earth."@en ;
    skos:historyNote "Created by separating 'Rock' alternate labels 2024-06-10. Definition adapted from Macquarie Dictionary." ;
    skos:inScheme cs: ;
    skos:prefLabel "Outcrop"@en ;
.

go:outstation
    a skos:Concept ;
    rdfs:isDefinedBy cs: ;
    skos:altLabel "Aboriginal Outstation"@en ;
    skos:definition "Accommodation outside of the main homestead complex within a rural property."@en ;
    skos:historyNote "Inherited from ICSM Place Names Working Group's National Feature Catalogue as at 21 December 2023, with 'pastoral' amended to 'rural' in description for continuity." ;
    skos:inScheme cs: ;
    skos:prefLabel "Outstation"@en ;
.

go:oxbow
    a skos:Concept ;
    rdfs:isDefinedBy cs: ;
    skos:definition "A former meander of a river remaining as a small bow-shaped lake after the river has straightened its course by cutting through the neck of the meander."@en ;
    skos:historyNote "Concept created by separating 'Lake' alternate labels 2024-06-10. Definition added from Macquarie Dictionary." ;
    skos:inScheme cs: ;
    skos:prefLabel "Oxbow"@en ;
.

go:paddock
    a skos:Concept ;
    rdfs:isDefinedBy cs: ;
    skos:altLabel "Field"@en ;
    skos:definition "A specific area, typically within a farm or pastoral property."@en ;
    skos:historyNote "Inherited from ICSM Place Names Working Group's National Feature Catalogue as at 21 December 2023." ;
    skos:inScheme cs: ;
    skos:prefLabel "Paddock"@en ;
.

go:pan
    a skos:Concept ;
    rdfs:isDefinedBy cs: ;
    skos:definition "A small depression, intermittently containing water, which may sometimes hold deposits, typically clay or salt."@en ;
    skos:historyNote "Inherited from ICSM Place Names Working Group's National Feature Catalogue as at 21 December 2023." ;
    skos:inScheme cs: ;
    skos:narrower
        go:clay-pan ,
        go:salt-pan ;
    skos:prefLabel "Pan"@en ;
.

go:parish
    a skos:Concept ;
    rdfs:isDefinedBy cs: ;
    skos:altLabel "Hundred"@en ;
    skos:definition "A subdivision of the Counties into land units."@en ;
    skos:historyNote "Inherited from ICSM Place Names Working Group's National Feature Catalogue as at 21 December 2023." ;
    skos:inScheme cs: ;
    skos:prefLabel "Parish"@en ;
	skos:scopeNote "No longer in use; recognised for historically named features only. Hundred the preferred term for South Australia. " ;
.

go:park
    a skos:Concept ;
    rdfs:isDefinedBy cs: ;
    skos:altLabel
        "City Square"@en ,
        "Common"@en ,
        "Forecourt"@en ,
        "Local Park"@en ,
        "Rec Reserve"@en ;
    skos:definition "An area of land often with recreational and other facilities which is set aside for public use"@en ;
    skos:historyNote "Inherited from ICSM Place Names Working Group's National Feature Catalogue as at 21 December 2023." ;
    skos:inScheme cs: ;
    skos:prefLabel "Park"@en ;
.

go:pass
    a skos:Concept ;
    rdfs:isDefinedBy cs: ;
    skos:altLabel
        "Col"@en ,
        "Gap"@en ,
        "Saddle"@en ;
    skos:definition "A break or gap in a mountain range permitting easier passage from one side to the other."@en ;
    skos:historyNote "Inherited from ICSM Place Names Working Group's National Feature Catalogue as at 21 December 2023." ;
    skos:inScheme cs: ;
    skos:narrower go:marine-gap ;
    skos:prefLabel "Pass"@en ;
.

go:passenger-ferry-route
    a skos:Concept ;
    rdfs:isDefinedBy cs: ;
    skos:definition "Route for a passenger only ferry."@en ;
    skos:historyNote "Added by Queensland 2024-06-04 from Queensland Roads and Tracks dataset." ;
    skos:inScheme cs: ;
    skos:prefLabel "Passenger ferry route"@en ;
.

go:pastoral-district
    a skos:Concept ;
    rdfs:isDefinedBy cs: ;
    skos:definition "A delineation of land to assist in the administration of pastoral runs."@en ;
    skos:historyNote "Inherited from ICSM Place Names Working Group's National Feature Catalogue as at 21 December 2023." ;
    skos:inScheme cs: ;
    skos:prefLabel "Pastoral District"@en ;
.

go:path
    a skos:Concept ;
    rdfs:isDefinedBy cs: ;
    skos:definition "A path primarily for pedestrian and/or bicycle use. This is not a shared roadway with vehicular traffic."@en ;
    skos:historyNote "Broader concept introduced 2024-06-04." ;
    skos:inScheme cs: ;
    skos:narrower
        go:bikeway ,
        go:cycle-crossing ,
        go:foot-tunnel ,
        go:green-bridge ,
        go:walkway ;
    skos:prefLabel "Path"@en ;
.

go:peak
    a skos:Concept ;
    rdfs:isDefinedBy cs: ;
    skos:altLabel
        "Pillar"@en ,
        "Rock Column"@en ,
        "Summit"@en ;
    skos:definition "A high point of a mountain or a ridge."@en ;
    skos:historyNote "Inherited from ICSM Place Names Working Group's National Feature Catalogue as at 21 December 2023." ;
    skos:inScheme cs: ;
    skos:narrower go:aiguille ;
    skos:prefLabel "Peak"@en ;
.

go:peninsula
    a skos:Concept ;
    rdfs:isDefinedBy cs: ;
    skos:altLabel "Promontory"@en ;
    skos:definition "An area of land almost surrounded by water and significantly larger than a cape."@en ;
    skos:historyNote "Inherited from ICSM Place Names Working Group's National Feature Catalogue as at 21 December 2023." ;
    skos:inScheme cs: ;
    skos:prefLabel "Peninsula"@en ;
.

go:phone-tower
    a skos:Concept ;
    rdfs:isDefinedBy cs: ;
    skos:altLabel "Telephone Tower"@en ;
    skos:definition "Tower that supports the antennas and transmitters needed for telephone communication, including landline and cellular services. They enable the wireless connectivity for telephone calls over a wide area."@en ;
    skos:historyNote "Created by separating 'Communication Tower' alternate labels 2024-06-10." ;
    skos:inScheme cs: ;
    skos:narrower go:mobile-phone-tower ;
    skos:prefLabel "Phone Tower"@en ;
.

go:picnic-site
    a skos:Concept ;
    rdfs:isDefinedBy cs: ;
    skos:altLabel
        "DUA"@en ,
        "Day Use Area"@en ,
        "Picnic Area"@en ;
    skos:definition "A tract of land reserved for day picnic purposes, sometimes with constructed fireplaces and other facilities"@en ;
    skos:historyNote "Inherited from ICSM Place Names Working Group's National Feature Catalogue as at 21 December 2023." ;
    skos:inScheme cs: ;
    skos:prefLabel "Picnic Site"@en ;
.

go:pier
    a skos:Concept ;
    rdfs:isDefinedBy cs: ;
    skos:definition "A long narrow structure extending into the water to afford a berthing place for vessels; also serves as a pleasure promenade."@en ;
    skos:historyNote "Inherited from ICSM Place Names Working Group's National Feature Catalogue as at 21 December 2023." ;
    skos:inScheme cs: ;
    skos:prefLabel "Pier"@en ;
.

go:pipeline
    a skos:Concept ;
    rdfs:isDefinedBy cs: ;
    skos:definition "A long pipe, typically underground, used to transport substances over long distances."@en ;
    skos:historyNote "Broader concept introduced 2024-06-04." ;
    skos:inScheme cs: ;
    skos:narrower
        go:gas-pipeline ,
        go:oil-pipeline ;
    skos:prefLabel "Pipeline"@en ;
.

go:place-industrial-activity
    a skos:Concept ;
    rdfs:isDefinedBy cs: ;
    skos:definition "Place where an industrial activity takes place."@en ;
    skos:historyNote "New broader term added 2024-06-05." ;
    skos:inScheme cs: ;
    skos:narrower
        go:agriculture ,
        go:aquaculture ,
        go:industrial-production-facility ,
        go:mining-feature ;
    skos:prefLabel "Place of Industrial Activity"@en ;
    skos:topConceptOf cs: ;
.

go:place-of-worship
    a skos:Concept ;
    rdfs:isDefinedBy cs: ;
    skos:definition "Places used for spiritual observation or ceremonial purposes."@en ;
    skos:historyNote "Inherited from ICSM Place Names Working Group's National Feature Catalogue as at 21 December 2023." ;
    skos:inScheme cs: ;
    skos:narrower
        go:abbey ,
        go:cathedral ,
        go:chapel ,
        go:church ,
        go:gurdwara ,
        go:mission ,
        go:mondir ,
        go:mosque ,
        go:synagogue ,
        go:vihara ;
    skos:prefLabel "Place of Worship"@en ;
.

go:plain
    a skos:Concept ;
    rdfs:isDefinedBy cs: ;
    skos:altLabel "Flat"@en ;
    skos:definition "A tract of country, the general surface of which is comparatively flat and which is sparsely, if at all, timbered."@en ;
    skos:historyNote "Inherited from ICSM Place Names Working Group's National Feature Catalogue as at 21 December 2023." ;
    skos:inScheme cs: ;
    skos:narrower
        go:alluvial-plain ,
        go:clearing ,
        go:downs ,
        go:prairie ,
        go:volcanic-plain ;
    skos:prefLabel "Plain"@en ;
.

go:plateau
    a skos:Concept ;
    rdfs:isDefinedBy cs: ;
    skos:altLabel
        "Platform"@en ,
        "Tableland"@en ;
    skos:definition "An elevated tract of comparatively flat or level land."@en ;
    skos:historyNote "Inherited from ICSM Place Names Working Group's National Feature Catalogue as at 21 December 2023." ;
    skos:inScheme cs: ;
    skos:narrower go:marine-plateau ;
    skos:prefLabel "Plateau"@en ;
.

go:playground
    a skos:Concept ;
    rdfs:isDefinedBy cs: ;
    skos:altLabel "Play Park"@en ;
    skos:definition "An outdoor area for children's play."@en ;
    skos:historyNote "Inherited from ICSM Place Names Working Group's National Feature Catalogue as at 21 December 2023." ;
    skos:inScheme cs: ;
    skos:prefLabel "Playground"@en ;
.

go:pocket
    a skos:Concept ;
    rdfs:isDefinedBy cs: ;
    skos:definition "An area of land encompassed by the meander of a river."@en ;
    skos:historyNote "Inherited from ICSM Place Names Working Group's National Feature Catalogue as at 21 December 2023." ;
    skos:inScheme cs: ;
    skos:prefLabel "Pocket"@en ;
.

go:point
    a skos:Concept ;
    rdfs:isDefinedBy cs: ;
    skos:definition "A small protrusion of land into the sea or a lake, often the outer end of a larger landform such as a cape."@en ;
    skos:historyNote "Inherited from ICSM Place Names Working Group's National Feature Catalogue as at 21 December 2023." ;
    skos:inScheme cs: ;
    skos:prefLabel "Point"@en ;
.

go:police-station
    a skos:Concept ;
    rdfs:isDefinedBy cs: ;
    skos:definition "An office of the local police force; it may or may not have an associated lock-up."@en ;
    skos:historyNote "Inherited from ICSM Place Names Working Group's National Feature Catalogue as at 21 December 2023." ;
    skos:inScheme cs: ;
    skos:prefLabel "Police Station"@en ;
.

go:populated-place
    a skos:Concept ;
    rdfs:isDefinedBy cs: ;
    skos:definition "Places relating to population entities, both current and historical."@en ;
    skos:historyNote "Inherited from ICSM Place Names Working Group's National Feature Catalogue as at 21 December 2023." ;
    skos:inScheme cs: ;
    skos:narrower
        go:neighbourhood ,
        go:outcamp ,
        go:population-centre ,
        go:settlement ;
    skos:prefLabel "Populated Place"@en ;
.

go:population-centre
    a skos:Concept ;
    rdfs:isDefinedBy cs: ;
    skos:altLabel
        "City"@en ,
        "Town"@en ,
        "Township"@en ,
        "Village"@en ;
    skos:definition "A significant place where there is permanent human habitation, infrastructure and services."@en ;
    skos:historyNote "Inherited from ICSM Place Names Working Group's National Feature Catalogue as at 21 December 2023." ;
    skos:inScheme cs: ;
    skos:prefLabel "Population Centre"@en ;
.

go:port
    a skos:Concept ;
    rdfs:isDefinedBy cs: ;
    skos:definition "A place provided with terminal and transfer facilities for loading and discharging cargo or passengers, usually located in a harbour."@en ;
    skos:historyNote "Inherited from ICSM Place Names Working Group's National Feature Catalogue as at 21 December 2023." ;
    skos:inScheme cs: ;
    skos:prefLabel "Port"@en ;
.

go:post-office
    a skos:Concept ;
    rdfs:isDefinedBy cs: ;
    skos:definition "A local office for receiving, distributing and transmitting mail, providing telecommunication services."@en ;
    skos:historyNote "Inherited from ICSM Place Names Working Group's National Feature Catalogue as at 21 December 2023." ;
    skos:inScheme cs: ;
    skos:prefLabel "Post Office"@en ;
.

go:power-distribution-line
    a skos:Concept ;
    rdfs:isDefinedBy cs: ;
    skos:definition "A wire used for the distribution of electricity."@en ;
    skos:historyNote "Inherited from ICSM Place Names Working Group's National Feature Catalogue as at 21 December 2023, with name label amended from 'Power Distribution'." ;
    skos:inScheme cs: ;
    skos:prefLabel "Power Distribution Line"@en ;
.

go:power-station
    a skos:Concept ;
    rdfs:isDefinedBy cs: ;
    skos:definition "A process plant that creates power from one or more sources."@en ;
    skos:historyNote "Inherited from ICSM Place Names Working Group's National Feature Catalogue as at 21 December 2023." ;
    skos:inScheme cs: ;
    skos:narrower
        go:biomass-power-station ,
        go:coal-power-station ,
        go:gas-power-station ,
        go:geothermal-power-station ,
        go:hydroelectric-power-station ,
        go:solar-power-station ,
        go:wind-farm ;
    skos:prefLabel "Power Station"@en ;
.

go:power-sub-station
    a skos:Concept ;
    rdfs:isDefinedBy cs: ;
    skos:altLabel
        "Power Terminal Sub Station"@en ,
        "Zone Substation"@en ;
    skos:definition "A facility whose primary purpose is to convert incoming sub-transmission voltages to high voltage distribution voltages -usually owned by the distribution company."@en ;
    skos:historyNote "Inherited from ICSM Place Names Working Group's National Feature Catalogue as at 21 December 2023." ;
    skos:inScheme cs: ;
    skos:prefLabel "Power Sub Station"@en ;
.

go:power-sub-transmission-line
    a skos:Concept ;
    rdfs:isDefinedBy cs: ;
    skos:altLabel "Power Subtransmission"@en ;
    skos:definition "A wire used for the transmission of electricity usually < 66KV."@en ;
    skos:historyNote "Inherited from ICSM Place Names Working Group's National Feature Catalogue as at 21 December 2023, with name label amended from 'Power Sub Transmission'." ;
    skos:inScheme cs: ;
    skos:prefLabel "Power Sub Transmission Line"@en ;
.

go:power-terminal-station
    a skos:Concept ;
    rdfs:isDefinedBy cs: ;
    skos:altLabel "Power Terminal"@en ;
    skos:definition "A facility whose primary purpose is to convert incoming transmission voltages to voltages suitable for distribution networks-usually owned by the transmission company."@en ;
    skos:historyNote "Inherited from ICSM Place Names Working Group's National Feature Catalogue as at 21 December 2023." ;
    skos:inScheme cs: ;
    skos:prefLabel "Power Terminal Station"@en ;
.

go:power-transmission-line
    a skos:Concept ;
    rdfs:isDefinedBy cs: ;
    skos:definition "A wire used for the transmission of electricity usually > 66KV."@en ;
    skos:historyNote "Inherited from ICSM Place Names Working Group's National Feature Catalogue as at 21 December 2023, with name label amended from 'Power Transmission'." ;
    skos:inScheme cs: ;
    skos:prefLabel "Power Transmission Line"@en ;
.

go:prairie
    a skos:Concept ;
    rdfs:isDefinedBy cs: ;
    skos:definition "An extensive or slightly undulating treeless tract of land, characterised by highly fertile soil and originally grassland, which occurs in the interior of continents in temperate latitudes."@en ;
    skos:historyNote "Created by separating 'Plain' alternate labels 2024-06-10. Definition from Macquarie Dictionary." ;
    skos:inScheme cs: ;
    skos:prefLabel "Prairie"@en ;
.

go:precipice
    a skos:Concept ;
    rdfs:isDefinedBy cs: ;
    skos:definition "A cliff with a vertical, or nearly vertical, or overhanging face."@en ;
    skos:historyNote "Created by separating 'Cliff' alternate labels 2024-05-10. Definition from Macquarie Dictionary." ;
    skos:inScheme cs: ;
    skos:prefLabel "Precipice"@en ;
.

go:primary-school
    a skos:Concept ;
    rdfs:isDefinedBy cs: ;
    skos:definition "An education facility that caters for 5- 12 year olds, private and public."@en ;
    skos:historyNote "Inherited from ICSM Place Names Working Group's National Feature Catalogue as at 21 December 2023." ;
    skos:inScheme cs: ;
    skos:prefLabel "Primary School"@en ;
.

go:primary-secondary-school
    a skos:Concept ;
    rdfs:isDefinedBy cs: ;
    skos:altLabel "Combined School"@en ;
    skos:definition "A combined primary and secondary school."@en ;
    skos:historyNote "Inherited from ICSM Place Names Working Group's National Feature Catalogue as at 21 December 2023." ;
    skos:inScheme cs: ;
    skos:prefLabel "Primary and Secondary School"@en ;
.

go:prison
    a skos:Concept ;
    rdfs:isDefinedBy cs: ;
    skos:altLabel
        "Detention Centre"@en ,
        "Gaol"@en ,
        "Jail"@en ,
        "Rehabilitation Centre"@en ,
        "Remand Centre"@en ;
    skos:definition "A building where persons are legally committed for punishment or while awaiting trial."@en ;
    skos:historyNote "Inherited from ICSM Place Names Working Group's National Feature Catalogue as at 21 December 2023." ;
    skos:inScheme cs: ;
    skos:prefLabel "Prison"@en ;
.

go:property
    a skos:Concept ;
    rdfs:isDefinedBy cs: ;
    skos:definition "An area of commonly owned land with a single usage by a individual entity."@en ;
    skos:historyNote "Added by Queensland 2024-06-05." ;
    skos:inScheme cs: ;
    skos:narrower
        go:addressable-property ,
        go:rural-property ;
    skos:prefLabel "Property"@en ;
.

go:protected-area
    a skos:Concept ;
    rdfs:isDefinedBy cs: ;
    skos:definition "An area of land and/or sea especially dedicated to the protection and maintenance of biological diversity and/or of natural and associated cultural resources. The area is managed through legal or other effective means."@en ;
    skos:historyNote "Inherited from ICSM Place Names Working Group's National Feature Catalogue as at 21 December 2023. Definition from the Australian Antarctic Division." ;
    skos:inScheme cs: ;
    skos:narrower
        go:antarctic-specially-managed-areas ,
        go:antarctic-specially-protected-areas ,
        go:coastal-reserve ,
        go:conservation-park ,
        go:indigenous-protected-area ,
        go:marine-park ,
        go:national-park ,
        go:state-forest ;
    skos:prefLabel "Protected Area"@en ;
    schema:citation "https://data.aad.gov.au/aadc/ftc/display_feature_type.cfm?feature_type_code=267"^^xsd:anyURI ;
.

go:pumping-station
    a skos:Concept ;
    rdfs:isDefinedBy cs: ;
    skos:definition "A pumping station to support water flows."@en ;
    skos:historyNote "Inherited from ICSM Place Names Working Group's National Feature Catalogue as at 21 December 2023." ;
    skos:inScheme cs: ;
    skos:prefLabel "Pumping Station"@en ;
.

go:quarry
    a skos:Concept ;
    rdfs:isDefinedBy cs: ;
    skos:altLabel
        "Clay Pit"@en ,
        "Pit"@en ;
    skos:definition "An open surface excavation used for the extraction of stone."@en ;
    skos:historyNote "Inherited from ICSM Place Names Working Group's National Feature Catalogue as at 21 December 2023." ;
    skos:inScheme cs: ;
    skos:narrower go:abandoned-quarry ;
    skos:prefLabel "Quarry"@en ;
.

go:racecourse
    a skos:Concept ;
    rdfs:isDefinedBy cs: ;
    skos:altLabel "Horse Racetrack"@en ;
    skos:definition "A piece of ground on which horse races are held for public entertainment; any place where horse races are held."@en ;
    skos:historyNote "Inherited from ICSM Place Names Working Group's National Feature Catalogue as at 21 December 2023." ;
    skos:inScheme cs: ;
    skos:prefLabel "Racecourse"@en ;
.

go:racetrack
    a skos:Concept ;
    rdfs:isDefinedBy cs: ;
    skos:definition "A typically oval course or track on which races are held."@en ;
    skos:historyNote "Broader concept introduced 2024-03-05. Definition from the Oxford English Dictionary." ;
    skos:inScheme cs: ;
    skos:narrower
        go:greyhound-racetrack ,
        go:harness-racetrack ,
        go:motor-track ,
        go:racecourse ;
    skos:prefLabel "Racetrack"@en ;
.

go:radio-communication-facility
    a skos:Concept ;
    rdfs:isDefinedBy cs: ;
    skos:altLabel "Radio Broadcasting Facility"@en ;
    skos:definition "A set of equipment including a radio tower and the associated equipment like transmitters, receivers, control systems, and other infrastructures necessary for radio communication."@en ;
    skos:historyNote "Inherited from ICSM Place Names Working Group's National Feature Catalogue as at 21 December 2023. Definition updated 2024-06-10." ;
    skos:inScheme cs: ;
    skos:prefLabel "Radio Communication Facility"@en ;
.

go:radio-mast
    a skos:Concept ;
    rdfs:isDefinedBy cs: ;
    skos:definition "A tall, slender structure designed to support antennas at a high elevation for radio broadcasting and communication. Unlike towers, which are usually freestanding and have accessible platforms or equipment rooms, a mast is often supported by guy-wires for stability and may not be accessible for human occupation."@en ;
    skos:historyNote "Created by separating 'Communication Tower' alternate labels 2024-06-10." ;
    skos:inScheme cs: ;
    skos:prefLabel "Radio Mast"@en ;
.

go:radio-station
    a skos:Concept ;
    rdfs:isDefinedBy cs: ;
    skos:definition "A facility to operate the transmission of radio broadcasts."@en ;
    skos:historyNote "Inherited from ICSM Place Names Working Group's National Feature Catalogue as at 21 December 2023." ;
    skos:inScheme cs: ;
    skos:prefLabel "Radio Station"@en ;
.

go:radio-tower
    a skos:Concept ;
    rdfs:isDefinedBy cs: ;
    skos:definition "A structure designed specifically to support the antennas for transmitting and receiving radio waves. These towers are used for broadcasting radio programming across various frequencies, including AM and FM radio services. The term can sometimes be used interchangeably with a broadcasting tower."@en ;
    skos:historyNote "Created by separating 'Communication Tower' alternate labels 2024-06-10." ;
    skos:inScheme cs: ;
    skos:prefLabel "Radio Tower"@en ;
.

go:rail-cutting
    a skos:Concept ;
    rdfs:isDefinedBy cs: ;
    skos:definition "An excavation in the Earth's surface to create a thoroughfare for a rail line."@en ;
    skos:historyNote "Inherited from ICSM Place Names Working Group's National Feature Catalogue as at 21 December 2023." ;
    skos:inScheme cs: ;
    skos:prefLabel "Rail Cutting"@en ;
.

go:rail-transport-infrastructure
    a skos:Concept ;
    rdfs:isDefinedBy cs: ;
    skos:definition "Installations, systems, and structures that enable the operation of trains and serve as the foundation for railway transportation."@en ;
    skos:historyNote "Broader concept introduced 2024-03-05." ;
    skos:inScheme cs: ;
    skos:narrower
        go:light-rail-transport-infrastructure ,
        go:rail-bridge ,
        go:rail-cutting ,
        go:rail-station ,
        go:rail-tunnel ,
        go:rail-yard ,
        go:railway ,
        go:siding ,
        go:tram-transport-infrastructure ;
    skos:prefLabel "Rail Transport Infrastructure"@en ;
.

go:rail-yard
    a skos:Concept ;
    rdfs:isDefinedBy cs: ;
    skos:altLabel
        "Marshalling Yard"@en ,
        "Railway Yard"@en ;
    skos:definition "An area of railway tracks and sidings for storage and maintenance of trains."@en ;
    skos:historyNote "Inherited from ICSM Place Names Working Group's National Feature Catalogue as at 21 December 2023." ;
    skos:inScheme cs: ;
    skos:prefLabel "Rail Yard"@en ;
.

go:railway
    a skos:Concept ;
    rdfs:isDefinedBy cs: ;
    skos:altLabel "Rail"@en ;
    skos:definition "A track or set of tracks of iron or steel rails used for the passage of trains."@en ;
    skos:historyNote "Inherited from ICSM Place Names Working Group's National Feature Catalogue as at 21 December 2023." ;
    skos:inScheme cs: ;
    skos:prefLabel "Railway"@en ;
.

go:ramp
    a skos:Concept ;
    rdfs:isDefinedBy cs: ;
    skos:altLabel
        "Exit Ramp"@en ,
        "Off Ramp"@en ,
        "On Ramp"@en ;
    skos:definition "Roadways that enable vehicles to enter or leave major roads. On ramps enable vehicles to accelerate and merge onto highways or motorways, increasing their speed to match that of the traffic already on the highway, thereby safely merging with the through traffic. Off-ramps are designed to facilitate a smooth transition from high-speed travelling lanes to lower-speed areas or different directions of travel."@en ;
    skos:historyNote "Added by Queensland 2024-06-04 from Queensland Roads and Tracks dataset." ;
    skos:inScheme cs: ;
    skos:prefLabel "Ramp"@en ;
.

go:range
    a skos:Concept ;
    rdfs:isDefinedBy cs: ;
    skos:altLabel
        "Hills"@en ,
        "Mountain Chain"@en ,
        "Mountain Range"@en ,
        "Mountains"@en ;
    skos:definition "A series or line of mountains or hills with or without peaks in which the crests are relatively narrow."@en ;
    skos:historyNote "Inherited from ICSM Place Names Working Group's National Feature Catalogue as at 21 December 2023." ;
    skos:inScheme cs: ;
    skos:narrower go:seamount-chain ;
    skos:prefLabel "Range"@en ;
.

go:rapids
    a skos:Concept ;
    rdfs:isDefinedBy cs: ;
    skos:definition "Portions of a stream with accelerated current where it descends rapidly without a break in the slope of the bed sufficient to form a waterfall."@en ;
    skos:historyNote "Inherited from ICSM Place Names Working Group's National Feature Catalogue as at 21 December 2023." ;
    skos:inScheme cs: ;
    skos:prefLabel "Rapids"@en ;
.

go:reach
    a skos:Concept ;
    rdfs:isDefinedBy cs: ;
    skos:definition "A straight portion of watercourse from one bend to another."@en ;
    skos:historyNote "Inherited from ICSM Place Names Working Group's National Feature Catalogue as at 21 December 2023." ;
    skos:inScheme cs: ;
    skos:prefLabel "Reach"@en ;
.

go:recreational-facility
    a skos:Concept ;
    rdfs:isDefinedBy cs: ;
    skos:definition "Places where the major activity is of a sporting nature."@en ;
    skos:historyNote "Inherited from ICSM Place Names Working Group's National Feature Catalogue as at 21 December 2023, with name label amended 2024-05-04 from 'Recreation' 2024-03-05." ;
    skos:inScheme cs: ;
    skos:narrower
        go:bmx-track ,
        go:boating-club ,
        go:bowling-green ,
        go:croquet-green ,
        go:equestrian-centre ,
        go:firing-range ,
        go:golf-course ,
        go:grandstand ,
        go:playground ,
        go:rowing-course ,
        go:skate-park ,
        go:sports-complex ,
        go:sports-facility ,
        go:sports-pavilion ,
        go:surfing-spot ;
    skos:prefLabel "Recreational Facility"@en ;
.

go:recycling-depot
    a skos:Concept ;
    rdfs:isDefinedBy cs: ;
    skos:definition "A facility where individuals and businesses can bring recyclable materials to be sorted, cleaned, and prepared for processing into new products."@en ;
    skos:historyNote "Created by separating 'Refuse Transfer Station' alternate labels 2024-06-10." ;
    skos:inScheme cs: ;
    skos:prefLabel "Recycling Depot"@en ;
.

go:refuge
    a skos:Concept ;
    rdfs:isDefinedBy cs: ;
    skos:definition "A purpose built or modified structure to provide shelter and supplies to community members in the event of an emergency."@en ;
    skos:historyNote "Inherited from ICSM Place Names Working Group's National Feature Catalogue as at 21 December 2023." ;
    skos:inScheme cs: ;
    skos:narrower
        go:community-fire-refuge ,
        go:cyclone-shelter ;
    skos:prefLabel "Refuge"@en ;
.

go:refuse-transfer-station
    a skos:Concept ;
    rdfs:isDefinedBy cs: ;
    skos:altLabel "Waste Transfer Station"@en ;
    skos:definition "A site used for the temporary sorting of refuse."@en ;
    skos:historyNote "Inherited from ICSM Place Names Working Group's National Feature Catalogue as at 21 December 2023, with name label amended from 'Transfer Station'." ;
    skos:inScheme cs: ;
    skos:narrower
        go:composting-facility ,
        go:recycling-depot ;
    skos:prefLabel "Refuse Transfer Station"@en ;
.

go:reservoir
    a skos:Concept ;
    rdfs:isDefinedBy cs: ;
    skos:definition "An artificial lake for the storage, regulation and control of water for domestic or other use."@en ;
    skos:historyNote "Inherited from ICSM Place Names Working Group's National Feature Catalogue as at 21 December 2023." ;
    skos:inScheme cs: ;
    skos:prefLabel "Reservoir"@en ;
.

go:resource-extraction-feature
    a skos:Concept ;
    rdfs:isDefinedBy cs: ;
    skos:definition "Feature related to extraction of resources."@en ;
    skos:historyNote "Inherited from ICSM Place Names Working Group's National Feature Catalogue as at 21 December 2023, with name label amended 2024-05-04 from 'Extraction' 2024-03-05." ;
    skos:inScheme cs: ;
    skos:narrower
        go:adit ,
        go:mine ,
        go:oil-gas-platform ,
        go:oil-gas-well ,
        go:quarry ;
    skos:prefLabel "Resource Extraction Feature"@en ;
.

go:resource-processing-facility
    a skos:Concept ;
    rdfs:isDefinedBy cs: ;
    skos:definition "A facility for treating or preparing mined materials."@en ;
    skos:historyNote "Inherited from ICSM Place Names Working Group's National Feature Catalogue as at 21 December 2023, with name label amended 2024-05-04 from 'Processing' 2024-03-05." ;
    skos:inScheme cs: ;
    skos:narrower
        go:alumina-refinery ,
        go:battery ,
        go:gold-refinery ,
        go:iron-ore-processor ,
        go:mineral-sand-processing-plant ,
        go:nickel-refinery ,
        go:oil-refinery ,
        go:smelter ;
    skos:prefLabel "Resource Processing Facility"@en ;
.

go:rest-area
    a skos:Concept ;
    rdfs:isDefinedBy cs: ;
    skos:definition "An area at the side of a road or highway for vehicles to stop away from traffic; possibly with toilet and/or picnic facilities."@en ;
    skos:historyNote "Inherited from ICSM Place Names Working Group's National Feature Catalogue as at 21 December 2023." ;
    skos:inScheme cs: ;
    skos:prefLabel "Rest Area"@en ;
.

go:restricted-access-road
    a skos:Concept ;
    rdfs:isDefinedBy cs: ;
    skos:definition "Roads with a physical restriction or barrier to entry, e.g., gates."@en ;
    skos:historyNote "Added by Queensland 2024-06-04 from Queensland Roads and Tracks dataset." ;
    skos:inScheme cs: ;
    skos:prefLabel "Restricted Access Road"@en ;
.

go:retirement-village
    a skos:Concept ;
    rdfs:isDefinedBy cs: ;
    skos:altLabel
        "Retirement Complex"@en ,
        "Retirement Estate"@en ;
    skos:definition "A complex containing residential premises that are intended to be occupied by retired persons."@en ;
    skos:historyNote "Inherited from ICSM Place Names Working Group's National Feature Catalogue as at 21 December 2023." ;
    skos:inScheme cs: ;
    skos:prefLabel "Retirement Village"@en ;
.

go:ridge
    a skos:Concept ;
    rdfs:isDefinedBy cs: ;
    skos:altLabel "Spur"@en ;
    skos:definition "A long and narrow stretch of elevated ground, either isolated or located in a range."@en ;
    skos:historyNote "Inherited from ICSM Place Names Working Group's National Feature Catalogue as at 21 December 2023." ;
    skos:inScheme cs: ;
    skos:prefLabel "Ridge"@en ;
.

go:river
    a skos:Concept ;
    rdfs:isDefinedBy cs: ;
    skos:definition "A defined watercourse of considerable size and length, whether flowing or dry according to the seasons, and whether a single channel or a number of diverging or converging channels."@en ;
    skos:historyNote "Concept created by separating 'Watercourse' alternate labels 2024-06-10. Definition added from Macquarie Dictionary." ;
    skos:inScheme cs: ;
    skos:prefLabel "River"@en ;
.

go:road
    a skos:Concept ;
    rdfs:isDefinedBy cs: ;
    skos:definition "A defined route or path, typically constructed and maintained for the passage of vehicles, bicycles, and pedestrians, connecting different locations and facilitating transportation and communication."@en ;
    skos:historyNote "Inherited from ICSM Place Names Working Group's National Feature Catalogue as at 21 December 2023. Definition from Macquarie Dictionary." ;
    skos:inScheme cs: ;
    skos:narrower
        go:connector-road ,
        go:highway ,
        go:local-road ,
        go:mall ,
        go:motorway ,
        go:restricted-access-road ,
        go:secondary-road ,
        go:unconstructed-road ;
    skos:prefLabel "Road"@en ;
.

go:road-cutting
    a skos:Concept ;
    rdfs:isDefinedBy cs: ;
    skos:definition "An excavation in the Earth's surface to create a thoroughfare for a road."@en ;
    skos:historyNote "Inherited from ICSM Place Names Working Group's National Feature Catalogue as at 21 December 2023." ;
    skos:inScheme cs: ;
    skos:prefLabel "Road Cutting"@en ;
.

go:road-transport-infrastructure
    a skos:Concept ;
    rdfs:isDefinedBy cs: ;
    skos:definition "Facilities and structures designed and built to support the movement of vehicles, goods, and people by road."@en ;
    skos:historyNote "Inherited from ICSM Place Names Working Group's National Feature Catalogue as at 21 December 2023, with name label amended 2024-05-04 from 'Road'." ;
    skos:inScheme cs: ;
    skos:narrower
        go:bus-transport-infrastructure ,
        go:car-park ,
        go:causeway ,
        go:crossover ,
        go:ford ,
        go:gate ,
        go:level-crossing ,
        go:ramp ,
        go:rest-area ,
        go:road ,
        go:road-bridge ,
        go:road-cutting ,
        go:road-tunnel ,
        go:roundabout ,
        go:slip-road ,
        go:taxi-rank ,
        go:toll ,
        go:tourist-route ,
        go:u-turn ,
        go:underpass ,
        go:weighbridge ;
    skos:prefLabel "Road Transport Infrastructure"@en ;
.

go:rock
    a skos:Concept ;
    rdfs:isDefinedBy cs: ;
    skos:definition "A prominent or isolated outcrop of stone."@en ;
    skos:historyNote "Inherited from ICSM Place Names Working Group's National Feature Catalogue as at 21 December 2023." ;
    skos:inScheme cs: ;
    skos:narrower
        go:boulder ,
        go:monolith ,
        go:offshore-rock ,
        go:outcrop ,
        go:stack ;
    skos:prefLabel "Rock"@en ;
.

go:rock-wall
    a skos:Concept ;
    rdfs:isDefinedBy cs: ;
    skos:definition "A perpendicular or steep face of rock, considerable in height."@en ;
    skos:historyNote "Added by Queensland 2024-03-05. Definition from original 'Ice Wall'." ;
    skos:inScheme cs: ;
    skos:prefLabel "Rock Wall"@en ;
.

go:rockface
    a skos:Concept ;
    rdfs:isDefinedBy cs: ;
    skos:definition "The rock surface of the side of a cliff or mountain, especially nearly vertical rock."@en ;
    skos:historyNote "Created by separating 'Cliff' alternate labels 2024-05-10. Definition from Macquarie Dictionary." ;
    skos:inScheme cs: ;
    skos:prefLabel "Rockface"@en ;
.

go:rockhole
    a skos:Concept ;
    rdfs:isDefinedBy cs: ;
    skos:definition "A hole excavated in solid rock by water action."@en ;
    skos:historyNote "Inherited from ICSM Place Names Working Group's National Feature Catalogue as at 21 December 2023." ;
    skos:inScheme cs: ;
    skos:narrower
        go:gnamma-hole ,
        go:native-well ,
        go:runaway-hole ,
        go:sinkhole ;
    skos:prefLabel "Rockhole"@en ;
.

go:rotunda
    a skos:Concept ;
    rdfs:isDefinedBy cs: ;
    skos:altLabel
        "Band Stand"@en ,
        "Pavilion"@en ;
    skos:definition "A building which has a circular plan, especially with a dome, typically found within a park or reserve."@en ;
    skos:historyNote "Inherited from ICSM Place Names Working Group's National Feature Catalogue as at 21 December 2023." ;
    skos:inScheme cs: ;
    skos:prefLabel "Rotunda"@en ;
.

go:roundabout
    a skos:Concept ;
    rdfs:isDefinedBy cs: ;
    skos:definition "A road junction at which traffic moves in one direction around a central island to reach one of the roads converging on it."@en ;
    skos:historyNote "Inherited from ICSM Place Names Working Group's National Feature Catalogue as at 21 December 2023." ;
    skos:inScheme cs: ;
    skos:prefLabel "Roundabout"@en ;
.

go:rowing-course
    a skos:Concept ;
    rdfs:isDefinedBy cs: ;
    skos:definition "An area of water on which rowing is undertaken."@en ;
    skos:historyNote "Inherited from ICSM Place Names Working Group's National Feature Catalogue as at 21 December 2023." ;
    skos:inScheme cs: ;
    skos:prefLabel "Rowing Course"@en ;
.

go:runaway-hole
    a skos:Concept ;
    rdfs:isDefinedBy cs: ;
    skos:altLabel
        "Crabhole"@en ,
        "Gilgai"@en ,
        "Melon Hole"@en ;
    skos:definition "A depression or hole in the ground, especially one which drains off surface water, forming a natural reservoir and resulting from a natural soil formation occurring extensively in inland Australia, characterised by a markedly undulating surface sometimes with mounds and depressions; probably caused by swelling and cracking of clays during alternating wet and dry seasons."@en ;
    skos:historyNote "Created by separating 'Rockhole' alternate labels 2024-06-10. Definition from Macquarie Dictionary." ;
    skos:inScheme cs: ;
    skos:prefLabel "Runaway Hole"@en ;
.

go:runway
    a skos:Concept ;
    rdfs:isDefinedBy cs: ;
    skos:definition "A paved or cleared strip within an airport, airfield, or airstrip, on which aeroplanes land and take off."@en ;
    skos:historyNote "Created by separating 'Landing Area' alternate labels 2024-06-10. Definition adapted from Macquarie Dictionary." ;
    skos:inScheme cs: ;
    skos:prefLabel "Runway"@en ;
.

go:rural-fire-station
    a skos:Concept ;
    rdfs:isDefinedBy cs: ;
    skos:definition "A building in a rural area in which a rural fire brigade is based, and which houses fire engines and other equipment."@en ;
    skos:historyNote "Created by separating 'Fire Station' alternate labels 2024-03-05." ;
    skos:inScheme cs: ;
    skos:prefLabel "Rural Fire Station"@en ;
.

go:rural-property
    a skos:Concept ;
    rdfs:isDefinedBy cs: ;
    skos:altLabel
        "Pastoral Property"@en ,
        "Rural Station"@en ;
    skos:definition "An area of commonly owned land with a single usage by a individual entity, with that usage relating to agricultural or aquacultural activities in a rural area."@en ;
    skos:historyNote "Added by Queensland 2024-03-05." ;
    skos:inScheme cs: ;
    skos:prefLabel "Rural Property"@en ;
.

go:salt-marsh
    a skos:Concept ;
    rdfs:isDefinedBy cs: ;
    skos:definition "A marshy area forming a habitat for a community of plants and low shrubs that can tolerate high soil salinity and the occasional inundation of salt water; often located at the upper levels of the intertidal zone or behind sand dunes."@en ;
    skos:historyNote "Concept created by separating 'Wetland' alternate labels 2024-06-10. Definition added from Macquarie Dictionary." ;
    skos:inScheme cs: ;
    skos:prefLabel "Salt Marsh"@en ;
.

go:salt-pan
    a skos:Concept ;
    rdfs:isDefinedBy cs: ;
    skos:definition "A small depression, intermittently containing water, which holds salt deposits."@en ;
    skos:historyNote "Inherited from ICSM Place Names Working Group's National Feature Catalogue as at 21 December 2023." ;
    skos:inScheme cs: ;
    skos:prefLabel "Salt Pan"@en ;
.

go:sandbar
    a skos:Concept ;
    rdfs:isDefinedBy cs: ;
    skos:altLabel "Sandbank"@en ;
    skos:definition "A bar of sand formed in a sea or river, exposed at low tide and formed by the action of the tides or currents."@en ;
    skos:historyNote "Created by separating 'Bar' alternate labels 2024-05-10. Definition adapted from 'Bar'." ;
    skos:inScheme cs: ;
    skos:prefLabel "Sandbar"@en ;
.

go:sandspit
    a skos:Concept ;
    rdfs:isDefinedBy cs: ;
    skos:altLabel "Sand Spit"@en ;
    skos:definition "A long narrow stretch of sand extending from the land into a body of water, often covered at high tide."@en ;
    skos:historyNote "Created by separating 'Spit' alternate labels 2024-03-05. Definition from Macquarie Dictionary." ;
    skos:inScheme cs: ;
    skos:prefLabel "Sandspit"@en ;
.

go:school
    a skos:Concept ;
    rdfs:isDefinedBy cs: ;
    skos:definition "And educational facility for children."@en ;
    skos:historyNote "New broader concept added by Queensland 2024-03-05" ;
    skos:inScheme cs: ;
    skos:narrower
        go:distance-education ,
        go:primary-school ,
        go:primary-secondary-school ,
        go:secondary-school ,
        go:special-school ;
    skos:prefLabel "School"@en ;
.

go:school-camp
    a skos:Concept ;
    rdfs:isDefinedBy cs: ;
    skos:definition "A camping facility administered by an education centre."@en ;
    skos:historyNote "Inherited from ICSM Place Names Working Group's National Feature Catalogue as at 21 December 2023." ;
    skos:inScheme cs: ;
    skos:prefLabel "School Camp"@en ;
.

go:scrap-yard
    a skos:Concept ;
    rdfs:isDefinedBy cs: ;
    skos:altLabel
        "Junkyard"@en ,
        "Salvage Yard"@en ,
        "Wreckers"@en ,
        "Wrecking Yard"@en ;
    skos:definition "A site on which anything discarded as useless, unwanted or worn out may be dumped."@en ;
    skos:historyNote "Inherited from ICSM Place Names Working Group's National Feature Catalogue as at 21 December 2023." ;
    skos:inScheme cs: ;
    skos:prefLabel "Scrap Yard"@en ;
.

go:scrub
    a skos:Concept ;
    rdfs:isDefinedBy cs: ;
    skos:altLabel "Heath"@en ;
    skos:definition "A tract of country, not large in extent, which is uncultivated and which bears a dense growth of low-growing bushes or shrubs."@en ;
    skos:historyNote "Inherited from ICSM Place Names Working Group's National Feature Catalogue as at 21 December 2023." ;
    skos:inScheme cs: ;
    skos:prefLabel "Scrub"@en ;
.

go:sea
    a skos:Concept ;
    rdfs:isDefinedBy cs: ;
    skos:definition "One of the smaller divisions of the oceans, especially if partly enclosed by land."@en ;
    skos:historyNote "Inherited from ICSM Place Names Working Group's National Feature Catalogue as at 21 December 2023." ;
    skos:inScheme cs: ;
    skos:prefLabel "Sea"@en ;
.

go:sea-channel
    a skos:Concept ;
    rdfs:isDefinedBy cs: ;
    skos:altLabel "Channel"@en ;
    skos:definition "An elongated, meandering depression, usually occurring on a gently sloping plain or Fan."@en ;
    skos:historyNote "Inherited from ICSM Place Names Working Group's National Feature Catalogue as at 21 December 2023. Definition from General Bathymetric Chart of the Oceans (GEBCO) Sub-Committee on Undersea Features Names (SCUFN)." ;
    skos:inScheme cs: ;
    skos:prefLabel "Sea Channel"@en ;
	skos:scopeNote "Term 'Channel' now obsolete and recognised for historically named features only. " ;
    schema:citation "https://iho.int/en/basic-documents-1"^^xsd:anyURI ;
.

go:secondary-road
    a skos:Concept ;
    rdfs:isDefinedBy cs: ;
    skos:altLabel "Sub-Arterial Road"@en ;
    skos:definition "Well maintained and widely used roads which are major connectors for national highways or state highways, major centres, key towns, or have major tourist importance or which main function is to form the principal avenue of communication for metropolitan traffic movements. These are sometimes referred to as sub-arterial roads."@en ;
    skos:historyNote "Added by Queensland 2024-06-04 from Queensland Roads and Tracks dataset." ;
    skos:inScheme cs: ;
    skos:prefLabel "Secondary Road"@en ;
.

go:secondary-school
    a skos:Concept ;
    rdfs:isDefinedBy cs: ;
    skos:altLabel "High School"@en ;
    skos:definition "An education facility that caters for 12- 18 year olds, private and public."@en ;
    skos:historyNote "Inherited from ICSM Place Names Working Group's National Feature Catalogue as at 21 December 2023." ;
    skos:inScheme cs: ;
    skos:prefLabel "Secondary School"@en ;
.

go:ses-facility
    a skos:Concept ;
    rdfs:isDefinedBy cs: ;
    skos:altLabel "State Emergency Services Facility"@en ;
    skos:definition "State Emergency Services Facility."@en ;
    skos:historyNote "Inherited from ICSM Place Names Working Group's National Feature Catalogue as at 21 December 2023." ;
    skos:inScheme cs: ;
    skos:prefLabel "SES Facility"@en ;
.

go:settlement
    a skos:Concept ;
    rdfs:isDefinedBy cs: ;
    skos:definition "A small rural community, typically outside a larger urban area."@en ;
    skos:historyNote "Inherited from ICSM Place Names Working Group's National Feature Catalogue as at 21 December 2023." ;
    skos:inScheme cs: ;
    skos:prefLabel "Settlement"@en ;
.

go:sewage-treatment-plant
    a skos:Concept ;
    rdfs:isDefinedBy cs: ;
    skos:definition "A facility for the process of removing contaminants from wastewater."@en ;
    skos:historyNote "Inherited from ICSM Place Names Working Group's National Feature Catalogue as at 21 December 2023." ;
    skos:inScheme cs: ;
    skos:prefLabel "Sewage Treatment Plant"@en ;
.

go:sewer-pipeline
    a skos:Concept ;
    rdfs:isDefinedBy cs: ;
    skos:definition "A long pipe, typically underground used to transport sewage over long distances."@en ;
    skos:historyNote "Inherited from ICSM Place Names Working Group's National Feature Catalogue as at 21 December 2023." ;
    skos:inScheme cs: ;
    skos:prefLabel "Sewer Pipeline"@en ;
.

go:shared-use-track
    a skos:Concept ;
    rdfs:isDefinedBy cs: ;
    skos:definition "Shared track for vehicular and non-vehicular users."@en ;
    skos:historyNote "Added by Queensland 2024-06-04 from Queensland Roads and Tracks dataset." ;
    skos:inScheme cs: ;
    skos:prefLabel "Shared use track"@en ;
.

go:ship-wreck
    a skos:Concept ;
    rdfs:isDefinedBy cs: ;
    skos:altLabel "Wreck"@en ;
    skos:definition "The ruined remains of a stranded or sunken vessel which has been rendered useless."@en ;
    skos:historyNote "Inherited from ICSM Place Names Working Group's National Feature Catalogue as at 21 December 2023." ;
    skos:inScheme cs: ;
    skos:prefLabel "Ship Wreck"@en ;
.

go:shopping-centre
    a skos:Concept ;
    rdfs:isDefinedBy cs: ;
    skos:altLabel
        "Arcade"@en ,
        "Plaza"@en ,
        "Shopping Mall"@en ,
        "Shopping Precinct"@en ;
    skos:definition "Typically a named area/property or group of retail businesses with their own infrastructure such as carparks."@en ;
    skos:historyNote "Inherited from ICSM Place Names Working Group's National Feature Catalogue as at 21 December 2023." ;
    skos:inScheme cs: ;
    skos:prefLabel "Shopping Centre"@en ;
.

go:showground
    a skos:Concept ;
    rdfs:isDefinedBy cs: ;
    skos:definition "A tract of land with pavilion(s) and arena(s) for exhibition and display of livestock and produce"@en ;
    skos:historyNote "Inherited from ICSM Place Names Working Group's National Feature Catalogue as at 21 December 2023." ;
    skos:inScheme cs: ;
    skos:prefLabel "Showground"@en ;
.

go:shrine
    a skos:Concept ;
    rdfs:isDefinedBy cs: ;
    skos:definition "A place or object hallowed by its history or associations."@en ;
    skos:historyNote "Created by separating 'Monument' alternate labels 2024-03-05. Definition from Macquarie Dictionary." ;
    skos:inScheme cs: ;
    skos:prefLabel "Shrine"@en ;
.

go:siding
    a skos:Concept ;
    rdfs:isDefinedBy cs: ;
    skos:altLabel
        "Rail Siding"@en ,
        "Railway Siding"@en ;
    skos:definition "A short branch off a RAILWAY track, often connected at both ends to the mainline track, and used for shunting or for loading, unloading, and storing goods trucks."@en ;
    skos:historyNote "Inherited from ICSM Place Names Working Group's National Feature Catalogue as at 21 December 2023." ;
    skos:inScheme cs: ;
    skos:prefLabel "Siding"@en ;
.

go:sinkhole
    a skos:Concept ;
    rdfs:isDefinedBy cs: ;
    skos:altLabel
        "Pothole"@en ,
        "Sink Hole"@en ,
        "Swallow-hole"@en ;
    skos:definition "A hole formed in soluble rock by the action of water, serving to conduct surface water to an underground passage."@en ;
    skos:historyNote "Created by separating 'Rockhole' alternate labels 2024-06-10. Definition from Macquarie Dictionary." ;
    skos:inScheme cs: ;
    skos:prefLabel "Sinkhole"@en ;
.

go:skate-park
    a skos:Concept ;
    rdfs:isDefinedBy cs: ;
    skos:altLabel "Skateboard Park"@en ;
    skos:definition "A place where the primary activity is skating or skateboarding."@en ;
    skos:historyNote "Inherited from ICSM Place Names Working Group's National Feature Catalogue as at 21 December 2023." ;
    skos:inScheme cs: ;
    skos:prefLabel "Skate Park"@en ;
.

go:skerry
    a skos:Concept ;
    rdfs:isDefinedBy cs: ;
    skos:definition "A rugged stretch of sea-rock, covered by the sea at high tide or in stormy weather; reef."@en ;
    skos:historyNote "Created by separating 'Island' alternate labels 2024-03-05. Definition from Macquarie Dictionary." ;
    skos:inScheme cs: ;
    skos:prefLabel "Skerry"@en ;
.

go:ski-trail
    a skos:Concept ;
    rdfs:isDefinedBy cs: ;
    skos:definition "A trail designed for downhill or cross country in the main."@en ;
    skos:historyNote "Inherited from ICSM Place Names Working Group's National Feature Catalogue as at 21 December 2023." ;
    skos:inScheme cs: ;
    skos:prefLabel "Ski Trail"@en ;
.

go:slip-road
    a skos:Concept ;
    rdfs:isDefinedBy cs: ;
    skos:altLabel "Slip Lane"@en ;
    skos:definition "Slip road or slip lane. A short road that allows vehicles to join or leave a main road with a more gradual merge, reducing the potential for disruption in the traffic flow. Slip roads can be found at intersections, roundabouts, and dual carriageways, and they facilitate changes between roads at different speeds or directions."@en ;
    skos:historyNote "Added by Queensland 2024-06-04 from Queensland Roads and Tracks dataset." ;
    skos:inScheme cs: ;
    skos:prefLabel "Slip Road"@en ;
.

go:slope
    a skos:Concept ;
    rdfs:isDefinedBy cs: ;
    skos:definition "A gradient on the side or end of an elevated relief feature."@en ;
    skos:historyNote "Inherited from ICSM Place Names Working Group's National Feature Catalogue as at 21 December 2023." ;
    skos:inScheme cs: ;
    skos:narrower
        go:hillside ,
        go:marine-slope ;
    skos:prefLabel "Slope"@en ;
.

go:smelter
    a skos:Concept ;
    rdfs:isDefinedBy cs: ;
    skos:altLabel "Foundry"@en ;
    skos:definition "An industrial plant for smelting."@en ;
    skos:historyNote "Inherited from ICSM Place Names Working Group's National Feature Catalogue as at 21 December 2023." ;
    skos:inScheme cs: ;
    skos:prefLabel "Smelter"@en ;
.

go:soak
    a skos:Concept ;
    rdfs:isDefinedBy cs: ;
    skos:definition "A hollow, often in sandy soil and around the base of granite rocks, where water collects, on or below the surface of the ground."@en ;
    skos:historyNote "Inherited from ICSM Place Names Working Group's National Feature Catalogue as at 21 December 2023." ;
    skos:inScheme cs: ;
    skos:prefLabel "Soak"@en ;
.

go:solar-power-station
    a skos:Concept ;
    rdfs:isDefinedBy cs: ;
    skos:altLabel "Solar Farm"@en ;
    skos:definition "A process plant that creates power from the sun."@en ;
    skos:historyNote "Created by separating 'Power Station' alternate labels 2024-03-05." ;
    skos:inScheme cs: ;
    skos:prefLabel "Solar Power Station"@en ;
.

go:sound
    a skos:Concept ;
    rdfs:isDefinedBy cs: ;
    skos:definition "A relatively long arm of a sea or ocean forming a channel between an island and the mainland or connecting two larger bodies, as, a sea and the ocean, or two parts of the same body; usually wider and more extensive than a strait."@en ;
    skos:historyNote "Inherited from ICSM Place Names Working Group's National Feature Catalogue as at 21 December 2023." ;
    skos:inScheme cs: ;
    skos:prefLabel "Sound"@en ;
.

go:special-school
    a skos:Concept ;
    rdfs:isDefinedBy cs: ;
    skos:altLabel
        "SSP"@en ,
        "Schools For Specific Purposes"@en ,
        "Special Education School"@en ,
        "Special Needs School"@en ,
        "Specialist School"@en ;
    skos:definition "An educational facility that caters for those with learning disabilities."@en ;
    skos:historyNote "Inherited from ICSM Place Names Working Group's National Feature Catalogue as at 21 December 2023." ;
    skos:inScheme cs: ;
    skos:prefLabel "Special School"@en ;
.

go:specialised-hospital
    a skos:Concept ;
    rdfs:isDefinedBy cs: ;
    skos:definition "A hospital specifically for the care of a specific group or part of the body."@en ;
    skos:historyNote "Inherited from ICSM Place Names Working Group's National Feature Catalogue as at 21 December 2023." ;
    skos:inScheme cs: ;
    skos:narrower
        go:childrens-hospital ,
        go:dental-hospital ,
        go:eye-and-ear-hospital ,
        go:womens-hospital ;
    skos:prefLabel "Specialised Hospital"@en ;
.

go:spillway
    a skos:Concept ;
    rdfs:isDefinedBy cs: ;
    skos:definition "A passageway through which surplus water escapes from a reservoir."@en ;
    skos:historyNote "Concept created by separating 'Weir' alternate labels 2024-06-10. Definition added from Macquarie Dictionary." ;
    skos:inScheme cs: ;
    skos:prefLabel "Spillway"@en ;
.

go:spit
    a skos:Concept ;
    rdfs:isDefinedBy cs: ;
    skos:definition "A narrow strip of land projecting into a body of water from the coast."@en ;
    skos:historyNote "Inherited from ICSM Place Names Working Group's National Feature Catalogue as at 21 December 2023." ;
    skos:inScheme cs: ;
    skos:narrower go:sandspit ;
    skos:prefLabel "Spit"@en ;
.

go:sports-complex
    a skos:Concept ;
    rdfs:isDefinedBy cs: ;
    skos:altLabel
        "Sporting Complex"@en ,
        "Sports Precinct"@en ;
    skos:definition "Area containing multiple recreation facilities."@en ;
    skos:historyNote "Inherited from ICSM Place Names Working Group's National Feature Catalogue as at 21 December 2023." ;
    skos:inScheme cs: ;
    skos:prefLabel "Sports Complex"@en ;
.

go:sports-court
    a skos:Concept ;
    rdfs:isDefinedBy cs: ;
    skos:definition "An area marked on the ground that is used for playing sport such as tennis or netball."@en ;
    skos:historyNote "Broader concept introduced 2024-06-04." ;
    skos:inScheme cs: ;
    skos:narrower
        go:basketball-court ,
        go:netball-court ,
        go:tennis-court ;
    skos:prefLabel "Sports Court"@en ;
.

go:sports-facility
    a skos:Concept ;
    rdfs:isDefinedBy cs: ;
    skos:altLabel "Sports Centre"@en ;
    skos:definition "A place, amenity, or piece of equipment related to sport provided for a particular purpose. This can range from single-use facilities, such as a gymnasium, swimming pool, or a single football pitch, to multi-purpose sports centres that might house several different activities under one roof or in one area but on a smaller scale than a sports complex."@en ;
    skos:historyNote "Inherited from ICSM Place Names Working Group's National Feature Catalogue as at 21 December 2023. Definition updated 2024-06-10." ;
    skos:inScheme cs: ;
    skos:narrower
        go:arena ,
        go:fitness-centre ,
        go:sports-court ,
        go:sports-field ,
        go:sports-stadium ,
        go:swimming-pool ,
        go:velodrome ;
    skos:prefLabel "Sports Facility"@en ;
.

go:sports-field
    a skos:Concept ;
    rdfs:isDefinedBy cs: ;
    skos:altLabel
        "Oval"@en ,
        "Playing Field"@en ,
        "Sports Ground"@en ,
        "Sportsground"@en ;
    skos:definition "A reserve used for sporting fixtures. A field on which sporting activities are carried out."@en ;
    skos:historyNote "Inherited from ICSM Place Names Working Group's National Feature Catalogue as at 21 December 2023. Definition amended 2024-06-10." ;
    skos:inScheme cs: ;
    skos:narrower
        go:athletic-field ,
        go:baseball-field ,
        go:cricket-field ,
        go:football-field ,
        go:hockey-field ;
    skos:prefLabel "Sports Field"@en ;
.

go:sports-pavilion
    a skos:Concept ;
    rdfs:isDefinedBy cs: ;
    skos:definition "A building at a sports ground that provides facilities for players and sometimes spectators. These facilities can include changing rooms, showers, restrooms, and sometimes a social area or clubhouse where players might meet for functions or refreshments. Pavilions may have space for meetings, trophy displays, or social events related to the sport. They are often situated near the playing area but are not primarily designed for watching the sport itself."@en ;
    skos:historyNote "Created by separating 'Sports Facility' alternate labels 2024-05-10." ;
    skos:inScheme cs: ;
    skos:prefLabel "Sports Pavilion"@en ;
.

go:sports-stadium
    a skos:Concept ;
    rdfs:isDefinedBy cs: ;
    skos:definition "A sporting facility, often enclosed, comprising an arena, tiers or seats for spectators, parking, etc."@en ;
    skos:historyNote "Created by separating 'Sports Facility' alternate labels 2024-05-10. Definition from Macquarie Dictionary." ;
    skos:inScheme cs: ;
    skos:prefLabel "Sports Stadium"@en ;
.

go:spring
    a skos:Concept ;
    rdfs:isDefinedBy cs: ;
    skos:altLabel
        "Mineral Spring"@en ,
        "Pool Spring"@en ;
    skos:definition "A flow of water issuing naturally out of the ground, either continuously or intermittently."@en ;
    skos:historyNote "Inherited from ICSM Place Names Working Group's National Feature Catalogue as at 21 December 2023." ;
    skos:inScheme cs: ;
    skos:narrower go:hot-spring ;
    skos:prefLabel "Spring"@en ;
.

go:stack
    a skos:Concept ;
    rdfs:isDefinedBy cs: ;
    skos:definition "A column or pillar of rock, isolated from the shore by the erosive action of waves."@en ;
    skos:historyNote "Created by separating 'Rock' alternate labels 2024-06-10. Definition from Macquarie Dictionary." ;
    skos:inScheme cs: ;
    skos:prefLabel "Stack"@en ;
.

go:state
    a skos:Concept ;
    rdfs:isDefinedBy cs: ;
    skos:definition "One of the six constituent political entities that together, along with other territories, form the federation known as the Commonwealth of Australia."@en ;
    skos:historyNote "Inherited from ICSM Place Names Working Group's National Feature Catalogue as at 21 December 2023." ;
    skos:inScheme cs: ;
    skos:prefLabel "State"@en ;
.

go:state-border-section
    a skos:Concept ;
    rdfs:isDefinedBy cs: ;
    skos:definition "A named line that makes up part of the border of a state or territory."@en ;
    skos:historyNote "Inherited from ICSM Place Names Working Group's National Feature Catalogue as at 21 December 2023. Refined label from original 'state border' feature type." ;
    skos:inScheme cs: ;
    skos:prefLabel "State Border Section"@en ;
.

go:state-electorate
    a skos:Concept ;
    rdfs:isDefinedBy cs: ;
    skos:definition "An administrative division of a State or Territory represented by a member of Parliament elected at a House of Representatives election."@en ;
    skos:historyNote "Inherited from ICSM Place Names Working Group's National Feature Catalogue as at 21 December 2023." ;
    skos:inScheme cs: ;
    skos:prefLabel "State Electorate"@en ;
.

go:state-forest
    a skos:Concept ;
    rdfs:isDefinedBy cs: ;
    skos:altLabel
        "Forest Reserve"@en ,
        "Timber Reserve"@en ;
    skos:definition "An area of protected forest under a Forest Act."@en ;
    skos:historyNote "Inherited from ICSM Place Names Working Group's National Feature Catalogue as at 21 December 2023." ;
    skos:inScheme cs: ;
    skos:prefLabel "State Forest"@en ;
.

go:state-territory
    a skos:Concept ;
    rdfs:isDefinedBy cs: ;
    skos:definition "Any of the sixteen major divisions which contribute to the federated Commonwealth of Australia."@en ;
    skos:historyNote "Inherited from ICSM Place Names Working Group's National Feature Catalogue as at 21 December 2023." ;
    skos:inScheme cs: ;
    skos:narrower
        go:state ,
        go:territory ;
    skos:prefLabel "State Or Territory"@en ;
.

go:steel-works
    a skos:Concept ;
    rdfs:isDefinedBy cs: ;
    skos:definition "A factory where steel is made and formed into girders, rails and other goods."@en ;
    skos:historyNote "Inherited from ICSM Place Names Working Group's National Feature Catalogue as at 21 December 2023." ;
    skos:inScheme cs: ;
    skos:prefLabel "Steel Works"@en ;
.

go:stock-route
    a skos:Concept ;
    rdfs:isDefinedBy cs: ;
    skos:definition "A route designated for droving stock, with the intent of avoiding vehicular traffic."@en ;
    skos:historyNote "Inherited from ICSM Place Names Working Group's National Feature Catalogue as at 21 December 2023." ;
    skos:inScheme cs: ;
    skos:prefLabel "Stock Route"@en ;
.

go:stockyard
    a skos:Concept ;
    rdfs:isDefinedBy cs: ;
    skos:altLabel
        "Yard"@en ,
        "Yards"@en ;
    skos:definition "An enclosure forming a pen for livestock."@en ;
    skos:historyNote "Inherited from ICSM Place Names Working Group's National Feature Catalogue as at 21 December 2023." ;
    skos:inScheme cs: ;
    skos:prefLabel "Stockyard"@en ;
.

go:subglacial-feature
    a skos:Concept ;
    rdfs:isDefinedBy cs: ;
    skos:altLabel "Under Ice Feature"@en ;
    skos:definition "Natural features of the Earth's surface under ice."@en ;
    skos:historyNote "Inherited from ICSM Place Names Working Group's National Feature Catalogue as at 21 December 2023, with name label amended 2024-05-04 from 'Under Ice'." ;
    skos:inScheme cs: ;
    skos:narrower
        go:subglacial-basin ,
        go:subglacial-mount ,
        go:subglacial-trench ;
    skos:prefLabel "Subglacial Feature"@en ;
.

go:sugar-refinery
    a skos:Concept ;
    rdfs:isDefinedBy cs: ;
    skos:definition "A refinery to convert sugar cane and sugar beets into crystallized sugar and sugar syrups."@en ;
    skos:historyNote "Inherited from ICSM Place Names Working Group's National Feature Catalogue as at 21 December 2023." ;
    skos:inScheme cs: ;
    skos:prefLabel "Sugar Refinery"@en ;
.

go:sugarloaf
    a skos:Concept ;
    rdfs:isDefinedBy cs: ;
    skos:definition "A small conical hill resembling the shape of a large approximately conical loaf or mass of hard refined sugar."@en ;
    skos:historyNote "Created by separating 'Hill' alternate labels 2024-05-10. Definition adapted from Macquarie Dictionary." ;
    skos:inScheme cs: ;
    skos:prefLabel "Sugarloaf"@en ;
.

go:surfing-spot
    a skos:Concept ;
    rdfs:isDefinedBy cs: ;
    skos:altLabel "Surf Break"@en ;
    skos:definition "A place where waves break on the shore or reef identified as suitable for surfing."@en ;
    skos:historyNote "Inherited from ICSM Place Names Working Group's National Feature Catalogue as at 21 December 2023." ;
    skos:inScheme cs: ;
    skos:prefLabel "Surfing Spot"@en ;
.

go:survey-marker
    a skos:Concept ;
    rdfs:isDefinedBy cs: ;
    skos:altLabel
        "Horizontal Control Point"@en ,
        "Permanent Survey Mark"@en ,
        "Survey Cairn"@en ,
        "Survey Monument"@en ,
        "Survey Obelisk"@en ,
        "Survey Pillar"@en ,
        "Triangulation Station"@en ,
        "Trig Point"@en ,
        "Trigonometric Point"@en ,
        "Trigonometric Station"@en ;
    skos:definition "A control mark used in surveys."@en ;
    skos:historyNote "Inherited from ICSM Place Names Working Group's National Feature Catalogue as at 21 December 2023." ;
    skos:inScheme cs: ;
    skos:prefLabel "Survey Marker"@en ;
.

go:swimming-enclosure
    a skos:Concept ;
    rdfs:isDefinedBy cs: ;
    skos:definition "A barrier designed as a safety precaution to provide protection from marine predators and stingers."@en ;
    skos:historyNote "Added by Queensland 2024-06-05." ;
    skos:inScheme cs: ;
    skos:prefLabel "Swimming Enclosure"@en ;
.

go:swimming-pool
    a skos:Concept ;
    rdfs:isDefinedBy cs: ;
    skos:altLabel
        "Aquatic Centre"@en ,
        "Baths"@en ;
    skos:definition "An artificial pool for swimming."@en ;
    skos:historyNote "Inherited from ICSM Place Names Working Group's National Feature Catalogue as at 21 December 2023." ;
    skos:inScheme cs: ;
    skos:narrower go:swimming-enclosure ;
    skos:prefLabel "Swimming Pool"@en ;
.

go:synagogue
    a skos:Concept ;
    rdfs:isDefinedBy cs: ;
    skos:definition "Jewish house of worship, usually also providing religious instruction."@en ;
    skos:historyNote "Inherited from ICSM Place Names Working Group's National Feature Catalogue as at 21 December 2023. Definition from Macquarie Dictionary." ;
    skos:inScheme cs: ;
    skos:prefLabel "Synagogue"@en ;
.

go:tafe-facility
    a skos:Concept ;
    rdfs:isDefinedBy cs: ;
    skos:altLabel
        "Institute Of Technology"@en ,
        "TAFE"@en ;
    skos:definition "Post secondary (TAFE) education."@en ;
    skos:historyNote "Inherited from ICSM Place Names Working Group's National Feature Catalogue as at 21 December 2023, with name label amended 2024-05-04 from 'Tertiary Institution' 2024-03-05." ;
    skos:inScheme cs: ;
    skos:prefLabel "Technical and Further Education Facility"@en ;
.

go:tannery
    a skos:Concept ;
    rdfs:isDefinedBy cs: ;
    skos:definition "A building where animal hides and skins are processed into leather."@en ;
    skos:historyNote "Inherited from ICSM Place Names Working Group's National Feature Catalogue as at 21 December 2023." ;
    skos:inScheme cs: ;
    skos:prefLabel "Tannery"@en ;
.

go:taxi-rank
    a skos:Concept ;
    rdfs:isDefinedBy cs: ;
    skos:definition "A designated place where taxis stop for passengers to board or alight."@en ;
    skos:historyNote "Inherited from ICSM Place Names Working Group's National Feature Catalogue as at 21 December 2023." ;
    skos:inScheme cs: ;
    skos:prefLabel "Taxi Rank"@en ;
.

go:telephone-exchange
    a skos:Concept ;
    rdfs:isDefinedBy cs: ;
    skos:altLabel
        "Telegraph Office"@en ,
        "Telephone Office"@en ;
    skos:definition "A facility to establish telecommunication connections."@en ;
    skos:historyNote "Inherited from ICSM Place Names Working Group's National Feature Catalogue as at 21 December 2023." ;
    skos:inScheme cs: ;
    skos:prefLabel "Telephone Exchange"@en ;
.

go:television-communication-facility
    a skos:Concept ;
    rdfs:isDefinedBy cs: ;
    skos:altLabel "Television Broadcasting Facility"@en ;
    skos:definition "A complex or site that is involved in the transmission, relaying, and broadcasting of television signals. These facilities can include a range of infrastructure and equipment necessary for the delivery of television programming."@en ;
    skos:historyNote "Inherited from ICSM Place Names Working Group's National Feature Catalogue as at 21 December 2023. Definition updated 2024-06-10." ;
    skos:inScheme cs: ;
    skos:prefLabel "Television Communication Facility"@en ;
.

go:television-station
    a skos:Concept ;
    rdfs:isDefinedBy cs: ;
    skos:definition "A facility to operate the transmission of television broadcasts."@en ;
    skos:historyNote "Inherited from ICSM Place Names Working Group's National Feature Catalogue as at 21 December 2023." ;
    skos:inScheme cs: ;
    skos:prefLabel "Television Station"@en ;
.

go:television-tower
    a skos:Concept ;
    rdfs:isDefinedBy cs: ;
    skos:definition "A structure built to support antennas for transmitting television signals. They are usually tall so that the signals can cover a large area without obstruction."@en ;
    skos:historyNote "Created by separating 'Communication Tower' alternate labels 2024-06-10." ;
    skos:inScheme cs: ;
    skos:prefLabel "Television Tower"@en ;
.

go:tennis-court
    a skos:Concept ;
    rdfs:isDefinedBy cs: ;
    skos:definition "A place where tennis is played."@en ;
    skos:historyNote "Inherited from ICSM Place Names Working Group's National Feature Catalogue as at 21 December 2023." ;
    skos:inScheme cs: ;
    skos:prefLabel "Tennis Court"@en ;
.

go:terrain-feature
    a skos:Concept ;
    rdfs:isDefinedBy cs: ;
    skos:definition "Places that reflect the physical attributes of the land surface."@en ;
    skos:historyNote "Inherited from ICSM Place Names Working Group's National Feature Catalogue as at 21 December 2023, with name label amended 2024-05-04 from 'Terrain' 2024-03-05." ;
    skos:inScheme cs: ;
    skos:narrower
        go:landform ,
        go:subglacial-feature ,
        go:undersea-feature ;
    skos:prefLabel "Terrain Feature"@en ;
    skos:topConceptOf cs: ;
.

go:territory
    a skos:Concept ;
    rdfs:isDefinedBy cs: ;
    skos:definition "A geographic region in the Commonwealth of Australia under the jurisdiction of the Federal Government of Australia, that is not part of a State."@en ;
    skos:historyNote "Inherited from ICSM Place Names Working Group's National Feature Catalogue as at 21 December 2023." ;
    skos:inScheme cs: ;
    skos:prefLabel "Territory"@en ;
.

go:theme-park
    a skos:Concept ;
    rdfs:isDefinedBy cs: ;
    skos:definition "A type of amusement park with a central theme and unifying ideas."@en ;
    skos:historyNote "Inherited from ICSM Place Names Working Group's National Feature Catalogue as at 21 December 2023." ;
    skos:inScheme cs: ;
    skos:prefLabel "Theme Park"@en ;
.

go:thicket
    a skos:Concept ;
    rdfs:isDefinedBy cs: ;
    skos:altLabel "Brushwood"@en ;
    skos:definition "A thick or dense growth of shrubs, bushes, or small trees."@en ;
    skos:historyNote "Concept created by separating 'Forest' alternate labels 2024-06-11. Definition from Macquarie Dictionary." ;
    skos:inScheme cs: ;
    skos:prefLabel "Thicket"@en ;
.

go:tidal-flat
    a skos:Concept ;
    rdfs:isDefinedBy cs: ;
    skos:definition "A large area of nearly level land, usually of mud, covered at high water and attached to the shore."@en ;
    skos:historyNote "Inherited from ICSM Place Names Working Group's National Feature Catalogue as at 21 December 2023." ;
    skos:inScheme cs: ;
    skos:prefLabel "Tidal Flat"@en ;
.

go:timber-operations
    a skos:Concept ;
    rdfs:isDefinedBy cs: ;
    skos:altLabel
        "Mill"@en ,
        "Mill Operations"@en ,
        "Paper Mill"@en ,
        "Sawmill"@en ;
    skos:definition "A place where trees are milled to create timber and or paper."@en ;
    skos:historyNote "Inherited from ICSM Place Names Working Group's National Feature Catalogue as at 21 December 2023." ;
    skos:inScheme cs: ;
    skos:prefLabel "Timber Operations"@en ;
.

go:toll
    a skos:Concept ;
    rdfs:isDefinedBy cs: ;
    skos:altLabel
        "Toll Road"@en ,
        "Tollway"@en ,
        "Turnpike"@en ;
    skos:definition "A structure used to regulate movement associated with road or rail."@en ;
    skos:historyNote "Inherited from ICSM Place Names Working Group's National Feature Catalogue as at 21 December 2023." ;
    skos:inScheme cs: ;
    skos:prefLabel "Toll"@en ;
.

go:tor
    a skos:Concept ;
    rdfs:isDefinedBy cs: ;
    skos:definition "A rocky eminence, typically consisting of a pile or stack of weathered rock, formed through the gradual weathering and erosion of jointed bedrock.."@en ;
    skos:historyNote "Created by separating 'Hill' alternate labels 2024-05-10. Definition adapted from Macquarie Dictionary." ;
    skos:inScheme cs: ;
    skos:prefLabel "Tor"@en ;
.

go:tourist-attraction
    a skos:Concept ;
    rdfs:isDefinedBy cs: ;
    skos:definition "A place or facility which attracts people to visit."@en ;
    skos:historyNote "Inherited from ICSM Place Names Working Group's National Feature Catalogue as at 21 December 2023." ;
    skos:inScheme cs: ;
    skos:narrower
        go:amusement-centre ,
        go:aquarium ,
        go:art-gallery ,
        go:museum ,
        go:theme-park ,
        go:winery ,
        go:zoo ;
    skos:prefLabel "Tourist Attraction"@en ;
.

go:tourist-region
    a skos:Concept ;
    rdfs:isDefinedBy cs: ;
    skos:definition "A relatively large area, usually within the bounds of a State or Territory, which is distinguished by certain common characteristics, natural or cultural, and recognised as such for various tourist administrative or cultural purposes."@en ;
    skos:historyNote "Inherited from ICSM Place Names Working Group's National Feature Catalogue as at 21 December 2023." ;
    skos:inScheme cs: ;
    skos:prefLabel "Tourist Region"@en ;
.

go:tourist-route
    a skos:Concept ;
    rdfs:isDefinedBy cs: ;
    skos:altLabel
        "Tourist Drive"@en ,
        "Tourist Way"@en ;
    skos:definition "A route specifically identified for tourists through an area of natural or cultural beauty and/or interest."@en ;
    skos:historyNote "Inherited from ICSM Place Names Working Group's National Feature Catalogue as at 21 December 2023." ;
    skos:inScheme cs: ;
    skos:prefLabel "Tourist Route"@en ;
.

go:town-hall
    a skos:Concept ;
    rdfs:isDefinedBy cs: ;
    skos:definition "A hall or building belonging to a town, used for the transaction of the town’s business, etc., and often also as a place of public assembly"@en ;
    skos:historyNote "Inherited from ICSM Place Names Working Group's National Feature Catalogue as at 21 December 2023. Definition from Macquarie Dictionary." ;
    skos:inScheme cs: ;
    skos:prefLabel "Town Hall"@en ;
.

go:town-site
    a skos:Concept ;
    rdfs:isDefinedBy cs: ;
    skos:definition "An original crown subdivision of land within a Parish or Hundred which has officially recognised and gazetted boundaries."@en ;
    skos:historyNote "Inherited from ICSM Place Names Working Group's National Feature Catalogue as at 21 December 2023." ;
    skos:inScheme cs: ;
    skos:prefLabel "Town Site"@en ;
.

go:track
    a skos:Concept ;
    rdfs:isDefinedBy cs: ;
    skos:definition "A natural or minimally developed path or roadway designed for travel by foot, bicycle, horse or vehicles."@en ;
    skos:historyNote "Broader concept introduced 2024-03-05." ;
    skos:inScheme cs: ;
    skos:narrower
        go:firebreak ,
        go:non-vehicular-track ,
        go:shared-use-track ,
        go:vehicular-track ;
    skos:prefLabel "Track"@en ;
.

go:tram-transport-infrastructure
    a skos:Concept ;
    rdfs:isDefinedBy cs: ;
    skos:definition "Installations, systems, and structures that enable the operation of trams and serve as the foundation for tram transportation."@en ;
    skos:historyNote "Broader concept introduced 2024-03-05." ;
    skos:inScheme cs: ;
    skos:narrower
        go:tram-station ,
        go:tram-tunnel ,
        go:tramway ;
    skos:prefLabel "Tram Transport Infrastructure"@en ;
.

go:tramway
    a skos:Concept ;
    rdfs:isDefinedBy cs: ;
    skos:altLabel "Tram Line"@en ;
    skos:definition "A system of grooved tracks laid in urban streets, forming routes for the conveyance of passengers in trams."@en ;
    skos:historyNote "Created by separating 'Light Rail' alternate labels 2024-06-10. Definition adapted from Macquarie Dictionary." ;
    skos:inScheme cs: ;
    skos:prefLabel "Tramway"@en ;
.

go:transport-infrastructure
    a skos:Concept ;
    rdfs:isDefinedBy cs: ;
    skos:definition "Places associated with the movement of people, goods, freight and cargo."@en ;
    skos:historyNote "Inherited from ICSM Place Names Working Group's National Feature Catalogue as at 21 December 2023. with name label amended 2024-05-04 from 'Transport'." ;
    skos:inScheme cs: ;
    skos:narrower
        go:air-transport-infrastructure ,
        go:bridge ,
        go:cableway-transport-infrastructure ,
        go:control-tower ,
        go:path ,
        go:rail-transport-infrastructure ,
        go:road-transport-infrastructure ,
        go:track ,
        go:transport-terminal ,
        go:tunnel ,
        go:water-transport-infrastructure ;
    skos:prefLabel "Transport Infrastructure"@en ;
    skos:topConceptOf cs: ;
.

go:transport-terminal
    a skos:Concept ;
    rdfs:isDefinedBy cs: ;
    skos:altLabel "Transport Station"@en ;
    skos:definition "A structure beside transportation infrastructure with facilities for passengers to board or alight."@en ;
    skos:historyNote "Broader concept introduced 2024-03-05." ;
    skos:inScheme cs: ;
    skos:narrower
        go:bus-station ,
        go:cableway-terminal ,
        go:ferry-station ,
        go:light-rail-station ,
        go:rail-station ,
        go:tram-station ;
    skos:prefLabel "Transport Terminal"@en ;
.

go:trench
    a skos:Concept ;
    rdfs:isDefinedBy cs: ;
    skos:definition "A deep, or elongated trough, in a floor of the ocean."@en ;
    skos:historyNote "Added by Queensland 2024-03-05. Definition from part of 'Subglacial Trench'." ;
    skos:inScheme cs: ;
    skos:narrower
        go:marine-trench ,
        go:subglacial-trench ;
    skos:prefLabel "Trench"@en ;
.

go:tunnel
    a skos:Concept ;
    rdfs:isDefinedBy cs: ;
    skos:definition "A long, enclosed passageway that goes through a barrier or obstacle such as a mountain, hill, or beneath a body of water, allowing transportation routes to pass beneath an obstruction."@en ;
    skos:historyNote "Broader concept introduced 2024-03-05." ;
    skos:inScheme cs: ;
    skos:narrower
        go:foot-tunnel ,
        go:light-rail-tunnel ,
        go:rail-tunnel ,
        go:road-tunnel ,
        go:tram-tunnel ;
    skos:prefLabel "Tunnel"@en ;
.

go:u-turn
    a skos:Concept ;
    rdfs:isDefinedBy cs: ;
    skos:definition "Lane or bay to enable a turn executed by the driver of a motor vehicle in which the vehicle is turned sharply to face the direction from which it was coming."@en ;
    skos:historyNote "Added by Queensland 2024-06-04 from Queensland Roads and Tracks dataset. Definition from Macquarie Dictionary." ;
    skos:inScheme cs: ;
    skos:prefLabel "U turn"@en ;
.

go:unclassified
    a skos:Concept ;
    rdfs:isDefinedBy cs: ;
    skos:definition "Geographic feature type not yet determined."@en ;
    skos:historyNote "Inherited from ICSM Place Names Working Group's National Feature Catalogue as at 21 December 2023." ;
    skos:inScheme cs: ;
    skos:prefLabel "Unclassified"@en ;
    skos:topConceptOf cs: ;
.

go:unconstructed-road
    a skos:Concept ;
    rdfs:isDefinedBy cs: ;
    skos:altLabel "Paper Road"@en ;
    skos:definition "A road designation has been made in the spatial cadastre or in Government plans, but road currently does not physically exist. Sometimes referred to as a paper road."@en ;
    skos:historyNote "Added by Queensland 2024-06-04 from Queensland Roads and Tracks dataset." ;
    skos:inScheme cs: ;
    skos:prefLabel "Unconstructed Road"@en ;
.

go:underground-mine
    a skos:Concept ;
    rdfs:isDefinedBy cs: ;
    skos:altLabel
        "Mineshaft"@en ,
        "Shaft"@en ,
        "Sub-Surface Mine"@en ;
    skos:definition "A place or area from which commercial minerals are removed from the Earth."@en ;
    skos:historyNote "Inherited from ICSM Place Names Working Group's National Feature Catalogue as at 21 December 2023." ;
    skos:inScheme cs: ;
    skos:prefLabel "Underground Mine"@en ;
.

go:underpass
    a skos:Concept ;
    rdfs:isDefinedBy cs: ;
    skos:definition "A shorter structure that allows a road, path, or railway to cross beneath another road, railway, or other types of barriers. It is generally less complex than a tunnel and is often found in urban settings facilitating the flow of traffic or pedestrians and preventing the need for an intersection."@en ;
    skos:historyNote "Added by Queensland 2024-06-04." ;
    skos:inScheme cs: ;
    skos:prefLabel "Underpass"@en ;
.

go:undersea-feature
    a skos:Concept ;
    rdfs:isDefinedBy cs: ;
    skos:definition "Natural features of the Earth's surface under water."@en ;
    skos:historyNote "Inherited from ICSM Place Names Working Group's National Feature Catalogue as at 21 December 2023, with name label amended 2024-05-04 from 'Undersea'." ;
    skos:inScheme cs: ;
    skos:narrower
        go:abyssal-plain ,
        go:deep ,
        go:guyot ,
        go:marine-apron ,
        go:marine-bank ,
        go:marine-basin ,
        go:marine-caldera ,
        go:marine-canyon ,
        go:marine-continental-margin ,
        go:marine-escarpment ,
        go:marine-fan ,
        go:marine-fracture-zone ,
        go:marine-gap ,
        go:marine-hill ,
        go:marine-hole ,
        go:marine-knoll ,
        go:marine-levee ,
        go:marine-moat ,
        go:marine-mound ,
        go:marine-mud-volcano ,
        go:marine-peak ,
        go:marine-pinnacle ,
        go:marine-plateau ,
        go:marine-province ,
        go:marine-reef ,
        go:marine-ridge ,
        go:marine-rift ,
        go:marine-rise ,
        go:marine-saddle ,
        go:marine-salt-dome ,
        go:marine-sand-ridge ,
        go:marine-shelf ,
        go:marine-shoal ,
        go:marine-sill ,
        go:marine-slope ,
        go:marine-spur ,
        go:marine-terrace ,
        go:marine-trench ,
        go:marine-trough ,
        go:marine-valley ,
        go:sea-channel ,
        go:seamount ,
        go:seamount-chain ,
        go:subglacial-basin ;
    skos:prefLabel "Undersea Feature"@en ;
.

go:university
    a skos:Concept ;
    rdfs:isDefinedBy cs: ;
    skos:definition "An educational institution for both instruction and examination in the higher branches of knowledge with the power to confer degrees."@en ;
    skos:historyNote "Inherited from ICSM Place Names Working Group's National Feature Catalogue as at 21 December 2023." ;
    skos:inScheme cs: ;
    skos:prefLabel "University"@en ;
.

go:utility-infrastructure
    a skos:Concept ;
    rdfs:isDefinedBy cs: ;
    skos:definition "Places relating to the provision of information and functional services in the community."@en ;
    skos:historyNote "Inherited from ICSM Place Names Working Group's National Feature Catalogue as at 21 December 2023, with name label amended from 'Utilities'." ;
    skos:inScheme cs: ;
    skos:narrower
        go:communication-infrastructure ,
        go:energy-infrastructure ,
        go:observatory ,
        go:waste-infrastructure ;
    skos:prefLabel "Utility Infrastructure"@en ;
    skos:topConceptOf cs: ;
.

go:valley
    a skos:Concept ;
    rdfs:isDefinedBy cs: ;
    skos:altLabel
        "Dale"@en ,
        "Dell"@en ,
        "Glen"@en ,
        "Vale"@en ;
    skos:definition "A long area of lower elevation within an area of elevated relief, bounded by hills or mountains, usually with a river flowing through it, and formed by erosion or by movements in the earth's crust."@en ;
    skos:historyNote "Inherited from ICSM Place Names Working Group's National Feature Catalogue as at 21 December 2023." ;
    skos:inScheme cs: ;
    skos:narrower go:marine-valley ;
    skos:prefLabel "Valley"@en ;
.

go:vegetation
    a skos:Concept ;
    rdfs:isDefinedBy cs: ;
    skos:definition "Places named as a result of the naturally occurring flora."@en ;
    skos:historyNote "Inherited from ICSM Place Names Working Group's National Feature Catalogue as at 21 December 2023." ;
    skos:inScheme cs: ;
    skos:narrower
        go:copse ,
        go:forest ,
        go:glade ,
        go:grassland ,
        go:grove ,
        go:scrub ,
        go:thicket ,
        go:wood ;
    skos:prefLabel "Vegetation"@en ;
    skos:topConceptOf cs: ;
.

go:vehicular-ferry-route
    a skos:Concept ;
    rdfs:isDefinedBy cs: ;
    skos:definition "Route for a ferry that a vehicle can be transported on."@en ;
    skos:historyNote "Added by Queensland 2024-06-04 from Queensland Roads and Tracks dataset." ;
    skos:inScheme cs: ;
    skos:prefLabel "Vehicular ferry route"@en ;
.

go:vehicular-track
    a skos:Concept ;
    rdfs:isDefinedBy cs: ;
    skos:definition "A natural or minimally developed path or roadway designed for use for vehicles. Usually requires a 4WD or high clearance vehicle."@en ;
    skos:historyNote "Added by Queensland 2024-06-04 from Queensland Roads and Tracks dataset." ;
    skos:inScheme cs: ;
    skos:prefLabel "Vehicular Track"@en ;
.

go:velodrome
    a skos:Concept ;
    rdfs:isDefinedBy cs: ;
    skos:definition "An arena with a suitably banked track for cycle races."@en ;
    skos:historyNote "Inherited from ICSM Place Names Working Group's National Feature Catalogue as at 21 December 2023." ;
    skos:inScheme cs: ;
    skos:prefLabel "Velodrome"@en ;
.

go:vihara
    a skos:Concept ;
    rdfs:isDefinedBy cs: ;
    skos:definition "Buddhist place of worship."@en ;
    skos:historyNote "Inherited from ICSM Place Names Working Group's National Feature Catalogue as at 21 December 2023." ;
    skos:inScheme cs: ;
    skos:prefLabel "Vihara"@en ;
.

go:vineyard
    a skos:Concept ;
    rdfs:isDefinedBy cs: ;
    skos:definition "A plantation of grapevines, for producing grapes for winemaking."@en ;
    skos:historyNote "Inherited from ICSM Place Names Working Group's National Feature Catalogue as at 21 December 2023." ;
    skos:inScheme cs: ;
    skos:narrower go:plantation ;
    skos:prefLabel "Vineyard"@en ;
.

go:volcanic-crater
    a skos:Concept ;
    rdfs:isDefinedBy cs: ;
    skos:definition "A funnel-shaped hollow at the top of the cone of a volcano."@en ;
    skos:historyNote "Inherited from ICSM Place Names Working Group's National Feature Catalogue as at 21 December 2023." ;
    skos:inScheme cs: ;
    skos:prefLabel "Volcanic Crater"@en ;
.

go:volcanic-plain
    a skos:Concept ;
    rdfs:isDefinedBy cs: ;
    skos:altLabel "Lava Plain"@en ;
    skos:definition "An expansive, flat or gently undulating landscape that forms as a result of widespread volcanic activity. Covered with volcanic materials like lava flows and ash deposits."@en ;
    skos:historyNote "Created by separating 'Plain' alternate labels 2024-06-10." ;
    skos:inScheme cs: ;
    skos:prefLabel "Volcanic Plain"@en ;
.

go:walking-trail
    a skos:Concept ;
    rdfs:isDefinedBy cs: ;
    skos:altLabel
        "Hiking Trail"@en ,
        "Walking Track"@en ;
    skos:definition "A non-vehicular trail designed for foot traffic in the main. This is not a shared roadway with vehicular traffic. Main use is walking."@en ;
    skos:historyNote "Inherited from ICSM Place Names Working Group's National Feature Catalogue as at 21 December 2023, with name label amended 2024-05-04 from 'Walking Track' and 'non vehicular' appended to description." ;
    skos:inScheme cs: ;
    skos:narrower go:boardwalk ;
    skos:prefLabel "Walking Trail"@en ;
.

go:walkway
    a skos:Concept ;
    rdfs:isDefinedBy cs: ;
    skos:altLabel "Pathway"@en ;
    skos:definition "A designated path primarily for pedestrian use."@en ;
    skos:historyNote "Added by Queensland 2024-06-04 from Queensland Roads and Tracks dataset." ;
    skos:inScheme cs: ;
    skos:prefLabel "Walkway"@en ;
.

go:wall
    a skos:Concept ;
    rdfs:isDefinedBy cs: ;
    skos:definition "A perpendicular or steep face of a feature, considerable in height."@en ;
    skos:historyNote "Broader concept introduced 2024-03-05." ;
    skos:inScheme cs: ;
    skos:narrower
        go:breakwater ,
        go:ice-wall ,
        go:rock-wall ;
    skos:prefLabel "Wall"@en ;
.

go:waste-infrastructure
    a skos:Concept ;
    rdfs:isDefinedBy cs: ;
    skos:definition "An area for disposal of various types of material."@en ;
    skos:historyNote "Inherited from ICSM Place Names Working Group's National Feature Catalogue as at 21 December 2023, with name label amended from 'Waste'." ;
    skos:inScheme cs: ;
    skos:narrower
        go:landfill ,
        go:liquid-waste-disposal-site ,
        go:refuse-transfer-station ,
        go:scrap-yard ,
        go:sewage-treatment-plant ,
        go:sewer-pipeline ;
    skos:prefLabel "Waste Infrastructure"@en ;
.

go:waterbody
    a skos:Concept ;
    rdfs:isDefinedBy cs: ;
    skos:definition "Natural or constructed places where a body of water may be available."@en ;
    skos:historyNote "Inherited from ICSM Place Names Working Group's National Feature Catalogue as at 21 December 2023." ;
    skos:inScheme cs: ;
    skos:narrower
        go:aquatic-passage ,
        go:aquifer ,
        go:bay ,
        go:dam ,
        go:entrance ,
        go:fjord ,
        go:gulf ,
        go:inlet ,
        go:lagoon ,
        go:lake ,
        go:ocean ,
        go:reservoir ,
        go:sound ,
        go:waterhole ,
        go:wetland ;
    skos:prefLabel "Waterbody"@en ;
.

go:water-infrastructure
    a skos:Concept ;
    rdfs:isDefinedBy cs: ;
    skos:definition "Places that indicate constructed features associated with water."@en ;
    skos:historyNote "Inherited from ICSM Place Names Working Group's National Feature Catalogue as at 21 December 2023." ;
    skos:inScheme cs: ;
    skos:narrower
        go:boat-ramp ,
        go:breakwater ,
        go:dam-wall ,
        go:groyne ,
        go:harbour ,
        go:jetty ,
        go:landing-place ,
        go:levee ,
        go:lock ,
        go:pumping-station ,
        go:spillway ,
        go:water-pipeline ,
        go:water-plant ,
        go:weir ;
    skos:prefLabel "Water Infrastructure"@en ;
.

go:water-pipeline
    a skos:Concept ;
    rdfs:isDefinedBy cs: ;
    skos:definition "A long pipe used to transport water over long distances."@en ;
    skos:historyNote "Inherited from ICSM Place Names Working Group's National Feature Catalogue as at 21 December 2023." ;
    skos:inScheme cs: ;
    skos:prefLabel "Water Pipeline"@en ;
.

go:water-plant
    a skos:Concept ;
    rdfs:isDefinedBy cs: ;
    skos:definition "A facility for the processes of making water more acceptable to end-users."@en ;
    skos:historyNote "Inherited from ICSM Place Names Working Group's National Feature Catalogue as at 21 December 2023." ;
    skos:inScheme cs: ;
    skos:prefLabel "Water Treatment Plant"@en ;
.

go:water-point
    a skos:Concept ;
    rdfs:isDefinedBy cs: ;
    skos:definition "Natural or constructed places where water may be available."@en ;
    skos:historyNote "Inherited from ICSM Place Names Working Group's National Feature Catalogue as at 21 December 2023." ;
    skos:inScheme cs: ;
    skos:narrower
        go:bore ,
        go:soak ,
        go:spring ,
        go:water-tank ;
    skos:prefLabel "Water Point"@en ;
.

go:water-tank
    a skos:Concept ;
    rdfs:isDefinedBy cs: ;
    skos:altLabel "Water Tower"@en ;
    skos:definition "A large container for the storage of water."@en ;
    skos:historyNote "Inherited from ICSM Place Names Working Group's National Feature Catalogue as at 21 December 2023." ;
    skos:inScheme cs: ;
    skos:narrower go:elevated-water-tank ;
    skos:prefLabel "Water Tank"@en ;
.

go:water-transport-infrastructure
    a skos:Concept ;
    rdfs:isDefinedBy cs: ;
    skos:definition "Infrastructure to support navigation, safety, watercraft and shipping activities."@en ;
    skos:historyNote "Inherited from ICSM Place Names Working Group's National Feature Catalogue as at 21 December 2023, with name label amended from 'Water'." ;
    skos:inScheme cs: ;
    skos:narrower
        go:beacon ,
        go:cargo-terminal ,
        go:dock ,
        go:ferry-transport-infrastructure ,
        go:harbour-control-tower ,
        go:lighthouse ,
        go:marina ,
        go:pier ,
        go:port ,
        go:port-control-tower ,
        go:wharf ;
    skos:prefLabel "Water Transport Infrastructure"@en ;
.

go:watercourse
    a skos:Concept ;
    rdfs:isDefinedBy cs: ;
    skos:altLabel
        "Run"@en ,
        "Stream"@en ;
    skos:definition "A course of running water (either permanent, intermittent or largely dry)."@en ;
    skos:historyNote "Inherited from ICSM Place Names Working Group's National Feature Catalogue as at 21 December 2023." ;
    skos:inScheme cs: ;
    skos:narrower
        go:anabranch ,
        go:brook ,
        go:creek ,
        go:gully ,
        go:river ,
        go:watercourse-branch ;
    skos:prefLabel "Watercourse"@en ;
.

go:watercourse-branch
    a skos:Concept ;
    rdfs:isDefinedBy cs: ;
    skos:altLabel "Watercourse Arm"@en ;
    skos:definition "A watercourse that is a branch of the main watercourse."@en ;
    skos:historyNote "Added by Queensland 2024-06-11. Definition amended from Macquarie Dictionary." ;
    skos:inScheme cs: ;
    skos:prefLabel "Watercourse Branch"@en ;
.

go:waterfall
    a skos:Concept ;
    rdfs:isDefinedBy cs: ;
    skos:altLabel
        "Cascade"@en ,
        "Cataract"@en ,
        "Fall"@en ,
        "Falls"@en ;
    skos:definition "A sudden descent of water over a step in the bed of a stream."@en ;
    skos:historyNote "Inherited from ICSM Place Names Working Group's National Feature Catalogue as at 21 December 2023." ;
    skos:inScheme cs: ;
    skos:prefLabel "Waterfall"@en ;
.

go:waterhole
    a skos:Concept ;
    rdfs:isDefinedBy cs: ;
    skos:altLabel
        "Pond"@en ,
        "Pool"@en ,
        "Rock Pool"@en ;
    skos:definition "A small body of still or standing water, permanent or temporary, often in the bed of an intermittent river or stream, and sometimes spring fed, chiefly one of natural formation."@en ;
    skos:historyNote "Inherited from ICSM Place Names Working Group's National Feature Catalogue as at 21 December 2023." ;
    skos:inScheme cs: ;
    skos:prefLabel "Waterhole"@en ;
.

go:waterway
    a skos:Concept ;
    rdfs:isDefinedBy cs: ;
    skos:definition "Natural or constructed places that are associated with the movement of water."@en ;
    skos:historyNote "Inherited from ICSM Place Names Working Group's National Feature Catalogue as at 21 December 2023." ;
    skos:inScheme cs: ;
    skos:narrower
        go:bend ,
        go:canal ,
        go:drain ,
        go:estuary ,
        go:irrigation-channel ,
        go:rapids ,
        go:reach ,
        go:watercourse ,
        go:waterfall ;
    skos:prefLabel "Waterway"@en ;
.

go:weather-station
    a skos:Concept ;
    rdfs:isDefinedBy cs: ;
    skos:altLabel "Meteorological Station"@en ;
    skos:definition "An installation equipped and used for the making of meteorological observation."@en ;
    skos:historyNote "Inherited from ICSM Place Names Working Group's National Feature Catalogue as at 21 December 2023." ;
    skos:inScheme cs: ;
    skos:narrower go:automatic-weather-station ;
    skos:prefLabel "Weather Station"@en ;
.

go:weighbridge
    a skos:Concept ;
    rdfs:isDefinedBy cs: ;
    skos:definition "A device located at the side of a road for weighing vehicles and their loads."@en ;
    skos:historyNote "Inherited from ICSM Place Names Working Group's National Feature Catalogue as at 21 December 2023." ;
    skos:inScheme cs: ;
    skos:prefLabel "Weighbridge"@en ;
.

go:weir
    a skos:Concept ;
    rdfs:isDefinedBy cs: ;
    skos:altLabel "Barrage"@en ;
    skos:definition "A low barrier across a watercourse over which water is allowed to flow steadily. A weir raises the water level upstream, and can also be used to measure flow and control the depth of water impounded."@en ;
    skos:historyNote "Inherited from ICSM Place Names Working Group's National Feature Catalogue as at 21 December 2023. 2023-09-19" ;
    skos:inScheme cs: ;
    skos:prefLabel "Weir"@en ;
.

go:wet-dock
    a skos:Concept ;
    rdfs:isDefinedBy cs: ;
    skos:definition "A basin into which vessels enter and in which the water is kept at one level by dock gates, irrespective of outside tides."@en ;
    skos:historyNote "Created by separating 'Dock' alternate labels 2024-06-10. Definition from Macquarie Dictionary." ;
    skos:inScheme cs: ;
    skos:prefLabel "Wet Dock"@en ;
.

go:wetland
    a skos:Concept ;
    rdfs:isDefinedBy cs: ;
    skos:altLabel
        "Bog"@en ,
        "Marsh"@en ,
        "Morass"@en ,
        "Swamp"@en ;
    skos:definition "Areas inundated or saturated by surface or groundwater at a frequency and duration sufficient to support vegetation typical of swamps, marshes, bogs."@en ;
    skos:historyNote "Inherited from ICSM Place Names Working Group's National Feature Catalogue as at 21 December 2023." ;
    skos:inScheme cs: ;
    skos:narrower go:salt-marsh ;
    skos:prefLabel "Wetland"@en ;
.

go:wharf
    a skos:Concept ;
    rdfs:isDefinedBy cs: ;
    skos:altLabel "Quay"@en ;
    skos:definition "A platform, contiguous to and more or less parallel with the shoreline, alongside which ships may be secured for loading or unloading cargo or passengers."@en ;
    skos:historyNote "Inherited from ICSM Place Names Working Group's National Feature Catalogue as at 21 December 2023." ;
    skos:inScheme cs: ;
    skos:prefLabel "Wharf"@en ;
.

go:wildlife-park
    a skos:Concept ;
    rdfs:isDefinedBy cs: ;
    skos:definition "A larger area for animals to roam that is closer to their natural environment than a traditional zoo. Visitors often drive through these parks to observe animals roaming in semi-natural conditions."@en ;
    skos:historyNote "Created by separating 'Zoo' alternate labels 2024-05-10." ;
    skos:inScheme cs: ;
    skos:prefLabel "Wildlife Park"@en ;
.

go:wildlife-sanctuary
    a skos:Concept ;
    rdfs:isDefinedBy cs: ;
    skos:definition "A protected area that is a reserve for the conservation of wildlife, where hunting and fishing are often prohibited. Sanctuaries provide habitat and protection for animals, especially those that are endangered or have been rescued from adverse conditions. They usually allow animals to live in a setting that's closer to their natural habitat compared to zoos."@en ;
    skos:historyNote "Created by separating 'Zoo' alternate labels 2024-05-10." ;
    skos:inScheme cs: ;
    skos:prefLabel "Wildlife Sanctuary"@en ;
.

go:wind-farm
    a skos:Concept ;
    rdfs:isDefinedBy cs: ;
    skos:definition "Consists of a group of individual wind turbines which are connected to the electric power transmission network."@en ;
    skos:historyNote "Inherited from ICSM Place Names Working Group's National Feature Catalogue as at 21 December 2023." ;
    skos:inScheme cs: ;
    skos:prefLabel "Wind Farm"@en ;
.

go:wind-turbine
    a skos:Concept ;
    rdfs:isDefinedBy cs: ;
    skos:definition "A turbine used to generate electricity in areas with strong, steady winds, sometimes offshore."@en ;
    skos:historyNote "Inherited from ICSM Place Names Working Group's National Feature Catalogue as at 21 December 2023." ;
    skos:inScheme cs: ;
    skos:prefLabel "Wind Turbine"@en ;
.

go:womens-hospital
    a skos:Concept ;
    rdfs:isDefinedBy cs: ;
    skos:definition "An institution in which sick or injured female persons are given medical or surgical treatment."@en ;
    skos:historyNote "Created by separating Hospital alternate labels, definition adapted from Hospital Queensland 2024-03-05." ;
    skos:inScheme cs: ;
    skos:prefLabel "Womens Hospital"@en ;
.

go:wood
    a skos:Concept ;
    rdfs:isDefinedBy cs: ;
    skos:altLabel "Woodland"@en ;
    skos:definition "A stretch of land on which the vegetation is dominated by trees, sometimes of one or few species, smaller than a forest."@en ;
    skos:historyNote "Concept created by separating 'Forest' alternate labels 2024-06-11. Definition from Macquarie Dictionary." ;
    skos:inScheme cs: ;
    skos:prefLabel "Wood"@en ;
.

go:zoo
    a skos:Concept ;
    rdfs:isDefinedBy cs: ;
    skos:altLabel "Zoological Gardens"@en ;
    skos:definition "An establishment which maintains a collection of wild animals, typically in a park or gardens, for study, conservation, or display to the public."@en ;
    skos:historyNote "Inherited from ICSM Place Names Working Group's National Feature Catalogue as at 21 December 2023." ;
    skos:inScheme cs: ;
    skos:narrower
        go:wildlife-park ,
        go:wildlife-sanctuary ;
    skos:prefLabel "Zoo"@en ;
.

go:air-traffic-control-tower
    a skos:Concept ;
    rdfs:isDefinedBy cs: ;
    skos:definition "A tower-shaped building, as at an airport, from which instructions to planes arriving and departing can be given."@en ;
    skos:historyNote "Created by separating 'Control Tower' alternate labels 2024-06-10. Definition adapted from 'Control Tower'." ;
    skos:inScheme cs: ;
    skos:prefLabel "Air Traffic Control Tower"@en ;
.

go:breakwater
    a skos:Concept ;
    rdfs:isDefinedBy cs: ;
    skos:altLabel
        "Mole"@en ,
        "Sea Wall"@en ;
    skos:definition """A natural or artificial structure along a coast 
capable of checking the force of the waves, 
thereby reducing beach erosion."""@en ;
    skos:historyNote "Inherited from ICSM Place Names Working Group's National Feature Catalogue as at 21 December 2023. Definition from Geographical Names Board, NSW." ;
    skos:inScheme cs: ;
    skos:narrower
        go:groyne ,
        go:levee ;
    skos:prefLabel "Breakwater"@en ;
    schema:citation "https://www.gnb.nsw.gov.au/__data/assets/pdf_file/0011/59627/Glossary_of_Designation_Values.pdf"^^xsd:anyURI ;
.

go:bus-station
    a skos:Concept ;
    rdfs:isDefinedBy cs: ;
    skos:definition "A structure beside the road with facilities for passengers to board or alight."@en ;
    skos:historyNote "Inherited from ICSM Place Names Working Group's National Feature Catalogue as at 21 December 2023." ;
    skos:inScheme cs: ;
    skos:prefLabel "Bus Station"@en ;
.

go:cableway-terminal
    a skos:Concept ;
    rdfs:isDefinedBy cs: ;
    skos:altLabel "Gondola Terminal"@en ;
    skos:definition "A building associated with a cableway."@en ;
    skos:historyNote "Inherited from ICSM Place Names Working Group's National Feature Catalogue as at 21 December 2023." ;
    skos:inScheme cs: ;
    skos:prefLabel "Cableway Terminal"@en ;
.

go:ferry-station
    a skos:Concept ;
    rdfs:isDefinedBy cs: ;
    skos:altLabel "Ferry Passenger Terminal"@en ;
    skos:definition "A designated place where ferries stop for passengers to board or alight."@en ;
    skos:historyNote "Inherited from ICSM Place Names Working Group's National Feature Catalogue as at 21 December 2023." ;
    skos:inScheme cs: ;
    skos:prefLabel "Ferry Station"@en ;
.

go:foot-tunnel
    a skos:Concept ;
    rdfs:isDefinedBy cs: ;
    skos:altLabel "Subway"@en ;
    skos:definition "A long, enclosed passageway that goes through a barrier or obstacle such as a mountain, hill, or beneath a body of water, allowing a pedestrian thoroughfare to pass beneath an obstruction."@en ;
    skos:historyNote "Inherited from ICSM Place Names Working Group's National Feature Catalogue as at 21 December 2023." ;
    skos:inScheme cs: ;
    skos:prefLabel "Foot Tunnel"@en ;
.

go:green-bridge
    a skos:Concept ;
    rdfs:isDefinedBy cs: ;
    skos:definition "A structure erected over a depression or obstacle designed for sustainable transport use, such as buses, cyclists and/or pedestrians. Not for general vehicular access."@en ;
    skos:historyNote "Broader concept introduced 2024-03-05." ;
    skos:inScheme cs: ;
    skos:narrower go:footbridge ;
    skos:prefLabel "Green Bridge"@en ;
.

go:groyne
    a skos:Concept ;
    rdfs:isDefinedBy cs: ;
    skos:definition "A low artificial wall-like structure constructed of timber, stone, concrete or steel, usually extending roughly perpendicular to the shoreline and designed to protect the shore from erosion or to trap sand."@en ;
    skos:historyNote "Inherited from ICSM Place Names Working Group's National Feature Catalogue as at 21 December 2023." ;
    skos:inScheme cs: ;
    skos:prefLabel "Groyne"@en ;
.

go:guyot
    a skos:Concept ;
    rdfs:isDefinedBy cs: ;
    skos:altLabel "Tablemount"@en ;
    skos:definition "A seamount with a comparatively smooth flat top."@en ;
    skos:historyNote "Inherited from ICSM Place Names Working Group's National Feature Catalogue as at 21 December 2023. Definition from General Bathymetric Chart of the Oceans (GEBCO) Sub-Committee on Undersea Features Names (SCUFN)." ;
    skos:inScheme cs: ;
    skos:prefLabel "Guyot"@en ;
	skos:scopeNote "Term 'Tablemount' now obsolete and recognised for historically named features only. " ;
    schema:citation "https://iho.int/en/basic-documents-1"^^xsd:anyURI ;
.

go:harbour-control-tower
    a skos:Concept ;
    rdfs:isDefinedBy cs: ;
    skos:definition "A tower-shaped building at a harbour, from which instructions to ships arriving and departing can be given."@en ;
    skos:historyNote "Created by separating 'Control Tower' alternate labels 2024-06-10. Definition adapted from 'Control Tower'." ;
    skos:inScheme cs: ;
    skos:prefLabel "Harbour Control Tower"@en ;
.

go:ice-wall
    a skos:Concept ;
    rdfs:isDefinedBy cs: ;
    skos:definition "An ice cliff forming the seaward margin of an inland ice sheet, ice cap, ice piedmont or ice rise. The rock basement may be at or below sea level."@en ;
    skos:historyNote "Inherited from ICSM Place Names Working Group's National Feature Catalogue as at 21 December 2023. Concept and definition from the Australian Antarctic Division." ;
    skos:inScheme cs: ;
    skos:prefLabel "Ice Wall"@en ;
    schema:citation "https://data.aad.gov.au/aadc/ftc/display_feature_type.cfm?feature_type_code=343"^^xsd:anyURI ;
.

go:levee
    a skos:Concept ;
    rdfs:isDefinedBy cs: ;
    skos:definition "An embankment built to confine a river from flooding."@en ;
    skos:historyNote "Inherited from ICSM Place Names Working Group's National Feature Catalogue as at 21 December 2023." ;
    skos:inScheme cs: ;
    skos:prefLabel "Levee"@en ;
.

go:light-rail-station
    a skos:Concept ;
    rdfs:isDefinedBy cs: ;
    skos:altLabel "Light Railway Station"@en ;
    skos:definition "A structure beside a light rail line with facilities for receiving and discharging passengers."@en ;
    skos:historyNote "Inherited from ICSM Place Names Working Group's National Feature Catalogue as at 21 December 2023." ;
    skos:inScheme cs: ;
    skos:prefLabel "Light Rail Station"@en ;
.

go:light-rail-tunnel
    a skos:Concept ;
    rdfs:isDefinedBy cs: ;
    skos:altLabel "Light Railway Tunnel"@en ;
    skos:definition "A passageway for light rail trains through or under an obstruction."@en ;
    skos:historyNote "Inherited from ICSM Place Names Working Group's National Feature Catalogue as at 21 December 2023." ;
    skos:inScheme cs: ;
    skos:prefLabel "Light Rail Tunnel"@en ;
.

go:marine-apron
    a skos:Concept ;
    rdfs:isDefinedBy cs: ;
    skos:altLabel "Archipelagic Apron"@en ;
    skos:definition "A gently dipping slope, with a smooth surface, commonly found around groups of islands and seamounts."@en ;
    skos:historyNote "Inherited from ICSM Place Names Working Group's National Feature Catalogue as at 21 December 2023. Definition from General Bathymetric Chart of the Oceans (GEBCO) Sub-Committee on Undersea Features Names (SCUFN)." ;
    skos:inScheme cs: ;
    skos:prefLabel "Marine Apron"@en ;
	skos:scopeNote "Term 'Archipelagic Apron' now obsolete and recognised for historically named features only. " ;
    schema:citation "https://iho.int/en/basic-documents-1"^^xsd:anyURI ;
.

go:marine-bank
    a skos:Concept ;
    rdfs:isDefinedBy cs: ;
    skos:altLabel "Cap"@en ;
    skos:definition "An elevation of the seafloor at depths generally less than 200m, but sufficient for safe surface navigation commonly found on the continental shelf or near an island."@en ;
    skos:historyNote "Inherited from ICSM Place Names Working Group's National Feature Catalogue as at 21 December 2023. Definition from General Bathymetric Chart of the Oceans (GEBCO) Sub-Committee on Undersea Features Names (SCUFN)." ;
    skos:inScheme cs: ;
    skos:prefLabel "Marine Bank"@en ;
	skos:scopeNote "Term 'Cap' now obsolete and recognised for historically named features only. " ;
    schema:citation "https://iho.int/en/basic-documents-1"^^xsd:anyURI ;
.

go:marine-basin
    a skos:Concept ;
    rdfs:isDefinedBy cs: ;
    skos:definition "A depression more or less equidimensional in plan and of variable extent."@en ;
    skos:historyNote "Inherited from ICSM Place Names Working Group's National Feature Catalogue as at 21 December 2023. Definition from General Bathymetric Chart of the Oceans (GEBCO) Sub-Committee on Undersea Features Names (SCUFN)." ;
    skos:inScheme cs: ;
    skos:narrower go:deep ;
    skos:prefLabel "Marine Basin"@en ;
    schema:citation "https://iho.int/en/basic-documents-1"^^xsd:anyURI ;
.

go:marine-gap
    a skos:Concept ;
    rdfs:isDefinedBy cs: ;
    skos:definition "A narrow break in a ridge, rise or other elevation."@en ;
    skos:historyNote "Inherited from ICSM Place Names Working Group's National Feature Catalogue as at 21 December 2023. Definition from General Bathymetric Chart of the Oceans (GEBCO) Sub-Committee on Undersea Features Names (SCUFN)." ;
    skos:inScheme cs: ;
    skos:prefLabel "Marine Gap"@en ;
    schema:citation "https://iho.int/en/basic-documents-1"^^xsd:anyURI ;
.

go:marine-hill
    a skos:Concept ;
    rdfs:isDefinedBy cs: ;
    skos:altLabel "Abyssal Hill"@en ;
    skos:definition "A distinct elevation generally of irregular shape, less than 1000m above the surrounding relief as measured from the deepest isobath that surrounds most of the feature."@en ;
    skos:historyNote "Inherited from ICSM Place Names Working Group's National Feature Catalogue as at 21 December 2023. Definition from General Bathymetric Chart of the Oceans (GEBCO) Sub-Committee on Undersea Features Names (SCUFN)." ;
    skos:inScheme cs: ;
    skos:prefLabel "Marine Hill"@en ;
	skos:scopeNote "Term 'Abyssal Hill' now obsolete and recognised for historically named features only. " ;
    schema:citation "https://iho.int/en/basic-documents-1"^^xsd:anyURI ;
.

go:marine-plateau
    a skos:Concept ;
    rdfs:isDefinedBy cs: ;
    skos:definition "A large, relatively flat elevation that is higher than the surrounding relief with one or more relatively steep sides."@en ;
    skos:historyNote "Inherited from ICSM Place Names Working Group's National Feature Catalogue as at 21 December 2023. Definition from General Bathymetric Chart of the Oceans (GEBCO) Sub-Committee on Undersea Features Names (SCUFN)." ;
    skos:inScheme cs: ;
    skos:prefLabel "Marine Plateau"@en ;
    schema:citation "https://iho.int/en/basic-documents-1"^^xsd:anyURI ;
.

go:marine-slope
    a skos:Concept ;
    rdfs:isDefinedBy cs: ;
    skos:altLabel
        "Continental Rise"@en ,
        "Continental Slope"@en ;
    skos:definition "The sloping region that deepens from a shelf to the point where there is a general decrease in gradient."@en ;
    skos:historyNote "Inherited from ICSM Place Names Working Group's National Feature Catalogue as at 21 December 2023. Definition from General Bathymetric Chart of the Oceans (GEBCO) Sub-Committee on Undersea Features Names (SCUFN)." ;
    skos:inScheme cs: ;
    skos:narrower
        go:marine-apron ,
        go:marine-escarpment ;
    skos:prefLabel "Marine Slope"@en ;
	skos:scopeNote "Terms 'Continental Rise' and 'Continental Slope' now obsolete and recognised for historically named features only. " ;
    schema:citation "https://iho.int/en/basic-documents-1"^^xsd:anyURI ;
.

go:marine-trench
    a skos:Concept ;
    rdfs:isDefinedBy cs: ;
    skos:definition "A long, deep, asymmetrical depression with relatively steep sides, that is associated with subduction."@en ;
    skos:historyNote "Inherited from ICSM Place Names Working Group's National Feature Catalogue as at 21 December 2023. Definition from General Bathymetric Chart of the Oceans (GEBCO) Sub-Committee on Undersea Features Names (SCUFN)." ;
    skos:inScheme cs: ;
    skos:narrower go:deep ;
    skos:prefLabel "Marine Trench"@en ;
    schema:citation "https://iho.int/en/basic-documents-1"^^xsd:anyURI ;
.

go:marine-valley
    a skos:Concept ;
    rdfs:isDefinedBy cs: ;
    skos:altLabel
        "Median Valley"@en ,
        "Sea Valley"@en ,
        "Seabight"@en ,
        "Submarine Valley"@en ;
    skos:definition "An elongated depression that generally widens and deepens down-slope."@en ;
    skos:historyNote "Inherited from ICSM Place Names Working Group's National Feature Catalogue as at 21 December 2023. Definition from General Bathymetric Chart of the Oceans (GEBCO) Sub-Committee on Undersea Features Names (SCUFN)." ;
    skos:inScheme cs: ;
    skos:prefLabel "Marine Valley"@en ;
	skos:scopeNote "Terms 'Median Valley', 'Sea Valley', 'Submarine Valley' and 'Seabight' now obsolete and recognised for historically named features only. " ;
    schema:citation "https://iho.int/en/basic-documents-1"^^xsd:anyURI ;
.

go:mining-centre
    a skos:Concept ;
    rdfs:isDefinedBy cs: ;
    skos:definition "A facility built to support a mine or other area from which ores, precious stones or minerals are or were extracted from the earth."@en ;
    skos:historyNote "Inherited from ICSM Place Names Working Group's National Feature Catalogue as at 21 December 2023." ;
    skos:inScheme cs: ;
    skos:prefLabel "Mining Centre"@en ;
.

go:offshore-rock
    a skos:Concept ;
    rdfs:isDefinedBy cs: ;
    skos:definition "A typically unvegetated rock protruding from the sea."@en ;
    skos:historyNote "Created by separating 'Island' alternate labels 2024-03-05." ;
    skos:inScheme cs: ;
    skos:prefLabel "Offshore Rock"@en ;
.

go:plantation
    a skos:Concept ;
    rdfs:isDefinedBy cs: ;
    skos:altLabel "Orchard"@en ;
    skos:definition "A plot in which trees are planted and cultivated, usually for commercial purposes."@en ;
    skos:historyNote "Inherited from ICSM Place Names Working Group's National Feature Catalogue as at 21 December 2023." ;
    skos:inScheme cs: ;
    skos:prefLabel "Plantation"@en ;
.

go:port-control-tower
    a skos:Concept ;
    rdfs:isDefinedBy cs: ;
    skos:definition "A tower-shaped building at a port, from which instructions to ships arriving and departing can be given."@en ;
    skos:historyNote "Created by separating 'Control Tower' alternate labels 2024-06-10. Definition adapted from 'Control Tower'." ;
    skos:inScheme cs: ;
    skos:prefLabel "Port Control Tower"@en ;
.

go:rail-bridge
    a skos:Concept ;
    rdfs:isDefinedBy cs: ;
    skos:altLabel "Railway Bridge"@en ;
    skos:definition "A structure over an obstruction affording safe rail passage."@en ;
    skos:historyNote "Inherited from ICSM Place Names Working Group's National Feature Catalogue as at 21 December 2023." ;
    skos:inScheme cs: ;
    skos:prefLabel "Rail Bridge"@en ;
.

go:rail-station
    a skos:Concept ;
    rdfs:isDefinedBy cs: ;
    skos:altLabel
        "Railway Station"@en ,
        "Station"@en ,
        "Train Station"@en ;
    skos:definition "A structure beside a railway line with facilities for receiving and discharging passengers and freight."@en ;
    skos:historyNote "Inherited from ICSM Place Names Working Group's National Feature Catalogue as at 21 December 2023." ;
    skos:inScheme cs: ;
    skos:prefLabel "Rail Station"@en ;
.

go:rail-tunnel
    a skos:Concept ;
    rdfs:isDefinedBy cs: ;
    skos:altLabel "Railway Tunnel"@en ;
    skos:definition "A passageway for trains through or under an obstruction."@en ;
    skos:historyNote "Inherited from ICSM Place Names Working Group's National Feature Catalogue as at 21 December 2023." ;
    skos:inScheme cs: ;
    skos:prefLabel "Rail Tunnel"@en ;
.

go:residential-aged-care
    a skos:Concept ;
    rdfs:isDefinedBy cs: ;
    skos:definition "A residential facility that supports the care of the elderly."@en ;
    skos:historyNote "Created by separating 'Aged Care' alternate labels 2024-03-05." ;
    skos:inScheme cs: ;
    skos:prefLabel "Residential Aged Care"@en ;
.

go:road-bridge
    a skos:Concept ;
    rdfs:isDefinedBy cs: ;
    skos:altLabel
        "Flyover"@en ,
        "Overpass"@en ;
    skos:definition "A structure spanning a rail line, river, road or the like affording safe road passage."@en ;
    skos:historyNote "Inherited from ICSM Place Names Working Group's National Feature Catalogue as at 21 December 2023." ;
    skos:inScheme cs: ;
    skos:prefLabel "Road Bridge"@en ;
.

go:road-tunnel
    a skos:Concept ;
    rdfs:isDefinedBy cs: ;
    skos:definition "A long, enclosed passageway that goes through a barrier or obstacle such as a mountain, hill, or beneath a body of water, allowing a road to pass beneath an obstruction."@en ;
    skos:historyNote "Inherited from ICSM Place Names Working Group's National Feature Catalogue as at 21 December 2023." ;
    skos:inScheme cs: ;
    skos:prefLabel "Road Tunnel"@en ;
.

go:seamount
    a skos:Concept ;
    rdfs:isDefinedBy cs: ;
    skos:definition "A distinct generally equidimensional elevation greater than 1000m above the surrounding relief as measured from the deepest isobath that surrounds most of the feature."@en ;
    skos:historyNote "Inherited from ICSM Place Names Working Group's National Feature Catalogue as at 21 December 2023. Definition from General Bathymetric Chart of the Oceans (GEBCO) Sub-Committee on Undersea Features Names (SCUFN)." ;
    skos:inScheme cs: ;
    skos:narrower go:guyot ;
    skos:prefLabel "Seamount"@en ;
    schema:citation "https://iho.int/en/basic-documents-1"^^xsd:anyURI ;
.

go:seamount-chain
    a skos:Concept ;
    rdfs:isDefinedBy cs: ;
    skos:definition "A linear or arcuate alignment of discrete Seamounts."@en ;
    skos:historyNote "Inherited from ICSM Place Names Working Group's National Feature Catalogue as at 21 December 2023. Definition from General Bathymetric Chart of the Oceans (GEBCO) Sub-Committee on Undersea Features Names (SCUFN)." ;
    skos:inScheme cs: ;
    skos:prefLabel "Seamount Chain"@en ;
    schema:citation "https://iho.int/en/basic-documents-1"^^xsd:anyURI ;
.

go:subglacial-mount
    a skos:Concept ;
    rdfs:isDefinedBy cs: ;
    skos:altLabel "Subglacial Mountain"@en ;
    skos:definition "Subglacial: a term meaning 'beneath the ice'. Mountain: A mass of land considerably higher than its surroundings and of greater altitude than a hill."@en ;
    skos:historyNote "Inherited from ICSM Place Names Working Group's National Feature Catalogue as at 21 December 2023. Derived from definition from the Australian Antarctic Division." ;
    skos:inScheme cs: ;
    skos:prefLabel "Subglacial Mount"@en ;
    schema:citation "https://data.aad.gov.au/aadc/ftc/display_feature_type.cfm?feature_type_code=427"^^xsd:anyURI ;
.

go:subglacial-trench
    a skos:Concept ;
    rdfs:isDefinedBy cs: ;
    skos:definition "Subglacial: a term meaning 'beneath the ice'. Trench: A deep, or elongated trough, in a floor of the ocean."@en ;
    skos:historyNote "Inherited from ICSM Place Names Working Group's National Feature Catalogue as at 21 December 2023." ;
    skos:inScheme cs: ;
    skos:prefLabel "Subglacial Trench"@en ;
.

go:tram-station
    a skos:Concept ;
    rdfs:isDefinedBy cs: ;
    skos:altLabel
        "Tram Stop"@en ,
        "Tramway Station"@en ;
    skos:definition "A structure beside a tramway with facilities for receiving and discharging passengers."@en ;
    skos:historyNote "Created by separating 'Light Rail Station' alternate labels 2024-06-10. Definition adapted from 'Light Rail Station'." ;
    skos:inScheme cs: ;
    skos:prefLabel "Tram Station"@en ;
.

go:tram-tunnel
    a skos:Concept ;
    rdfs:isDefinedBy cs: ;
    skos:altLabel "Tramway Tunnel"@en ;
    skos:definition "A passageway for trams through or under an obstruction."@en ;
    skos:historyNote "Inherited from ICSM Place Names Working Group's National Feature Catalogue as at 21 December 2023." ;
    skos:inScheme cs: ;
    skos:prefLabel "Tram Tunnel"@en ;
.

go:winery
    a skos:Concept ;
    rdfs:isDefinedBy cs: ;
    skos:altLabel
        "Cellar"@en ,
        "Cellar Door"@en ;
    skos:definition "A commercial establishment where wine is made."@en ;
    skos:historyNote "Inherited from ICSM Place Names Working Group's National Feature Catalogue as at 21 December 2023." ;
    skos:inScheme cs: ;
    skos:prefLabel "Winery"@en ;
.

go:marine-escarpment
    a skos:Concept ;
    rdfs:isDefinedBy cs: ;
    skos:altLabel "Marine Scarp"@en ;
    skos:definition "An elongated, characteristically linear, steep slope separating horizontal or gently sloping areas of the sea floor."@en ;
    skos:historyNote "Inherited from ICSM Place Names Working Group's National Feature Catalogue as at 21 December 2023. Definition from General Bathymetric Chart of the Oceans (GEBCO) Sub-Committee on Undersea Features Names (SCUFN)." ;
    skos:inScheme cs: ;
    skos:prefLabel "Marine Escarpment"@en ;
	skos:scopeNote "Term 'Marine Scarp' now obsolete and recognised for historically named features only. " ;
    schema:citation "https://iho.int/en/basic-documents-1"^^xsd:anyURI ;
.

go:subglacial-basin
    a skos:Concept ;
    rdfs:isDefinedBy cs: ;
    skos:definition "Subglacial: a term meaning 'beneath the ice'. Basin: a very large depression occupied by sea water, ie. an ocean basin."@en ;
    skos:historyNote "Inherited from ICSM Place Names Working Group's National Feature Catalogue as at 21 December 2023. Concept and definition from the Australian Antarctic Division." ;
    skos:inScheme cs: ;
    skos:prefLabel "Subglacial Basin"@en ;
    schema:citation "https://data.aad.gov.au/aadc/ftc/display_feature_type.cfm?feature_type_code=426"^^xsd:anyURI ;
.

go:deep
    a skos:Concept ;
    rdfs:isDefinedBy cs: ;
    skos:definition "A localised depression within the confines of a larger feature, such as a trough, basin or trench."@en ;
    skos:historyNote "Inherited from ICSM Place Names Working Group's National Feature Catalogue as at 21 December 2023. Definition from General Bathymetric Chart of the Oceans (GEBCO) Sub-Committee on Undersea Features Names (SCUFN)." ;
    skos:inScheme cs: ;
    skos:prefLabel "Deep"@en ;
    schema:citation "https://iho.int/en/basic-documents-1"^^xsd:anyURI ;
.

cs:
    a skos:ConceptScheme ;
    reg:status <https://linked.data.gov.au/def/reg-statuses/experimental> ;
    owl:versionIRI go:1.0.1 ;
    skos:definition "A hierarchy of Geographical (Place) Object categories"@en ;
    skos:hasTopConcept
        go:administrative-construct ,
        go:care-facility ,
        go:cultural-feature ,
        go:defence-site ,
        go:educational-facility ,
        go:emergency-facility ,
        go:health-facility ,
        go:hydrological-feature ,
        go:ice-feature ,
        go:legal-institution ,
        go:place-industrial-activity ,
        go:terrain-feature ,
        go:transport-infrastructure ,
        go:unclassified ,
        go:utility-infrastructure ,
        go:vegetation ;
    skos:historyNote "This vocabulary was originally generated from the Geoscience Australia's Composite Gazetteer of Australia, and has been amended by the Department of Resources (Queensland) to refine and expand the vocabulary."@en ;
    skos:prefLabel "Geographical Object Categories"@en ;
    schema:creator
        [
            a schema:Organization ;
            schema:name "ICSM Place Names Working Group" ;
            schema:url ""^^xsd:anyURI ;
        ] ;
    dcterms:created "2015-01-01"^^xsd:date ;
    dcterms:modified "2024-06-11"^^xsd:date ;
    schema:keywords
        "Geographic Names" ,
        "Geographic Objects" ,
        "Place Names" ;
    schema:publisher <https://linked.data.gov.au/org/qld-resources> ;
    schema:version "1.0.1" ;
    prov:qualifiedAttribution
        [
            prov:hadRole droles:custodian ;
            prov:agent <https://linked.data.gov.au/org/icsm>
        ] ;
.

<https://linked.data.gov.au/org/qld-resources>
    a schema:Organization ;
    schema:name "Queensland Department of Resources" ;
    schema:url "https://www.resources.qld.gov.au"^^xsd:anyURI ;
.