PREFIX ls: <https://linked.data.gov.au/def/lifecycle-stage-types/>
PREFIX cs: <https://linked.data.gov.au/def/lifecycle-stage-types>
PREFIX dcat: <http://www.w3.org/ns/dcat#>
PREFIX isoroles: <https://linked.data.gov.au/def/data-roles/>
PREFIX owl: <http://www.w3.org/2002/07/owl#>
PREFIX prov: <http://www.w3.org/ns/prov#>
PREFIX rdfs: <http://www.w3.org/2000/01/rdf-schema#>
PREFIX schema: <https://schema.org/>
PREFIX skos: <http://www.w3.org/2004/02/skos/core#>
PREFIX xsd: <http://www.w3.org/2001/XMLSchema#>
PREFIX agldwgstatus: <https://linked.data.gov.au/def/reg-statuses/>
PREFIX dcterms: <http://purl.org/dc/terms/>
PREFIX reg: <http://purl.org/linked-data/registry#>
PREFIX sdo: <https://schema.org/>
PREFIX themes: <https://linked.data.gov.au/def/fsdf/themes/>

ls:current
    a skos:Concept ;
    rdfs:isDefinedBy cs: ;
    skos:definition "The feature or feature label is recognised by the authoritative jurisdiction and is in use."@en ;
	skos:historyNote "Adapted from ISO19160-1's AddressLifecycleStage vocabulary. " ;
    skos:inScheme cs: ;
    skos:prefLabel "Current"@en ;
    skos:topConceptOf cs: ;
.

ls:proposed
    a skos:Concept ;
    rdfs:isDefinedBy cs: ;
    skos:definition "The feature or feature label has been suggested for use but not yet accepted."@en ;
	skos:historyNote "Adapted from ISO19160-1's AddressLifecycleStage vocabulary. " ;
    skos:inScheme cs: ;
    skos:prefLabel "Proposed"@en ;
    skos:topConceptOf cs: ;
.

ls:rejected
    a skos:Concept ;
    rdfs:isDefinedBy cs: ;
    skos:definition "The feature or feature label has been ruled not for use."@en ;
	skos:historyNote "Adapted from ISO19160-1's AddressLifecycleStage vocabulary. " ;
    skos:inScheme cs: ;
    skos:prefLabel "Rejected"@en ;
    skos:topConceptOf cs: ;
.

ls:reserved
    a skos:Concept ;
    rdfs:isDefinedBy cs: ;
    skos:definition "The feature or feature label is recognised by the authoritative jurisdiction but is not yet in use."@en ;
	skos:historyNote "Adapted from ISO19160-1's AddressLifecycleStage vocabulary. " ;
    skos:inScheme cs: ;
    skos:prefLabel "Reserved"@en ;
    skos:topConceptOf cs: ;
.

ls:retired
    a skos:Concept ;
    rdfs:isDefinedBy cs: ;
    skos:definition "The feature or feature label was recognised by the authoritative jurisdiction but is no longer in use."@en ;
	skos:historyNote "Adapted from ISO19160-1's AddressLifecycleStage vocabulary. " ;
    skos:inScheme cs: ;
    skos:prefLabel "Retired"@en ;
    skos:topConceptOf cs: ;
.

ls:unknown
    a skos:Concept ;
    rdfs:isDefinedBy cs: ;
    skos:definition "The stage of this feature or feature label's life is unknown, therefore it is assumed to be unofficial."@en ;
	skos:historyNote "Adapted from ISO19160-1's AddressLifecycleStage vocabulary. " ;
    skos:inScheme cs: ;
    skos:prefLabel "Unknown"@en ;
    skos:topConceptOf cs: ;
.

cs:
    a skos:ConceptScheme ;
    owl:versionIRI ls:None ;
    skos:definition "This vocabulary describes types of lifecycle stage for a feature or feature label. "@en ;
    skos:hasTopConcept
        ls:current ,
        ls:proposed ,
        ls:rejected ,
        ls:reserved ,
        ls:retired ,
        ls:unknown ;
    skos:historyNote "This vocabulary contains lifecycle stage types for features and feature labels such as addresses, roads and geographical names. Adapted from ISO19160-1's AddressLifecycleStage vocabulary. "@en ;
    skos:prefLabel "Lifecycle Stage Types"@en ;
    prov:qualifiedAttribution
        [
            dcat:hadRole isoroles:custodian ;
            prov:agent
                [
                    a schema:Person ;
                    schema:email ""^^xsd:anyURI ;
                    schema:name "Icsm" ;
                ] ;
        ] ;
    schema:creator
        [
            a schema:Organization ;
            schema:name "Department Of Resources" ;
            schema:url ""^^xsd:anyURI ;
        ] ;
    dcterms:created "2024-06-12"^^xsd:date ;
	dcterms:modified "2024-06-12"^^xsd:date ;
    schema:publisher
        [
            a schema:Organization ;
            schema:name "Icsm" ;
            schema:url ""^^xsd:anyURI ;
        ] ;
    schema:version "None" ;
.
