PREFIX : <https://linked.data.gov.au/def/naming-authority/>
PREFIX cs: <https://linked.data.gov.au/def/naming-authority>
PREFIX dcat: <http://www.w3.org/ns/dcat#>
PREFIX isoroles: <https://linked.data.gov.au/def/data-roles/>
PREFIX owl: <http://www.w3.org/2002/07/owl#>
PREFIX prov: <http://www.w3.org/ns/prov#>
PREFIX rdfs: <http://www.w3.org/2000/01/rdf-schema#>
PREFIX schema: <https://schema.org/>
PREFIX skos: <http://www.w3.org/2004/02/skos/core#>
PREFIX xsd: <http://www.w3.org/2001/XMLSchema#>
PREFIX agldwgstatus: <https://linked.data.gov.au/def/reg-statuses/>
PREFIX dcterms: <http://purl.org/dc/terms/>
PREFIX reg: <http://purl.org/linked-data/registry#>
PREFIX sdo: <https://schema.org/>
PREFIX themes: <https://linked.data.gov.au/def/fsdf/themes/>

:aus-hydrographic-office
    a skos:Concept ;
    rdfs:isDefinedBy cs: ;
    skos:altLabel "AHO"@en ;
    skos:definition "Naming of underwater features, maritime navigation aids and maritime boundaries. Applies nationally in Australia."@en ;
	skos:historyNote "Queensland Department of Resources. " ;
    skos:inScheme cs: ;
    skos:prefLabel "Australian Hydrographic Office"@en ;
    skos:topConceptOf cs: ;
    schema:citation "https://www.hydro.gov.au/"^^xsd:anyURI ;
.

:aus-post
    a skos:Concept ;
    rdfs:isDefinedBy cs: ;
    skos:definition "Creation of postcodes and naming of mail delivery infrastructure.  Applies nationally in Australia."@en ;
	skos:historyNote "Queensland Department of Resources. " ;
    skos:inScheme cs: ;
    skos:prefLabel "Australia Post"@en ;
    skos:topConceptOf cs: ;
    schema:citation "https://auspost.com.au/"^^xsd:anyURI ;
.

:cth-cac-act
    a skos:Concept ;
    rdfs:isDefinedBy cs: ;
    skos:definition "Names of the \"Original States\" identified in the Commonwealth of Australia Constitution Act. Applies nationally in Australia."@en ;
	skos:historyNote "Queensland Department of Resources. " ;
    skos:inScheme cs: ;
    skos:prefLabel "Commonwealth of Australia Constitution Act (Cth)"@en ;
    skos:topConceptOf cs: ;
    schema:citation "https://www.legislation.gov.au/C2004Q00685/latest/text"^^xsd:anyURI ;
.

:cth-ce-act-1918
    a skos:Concept ;
    rdfs:isDefinedBy cs: ;
    skos:definition "Naming of federal electoral divisions. Applies nationally in Australia."@en ;
	skos:historyNote "Queensland Department of Resources. " ;
    skos:inScheme cs: ;
    skos:prefLabel "Commonwealth Electoral Act 1918 (Cth)"@en ;
    skos:topConceptOf cs: ;
    schema:citation "https://www.legislation.gov.au/C1918A00027/2023-01-01/text"^^xsd:anyURI ;
.

:cth-epbc-act-1999
    a skos:Concept ;
    rdfs:isDefinedBy cs: ;
    skos:definition "Declaration of World Heritage properties for consideration by the international approving body."@en ;
	skos:historyNote "Queensland Department of Resources. " ;
    skos:inScheme cs: ;
    skos:prefLabel "Environment Protection and Biodiversity Conservation Act 1999 (Cth)"@en ;
    skos:topConceptOf cs: ;
    schema:citation "https://www.legislation.gov.au/C2004A00485/latest/text"^^xsd:anyURI ;
.

:gbrmpa
    a skos:Concept ;
    rdfs:isDefinedBy cs: ;
    skos:altLabel "GBRMPA"@en ;
    skos:definition "Entity established under the Great Barrier Reef Marine Park Act 1975 (Cth) with a recognised role of unofficially assigning names to undersea features within the Great Barrier Reef Marine Park."@en ;
	skos:historyNote "Queensland Department of Resources. " ;
    skos:inScheme cs: ;
    skos:prefLabel "Great Barrier Reef Marine Park Authority"@en ;
    skos:topConceptOf cs: ;
    schema:citation "https://www2.gbrmpa.gov.au/"^^xsd:anyURI ;
.

:port-authority
    a skos:Concept ;
    rdfs:isDefinedBy cs: ;
    skos:definition "Port authority with a naming role."@en ;
	skos:historyNote "Queensland Department of Resources. " ;
    skos:inScheme cs: ;
    skos:prefLabel "Port Authority"@en ;
    skos:topConceptOf cs: ;
.

:private
    a skos:Concept ;
    rdfs:isDefinedBy cs: ;
    skos:definition "Individual or group with a naming role."@en ;
	skos:historyNote "Queensland Department of Resources. " ;
    skos:inScheme cs: ;
    skos:prefLabel "Private"@en ;
    skos:topConceptOf cs: ;
.

:qld-ambulance
    a skos:Concept ;
    rdfs:isDefinedBy cs: ;
    skos:altLabel "QAS"@en ;
    skos:definition "Naming of authorised entities by Queensland Ambulance Service. Applies in Queensland."@en ;
	skos:historyNote "Queensland Department of Resources. " ;
    skos:inScheme cs: ;
    skos:prefLabel "Queensland Ambulance Service"@en ;
    skos:topConceptOf cs: ;
.

:qld-bccm-act-1997
    a skos:Concept ;
    rdfs:isDefinedBy cs: ;
    skos:definition "Naming of community title schemes. Applies in Queensland."@en ;
	skos:historyNote "Queensland Department of Resources. " ;
    skos:inScheme cs: ;
    skos:prefLabel "Body Corporate and Community Management Act 1997 (Qld)"@en ;
    skos:topConceptOf cs: ;
    schema:citation "https://www.legislation.qld.gov.au/view/html/inforce/current/act-1997-028"^^xsd:anyURI ;
.

:qld-caca-act-1957
    a skos:Concept ;
    rdfs:isDefinedBy cs: ;
    skos:definition "Naming of entities under the control of Weipa Town Authority e.g. road naming, street numbering, parks. Applies in the area of Weipa Town covered by the Act."@en ;
	skos:historyNote "Queensland Department of Resources. " ;
    skos:inScheme cs: ;
    skos:prefLabel "Commonwealth Aluminium Corporation Pty. Limited Agreement Act 1957 (Qld)"@en ;
    skos:topConceptOf cs: ;
    schema:citation "https://www.legislation.qld.gov.au/view/2010-12-10/act-1957-029"^^xsd:anyURI ;
.

:qld-cb-act-2010
    a skos:Concept ;
    rdfs:isDefinedBy cs: ;
    skos:definition "Naming of Local Government Area Divisions for Brisbane. Naming of entities under the control of local government e.g. road naming, street numbering, parks and public facilities, public areas, bridges and ther infrastructure. Applies to the area covered by the City of Brisbane Act."@en ;
	skos:historyNote "Queensland Department of Resources. " ;
    skos:inScheme cs: ;
    skos:prefLabel "City of Brisbane Act 2010 (Qld)"@en ;
    skos:topConceptOf cs: ;
    schema:citation "https://www.legislation.qld.gov.au/view/html/inforce/current/act-2010-023"^^xsd:anyURI ;
.

:qld-cs-act-2006
    a skos:Concept ;
    rdfs:isDefinedBy cs: ;
    skos:definition "Naming of corrections centres. Applies in Queensland."@en ;
	skos:historyNote "Queensland Department of Resources. " ;
    skos:inScheme cs: ;
    skos:prefLabel "Corrective Services Act 2006 (Qld)"@en ;
    skos:topConceptOf cs: ;
    schema:citation "https://www.legislation.qld.gov.au/view/html/inforce/current/act-2006-029"^^xsd:anyURI ;
.

:qld-e-act-1992
    a skos:Concept ;
    rdfs:isDefinedBy cs: ;
    skos:definition "Naming of state electoral districts. Applies in Queensland."@en ;
	skos:historyNote "Queensland Department of Resources. " ;
    skos:inScheme cs: ;
    skos:prefLabel "Electoral Act 1992 (Qld)"@en ;
    skos:topConceptOf cs: ;
    schema:citation "https://www.legislation.qld.gov.au/view/html/inforce/current/act-1992-028"^^xsd:anyURI ;
.

:qld-egp-act-2006
    a skos:Concept ;
    rdfs:isDefinedBy cs: ;
    skos:definition "Naming of state educational institutions (including the provision of temporary names during planning and construction phase), school precincts and school buildings, sporting grounds and sporting facilities. Applies in Queensland."@en ;
	skos:historyNote "Queensland Department of Resources. " ;
    skos:inScheme cs: ;
    skos:prefLabel "Education (General Provisions) Act 2006 (Qld)"@en ;
    skos:topConceptOf cs: ;
    schema:citation "https://www.legislation.qld.gov.au/view/html/inforce/current/act-2006-039 https://ppr.qed.qld.gov.au/pp/naming-and-opening-of-departmental-assets-procedure"^^xsd:anyURI ;
.

:qld-f-act-1959
    a skos:Concept ;
    rdfs:isDefinedBy cs: ;
    skos:definition "Plans for timber reserves and state forests. Applies in Queensland."@en ;
	skos:historyNote "Queensland Department of Resources. " ;
    skos:inScheme cs: ;
    skos:prefLabel "Forestry Act 1959 (Qld)"@en ;
    skos:topConceptOf cs: ;
    schema:citation "https://www.legislation.qld.gov.au/view/html/inforce/current/act-1959-058"^^xsd:anyURI ;
.

:qld-fire
    a skos:Concept ;
    rdfs:isDefinedBy cs: ;
    skos:altLabel
        "QFD"@en ,
        "QFES"@en ;
    skos:definition "Naming of authorised entities and Fire Levy Districts by Queensland Fire Department. Applies in Queensland."@en ;
	skos:historyNote "Queensland Department of Resources. " ;
    skos:inScheme cs: ;
    skos:prefLabel "Queensland Fire Department"@en ;
    skos:topConceptOf cs: ;
    schema:citation "https://www.qfes.qld.gov.au/"^^xsd:anyURI ;
.

:qld-hans-2021
    a skos:Concept ;
    rdfs:isDefinedBy cs: ;
    skos:definition "Naming of hospitals and health facilities. Applies in Queensland."@en ;
	skos:historyNote "Queensland Department of Resources. " ;
    skos:inScheme cs: ;
    skos:prefLabel "Department of Health Asset Naming StandardÂ 2021"@en ;
    skos:topConceptOf cs: ;
    schema:citation "https://www.health.qld.gov.au/__data/assets/pdf_file/0013/1101280/qh-imp-485-1.pdf"^^xsd:anyURI ;
.

:qld-health
    a skos:Concept ;
    rdfs:isDefinedBy cs: ;
    skos:definition "Health Service Areas. Applies in Queensland."@en ;
	skos:historyNote "Queensland Department of Resources. " ;
    skos:inScheme cs: ;
    skos:prefLabel "Queensland Health"@en ;
    skos:topConceptOf cs: ;
    schema:citation "https://www.health.qld.gov.au/"^^xsd:anyURI ;
.

:qld-ird-act-1987
    a skos:Concept ;
    rdfs:isDefinedBy cs: ;
    skos:definition "Naming of entities under the Integrated Resort Development Act 1987. Applies in Queensland."@en ;
	skos:historyNote "Queensland Department of Resources. " ;
    skos:inScheme cs: ;
    skos:prefLabel "Integrated Resort Development Act 1987 (Qld)"@en ;
    skos:topConceptOf cs: ;
    schema:citation "https://www.legislation.qld.gov.au/view/html/inforce/current/act-1987-023"^^xsd:anyURI ;
.

:qld-lg-act-2009
    a skos:Concept ;
    rdfs:isDefinedBy cs: ;
    skos:definition "Naming of Local Government Areas and Divisions. Naming of entities under the control of local government e.g. road naming, street numbering, parks and public facilities, public areas, bridges and their infrastructure. Applies in Queensland."@en ;
	skos:historyNote "Queensland Department of Resources. " ;
    skos:inScheme cs: ;
    skos:prefLabel "Local Government Act 2009 (Qld)"@en ;
    skos:topConceptOf cs: ;
    schema:citation "https://www.legislation.qld.gov.au/view/html/inforce/current/act-2009-017"^^xsd:anyURI ;
.

:qld-lt-act-1994
    a skos:Concept ;
    rdfs:isDefinedBy cs: ;
    skos:definition "Naming of community title schemes. Applies in Queensland."@en ;
	skos:historyNote "Queensland Department of Resources. " ;
    skos:inScheme cs: ;
    skos:prefLabel "Land Title Act 1994 (Qld)"@en ;
    skos:topConceptOf cs: ;
    schema:citation "https://www.legislation.qld.gov.au/view/html/inforce/current/act-1994-011"^^xsd:anyURI ;
.

:qld-mp-act-2004
    a skos:Concept ;
    rdfs:isDefinedBy cs: ;
    skos:definition "Naming of marine parks. Applies in Queensland."@en ;
	skos:historyNote "Queensland Department of Resources. " ;
    skos:inScheme cs: ;
    skos:prefLabel "Marine Parks Act 2004 (Qld)"@en ;
    skos:topConceptOf cs: ;
    schema:citation "https://www.legislation.qld.gov.au/view/html/inforce/current/act-2004-031"^^xsd:anyURI ;
.

:qld-mud-act-1993
    a skos:Concept ;
    rdfs:isDefinedBy cs: ;
    skos:definition "Naming of entities under the Mixed Use Development Act 1993. Applies in Queensland."@en ;
	skos:historyNote "Queensland Department of Resources. " ;
    skos:inScheme cs: ;
    skos:prefLabel "Mixed Use Development Act 1993 (Qld)"@en ;
    skos:topConceptOf cs: ;
    schema:citation "https://www.legislation.qld.gov.au/view/html/inforce/current/act-1993-021"^^xsd:anyURI ;
.

:qld-nc-act-1992
    a skos:Concept ;
    rdfs:isDefinedBy cs: ;
    skos:definition "Naming of national parks, conservation parks, resources reserves, special wildlife reserves, nature refuges, coordinated conservation areas and Indigenous Joint Management Areas. Applies in Queensland."@en ;
	skos:historyNote "Queensland Department of Resources. " ;
    skos:inScheme cs: ;
    skos:prefLabel "Nature Conservation Act 1992 (Qld)"@en ;
    skos:topConceptOf cs: ;
    schema:citation "https://www.legislation.qld.gov.au/view/html/inforce/current/act-1992-020"^^xsd:anyURI ;
.

:qld-pn-act-1994
    a skos:Concept ;
    rdfs:isDefinedBy cs: ;
    skos:definition "Naming of aÂ place, described as an area or geographical feature (whether natural or artificial) other than an excluded place. Excluded places are a road within the meaning of theÂ Transport Operations (Road Use Management) Act 1995, a canal associated with a residential or commercial development, a building or similar structure, a dam wall or similar structure, a division or ward of a local government area, a place given a name under another law of the State or the Commonwealth such as a port, electoral district or local government areas, or any other place described by a regulation. For a place name to be entered into the Gazetteer of Place Names, the name must have been designated in accordance with the procedure prescribed in the Place Names Act 1994. Applies in Queensland."@en ;
	skos:historyNote "Queensland Department of Resources. " ;
    skos:inScheme cs: ;
    skos:prefLabel "Place Names Act 1994 (Qld)"@en ;
    skos:topConceptOf cs: ;
    schema:citation "https://www.legislation.qld.gov.au/view/html/inforce/current/act-1994-057"^^xsd:anyURI ;
.

:qld-police
    a skos:Concept ;
    rdfs:isDefinedBy cs: ;
    skos:altLabel "QPS"@en ;
    skos:definition "Naming of authorised entities by Queensland Police Service. Applies in Queensland."@en ;
	skos:historyNote "Queensland Department of Resources. " ;
    skos:inScheme cs: ;
    skos:prefLabel "Queensland Police Service"@en ;
    skos:topConceptOf cs: ;
.

:qld-qpws
    a skos:Concept ;
    rdfs:isDefinedBy cs: ;
    skos:altLabel "QPWS"@en ;
    skos:definition "Naming of a Queensland Parks and Wildlife Service (QPWS) managed area, place, site or geographical feature that does not fall under the Place Names Act 1994. Applies in Queensland."@en ;
	skos:historyNote "Queensland Department of Resources. " ;
    skos:inScheme cs: ;
    skos:prefLabel "Queensland Parks and Wildlife Service"@en ;
    skos:topConceptOf cs: ;
    schema:citation "https://parks.desi.qld.gov.au/ https://www.des.qld.gov.au/policies?a=272936:policy_registry/op-pk-nrm-naming-qpws-managed-areas-places-sites-features.pdf"^^xsd:anyURI ;
.

:qld-rail
    a skos:Concept ;
    rdfs:isDefinedBy cs: ;
    skos:altLabel "QR"@en ;
    skos:definition "Queensland Rail name railway infrastructure including stations and facilities, rolling stock, railway lines and rail services. Applies in Queensland."@en ;
	skos:historyNote "Queensland Department of Resources. " ;
    skos:inScheme cs: ;
    skos:prefLabel "Queensland Rail"@en ;
    skos:topConceptOf cs: ;
    schema:citation "https://www.queenslandrail.com.au/"^^xsd:anyURI ;
.

:qld-sbc-act-1989
    a skos:Concept ;
    rdfs:isDefinedBy cs: ;
    skos:definition "Naming streets, buildings, parks, and other significant structures within its area of control under the South Bank Corporation Act 1989, consistent with their management and developmental responsibilities. Applies in Queensland."@en ;
	skos:historyNote "Queensland Department of Resources. " ;
    skos:inScheme cs: ;
    skos:prefLabel "South Bank Corporation Act 1989 (Qld)"@en ;
    skos:topConceptOf cs: ;
    schema:citation "https://www.legislation.qld.gov.au/view/html/inforce/current/act-1989-037"^^xsd:anyURI ;
.

:qld-scr-act-1985
    a skos:Concept ;
    rdfs:isDefinedBy cs: ;
    skos:definition "Naming and numbering of roads within the Sanctuary Cove Resort area. Applies in Queensland."@en ;
	skos:historyNote "Queensland Department of Resources. " ;
    skos:inScheme cs: ;
    skos:prefLabel "Sanctuary Cove Resort Act 1985 (Qld)"@en ;
    skos:topConceptOf cs: ;
    schema:citation "https://www.legislation.qld.gov.au/view/html/inforce/current/act-1985-079"^^xsd:anyURI ;
.

:qld-stadiums
    a skos:Concept ;
    rdfs:isDefinedBy cs: ;
    skos:definition "Naming of major sports facilities. Applies in Queensland."@en ;
	skos:historyNote "Queensland Department of Resources. " ;
    skos:inScheme cs: ;
    skos:prefLabel "Stadiums Queensland"@en ;
    skos:topConceptOf cs: ;
    schema:citation "https://www.stadiums.qld.gov.au/"^^xsd:anyURI ;
.

:qld-teq
    a skos:Concept ;
    rdfs:isDefinedBy cs: ;
    skos:definition "Naming of tourism regions. Applies in Queensland."@en ;
	skos:historyNote "Queensland Department of Resources. " ;
    skos:inScheme cs: ;
    skos:prefLabel "Tourism and Events Queensland"@en ;
    skos:topConceptOf cs: ;
    schema:citation "https://teq.queensland.com/au/en/industry"^^xsd:anyURI ;
.

:qld-ti-act-1994
    a skos:Concept ;
    rdfs:isDefinedBy cs: ;
    skos:definition "Naming of Queensland state transport infrastructure including state-controlled roads & bridges, railways, public transport facilities, ports, airports, cycling and walking infrastructure, boat ramps and other marine infrastructure. Applies in Queensland."@en ;
	skos:historyNote "Queensland Department of Resources. " ;
    skos:inScheme cs: ;
    skos:prefLabel "Transport Infrastructure Act 1994 (Qld)"@en ;
    skos:topConceptOf cs: ;
    schema:citation "https://www.legislation.qld.gov.au/view/html/inforce/current/act-1994-008"^^xsd:anyURI ;
.

:qld-translink
    a skos:Concept ;
    rdfs:isDefinedBy cs: ;
    skos:definition "Naming of public transport services and infrastructure in the Translink area. Part of the Department of Transport and Main Roads in Queensland. Applies in Queensland."@en ;
	skos:historyNote "Queensland Department of Resources. " ;
    skos:inScheme cs: ;
    skos:prefLabel "Translink"@en ;
    skos:topConceptOf cs: ;
    schema:citation "https://translink.com.au/"^^xsd:anyURI ;
.

:state-other
    a skos:Concept ;
    rdfs:isDefinedBy cs: ;
    skos:definition "Another state authority with a naming role."@en ;
	skos:historyNote "Queensland Department of Resources. " ;
    skos:inScheme cs: ;
    skos:prefLabel "Other state authority"@en ;
    skos:topConceptOf cs: ;
.

:utility-provider
    a skos:Concept ;
    rdfs:isDefinedBy cs: ;
    skos:definition "Utility provider with a naming role."@en ;
	skos:historyNote "Queensland Department of Resources. " ;
    skos:inScheme cs: ;
    skos:prefLabel "Utility Provider"@en ;
    skos:topConceptOf cs: ;
.

:water-authority
    a skos:Concept ;
    rdfs:isDefinedBy cs: ;
    skos:definition "Water authority with a naming power, e.g. Seqwater and Sunwater have naming power for dams."@en ;
	skos:historyNote "Queensland Department of Resources. " ;
    skos:inScheme cs: ;
    skos:prefLabel "Water Authority"@en ;
    skos:topConceptOf cs: ;
.

cs:
    a skos:ConceptScheme ;
    owl:versionIRI :None ;
    skos:definition "This vocabulary describes the legal instrument under which, or agency with responsibility for, naming of a feature."@en ;
    skos:hasTopConcept
        :aus-hydrographic-office ,
        :aus-post ,
        :cth-cac-act ,
        :cth-ce-act-1918 ,
        :cth-epbc-act-1999 ,
        :gbrmpa ,
        :port-authority ,
        :private ,
        :qld-ambulance ,
        :qld-bccm-act-1997 ,
        :qld-caca-act-1957 ,
        :qld-cb-act-2010 ,
        :qld-cs-act-2006 ,
        :qld-e-act-1992 ,
        :qld-egp-act-2006 ,
        :qld-f-act-1959 ,
        :qld-fire ,
        :qld-hans-2021 ,
        :qld-health ,
        :qld-ird-act-1987 ,
        :qld-lg-act-2009 ,
        :qld-lt-act-1994 ,
        :qld-mp-act-2004 ,
        :qld-mud-act-1993 ,
        :qld-nc-act-1992 ,
        :qld-pn-act-1994 ,
        :qld-police ,
        :qld-qpws ,
        :qld-rail ,
        :qld-sbc-act-1989 ,
        :qld-scr-act-1985 ,
        :qld-stadiums ,
        :qld-teq ,
        :qld-ti-act-1994 ,
        :qld-translink ,
        :state-other ,
        :utility-provider ,
        :water-authority ;
    skos:historyNote "This vocabulary contains naming authorities identified in relation to geographic names and addresses in Queensland. "@en ;
    skos:prefLabel "Naming Authority"@en ;
    prov:qualifiedAttribution
        [
            dcat:hadRole isoroles:custodian ;
            prov:agent
                [
                    a schema:Person ;
                    schema:email ""^^xsd:anyURI ;
                    schema:name "Icsm" ;
                ] ;
        ] ;
    schema:creator
        [
            a schema:Organization ;
            schema:name "Department Of Resources, Qld" ;
            schema:url ""^^xsd:anyURI ;
        ] ;
    dcterms:created "2023-06-03"^^xsd:date ;
	dcterms:modified "2024-08-01"^^xsd:date ;
    schema:publisher
        [
            a schema:Organization ;
            schema:name "Department Of Resources, Qld" ;
            schema:url ""^^xsd:anyURI ;
        ] ;
    schema:version "None" ;
.
