PREFIX : <https://linked.data.gov.au/def/positional-accuracy/>
PREFIX agldwgstatus: <https://linked.data.gov.au/def/reg-statuses/>
PREFIX cs: <https://linked.data.gov.au/def/positional-accuracy>
PREFIX dcterms: <http://purl.org/dc/terms/>
PREFIX droles: <https://linked.data.gov.au/def/data-roles/>
PREFIX owl: <http://www.w3.org/2002/07/owl#>
PREFIX prov: <http://www.w3.org/ns/prov#>
PREFIX reg: <http://purl.org/linked-data/registry#>
PREFIX sdo: <https://schema.org/>
PREFIX skos: <http://www.w3.org/2004/02/skos/core#>
PREFIX themes: <https://linked.data.gov.au/def/fsdf/themes/>
PREFIX xsd: <http://www.w3.org/2001/XMLSchema#>

:100m
    a skos:Concept ;
    skos:altLabel "Remote"@en ;
    skos:definition "Minimum spatial accuracy of plus or minus 100 metres. Typically remote area capture"@en ;
    skos:historyNote "Queensland Roads and Tracks dataset, influenced by the Queensland Spatial Information Council Digital Road Network Standard." ;
    skos:inScheme cs: ;
    skos:prefLabel "100m"@en ;
.

:25m
    a skos:Concept ;
    skos:altLabel "Rural"@en ;
    skos:definition "Minimum spatial accuracy of plus or minus 25 metres. Typically rural capture"@en ;
    skos:historyNote "Queensland Roads and Tracks dataset, influenced by the Queensland Spatial Information Council Digital Road Network Standard." ;
    skos:inScheme cs: ;
    skos:prefLabel "25m"@en ;
.

:2m
    a skos:Concept ;
    skos:altLabel "Urban"@en ;
    skos:definition "Minimum spatial accuracy of plus or minus 2 metres. Typically urban capture"@en ;
    skos:historyNote "Queensland Roads and Tracks dataset, influenced by the Queensland Spatial Information Council Digital Road Network Standard." ;
    skos:inScheme cs: ;
    skos:prefLabel "2m"@en ;
.

:5m
    a skos:Concept ;
    skos:altLabel "Peri-Urban"@en ;
    skos:definition "Minimum spatial accuracy of plus or minus 5 metres. Typically peri-urban capture"@en ;
    skos:historyNote "Queensland Roads and Tracks dataset, influenced by the Queensland Spatial Information Council Digital Road Network Standard." ;
    skos:inScheme cs: ;
    skos:prefLabel "5m"@en ;
.

:unknown
    a skos:Concept ;
    skos:altLabel "U"@en ;
    skos:definition "Minimum spatial accuracy unknown"@en ;
    skos:historyNote "Queensland Roads and Tracks dataset, influenced by the Queensland Spatial Information Council Digital Road Network Standard." ;
    skos:inScheme cs: ;
    skos:prefLabel "Unknown"@en ;
.

<https://linked.data.gov.au/org/qsi>
    a sdo:Organization ;
    sdo:name "Queensland Spatial Information" ;
    sdo:url "https://www.resources.qld.gov.au/data-mapping"^^xsd:anyURI ;
.

<https://linked.data.gov.au/org/icsm>
    a sdo:Organization ;
    sdo:name "Intergovernmental Committee on Surveying & Mapping" ;
    sdo:url "https://icsm.gov.au"^^xsd:anyURI ;
.

cs:
    a skos:ConceptScheme ;
    sdo:keywords themes:positioning ;
    dcterms:created "2023-05-31"^^xsd:date ;
    dcterms:creator <https://linked.data.gov.au/org/qsi> ;
    dcterms:identifier "positional-accuracy"^^xsd:token ;
    dcterms:modified "2023-11-30"^^xsd:date ;
    dcterms:publisher <https://linked.data.gov.au/org/icsm> ;
    reg:status agldwgstatus:experimental ;
    owl:versionIRI :1.0 ;
    owl:versionInfo "1.0" ;
    skos:definition "This vocabulary describes categories of positional accuracy information to indicate the spatial accuracy of data capture. "@en ;
    skos:hasTopConcept
        :100m ,
        :25m ,
        :2m ,
        :5m ,
        :unknown ;
    skos:historyNote "This vocabulary was created by the Queensland Spatial Information services." ;
    skos:prefLabel "Positional Accuracy"@en ;
    prov:qualifiedAttribution
        [
            prov:hadRole droles:custodian ;
            prov:agent <https://linked.data.gov.au/org/icsm>
        ] ;
.

