PREFIX : <https://linked.data.gov.au/def/lrrs-indicator/>
PREFIX agldwgstatus: <https://linked.data.gov.au/def/reg-statuses/>
PREFIX cs: <https://linked.data.gov.au/def/lrrs-indicator>
PREFIX dcterms: <http://purl.org/dc/terms/>
PREFIX droles: <https://linked.data.gov.au/def/data-roles/>
PREFIX owl: <http://www.w3.org/2002/07/owl#>
PREFIX prov: <http://www.w3.org/ns/prov#>
PREFIX reg: <http://purl.org/linked-data/registry#>
PREFIX sdo: <https://schema.org/>
PREFIX skos: <http://www.w3.org/2004/02/skos/core#>
PREFIX themes: <https://linked.data.gov.au/def/fsdf/themes/>
PREFIX xsd: <http://www.w3.org/2001/XMLSchema#>

:local-road-of-regional-significance
    a skos:Concept ;
    skos:altLabel
        "T"@en ,
        "True"@en ;
    skos:definition "Road is designated as a Local Road of Regional Significance"@en ;
    skos:historyNote "Queensland Roads and Tracks dataset" ;
    skos:inScheme cs: ;
    skos:prefLabel "Local Road of Regional Significance"@en ;
.

:not-local-road-of-regional-significance
    a skos:Concept ;
    skos:altLabel
        "F"@en ,
        "False"@en ;
    skos:definition "Road is not designated as a Local Road of Regional Significance"@en ;
    skos:historyNote "Queensland Roads and Tracks dataset" ;
    skos:inScheme cs: ;
    skos:prefLabel "Not Local Road of Regional Significance"@en ;
.

:unknown
    a skos:Concept ;
    skos:altLabel "U"@en ;
    skos:definition "Unknown - It is not known if the road is designated as a Local Road of Regional Significance"@en ;
    skos:historyNote "Queensland Roads and Tracks dataset" ;
    skos:inScheme cs: ;
    skos:prefLabel "Unknown"@en ;
.

<https://linked.data.gov.au/org/qsi>
    a sdo:Organization ;
    sdo:name "Queensland Spatial Information" ;
    sdo:url "https://www.resources.qld.gov.au/data-mapping"^^xsd:anyURI ;
.

cs:
    a skos:ConceptScheme ;
    sdo:keywords themes:transport ;
    dcterms:created "2023-05-31"^^xsd:date ;
    dcterms:creator <https://linked.data.gov.au/org/qsi> ;
    dcterms:identifier "lrrs-indicator"^^xsd:token ;
    dcterms:modified "2023-11-30"^^xsd:date ;
    dcterms:publisher <https://linked.data.gov.au/org/icsm> ;
    reg:status agldwgstatus:experimental ;
    owl:versionIRI :1.0 ;
    owl:versionInfo "1.0" ;
    skos:definition "This vocabulary describes whether a road is designated as a local road of regional significance (LRSS)"@en ;
    skos:hasTopConcept
        :local-road-of-regional-significance ,
        :not-local-road-of-regional-significance ,
        :unknown ;
    skos:historyNote "This vocabulary was created by the Queensland Spatial Information services." ;
    skos:prefLabel "Local Road of Regional Significance Indicator"@en ;
    prov:qualifiedAttribution
        [
            prov:hadRole droles:custodian ;
            prov:agent <https://linked.data.gov.au/org/icsm>
        ] ;
.

<https://linked.data.gov.au/org/icsm>
    a sdo:Organization ;
    sdo:name "Intergovernmental Committee on Surveying & Mapping" ;
    sdo:url "https://icsm.gov.au"^^xsd:anyURI ;
.

