PREFIX : <https://linked.data.gov.au/def/spatial-capture-method/>
PREFIX agldwgstatus: <https://linked.data.gov.au/def/reg-statuses/>
PREFIX cs: <https://linked.data.gov.au/def/spatial-capture-method>
PREFIX dcterms: <http://purl.org/dc/terms/>
PREFIX droles: <https://linked.data.gov.au/def/data-roles/>
PREFIX owl: <http://www.w3.org/2002/07/owl#>
PREFIX prov: <http://www.w3.org/ns/prov#>
PREFIX reg: <http://purl.org/linked-data/registry#>
PREFIX sdo: <https://schema.org/>
PREFIX skos: <http://www.w3.org/2004/02/skos/core#>
PREFIX themes: <https://linked.data.gov.au/def/fsdf/themes/>
PREFIX xsd: <http://www.w3.org/2001/XMLSchema#>

:cadastre
    a skos:Concept ;
    skos:definition "Spatial feature has been derived from cadastral information. "@en ;
    skos:historyNote "Queensland Roads and Tracks dataset" ;
    skos:inScheme cs: ;
    skos:prefLabel "Cadastre"@en ;
.

:estimate
    a skos:Concept ;
    skos:definition "Spatial feature has been estimated. "@en ;
    skos:historyNote "Queensland Roads and Tracks dataset" ;
    skos:inScheme cs: ;
    skos:prefLabel "Estimate"@en ;
.

:gps
    a skos:Concept ;
    skos:definition "Spatial feature has been derived using Global Positioning System (GPS) data. "@en ;
    skos:historyNote "Queensland Roads and Tracks dataset" ;
    skos:inScheme cs: ;
    skos:prefLabel "GPS"@en ;
.

:imagery-automated
    a skos:Concept ;
    skos:definition "Spatial feature has been extracted from imagery. "@en ;
    skos:historyNote "Queensland Roads and Tracks dataset" ;
    skos:inScheme cs: ;
    skos:prefLabel "Imagery automated"@en ;
.

:imagery-manual
    a skos:Concept ;
    skos:definition "Spatial feature has been digitised from imagery. "@en ;
    skos:historyNote "Queensland Roads and Tracks dataset" ;
    skos:inScheme cs: ;
    skos:prefLabel "Imagery manual"@en ;
.

:map-digitised
    a skos:Concept ;
    skos:definition "Spatial feature has been digitised from a scanned map. "@en ;
    skos:historyNote "Queensland Roads and Tracks dataset" ;
    skos:inScheme cs: ;
    skos:prefLabel "Map digitised"@en ;
.

:non-spatial
    a skos:Concept ;
    skos:definition "Spatial feature has been digitised from a non spatial entity such as a scanned map. "@en ;
    skos:historyNote "Queensland Roads and Tracks dataset" ;
    skos:inScheme cs: ;
    skos:prefLabel "Non spatial"@en ;
.

:other
    a skos:Concept ;
    skos:definition "Spatial feature has been created from another spatial source. "@en ;
    skos:historyNote "Queensland Roads and Tracks dataset" ;
    skos:inScheme cs: ;
    skos:prefLabel "Other"@en ;
.

:survey-data
    a skos:Concept ;
    skos:definition "Spatial feature has been digitised from engineering/survey data. "@en ;
    skos:historyNote "Queensland Roads and Tracks dataset" ;
    skos:inScheme cs: ;
    skos:prefLabel "Survey data"@en ;
.

:unknown
    a skos:Concept ;
    skos:definition "Spatial feature has an unknown source. "@en ;
    skos:historyNote "Queensland Roads and Tracks dataset" ;
    skos:inScheme cs: ;
    skos:prefLabel "Unknown"@en ;
.

<https://linked.data.gov.au/org/qsi>
    a sdo:Organization ;
    sdo:name "Queensland Spatial Information" ;
    sdo:url "https://www.resources.qld.gov.au/data-mapping"^^xsd:anyURI ;
.

<https://linked.data.gov.au/org/icsm>
    a sdo:Organization ;
    sdo:name "Intergovernmental Committee on Surveying & Mapping" ;
    sdo:url "https://icsm.gov.au"^^xsd:anyURI ;
.

cs:
    a skos:ConceptScheme ;
    sdo:keywords themes:spatial ;
    dcterms:created "2023-05-30"^^xsd:date ;
    dcterms:creator <https://linked.data.gov.au/org/qsi> ;
    dcterms:identifier "spatial-capture-method"^^xsd:token ;
    dcterms:modified "2023-11-30"^^xsd:date ;
    dcterms:publisher <https://linked.data.gov.au/org/icsm> ;
    reg:status agldwgstatus:experimental ;
    owl:versionIRI :1.0 ;
    owl:versionInfo "1.0" ;
    skos:definition "This vocabulary describes the method in which geometry was captured. "@en ;
    skos:hasTopConcept
        :cadastre ,
        :estimate ,
        :gps ,
        :imagery-automated ,
        :imagery-manual ,
        :map-digitised ,
        :non-spatial ,
        :other ,
        :survey-data ,
        :unknown ;
    skos:historyNote "This vocabulary was created by the Queensland Spatial Information services." ;
    skos:prefLabel "Spatial capture method"@en ;
    prov:qualifiedAttribution
        [
            prov:hadRole droles:custodian ;
            prov:agent <https://linked.data.gov.au/org/icsm>
        ] ;
.

