@prefix dc: <http://purl.org/dc/elements/1.1/> .
@prefix dcterms: <http://purl.org/dc/terms/> .
@prefix owl: <http://www.w3.org/2002/07/owl#> .
@prefix sdo: <https://schema.org/> .
@prefix skos: <http://www.w3.org/2004/02/skos/core#> .
@prefix bhfunc: <https://linked.data.gov.au/def/borehole-sub-purpose/> .
@prefix xsd: <http://www.w3.org/2001/XMLSchema#> .

<https://linked.data.gov.au/def/borehole-sub-purpose> a owl:Ontology,
        skos:ConceptScheme ;
    dcterms:created "2020-01-23"^^xsd:date ;
    dcterms:creator <https://linked.data.gov.au/org/gsq> ;
    dcterms:publisher <https://linked.data.gov.au/org/gsq> ;
    dcterms:modified "2020-10-14"^^xsd:date ;
    dcterms:provenance "Compiled by the Geological Survey of Queensland" ;
    skos:definition "The intended function of a borehole."@en ;
    skos:hasTopConcept bhfunc:blasthole,
        bhfunc:disposal,
        bhfunc:environmental,
        bhfunc:gas-management,
        bhfunc:geotech,
        bhfunc:observation,
        bhfunc:petroleum-injection,
        bhfunc:petroleum-production,
        bhfunc:resource-assessment,
        bhfunc:service,
        bhfunc:stimulation,
        bhfunc:stratigraphic,
        bhfunc:investigation,
        bhfunc:structure,
        bhfunc:water-injection,
        bhfunc:water-supply ;
    skos:prefLabel "Borehole Sub-Purpose"@en .

<https://linked.data.gov.au/org/gsq> a sdo:Organization ;
    sdo:name "Geological Survey of Queensland" ;
    sdo:url <https://www.business.qld.gov.au/industries/mining-energy-water/resources/geoscience-information/gsq> .

bhfunc:acid-leachate-testing a skos:Concept ;
    skos:broader bhfunc:environmental ;
    skos:definition "A well or bore drilled to recover strata samples for their use in acid leachate testing."@en ;
    skos:inScheme <https://linked.data.gov.au/def/borehole-sub-purpose> ;
    skos:prefLabel "acid leachate testing"@en .

bhfunc:ballast a skos:Concept ;
    skos:broader bhfunc:service ;
    skos:definition "A well or bore through which ballast is transported to and from mine workings."@en ;
    skos:inScheme <https://linked.data.gov.au/def/borehole-sub-purpose> ;
    skos:prefLabel "ballast"@en .

bhfunc:cement a skos:Concept ;
    skos:broader bhfunc:service ;
    skos:definition "A well or bore through which cement is transported to and from mine workings."@en ;
    skos:inScheme <https://linked.data.gov.au/def/borehole-sub-purpose> ;
    skos:prefLabel "cement"@en .

bhfunc:chemical-flood a skos:Concept ;
    skos:broader bhfunc:stimulation ;
    skos:definition "The introduction of chemicals to either increase the receptiveness of a petroleum system to other improved recovery techniques, or to improve recovery in its own right."@en ;
    skos:inScheme <https://linked.data.gov.au/def/borehole-sub-purpose> ;
    skos:prefLabel "Chemical Flood"@en .

bhfunc:compliance-gas-testing a skos:Concept ;
    skos:broader bhfunc:gas-management ;
    skos:definition "Gas content testing in drainage areas to ensure remaining gas content is below the mining threshold."@en ;
    skos:inScheme <https://linked.data.gov.au/def/borehole-sub-purpose> ;
    skos:prefLabel "compliance gas testing"@en .

bhfunc:controlled-pressure-well a skos:Concept ;
    skos:broader bhfunc:gas-management ;
    skos:definition "A well drilled to provide a mechanism for the control of pressure in a system."@en ;
    skos:inScheme <https://linked.data.gov.au/def/borehole-sub-purpose> ;
    skos:prefLabel "controlled pressure well"@en .

bhfunc:electricity a skos:Concept ;
    skos:broader bhfunc:service ;
    skos:definition "A well or bore through which electricity is provided to mine workings."@en ;
    skos:inScheme <https://linked.data.gov.au/def/borehole-sub-purpose> ;
    skos:prefLabel "electricity"@en .

bhfunc:end-of-borehole-well a skos:Concept ;
    skos:broader bhfunc:gas-management ;
    skos:definition "A well drilled to be intersected by a ranging well."@en ;
    skos:inScheme <https://linked.data.gov.au/def/borehole-sub-purpose> ;
    skos:prefLabel "end of borehole well"@en .

bhfunc:extensometer a skos:Concept ;
    skos:broader bhfunc:geotech ;
    skos:definition "A well or bore drilled to facilitate strain measurements and tensile tests through the use of an extensometer."@en ;
    skos:inScheme <https://linked.data.gov.au/def/borehole-sub-purpose> ;
    skos:prefLabel "extensometer"@en .

bhfunc:fault-delineation a skos:Concept ;
    skos:broader bhfunc:structure ;
    skos:definition "Borehole drilled to define a fault structure."@en ;
    skos:inScheme <https://linked.data.gov.au/def/borehole-sub-purpose> ;
    skos:prefLabel "fault delineation"@en .

bhfunc:fire-flood a skos:Concept ;
    skos:broader bhfunc:stimulation ;
    skos:definition "The ignition of a petroleum system to inject heat, improving recovery through the reduction of viscosity, displacement by combustion products and more beneficial pressure gradients."@en ;
    skos:inScheme <https://linked.data.gov.au/def/borehole-sub-purpose> ;
    skos:prefLabel "Fire Flood"@en .

bhfunc:gas-drainage-undifferentiated a skos:Concept ;
    skos:broader bhfunc:gas-management ;
    skos:definition "A well or bore drilled to remove gas from a subsurface system without any intent for commercialisation."@en ;
    skos:inScheme <https://linked.data.gov.au/def/borehole-sub-purpose> ;
    skos:prefLabel "gas drainage undifferentiated"@en .

bhfunc:gas-flood a skos:Concept ;
    skos:broader bhfunc:stimulation ;
    skos:definition "The introduction of a gas to a petroleum system to improve recovery through displacement and more beneficial pressure gradients."@en ;
    skos:inScheme <https://linked.data.gov.au/def/borehole-sub-purpose> ;
    skos:prefLabel "Gas Flood"@en .

bhfunc:geotechnical-properties a skos:Concept ;
    skos:broader bhfunc:geotech ;
    skos:definition "A borehole drilled to obtain strata core for geotechnical rock property testing."@en ;
    skos:inScheme <https://linked.data.gov.au/def/borehole-sub-purpose> ;
    skos:prefLabel "geotechnical properties"@en .

bhfunc:goaf-drainage a skos:Concept ;
    skos:broader bhfunc:gas-management ;
    skos:definition "A well or bore drilled to remove fluids and or dangerous gases from the goaf."@en ;
    skos:inScheme <https://linked.data.gov.au/def/borehole-sub-purpose> ;
    skos:prefLabel "goaf drainage"@en .

bhfunc:heat-flow a skos:Concept ;
    skos:altLabel "Heat flow"@en ;
    skos:broader bhfunc:resource-assessment ;
    skos:definition "purposely drilled to directly measure downhole temperature gradient as well as collecting core samples (to measure thermal conductivity of formations intersected), then to be able to calculate / determine heat flow in the drilled section of the borehole."@en ;
    skos:inScheme <https://linked.data.gov.au/def/borehole-sub-purpose> ;
    skos:prefLabel "Geothermal heat flow"@en .

bhfunc:intrusion-delineation a skos:Concept ;
    skos:broader bhfunc:structure ;
    skos:definition "Borehole drilled to define an intrusion."@en ;
    skos:inScheme <https://linked.data.gov.au/def/borehole-sub-purpose> ;
    skos:prefLabel "intrusion delineation"@en .

bhfunc:large-diameter a skos:Concept ;
    skos:broader bhfunc:coal-quality ;
    skos:definition "Large diameter tests for coal physical properties and washability"@en ;
    skos:inScheme <https://linked.data.gov.au/def/borehole-sub-purpose> ;
    skos:prefLabel "large diameter"@en .

bhfunc:limit-of-oxidation a skos:Concept ;
    skos:broader bhfunc:resource-assessment ;
    skos:definition "Borehole drilled to obtain samples to determine the amount of oxidation of any coal seam by either visual and tactile or coal analysis methods."@en ;
    skos:inScheme <https://linked.data.gov.au/def/borehole-sub-purpose> ;
    skos:notation "LOX" ;
    skos:prefLabel "Limit of Oxidation"@en .

bhfunc:mineral-ore-body-assessment a skos:Concept ;
    skos:broader bhfunc:resource-assessment ;
    skos:definition "A well drilled to delineate a mineral ore deposit and/or define physical properties such as grade and quality"@en ;
    skos:inScheme <https://linked.data.gov.au/def/borehole-sub-purpose> ;
    skos:prefLabel "Mineral Ore Body Assessment"@en .

bhfunc:multi-channel-vibrating-wire-piezometer a skos:Concept ;
    skos:broader bhfunc:observation ;
    skos:definition "A well or bore drilled to provide a location in which Multi-Channel Vibrating Wire Piezometer can be used to register changes in fluid pressure."@en ;
    skos:inScheme <https://linked.data.gov.au/def/borehole-sub-purpose> ;
    skos:prefLabel "multi-channel vibrating wire piezometer"@en .

bhfunc:nested-standpipe-piezometer a skos:Concept ;
    skos:broader bhfunc:observation ;
    skos:definition "A well or bore drilled to provide a location in which Nested Standpipe Piezometer can be used to register changes in fluid pressure."@en ;
    skos:inScheme <https://linked.data.gov.au/def/borehole-sub-purpose> ;
    skos:prefLabel "nested standpipe piezometer"@en .

bhfunc:nitrogen a skos:Concept ;
    skos:broader bhfunc:service ;
    skos:definition "A well or bore through which nitrogen is transported to and from mine workings."@en ;
    skos:inScheme <https://linked.data.gov.au/def/borehole-sub-purpose> ;
    skos:prefLabel "nitrogen"@en .

bhfunc:penetrometer a skos:Concept ;
    skos:broader bhfunc:geotech ;
    skos:definition "A well or bore drilled to facilitate strength measurements through the use of a penetrometer."@en ;
    skos:inScheme <https://linked.data.gov.au/def/borehole-sub-purpose> ;
    skos:prefLabel "penetrometer"@en .

bhfunc:petroleum-reservoir-characterisation a skos:Concept ;
    skos:broader bhfunc:resource-assessment ;
    skos:definition "A well drilled to determine how to develop a hydrocarbon field most efficiently or quantify reservoir characteristics such as pay zone thickness, porosity, permeability, saturation, fluid column heights, and the presence of cap rock. Most commonly associated with the Appraisal stage of the resource lifecycle."@en ;
    skos:inScheme <https://linked.data.gov.au/def/borehole-sub-purpose> ;
    skos:prefLabel "Petroleum Resource Characterisation"@en .

bhfunc:petroleum-prod-test a skos:Concept ;
    skos:broader bhfunc:resource-assessment ;
    skos:definition "A well drilled primarily to test the ability of a target reservoir to  produce hydrocarbons, and to measure production parameters such as flow rates, well interference, pressure decline etc."@en ;
    skos:inScheme <https://linked.data.gov.au/def/borehole-sub-purpose> ;
    skos:prefLabel "Petroleum Production Testing"@en .

bhfunc:plug a skos:Concept ;
    skos:broader bhfunc:service ;
    skos:definition "Plug hole"@en ;
    skos:inScheme <https://linked.data.gov.au/def/borehole-sub-purpose> ;
    skos:prefLabel "plug"@en .

bhfunc:primary-hydraulic-fracturing a skos:Concept ;
    skos:broader bhfunc:geotech ;
    skos:definition "A well or bore drilled to facilitate the introduction of a liquid solution to a system, under significant pressure, to introduce fractures into strata."@en ;
    skos:inScheme <https://linked.data.gov.au/def/borehole-sub-purpose> ;
    skos:prefLabel "primary hydraulic fracturing"@en .

bhfunc:ranging-well a skos:Concept ;
    skos:broader bhfunc:gas-management ;
    skos:definition "A well drilled to intersect with another well."@en ;
    skos:inScheme <https://linked.data.gov.au/def/borehole-sub-purpose> ;
    skos:prefLabel "ranging well"@en .

bhfunc:refuge a skos:Concept ;
    skos:broader bhfunc:service ;
    skos:definition "A well or bore which provides access to, for ventilation or rescue, a refuge."@en ;
    skos:inScheme <https://linked.data.gov.au/def/borehole-sub-purpose> ;
    skos:prefLabel "refuge"@en .

bhfunc:slim-core-testing a skos:Concept ;
    skos:broader bhfunc:coal-quality ;
    skos:definition "Slim core testing for basic coal quality"@en ;
    skos:inScheme <https://linked.data.gov.au/def/borehole-sub-purpose> ;
    skos:prefLabel "slim core testing"@en .

bhfunc:spontaneous-combustion-testing a skos:Concept ;
    skos:broader bhfunc:coal-quality ;
    skos:definition "Borehole Drilled to obtains samples for spontaneous combustion testing"@en ;
    skos:inScheme <https://linked.data.gov.au/def/borehole-sub-purpose> ;
    skos:prefLabel "spontaneous combustion testing"@en .

bhfunc:standpipe-piezometer a skos:Concept ;
    skos:broader bhfunc:observation ;
    skos:definition "A well or bore drilled to provide a location in which Standpipe Piezometer can be used to register changes in fluid pressure."@en ;
    skos:inScheme <https://linked.data.gov.au/def/borehole-sub-purpose> ;
    skos:prefLabel "standpipe piezometer"@en .

bhfunc:steam-flood a skos:Concept ;
    skos:altLabel "CSS"@en,
        "Cyclic Steam Stimulation"@en,
        "SAGD"@en,
        "Steam Assisted Gravity Drainage"@en ;
    skos:broader bhfunc:stimulation ;
    skos:definition "The injection of steam into a petroleum system to improve recovery through the reduction of viscosity, displacement and more beneficial pressure gradients."@en ;
    skos:inScheme <https://linked.data.gov.au/def/borehole-sub-purpose> ;
    skos:prefLabel "Steam Flood"@en .

bhfunc:stone-dust a skos:Concept ;
    skos:broader bhfunc:service ;
    skos:definition "A well or bore through which stone dust is transported to and from mine workings."@en ;
    skos:inScheme <https://linked.data.gov.au/def/borehole-sub-purpose> ;
    skos:prefLabel "stone dust"@en .

bhfunc:stress-test-cell-over-stress-overcore a skos:Concept ;
    skos:broader bhfunc:geotech ;
    skos:definition "A well or bore drilled to facilitate the installation and subsequent retrieval of (Through overcoring) a stress cell."@en ;
    skos:inScheme <https://linked.data.gov.au/def/borehole-sub-purpose> ;
    skos:prefLabel "stress test cell / stress overcore"@en .

bhfunc:stygofauna-monitoring a skos:Concept ;
    skos:broader bhfunc:environmental ;
    skos:definition "A well or bore drilled to facilitate the monitoring of the population, biodiversity and overall 'health' parameters of stygofauna."@en ;
    skos:inScheme <https://linked.data.gov.au/def/borehole-sub-purpose> ;
    skos:prefLabel "stygofauna monitoring"@en .

bhfunc:surface-to-in-seam-well a skos:Concept ;
    skos:broader bhfunc:petroleum-production ;
    skos:definition "A well drilled to laterally intersect and drain hydrocarbons from a subsurface system."@en ;
    skos:inScheme <https://linked.data.gov.au/def/borehole-sub-purpose> ;
    skos:prefLabel "surface to in-seam well"@en .

bhfunc:tiltmeter a skos:Concept ;
    skos:broader bhfunc:geotech ;
    skos:definition "A well or bore drilled to facilitate the installation of a tiltmeter."@en ;
    skos:inScheme <https://linked.data.gov.au/def/borehole-sub-purpose> ;
    skos:prefLabel "tiltmeter"@en .

bhfunc:underground-in-seam-gas-riser a skos:Concept ;
    skos:broader bhfunc:gas-management ;
    skos:definition "A well drilled to improve the transport of gas away from a coal seam."@en ;
    skos:inScheme <https://linked.data.gov.au/def/borehole-sub-purpose> ;
    skos:prefLabel "underground in-seam gas-riser"@en .

bhfunc:vertical-production-well a skos:Concept ;
    skos:broader bhfunc:petroleum-production ;
    skos:definition "A vertical well drilled to drain hydrocarbons from a subsurface system."@en ;
    skos:inScheme <https://linked.data.gov.au/def/borehole-sub-purpose> ;
    skos:prefLabel "vertical production well"@en .

bhfunc:vibrating-wire-piezometer a skos:Concept ;
    skos:broader bhfunc:observation ;
    skos:definition "A well or bore drilled to provide a location in which Vibrating Wire Piezometer can be used to register changes in fluid pressure."@en ;
    skos:inScheme <https://linked.data.gov.au/def/borehole-sub-purpose> ;
    skos:prefLabel "vibrating wire piezometer"@en .

bhfunc:virgin-gas-testing a skos:Concept ;
    skos:broader bhfunc:gas-management ;
    skos:definition "Gas content testing in areas not subject to gas drainage."@en ;
    skos:inScheme <https://linked.data.gov.au/def/borehole-sub-purpose> ;
    skos:prefLabel "virgin gas testing"@en .

bhfunc:water-flood a skos:Concept ;
    skos:broader bhfunc:stimulation ;
    skos:definition "The introduction of liquid water to a petroleum system to improve recovery through displacement and more beneficial pressure gradients."@en ;
    skos:inScheme <https://linked.data.gov.au/def/borehole-sub-purpose> ;
    skos:prefLabel "Water Flood"@en .

bhfunc:blasthole a skos:Concept ;
    skos:definition "A well or bore drilled to facilitate the installation and subsequent detonation of explosives, pulverising material and throwing it away from the wall or face, reducing the effort required to advance the face or recover and remove materials."@en ;
    skos:inScheme <https://linked.data.gov.au/def/borehole-sub-purpose> ;
    skos:prefLabel "Blasthole"@en ;
    skos:topConceptOf <https://linked.data.gov.au/def/borehole-sub-purpose> .

bhfunc:disposal a skos:Concept ;
    skos:definition "A well in which fluids are injected rather than produced, where the primary objective is to dispose of fluid into an isolated formation."@en ;
    skos:inScheme <https://linked.data.gov.au/def/borehole-sub-purpose> ;
    skos:prefLabel "Disposal"@en ;
    skos:topConceptOf <https://linked.data.gov.au/def/borehole-sub-purpose> .

bhfunc:petroleum-injection a skos:Concept ;
    skos:altLabel "Petroleum Storage"@en ;
    skos:definition "A well in which hydrocarbons are injected rather than produced, the primary objective typically to store gas in a high quality reservoir for later production to maintain consistent rates of gas supply."@en ;
    skos:inScheme <https://linked.data.gov.au/def/borehole-sub-purpose> ;
    skos:prefLabel "Petroleum Injection"@en ;
    skos:topConceptOf <https://linked.data.gov.au/def/borehole-sub-purpose> .

bhfunc:stratigraphic a skos:Concept ;
    skos:definition "A well determining the lithological intervals present at a location. Typically to determine on the presence, location and extent of a potential resource. Most commonly associated with the Exploration stage of the resource lifecycle."@en ;
    skos:inScheme <https://linked.data.gov.au/def/borehole-sub-purpose> ;
    skos:notation "STRAT" ;
    skos:prefLabel "Stratigraphic"@en ;
    skos:topConceptOf <https://linked.data.gov.au/def/borehole-sub-purpose> .

bhfunc:investigation a skos:Concept ;
    skos:definition "A well drilled with scant or nil prior knowledge of the geology of an area to identify the presence of any lithologic, structural, hydrological, geochemical, or other geologic properties of interest."@en ;
    skos:inScheme <https://linked.data.gov.au/def/borehole-sub-purpose> ;
    skos:prefLabel "Investigation"@en ;
    skos:topConceptOf <https://linked.data.gov.au/def/borehole-sub-purpose> .

bhfunc:water-injection a skos:Concept ;
    skos:altLabel "Water Storage"@en ;
    skos:definition "A well in which water is injected rather than produced, where the primary objective is to store water in a reservoir or aquifer for later production."@en ;
    skos:inScheme <https://linked.data.gov.au/def/borehole-sub-purpose> ;
    skos:prefLabel "Water Injection"@en ;
    skos:topConceptOf <https://linked.data.gov.au/def/borehole-sub-purpose> .

bhfunc:water-supply a skos:Concept ;
    skos:altLabel "Production Water Bore"@en,
        "Water Production"@en ;
    skos:definition "A well drilled to drain water from an aquifer."@en ;
    skos:inScheme <https://linked.data.gov.au/def/borehole-sub-purpose> ;
    skos:prefLabel "Water Supply"@en ;
    skos:topConceptOf <https://linked.data.gov.au/def/borehole-sub-purpose> .

bhfunc:coal-quality a skos:Concept ;
    skos:broader bhfunc:resource-assessment ;
    skos:definition "Borehole drilled to obtain samples for laboratory testing and coal analysis."@en ;
    skos:inScheme <https://linked.data.gov.au/def/borehole-sub-purpose> ;
    skos:prefLabel "Coal Quality"@en .

bhfunc:environmental a skos:Concept ;
    skos:definition "Borehole drilled to obtain samples of strata for laboratory analysis of parameters which may impact on the environment."@en ;
    skos:inScheme <https://linked.data.gov.au/def/borehole-sub-purpose> ;
    skos:prefLabel "Environmental"@en ;
    skos:topConceptOf <https://linked.data.gov.au/def/borehole-sub-purpose> .

bhfunc:petroleum-production a skos:Concept ;
    skos:definition "A well drilled to drain hydrocarbons from an oil or gas field, including during the degasification of a coal seam."@en ;
    skos:inScheme <https://linked.data.gov.au/def/borehole-sub-purpose> ;
    skos:prefLabel "Petroleum Production"@en ;
    skos:topConceptOf <https://linked.data.gov.au/def/borehole-sub-purpose> .

bhfunc:structure a skos:Concept ;
    skos:definition "Borehole drilled to investigate the attitude of strata and the impact of any tectonic features."@en ;
    skos:inScheme <https://linked.data.gov.au/def/borehole-sub-purpose> ;
    skos:prefLabel "Structure"@en ;
    skos:topConceptOf <https://linked.data.gov.au/def/borehole-sub-purpose> .

bhfunc:observation a skos:Concept ;
    skos:definition "Borehole drilled to investigate water level or for piezometer installation."@en ;
    skos:inScheme <https://linked.data.gov.au/def/borehole-sub-purpose> ;
    skos:prefLabel "Observation"@en ;
    skos:topConceptOf <https://linked.data.gov.au/def/borehole-sub-purpose> .

bhfunc:resource-assessment a skos:Concept ;
    skos:definition "A well determining the geological properties of a resource specific to the type of commodity. This may include quantification of volume, grade, porosity, permeability, quality, or ease-of-extraction."@en ;
    skos:inScheme <https://linked.data.gov.au/def/borehole-sub-purpose> ;
    skos:prefLabel "Resource Assessment"@en ;
    skos:topConceptOf <https://linked.data.gov.au/def/borehole-sub-purpose> .

bhfunc:stimulation a skos:Concept ;
    skos:definition "A well drilled to enhance the production of a fluid from an offset production well. Typically to maintain reservoir pressure, to overcome to low permeability or high viscosity fluids in petroleum systems, or to introduce additional fluid in geothermal systems."@en ;
    skos:inScheme <https://linked.data.gov.au/def/borehole-sub-purpose> ;
    skos:prefLabel "Stimulation"@en ;
    skos:topConceptOf <https://linked.data.gov.au/def/borehole-sub-purpose> .

bhfunc:geotech a skos:Concept ;
    skos:definition "A borehole drilled to investigate the geotechnical properties of the strata and provide samples for mechanical testing."@en ;
    skos:inScheme <https://linked.data.gov.au/def/borehole-sub-purpose> ;
    skos:prefLabel "Geotech"@en ;
    skos:topConceptOf <https://linked.data.gov.au/def/borehole-sub-purpose> .

bhfunc:service a skos:Concept ;
    skos:definition "Borehole drilled to provide a conduit or access to and from mine workings for equipment or materials."@en ;
    skos:inScheme <https://linked.data.gov.au/def/borehole-sub-purpose> ;
    skos:prefLabel "Service"@en ;
    skos:topConceptOf <https://linked.data.gov.au/def/borehole-sub-purpose> .

bhfunc:gas-management a skos:Concept ;
    skos:definition "Borehole drilled for gas analysis and management. Typical applications include exploration, management of gas in coal mines, compliance and greenhouse gas emissions."@en ;
    skos:inScheme <https://linked.data.gov.au/def/borehole-sub-purpose> ;
    skos:prefLabel "Gas Management"@en ;
    skos:topConceptOf <https://linked.data.gov.au/def/borehole-sub-purpose> .

bhfunc:pggd-functions a skos:Collection ;
    skos:definition "The functions of boreholes specific to petroleum, greenhouse gas, and geothermal wells and bores i.e. those that require a statutory notification in Queensland regulation."@en ;
    skos:member bhfunc:water-supply,
        bhfunc:water-injection,
        bhfunc:stratigraphic,
        bhfunc:stimulation,
        bhfunc:petroleum-reservoir-characterisation,
        bhfunc:petroleum-production,
        bhfunc:petroleum-prod-test,
        bhfunc:petroleum-injection,
        bhfunc:observation,
        bhfunc:disposal,
        bhfunc:heat-flow ;
    skos:prefLabel "Petroleum Borehole Functions"@en .
