@prefix bhsts: <http://linked.data.gov.au/def/borehole-status/> .
@prefix dc: <http://purl.org/dc/elements/1.1/> .
@prefix dct: <http://purl.org/dc/terms/> .
@prefix owl: <http://www.w3.org/2002/07/owl#> .
@prefix rdf: <http://www.w3.org/1999/02/22-rdf-syntax-ns#> .
@prefix rdfs: <http://www.w3.org/2000/01/rdf-schema#> .
@prefix skos: <http://www.w3.org/2004/02/skos/core#> .
@prefix xml: <http://www.w3.org/XML/1998/namespace> .
@prefix xsd: <http://www.w3.org/2001/XMLSchema#> .

<http://linked.data.gov.au/def/borehole-status> a owl:Ontology .

bhsts:conceptScheme a skos:ConceptScheme ;
    dct:creator "Geological Survey of Queensland" ;
    dct:modified "2020-01-21T11:52:35+10:00"^^xsd:dateTime,
        "2020-01-21T11:52:42+10:00"^^xsd:dateTime ;
    dct:source "Compiled by the Geological Survey of Queensland" ;
    skos:definition "The status of a borehole describing the borehole lifecycle from proposed through operational through to abandonment. Lifecycle stages are commonly related to regulatory conditions administered by government agencies."@en ;
    skos:hasTopConcept bhsts:abandoned,
        bhsts:drilled,
        bhsts:drilling,
        bhsts:never-drilled,
        bhsts:proposed,
        bhsts:unknown ;
    skos:prefLabel "Borehole Statuses"@en .

bhsts:capped-and-abandoned a skos:Concept ;
    skos:broader bhsts:abandoned ;
    skos:definition "A well that has been capped  and abandoned as per the relevant Code of Practice."@en ;
    skos:inScheme bhsts:conceptScheme ;
    skos:prefLabel "Capped and Abandoned"@en .

bhsts:cased-and-suspended a skos:Concept ;
    skos:broader bhsts:drilled ;
    skos:definition "A well in which casing has been installed but is suspended and inactive pending installation of completion, monitoring, or other equipment."@en ;
    skos:inScheme bhsts:conceptScheme ;
    skos:prefLabel "Cased and Suspended"@en .

bhsts:completed a skos:Concept ;
    skos:broader bhsts:drilled ;
    skos:definition "A well that has had all relevant casing, tubing, and completion equipment such as pumps installed."@en ;
    skos:inScheme bhsts:conceptScheme ;
    skos:prefLabel "Completed"@en .

bhsts:monitoring a skos:Concept ;
    skos:broader bhsts:drilled ;
    skos:definition "A well that is actively monitoring reservoir, aquifer, or other geological parameters."@en ;
    skos:inScheme bhsts:conceptScheme ;
    skos:prefLabel "Monitoring"@en .

bhsts:on-injection a skos:Concept ;
    skos:broader bhsts:drilled ;
    skos:definition "A well that is injecting fluids such as water or hydrocarbons into a reservoir for disposal or future production."@en ;
    skos:inScheme bhsts:conceptScheme ;
    skos:prefLabel "On Injection"@en .

bhsts:on-production a skos:Concept ;
    skos:broader bhsts:drilled ;
    skos:definition "A well that is producing hydrocarbons or other non-water resources."@en ;
    skos:inScheme bhsts:conceptScheme ;
    skos:prefLabel "On Production"@en .

bhsts:plugged-and-abandoned a skos:Concept ;
    skos:broader bhsts:abandoned ;
    skos:definition "A well that has been plugged with cement or another accepted plugging method and abandoned as per the relevant Code of Practice."@en ;
    skos:inScheme bhsts:conceptScheme ;
    skos:prefLabel "Plugged and Abandoned"@en .

bhsts:suspended a skos:Concept ;
    skos:broader bhsts:drilled ;
    skos:definition "A well that has been suspended without casing or completion equipment installed"@en ;
    skos:inScheme bhsts:conceptScheme ;
    skos:prefLabel "Suspended"@en .

bhsts:water-supply a skos:Concept ;
    skos:broader bhsts:drilled ;
    skos:definition "A well that is primarliy producing water"@en ;
    skos:inScheme bhsts:conceptScheme ;
    skos:prefLabel "Water Supply"@en .

bhsts:drilling a skos:Concept ;
    skos:definition "A well in the active state of being drilled i.e. between spud date and rig release."@en ;
    skos:inScheme bhsts:conceptScheme ;
    skos:prefLabel "Drilling"@en ;
    skos:topConceptOf bhsts:conceptScheme .

bhsts:never-drilled a skos:Concept ;
    skos:definition "A well that was once proposed but was never drilled and is no longer intended to be drilled."@en ;
    skos:inScheme bhsts:conceptScheme ;
    skos:prefLabel "Never Drilled"@en ;
    skos:topConceptOf bhsts:conceptScheme .

bhsts:proposed a skos:Concept ;
    skos:definition "A proposed well or bore that has not yet been drilled. Created at lodgement of a PGGD-01 form for petroleum wells in Queensland"@en ;
    skos:inScheme bhsts:conceptScheme ;
    skos:prefLabel "Proposed"@en ;
    skos:topConceptOf bhsts:conceptScheme .

bhsts:unknown a skos:Concept ;
    skos:definition "A well that has been drilled, but whose further status is unknown."@en ;
    skos:inScheme bhsts:conceptScheme ;
    skos:prefLabel "Unknown"@en ;
    skos:topConceptOf bhsts:conceptScheme .

bhsts:abandoned a skos:Concept ;
    skos:definition "A well that has been abandoned and the cap and plug status is unknown."@en ;
    skos:inScheme bhsts:conceptScheme ;
    skos:prefLabel "Abandoned"@en ;
    skos:topConceptOf bhsts:conceptScheme .

bhsts:drilled a skos:Concept ;
    skos:definition "A well that has been drilled to its intended total depth and the drilling rig has been released from site."@en ;
    skos:inScheme bhsts:conceptScheme ;
    skos:prefLabel "Drilled"@en ;
    skos:topConceptOf bhsts:conceptScheme .
