@prefix dcterms: <http://purl.org/dc/terms/> .
@prefix geoad: <https://linked.data.gov.au/def/geoadminfeatures/> .
@prefix owl: <http://www.w3.org/2002/07/owl#> .
@prefix sdo: <https://schema.org/> .
@prefix skos: <http://www.w3.org/2004/02/skos/core#> .
@prefix rdfs: <http://www.w3.org/2000/01/rdf-schema#> .
@prefix xsd: <http://www.w3.org/2001/XMLSchema#> .

<https://linked.data.gov.au/def/geoadminfeatures> a owl:Ontology,
        skos:ConceptScheme ;
    dcterms:created "2019-12-04"^^xsd:date ;
    dcterms:creator <https://linked.data.gov.au/org/gsq> ;
    dcterms:modified "2020-08-25"^^xsd:date ;
    dcterms:publisher <https://linked.data.gov.au/org/gsq> ;
    owl:imports <http://www.opengis.net/ont/geosparql> ;
    skos:definition "This vocabulary lists types of geological administrative features relevant to the duties of the Geological Survey of Queensland. An Administrative Feature is a geo:Feature that is defined by adminstrative processes such as legislation, regulation, policy or procedure."@en ;
    skos:hasTopConcept geoad:Block, geoad:Permit, geoad:SubBlock, geoad:MapSeries ;
    skos:prefLabel "GeoAdmin Features"@en .

geoad:Block a skos:Concept ;
    skos:definition "A Block is an administrative division of the State of Queensland that is used for tenure management. A Block is defined as five minutes of latitude by five minutes of longitude. Blocks are grouped by 1:1,000,000 map sheet areas, the names of which provide the containing Blocks with a four letter prefix (e.g. Clermont 1:1,000,000 provides CLER). Each sheet area contains 3456 Blocks, with the Blocks numbered between 1 and 3456 inclusive. A Block is divided into 25 Sub-Blocks."@en ;
    rdfs:isDefinedBy <https://linked.data.gov.au/def/geoadminfeatures> ;
    skos:inScheme <https://linked.data.gov.au/def/geoadminfeatures> ;
    skos:prefLabel "Block"@en .

geoad:Permit a skos:Concept ;
    skos:definition "Permits are a license granted over a spatial region within the State of Queensland. Permits govern the activities which can be conducted upon them. Activities include exploration, development, and extraction of a specific commodity or commodities."@en ;
    rdfs:isDefinedBy <https://linked.data.gov.au/def/geoadminfeatures> ;
    skos:inScheme <https://linked.data.gov.au/def/geoadminfeatures> ;
    skos:prefLabel "Permit"@en .

geoad:SubBlock a skos:Concept ;
    skos:definition "A Sub-Block is an administrative sub-division of a Block. Each Block is divided into 25 Sub-Blocks. A Sub-Block is defined as one minute of latitude by one minute of longitude. The Sub-Blocks are prefixed with their corresponding Block name and are labelled from A to Z, excluding I. Labels are allocated from left to right, top to bottom, starting from the northwest corner."@en ;
    rdfs:isDefinedBy <https://linked.data.gov.au/def/geoadminfeatures> ;
    skos:inScheme <https://linked.data.gov.au/def/geoadminfeatures> ;
    skos:prefLabel "Sub-Block"@en .

geoad:MapSeries a skos:Concept ;
    skos:definition "A map series is a group of topographic or thematic maps or charts usually having the same scale and cartographic specifications, and with each sheet appropriately identified by its publisher as belonging to the same series. Map series occur when an area is to be covered by a map that, due to its scale, must be spread over several sheets. Nevertheless, the individual sheets of a map series can also be used quite independently, as they generally have full map surround details and legends. If a publisher produces several map series at different scales, then these series are called scale series."@en ;
    rdfs:isDefinedBy <https://linked.data.gov.au/def/geoadminfeatures> ;
    skos:inScheme <https://linked.data.gov.au/def/geoadminfeatures> ;
    skos:prefLabel "Map Series"@en .

geoad:BrambleCay7679 a skos:Concept ;skos:definition "Map sheet for Bramble Cay at 1:100 000 scale. The first two digits define a longitude band 0.5 degree wide and the second two digits a latitude band 0.5 degree wide."@en ;skos:inScheme <https://linked.data.gov.au/def/geoadminfeatures> ;skos:broader geoad:MapSeries ;skos:notation "7679" ;skos:prefLabel "Bramble Cay:7679"@en .
geoad:TuruCay7178 a skos:Concept ;skos:definition "Map sheet for Turu Cay at 1:100 000 scale. The first two digits define a longitude band 0.5 degree wide and the second two digits a latitude band 0.5 degree wide."@en ;skos:inScheme <https://linked.data.gov.au/def/geoadminfeatures> ;skos:broader geoad:MapSeries ;skos:notation "7178" ;skos:prefLabel "Turu Cay:7178"@en .
geoad:DeliveranceIsland7278 a skos:Concept ;skos:definition "Map sheet for Deliverance Island at 1:100 000 scale. The first two digits define a longitude band 0.5 degree wide and the second two digits a latitude band 0.5 degree wide."@en ;skos:inScheme <https://linked.data.gov.au/def/geoadminfeatures> ;skos:broader geoad:MapSeries ;skos:notation "7278" ;skos:prefLabel "Deliverance Island:7278"@en .
geoad:MabuiagIsland7378 a skos:Concept ;skos:definition "Map sheet for Mabuiag Island at 1:100 000 scale. The first two digits define a longitude band 0.5 degree wide and the second two digits a latitude band 0.5 degree wide."@en ;skos:inScheme <https://linked.data.gov.au/def/geoadminfeatures> ;skos:broader geoad:MapSeries ;skos:notation "7378" ;skos:prefLabel "Mabuiag Island:7378"@en .
geoad:GabbaIsland7478 a skos:Concept ;skos:definition "Map sheet for Gabba Island at 1:100 000 scale. The first two digits define a longitude band 0.5 degree wide and the second two digits a latitude band 0.5 degree wide."@en ;skos:inScheme <https://linked.data.gov.au/def/geoadminfeatures> ;skos:broader geoad:MapSeries ;skos:notation "7478" ;skos:prefLabel "Gabba Island:7478"@en .
geoad:RennelIsland7578 a skos:Concept ;skos:definition "Map sheet for Rennel Island at 1:100 000 scale. The first two digits define a longitude band 0.5 degree wide and the second two digits a latitude band 0.5 degree wide."@en ;skos:inScheme <https://linked.data.gov.au/def/geoadminfeatures> ;skos:broader geoad:MapSeries ;skos:notation "7578" ;skos:prefLabel "Rennel Island:7578"@en .
geoad:DarnleyIsland7678 a skos:Concept ;skos:definition "Map sheet for Darnley Island at 1:100 000 scale. The first two digits define a longitude band 0.5 degree wide and the second two digits a latitude band 0.5 degree wide."@en ;skos:inScheme <https://linked.data.gov.au/def/geoadminfeatures> ;skos:broader geoad:MapSeries ;skos:notation "7678" ;skos:prefLabel "Darnley Island:7678"@en .
geoad:MurrayIslands7778 a skos:Concept ;skos:definition "Map sheet for Murray Islands at 1:100 000 scale. The first two digits define a longitude band 0.5 degree wide and the second two digits a latitude band 0.5 degree wide."@en ;skos:inScheme <https://linked.data.gov.au/def/geoadminfeatures> ;skos:broader geoad:MapSeries ;skos:notation "7778" ;skos:prefLabel "Murray Islands:7778"@en .
geoad:MoaIsland7377 a skos:Concept ;skos:definition "Map sheet for Moa Island at 1:100 000 scale. The first two digits define a longitude band 0.5 degree wide and the second two digits a latitude band 0.5 degree wide."@en ;skos:inScheme <https://linked.data.gov.au/def/geoadminfeatures> ;skos:broader geoad:MapSeries ;skos:notation "7377" ;skos:prefLabel "Moa Island:7377"@en .
geoad:SassieIsland7477 a skos:Concept ;skos:definition "Map sheet for Sassie Island at 1:100 000 scale. The first two digits define a longitude band 0.5 degree wide and the second two digits a latitude band 0.5 degree wide."@en ;skos:inScheme <https://linked.data.gov.au/def/geoadminfeatures> ;skos:broader geoad:MapSeries ;skos:notation "7477" ;skos:prefLabel "Sassie Island:7477"@en .
geoad:CoconutIsland7577 a skos:Concept ;skos:definition "Map sheet for Coconut Island at 1:100 000 scale. The first two digits define a longitude band 0.5 degree wide and the second two digits a latitude band 0.5 degree wide."@en ;skos:inScheme <https://linked.data.gov.au/def/geoadminfeatures> ;skos:broader geoad:MapSeries ;skos:notation "7577" ;skos:prefLabel "Coconut Island:7577"@en .
geoad:BoobyIsland7276 a skos:Concept ;skos:definition "Map sheet for Booby Island at 1:100 000 scale. The first two digits define a longitude band 0.5 degree wide and the second two digits a latitude band 0.5 degree wide."@en ;skos:inScheme <https://linked.data.gov.au/def/geoadminfeatures> ;skos:broader geoad:MapSeries ;skos:notation "7276" ;skos:prefLabel "Booby Island:7276"@en .
geoad:ThursdayIsland7376 a skos:Concept ;skos:definition "Map sheet for Thursday Island at 1:100 000 scale. The first two digits define a longitude band 0.5 degree wide and the second two digits a latitude band 0.5 degree wide."@en ;skos:inScheme <https://linked.data.gov.au/def/geoadminfeatures> ;skos:broader geoad:MapSeries ;skos:notation "7376" ;skos:prefLabel "Thursday Island:7376"@en .
geoad:CapeYork7476 a skos:Concept ;skos:definition "Map sheet for Cape York at 1:100 000 scale. The first two digits define a longitude band 0.5 degree wide and the second two digits a latitude band 0.5 degree wide."@en ;skos:inScheme <https://linked.data.gov.au/def/geoadminfeatures> ;skos:broader geoad:MapSeries ;skos:notation "7476" ;skos:prefLabel "Cape York:7476"@en .
geoad:ArtubIslet7576 a skos:Concept ;skos:definition "Map sheet for Artub Islet at 1:100 000 scale. The first two digits define a longitude band 0.5 degree wide and the second two digits a latitude band 0.5 degree wide."@en ;skos:inScheme <https://linked.data.gov.au/def/geoadminfeatures> ;skos:broader geoad:MapSeries ;skos:notation "7576" ;skos:prefLabel "Artub Islet:7576"@en .
geoad:VrilyaPoint7375 a skos:Concept ;skos:definition "Map sheet for Vrilya Point at 1:100 000 scale. The first two digits define a longitude band 0.5 degree wide and the second two digits a latitude band 0.5 degree wide."@en ;skos:inScheme <https://linked.data.gov.au/def/geoadminfeatures> ;skos:broader geoad:MapSeries ;skos:notation "7375" ;skos:prefLabel "Vrilya Point:7375"@en .
geoad:OrfordBay7475 a skos:Concept ;skos:definition "Map sheet for Orford Bay at 1:100 000 scale. The first two digits define a longitude band 0.5 degree wide and the second two digits a latitude band 0.5 degree wide."@en ;skos:inScheme <https://linked.data.gov.au/def/geoadminfeatures> ;skos:broader geoad:MapSeries ;skos:notation "7475" ;skos:prefLabel "Orford Bay:7475"@en .
geoad:BoydongIsland7575 a skos:Concept ;skos:definition "Map sheet for Boydong Island at 1:100 000 scale. The first two digits define a longitude band 0.5 degree wide and the second two digits a latitude band 0.5 degree wide."@en ;skos:inScheme <https://linked.data.gov.au/def/geoadminfeatures> ;skos:broader geoad:MapSeries ;skos:notation "7575" ;skos:prefLabel "Boydong Island:7575"@en .
geoad:Mapoon7274 a skos:Concept ;skos:definition "Map sheet for Mapoon at 1:100 000 scale. The first two digits define a longitude band 0.5 degree wide and the second two digits a latitude band 0.5 degree wide."@en ;skos:inScheme <https://linked.data.gov.au/def/geoadminfeatures> ;skos:broader geoad:MapSeries ;skos:notation "7274" ;skos:prefLabel "Mapoon:7274"@en .
geoad:SkardonRiver7374 a skos:Concept ;skos:definition "Map sheet for Skardon River at 1:100 000 scale. The first two digits define a longitude band 0.5 degree wide and the second two digits a latitude band 0.5 degree wide."@en ;skos:inScheme <https://linked.data.gov.au/def/geoadminfeatures> ;skos:broader geoad:MapSeries ;skos:notation "7374" ;skos:prefLabel "Skardon River:7374"@en .
geoad:ShelburneBay7474 a skos:Concept ;skos:definition "Map sheet for Shelburne Bay at 1:100 000 scale. The first two digits define a longitude band 0.5 degree wide and the second two digits a latitude band 0.5 degree wide."@en ;skos:inScheme <https://linked.data.gov.au/def/geoadminfeatures> ;skos:broader geoad:MapSeries ;skos:notation "7474" ;skos:prefLabel "Shelburne Bay:7474"@en .
geoad:CapeGrenville7574 a skos:Concept ;skos:definition "Map sheet for Cape Grenville at 1:100 000 scale. The first two digits define a longitude band 0.5 degree wide and the second two digits a latitude band 0.5 degree wide."@en ;skos:inScheme <https://linked.data.gov.au/def/geoadminfeatures> ;skos:broader geoad:MapSeries ;skos:notation "7574" ;skos:prefLabel "Cape Grenville:7574"@en .
geoad:PennefatherRiver7273 a skos:Concept ;skos:definition "Map sheet for Pennefather River at 1:100 000 scale. The first two digits define a longitude band 0.5 degree wide and the second two digits a latitude band 0.5 degree wide."@en ;skos:inScheme <https://linked.data.gov.au/def/geoadminfeatures> ;skos:broader geoad:MapSeries ;skos:notation "7273" ;skos:prefLabel "Pennefather River:7273"@en .
geoad:Agnew7373 a skos:Concept ;skos:definition "Map sheet for Agnew at 1:100 000 scale. The first two digits define a longitude band 0.5 degree wide and the second two digits a latitude band 0.5 degree wide."@en ;skos:inScheme <https://linked.data.gov.au/def/geoadminfeatures> ;skos:broader geoad:MapSeries ;skos:notation "7373" ;skos:prefLabel "Agnew:7373"@en .
geoad:Moreton7473 a skos:Concept ;skos:definition "Map sheet for Moreton at 1:100 000 scale. The first two digits define a longitude band 0.5 degree wide and the second two digits a latitude band 0.5 degree wide."@en ;skos:inScheme <https://linked.data.gov.au/def/geoadminfeatures> ;skos:broader geoad:MapSeries ;skos:notation "7473" ;skos:prefLabel "Moreton:7473"@en .
geoad:TempleBay7573 a skos:Concept ;skos:definition "Map sheet for Temple Bay at 1:100 000 scale. The first two digits define a longitude band 0.5 degree wide and the second two digits a latitude band 0.5 degree wide."@en ;skos:inScheme <https://linked.data.gov.au/def/geoadminfeatures> ;skos:broader geoad:MapSeries ;skos:notation "7573" ;skos:prefLabel "Temple Bay:7573"@en .
geoad:Weipa7272 a skos:Concept ;skos:definition "Map sheet for Weipa at 1:100 000 scale. The first two digits define a longitude band 0.5 degree wide and the second two digits a latitude band 0.5 degree wide."@en ;skos:inScheme <https://linked.data.gov.au/def/geoadminfeatures> ;skos:broader geoad:MapSeries ;skos:notation "7272" ;skos:prefLabel "Weipa:7272"@en .
geoad:YorkDowns7372 a skos:Concept ;skos:definition "Map sheet for York Downs at 1:100 000 scale. The first two digits define a longitude band 0.5 degree wide and the second two digits a latitude band 0.5 degree wide."@en ;skos:inScheme <https://linked.data.gov.au/def/geoadminfeatures> ;skos:broader geoad:MapSeries ;skos:notation "7372" ;skos:prefLabel "York Downs:7372"@en .
geoad:BataviaDowns7472 a skos:Concept ;skos:definition "Map sheet for Batavia Downs at 1:100 000 scale. The first two digits define a longitude band 0.5 degree wide and the second two digits a latitude band 0.5 degree wide."@en ;skos:inScheme <https://linked.data.gov.au/def/geoadminfeatures> ;skos:broader geoad:MapSeries ;skos:notation "7472" ;skos:prefLabel "Batavia Downs:7472"@en .
geoad:CapeWeymouth7572 a skos:Concept ;skos:definition "Map sheet for Cape Weymouth at 1:100 000 scale. The first two digits define a longitude band 0.5 degree wide and the second two digits a latitude band 0.5 degree wide."@en ;skos:inScheme <https://linked.data.gov.au/def/geoadminfeatures> ;skos:broader geoad:MapSeries ;skos:notation "7572" ;skos:prefLabel "Cape Weymouth:7572"@en .
geoad:CapeDirection7672 a skos:Concept ;skos:definition "Map sheet for Cape Direction at 1:100 000 scale. The first two digits define a longitude band 0.5 degree wide and the second two digits a latitude band 0.5 degree wide."@en ;skos:inScheme <https://linked.data.gov.au/def/geoadminfeatures> ;skos:broader geoad:MapSeries ;skos:notation "7672" ;skos:prefLabel "Cape Direction:7672"@en .
geoad:Aurukun7271 a skos:Concept ;skos:definition "Map sheet for Aurukun at 1:100 000 scale. The first two digits define a longitude band 0.5 degree wide and the second two digits a latitude band 0.5 degree wide."@en ;skos:inScheme <https://linked.data.gov.au/def/geoadminfeatures> ;skos:broader geoad:MapSeries ;skos:notation "7271" ;skos:prefLabel "Aurukun:7271"@en .
geoad:Merluna7371 a skos:Concept ;skos:definition "Map sheet for Merluna at 1:100 000 scale. The first two digits define a longitude band 0.5 degree wide and the second two digits a latitude band 0.5 degree wide."@en ;skos:inScheme <https://linked.data.gov.au/def/geoadminfeatures> ;skos:broader geoad:MapSeries ;skos:notation "7371" ;skos:prefLabel "Merluna:7371"@en .
geoad:Wenlock7471 a skos:Concept ;skos:definition "Map sheet for Wenlock at 1:100 000 scale. The first two digits define a longitude band 0.5 degree wide and the second two digits a latitude band 0.5 degree wide."@en ;skos:inScheme <https://linked.data.gov.au/def/geoadminfeatures> ;skos:broader geoad:MapSeries ;skos:notation "7471" ;skos:prefLabel "Wenlock:7471"@en .
geoad:LockhartRiver7571 a skos:Concept ;skos:definition "Map sheet for Lockhart River at 1:100 000 scale. The first two digits define a longitude band 0.5 degree wide and the second two digits a latitude band 0.5 degree wide."@en ;skos:inScheme <https://linked.data.gov.au/def/geoadminfeatures> ;skos:broader geoad:MapSeries ;skos:notation "7571" ;skos:prefLabel "Lockhart River:7571"@en .
geoad:CapeSidmouth7671 a skos:Concept ;skos:definition "Map sheet for Cape Sidmouth at 1:100 000 scale. The first two digits define a longitude band 0.5 degree wide and the second two digits a latitude band 0.5 degree wide."@en ;skos:inScheme <https://linked.data.gov.au/def/geoadminfeatures> ;skos:broader geoad:MapSeries ;skos:notation "7671" ;skos:prefLabel "Cape Sidmouth:7671"@en .
geoad:CapeKeerweer7170 a skos:Concept ;skos:definition "Map sheet for Cape Keerweer at 1:100 000 scale. The first two digits define a longitude band 0.5 degree wide and the second two digits a latitude band 0.5 degree wide."@en ;skos:inScheme <https://linked.data.gov.au/def/geoadminfeatures> ;skos:broader geoad:MapSeries ;skos:notation "7170" ;skos:prefLabel "Cape Keerweer:7170"@en .
geoad:ArcherRiver7270 a skos:Concept ;skos:definition "Map sheet for Archer River at 1:100 000 scale. The first two digits define a longitude band 0.5 degree wide and the second two digits a latitude band 0.5 degree wide."@en ;skos:inScheme <https://linked.data.gov.au/def/geoadminfeatures> ;skos:broader geoad:MapSeries ;skos:notation "7270" ;skos:prefLabel "Archer River:7270"@en .
geoad:Merapah7370 a skos:Concept ;skos:definition "Map sheet for Merapah at 1:100 000 scale. The first two digits define a longitude band 0.5 degree wide and the second two digits a latitude band 0.5 degree wide."@en ;skos:inScheme <https://linked.data.gov.au/def/geoadminfeatures> ;skos:broader geoad:MapSeries ;skos:notation "7370" ;skos:prefLabel "Merapah:7370"@en .
geoad:Rokeby7470 a skos:Concept ;skos:definition "Map sheet for Rokeby at 1:100 000 scale. The first two digits define a longitude band 0.5 degree wide and the second two digits a latitude band 0.5 degree wide."@en ;skos:inScheme <https://linked.data.gov.au/def/geoadminfeatures> ;skos:broader geoad:MapSeries ;skos:notation "7470" ;skos:prefLabel "Rokeby:7470"@en .
geoad:Coen7570 a skos:Concept ;skos:definition "Map sheet for Coen at 1:100 000 scale. The first two digits define a longitude band 0.5 degree wide and the second two digits a latitude band 0.5 degree wide."@en ;skos:inScheme <https://linked.data.gov.au/def/geoadminfeatures> ;skos:broader geoad:MapSeries ;skos:notation "7570" ;skos:prefLabel "Coen:7570"@en .
geoad:SilverPlains7670 a skos:Concept ;skos:definition "Map sheet for Silver Plains at 1:100 000 scale. The first two digits define a longitude band 0.5 degree wide and the second two digits a latitude band 0.5 degree wide."@en ;skos:inScheme <https://linked.data.gov.au/def/geoadminfeatures> ;skos:broader geoad:MapSeries ;skos:notation "7670" ;skos:prefLabel "Silver Plains:7670"@en .
geoad:Holroyd7269 a skos:Concept ;skos:definition "Map sheet for Holroyd at 1:100 000 scale. The first two digits define a longitude band 0.5 degree wide and the second two digits a latitude band 0.5 degree wide."@en ;skos:inScheme <https://linked.data.gov.au/def/geoadminfeatures> ;skos:broader geoad:MapSeries ;skos:notation "7269" ;skos:prefLabel "Holroyd:7269"@en .
geoad:KendallRiver7369 a skos:Concept ;skos:definition "Map sheet for Kendall River at 1:100 000 scale. The first two digits define a longitude band 0.5 degree wide and the second two digits a latitude band 0.5 degree wide."@en ;skos:inScheme <https://linked.data.gov.au/def/geoadminfeatures> ;skos:broader geoad:MapSeries ;skos:notation "7369" ;skos:prefLabel "Kendall River:7369"@en .
geoad:Strathburn7469 a skos:Concept ;skos:definition "Map sheet for Strathburn at 1:100 000 scale. The first two digits define a longitude band 0.5 degree wide and the second two digits a latitude band 0.5 degree wide."@en ;skos:inScheme <https://linked.data.gov.au/def/geoadminfeatures> ;skos:broader geoad:MapSeries ;skos:notation "7469" ;skos:prefLabel "Strathburn:7469"@en .
geoad:Ebagoola7569 a skos:Concept ;skos:definition "Map sheet for Ebagoola at 1:100 000 scale. The first two digits define a longitude band 0.5 degree wide and the second two digits a latitude band 0.5 degree wide."@en ;skos:inScheme <https://linked.data.gov.au/def/geoadminfeatures> ;skos:broader geoad:MapSeries ;skos:notation "7569" ;skos:prefLabel "Ebagoola:7569"@en .
geoad:PrincessCharlotteBay7669 a skos:Concept ;skos:definition "Map sheet for Princess Charlotte Bay at 1:100 000 scale. The first two digits define a longitude band 0.5 degree wide and the second two digits a latitude band 0.5 degree wide."@en ;skos:inScheme <https://linked.data.gov.au/def/geoadminfeatures> ;skos:broader geoad:MapSeries ;skos:notation "7669" ;skos:prefLabel "Princess Charlotte Bay:7669"@en .
geoad:BathurstRange7769 a skos:Concept ;skos:definition "Map sheet for Bathurst Range at 1:100 000 scale. The first two digits define a longitude band 0.5 degree wide and the second two digits a latitude band 0.5 degree wide."@en ;skos:inScheme <https://linked.data.gov.au/def/geoadminfeatures> ;skos:broader geoad:MapSeries ;skos:notation "7769" ;skos:prefLabel "Bathurst Range:7769"@en .
geoad:CapeMelville7869 a skos:Concept ;skos:definition "Map sheet for Cape Melville at 1:100 000 scale. The first two digits define a longitude band 0.5 degree wide and the second two digits a latitude band 0.5 degree wide."@en ;skos:inScheme <https://linked.data.gov.au/def/geoadminfeatures> ;skos:broader geoad:MapSeries ;skos:notation "7869" ;skos:prefLabel "Cape Melville:7869"@en .
geoad:EdwardRiver7268 a skos:Concept ;skos:definition "Map sheet for Edward River at 1:100 000 scale. The first two digits define a longitude band 0.5 degree wide and the second two digits a latitude band 0.5 degree wide."@en ;skos:inScheme <https://linked.data.gov.au/def/geoadminfeatures> ;skos:broader geoad:MapSeries ;skos:notation "7268" ;skos:prefLabel "Edward River:7268"@en .
geoad:Strathgordon7368 a skos:Concept ;skos:definition "Map sheet for Strathgordon at 1:100 000 scale. The first two digits define a longitude band 0.5 degree wide and the second two digits a latitude band 0.5 degree wide."@en ;skos:inScheme <https://linked.data.gov.au/def/geoadminfeatures> ;skos:broader geoad:MapSeries ;skos:notation "7368" ;skos:prefLabel "Strathgordon:7368"@en .
geoad:Strathmay7468 a skos:Concept ;skos:definition "Map sheet for Strathmay at 1:100 000 scale. The first two digits define a longitude band 0.5 degree wide and the second two digits a latitude band 0.5 degree wide."@en ;skos:inScheme <https://linked.data.gov.au/def/geoadminfeatures> ;skos:broader geoad:MapSeries ;skos:notation "7468" ;skos:prefLabel "Strathmay:7468"@en .
geoad:Kalkah7568 a skos:Concept ;skos:definition "Map sheet for Kalkah at 1:100 000 scale. The first two digits define a longitude band 0.5 degree wide and the second two digits a latitude band 0.5 degree wide."@en ;skos:inScheme <https://linked.data.gov.au/def/geoadminfeatures> ;skos:broader geoad:MapSeries ;skos:notation "7568" ;skos:prefLabel "Kalkah:7568"@en .
geoad:MarinaPlains7668 a skos:Concept ;skos:definition "Map sheet for Marina Plains at 1:100 000 scale. The first two digits define a longitude band 0.5 degree wide and the second two digits a latitude band 0.5 degree wide."@en ;skos:inScheme <https://linked.data.gov.au/def/geoadminfeatures> ;skos:broader geoad:MapSeries ;skos:notation "7668" ;skos:prefLabel "Marina Plains:7668"@en .
geoad:Lakefield7768 a skos:Concept ;skos:definition "Map sheet for Lakefield at 1:100 000 scale. The first two digits define a longitude band 0.5 degree wide and the second two digits a latitude band 0.5 degree wide."@en ;skos:inScheme <https://linked.data.gov.au/def/geoadminfeatures> ;skos:broader geoad:MapSeries ;skos:notation "7768" ;skos:prefLabel "Lakefield:7768"@en .
geoad:JeannieRiver7868 a skos:Concept ;skos:definition "Map sheet for Jeannie River at 1:100 000 scale. The first two digits define a longitude band 0.5 degree wide and the second two digits a latitude band 0.5 degree wide."@en ;skos:inScheme <https://linked.data.gov.au/def/geoadminfeatures> ;skos:broader geoad:MapSeries ;skos:notation "7868" ;skos:prefLabel "Jeannie River:7868"@en .
geoad:CapeFlattery7968 a skos:Concept ;skos:definition "Map sheet for Cape Flattery at 1:100 000 scale. The first two digits define a longitude band 0.5 degree wide and the second two digits a latitude band 0.5 degree wide."@en ;skos:inScheme <https://linked.data.gov.au/def/geoadminfeatures> ;skos:broader geoad:MapSeries ;skos:notation "7968" ;skos:prefLabel "Cape Flattery:7968"@en .
geoad:MitchellRiver7267 a skos:Concept ;skos:definition "Map sheet for Mitchell River at 1:100 000 scale. The first two digits define a longitude band 0.5 degree wide and the second two digits a latitude band 0.5 degree wide."@en ;skos:inScheme <https://linked.data.gov.au/def/geoadminfeatures> ;skos:broader geoad:MapSeries ;skos:notation "7267" ;skos:prefLabel "Mitchell River:7267"@en .
geoad:ParadiseCreek7367 a skos:Concept ;skos:definition "Map sheet for Paradise Creek at 1:100 000 scale. The first two digits define a longitude band 0.5 degree wide and the second two digits a latitude band 0.5 degree wide."@en ;skos:inScheme <https://linked.data.gov.au/def/geoadminfeatures> ;skos:broader geoad:MapSeries ;skos:notation "7367" ;skos:prefLabel "Paradise Creek:7367"@en .
geoad:CrosbieCreek7467 a skos:Concept ;skos:definition "Map sheet for Crosbie Creek at 1:100 000 scale. The first two digits define a longitude band 0.5 degree wide and the second two digits a latitude band 0.5 degree wide."@en ;skos:inScheme <https://linked.data.gov.au/def/geoadminfeatures> ;skos:broader geoad:MapSeries ;skos:notation "7467" ;skos:prefLabel "Crosbie Creek:7467"@en .
geoad:Dixie7567 a skos:Concept ;skos:definition "Map sheet for Dixie at 1:100 000 scale. The first two digits define a longitude band 0.5 degree wide and the second two digits a latitude band 0.5 degree wide."@en ;skos:inScheme <https://linked.data.gov.au/def/geoadminfeatures> ;skos:broader geoad:MapSeries ;skos:notation "7567" ;skos:prefLabel "Dixie:7567"@en .
geoad:Kalinga7667 a skos:Concept ;skos:definition "Map sheet for Kalinga at 1:100 000 scale. The first two digits define a longitude band 0.5 degree wide and the second two digits a latitude band 0.5 degree wide."@en ;skos:inScheme <https://linked.data.gov.au/def/geoadminfeatures> ;skos:broader geoad:MapSeries ;skos:notation "7667" ;skos:prefLabel "Kalinga:7667"@en .
geoad:KennedyBend7767 a skos:Concept ;skos:definition "Map sheet for Kennedy Bend at 1:100 000 scale. The first two digits define a longitude band 0.5 degree wide and the second two digits a latitude band 0.5 degree wide."@en ;skos:inScheme <https://linked.data.gov.au/def/geoadminfeatures> ;skos:broader geoad:MapSeries ;skos:notation "7767" ;skos:prefLabel "Kennedy Bend:7767"@en .
geoad:BattleCamp7867 a skos:Concept ;skos:definition "Map sheet for Battle Camp at 1:100 000 scale. The first two digits define a longitude band 0.5 degree wide and the second two digits a latitude band 0.5 degree wide."@en ;skos:inScheme <https://linked.data.gov.au/def/geoadminfeatures> ;skos:broader geoad:MapSeries ;skos:notation "7867" ;skos:prefLabel "Battle Camp:7867"@en .
geoad:Cooktown7967 a skos:Concept ;skos:definition "Map sheet for Cooktown at 1:100 000 scale. The first two digits define a longitude band 0.5 degree wide and the second two digits a latitude band 0.5 degree wide."@en ;skos:inScheme <https://linked.data.gov.au/def/geoadminfeatures> ;skos:broader geoad:MapSeries ;skos:notation "7967" ;skos:prefLabel "Cooktown:7967"@en .
geoad:NassauRiver7166 a skos:Concept ;skos:definition "Map sheet for Nassau River at 1:100 000 scale. The first two digits define a longitude band 0.5 degree wide and the second two digits a latitude band 0.5 degree wide."@en ;skos:inScheme <https://linked.data.gov.au/def/geoadminfeatures> ;skos:broader geoad:MapSeries ;skos:notation "7166" ;skos:prefLabel "Nassau River:7166"@en .
geoad:RutlandPlains7266 a skos:Concept ;skos:definition "Map sheet for Rutland Plains at 1:100 000 scale. The first two digits define a longitude band 0.5 degree wide and the second two digits a latitude band 0.5 degree wide."@en ;skos:inScheme <https://linked.data.gov.au/def/geoadminfeatures> ;skos:broader geoad:MapSeries ;skos:notation "7266" ;skos:prefLabel "Rutland Plains:7266"@en .
geoad:Koolatah7366 a skos:Concept ;skos:definition "Map sheet for Koolatah at 1:100 000 scale. The first two digits define a longitude band 0.5 degree wide and the second two digits a latitude band 0.5 degree wide."@en ;skos:inScheme <https://linked.data.gov.au/def/geoadminfeatures> ;skos:broader geoad:MapSeries ;skos:notation "7366" ;skos:prefLabel "Koolatah:7366"@en .
geoad:PetersLagoon7466 a skos:Concept ;skos:definition "Map sheet for Peters Lagoon at 1:100 000 scale. The first two digits define a longitude band 0.5 degree wide and the second two digits a latitude band 0.5 degree wide."@en ;skos:inScheme <https://linked.data.gov.au/def/geoadminfeatures> ;skos:broader geoad:MapSeries ;skos:notation "7466" ;skos:prefLabel "Peters Lagoon:7466"@en .
geoad:Strathleven7566 a skos:Concept ;skos:definition "Map sheet for Strathleven at 1:100 000 scale. The first two digits define a longitude band 0.5 degree wide and the second two digits a latitude band 0.5 degree wide."@en ;skos:inScheme <https://linked.data.gov.au/def/geoadminfeatures> ;skos:broader geoad:MapSeries ;skos:notation "7566" ;skos:prefLabel "Strathleven:7566"@en .
geoad:JeddaCreek7666 a skos:Concept ;skos:definition "Map sheet for Jedda Creek at 1:100 000 scale. The first two digits define a longitude band 0.5 degree wide and the second two digits a latitude band 0.5 degree wide."@en ;skos:inScheme <https://linked.data.gov.au/def/geoadminfeatures> ;skos:broader geoad:MapSeries ;skos:notation "7666" ;skos:prefLabel "Jedda Creek:7666"@en .
geoad:Laura7766 a skos:Concept ;skos:definition "Map sheet for Laura at 1:100 000 scale. The first two digits define a longitude band 0.5 degree wide and the second two digits a latitude band 0.5 degree wide."@en ;skos:inScheme <https://linked.data.gov.au/def/geoadminfeatures> ;skos:broader geoad:MapSeries ;skos:notation "7766" ;skos:prefLabel "Laura:7766"@en .
geoad:ButchersHill7866 a skos:Concept ;skos:definition "Map sheet for Butchers Hill at 1:100 000 scale. The first two digits define a longitude band 0.5 degree wide and the second two digits a latitude band 0.5 degree wide."@en ;skos:inScheme <https://linked.data.gov.au/def/geoadminfeatures> ;skos:broader geoad:MapSeries ;skos:notation "7866" ;skos:prefLabel "Butchers Hill:7866"@en .
geoad:Helenvale7966 a skos:Concept ;skos:definition "Map sheet for Helenvale at 1:100 000 scale. The first two digits define a longitude band 0.5 degree wide and the second two digits a latitude band 0.5 degree wide."@en ;skos:inScheme <https://linked.data.gov.au/def/geoadminfeatures> ;skos:broader geoad:MapSeries ;skos:notation "7966" ;skos:prefLabel "Helenvale:7966"@en .
geoad:LowareahPoint6765 a skos:Concept ;skos:definition "Map sheet for Lowareah Point at 1:100 000 scale. The first two digits define a longitude band 0.5 degree wide and the second two digits a latitude band 0.5 degree wide."@en ;skos:inScheme <https://linked.data.gov.au/def/geoadminfeatures> ;skos:broader geoad:MapSeries ;skos:notation "6765" ;skos:prefLabel "Lowareah Point:6765"@en .
geoad:ElizabethRiver6865 a skos:Concept ;skos:definition "Map sheet for Elizabeth River at 1:100 000 scale. The first two digits define a longitude band 0.5 degree wide and the second two digits a latitude band 0.5 degree wide."@en ;skos:inScheme <https://linked.data.gov.au/def/geoadminfeatures> ;skos:broader geoad:MapSeries ;skos:notation "6865" ;skos:prefLabel "Elizabeth River:6865"@en .
geoad:DinahIsland7165 a skos:Concept ;skos:definition "Map sheet for Dinah Island at 1:100 000 scale. The first two digits define a longitude band 0.5 degree wide and the second two digits a latitude band 0.5 degree wide."@en ;skos:inScheme <https://linked.data.gov.au/def/geoadminfeatures> ;skos:broader geoad:MapSeries ;skos:notation "7165" ;skos:prefLabel "Dinah Island:7165"@en .
geoad:Galbraith7265 a skos:Concept ;skos:definition "Map sheet for Galbraith at 1:100 000 scale. The first two digits define a longitude band 0.5 degree wide and the second two digits a latitude band 0.5 degree wide."@en ;skos:inScheme <https://linked.data.gov.au/def/geoadminfeatures> ;skos:broader geoad:MapSeries ;skos:notation "7265" ;skos:prefLabel "Galbraith:7265"@en .
geoad:Dunbar7365 a skos:Concept ;skos:definition "Map sheet for Dunbar at 1:100 000 scale. The first two digits define a longitude band 0.5 degree wide and the second two digits a latitude band 0.5 degree wide."@en ;skos:inScheme <https://linked.data.gov.au/def/geoadminfeatures> ;skos:broader geoad:MapSeries ;skos:notation "7365" ;skos:prefLabel "Dunbar:7365"@en .
geoad:KingfishLagoon7465 a skos:Concept ;skos:definition "Map sheet for Kingfish Lagoon at 1:100 000 scale. The first two digits define a longitude band 0.5 degree wide and the second two digits a latitude band 0.5 degree wide."@en ;skos:inScheme <https://linked.data.gov.au/def/geoadminfeatures> ;skos:broader geoad:MapSeries ;skos:notation "7465" ;skos:prefLabel "Kingfish Lagoon:7465"@en .
geoad:Highbury7565 a skos:Concept ;skos:definition "Map sheet for Highbury at 1:100 000 scale. The first two digits define a longitude band 0.5 degree wide and the second two digits a latitude band 0.5 degree wide."@en ;skos:inScheme <https://linked.data.gov.au/def/geoadminfeatures> ;skos:broader geoad:MapSeries ;skos:notation "7565" ;skos:prefLabel "Highbury:7565"@en .
geoad:MountMulgrave7665 a skos:Concept ;skos:definition "Map sheet for Mount Mulgrave at 1:100 000 scale. The first two digits define a longitude band 0.5 degree wide and the second two digits a latitude band 0.5 degree wide."@en ;skos:inScheme <https://linked.data.gov.au/def/geoadminfeatures> ;skos:broader geoad:MapSeries ;skos:notation "7665" ;skos:prefLabel "Mount Mulgrave:7665"@en .
geoad:Maytown7765 a skos:Concept ;skos:definition "Map sheet for Maytown at 1:100 000 scale. The first two digits define a longitude band 0.5 degree wide and the second two digits a latitude band 0.5 degree wide."@en ;skos:inScheme <https://linked.data.gov.au/def/geoadminfeatures> ;skos:broader geoad:MapSeries ;skos:notation "7765" ;skos:prefLabel "Maytown:7765"@en .
geoad:SouthPalmerRiver7865 a skos:Concept ;skos:definition "Map sheet for South Palmer River at 1:100 000 scale. The first two digits define a longitude band 0.5 degree wide and the second two digits a latitude band 0.5 degree wide."@en ;skos:inScheme <https://linked.data.gov.au/def/geoadminfeatures> ;skos:broader geoad:MapSeries ;skos:notation "7865" ;skos:prefLabel "South Palmer River:7865"@en .
geoad:Mossman7965 a skos:Concept ;skos:definition "Map sheet for Mossman at 1:100 000 scale. The first two digits define a longitude band 0.5 degree wide and the second two digits a latitude band 0.5 degree wide."@en ;skos:inScheme <https://linked.data.gov.au/def/geoadminfeatures> ;skos:broader geoad:MapSeries ;skos:notation "7965" ;skos:prefLabel "Mossman:7965"@en .
geoad:MassacreInlet6564 a skos:Concept ;skos:definition "Map sheet for Massacre Inlet at 1:100 000 scale. The first two digits define a longitude band 0.5 degree wide and the second two digits a latitude band 0.5 degree wide."@en ;skos:inScheme <https://linked.data.gov.au/def/geoadminfeatures> ;skos:broader geoad:MapSeries ;skos:notation "6564" ;skos:prefLabel "Massacre Inlet:6564"@en .
geoad:CliffdaleCreek6664 a skos:Concept ;skos:definition "Map sheet for Cliffdale Creek at 1:100 000 scale. The first two digits define a longitude band 0.5 degree wide and the second two digits a latitude band 0.5 degree wide."@en ;skos:inScheme <https://linked.data.gov.au/def/geoadminfeatures> ;skos:broader geoad:MapSeries ;skos:notation "6664" ;skos:prefLabel "Cliffdale Creek:6664"@en .
geoad:Mornington6764 a skos:Concept ;skos:definition "Map sheet for Mornington at 1:100 000 scale. The first two digits define a longitude band 0.5 degree wide and the second two digits a latitude band 0.5 degree wide."@en ;skos:inScheme <https://linked.data.gov.au/def/geoadminfeatures> ;skos:broader geoad:MapSeries ;skos:notation "6764" ;skos:prefLabel "Mornington:6764"@en .
geoad:CapeVanDiemen6864 a skos:Concept ;skos:definition "Map sheet for Cape Van Diemen at 1:100 000 scale. The first two digits define a longitude band 0.5 degree wide and the second two digits a latitude band 0.5 degree wide."@en ;skos:inScheme <https://linked.data.gov.au/def/geoadminfeatures> ;skos:broader geoad:MapSeries ;skos:notation "6864" ;skos:prefLabel "Cape Van Diemen:6864"@en .
geoad:Macaroni7164 a skos:Concept ;skos:definition "Map sheet for Macaroni at 1:100 000 scale. The first two digits define a longitude band 0.5 degree wide and the second two digits a latitude band 0.5 degree wide."@en ;skos:inScheme <https://linked.data.gov.au/def/geoadminfeatures> ;skos:broader geoad:MapSeries ;skos:notation "7164" ;skos:prefLabel "Macaroni:7164"@en .
geoad:Vanrook7264 a skos:Concept ;skos:definition "Map sheet for Vanrook at 1:100 000 scale. The first two digits define a longitude band 0.5 degree wide and the second two digits a latitude band 0.5 degree wide."@en ;skos:inScheme <https://linked.data.gov.au/def/geoadminfeatures> ;skos:broader geoad:MapSeries ;skos:notation "7264" ;skos:prefLabel "Vanrook:7264"@en .
geoad:StaatenRiver7364 a skos:Concept ;skos:definition "Map sheet for Staaten River at 1:100 000 scale. The first two digits define a longitude band 0.5 degree wide and the second two digits a latitude band 0.5 degree wide."@en ;skos:inScheme <https://linked.data.gov.au/def/geoadminfeatures> ;skos:broader geoad:MapSeries ;skos:notation "7364" ;skos:prefLabel "Staaten River:7364"@en .
geoad:PandanusCreek7464 a skos:Concept ;skos:definition "Map sheet for Pandanus Creek at 1:100 000 scale. The first two digits define a longitude band 0.5 degree wide and the second two digits a latitude band 0.5 degree wide."@en ;skos:inScheme <https://linked.data.gov.au/def/geoadminfeatures> ;skos:broader geoad:MapSeries ;skos:notation "7464" ;skos:prefLabel "Pandanus Creek:7464"@en .
geoad:Bulimba7564 a skos:Concept ;skos:definition "Map sheet for Bulimba at 1:100 000 scale. The first two digits define a longitude band 0.5 degree wide and the second two digits a latitude band 0.5 degree wide."@en ;skos:inScheme <https://linked.data.gov.au/def/geoadminfeatures> ;skos:broader geoad:MapSeries ;skos:notation "7564" ;skos:prefLabel "Bulimba:7564"@en .
geoad:Walsh7664 a skos:Concept ;skos:definition "Map sheet for Walsh at 1:100 000 scale. The first two digits define a longitude band 0.5 degree wide and the second two digits a latitude band 0.5 degree wide."@en ;skos:inScheme <https://linked.data.gov.au/def/geoadminfeatures> ;skos:broader geoad:MapSeries ;skos:notation "7664" ;skos:prefLabel "Walsh:7664"@en .
geoad:Bellevue7764 a skos:Concept ;skos:definition "Map sheet for Bellevue at 1:100 000 scale. The first two digits define a longitude band 0.5 degree wide and the second two digits a latitude band 0.5 degree wide."@en ;skos:inScheme <https://linked.data.gov.au/def/geoadminfeatures> ;skos:broader geoad:MapSeries ;skos:notation "7764" ;skos:prefLabel "Bellevue:7764"@en .
geoad:MountMulligan7864 a skos:Concept ;skos:definition "Map sheet for Mount Mulligan at 1:100 000 scale. The first two digits define a longitude band 0.5 degree wide and the second two digits a latitude band 0.5 degree wide."@en ;skos:inScheme <https://linked.data.gov.au/def/geoadminfeatures> ;skos:broader geoad:MapSeries ;skos:notation "7864" ;skos:prefLabel "Mount Mulligan:7864"@en .
geoad:Rumula7964 a skos:Concept ;skos:definition "Map sheet for Rumula at 1:100 000 scale. The first two digits define a longitude band 0.5 degree wide and the second two digits a latitude band 0.5 degree wide."@en ;skos:inScheme <https://linked.data.gov.au/def/geoadminfeatures> ;skos:broader geoad:MapSeries ;skos:notation "7964" ;skos:prefLabel "Rumula:7964"@en .
geoad:Cairns8064 a skos:Concept ;skos:definition "Map sheet for Cairns at 1:100 000 scale. The first two digits define a longitude band 0.5 degree wide and the second two digits a latitude band 0.5 degree wide."@en ;skos:inScheme <https://linked.data.gov.au/def/geoadminfeatures> ;skos:broader geoad:MapSeries ;skos:notation "8064" ;skos:prefLabel "Cairns:8064"@en .
geoad:Westmoreland6563 a skos:Concept ;skos:definition "Map sheet for Westmoreland at 1:100 000 scale. The first two digits define a longitude band 0.5 degree wide and the second two digits a latitude band 0.5 degree wide."@en ;skos:inScheme <https://linked.data.gov.au/def/geoadminfeatures> ;skos:broader geoad:MapSeries ;skos:notation "6563" ;skos:prefLabel "Westmoreland:6563"@en .
geoad:BallysLagoon6663 a skos:Concept ;skos:definition "Map sheet for Ballys Lagoon at 1:100 000 scale. The first two digits define a longitude band 0.5 degree wide and the second two digits a latitude band 0.5 degree wide."@en ;skos:inScheme <https://linked.data.gov.au/def/geoadminfeatures> ;skos:broader geoad:MapSeries ;skos:notation "6663" ;skos:prefLabel "Ballys Lagoon:6663"@en .
geoad:PointParker6763 a skos:Concept ;skos:definition "Map sheet for Point Parker at 1:100 000 scale. The first two digits define a longitude band 0.5 degree wide and the second two digits a latitude band 0.5 degree wide."@en ;skos:inScheme <https://linked.data.gov.au/def/geoadminfeatures> ;skos:broader geoad:MapSeries ;skos:notation "6763" ;skos:prefLabel "Point Parker:6763"@en .
geoad:SweersIsland6863 a skos:Concept ;skos:definition "Map sheet for Sweers Island at 1:100 000 scale. The first two digits define a longitude band 0.5 degree wide and the second two digits a latitude band 0.5 degree wide."@en ;skos:inScheme <https://linked.data.gov.au/def/geoadminfeatures> ;skos:broader geoad:MapSeries ;skos:notation "6863" ;skos:prefLabel "Sweers Island:6863"@en .
geoad:Karumba7063 a skos:Concept ;skos:definition "Map sheet for Karumba at 1:100 000 scale. The first two digits define a longitude band 0.5 degree wide and the second two digits a latitude band 0.5 degree wide."@en ;skos:inScheme <https://linked.data.gov.au/def/geoadminfeatures> ;skos:broader geoad:MapSeries ;skos:notation "7063" ;skos:prefLabel "Karumba:7063"@en .
geoad:DoubleLagoon7163 a skos:Concept ;skos:definition "Map sheet for Double Lagoon at 1:100 000 scale. The first two digits define a longitude band 0.5 degree wide and the second two digits a latitude band 0.5 degree wide."@en ;skos:inScheme <https://linked.data.gov.au/def/geoadminfeatures> ;skos:broader geoad:MapSeries ;skos:notation "7163" ;skos:prefLabel "Double Lagoon:7163"@en .
geoad:Stirling7263 a skos:Concept ;skos:definition "Map sheet for Stirling at 1:100 000 scale. The first two digits define a longitude band 0.5 degree wide and the second two digits a latitude band 0.5 degree wide."@en ;skos:inScheme <https://linked.data.gov.au/def/geoadminfeatures> ;skos:broader geoad:MapSeries ;skos:notation "7263" ;skos:prefLabel "Stirling:7263"@en .
geoad:EchoCreek7363 a skos:Concept ;skos:definition "Map sheet for Echo Creek at 1:100 000 scale. The first two digits define a longitude band 0.5 degree wide and the second two digits a latitude band 0.5 degree wide."@en ;skos:inScheme <https://linked.data.gov.au/def/geoadminfeatures> ;skos:broader geoad:MapSeries ;skos:notation "7363" ;skos:prefLabel "Echo Creek:7363"@en .
geoad:CrookedCreek7463 a skos:Concept ;skos:definition "Map sheet for Crooked Creek at 1:100 000 scale. The first two digits define a longitude band 0.5 degree wide and the second two digits a latitude band 0.5 degree wide."@en ;skos:inScheme <https://linked.data.gov.au/def/geoadminfeatures> ;skos:broader geoad:MapSeries ;skos:notation "7463" ;skos:prefLabel "Crooked Creek:7463"@en .
geoad:RedRiver7563 a skos:Concept ;skos:definition "Map sheet for Red River at 1:100 000 scale. The first two digits define a longitude band 0.5 degree wide and the second two digits a latitude band 0.5 degree wide."@en ;skos:inScheme <https://linked.data.gov.au/def/geoadminfeatures> ;skos:broader geoad:MapSeries ;skos:notation "7563" ;skos:prefLabel "Red River:7563"@en .
geoad:Blackdown7663 a skos:Concept ;skos:definition "Map sheet for Blackdown at 1:100 000 scale. The first two digits define a longitude band 0.5 degree wide and the second two digits a latitude band 0.5 degree wide."@en ;skos:inScheme <https://linked.data.gov.au/def/geoadminfeatures> ;skos:broader geoad:MapSeries ;skos:notation "7663" ;skos:prefLabel "Blackdown:7663"@en .
geoad:Mungana7763 a skos:Concept ;skos:definition "Map sheet for Mungana at 1:100 000 scale. The first two digits define a longitude band 0.5 degree wide and the second two digits a latitude band 0.5 degree wide."@en ;skos:inScheme <https://linked.data.gov.au/def/geoadminfeatures> ;skos:broader geoad:MapSeries ;skos:notation "7763" ;skos:prefLabel "Mungana:7763"@en .
geoad:Chillagoe7863 a skos:Concept ;skos:definition "Map sheet for Chillagoe at 1:100 000 scale. The first two digits define a longitude band 0.5 degree wide and the second two digits a latitude band 0.5 degree wide."@en ;skos:inScheme <https://linked.data.gov.au/def/geoadminfeatures> ;skos:broader geoad:MapSeries ;skos:notation "7863" ;skos:prefLabel "Chillagoe:7863"@en .
geoad:Atherton7963 a skos:Concept ;skos:definition "Map sheet for Atherton at 1:100 000 scale. The first two digits define a longitude band 0.5 degree wide and the second two digits a latitude band 0.5 degree wide."@en ;skos:inScheme <https://linked.data.gov.au/def/geoadminfeatures> ;skos:broader geoad:MapSeries ;skos:notation "7963" ;skos:prefLabel "Atherton:7963"@en .
geoad:BartleFrere8063 a skos:Concept ;skos:definition "Map sheet for Bartle Frere at 1:100 000 scale. The first two digits define a longitude band 0.5 degree wide and the second two digits a latitude band 0.5 degree wide."@en ;skos:inScheme <https://linked.data.gov.au/def/geoadminfeatures> ;skos:broader geoad:MapSeries ;skos:notation "8063" ;skos:prefLabel "Bartle Frere:8063"@en .
geoad:CooperPoint8163 a skos:Concept ;skos:definition "Map sheet for Cooper Point at 1:100 000 scale. The first two digits define a longitude band 0.5 degree wide and the second two digits a latitude band 0.5 degree wide."@en ;skos:inScheme <https://linked.data.gov.au/def/geoadminfeatures> ;skos:broader geoad:MapSeries ;skos:notation "8163" ;skos:prefLabel "Cooper Point:8163"@en .
geoad:HedleysCreek6562 a skos:Concept ;skos:definition "Map sheet for Hedleys Creek at 1:100 000 scale. The first two digits define a longitude band 0.5 degree wide and the second two digits a latitude band 0.5 degree wide."@en ;skos:inScheme <https://linked.data.gov.au/def/geoadminfeatures> ;skos:broader geoad:MapSeries ;skos:notation "6562" ;skos:prefLabel "Hedleys Creek:6562"@en .
geoad:Doomadgee6662 a skos:Concept ;skos:definition "Map sheet for Doomadgee at 1:100 000 scale. The first two digits define a longitude band 0.5 degree wide and the second two digits a latitude band 0.5 degree wide."@en ;skos:inScheme <https://linked.data.gov.au/def/geoadminfeatures> ;skos:broader geoad:MapSeries ;skos:notation "6662" ;skos:prefLabel "Doomadgee:6662"@en .
geoad:Escott6762 a skos:Concept ;skos:definition "Map sheet for Escott at 1:100 000 scale. The first two digits define a longitude band 0.5 degree wide and the second two digits a latitude band 0.5 degree wide."@en ;skos:inScheme <https://linked.data.gov.au/def/geoadminfeatures> ;skos:broader geoad:MapSeries ;skos:notation "6762" ;skos:prefLabel "Escott:6762"@en .
geoad:Burketown6862 a skos:Concept ;skos:definition "Map sheet for Burketown at 1:100 000 scale. The first two digits define a longitude band 0.5 degree wide and the second two digits a latitude band 0.5 degree wide."@en ;skos:inScheme <https://linked.data.gov.au/def/geoadminfeatures> ;skos:broader geoad:MapSeries ;skos:notation "6862" ;skos:prefLabel "Burketown:6862"@en .
geoad:MiddlePoint6962 a skos:Concept ;skos:definition "Map sheet for Middle Point at 1:100 000 scale. The first two digits define a longitude band 0.5 degree wide and the second two digits a latitude band 0.5 degree wide."@en ;skos:inScheme <https://linked.data.gov.au/def/geoadminfeatures> ;skos:broader geoad:MapSeries ;skos:notation "6962" ;skos:prefLabel "Middle Point:6962"@en .
geoad:Magowra7062 a skos:Concept ;skos:definition "Map sheet for Magowra at 1:100 000 scale. The first two digits define a longitude band 0.5 degree wide and the second two digits a latitude band 0.5 degree wide."@en ;skos:inScheme <https://linked.data.gov.au/def/geoadminfeatures> ;skos:broader geoad:MapSeries ;skos:notation "7062" ;skos:prefLabel "Magowra:7062"@en .
geoad:Normanton7162 a skos:Concept ;skos:definition "Map sheet for Normanton at 1:100 000 scale. The first two digits define a longitude band 0.5 degree wide and the second two digits a latitude band 0.5 degree wide."@en ;skos:inScheme <https://linked.data.gov.au/def/geoadminfeatures> ;skos:broader geoad:MapSeries ;skos:notation "7162" ;skos:prefLabel "Normanton:7162"@en .
geoad:Blackbull7262 a skos:Concept ;skos:definition "Map sheet for Blackbull at 1:100 000 scale. The first two digits define a longitude band 0.5 degree wide and the second two digits a latitude band 0.5 degree wide."@en ;skos:inScheme <https://linked.data.gov.au/def/geoadminfeatures> ;skos:broader geoad:MapSeries ;skos:notation "7262" ;skos:prefLabel "Blackbull:7262"@en .
geoad:Wallabadah7362 a skos:Concept ;skos:definition "Map sheet for Wallabadah at 1:100 000 scale. The first two digits define a longitude band 0.5 degree wide and the second two digits a latitude band 0.5 degree wide."@en ;skos:inScheme <https://linked.data.gov.au/def/geoadminfeatures> ;skos:broader geoad:MapSeries ;skos:notation "7362" ;skos:prefLabel "Wallabadah:7362"@en .
geoad:Strathmore7462 a skos:Concept ;skos:definition "Map sheet for Strathmore at 1:100 000 scale. The first two digits define a longitude band 0.5 degree wide and the second two digits a latitude band 0.5 degree wide."@en ;skos:inScheme <https://linked.data.gov.au/def/geoadminfeatures> ;skos:broader geoad:MapSeries ;skos:notation "7462" ;skos:prefLabel "Strathmore:7462"@en .
geoad:AbingdonDowns7562 a skos:Concept ;skos:definition "Map sheet for Abingdon Downs at 1:100 000 scale. The first two digits define a longitude band 0.5 degree wide and the second two digits a latitude band 0.5 degree wide."@en ;skos:inScheme <https://linked.data.gov.au/def/geoadminfeatures> ;skos:broader geoad:MapSeries ;skos:notation "7562" ;skos:prefLabel "Abingdon Downs:7562"@en .
geoad:Galloway7662 a skos:Concept ;skos:definition "Map sheet for Galloway at 1:100 000 scale. The first two digits define a longitude band 0.5 degree wide and the second two digits a latitude band 0.5 degree wide."@en ;skos:inScheme <https://linked.data.gov.au/def/geoadminfeatures> ;skos:broader geoad:MapSeries ;skos:notation "7662" ;skos:prefLabel "Galloway:7662"@en .
geoad:Lyndbrook7762 a skos:Concept ;skos:definition "Map sheet for Lyndbrook at 1:100 000 scale. The first two digits define a longitude band 0.5 degree wide and the second two digits a latitude band 0.5 degree wide."@en ;skos:inScheme <https://linked.data.gov.au/def/geoadminfeatures> ;skos:broader geoad:MapSeries ;skos:notation "7762" ;skos:prefLabel "Lyndbrook:7762"@en .
geoad:BullockCreek7862 a skos:Concept ;skos:definition "Map sheet for Bullock Creek at 1:100 000 scale. The first two digits define a longitude band 0.5 degree wide and the second two digits a latitude band 0.5 degree wide."@en ;skos:inScheme <https://linked.data.gov.au/def/geoadminfeatures> ;skos:broader geoad:MapSeries ;skos:notation "7862" ;skos:prefLabel "Bullock Creek:7862"@en .
geoad:Ravenshoe7962 a skos:Concept ;skos:definition "Map sheet for Ravenshoe at 1:100 000 scale. The first two digits define a longitude band 0.5 degree wide and the second two digits a latitude band 0.5 degree wide."@en ;skos:inScheme <https://linked.data.gov.au/def/geoadminfeatures> ;skos:broader geoad:MapSeries ;skos:notation "7962" ;skos:prefLabel "Ravenshoe:7962"@en .
geoad:Tully8062 a skos:Concept ;skos:definition "Map sheet for Tully at 1:100 000 scale. The first two digits define a longitude band 0.5 degree wide and the second two digits a latitude band 0.5 degree wide."@en ;skos:inScheme <https://linked.data.gov.au/def/geoadminfeatures> ;skos:broader geoad:MapSeries ;skos:notation "8062" ;skos:prefLabel "Tully:8062"@en .
geoad:Innisfail8162 a skos:Concept ;skos:definition "Map sheet for Innisfail at 1:100 000 scale. The first two digits define a longitude band 0.5 degree wide and the second two digits a latitude band 0.5 degree wide."@en ;skos:inScheme <https://linked.data.gov.au/def/geoadminfeatures> ;skos:broader geoad:MapSeries ;skos:notation "8162" ;skos:prefLabel "Innisfail:8162"@en .
geoad:Bowthorn6561 a skos:Concept ;skos:definition "Map sheet for Bowthorn at 1:100 000 scale. The first two digits define a longitude band 0.5 degree wide and the second two digits a latitude band 0.5 degree wide."@en ;skos:inScheme <https://linked.data.gov.au/def/geoadminfeatures> ;skos:broader geoad:MapSeries ;skos:notation "6561" ;skos:prefLabel "Bowthorn:6561"@en .
geoad:MountOscar6661 a skos:Concept ;skos:definition "Map sheet for Mount Oscar at 1:100 000 scale. The first two digits define a longitude band 0.5 degree wide and the second two digits a latitude band 0.5 degree wide."@en ;skos:inScheme <https://linked.data.gov.au/def/geoadminfeatures> ;skos:broader geoad:MapSeries ;skos:notation "6661" ;skos:prefLabel "Mount Oscar:6661"@en .
geoad:Punjaub6761 a skos:Concept ;skos:definition "Map sheet for Punjaub at 1:100 000 scale. The first two digits define a longitude band 0.5 degree wide and the second two digits a latitude band 0.5 degree wide."@en ;skos:inScheme <https://linked.data.gov.au/def/geoadminfeatures> ;skos:broader geoad:MapSeries ;skos:notation "6761" ;skos:prefLabel "Punjaub:6761"@en .
geoad:Wernadinga6861 a skos:Concept ;skos:definition "Map sheet for Wernadinga at 1:100 000 scale. The first two digits define a longitude band 0.5 degree wide and the second two digits a latitude band 0.5 degree wide."@en ;skos:inScheme <https://linked.data.gov.au/def/geoadminfeatures> ;skos:broader geoad:MapSeries ;skos:notation "6861" ;skos:prefLabel "Wernadinga:6861"@en .
geoad:NeumayerValley6961 a skos:Concept ;skos:definition "Map sheet for Neumayer Valley at 1:100 000 scale. The first two digits define a longitude band 0.5 degree wide and the second two digits a latitude band 0.5 degree wide."@en ;skos:inScheme <https://linked.data.gov.au/def/geoadminfeatures> ;skos:broader geoad:MapSeries ;skos:notation "6961" ;skos:prefLabel "Neumayer Valley:6961"@en .
geoad:Milgarra7061 a skos:Concept ;skos:definition "Map sheet for Milgarra at 1:100 000 scale. The first two digits define a longitude band 0.5 degree wide and the second two digits a latitude band 0.5 degree wide."@en ;skos:inScheme <https://linked.data.gov.au/def/geoadminfeatures> ;skos:broader geoad:MapSeries ;skos:notation "7061" ;skos:prefLabel "Milgarra:7061"@en .
geoad:BrownCreek7161 a skos:Concept ;skos:definition "Map sheet for Brown Creek at 1:100 000 scale. The first two digits define a longitude band 0.5 degree wide and the second two digits a latitude band 0.5 degree wide."@en ;skos:inScheme <https://linked.data.gov.au/def/geoadminfeatures> ;skos:broader geoad:MapSeries ;skos:notation "7161" ;skos:prefLabel "Brown Creek:7161"@en .
geoad:Coralie7261 a skos:Concept ;skos:definition "Map sheet for Coralie at 1:100 000 scale. The first two digits define a longitude band 0.5 degree wide and the second two digits a latitude band 0.5 degree wide."@en ;skos:inScheme <https://linked.data.gov.au/def/geoadminfeatures> ;skos:broader geoad:MapSeries ;skos:notation "7261" ;skos:prefLabel "Coralie:7261"@en .
geoad:Croydon7361 a skos:Concept ;skos:definition "Map sheet for Croydon at 1:100 000 scale. The first two digits define a longitude band 0.5 degree wide and the second two digits a latitude band 0.5 degree wide."@en ;skos:inScheme <https://linked.data.gov.au/def/geoadminfeatures> ;skos:broader geoad:MapSeries ;skos:notation "7361" ;skos:prefLabel "Croydon:7361"@en .
geoad:GilbertRiver7461 a skos:Concept ;skos:definition "Map sheet for Gilbert River at 1:100 000 scale. The first two digits define a longitude band 0.5 degree wide and the second two digits a latitude band 0.5 degree wide."@en ;skos:inScheme <https://linked.data.gov.au/def/geoadminfeatures> ;skos:broader geoad:MapSeries ;skos:notation "7461" ;skos:prefLabel "Gilbert River:7461"@en .
geoad:ForestHome7561 a skos:Concept ;skos:definition "Map sheet for Forest Home at 1:100 000 scale. The first two digits define a longitude band 0.5 degree wide and the second two digits a latitude band 0.5 degree wide."@en ;skos:inScheme <https://linked.data.gov.au/def/geoadminfeatures> ;skos:broader geoad:MapSeries ;skos:notation "7561" ;skos:prefLabel "Forest Home:7561"@en .
geoad:Georgetown7661 a skos:Concept ;skos:definition "Map sheet for Georgetown at 1:100 000 scale. The first two digits define a longitude band 0.5 degree wide and the second two digits a latitude band 0.5 degree wide."@en ;skos:inScheme <https://linked.data.gov.au/def/geoadminfeatures> ;skos:broader geoad:MapSeries ;skos:notation "7661" ;skos:prefLabel "Georgetown:7661"@en .
geoad:MountSurprise7761 a skos:Concept ;skos:definition "Map sheet for Mount Surprise at 1:100 000 scale. The first two digits define a longitude band 0.5 degree wide and the second two digits a latitude band 0.5 degree wide."@en ;skos:inScheme <https://linked.data.gov.au/def/geoadminfeatures> ;skos:broader geoad:MapSeries ;skos:notation "7761" ;skos:prefLabel "Mount Surprise:7761"@en .
geoad:StRonans7861 a skos:Concept ;skos:definition "Map sheet for St Ronans at 1:100 000 scale. The first two digits define a longitude band 0.5 degree wide and the second two digits a latitude band 0.5 degree wide."@en ;skos:inScheme <https://linked.data.gov.au/def/geoadminfeatures> ;skos:broader geoad:MapSeries ;skos:notation "7861" ;skos:prefLabel "St Ronans:7861"@en .
geoad:Cashmere7961 a skos:Concept ;skos:definition "Map sheet for Cashmere at 1:100 000 scale. The first two digits define a longitude band 0.5 degree wide and the second two digits a latitude band 0.5 degree wide."@en ;skos:inScheme <https://linked.data.gov.au/def/geoadminfeatures> ;skos:broader geoad:MapSeries ;skos:notation "7961" ;skos:prefLabel "Cashmere:7961"@en .
geoad:Kirrama8061 a skos:Concept ;skos:definition "Map sheet for Kirrama at 1:100 000 scale. The first two digits define a longitude band 0.5 degree wide and the second two digits a latitude band 0.5 degree wide."@en ;skos:inScheme <https://linked.data.gov.au/def/geoadminfeatures> ;skos:broader geoad:MapSeries ;skos:notation "8061" ;skos:prefLabel "Kirrama:8061"@en .
geoad:Cardwell8161 a skos:Concept ;skos:definition "Map sheet for Cardwell at 1:100 000 scale. The first two digits define a longitude band 0.5 degree wide and the second two digits a latitude band 0.5 degree wide."@en ;skos:inScheme <https://linked.data.gov.au/def/geoadminfeatures> ;skos:broader geoad:MapSeries ;skos:notation "8161" ;skos:prefLabel "Cardwell:8161"@en .
geoad:Musselbrook6560 a skos:Concept ;skos:definition "Map sheet for Musselbrook at 1:100 000 scale. The first two digits define a longitude band 0.5 degree wide and the second two digits a latitude band 0.5 degree wide."@en ;skos:inScheme <https://linked.data.gov.au/def/geoadminfeatures> ;skos:broader geoad:MapSeries ;skos:notation "6560" ;skos:prefLabel "Musselbrook:6560"@en .
geoad:LawnHill6660 a skos:Concept ;skos:definition "Map sheet for Lawn Hill at 1:100 000 scale. The first two digits define a longitude band 0.5 degree wide and the second two digits a latitude band 0.5 degree wide."@en ;skos:inScheme <https://linked.data.gov.au/def/geoadminfeatures> ;skos:broader geoad:MapSeries ;skos:notation "6660" ;skos:prefLabel "Lawn Hill:6660"@en .
geoad:GregoryDowns6760 a skos:Concept ;skos:definition "Map sheet for Gregory Downs at 1:100 000 scale. The first two digits define a longitude band 0.5 degree wide and the second two digits a latitude band 0.5 degree wide."@en ;skos:inScheme <https://linked.data.gov.au/def/geoadminfeatures> ;skos:broader geoad:MapSeries ;skos:notation "6760" ;skos:prefLabel "Gregory Downs:6760"@en .
geoad:AugustusDowns6860 a skos:Concept ;skos:definition "Map sheet for Augustus Downs at 1:100 000 scale. The first two digits define a longitude band 0.5 degree wide and the second two digits a latitude band 0.5 degree wide."@en ;skos:inScheme <https://linked.data.gov.au/def/geoadminfeatures> ;skos:broader geoad:MapSeries ;skos:notation "6860" ;skos:prefLabel "Augustus Downs:6860"@en .
geoad:Talawanta6960 a skos:Concept ;skos:definition "Map sheet for Talawanta at 1:100 000 scale. The first two digits define a longitude band 0.5 degree wide and the second two digits a latitude band 0.5 degree wide."@en ;skos:inScheme <https://linked.data.gov.au/def/geoadminfeatures> ;skos:broader geoad:MapSeries ;skos:notation "6960" ;skos:prefLabel "Talawanta:6960"@en .
geoad:DonorsHill7060 a skos:Concept ;skos:definition "Map sheet for Donors Hill at 1:100 000 scale. The first two digits define a longitude band 0.5 degree wide and the second two digits a latitude band 0.5 degree wide."@en ;skos:inScheme <https://linked.data.gov.au/def/geoadminfeatures> ;skos:broader geoad:MapSeries ;skos:notation "7060" ;skos:prefLabel "Donors Hill:7060"@en .
geoad:Iffley7160 a skos:Concept ;skos:definition "Map sheet for Iffley at 1:100 000 scale. The first two digits define a longitude band 0.5 degree wide and the second two digits a latitude band 0.5 degree wide."@en ;skos:inScheme <https://linked.data.gov.au/def/geoadminfeatures> ;skos:broader geoad:MapSeries ;skos:notation "7160" ;skos:prefLabel "Iffley:7160"@en .
geoad:Claraville7260 a skos:Concept ;skos:definition "Map sheet for Claraville at 1:100 000 scale. The first two digits define a longitude band 0.5 degree wide and the second two digits a latitude band 0.5 degree wide."@en ;skos:inScheme <https://linked.data.gov.au/def/geoadminfeatures> ;skos:broader geoad:MapSeries ;skos:notation "7260" ;skos:prefLabel "Claraville:7260"@en .
geoad:Prospect7360 a skos:Concept ;skos:definition "Map sheet for Prospect at 1:100 000 scale. The first two digits define a longitude band 0.5 degree wide and the second two digits a latitude band 0.5 degree wide."@en ;skos:inScheme <https://linked.data.gov.au/def/geoadminfeatures> ;skos:broader geoad:MapSeries ;skos:notation "7360" ;skos:prefLabel "Prospect:7360"@en .
geoad:Esmeralda7460 a skos:Concept ;skos:definition "Map sheet for Esmeralda at 1:100 000 scale. The first two digits define a longitude band 0.5 degree wide and the second two digits a latitude band 0.5 degree wide."@en ;skos:inScheme <https://linked.data.gov.au/def/geoadminfeatures> ;skos:broader geoad:MapSeries ;skos:notation "7460" ;skos:prefLabel "Esmeralda:7460"@en .
geoad:NorthHead7560 a skos:Concept ;skos:definition "Map sheet for North Head at 1:100 000 scale. The first two digits define a longitude band 0.5 degree wide and the second two digits a latitude band 0.5 degree wide."@en ;skos:inScheme <https://linked.data.gov.au/def/geoadminfeatures> ;skos:broader geoad:MapSeries ;skos:notation "7560" ;skos:prefLabel "North Head:7560"@en .
geoad:Forsayth7660 a skos:Concept ;skos:definition "Map sheet for Forsayth at 1:100 000 scale. The first two digits define a longitude band 0.5 degree wide and the second two digits a latitude band 0.5 degree wide."@en ;skos:inScheme <https://linked.data.gov.au/def/geoadminfeatures> ;skos:broader geoad:MapSeries ;skos:notation "7660" ;skos:prefLabel "Forsayth:7660"@en .
geoad:Einasleigh7760 a skos:Concept ;skos:definition "Map sheet for Einasleigh at 1:100 000 scale. The first two digits define a longitude band 0.5 degree wide and the second two digits a latitude band 0.5 degree wide."@en ;skos:inScheme <https://linked.data.gov.au/def/geoadminfeatures> ;skos:broader geoad:MapSeries ;skos:notation "7760" ;skos:prefLabel "Einasleigh:7760"@en .
geoad:Conjuboy7860 a skos:Concept ;skos:definition "Map sheet for Conjuboy at 1:100 000 scale. The first two digits define a longitude band 0.5 degree wide and the second two digits a latitude band 0.5 degree wide."@en ;skos:inScheme <https://linked.data.gov.au/def/geoadminfeatures> ;skos:broader geoad:MapSeries ;skos:notation "7860" ;skos:prefLabel "Conjuboy:7860"@en .
geoad:ValleyOfLagoons7960 a skos:Concept ;skos:definition "Map sheet for Valley Of Lagoons at 1:100 000 scale. The first two digits define a longitude band 0.5 degree wide and the second two digits a latitude band 0.5 degree wide."@en ;skos:inScheme <https://linked.data.gov.au/def/geoadminfeatures> ;skos:broader geoad:MapSeries ;skos:notation "7960" ;skos:prefLabel "Valley Of Lagoons:7960"@en .
geoad:KangarooHills8060 a skos:Concept ;skos:definition "Map sheet for Kangaroo Hills at 1:100 000 scale. The first two digits define a longitude band 0.5 degree wide and the second two digits a latitude band 0.5 degree wide."@en ;skos:inScheme <https://linked.data.gov.au/def/geoadminfeatures> ;skos:broader geoad:MapSeries ;skos:notation "8060" ;skos:prefLabel "Kangaroo Hills:8060"@en .
geoad:Ingham8160 a skos:Concept ;skos:definition "Map sheet for Ingham at 1:100 000 scale. The first two digits define a longitude band 0.5 degree wide and the second two digits a latitude band 0.5 degree wide."@en ;skos:inScheme <https://linked.data.gov.au/def/geoadminfeatures> ;skos:broader geoad:MapSeries ;skos:notation "8160" ;skos:prefLabel "Ingham:8160"@en .
geoad:PalmIslands8260 a skos:Concept ;skos:definition "Map sheet for Palm Islands at 1:100 000 scale. The first two digits define a longitude band 0.5 degree wide and the second two digits a latitude band 0.5 degree wide."@en ;skos:inScheme <https://linked.data.gov.au/def/geoadminfeatures> ;skos:broader geoad:MapSeries ;skos:notation "8260" ;skos:prefLabel "Palm Islands:8260"@en .
geoad:Norfolk6559 a skos:Concept ;skos:definition "Map sheet for Norfolk at 1:100 000 scale. The first two digits define a longitude band 0.5 degree wide and the second two digits a latitude band 0.5 degree wide."@en ;skos:inScheme <https://linked.data.gov.au/def/geoadminfeatures> ;skos:broader geoad:MapSeries ;skos:notation "6559" ;skos:prefLabel "Norfolk:6559"@en .
geoad:Riversleigh6659 a skos:Concept ;skos:definition "Map sheet for Riversleigh at 1:100 000 scale. The first two digits define a longitude band 0.5 degree wide and the second two digits a latitude band 0.5 degree wide."@en ;skos:inScheme <https://linked.data.gov.au/def/geoadminfeatures> ;skos:broader geoad:MapSeries ;skos:notation "6659" ;skos:prefLabel "Riversleigh:6659"@en .
geoad:MountOxide6759 a skos:Concept ;skos:definition "Map sheet for Mount Oxide at 1:100 000 scale. The first two digits define a longitude band 0.5 degree wide and the second two digits a latitude band 0.5 degree wide."@en ;skos:inScheme <https://linked.data.gov.au/def/geoadminfeatures> ;skos:broader geoad:MapSeries ;skos:notation "6759" ;skos:prefLabel "Mount Oxide:6759"@en .
geoad:Myally6859 a skos:Concept ;skos:definition "Map sheet for Myally at 1:100 000 scale. The first two digits define a longitude band 0.5 degree wide and the second two digits a latitude band 0.5 degree wide."@en ;skos:inScheme <https://linked.data.gov.au/def/geoadminfeatures> ;skos:broader geoad:MapSeries ;skos:notation "6859" ;skos:prefLabel "Myally:6859"@en .
geoad:Kamileroi6959 a skos:Concept ;skos:definition "Map sheet for Kamileroi at 1:100 000 scale. The first two digits define a longitude band 0.5 degree wide and the second two digits a latitude band 0.5 degree wide."@en ;skos:inScheme <https://linked.data.gov.au/def/geoadminfeatures> ;skos:broader geoad:MapSeries ;skos:notation "6959" ;skos:prefLabel "Kamileroi:6959"@en .
geoad:Canobie7059 a skos:Concept ;skos:definition "Map sheet for Canobie at 1:100 000 scale. The first two digits define a longitude band 0.5 degree wide and the second two digits a latitude band 0.5 degree wide."@en ;skos:inScheme <https://linked.data.gov.au/def/geoadminfeatures> ;skos:broader geoad:MapSeries ;skos:notation "7059" ;skos:prefLabel "Canobie:7059"@en .
geoad:Taldora7159 a skos:Concept ;skos:definition "Map sheet for Taldora at 1:100 000 scale. The first two digits define a longitude band 0.5 degree wide and the second two digits a latitude band 0.5 degree wide."@en ;skos:inScheme <https://linked.data.gov.au/def/geoadminfeatures> ;skos:broader geoad:MapSeries ;skos:notation "7159" ;skos:prefLabel "Taldora:7159"@en .
geoad:SavannahDowns7259 a skos:Concept ;skos:definition "Map sheet for Savannah Downs at 1:100 000 scale. The first two digits define a longitude band 0.5 degree wide and the second two digits a latitude band 0.5 degree wide."@en ;skos:inScheme <https://linked.data.gov.au/def/geoadminfeatures> ;skos:broader geoad:MapSeries ;skos:notation "7259" ;skos:prefLabel "Savannah Downs:7259"@en .
geoad:Trenton7359 a skos:Concept ;skos:definition "Map sheet for Trenton at 1:100 000 scale. The first two digits define a longitude band 0.5 degree wide and the second two digits a latitude band 0.5 degree wide."@en ;skos:inScheme <https://linked.data.gov.au/def/geoadminfeatures> ;skos:broader geoad:MapSeries ;skos:notation "7359" ;skos:prefLabel "Trenton:7359"@en .
geoad:Pelham7459 a skos:Concept ;skos:definition "Map sheet for Pelham at 1:100 000 scale. The first two digits define a longitude band 0.5 degree wide and the second two digits a latitude band 0.5 degree wide."@en ;skos:inScheme <https://linked.data.gov.au/def/geoadminfeatures> ;skos:broader geoad:MapSeries ;skos:notation "7459" ;skos:prefLabel "Pelham:7459"@en .
geoad:Bellfield7559 a skos:Concept ;skos:definition "Map sheet for Bellfield at 1:100 000 scale. The first two digits define a longitude band 0.5 degree wide and the second two digits a latitude band 0.5 degree wide."@en ;skos:inScheme <https://linked.data.gov.au/def/geoadminfeatures> ;skos:broader geoad:MapSeries ;skos:notation "7559" ;skos:prefLabel "Bellfield:7559"@en .
geoad:Gilberton7659 a skos:Concept ;skos:definition "Map sheet for Gilberton at 1:100 000 scale. The first two digits define a longitude band 0.5 degree wide and the second two digits a latitude band 0.5 degree wide."@en ;skos:inScheme <https://linked.data.gov.au/def/geoadminfeatures> ;skos:broader geoad:MapSeries ;skos:notation "7659" ;skos:prefLabel "Gilberton:7659"@en .
geoad:Lyndhurst7759 a skos:Concept ;skos:definition "Map sheet for Lyndhurst at 1:100 000 scale. The first two digits define a longitude band 0.5 degree wide and the second two digits a latitude band 0.5 degree wide."@en ;skos:inScheme <https://linked.data.gov.au/def/geoadminfeatures> ;skos:broader geoad:MapSeries ;skos:notation "7759" ;skos:prefLabel "Lyndhurst:7759"@en .
geoad:Burges7859 a skos:Concept ;skos:definition "Map sheet for Burges at 1:100 000 scale. The first two digits define a longitude band 0.5 degree wide and the second two digits a latitude band 0.5 degree wide."@en ;skos:inScheme <https://linked.data.gov.au/def/geoadminfeatures> ;skos:broader geoad:MapSeries ;skos:notation "7859" ;skos:prefLabel "Burges:7859"@en .
geoad:ClarkeRiver7959 a skos:Concept ;skos:definition "Map sheet for Clarke River at 1:100 000 scale. The first two digits define a longitude band 0.5 degree wide and the second two digits a latitude band 0.5 degree wide."@en ;skos:inScheme <https://linked.data.gov.au/def/geoadminfeatures> ;skos:broader geoad:MapSeries ;skos:notation "7959" ;skos:prefLabel "Clarke River:7959"@en .
geoad:Ewan8059 a skos:Concept ;skos:definition "Map sheet for Ewan at 1:100 000 scale. The first two digits define a longitude band 0.5 degree wide and the second two digits a latitude band 0.5 degree wide."@en ;skos:inScheme <https://linked.data.gov.au/def/geoadminfeatures> ;skos:broader geoad:MapSeries ;skos:notation "8059" ;skos:prefLabel "Ewan:8059"@en .
geoad:Rollingstone8159 a skos:Concept ;skos:definition "Map sheet for Rollingstone at 1:100 000 scale. The first two digits define a longitude band 0.5 degree wide and the second two digits a latitude band 0.5 degree wide."@en ;skos:inScheme <https://linked.data.gov.au/def/geoadminfeatures> ;skos:broader geoad:MapSeries ;skos:notation "8159" ;skos:prefLabel "Rollingstone:8159"@en .
geoad:Townsville8259 a skos:Concept ;skos:definition "Map sheet for Townsville at 1:100 000 scale. The first two digits define a longitude band 0.5 degree wide and the second two digits a latitude band 0.5 degree wide."@en ;skos:inScheme <https://linked.data.gov.au/def/geoadminfeatures> ;skos:broader geoad:MapSeries ;skos:notation "8259" ;skos:prefLabel "Townsville:8259"@en .
geoad:BowlingGreenBay8359 a skos:Concept ;skos:definition "Map sheet for Bowling Green Bay at 1:100 000 scale. The first two digits define a longitude band 0.5 degree wide and the second two digits a latitude band 0.5 degree wide."@en ;skos:inScheme <https://linked.data.gov.au/def/geoadminfeatures> ;skos:broader geoad:MapSeries ;skos:notation "8359" ;skos:prefLabel "Bowling Green Bay:8359"@en .
geoad:Camooweal6558 a skos:Concept ;skos:definition "Map sheet for Camooweal at 1:100 000 scale. The first two digits define a longitude band 0.5 degree wide and the second two digits a latitude band 0.5 degree wide."@en ;skos:inScheme <https://linked.data.gov.au/def/geoadminfeatures> ;skos:broader geoad:MapSeries ;skos:notation "6558" ;skos:prefLabel "Camooweal:6558"@en .
geoad:Undilla6658 a skos:Concept ;skos:definition "Map sheet for Undilla at 1:100 000 scale. The first two digits define a longitude band 0.5 degree wide and the second two digits a latitude band 0.5 degree wide."@en ;skos:inScheme <https://linked.data.gov.au/def/geoadminfeatures> ;skos:broader geoad:MapSeries ;skos:notation "6658" ;skos:prefLabel "Undilla:6658"@en .
geoad:MammothMines6758 a skos:Concept ;skos:definition "Map sheet for Mammoth Mines at 1:100 000 scale. The first two digits define a longitude band 0.5 degree wide and the second two digits a latitude band 0.5 degree wide."@en ;skos:inScheme <https://linked.data.gov.au/def/geoadminfeatures> ;skos:broader geoad:MapSeries ;skos:notation "6758" ;skos:prefLabel "Mammoth Mines:6758"@en .
geoad:Alsace6858 a skos:Concept ;skos:definition "Map sheet for Alsace at 1:100 000 scale. The first two digits define a longitude band 0.5 degree wide and the second two digits a latitude band 0.5 degree wide."@en ;skos:inScheme <https://linked.data.gov.au/def/geoadminfeatures> ;skos:broader geoad:MapSeries ;skos:notation "6858" ;skos:prefLabel "Alsace:6858"@en .
geoad:Coolullah6958 a skos:Concept ;skos:definition "Map sheet for Coolullah at 1:100 000 scale. The first two digits define a longitude band 0.5 degree wide and the second two digits a latitude band 0.5 degree wide."@en ;skos:inScheme <https://linked.data.gov.au/def/geoadminfeatures> ;skos:broader geoad:MapSeries ;skos:notation "6958" ;skos:prefLabel "Coolullah:6958"@en .
geoad:Alcala7058 a skos:Concept ;skos:definition "Map sheet for Alcala at 1:100 000 scale. The first two digits define a longitude band 0.5 degree wide and the second two digits a latitude band 0.5 degree wide."@en ;skos:inScheme <https://linked.data.gov.au/def/geoadminfeatures> ;skos:broader geoad:MapSeries ;skos:notation "7058" ;skos:prefLabel "Alcala:7058"@en .
geoad:Numil7158 a skos:Concept ;skos:definition "Map sheet for Numil at 1:100 000 scale. The first two digits define a longitude band 0.5 degree wide and the second two digits a latitude band 0.5 degree wide."@en ;skos:inScheme <https://linked.data.gov.au/def/geoadminfeatures> ;skos:broader geoad:MapSeries ;skos:notation "7158" ;skos:prefLabel "Numil:7158"@en .
geoad:Millungera7258 a skos:Concept ;skos:definition "Map sheet for Millungera at 1:100 000 scale. The first two digits define a longitude band 0.5 degree wide and the second two digits a latitude band 0.5 degree wide."@en ;skos:inScheme <https://linked.data.gov.au/def/geoadminfeatures> ;skos:broader geoad:MapSeries ;skos:notation "7258" ;skos:prefLabel "Millungera:7258"@en .
geoad:Malpas7358 a skos:Concept ;skos:definition "Map sheet for Malpas at 1:100 000 scale. The first two digits define a longitude band 0.5 degree wide and the second two digits a latitude band 0.5 degree wide."@en ;skos:inScheme <https://linked.data.gov.au/def/geoadminfeatures> ;skos:broader geoad:MapSeries ;skos:notation "7358" ;skos:prefLabel "Malpas:7358"@en .
geoad:Etheldale7458 a skos:Concept ;skos:definition "Map sheet for Etheldale at 1:100 000 scale. The first two digits define a longitude band 0.5 degree wide and the second two digits a latitude band 0.5 degree wide."@en ;skos:inScheme <https://linked.data.gov.au/def/geoadminfeatures> ;skos:broader geoad:MapSeries ;skos:notation "7458" ;skos:prefLabel "Etheldale:7458"@en .
geoad:MountNorman7558 a skos:Concept ;skos:definition "Map sheet for Mount Norman at 1:100 000 scale. The first two digits define a longitude band 0.5 degree wide and the second two digits a latitude band 0.5 degree wide."@en ;skos:inScheme <https://linked.data.gov.au/def/geoadminfeatures> ;skos:broader geoad:MapSeries ;skos:notation "7558" ;skos:prefLabel "Mount Norman:7558"@en .
geoad:Hampstead7658 a skos:Concept ;skos:definition "Map sheet for Hampstead at 1:100 000 scale. The first two digits define a longitude band 0.5 degree wide and the second two digits a latitude band 0.5 degree wide."@en ;skos:inScheme <https://linked.data.gov.au/def/geoadminfeatures> ;skos:broader geoad:MapSeries ;skos:notation "7658" ;skos:prefLabel "Hampstead:7658"@en .
geoad:ChudleighPark7758 a skos:Concept ;skos:definition "Map sheet for Chudleigh Park at 1:100 000 scale. The first two digits define a longitude band 0.5 degree wide and the second two digits a latitude band 0.5 degree wide."@en ;skos:inScheme <https://linked.data.gov.au/def/geoadminfeatures> ;skos:broader geoad:MapSeries ;skos:notation "7758" ;skos:prefLabel "Chudleigh Park:7758"@en .
geoad:WandoVale7858 a skos:Concept ;skos:definition "Map sheet for Wando Vale at 1:100 000 scale. The first two digits define a longitude band 0.5 degree wide and the second two digits a latitude band 0.5 degree wide."@en ;skos:inScheme <https://linked.data.gov.au/def/geoadminfeatures> ;skos:broader geoad:MapSeries ;skos:notation "7858" ;skos:prefLabel "Wando Vale:7858"@en .
geoad:Maryvale7958 a skos:Concept ;skos:definition "Map sheet for Maryvale at 1:100 000 scale. The first two digits define a longitude band 0.5 degree wide and the second two digits a latitude band 0.5 degree wide."@en ;skos:inScheme <https://linked.data.gov.au/def/geoadminfeatures> ;skos:broader geoad:MapSeries ;skos:notation "7958" ;skos:prefLabel "Maryvale:7958"@en .
geoad:Hillgrove8058 a skos:Concept ;skos:definition "Map sheet for Hillgrove at 1:100 000 scale. The first two digits define a longitude band 0.5 degree wide and the second two digits a latitude band 0.5 degree wide."@en ;skos:inScheme <https://linked.data.gov.au/def/geoadminfeatures> ;skos:broader geoad:MapSeries ;skos:notation "8058" ;skos:prefLabel "Hillgrove:8058"@en .
geoad:Dotswood8158 a skos:Concept ;skos:definition "Map sheet for Dotswood at 1:100 000 scale. The first two digits define a longitude band 0.5 degree wide and the second two digits a latitude band 0.5 degree wide."@en ;skos:inScheme <https://linked.data.gov.au/def/geoadminfeatures> ;skos:broader geoad:MapSeries ;skos:notation "8158" ;skos:prefLabel "Dotswood:8158"@en .
geoad:Mingela8258 a skos:Concept ;skos:definition "Map sheet for Mingela at 1:100 000 scale. The first two digits define a longitude band 0.5 degree wide and the second two digits a latitude band 0.5 degree wide."@en ;skos:inScheme <https://linked.data.gov.au/def/geoadminfeatures> ;skos:broader geoad:MapSeries ;skos:notation "8258" ;skos:prefLabel "Mingela:8258"@en .
geoad:Ayr8358 a skos:Concept ;skos:definition "Map sheet for Ayr at 1:100 000 scale. The first two digits define a longitude band 0.5 degree wide and the second two digits a latitude band 0.5 degree wide."@en ;skos:inScheme <https://linked.data.gov.au/def/geoadminfeatures> ;skos:broader geoad:MapSeries ;skos:notation "8358" ;skos:prefLabel "Ayr:8358"@en .
geoad:CapeUpstart8458 a skos:Concept ;skos:definition "Map sheet for Cape Upstart at 1:100 000 scale. The first two digits define a longitude band 0.5 degree wide and the second two digits a latitude band 0.5 degree wide."@en ;skos:inScheme <https://linked.data.gov.au/def/geoadminfeatures> ;skos:broader geoad:MapSeries ;skos:notation "8458" ;skos:prefLabel "Cape Upstart:8458"@en .
geoad:AbbotPoint8558 a skos:Concept ;skos:definition "Map sheet for Abbot Point at 1:100 000 scale. The first two digits define a longitude band 0.5 degree wide and the second two digits a latitude band 0.5 degree wide."@en ;skos:inScheme <https://linked.data.gov.au/def/geoadminfeatures> ;skos:broader geoad:MapSeries ;skos:notation "8558" ;skos:prefLabel "Abbot Point:8558"@en .
geoad:Proserpine8657 a skos:Concept ;skos:definition "Map sheet for Proserpine at 1:100 000 scale. The first two digits define a longitude band 0.5 degree wide and the second two digits a latitude band 0.5 degree wide."@en ;skos:inScheme <https://linked.data.gov.au/def/geoadminfeatures> ;skos:broader geoad:MapSeries ;skos:notation "8657" ;skos:prefLabel "Proserpine:8657"@en .
geoad:Wooroona6557 a skos:Concept ;skos:definition "Map sheet for Wooroona at 1:100 000 scale. The first two digits define a longitude band 0.5 degree wide and the second two digits a latitude band 0.5 degree wide."@en ;skos:inScheme <https://linked.data.gov.au/def/geoadminfeatures> ;skos:broader geoad:MapSeries ;skos:notation "6557" ;skos:prefLabel "Wooroona:6557"@en .
geoad:Yelvertoft6657 a skos:Concept ;skos:definition "Map sheet for Yelvertoft at 1:100 000 scale. The first two digits define a longitude band 0.5 degree wide and the second two digits a latitude band 0.5 degree wide."@en ;skos:inScheme <https://linked.data.gov.au/def/geoadminfeatures> ;skos:broader geoad:MapSeries ;skos:notation "6657" ;skos:prefLabel "Yelvertoft:6657"@en .
geoad:KennedyGap6757 a skos:Concept ;skos:definition "Map sheet for Kennedy Gap at 1:100 000 scale. The first two digits define a longitude band 0.5 degree wide and the second two digits a latitude band 0.5 degree wide."@en ;skos:inScheme <https://linked.data.gov.au/def/geoadminfeatures> ;skos:broader geoad:MapSeries ;skos:notation "6757" ;skos:prefLabel "Kennedy Gap:6757"@en .
geoad:Prospector6857 a skos:Concept ;skos:definition "Map sheet for Prospector at 1:100 000 scale. The first two digits define a longitude band 0.5 degree wide and the second two digits a latitude band 0.5 degree wide."@en ;skos:inScheme <https://linked.data.gov.au/def/geoadminfeatures> ;skos:broader geoad:MapSeries ;skos:notation "6857" ;skos:prefLabel "Prospector:6857"@en .
geoad:Quamby6957 a skos:Concept ;skos:definition "Map sheet for Quamby at 1:100 000 scale. The first two digits define a longitude band 0.5 degree wide and the second two digits a latitude band 0.5 degree wide."@en ;skos:inScheme <https://linked.data.gov.au/def/geoadminfeatures> ;skos:broader geoad:MapSeries ;skos:notation "6957" ;skos:prefLabel "Quamby:6957"@en .
geoad:Clonagh7057 a skos:Concept ;skos:definition "Map sheet for Clonagh at 1:100 000 scale. The first two digits define a longitude band 0.5 degree wide and the second two digits a latitude band 0.5 degree wide."@en ;skos:inScheme <https://linked.data.gov.au/def/geoadminfeatures> ;skos:broader geoad:MapSeries ;skos:notation "7057" ;skos:prefLabel "Clonagh:7057"@en .
geoad:Dalgonally7157 a skos:Concept ;skos:definition "Map sheet for Dalgonally at 1:100 000 scale. The first two digits define a longitude band 0.5 degree wide and the second two digits a latitude band 0.5 degree wide."@en ;skos:inScheme <https://linked.data.gov.au/def/geoadminfeatures> ;skos:broader geoad:MapSeries ;skos:notation "7157" ;skos:prefLabel "Dalgonally:7157"@en .
geoad:Wyaldra7257 a skos:Concept ;skos:definition "Map sheet for Wyaldra at 1:100 000 scale. The first two digits define a longitude band 0.5 degree wide and the second two digits a latitude band 0.5 degree wide."@en ;skos:inScheme <https://linked.data.gov.au/def/geoadminfeatures> ;skos:broader geoad:MapSeries ;skos:notation "7257" ;skos:prefLabel "Wyaldra:7257"@en .
geoad:Kilterry7357 a skos:Concept ;skos:definition "Map sheet for Kilterry at 1:100 000 scale. The first two digits define a longitude band 0.5 degree wide and the second two digits a latitude band 0.5 degree wide."@en ;skos:inScheme <https://linked.data.gov.au/def/geoadminfeatures> ;skos:broader geoad:MapSeries ;skos:notation "7357" ;skos:prefLabel "Kilterry:7357"@en .
geoad:Runnymede7457 a skos:Concept ;skos:definition "Map sheet for Runnymede at 1:100 000 scale. The first two digits define a longitude band 0.5 degree wide and the second two digits a latitude band 0.5 degree wide."@en ;skos:inScheme <https://linked.data.gov.au/def/geoadminfeatures> ;skos:broader geoad:MapSeries ;skos:notation "7457" ;skos:prefLabel "Runnymede:7457"@en .
geoad:Coalbrook7557 a skos:Concept ;skos:definition "Map sheet for Coalbrook at 1:100 000 scale. The first two digits define a longitude band 0.5 degree wide and the second two digits a latitude band 0.5 degree wide."@en ;skos:inScheme <https://linked.data.gov.au/def/geoadminfeatures> ;skos:broader geoad:MapSeries ;skos:notation "7557" ;skos:prefLabel "Coalbrook:7557"@en .
geoad:DuttonRiver7657 a skos:Concept ;skos:definition "Map sheet for Dutton River at 1:100 000 scale. The first two digits define a longitude band 0.5 degree wide and the second two digits a latitude band 0.5 degree wide."@en ;skos:inScheme <https://linked.data.gov.au/def/geoadminfeatures> ;skos:broader geoad:MapSeries ;skos:notation "7657" ;skos:prefLabel "Dutton River:7657"@en .
geoad:Boonderoo7757 a skos:Concept ;skos:definition "Map sheet for Boonderoo at 1:100 000 scale. The first two digits define a longitude band 0.5 degree wide and the second two digits a latitude band 0.5 degree wide."@en ;skos:inScheme <https://linked.data.gov.au/def/geoadminfeatures> ;skos:broader geoad:MapSeries ;skos:notation "7757" ;skos:prefLabel "Boonderoo:7757"@en .
geoad:WhiteMountains7857 a skos:Concept ;skos:definition "Map sheet for White Mountains at 1:100 000 scale. The first two digits define a longitude band 0.5 degree wide and the second two digits a latitude band 0.5 degree wide."@en ;skos:inScheme <https://linked.data.gov.au/def/geoadminfeatures> ;skos:broader geoad:MapSeries ;skos:notation "7857" ;skos:prefLabel "White Mountains:7857"@en .
geoad:Lolworth7957 a skos:Concept ;skos:definition "Map sheet for Lolworth at 1:100 000 scale. The first two digits define a longitude band 0.5 degree wide and the second two digits a latitude band 0.5 degree wide."@en ;skos:inScheme <https://linked.data.gov.au/def/geoadminfeatures> ;skos:broader geoad:MapSeries ;skos:notation "7957" ;skos:prefLabel "Lolworth:7957"@en .
geoad:Homestead8057 a skos:Concept ;skos:definition "Map sheet for Homestead at 1:100 000 scale. The first two digits define a longitude band 0.5 degree wide and the second two digits a latitude band 0.5 degree wide."@en ;skos:inScheme <https://linked.data.gov.au/def/geoadminfeatures> ;skos:broader geoad:MapSeries ;skos:notation "8057" ;skos:prefLabel "Homestead:8057"@en .
geoad:ChartersTowers8157 a skos:Concept ;skos:definition "Map sheet for Charters Towers at 1:100 000 scale. The first two digits define a longitude band 0.5 degree wide and the second two digits a latitude band 0.5 degree wide."@en ;skos:inScheme <https://linked.data.gov.au/def/geoadminfeatures> ;skos:broader geoad:MapSeries ;skos:notation "8157" ;skos:prefLabel "Charters Towers:8157"@en .
geoad:Ravenswood8257 a skos:Concept ;skos:definition "Map sheet for Ravenswood at 1:100 000 scale. The first two digits define a longitude band 0.5 degree wide and the second two digits a latitude band 0.5 degree wide."@en ;skos:inScheme <https://linked.data.gov.au/def/geoadminfeatures> ;skos:broader geoad:MapSeries ;skos:notation "8257" ;skos:prefLabel "Ravenswood:8257"@en .
geoad:Strathalbyn8357 a skos:Concept ;skos:definition "Map sheet for Strathalbyn at 1:100 000 scale. The first two digits define a longitude band 0.5 degree wide and the second two digits a latitude band 0.5 degree wide."@en ;skos:inScheme <https://linked.data.gov.au/def/geoadminfeatures> ;skos:broader geoad:MapSeries ;skos:notation "8357" ;skos:prefLabel "Strathalbyn:8357"@en .
geoad:Bogie8457 a skos:Concept ;skos:definition "Map sheet for Bogie at 1:100 000 scale. The first two digits define a longitude band 0.5 degree wide and the second two digits a latitude band 0.5 degree wide."@en ;skos:inScheme <https://linked.data.gov.au/def/geoadminfeatures> ;skos:broader geoad:MapSeries ;skos:notation "8457" ;skos:prefLabel "Bogie:8457"@en .
geoad:Bowen8557 a skos:Concept ;skos:definition "Map sheet for Bowen at 1:100 000 scale. The first two digits define a longitude band 0.5 degree wide and the second two digits a latitude band 0.5 degree wide."@en ;skos:inScheme <https://linked.data.gov.au/def/geoadminfeatures> ;skos:broader geoad:MapSeries ;skos:notation "8557" ;skos:prefLabel "Bowen:8557"@en .
geoad:LindemanIsland8757 a skos:Concept ;skos:definition "Map sheet for Lindeman Island at 1:100 000 scale. The first two digits define a longitude band 0.5 degree wide and the second two digits a latitude band 0.5 degree wide."@en ;skos:inScheme <https://linked.data.gov.au/def/geoadminfeatures> ;skos:broader geoad:MapSeries ;skos:notation "8757" ;skos:prefLabel "Lindeman Island:8757"@en .
geoad:Bullecourt6556 a skos:Concept ;skos:definition "Map sheet for Bullecourt at 1:100 000 scale. The first two digits define a longitude band 0.5 degree wide and the second two digits a latitude band 0.5 degree wide."@en ;skos:inScheme <https://linked.data.gov.au/def/geoadminfeatures> ;skos:broader geoad:MapSeries ;skos:notation "6556" ;skos:prefLabel "Bullecourt:6556"@en .
geoad:Templeton6656 a skos:Concept ;skos:definition "Map sheet for Templeton at 1:100 000 scale. The first two digits define a longitude band 0.5 degree wide and the second two digits a latitude band 0.5 degree wide."@en ;skos:inScheme <https://linked.data.gov.au/def/geoadminfeatures> ;skos:broader geoad:MapSeries ;skos:notation "6656" ;skos:prefLabel "Templeton:6656"@en .
geoad:MountIsa6756 a skos:Concept ;skos:definition "Map sheet for Mount Isa at 1:100 000 scale. The first two digits define a longitude band 0.5 degree wide and the second two digits a latitude band 0.5 degree wide."@en ;skos:inScheme <https://linked.data.gov.au/def/geoadminfeatures> ;skos:broader geoad:MapSeries ;skos:notation "6756" ;skos:prefLabel "Mount Isa:6756"@en .
geoad:MaryKathleen6856 a skos:Concept ;skos:definition "Map sheet for Mary Kathleen at 1:100 000 scale. The first two digits define a longitude band 0.5 degree wide and the second two digits a latitude band 0.5 degree wide."@en ;skos:inScheme <https://linked.data.gov.au/def/geoadminfeatures> ;skos:broader geoad:MapSeries ;skos:notation "6856" ;skos:prefLabel "Mary Kathleen:6856"@en .
geoad:Marraba6956 a skos:Concept ;skos:definition "Map sheet for Marraba at 1:100 000 scale. The first two digits define a longitude band 0.5 degree wide and the second two digits a latitude band 0.5 degree wide."@en ;skos:inScheme <https://linked.data.gov.au/def/geoadminfeatures> ;skos:broader geoad:MapSeries ;skos:notation "6956" ;skos:prefLabel "Marraba:6956"@en .
geoad:Cloncurry7056 a skos:Concept ;skos:definition "Map sheet for Cloncurry at 1:100 000 scale. The first two digits define a longitude band 0.5 degree wide and the second two digits a latitude band 0.5 degree wide."@en ;skos:inScheme <https://linked.data.gov.au/def/geoadminfeatures> ;skos:broader geoad:MapSeries ;skos:notation "7056" ;skos:prefLabel "Cloncurry:7056"@en .
geoad:Oorindi7156 a skos:Concept ;skos:definition "Map sheet for Oorindi at 1:100 000 scale. The first two digits define a longitude band 0.5 degree wide and the second two digits a latitude band 0.5 degree wide."@en ;skos:inScheme <https://linked.data.gov.au/def/geoadminfeatures> ;skos:broader geoad:MapSeries ;skos:notation "7156" ;skos:prefLabel "Oorindi:7156"@en .
geoad:JuliaCreek7256 a skos:Concept ;skos:definition "Map sheet for Julia Creek at 1:100 000 scale. The first two digits define a longitude band 0.5 degree wide and the second two digits a latitude band 0.5 degree wide."@en ;skos:inScheme <https://linked.data.gov.au/def/geoadminfeatures> ;skos:broader geoad:MapSeries ;skos:notation "7256" ;skos:prefLabel "Julia Creek:7256"@en .
geoad:Nelia7356 a skos:Concept ;skos:definition "Map sheet for Nelia at 1:100 000 scale. The first two digits define a longitude band 0.5 degree wide and the second two digits a latitude band 0.5 degree wide."@en ;skos:inScheme <https://linked.data.gov.au/def/geoadminfeatures> ;skos:broader geoad:MapSeries ;skos:notation "7356" ;skos:prefLabel "Nelia:7356"@en .
geoad:Maxwelton7456 a skos:Concept ;skos:definition "Map sheet for Maxwelton at 1:100 000 scale. The first two digits define a longitude band 0.5 degree wide and the second two digits a latitude band 0.5 degree wide."@en ;skos:inScheme <https://linked.data.gov.au/def/geoadminfeatures> ;skos:broader geoad:MapSeries ;skos:notation "7456" ;skos:prefLabel "Maxwelton:7456"@en .
geoad:Richmond7556 a skos:Concept ;skos:definition "Map sheet for Richmond at 1:100 000 scale. The first two digits define a longitude band 0.5 degree wide and the second two digits a latitude band 0.5 degree wide."@en ;skos:inScheme <https://linked.data.gov.au/def/geoadminfeatures> ;skos:broader geoad:MapSeries ;skos:notation "7556" ;skos:prefLabel "Richmond:7556"@en .
geoad:Marathon7656 a skos:Concept ;skos:definition "Map sheet for Marathon at 1:100 000 scale. The first two digits define a longitude band 0.5 degree wide and the second two digits a latitude band 0.5 degree wide."@en ;skos:inScheme <https://linked.data.gov.au/def/geoadminfeatures> ;skos:broader geoad:MapSeries ;skos:notation "7656" ;skos:prefLabel "Marathon:7656"@en .
geoad:Hughenden7756 a skos:Concept ;skos:definition "Map sheet for Hughenden at 1:100 000 scale. The first two digits define a longitude band 0.5 degree wide and the second two digits a latitude band 0.5 degree wide."@en ;skos:inScheme <https://linked.data.gov.au/def/geoadminfeatures> ;skos:broader geoad:MapSeries ;skos:notation "7756" ;skos:prefLabel "Hughenden:7756"@en .
geoad:Prairie7856 a skos:Concept ;skos:definition "Map sheet for Prairie at 1:100 000 scale. The first two digits define a longitude band 0.5 degree wide and the second two digits a latitude band 0.5 degree wide."@en ;skos:inScheme <https://linked.data.gov.au/def/geoadminfeatures> ;skos:broader geoad:MapSeries ;skos:notation "7856" ;skos:prefLabel "Prairie:7856"@en .
geoad:Pentland7956 a skos:Concept ;skos:definition "Map sheet for Pentland at 1:100 000 scale. The first two digits define a longitude band 0.5 degree wide and the second two digits a latitude band 0.5 degree wide."@en ;skos:inScheme <https://linked.data.gov.au/def/geoadminfeatures> ;skos:broader geoad:MapSeries ;skos:notation "7956" ;skos:prefLabel "Pentland:7956"@en .
geoad:Milray8056 a skos:Concept ;skos:definition "Map sheet for Milray at 1:100 000 scale. The first two digits define a longitude band 0.5 degree wide and the second two digits a latitude band 0.5 degree wide."@en ;skos:inScheme <https://linked.data.gov.au/def/geoadminfeatures> ;skos:broader geoad:MapSeries ;skos:notation "8056" ;skos:prefLabel "Milray:8056"@en .
geoad:Pajingo8156 a skos:Concept ;skos:definition "Map sheet for Pajingo at 1:100 000 scale. The first two digits define a longitude band 0.5 degree wide and the second two digits a latitude band 0.5 degree wide."@en ;skos:inScheme <https://linked.data.gov.au/def/geoadminfeatures> ;skos:broader geoad:MapSeries ;skos:notation "8156" ;skos:prefLabel "Pajingo:8156"@en .
geoad:HarvestHome8256 a skos:Concept ;skos:definition "Map sheet for Harvest Home at 1:100 000 scale. The first two digits define a longitude band 0.5 degree wide and the second two digits a latitude band 0.5 degree wide."@en ;skos:inScheme <https://linked.data.gov.au/def/geoadminfeatures> ;skos:broader geoad:MapSeries ;skos:notation "8256" ;skos:prefLabel "Harvest Home:8256"@en .
geoad:Glendon8356 a skos:Concept ;skos:definition "Map sheet for Glendon at 1:100 000 scale. The first two digits define a longitude band 0.5 degree wide and the second two digits a latitude band 0.5 degree wide."@en ;skos:inScheme <https://linked.data.gov.au/def/geoadminfeatures> ;skos:broader geoad:MapSeries ;skos:notation "8356" ;skos:prefLabel "Glendon:8356"@en .
geoad:Collinsville8456 a skos:Concept ;skos:definition "Map sheet for Collinsville at 1:100 000 scale. The first two digits define a longitude band 0.5 degree wide and the second two digits a latitude band 0.5 degree wide."@en ;skos:inScheme <https://linked.data.gov.au/def/geoadminfeatures> ;skos:broader geoad:MapSeries ;skos:notation "8456" ;skos:prefLabel "Collinsville:8456"@en .
geoad:Urannah8556 a skos:Concept ;skos:definition "Map sheet for Urannah at 1:100 000 scale. The first two digits define a longitude band 0.5 degree wide and the second two digits a latitude band 0.5 degree wide."@en ;skos:inScheme <https://linked.data.gov.au/def/geoadminfeatures> ;skos:broader geoad:MapSeries ;skos:notation "8556" ;skos:prefLabel "Urannah:8556"@en .
geoad:Calen8656 a skos:Concept ;skos:definition "Map sheet for Calen at 1:100 000 scale. The first two digits define a longitude band 0.5 degree wide and the second two digits a latitude band 0.5 degree wide."@en ;skos:inScheme <https://linked.data.gov.au/def/geoadminfeatures> ;skos:broader geoad:MapSeries ;skos:notation "8656" ;skos:prefLabel "Calen:8656"@en .
geoad:CumberlandIslands8756 a skos:Concept ;skos:definition "Map sheet for Cumberland Islands at 1:100 000 scale. The first two digits define a longitude band 0.5 degree wide and the second two digits a latitude band 0.5 degree wide."@en ;skos:inScheme <https://linked.data.gov.au/def/geoadminfeatures> ;skos:broader geoad:MapSeries ;skos:notation "8756" ;skos:prefLabel "Cumberland Islands:8756"@en .
geoad:Scawfell8856 a skos:Concept ;skos:definition "Map sheet for Scawfell at 1:100 000 scale. The first two digits define a longitude band 0.5 degree wide and the second two digits a latitude band 0.5 degree wide."@en ;skos:inScheme <https://linked.data.gov.au/def/geoadminfeatures> ;skos:broader geoad:MapSeries ;skos:notation "8856" ;skos:prefLabel "Scawfell:8856"@en .
geoad:Headingly6555 a skos:Concept ;skos:definition "Map sheet for Headingly at 1:100 000 scale. The first two digits define a longitude band 0.5 degree wide and the second two digits a latitude band 0.5 degree wide."@en ;skos:inScheme <https://linked.data.gov.au/def/geoadminfeatures> ;skos:broader geoad:MapSeries ;skos:notation "6555" ;skos:prefLabel "Headingly:6555"@en .
geoad:GoaCreek6655 a skos:Concept ;skos:definition "Map sheet for Goa Creek at 1:100 000 scale. The first two digits define a longitude band 0.5 degree wide and the second two digits a latitude band 0.5 degree wide."@en ;skos:inScheme <https://linked.data.gov.au/def/geoadminfeatures> ;skos:broader geoad:MapSeries ;skos:notation "6655" ;skos:prefLabel "Goa Creek:6655"@en .
geoad:Oban6755 a skos:Concept ;skos:definition "Map sheet for Oban at 1:100 000 scale. The first two digits define a longitude band 0.5 degree wide and the second two digits a latitude band 0.5 degree wide."@en ;skos:inScheme <https://linked.data.gov.au/def/geoadminfeatures> ;skos:broader geoad:MapSeries ;skos:notation "6755" ;skos:prefLabel "Oban:6755"@en .
geoad:Duchess6855 a skos:Concept ;skos:definition "Map sheet for Duchess at 1:100 000 scale. The first two digits define a longitude band 0.5 degree wide and the second two digits a latitude band 0.5 degree wide."@en ;skos:inScheme <https://linked.data.gov.au/def/geoadminfeatures> ;skos:broader geoad:MapSeries ;skos:notation "6855" ;skos:prefLabel "Duchess:6855"@en .
geoad:Malbon6955 a skos:Concept ;skos:definition "Map sheet for Malbon at 1:100 000 scale. The first two digits define a longitude band 0.5 degree wide and the second two digits a latitude band 0.5 degree wide."@en ;skos:inScheme <https://linked.data.gov.au/def/geoadminfeatures> ;skos:broader geoad:MapSeries ;skos:notation "6955" ;skos:prefLabel "Malbon:6955"@en .
geoad:MountAngelay7055 a skos:Concept ;skos:definition "Map sheet for Mount Angelay at 1:100 000 scale. The first two digits define a longitude band 0.5 degree wide and the second two digits a latitude band 0.5 degree wide."@en ;skos:inScheme <https://linked.data.gov.au/def/geoadminfeatures> ;skos:broader geoad:MapSeries ;skos:notation "7055" ;skos:prefLabel "Mount Angelay:7055"@en .
geoad:Mckinlay7155 a skos:Concept ;skos:definition "Map sheet for Mckinlay at 1:100 000 scale. The first two digits define a longitude band 0.5 degree wide and the second two digits a latitude band 0.5 degree wide."@en ;skos:inScheme <https://linked.data.gov.au/def/geoadminfeatures> ;skos:broader geoad:MapSeries ;skos:notation "7155" ;skos:prefLabel "Mckinlay:7155"@en .
geoad:Eulolo7255 a skos:Concept ;skos:definition "Map sheet for Eulolo at 1:100 000 scale. The first two digits define a longitude band 0.5 degree wide and the second two digits a latitude band 0.5 degree wide."@en ;skos:inScheme <https://linked.data.gov.au/def/geoadminfeatures> ;skos:broader geoad:MapSeries ;skos:notation "7255" ;skos:prefLabel "Eulolo:7255"@en .
geoad:HamiltonDowns7355 a skos:Concept ;skos:definition "Map sheet for Hamilton Downs at 1:100 000 scale. The first two digits define a longitude band 0.5 degree wide and the second two digits a latitude band 0.5 degree wide."@en ;skos:inScheme <https://linked.data.gov.au/def/geoadminfeatures> ;skos:broader geoad:MapSeries ;skos:notation "7355" ;skos:prefLabel "Hamilton Downs:7355"@en .
geoad:Glenlyon7455 a skos:Concept ;skos:definition "Map sheet for Glenlyon at 1:100 000 scale. The first two digits define a longitude band 0.5 degree wide and the second two digits a latitude band 0.5 degree wide."@en ;skos:inScheme <https://linked.data.gov.au/def/geoadminfeatures> ;skos:broader geoad:MapSeries ;skos:notation "7455" ;skos:prefLabel "Glenlyon:7455"@en .
geoad:Cassilis7555 a skos:Concept ;skos:definition "Map sheet for Cassilis at 1:100 000 scale. The first two digits define a longitude band 0.5 degree wide and the second two digits a latitude band 0.5 degree wide."@en ;skos:inScheme <https://linked.data.gov.au/def/geoadminfeatures> ;skos:broader geoad:MapSeries ;skos:notation "7555" ;skos:prefLabel "Cassilis:7555"@en .
geoad:Stamford7655 a skos:Concept ;skos:definition "Map sheet for Stamford at 1:100 000 scale. The first two digits define a longitude band 0.5 degree wide and the second two digits a latitude band 0.5 degree wide."@en ;skos:inScheme <https://linked.data.gov.au/def/geoadminfeatures> ;skos:broader geoad:MapSeries ;skos:notation "7655" ;skos:prefLabel "Stamford:7655"@en .
geoad:CameronDowns7755 a skos:Concept ;skos:definition "Map sheet for Cameron Downs at 1:100 000 scale. The first two digits define a longitude band 0.5 degree wide and the second two digits a latitude band 0.5 degree wide."@en ;skos:inScheme <https://linked.data.gov.au/def/geoadminfeatures> ;skos:broader geoad:MapSeries ;skos:notation "7755" ;skos:prefLabel "Cameron Downs:7755"@en .
geoad:Lammermoor7855 a skos:Concept ;skos:definition "Map sheet for Lammermoor at 1:100 000 scale. The first two digits define a longitude band 0.5 degree wide and the second two digits a latitude band 0.5 degree wide."@en ;skos:inScheme <https://linked.data.gov.au/def/geoadminfeatures> ;skos:broader geoad:MapSeries ;skos:notation "7855" ;skos:prefLabel "Lammermoor:7855"@en .
geoad:WebbLake7955 a skos:Concept ;skos:definition "Map sheet for Webb Lake at 1:100 000 scale. The first two digits define a longitude band 0.5 degree wide and the second two digits a latitude band 0.5 degree wide."@en ;skos:inScheme <https://linked.data.gov.au/def/geoadminfeatures> ;skos:broader geoad:MapSeries ;skos:notation "7955" ;skos:prefLabel "Webb Lake:7955"@en .
geoad:Yarrowmere8055 a skos:Concept ;skos:definition "Map sheet for Yarrowmere at 1:100 000 scale. The first two digits define a longitude band 0.5 degree wide and the second two digits a latitude band 0.5 degree wide."@en ;skos:inScheme <https://linked.data.gov.au/def/geoadminfeatures> ;skos:broader geoad:MapSeries ;skos:notation "8055" ;skos:prefLabel "Yarrowmere:8055"@en .
geoad:NatalDowns8155 a skos:Concept ;skos:definition "Map sheet for Natal Downs at 1:100 000 scale. The first two digits define a longitude band 0.5 degree wide and the second two digits a latitude band 0.5 degree wide."@en ;skos:inScheme <https://linked.data.gov.au/def/geoadminfeatures> ;skos:broader geoad:MapSeries ;skos:notation "8155" ;skos:prefLabel "Natal Downs:8155"@en .
geoad:Scartwater8255 a skos:Concept ;skos:definition "Map sheet for Scartwater at 1:100 000 scale. The first two digits define a longitude band 0.5 degree wide and the second two digits a latitude band 0.5 degree wide."@en ;skos:inScheme <https://linked.data.gov.au/def/geoadminfeatures> ;skos:broader geoad:MapSeries ;skos:notation "8255" ;skos:prefLabel "Scartwater:8255"@en .
geoad:MountCoolon8355 a skos:Concept ;skos:definition "Map sheet for Mount Coolon at 1:100 000 scale. The first two digits define a longitude band 0.5 degree wide and the second two digits a latitude band 0.5 degree wide."@en ;skos:inScheme <https://linked.data.gov.au/def/geoadminfeatures> ;skos:broader geoad:MapSeries ;skos:notation "8355" ;skos:prefLabel "Mount Coolon:8355"@en .
geoad:Byerwen8455 a skos:Concept ;skos:definition "Map sheet for Byerwen at 1:100 000 scale. The first two digits define a longitude band 0.5 degree wide and the second two digits a latitude band 0.5 degree wide."@en ;skos:inScheme <https://linked.data.gov.au/def/geoadminfeatures> ;skos:broader geoad:MapSeries ;skos:notation "8455" ;skos:prefLabel "Byerwen:8455"@en .
geoad:Hillalong8555 a skos:Concept ;skos:definition "Map sheet for Hillalong at 1:100 000 scale. The first two digits define a longitude band 0.5 degree wide and the second two digits a latitude band 0.5 degree wide."@en ;skos:inScheme <https://linked.data.gov.au/def/geoadminfeatures> ;skos:broader geoad:MapSeries ;skos:notation "8555" ;skos:prefLabel "Hillalong:8555"@en .
geoad:Mirani8655 a skos:Concept ;skos:definition "Map sheet for Mirani at 1:100 000 scale. The first two digits define a longitude band 0.5 degree wide and the second two digits a latitude band 0.5 degree wide."@en ;skos:inScheme <https://linked.data.gov.au/def/geoadminfeatures> ;skos:broader geoad:MapSeries ;skos:notation "8655" ;skos:prefLabel "Mirani:8655"@en .
geoad:Mackay8755 a skos:Concept ;skos:definition "Map sheet for Mackay at 1:100 000 scale. The first two digits define a longitude band 0.5 degree wide and the second two digits a latitude band 0.5 degree wide."@en ;skos:inScheme <https://linked.data.gov.au/def/geoadminfeatures> ;skos:broader geoad:MapSeries ;skos:notation "8755" ;skos:prefLabel "Mackay:8755"@en .
geoad:PrudhoeIsland8855 a skos:Concept ;skos:definition "Map sheet for Prudhoe Island at 1:100 000 scale. The first two digits define a longitude band 0.5 degree wide and the second two digits a latitude band 0.5 degree wide."@en ;skos:inScheme <https://linked.data.gov.au/def/geoadminfeatures> ;skos:broader geoad:MapSeries ;skos:notation "8855" ;skos:prefLabel "Prudhoe Island:8855"@en .
geoad:HotspurIsland8955 a skos:Concept ;skos:definition "Map sheet for Hotspur Island at 1:100 000 scale. The first two digits define a longitude band 0.5 degree wide and the second two digits a latitude band 0.5 degree wide."@en ;skos:inScheme <https://linked.data.gov.au/def/geoadminfeatures> ;skos:broader geoad:MapSeries ;skos:notation "8955" ;skos:prefLabel "Hotspur Island:8955"@en .
geoad:Urandangi6554 a skos:Concept ;skos:definition "Map sheet for Urandangi at 1:100 000 scale. The first two digits define a longitude band 0.5 degree wide and the second two digits a latitude band 0.5 degree wide."@en ;skos:inScheme <https://linked.data.gov.au/def/geoadminfeatures> ;skos:broader geoad:MapSeries ;skos:notation "6554" ;skos:prefLabel "Urandangi:6554"@en .
geoad:Carandotta6654 a skos:Concept ;skos:definition "Map sheet for Carandotta at 1:100 000 scale. The first two digits define a longitude band 0.5 degree wide and the second two digits a latitude band 0.5 degree wide."@en ;skos:inScheme <https://linked.data.gov.au/def/geoadminfeatures> ;skos:broader geoad:MapSeries ;skos:notation "6654" ;skos:prefLabel "Carandotta:6654"@en .
geoad:Ardmore6754 a skos:Concept ;skos:definition "Map sheet for Ardmore at 1:100 000 scale. The first two digits define a longitude band 0.5 degree wide and the second two digits a latitude band 0.5 degree wide."@en ;skos:inScheme <https://linked.data.gov.au/def/geoadminfeatures> ;skos:broader geoad:MapSeries ;skos:notation "6754" ;skos:prefLabel "Ardmore:6754"@en .
geoad:Dajarra6854 a skos:Concept ;skos:definition "Map sheet for Dajarra at 1:100 000 scale. The first two digits define a longitude band 0.5 degree wide and the second two digits a latitude band 0.5 degree wide."@en ;skos:inScheme <https://linked.data.gov.au/def/geoadminfeatures> ;skos:broader geoad:MapSeries ;skos:notation "6854" ;skos:prefLabel "Dajarra:6854"@en .
geoad:MountMerlin6954 a skos:Concept ;skos:definition "Map sheet for Mount Merlin at 1:100 000 scale. The first two digits define a longitude band 0.5 degree wide and the second two digits a latitude band 0.5 degree wide."@en ;skos:inScheme <https://linked.data.gov.au/def/geoadminfeatures> ;skos:broader geoad:MapSeries ;skos:notation "6954" ;skos:prefLabel "Mount Merlin:6954"@en .
geoad:Selwyn7054 a skos:Concept ;skos:definition "Map sheet for Selwyn at 1:100 000 scale. The first two digits define a longitude band 0.5 degree wide and the second two digits a latitude band 0.5 degree wide."@en ;skos:inScheme <https://linked.data.gov.au/def/geoadminfeatures> ;skos:broader geoad:MapSeries ;skos:notation "7054" ;skos:prefLabel "Selwyn:7054"@en .
geoad:ElRita7154 a skos:Concept ;skos:definition "Map sheet for El Rita at 1:100 000 scale. The first two digits define a longitude band 0.5 degree wide and the second two digits a latitude band 0.5 degree wide."@en ;skos:inScheme <https://linked.data.gov.au/def/geoadminfeatures> ;skos:broader geoad:MapSeries ;skos:notation "7154" ;skos:prefLabel "El Rita:7154"@en .
geoad:Kynuna7254 a skos:Concept ;skos:definition "Map sheet for Kynuna at 1:100 000 scale. The first two digits define a longitude band 0.5 degree wide and the second two digits a latitude band 0.5 degree wide."@en ;skos:inScheme <https://linked.data.gov.au/def/geoadminfeatures> ;skos:broader geoad:MapSeries ;skos:notation "7254" ;skos:prefLabel "Kynuna:7254"@en .
geoad:Dagworth7354 a skos:Concept ;skos:definition "Map sheet for Dagworth at 1:100 000 scale. The first two digits define a longitude band 0.5 degree wide and the second two digits a latitude band 0.5 degree wide."@en ;skos:inScheme <https://linked.data.gov.au/def/geoadminfeatures> ;skos:broader geoad:MapSeries ;skos:notation "7354" ;skos:prefLabel "Dagworth:7354"@en .
geoad:AyrshireDowns7454 a skos:Concept ;skos:definition "Map sheet for Ayrshire Downs at 1:100 000 scale. The first two digits define a longitude band 0.5 degree wide and the second two digits a latitude band 0.5 degree wide."@en ;skos:inScheme <https://linked.data.gov.au/def/geoadminfeatures> ;skos:broader geoad:MapSeries ;skos:notation "7454" ;skos:prefLabel "Ayrshire Downs:7454"@en .
geoad:Manuka7554 a skos:Concept ;skos:definition "Map sheet for Manuka at 1:100 000 scale. The first two digits define a longitude band 0.5 degree wide and the second two digits a latitude band 0.5 degree wide."@en ;skos:inScheme <https://linked.data.gov.au/def/geoadminfeatures> ;skos:broader geoad:MapSeries ;skos:notation "7554" ;skos:prefLabel "Manuka:7554"@en .
geoad:Katandra7654 a skos:Concept ;skos:definition "Map sheet for Katandra at 1:100 000 scale. The first two digits define a longitude band 0.5 degree wide and the second two digits a latitude band 0.5 degree wide."@en ;skos:inScheme <https://linked.data.gov.au/def/geoadminfeatures> ;skos:broader geoad:MapSeries ;skos:notation "7654" ;skos:prefLabel "Katandra:7654"@en .
geoad:Tangorin7754 a skos:Concept ;skos:definition "Map sheet for Tangorin at 1:100 000 scale. The first two digits define a longitude band 0.5 degree wide and the second two digits a latitude band 0.5 degree wide."@en ;skos:inScheme <https://linked.data.gov.au/def/geoadminfeatures> ;skos:broader geoad:MapSeries ;skos:notation "7754" ;skos:prefLabel "Tangorin:7754"@en .
geoad:LudgateHill7854 a skos:Concept ;skos:definition "Map sheet for Ludgate Hill at 1:100 000 scale. The first two digits define a longitude band 0.5 degree wide and the second two digits a latitude band 0.5 degree wide."@en ;skos:inScheme <https://linked.data.gov.au/def/geoadminfeatures> ;skos:broader geoad:MapSeries ;skos:notation "7854" ;skos:prefLabel "Ludgate Hill:7854"@en .
geoad:Aberfoyle7954 a skos:Concept ;skos:definition "Map sheet for Aberfoyle at 1:100 000 scale. The first two digits define a longitude band 0.5 degree wide and the second two digits a latitude band 0.5 degree wide."@en ;skos:inScheme <https://linked.data.gov.au/def/geoadminfeatures> ;skos:broader geoad:MapSeries ;skos:notation "7954" ;skos:prefLabel "Aberfoyle:7954"@en .
geoad:Bowie8054 a skos:Concept ;skos:definition "Map sheet for Bowie at 1:100 000 scale. The first two digits define a longitude band 0.5 degree wide and the second two digits a latitude band 0.5 degree wide."@en ;skos:inScheme <https://linked.data.gov.au/def/geoadminfeatures> ;skos:broader geoad:MapSeries ;skos:notation "8054" ;skos:prefLabel "Bowie:8054"@en .
geoad:MountTutah8154 a skos:Concept ;skos:definition "Map sheet for Mount Tutah at 1:100 000 scale. The first two digits define a longitude band 0.5 degree wide and the second two digits a latitude band 0.5 degree wide."@en ;skos:inScheme <https://linked.data.gov.au/def/geoadminfeatures> ;skos:broader geoad:MapSeries ;skos:notation "8154" ;skos:prefLabel "Mount Tutah:8154"@en .
geoad:Bulliwallah8254 a skos:Concept ;skos:definition "Map sheet for Bulliwallah at 1:100 000 scale. The first two digits define a longitude band 0.5 degree wide and the second two digits a latitude band 0.5 degree wide."@en ;skos:inScheme <https://linked.data.gov.au/def/geoadminfeatures> ;skos:broader geoad:MapSeries ;skos:notation "8254" ;skos:prefLabel "Bulliwallah:8254"@en .
geoad:Gunjulla8354 a skos:Concept ;skos:definition "Map sheet for Gunjulla at 1:100 000 scale. The first two digits define a longitude band 0.5 degree wide and the second two digits a latitude band 0.5 degree wide."@en ;skos:inScheme <https://linked.data.gov.au/def/geoadminfeatures> ;skos:broader geoad:MapSeries ;skos:notation "8354" ;skos:prefLabel "Gunjulla:8354"@en .
geoad:Wyena8454 a skos:Concept ;skos:definition "Map sheet for Wyena at 1:100 000 scale. The first two digits define a longitude band 0.5 degree wide and the second two digits a latitude band 0.5 degree wide."@en ;skos:inScheme <https://linked.data.gov.au/def/geoadminfeatures> ;skos:broader geoad:MapSeries ;skos:notation "8454" ;skos:prefLabel "Wyena:8454"@en .
geoad:Harrybrandt8554 a skos:Concept ;skos:definition "Map sheet for Harrybrandt at 1:100 000 scale. The first two digits define a longitude band 0.5 degree wide and the second two digits a latitude band 0.5 degree wide."@en ;skos:inScheme <https://linked.data.gov.au/def/geoadminfeatures> ;skos:broader geoad:MapSeries ;skos:notation "8554" ;skos:prefLabel "Harrybrandt:8554"@en .
geoad:Nebo8654 a skos:Concept ;skos:definition "Map sheet for Nebo at 1:100 000 scale. The first two digits define a longitude band 0.5 degree wide and the second two digits a latitude band 0.5 degree wide."@en ;skos:inScheme <https://linked.data.gov.au/def/geoadminfeatures> ;skos:broader geoad:MapSeries ;skos:notation "8654" ;skos:prefLabel "Nebo:8654"@en .
geoad:Carmila8754 a skos:Concept ;skos:definition "Map sheet for Carmila at 1:100 000 scale. The first two digits define a longitude band 0.5 degree wide and the second two digits a latitude band 0.5 degree wide."@en ;skos:inScheme <https://linked.data.gov.au/def/geoadminfeatures> ;skos:broader geoad:MapSeries ;skos:notation "8754" ;skos:prefLabel "Carmila:8754"@en .
geoad:CurlewIsland8854 a skos:Concept ;skos:definition "Map sheet for Curlew Island at 1:100 000 scale. The first two digits define a longitude band 0.5 degree wide and the second two digits a latitude band 0.5 degree wide."@en ;skos:inScheme <https://linked.data.gov.au/def/geoadminfeatures> ;skos:broader geoad:MapSeries ;skos:notation "8854" ;skos:prefLabel "Curlew Island:8854"@en .
geoad:PercyIsles8954 a skos:Concept ;skos:definition "Map sheet for Percy Isles at 1:100 000 scale. The first two digits define a longitude band 0.5 degree wide and the second two digits a latitude band 0.5 degree wide."@en ;skos:inScheme <https://linked.data.gov.au/def/geoadminfeatures> ;skos:broader geoad:MapSeries ;skos:notation "8954" ;skos:prefLabel "Percy Isles:8954"@en .
geoad:HighPeakIsland9054 a skos:Concept ;skos:definition "Map sheet for High Peak Island at 1:100 000 scale. The first two digits define a longitude band 0.5 degree wide and the second two digits a latitude band 0.5 degree wide."@en ;skos:inScheme <https://linked.data.gov.au/def/geoadminfeatures> ;skos:broader geoad:MapSeries ;skos:notation "9054" ;skos:prefLabel "High Peak Island:9054"@en .
geoad:LindaDowns6553 a skos:Concept ;skos:definition "Map sheet for Linda Downs at 1:100 000 scale. The first two digits define a longitude band 0.5 degree wide and the second two digits a latitude band 0.5 degree wide."@en ;skos:inScheme <https://linked.data.gov.au/def/geoadminfeatures> ;skos:broader geoad:MapSeries ;skos:notation "6553" ;skos:prefLabel "Linda Downs:6553"@en .
geoad:LakeKatherine6653 a skos:Concept ;skos:definition "Map sheet for Lake Katherine at 1:100 000 scale. The first two digits define a longitude band 0.5 degree wide and the second two digits a latitude band 0.5 degree wide."@en ;skos:inScheme <https://linked.data.gov.au/def/geoadminfeatures> ;skos:broader geoad:MapSeries ;skos:notation "6653" ;skos:prefLabel "Lake Katherine:6653"@en .
geoad:LesliePeak6753 a skos:Concept ;skos:definition "Map sheet for Leslie Peak at 1:100 000 scale. The first two digits define a longitude band 0.5 degree wide and the second two digits a latitude band 0.5 degree wide."@en ;skos:inScheme <https://linked.data.gov.au/def/geoadminfeatures> ;skos:broader geoad:MapSeries ;skos:notation "6753" ;skos:prefLabel "Leslie Peak:6753"@en .
geoad:BuckinghamDowns6853 a skos:Concept ;skos:definition "Map sheet for Buckingham Downs at 1:100 000 scale. The first two digits define a longitude band 0.5 degree wide and the second two digits a latitude band 0.5 degree wide."@en ;skos:inScheme <https://linked.data.gov.au/def/geoadminfeatures> ;skos:broader geoad:MapSeries ;skos:notation "6853" ;skos:prefLabel "Buckingham Downs:6853"@en .
geoad:DigbyPeaks6953 a skos:Concept ;skos:definition "Map sheet for Digby Peaks at 1:100 000 scale. The first two digits define a longitude band 0.5 degree wide and the second two digits a latitude band 0.5 degree wide."@en ;skos:inScheme <https://linked.data.gov.au/def/geoadminfeatures> ;skos:broader geoad:MapSeries ;skos:notation "6953" ;skos:prefLabel "Digby Peaks:6953"@en .
geoad:Toolebuc7053 a skos:Concept ;skos:definition "Map sheet for Toolebuc at 1:100 000 scale. The first two digits define a longitude band 0.5 degree wide and the second two digits a latitude band 0.5 degree wide."@en ;skos:inScheme <https://linked.data.gov.au/def/geoadminfeatures> ;skos:broader geoad:MapSeries ;skos:notation "7053" ;skos:prefLabel "Toolebuc:7053"@en .
geoad:FinucaneRange7153 a skos:Concept ;skos:definition "Map sheet for Finucane Range at 1:100 000 scale. The first two digits define a longitude band 0.5 degree wide and the second two digits a latitude band 0.5 degree wide."@en ;skos:inScheme <https://linked.data.gov.au/def/geoadminfeatures> ;skos:broader geoad:MapSeries ;skos:notation "7153" ;skos:prefLabel "Finucane Range:7153"@en .
geoad:Middleton7253 a skos:Concept ;skos:definition "Map sheet for Middleton at 1:100 000 scale. The first two digits define a longitude band 0.5 degree wide and the second two digits a latitude band 0.5 degree wide."@en ;skos:inScheme <https://linked.data.gov.au/def/geoadminfeatures> ;skos:broader geoad:MapSeries ;skos:notation "7253" ;skos:prefLabel "Middleton:7253"@en .
geoad:JohnHills7353 a skos:Concept ;skos:definition "Map sheet for John Hills at 1:100 000 scale. The first two digits define a longitude band 0.5 degree wide and the second two digits a latitude band 0.5 degree wide."@en ;skos:inScheme <https://linked.data.gov.au/def/geoadminfeatures> ;skos:broader geoad:MapSeries ;skos:notation "7353" ;skos:prefLabel "John Hills:7353"@en .
geoad:Wokingham7453 a skos:Concept ;skos:definition "Map sheet for Wokingham at 1:100 000 scale. The first two digits define a longitude band 0.5 degree wide and the second two digits a latitude band 0.5 degree wide."@en ;skos:inScheme <https://linked.data.gov.au/def/geoadminfeatures> ;skos:broader geoad:MapSeries ;skos:notation "7453" ;skos:prefLabel "Wokingham:7453"@en .
geoad:Winton7553 a skos:Concept ;skos:definition "Map sheet for Winton at 1:100 000 scale. The first two digits define a longitude band 0.5 degree wide and the second two digits a latitude band 0.5 degree wide."@en ;skos:inScheme <https://linked.data.gov.au/def/geoadminfeatures> ;skos:broader geoad:MapSeries ;skos:notation "7553" ;skos:prefLabel "Winton:7553"@en .
geoad:Mahrigong7653 a skos:Concept ;skos:definition "Map sheet for Mahrigong at 1:100 000 scale. The first two digits define a longitude band 0.5 degree wide and the second two digits a latitude band 0.5 degree wide."@en ;skos:inScheme <https://linked.data.gov.au/def/geoadminfeatures> ;skos:broader geoad:MapSeries ;skos:notation "7653" ;skos:prefLabel "Mahrigong:7653"@en .
geoad:Culloden7753 a skos:Concept ;skos:definition "Map sheet for Culloden at 1:100 000 scale. The first two digits define a longitude band 0.5 degree wide and the second two digits a latitude band 0.5 degree wide."@en ;skos:inScheme <https://linked.data.gov.au/def/geoadminfeatures> ;skos:broader geoad:MapSeries ;skos:notation "7753" ;skos:prefLabel "Culloden:7753"@en .
geoad:Potosi7853 a skos:Concept ;skos:definition "Map sheet for Potosi at 1:100 000 scale. The first two digits define a longitude band 0.5 degree wide and the second two digits a latitude band 0.5 degree wide."@en ;skos:inScheme <https://linked.data.gov.au/def/geoadminfeatures> ;skos:broader geoad:MapSeries ;skos:notation "7853" ;skos:prefLabel "Potosi:7853"@en .
geoad:Caledonia7953 a skos:Concept ;skos:definition "Map sheet for Caledonia at 1:100 000 scale. The first two digits define a longitude band 0.5 degree wide and the second two digits a latitude band 0.5 degree wide."@en ;skos:inScheme <https://linked.data.gov.au/def/geoadminfeatures> ;skos:broader geoad:MapSeries ;skos:notation "7953" ;skos:prefLabel "Caledonia:7953"@en .
geoad:Galilee8053 a skos:Concept ;skos:definition "Map sheet for Galilee at 1:100 000 scale. The first two digits define a longitude band 0.5 degree wide and the second two digits a latitude band 0.5 degree wide."@en ;skos:inScheme <https://linked.data.gov.au/def/geoadminfeatures> ;skos:broader geoad:MapSeries ;skos:notation "8053" ;skos:prefLabel "Galilee:8053"@en .
geoad:LouLouPark8153 a skos:Concept ;skos:definition "Map sheet for Lou Lou Park at 1:100 000 scale. The first two digits define a longitude band 0.5 degree wide and the second two digits a latitude band 0.5 degree wide."@en ;skos:inScheme <https://linked.data.gov.au/def/geoadminfeatures> ;skos:broader geoad:MapSeries ;skos:notation "8153" ;skos:prefLabel "Lou Lou Park:8153"@en .
geoad:EppingForest8253 a skos:Concept ;skos:definition "Map sheet for Epping Forest at 1:100 000 scale. The first two digits define a longitude band 0.5 degree wide and the second two digits a latitude band 0.5 degree wide."@en ;skos:inScheme <https://linked.data.gov.au/def/geoadminfeatures> ;skos:broader geoad:MapSeries ;skos:notation "8253" ;skos:prefLabel "Epping Forest:8253"@en .
geoad:Frankfield8353 a skos:Concept ;skos:definition "Map sheet for Frankfield at 1:100 000 scale. The first two digits define a longitude band 0.5 degree wide and the second two digits a latitude band 0.5 degree wide."@en ;skos:inScheme <https://linked.data.gov.au/def/geoadminfeatures> ;skos:broader geoad:MapSeries ;skos:notation "8353" ;skos:prefLabel "Frankfield:8353"@en .
geoad:Kilcummin8453 a skos:Concept ;skos:definition "Map sheet for Kilcummin at 1:100 000 scale. The first two digits define a longitude band 0.5 degree wide and the second two digits a latitude band 0.5 degree wide."@en ;skos:inScheme <https://linked.data.gov.au/def/geoadminfeatures> ;skos:broader geoad:MapSeries ;skos:notation "8453" ;skos:prefLabel "Kilcummin:8453"@en .
geoad:GrosvenorDowns8553 a skos:Concept ;skos:definition "Map sheet for Grosvenor Downs at 1:100 000 scale. The first two digits define a longitude band 0.5 degree wide and the second two digits a latitude band 0.5 degree wide."@en ;skos:inScheme <https://linked.data.gov.au/def/geoadminfeatures> ;skos:broader geoad:MapSeries ;skos:notation "8553" ;skos:prefLabel "Grosvenor Downs:8553"@en .
geoad:Bombandy8653 a skos:Concept ;skos:definition "Map sheet for Bombandy at 1:100 000 scale. The first two digits define a longitude band 0.5 degree wide and the second two digits a latitude band 0.5 degree wide."@en ;skos:inScheme <https://linked.data.gov.au/def/geoadminfeatures> ;skos:broader geoad:MapSeries ;skos:notation "8653" ;skos:prefLabel "Bombandy:8653"@en .
geoad:ConnorsRange8753 a skos:Concept ;skos:definition "Map sheet for Connors Range at 1:100 000 scale. The first two digits define a longitude band 0.5 degree wide and the second two digits a latitude band 0.5 degree wide."@en ;skos:inScheme <https://linked.data.gov.au/def/geoadminfeatures> ;skos:broader geoad:MapSeries ;skos:notation "8753" ;skos:prefLabel "Connors Range:8753"@en .
geoad:StLawrence8853 a skos:Concept ;skos:definition "Map sheet for St Lawrence at 1:100 000 scale. The first two digits define a longitude band 0.5 degree wide and the second two digits a latitude band 0.5 degree wide."@en ;skos:inScheme <https://linked.data.gov.au/def/geoadminfeatures> ;skos:broader geoad:MapSeries ;skos:notation "8853" ;skos:prefLabel "St Lawrence:8853"@en .
geoad:Shoalwater8953 a skos:Concept ;skos:definition "Map sheet for Shoalwater at 1:100 000 scale. The first two digits define a longitude band 0.5 degree wide and the second two digits a latitude band 0.5 degree wide."@en ;skos:inScheme <https://linked.data.gov.au/def/geoadminfeatures> ;skos:broader geoad:MapSeries ;skos:notation "8953" ;skos:prefLabel "Shoalwater:8953"@en .
geoad:PeninsulaRange9053 a skos:Concept ;skos:definition "Map sheet for Peninsula Range at 1:100 000 scale. The first two digits define a longitude band 0.5 degree wide and the second two digits a latitude band 0.5 degree wide."@en ;skos:inScheme <https://linked.data.gov.au/def/geoadminfeatures> ;skos:broader geoad:MapSeries ;skos:notation "9053" ;skos:prefLabel "Peninsula Range:9053"@en .
geoad:NeeyambaHill6552 a skos:Concept ;skos:definition "Map sheet for Neeyamba Hill at 1:100 000 scale. The first two digits define a longitude band 0.5 degree wide and the second two digits a latitude band 0.5 degree wide."@en ;skos:inScheme <https://linked.data.gov.au/def/geoadminfeatures> ;skos:broader geoad:MapSeries ;skos:notation "6552" ;skos:prefLabel "Neeyamba Hill:6552"@en .
geoad:Glenormiston6652 a skos:Concept ;skos:definition "Map sheet for Glenormiston at 1:100 000 scale. The first two digits define a longitude band 0.5 degree wide and the second two digits a latitude band 0.5 degree wide."@en ;skos:inScheme <https://linked.data.gov.au/def/geoadminfeatures> ;skos:broader geoad:MapSeries ;skos:notation "6652" ;skos:prefLabel "Glenormiston:6652"@en .
geoad:Badalia6752 a skos:Concept ;skos:definition "Map sheet for Badalia at 1:100 000 scale. The first two digits define a longitude band 0.5 degree wide and the second two digits a latitude band 0.5 degree wide."@en ;skos:inScheme <https://linked.data.gov.au/def/geoadminfeatures> ;skos:broader geoad:MapSeries ;skos:notation "6752" ;skos:prefLabel "Badalia:6752"@en .
geoad:Boulia6852 a skos:Concept ;skos:definition "Map sheet for Boulia at 1:100 000 scale. The first two digits define a longitude band 0.5 degree wide and the second two digits a latitude band 0.5 degree wide."@en ;skos:inScheme <https://linked.data.gov.au/def/geoadminfeatures> ;skos:broader geoad:MapSeries ;skos:notation "6852" ;skos:prefLabel "Boulia:6852"@en .
geoad:Goodwood6952 a skos:Concept ;skos:definition "Map sheet for Goodwood at 1:100 000 scale. The first two digits define a longitude band 0.5 degree wide and the second two digits a latitude band 0.5 degree wide."@en ;skos:inScheme <https://linked.data.gov.au/def/geoadminfeatures> ;skos:broader geoad:MapSeries ;skos:notation "6952" ;skos:prefLabel "Goodwood:6952"@en .
geoad:Lucknow7052 a skos:Concept ;skos:definition "Map sheet for Lucknow at 1:100 000 scale. The first two digits define a longitude band 0.5 degree wide and the second two digits a latitude band 0.5 degree wide."@en ;skos:inScheme <https://linked.data.gov.au/def/geoadminfeatures> ;skos:broader geoad:MapSeries ;skos:notation "7052" ;skos:prefLabel "Lucknow:7052"@en .
geoad:Mackunda7152 a skos:Concept ;skos:definition "Map sheet for Mackunda at 1:100 000 scale. The first two digits define a longitude band 0.5 degree wide and the second two digits a latitude band 0.5 degree wide."@en ;skos:inScheme <https://linked.data.gov.au/def/geoadminfeatures> ;skos:broader geoad:MapSeries ;skos:notation "7152" ;skos:prefLabel "Mackunda:7152"@en .
geoad:HillsRange7252 a skos:Concept ;skos:definition "Map sheet for Hills Range at 1:100 000 scale. The first two digits define a longitude band 0.5 degree wide and the second two digits a latitude band 0.5 degree wide."@en ;skos:inScheme <https://linked.data.gov.au/def/geoadminfeatures> ;skos:broader geoad:MapSeries ;skos:notation "7252" ;skos:prefLabel "Hills Range:7252"@en .
geoad:Tulmur7352 a skos:Concept ;skos:definition "Map sheet for Tulmur at 1:100 000 scale. The first two digits define a longitude band 0.5 degree wide and the second two digits a latitude band 0.5 degree wide."@en ;skos:inScheme <https://linked.data.gov.au/def/geoadminfeatures> ;skos:broader geoad:MapSeries ;skos:notation "7352" ;skos:prefLabel "Tulmur:7352"@en .
geoad:Warnambool7452 a skos:Concept ;skos:definition "Map sheet for Warnambool at 1:100 000 scale. The first two digits define a longitude band 0.5 degree wide and the second two digits a latitude band 0.5 degree wide."@en ;skos:inScheme <https://linked.data.gov.au/def/geoadminfeatures> ;skos:broader geoad:MapSeries ;skos:notation "7452" ;skos:prefLabel "Warnambool:7452"@en .
geoad:Vindex7552 a skos:Concept ;skos:definition "Map sheet for Vindex at 1:100 000 scale. The first two digits define a longitude band 0.5 degree wide and the second two digits a latitude band 0.5 degree wide."@en ;skos:inScheme <https://linked.data.gov.au/def/geoadminfeatures> ;skos:broader geoad:MapSeries ;skos:notation "7552" ;skos:prefLabel "Vindex:7552"@en .
geoad:Rimbanda7652 a skos:Concept ;skos:definition "Map sheet for Rimbanda at 1:100 000 scale. The first two digits define a longitude band 0.5 degree wide and the second two digits a latitude band 0.5 degree wide."@en ;skos:inScheme <https://linked.data.gov.au/def/geoadminfeatures> ;skos:broader geoad:MapSeries ;skos:notation "7652" ;skos:prefLabel "Rimbanda:7652"@en .
geoad:BradleyCreek7752 a skos:Concept ;skos:definition "Map sheet for Bradley Creek at 1:100 000 scale. The first two digits define a longitude band 0.5 degree wide and the second two digits a latitude band 0.5 degree wide."@en ;skos:inScheme <https://linked.data.gov.au/def/geoadminfeatures> ;skos:broader geoad:MapSeries ;skos:notation "7752" ;skos:prefLabel "Bradley Creek:7752"@en .
geoad:Muttaburra7852 a skos:Concept ;skos:definition "Map sheet for Muttaburra at 1:100 000 scale. The first two digits define a longitude band 0.5 degree wide and the second two digits a latitude band 0.5 degree wide."@en ;skos:inScheme <https://linked.data.gov.au/def/geoadminfeatures> ;skos:broader geoad:MapSeries ;skos:notation "7852" ;skos:prefLabel "Muttaburra:7852"@en .
geoad:Aramac7952 a skos:Concept ;skos:definition "Map sheet for Aramac at 1:100 000 scale. The first two digits define a longitude band 0.5 degree wide and the second two digits a latitude band 0.5 degree wide."@en ;skos:inScheme <https://linked.data.gov.au/def/geoadminfeatures> ;skos:broader geoad:MapSeries ;skos:notation "7952" ;skos:prefLabel "Aramac:7952"@en .
geoad:Boongoondoo8052 a skos:Concept ;skos:definition "Map sheet for Boongoondoo at 1:100 000 scale. The first two digits define a longitude band 0.5 degree wide and the second two digits a latitude band 0.5 degree wide."@en ;skos:inScheme <https://linked.data.gov.au/def/geoadminfeatures> ;skos:broader geoad:MapSeries ;skos:notation "8052" ;skos:prefLabel "Boongoondoo:8052"@en .
geoad:Dunrobin8152 a skos:Concept ;skos:definition "Map sheet for Dunrobin at 1:100 000 scale. The first two digits define a longitude band 0.5 degree wide and the second two digits a latitude band 0.5 degree wide."@en ;skos:inScheme <https://linked.data.gov.au/def/geoadminfeatures> ;skos:broader geoad:MapSeries ;skos:notation "8152" ;skos:prefLabel "Dunrobin:8152"@en .
geoad:Albro8252 a skos:Concept ;skos:definition "Map sheet for Albro at 1:100 000 scale. The first two digits define a longitude band 0.5 degree wide and the second two digits a latitude band 0.5 degree wide."@en ;skos:inScheme <https://linked.data.gov.au/def/geoadminfeatures> ;skos:broader geoad:MapSeries ;skos:notation "8252" ;skos:prefLabel "Albro:8252"@en .
geoad:Monteagle8352 a skos:Concept ;skos:definition "Map sheet for Monteagle at 1:100 000 scale. The first two digits define a longitude band 0.5 degree wide and the second two digits a latitude band 0.5 degree wide."@en ;skos:inScheme <https://linked.data.gov.au/def/geoadminfeatures> ;skos:broader geoad:MapSeries ;skos:notation "8352" ;skos:prefLabel "Monteagle:8352"@en .
geoad:Clermont8452 a skos:Concept ;skos:definition "Map sheet for Clermont at 1:100 000 scale. The first two digits define a longitude band 0.5 degree wide and the second two digits a latitude band 0.5 degree wide."@en ;skos:inScheme <https://linked.data.gov.au/def/geoadminfeatures> ;skos:broader geoad:MapSeries ;skos:notation "8452" ;skos:prefLabel "Clermont:8452"@en .
geoad:Cotherstone8552 a skos:Concept ;skos:definition "Map sheet for Cotherstone at 1:100 000 scale. The first two digits define a longitude band 0.5 degree wide and the second two digits a latitude band 0.5 degree wide."@en ;skos:inScheme <https://linked.data.gov.au/def/geoadminfeatures> ;skos:broader geoad:MapSeries ;skos:notation "8552" ;skos:prefLabel "Cotherstone:8552"@en .
geoad:WindeyersHill8652 a skos:Concept ;skos:definition "Map sheet for Windeyers Hill at 1:100 000 scale. The first two digits define a longitude band 0.5 degree wide and the second two digits a latitude band 0.5 degree wide."@en ;skos:inScheme <https://linked.data.gov.au/def/geoadminfeatures> ;skos:broader geoad:MapSeries ;skos:notation "8652" ;skos:prefLabel "Windeyers Hill:8652"@en .
geoad:MountBluffkin8752 a skos:Concept ;skos:definition "Map sheet for Mount Bluffkin at 1:100 000 scale. The first two digits define a longitude band 0.5 degree wide and the second two digits a latitude band 0.5 degree wide."@en ;skos:inScheme <https://linked.data.gov.au/def/geoadminfeatures> ;skos:broader geoad:MapSeries ;skos:notation "8752" ;skos:prefLabel "Mount Bluffkin:8752"@en .
geoad:Marlborough8852 a skos:Concept ;skos:definition "Map sheet for Marlborough at 1:100 000 scale. The first two digits define a longitude band 0.5 degree wide and the second two digits a latitude band 0.5 degree wide."@en ;skos:inScheme <https://linked.data.gov.au/def/geoadminfeatures> ;skos:broader geoad:MapSeries ;skos:notation "8852" ;skos:prefLabel "Marlborough:8852"@en .
geoad:Princhester8952 a skos:Concept ;skos:definition "Map sheet for Princhester at 1:100 000 scale. The first two digits define a longitude band 0.5 degree wide and the second two digits a latitude band 0.5 degree wide."@en ;skos:inScheme <https://linked.data.gov.au/def/geoadminfeatures> ;skos:broader geoad:MapSeries ;skos:notation "8952" ;skos:prefLabel "Princhester:8952"@en .
geoad:Bayfield9052 a skos:Concept ;skos:definition "Map sheet for Bayfield at 1:100 000 scale. The first two digits define a longitude band 0.5 degree wide and the second two digits a latitude band 0.5 degree wide."@en ;skos:inScheme <https://linked.data.gov.au/def/geoadminfeatures> ;skos:broader geoad:MapSeries ;skos:notation "9052" ;skos:prefLabel "Bayfield:9052"@en .
geoad:AbuddaLakes6551 a skos:Concept ;skos:definition "Map sheet for Abudda Lakes at 1:100 000 scale. The first two digits define a longitude band 0.5 degree wide and the second two digits a latitude band 0.5 degree wide."@en ;skos:inScheme <https://linked.data.gov.au/def/geoadminfeatures> ;skos:broader geoad:MapSeries ;skos:notation "6551" ;skos:prefLabel "Abudda Lakes:6551"@en .
geoad:MountWhelan6651 a skos:Concept ;skos:definition "Map sheet for Mount Whelan at 1:100 000 scale. The first two digits define a longitude band 0.5 degree wide and the second two digits a latitude band 0.5 degree wide."@en ;skos:inScheme <https://linked.data.gov.au/def/geoadminfeatures> ;skos:broader geoad:MapSeries ;skos:notation "6651" ;skos:prefLabel "Mount Whelan:6651"@en .
geoad:HerbertDowns6751 a skos:Concept ;skos:definition "Map sheet for Herbert Downs at 1:100 000 scale. The first two digits define a longitude band 0.5 degree wide and the second two digits a latitude band 0.5 degree wide."@en ;skos:inScheme <https://linked.data.gov.au/def/geoadminfeatures> ;skos:broader geoad:MapSeries ;skos:notation "6751" ;skos:prefLabel "Herbert Downs:6751"@en .
geoad:MarionDowns6851 a skos:Concept ;skos:definition "Map sheet for Marion Downs at 1:100 000 scale. The first two digits define a longitude band 0.5 degree wide and the second two digits a latitude band 0.5 degree wide."@en ;skos:inScheme <https://linked.data.gov.au/def/geoadminfeatures> ;skos:broader geoad:MapSeries ;skos:notation "6851" ;skos:prefLabel "Marion Downs:6851"@en .
geoad:Canary6951 a skos:Concept ;skos:definition "Map sheet for Canary at 1:100 000 scale. The first two digits define a longitude band 0.5 degree wide and the second two digits a latitude band 0.5 degree wide."@en ;skos:inScheme <https://linked.data.gov.au/def/geoadminfeatures> ;skos:broader geoad:MapSeries ;skos:notation "6951" ;skos:prefLabel "Canary:6951"@en .
geoad:ElizabethSprings7051 a skos:Concept ;skos:definition "Map sheet for Elizabeth Springs at 1:100 000 scale. The first two digits define a longitude band 0.5 degree wide and the second two digits a latitude band 0.5 degree wide."@en ;skos:inScheme <https://linked.data.gov.au/def/geoadminfeatures> ;skos:broader geoad:MapSeries ;skos:notation "7051" ;skos:prefLabel "Elizabeth Springs:7051"@en .
geoad:MacartneyRange7151 a skos:Concept ;skos:definition "Map sheet for Macartney Range at 1:100 000 scale. The first two digits define a longitude band 0.5 degree wide and the second two digits a latitude band 0.5 degree wide."@en ;skos:inScheme <https://linked.data.gov.au/def/geoadminfeatures> ;skos:broader geoad:MapSeries ;skos:notation "7151" ;skos:prefLabel "Macartney Range:7151"@en .
geoad:BrightonDowns7251 a skos:Concept ;skos:definition "Map sheet for Brighton Downs at 1:100 000 scale. The first two digits define a longitude band 0.5 degree wide and the second two digits a latitude band 0.5 degree wide."@en ;skos:inScheme <https://linked.data.gov.au/def/geoadminfeatures> ;skos:broader geoad:MapSeries ;skos:notation "7251" ;skos:prefLabel "Brighton Downs:7251"@en .
geoad:Rosebrook7351 a skos:Concept ;skos:definition "Map sheet for Rosebrook at 1:100 000 scale. The first two digits define a longitude band 0.5 degree wide and the second two digits a latitude band 0.5 degree wide."@en ;skos:inScheme <https://linked.data.gov.au/def/geoadminfeatures> ;skos:broader geoad:MapSeries ;skos:notation "7351" ;skos:prefLabel "Rosebrook:7351"@en .
geoad:Opalton7451 a skos:Concept ;skos:definition "Map sheet for Opalton at 1:100 000 scale. The first two digits define a longitude band 0.5 degree wide and the second two digits a latitude band 0.5 degree wide."@en ;skos:inScheme <https://linked.data.gov.au/def/geoadminfeatures> ;skos:broader geoad:MapSeries ;skos:notation "7451" ;skos:prefLabel "Opalton:7451"@en .
geoad:Fermoy7551 a skos:Concept ;skos:definition "Map sheet for Fermoy at 1:100 000 scale. The first two digits define a longitude band 0.5 degree wide and the second two digits a latitude band 0.5 degree wide."@en ;skos:inScheme <https://linked.data.gov.au/def/geoadminfeatures> ;skos:broader geoad:MapSeries ;skos:notation "7551" ;skos:prefLabel "Fermoy:7551"@en .
geoad:Maneroo7651 a skos:Concept ;skos:definition "Map sheet for Maneroo at 1:100 000 scale. The first two digits define a longitude band 0.5 degree wide and the second two digits a latitude band 0.5 degree wide."@en ;skos:inScheme <https://linked.data.gov.au/def/geoadminfeatures> ;skos:broader geoad:MapSeries ;skos:notation "7651" ;skos:prefLabel "Maneroo:7651"@en .
geoad:Longreach7751 a skos:Concept ;skos:definition "Map sheet for Longreach at 1:100 000 scale. The first two digits define a longitude band 0.5 degree wide and the second two digits a latitude band 0.5 degree wide."@en ;skos:inScheme <https://linked.data.gov.au/def/geoadminfeatures> ;skos:broader geoad:MapSeries ;skos:notation "7751" ;skos:prefLabel "Longreach:7751"@en .
geoad:Ilfracombe7851 a skos:Concept ;skos:definition "Map sheet for Ilfracombe at 1:100 000 scale. The first two digits define a longitude band 0.5 degree wide and the second two digits a latitude band 0.5 degree wide."@en ;skos:inScheme <https://linked.data.gov.au/def/geoadminfeatures> ;skos:broader geoad:MapSeries ;skos:notation "7851" ;skos:prefLabel "Ilfracombe:7851"@en .
geoad:Bowyer7951 a skos:Concept ;skos:definition "Map sheet for Bowyer at 1:100 000 scale. The first two digits define a longitude band 0.5 degree wide and the second two digits a latitude band 0.5 degree wide."@en ;skos:inScheme <https://linked.data.gov.au/def/geoadminfeatures> ;skos:broader geoad:MapSeries ;skos:notation "7951" ;skos:prefLabel "Bowyer:7951"@en .
geoad:Garfield8051 a skos:Concept ;skos:definition "Map sheet for Garfield at 1:100 000 scale. The first two digits define a longitude band 0.5 degree wide and the second two digits a latitude band 0.5 degree wide."@en ;skos:inScheme <https://linked.data.gov.au/def/geoadminfeatures> ;skos:broader geoad:MapSeries ;skos:notation "8051" ;skos:prefLabel "Garfield:8051"@en .
geoad:Edwinstowe8151 a skos:Concept ;skos:definition "Map sheet for Edwinstowe at 1:100 000 scale. The first two digits define a longitude band 0.5 degree wide and the second two digits a latitude band 0.5 degree wide."@en ;skos:inScheme <https://linked.data.gov.au/def/geoadminfeatures> ;skos:broader geoad:MapSeries ;skos:notation "8151" ;skos:prefLabel "Edwinstowe:8151"@en .
geoad:Surbiton8251 a skos:Concept ;skos:definition "Map sheet for Surbiton at 1:100 000 scale. The first two digits define a longitude band 0.5 degree wide and the second two digits a latitude band 0.5 degree wide."@en ;skos:inScheme <https://linked.data.gov.au/def/geoadminfeatures> ;skos:broader geoad:MapSeries ;skos:notation "8251" ;skos:prefLabel "Surbiton:8251"@en .
geoad:ZigZag8351 a skos:Concept ;skos:definition "Map sheet for Zig Zag at 1:100 000 scale. The first two digits define a longitude band 0.5 degree wide and the second two digits a latitude band 0.5 degree wide."@en ;skos:inScheme <https://linked.data.gov.au/def/geoadminfeatures> ;skos:broader geoad:MapSeries ;skos:notation "8351" ;skos:prefLabel "Zig Zag:8351"@en .
geoad:Rubyvale8451 a skos:Concept ;skos:definition "Map sheet for Rubyvale at 1:100 000 scale. The first two digits define a longitude band 0.5 degree wide and the second two digits a latitude band 0.5 degree wide."@en ;skos:inScheme <https://linked.data.gov.au/def/geoadminfeatures> ;skos:broader geoad:MapSeries ;skos:notation "8451" ;skos:prefLabel "Rubyvale:8451"@en .
geoad:Capella8551 a skos:Concept ;skos:definition "Map sheet for Capella at 1:100 000 scale. The first two digits define a longitude band 0.5 degree wide and the second two digits a latitude band 0.5 degree wide."@en ;skos:inScheme <https://linked.data.gov.au/def/geoadminfeatures> ;skos:broader geoad:MapSeries ;skos:notation "8551" ;skos:prefLabel "Capella:8551"@en .
geoad:Cooroorah8651 a skos:Concept ;skos:definition "Map sheet for Cooroorah at 1:100 000 scale. The first two digits define a longitude band 0.5 degree wide and the second two digits a latitude band 0.5 degree wide."@en ;skos:inScheme <https://linked.data.gov.au/def/geoadminfeatures> ;skos:broader geoad:MapSeries ;skos:notation "8651" ;skos:prefLabel "Cooroorah:8651"@en .
geoad:Strathconan8751 a skos:Concept ;skos:definition "Map sheet for Strathconan at 1:100 000 scale. The first two digits define a longitude band 0.5 degree wide and the second two digits a latitude band 0.5 degree wide."@en ;skos:inScheme <https://linked.data.gov.au/def/geoadminfeatures> ;skos:broader geoad:MapSeries ;skos:notation "8751" ;skos:prefLabel "Strathconan:8751"@en .
geoad:Rookwood8851 a skos:Concept ;skos:definition "Map sheet for Rookwood at 1:100 000 scale. The first two digits define a longitude band 0.5 degree wide and the second two digits a latitude band 0.5 degree wide."@en ;skos:inScheme <https://linked.data.gov.au/def/geoadminfeatures> ;skos:broader geoad:MapSeries ;skos:notation "8851" ;skos:prefLabel "Rookwood:8851"@en .
geoad:Ridgelands8951 a skos:Concept ;skos:definition "Map sheet for Ridgelands at 1:100 000 scale. The first two digits define a longitude band 0.5 degree wide and the second two digits a latitude band 0.5 degree wide."@en ;skos:inScheme <https://linked.data.gov.au/def/geoadminfeatures> ;skos:broader geoad:MapSeries ;skos:notation "8951" ;skos:prefLabel "Ridgelands:8951"@en .
geoad:Rockhampton9051 a skos:Concept ;skos:definition "Map sheet for Rockhampton at 1:100 000 scale. The first two digits define a longitude band 0.5 degree wide and the second two digits a latitude band 0.5 degree wide."@en ;skos:inScheme <https://linked.data.gov.au/def/geoadminfeatures> ;skos:broader geoad:MapSeries ;skos:notation "9051" ;skos:prefLabel "Rockhampton:9051"@en .
geoad:CapeCapricorn9151 a skos:Concept ;skos:definition "Map sheet for Cape Capricorn at 1:100 000 scale. The first two digits define a longitude band 0.5 degree wide and the second two digits a latitude band 0.5 degree wide."@en ;skos:inScheme <https://linked.data.gov.au/def/geoadminfeatures> ;skos:broader geoad:MapSeries ;skos:notation "9151" ;skos:prefLabel "Cape Capricorn:9151"@en .
geoad:HeronIsland9251 a skos:Concept ;skos:definition "Map sheet for Heron Island at 1:100 000 scale. The first two digits define a longitude band 0.5 degree wide and the second two digits a latitude band 0.5 degree wide."@en ;skos:inScheme <https://linked.data.gov.au/def/geoadminfeatures> ;skos:broader geoad:MapSeries ;skos:notation "9251" ;skos:prefLabel "Heron Island:9251"@en .
geoad:MirricaBore6550 a skos:Concept ;skos:definition "Map sheet for Mirrica Bore at 1:100 000 scale. The first two digits define a longitude band 0.5 degree wide and the second two digits a latitude band 0.5 degree wide."@en ;skos:inScheme <https://linked.data.gov.au/def/geoadminfeatures> ;skos:broader geoad:MapSeries ;skos:notation "6550" ;skos:prefLabel "Mirrica Bore:6550"@en .
geoad:BarringtonPeak6650 a skos:Concept ;skos:definition "Map sheet for Barrington Peak at 1:100 000 scale. The first two digits define a longitude band 0.5 degree wide and the second two digits a latitude band 0.5 degree wide."@en ;skos:inScheme <https://linked.data.gov.au/def/geoadminfeatures> ;skos:broader geoad:MapSeries ;skos:notation "6650" ;skos:prefLabel "Barrington Peak:6650"@en .
geoad:MountTarley6750 a skos:Concept ;skos:definition "Map sheet for Mount Tarley at 1:100 000 scale. The first two digits define a longitude band 0.5 degree wide and the second two digits a latitude band 0.5 degree wide."@en ;skos:inScheme <https://linked.data.gov.au/def/geoadminfeatures> ;skos:broader geoad:MapSeries ;skos:notation "6750" ;skos:prefLabel "Mount Tarley:6750"@en .
geoad:Breadalbane6850 a skos:Concept ;skos:definition "Map sheet for Breadalbane at 1:100 000 scale. The first two digits define a longitude band 0.5 degree wide and the second two digits a latitude band 0.5 degree wide."@en ;skos:inScheme <https://linked.data.gov.au/def/geoadminfeatures> ;skos:broader geoad:MapSeries ;skos:notation "6850" ;skos:prefLabel "Breadalbane:6850"@en .
geoad:Coorabulka6950 a skos:Concept ;skos:definition "Map sheet for Coorabulka at 1:100 000 scale. The first two digits define a longitude band 0.5 degree wide and the second two digits a latitude band 0.5 degree wide."@en ;skos:inScheme <https://linked.data.gov.au/def/geoadminfeatures> ;skos:broader geoad:MapSeries ;skos:notation "6950" ;skos:prefLabel "Coorabulka:6950"@en .
geoad:Springvale7050 a skos:Concept ;skos:definition "Map sheet for Springvale at 1:100 000 scale. The first two digits define a longitude band 0.5 degree wide and the second two digits a latitude band 0.5 degree wide."@en ;skos:inScheme <https://linked.data.gov.au/def/geoadminfeatures> ;skos:broader geoad:MapSeries ;skos:notation "7050" ;skos:prefLabel "Springvale:7050"@en .
geoad:DiamantinaLakes7150 a skos:Concept ;skos:definition "Map sheet for Diamantina Lakes at 1:100 000 scale. The first two digits define a longitude band 0.5 degree wide and the second two digits a latitude band 0.5 degree wide."@en ;skos:inScheme <https://linked.data.gov.au/def/geoadminfeatures> ;skos:broader geoad:MapSeries ;skos:notation "7150" ;skos:prefLabel "Diamantina Lakes:7150"@en .
geoad:MountEdwardGraves7250 a skos:Concept ;skos:definition "Map sheet for Mount Edward Graves at 1:100 000 scale. The first two digits define a longitude band 0.5 degree wide and the second two digits a latitude band 0.5 degree wide."@en ;skos:inScheme <https://linked.data.gov.au/def/geoadminfeatures> ;skos:broader geoad:MapSeries ;skos:notation "7250" ;skos:prefLabel "Mount Edward Graves:7250"@en .
geoad:Tonkoro7350 a skos:Concept ;skos:definition "Map sheet for Tonkoro at 1:100 000 scale. The first two digits define a longitude band 0.5 degree wide and the second two digits a latitude band 0.5 degree wide."@en ;skos:inScheme <https://linked.data.gov.au/def/geoadminfeatures> ;skos:broader geoad:MapSeries ;skos:notation "7350" ;skos:prefLabel "Tonkoro:7350"@en .
geoad:Mayneside7450 a skos:Concept ;skos:definition "Map sheet for Mayneside at 1:100 000 scale. The first two digits define a longitude band 0.5 degree wide and the second two digits a latitude band 0.5 degree wide."@en ;skos:inScheme <https://linked.data.gov.au/def/geoadminfeatures> ;skos:broader geoad:MapSeries ;skos:notation "7450" ;skos:prefLabel "Mayneside:7450"@en .
geoad:Vergemont7550 a skos:Concept ;skos:definition "Map sheet for Vergemont at 1:100 000 scale. The first two digits define a longitude band 0.5 degree wide and the second two digits a latitude band 0.5 degree wide."@en ;skos:inScheme <https://linked.data.gov.au/def/geoadminfeatures> ;skos:broader geoad:MapSeries ;skos:notation "7550" ;skos:prefLabel "Vergemont:7550"@en .
geoad:Arrilalah7650 a skos:Concept ;skos:definition "Map sheet for Arrilalah at 1:100 000 scale. The first two digits define a longitude band 0.5 degree wide and the second two digits a latitude band 0.5 degree wide."@en ;skos:inScheme <https://linked.data.gov.au/def/geoadminfeatures> ;skos:broader geoad:MapSeries ;skos:notation "7650" ;skos:prefLabel "Arrilalah:7650"@en .
geoad:Wellshot7750 a skos:Concept ;skos:definition "Map sheet for Wellshot at 1:100 000 scale. The first two digits define a longitude band 0.5 degree wide and the second two digits a latitude band 0.5 degree wide."@en ;skos:inScheme <https://linked.data.gov.au/def/geoadminfeatures> ;skos:broader geoad:MapSeries ;skos:notation "7750" ;skos:prefLabel "Wellshot:7750"@en .
geoad:Oakhampton7850 a skos:Concept ;skos:definition "Map sheet for Oakhampton at 1:100 000 scale. The first two digits define a longitude band 0.5 degree wide and the second two digits a latitude band 0.5 degree wide."@en ;skos:inScheme <https://linked.data.gov.au/def/geoadminfeatures> ;skos:broader geoad:MapSeries ;skos:notation "7850" ;skos:prefLabel "Oakhampton:7850"@en .
geoad:Barcaldine7950 a skos:Concept ;skos:definition "Map sheet for Barcaldine at 1:100 000 scale. The first two digits define a longitude band 0.5 degree wide and the second two digits a latitude band 0.5 degree wide."@en ;skos:inScheme <https://linked.data.gov.au/def/geoadminfeatures> ;skos:broader geoad:MapSeries ;skos:notation "7950" ;skos:prefLabel "Barcaldine:7950"@en .
geoad:Busthinia8050 a skos:Concept ;skos:definition "Map sheet for Busthinia at 1:100 000 scale. The first two digits define a longitude band 0.5 degree wide and the second two digits a latitude band 0.5 degree wide."@en ;skos:inScheme <https://linked.data.gov.au/def/geoadminfeatures> ;skos:broader geoad:MapSeries ;skos:notation "8050" ;skos:prefLabel "Busthinia:8050"@en .
geoad:Jericho8150 a skos:Concept ;skos:definition "Map sheet for Jericho at 1:100 000 scale. The first two digits define a longitude band 0.5 degree wide and the second two digits a latitude band 0.5 degree wide."@en ;skos:inScheme <https://linked.data.gov.au/def/geoadminfeatures> ;skos:broader geoad:MapSeries ;skos:notation "8150" ;skos:prefLabel "Jericho:8150"@en .
geoad:Alpha8250 a skos:Concept ;skos:definition "Map sheet for Alpha at 1:100 000 scale. The first two digits define a longitude band 0.5 degree wide and the second two digits a latitude band 0.5 degree wide."@en ;skos:inScheme <https://linked.data.gov.au/def/geoadminfeatures> ;skos:broader geoad:MapSeries ;skos:notation "8250" ;skos:prefLabel "Alpha:8250"@en .
geoad:Bogantungan8350 a skos:Concept ;skos:definition "Map sheet for Bogantungan at 1:100 000 scale. The first two digits define a longitude band 0.5 degree wide and the second two digits a latitude band 0.5 degree wide."@en ;skos:inScheme <https://linked.data.gov.au/def/geoadminfeatures> ;skos:broader geoad:MapSeries ;skos:notation "8350" ;skos:prefLabel "Bogantungan:8350"@en .
geoad:Anakie8450 a skos:Concept ;skos:definition "Map sheet for Anakie at 1:100 000 scale. The first two digits define a longitude band 0.5 degree wide and the second two digits a latitude band 0.5 degree wide."@en ;skos:inScheme <https://linked.data.gov.au/def/geoadminfeatures> ;skos:broader geoad:MapSeries ;skos:notation "8450" ;skos:prefLabel "Anakie:8450"@en .
geoad:Emerald8550 a skos:Concept ;skos:definition "Map sheet for Emerald at 1:100 000 scale. The first two digits define a longitude band 0.5 degree wide and the second two digits a latitude band 0.5 degree wide."@en ;skos:inScheme <https://linked.data.gov.au/def/geoadminfeatures> ;skos:broader geoad:MapSeries ;skos:notation "8550" ;skos:prefLabel "Emerald:8550"@en .
geoad:Comet8650 a skos:Concept ;skos:definition "Map sheet for Comet at 1:100 000 scale. The first two digits define a longitude band 0.5 degree wide and the second two digits a latitude band 0.5 degree wide."@en ;skos:inScheme <https://linked.data.gov.au/def/geoadminfeatures> ;skos:broader geoad:MapSeries ;skos:notation "8650" ;skos:prefLabel "Comet:8650"@en .
geoad:Dingo8750 a skos:Concept ;skos:definition "Map sheet for Dingo at 1:100 000 scale. The first two digits define a longitude band 0.5 degree wide and the second two digits a latitude band 0.5 degree wide."@en ;skos:inScheme <https://linked.data.gov.au/def/geoadminfeatures> ;skos:broader geoad:MapSeries ;skos:notation "8750" ;skos:prefLabel "Dingo:8750"@en .
geoad:Duaringa8850 a skos:Concept ;skos:definition "Map sheet for Duaringa at 1:100 000 scale. The first two digits define a longitude band 0.5 degree wide and the second two digits a latitude band 0.5 degree wide."@en ;skos:inScheme <https://linked.data.gov.au/def/geoadminfeatures> ;skos:broader geoad:MapSeries ;skos:notation "8850" ;skos:prefLabel "Duaringa:8850"@en .
geoad:MountMorgan8950 a skos:Concept ;skos:definition "Map sheet for Mount Morgan at 1:100 000 scale. The first two digits define a longitude band 0.5 degree wide and the second two digits a latitude band 0.5 degree wide."@en ;skos:inScheme <https://linked.data.gov.au/def/geoadminfeatures> ;skos:broader geoad:MapSeries ;skos:notation "8950" ;skos:prefLabel "Mount Morgan:8950"@en .
geoad:Bajool9050 a skos:Concept ;skos:definition "Map sheet for Bajool at 1:100 000 scale. The first two digits define a longitude band 0.5 degree wide and the second two digits a latitude band 0.5 degree wide."@en ;skos:inScheme <https://linked.data.gov.au/def/geoadminfeatures> ;skos:broader geoad:MapSeries ;skos:notation "9050" ;skos:prefLabel "Bajool:9050"@en .
geoad:Gladstone9150 a skos:Concept ;skos:definition "Map sheet for Gladstone at 1:100 000 scale. The first two digits define a longitude band 0.5 degree wide and the second two digits a latitude band 0.5 degree wide."@en ;skos:inScheme <https://linked.data.gov.au/def/geoadminfeatures> ;skos:broader geoad:MapSeries ;skos:notation "9150" ;skos:prefLabel "Gladstone:9150"@en .
geoad:RoddsBay9250 a skos:Concept ;skos:definition "Map sheet for Rodds Bay at 1:100 000 scale. The first two digits define a longitude band 0.5 degree wide and the second two digits a latitude band 0.5 degree wide."@en ;skos:inScheme <https://linked.data.gov.au/def/geoadminfeatures> ;skos:broader geoad:MapSeries ;skos:notation "9250" ;skos:prefLabel "Rodds Bay:9250"@en .
geoad:HoskynIsland9350 a skos:Concept ;skos:definition "Map sheet for Hoskyn Island at 1:100 000 scale. The first two digits define a longitude band 0.5 degree wide and the second two digits a latitude band 0.5 degree wide."@en ;skos:inScheme <https://linked.data.gov.au/def/geoadminfeatures> ;skos:broader geoad:MapSeries ;skos:notation "9350" ;skos:prefLabel "Hoskyn Island:9350"@en .
geoad:GnallanAGeaCreek6549 a skos:Concept ;skos:definition "Map sheet for Gnallan A Gea Creek at 1:100 000 scale. The first two digits define a longitude band 0.5 degree wide and the second two digits a latitude band 0.5 degree wide."@en ;skos:inScheme <https://linked.data.gov.au/def/geoadminfeatures> ;skos:broader geoad:MapSeries ;skos:notation "6549" ;skos:prefLabel "Gnallan A Gea Creek:6549"@en .
geoad:Teriwa6649 a skos:Concept ;skos:definition "Map sheet for Teriwa at 1:100 000 scale. The first two digits define a longitude band 0.5 degree wide and the second two digits a latitude band 0.5 degree wide."@en ;skos:inScheme <https://linked.data.gov.au/def/geoadminfeatures> ;skos:broader geoad:MapSeries ;skos:notation "6649" ;skos:prefLabel "Teriwa:6649"@en .
geoad:Bedourie6749 a skos:Concept ;skos:definition "Map sheet for Bedourie at 1:100 000 scale. The first two digits define a longitude band 0.5 degree wide and the second two digits a latitude band 0.5 degree wide."@en ;skos:inScheme <https://linked.data.gov.au/def/geoadminfeatures> ;skos:broader geoad:MapSeries ;skos:notation "6749" ;skos:prefLabel "Bedourie:6749"@en .
geoad:Marduroo6849 a skos:Concept ;skos:definition "Map sheet for Marduroo at 1:100 000 scale. The first two digits define a longitude band 0.5 degree wide and the second two digits a latitude band 0.5 degree wide."@en ;skos:inScheme <https://linked.data.gov.au/def/geoadminfeatures> ;skos:broader geoad:MapSeries ;skos:notation "6849" ;skos:prefLabel "Marduroo:6849"@en .
geoad:MountWoneeala6949 a skos:Concept ;skos:definition "Map sheet for Mount Woneeala at 1:100 000 scale. The first two digits define a longitude band 0.5 degree wide and the second two digits a latitude band 0.5 degree wide."@en ;skos:inScheme <https://linked.data.gov.au/def/geoadminfeatures> ;skos:broader geoad:MapSeries ;skos:notation "6949" ;skos:prefLabel "Mount Woneeala:6949"@en .
geoad:Peleenah7049 a skos:Concept ;skos:definition "Map sheet for Peleenah at 1:100 000 scale. The first two digits define a longitude band 0.5 degree wide and the second two digits a latitude band 0.5 degree wide."@en ;skos:inScheme <https://linked.data.gov.au/def/geoadminfeatures> ;skos:broader geoad:MapSeries ;skos:notation "7049" ;skos:prefLabel "Peleenah:7049"@en .
geoad:DavenportDowns7149 a skos:Concept ;skos:definition "Map sheet for Davenport Downs at 1:100 000 scale. The first two digits define a longitude band 0.5 degree wide and the second two digits a latitude band 0.5 degree wide."@en ;skos:inScheme <https://linked.data.gov.au/def/geoadminfeatures> ;skos:broader geoad:MapSeries ;skos:notation "7149" ;skos:prefLabel "Davenport Downs:7149"@en .
geoad:Merabooka7249 a skos:Concept ;skos:definition "Map sheet for Merabooka at 1:100 000 scale. The first two digits define a longitude band 0.5 degree wide and the second two digits a latitude band 0.5 degree wide."@en ;skos:inScheme <https://linked.data.gov.au/def/geoadminfeatures> ;skos:broader geoad:MapSeries ;skos:notation "7249" ;skos:prefLabel "Merabooka:7249"@en .
geoad:Connemara7349 a skos:Concept ;skos:definition "Map sheet for Connemara at 1:100 000 scale. The first two digits define a longitude band 0.5 degree wide and the second two digits a latitude band 0.5 degree wide."@en ;skos:inScheme <https://linked.data.gov.au/def/geoadminfeatures> ;skos:broader geoad:MapSeries ;skos:notation "7349" ;skos:prefLabel "Connemara:7349"@en .
geoad:Warbreccan7449 a skos:Concept ;skos:definition "Map sheet for Warbreccan at 1:100 000 scale. The first two digits define a longitude band 0.5 degree wide and the second two digits a latitude band 0.5 degree wide."@en ;skos:inScheme <https://linked.data.gov.au/def/geoadminfeatures> ;skos:broader geoad:MapSeries ;skos:notation "7449" ;skos:prefLabel "Warbreccan:7449"@en .
geoad:Stonehenge7549 a skos:Concept ;skos:definition "Map sheet for Stonehenge at 1:100 000 scale. The first two digits define a longitude band 0.5 degree wide and the second two digits a latitude band 0.5 degree wide."@en ;skos:inScheme <https://linked.data.gov.au/def/geoadminfeatures> ;skos:broader geoad:MapSeries ;skos:notation "7549" ;skos:prefLabel "Stonehenge:7549"@en .
geoad:Bimerah7649 a skos:Concept ;skos:definition "Map sheet for Bimerah at 1:100 000 scale. The first two digits define a longitude band 0.5 degree wide and the second two digits a latitude band 0.5 degree wide."@en ;skos:inScheme <https://linked.data.gov.au/def/geoadminfeatures> ;skos:broader geoad:MapSeries ;skos:notation "7649" ;skos:prefLabel "Bimerah:7649"@en .
geoad:Isisford7749 a skos:Concept ;skos:definition "Map sheet for Isisford at 1:100 000 scale. The first two digits define a longitude band 0.5 degree wide and the second two digits a latitude band 0.5 degree wide."@en ;skos:inScheme <https://linked.data.gov.au/def/geoadminfeatures> ;skos:broader geoad:MapSeries ;skos:notation "7749" ;skos:prefLabel "Isisford:7749"@en .
geoad:PortlandDowns7849 a skos:Concept ;skos:definition "Map sheet for Portland Downs at 1:100 000 scale. The first two digits define a longitude band 0.5 degree wide and the second two digits a latitude band 0.5 degree wide."@en ;skos:inScheme <https://linked.data.gov.au/def/geoadminfeatures> ;skos:broader geoad:MapSeries ;skos:notation "7849" ;skos:prefLabel "Portland Downs:7849"@en .
geoad:Blackall7949 a skos:Concept ;skos:definition "Map sheet for Blackall at 1:100 000 scale. The first two digits define a longitude band 0.5 degree wide and the second two digits a latitude band 0.5 degree wide."@en ;skos:inScheme <https://linked.data.gov.au/def/geoadminfeatures> ;skos:broader geoad:MapSeries ;skos:notation "7949" ;skos:prefLabel "Blackall:7949"@en .
geoad:Glenusk8049 a skos:Concept ;skos:definition "Map sheet for Glenusk at 1:100 000 scale. The first two digits define a longitude band 0.5 degree wide and the second two digits a latitude band 0.5 degree wide."@en ;skos:inScheme <https://linked.data.gov.au/def/geoadminfeatures> ;skos:broader geoad:MapSeries ;skos:notation "8049" ;skos:prefLabel "Glenusk:8049"@en .
geoad:Cheshire8149 a skos:Concept ;skos:definition "Map sheet for Cheshire at 1:100 000 scale. The first two digits define a longitude band 0.5 degree wide and the second two digits a latitude band 0.5 degree wide."@en ;skos:inScheme <https://linked.data.gov.au/def/geoadminfeatures> ;skos:broader geoad:MapSeries ;skos:notation "8149" ;skos:prefLabel "Cheshire:8149"@en .
geoad:TroopersBluff8249 a skos:Concept ;skos:definition "Map sheet for Troopers Bluff at 1:100 000 scale. The first two digits define a longitude band 0.5 degree wide and the second two digits a latitude band 0.5 degree wide."@en ;skos:inScheme <https://linked.data.gov.au/def/geoadminfeatures> ;skos:broader geoad:MapSeries ;skos:notation "8249" ;skos:prefLabel "Troopers Bluff:8249"@en .
geoad:MantuanDowns8349 a skos:Concept ;skos:definition "Map sheet for Mantuan Downs at 1:100 000 scale. The first two digits define a longitude band 0.5 degree wide and the second two digits a latitude band 0.5 degree wide."@en ;skos:inScheme <https://linked.data.gov.au/def/geoadminfeatures> ;skos:broader geoad:MapSeries ;skos:notation "8349" ;skos:prefLabel "Mantuan Downs:8349"@en .
geoad:Nandowrie8449 a skos:Concept ;skos:definition "Map sheet for Nandowrie at 1:100 000 scale. The first two digits define a longitude band 0.5 degree wide and the second two digits a latitude band 0.5 degree wide."@en ;skos:inScheme <https://linked.data.gov.au/def/geoadminfeatures> ;skos:broader geoad:MapSeries ;skos:notation "8449" ;skos:prefLabel "Nandowrie:8449"@en .
geoad:Springsure8549 a skos:Concept ;skos:definition "Map sheet for Springsure at 1:100 000 scale. The first two digits define a longitude band 0.5 degree wide and the second two digits a latitude band 0.5 degree wide."@en ;skos:inScheme <https://linked.data.gov.au/def/geoadminfeatures> ;skos:broader geoad:MapSeries ;skos:notation "8549" ;skos:prefLabel "Springsure:8549"@en .
geoad:Rolleston8649 a skos:Concept ;skos:definition "Map sheet for Rolleston at 1:100 000 scale. The first two digits define a longitude band 0.5 degree wide and the second two digits a latitude band 0.5 degree wide."@en ;skos:inScheme <https://linked.data.gov.au/def/geoadminfeatures> ;skos:broader geoad:MapSeries ;skos:notation "8649" ;skos:prefLabel "Rolleston:8649"@en .
geoad:Woorabinda8749 a skos:Concept ;skos:definition "Map sheet for Woorabinda at 1:100 000 scale. The first two digits define a longitude band 0.5 degree wide and the second two digits a latitude band 0.5 degree wide."@en ;skos:inScheme <https://linked.data.gov.au/def/geoadminfeatures> ;skos:broader geoad:MapSeries ;skos:notation "8749" ;skos:prefLabel "Woorabinda:8749"@en .
geoad:Baralaba8849 a skos:Concept ;skos:definition "Map sheet for Baralaba at 1:100 000 scale. The first two digits define a longitude band 0.5 degree wide and the second two digits a latitude band 0.5 degree wide."@en ;skos:inScheme <https://linked.data.gov.au/def/geoadminfeatures> ;skos:broader geoad:MapSeries ;skos:notation "8849" ;skos:prefLabel "Baralaba:8849"@en .
geoad:Banana8949 a skos:Concept ;skos:definition "Map sheet for Banana at 1:100 000 scale. The first two digits define a longitude band 0.5 degree wide and the second two digits a latitude band 0.5 degree wide."@en ;skos:inScheme <https://linked.data.gov.au/def/geoadminfeatures> ;skos:broader geoad:MapSeries ;skos:notation "8949" ;skos:prefLabel "Banana:8949"@en .
geoad:Biloela9049 a skos:Concept ;skos:definition "Map sheet for Biloela at 1:100 000 scale. The first two digits define a longitude band 0.5 degree wide and the second two digits a latitude band 0.5 degree wide."@en ;skos:inScheme <https://linked.data.gov.au/def/geoadminfeatures> ;skos:broader geoad:MapSeries ;skos:notation "9049" ;skos:prefLabel "Biloela:9049"@en .
geoad:Calliope9149 a skos:Concept ;skos:definition "Map sheet for Calliope at 1:100 000 scale. The first two digits define a longitude band 0.5 degree wide and the second two digits a latitude band 0.5 degree wide."@en ;skos:inScheme <https://linked.data.gov.au/def/geoadminfeatures> ;skos:broader geoad:MapSeries ;skos:notation "9149" ;skos:prefLabel "Calliope:9149"@en .
geoad:MiriamVale9249 a skos:Concept ;skos:definition "Map sheet for Miriam Vale at 1:100 000 scale. The first two digits define a longitude band 0.5 degree wide and the second two digits a latitude band 0.5 degree wide."@en ;skos:inScheme <https://linked.data.gov.au/def/geoadminfeatures> ;skos:broader geoad:MapSeries ;skos:notation "9249" ;skos:prefLabel "Miriam Vale:9249"@en .
geoad:MitchellCreek9349 a skos:Concept ;skos:definition "Map sheet for Mitchell Creek at 1:100 000 scale. The first two digits define a longitude band 0.5 degree wide and the second two digits a latitude band 0.5 degree wide."@en ;skos:inScheme <https://linked.data.gov.au/def/geoadminfeatures> ;skos:broader geoad:MapSeries ;skos:notation "9349" ;skos:prefLabel "Mitchell Creek:9349"@en .
geoad:Mudloo6548 a skos:Concept ;skos:definition "Map sheet for Mudloo at 1:100 000 scale. The first two digits define a longitude band 0.5 degree wide and the second two digits a latitude band 0.5 degree wide."@en ;skos:inScheme <https://linked.data.gov.au/def/geoadminfeatures> ;skos:broader geoad:MapSeries ;skos:notation "6548" ;skos:prefLabel "Mudloo:6548"@en .
geoad:LakeTorquinie6648 a skos:Concept ;skos:definition "Map sheet for Lake Torquinie at 1:100 000 scale. The first two digits define a longitude band 0.5 degree wide and the second two digits a latitude band 0.5 degree wide."@en ;skos:inScheme <https://linked.data.gov.au/def/geoadminfeatures> ;skos:broader geoad:MapSeries ;skos:notation "6648" ;skos:prefLabel "Lake Torquinie:6648"@en .
geoad:Murraturley6748 a skos:Concept ;skos:definition "Map sheet for Murraturley at 1:100 000 scale. The first two digits define a longitude band 0.5 degree wide and the second two digits a latitude band 0.5 degree wide."@en ;skos:inScheme <https://linked.data.gov.au/def/geoadminfeatures> ;skos:broader geoad:MapSeries ;skos:notation "6748" ;skos:prefLabel "Murraturley:6748"@en .
geoad:Machattie6848 a skos:Concept ;skos:definition "Map sheet for Machattie at 1:100 000 scale. The first two digits define a longitude band 0.5 degree wide and the second two digits a latitude band 0.5 degree wide."@en ;skos:inScheme <https://linked.data.gov.au/def/geoadminfeatures> ;skos:broader geoad:MapSeries ;skos:notation "6848" ;skos:prefLabel "Machattie:6848"@en .
geoad:MountCuttiguree6948 a skos:Concept ;skos:definition "Map sheet for Mount Cuttiguree at 1:100 000 scale. The first two digits define a longitude band 0.5 degree wide and the second two digits a latitude band 0.5 degree wide."@en ;skos:inScheme <https://linked.data.gov.au/def/geoadminfeatures> ;skos:broader geoad:MapSeries ;skos:notation "6948" ;skos:prefLabel "Mount Cuttiguree:6948"@en .
geoad:Monkira7048 a skos:Concept ;skos:definition "Map sheet for Monkira at 1:100 000 scale. The first two digits define a longitude band 0.5 degree wide and the second two digits a latitude band 0.5 degree wide."@en ;skos:inScheme <https://linked.data.gov.au/def/geoadminfeatures> ;skos:broader geoad:MapSeries ;skos:notation "7048" ;skos:prefLabel "Monkira:7048"@en .
geoad:Palparara7148 a skos:Concept ;skos:definition "Map sheet for Palparara at 1:100 000 scale. The first two digits define a longitude band 0.5 degree wide and the second two digits a latitude band 0.5 degree wide."@en ;skos:inScheme <https://linked.data.gov.au/def/geoadminfeatures> ;skos:broader geoad:MapSeries ;skos:notation "7148" ;skos:prefLabel "Palparara:7148"@en .
geoad:Cathua7248 a skos:Concept ;skos:definition "Map sheet for Cathua at 1:100 000 scale. The first two digits define a longitude band 0.5 degree wide and the second two digits a latitude band 0.5 degree wide."@en ;skos:inScheme <https://linked.data.gov.au/def/geoadminfeatures> ;skos:broader geoad:MapSeries ;skos:notation "7248" ;skos:prefLabel "Cathua:7248"@en .
geoad:Lochiel7348 a skos:Concept ;skos:definition "Map sheet for Lochiel at 1:100 000 scale. The first two digits define a longitude band 0.5 degree wide and the second two digits a latitude band 0.5 degree wide."@en ;skos:inScheme <https://linked.data.gov.au/def/geoadminfeatures> ;skos:broader geoad:MapSeries ;skos:notation "7348" ;skos:prefLabel "Lochiel:7348"@en .
geoad:Trewalla7448 a skos:Concept ;skos:definition "Map sheet for Trewalla at 1:100 000 scale. The first two digits define a longitude band 0.5 degree wide and the second two digits a latitude band 0.5 degree wide."@en ;skos:inScheme <https://linked.data.gov.au/def/geoadminfeatures> ;skos:broader geoad:MapSeries ;skos:notation "7448" ;skos:prefLabel "Trewalla:7448"@en .
geoad:Jundah7548 a skos:Concept ;skos:definition "Map sheet for Jundah at 1:100 000 scale. The first two digits define a longitude band 0.5 degree wide and the second two digits a latitude band 0.5 degree wide."@en ;skos:inScheme <https://linked.data.gov.au/def/geoadminfeatures> ;skos:broader geoad:MapSeries ;skos:notation "7548" ;skos:prefLabel "Jundah:7548"@en .
geoad:Arno7648 a skos:Concept ;skos:definition "Map sheet for Arno at 1:100 000 scale. The first two digits define a longitude band 0.5 degree wide and the second two digits a latitude band 0.5 degree wide."@en ;skos:inScheme <https://linked.data.gov.au/def/geoadminfeatures> ;skos:broader geoad:MapSeries ;skos:notation "7648" ;skos:prefLabel "Arno:7648"@en .
geoad:Yaraka7748 a skos:Concept ;skos:definition "Map sheet for Yaraka at 1:100 000 scale. The first two digits define a longitude band 0.5 degree wide and the second two digits a latitude band 0.5 degree wide."@en ;skos:inScheme <https://linked.data.gov.au/def/geoadminfeatures> ;skos:broader geoad:MapSeries ;skos:notation "7748" ;skos:prefLabel "Yaraka:7748"@en .
geoad:Mekaree7848 a skos:Concept ;skos:definition "Map sheet for Mekaree at 1:100 000 scale. The first two digits define a longitude band 0.5 degree wide and the second two digits a latitude band 0.5 degree wide."@en ;skos:inScheme <https://linked.data.gov.au/def/geoadminfeatures> ;skos:broader geoad:MapSeries ;skos:notation "7848" ;skos:prefLabel "Mekaree:7848"@en .
geoad:TerrickTerrick7948 a skos:Concept ;skos:definition "Map sheet for Terrick Terrick at 1:100 000 scale. The first two digits define a longitude band 0.5 degree wide and the second two digits a latitude band 0.5 degree wide."@en ;skos:inScheme <https://linked.data.gov.au/def/geoadminfeatures> ;skos:broader geoad:MapSeries ;skos:notation "7948" ;skos:prefLabel "Terrick Terrick:7948"@en .
geoad:NorthamptonDowns8048 a skos:Concept ;skos:definition "Map sheet for Northampton Downs at 1:100 000 scale. The first two digits define a longitude band 0.5 degree wide and the second two digits a latitude band 0.5 degree wide."@en ;skos:inScheme <https://linked.data.gov.au/def/geoadminfeatures> ;skos:broader geoad:MapSeries ;skos:notation "8048" ;skos:prefLabel "Northampton Downs:8048"@en .
geoad:Tambo8148 a skos:Concept ;skos:definition "Map sheet for Tambo at 1:100 000 scale. The first two digits define a longitude band 0.5 degree wide and the second two digits a latitude band 0.5 degree wide."@en ;skos:inScheme <https://linked.data.gov.au/def/geoadminfeatures> ;skos:broader geoad:MapSeries ;skos:notation "8148" ;skos:prefLabel "Tambo:8148"@en .
geoad:Carwell8248 a skos:Concept ;skos:definition "Map sheet for Carwell at 1:100 000 scale. The first two digits define a longitude band 0.5 degree wide and the second two digits a latitude band 0.5 degree wide."@en ;skos:inScheme <https://linked.data.gov.au/def/geoadminfeatures> ;skos:broader geoad:MapSeries ;skos:notation "8248" ;skos:prefLabel "Carwell:8248"@en .
geoad:Cungelella8348 a skos:Concept ;skos:definition "Map sheet for Cungelella at 1:100 000 scale. The first two digits define a longitude band 0.5 degree wide and the second two digits a latitude band 0.5 degree wide."@en ;skos:inScheme <https://linked.data.gov.au/def/geoadminfeatures> ;skos:broader geoad:MapSeries ;skos:notation "8348" ;skos:prefLabel "Cungelella:8348"@en .
geoad:Vandyke8448 a skos:Concept ;skos:definition "Map sheet for Vandyke at 1:100 000 scale. The first two digits define a longitude band 0.5 degree wide and the second two digits a latitude band 0.5 degree wide."@en ;skos:inScheme <https://linked.data.gov.au/def/geoadminfeatures> ;skos:broader geoad:MapSeries ;skos:notation "8448" ;skos:prefLabel "Vandyke:8448"@en .
geoad:Consuelo8548 a skos:Concept ;skos:definition "Map sheet for Consuelo at 1:100 000 scale. The first two digits define a longitude band 0.5 degree wide and the second two digits a latitude band 0.5 degree wide."@en ;skos:inScheme <https://linked.data.gov.au/def/geoadminfeatures> ;skos:broader geoad:MapSeries ;skos:notation "8548" ;skos:prefLabel "Consuelo:8548"@en .
geoad:Warrinilla8648 a skos:Concept ;skos:definition "Map sheet for Warrinilla at 1:100 000 scale. The first two digits define a longitude band 0.5 degree wide and the second two digits a latitude band 0.5 degree wide."@en ;skos:inScheme <https://linked.data.gov.au/def/geoadminfeatures> ;skos:broader geoad:MapSeries ;skos:notation "8648" ;skos:prefLabel "Warrinilla:8648"@en .
geoad:Bauhinia8748 a skos:Concept ;skos:definition "Map sheet for Bauhinia at 1:100 000 scale. The first two digits define a longitude band 0.5 degree wide and the second two digits a latitude band 0.5 degree wide."@en ;skos:inScheme <https://linked.data.gov.au/def/geoadminfeatures> ;skos:broader geoad:MapSeries ;skos:notation "8748" ;skos:prefLabel "Bauhinia:8748"@en .
geoad:Moura8848 a skos:Concept ;skos:definition "Map sheet for Moura at 1:100 000 scale. The first two digits define a longitude band 0.5 degree wide and the second two digits a latitude band 0.5 degree wide."@en ;skos:inScheme <https://linked.data.gov.au/def/geoadminfeatures> ;skos:broader geoad:MapSeries ;skos:notation "8848" ;skos:prefLabel "Moura:8848"@en .
geoad:Theodore8948 a skos:Concept ;skos:definition "Map sheet for Theodore at 1:100 000 scale. The first two digits define a longitude band 0.5 degree wide and the second two digits a latitude band 0.5 degree wide."@en ;skos:inScheme <https://linked.data.gov.au/def/geoadminfeatures> ;skos:broader geoad:MapSeries ;skos:notation "8948" ;skos:prefLabel "Theodore:8948"@en .
geoad:Scoria9048 a skos:Concept ;skos:definition "Map sheet for Scoria at 1:100 000 scale. The first two digits define a longitude band 0.5 degree wide and the second two digits a latitude band 0.5 degree wide."@en ;skos:inScheme <https://linked.data.gov.au/def/geoadminfeatures> ;skos:broader geoad:MapSeries ;skos:notation "9048" ;skos:prefLabel "Scoria:9048"@en .
geoad:Monto9148 a skos:Concept ;skos:definition "Map sheet for Monto at 1:100 000 scale. The first two digits define a longitude band 0.5 degree wide and the second two digits a latitude band 0.5 degree wide."@en ;skos:inScheme <https://linked.data.gov.au/def/geoadminfeatures> ;skos:broader geoad:MapSeries ;skos:notation "9148" ;skos:prefLabel "Monto:9148"@en .
geoad:Rosedale9248 a skos:Concept ;skos:definition "Map sheet for Rosedale at 1:100 000 scale. The first two digits define a longitude band 0.5 degree wide and the second two digits a latitude band 0.5 degree wide."@en ;skos:inScheme <https://linked.data.gov.au/def/geoadminfeatures> ;skos:broader geoad:MapSeries ;skos:notation "9248" ;skos:prefLabel "Rosedale:9248"@en .
geoad:Bundaberg9348 a skos:Concept ;skos:definition "Map sheet for Bundaberg at 1:100 000 scale. The first two digits define a longitude band 0.5 degree wide and the second two digits a latitude band 0.5 degree wide."@en ;skos:inScheme <https://linked.data.gov.au/def/geoadminfeatures> ;skos:broader geoad:MapSeries ;skos:notation "9348" ;skos:prefLabel "Bundaberg:9348"@en .
geoad:WaddyPoint9548 a skos:Concept ;skos:definition "Map sheet for Waddy Point at 1:100 000 scale. The first two digits define a longitude band 0.5 degree wide and the second two digits a latitude band 0.5 degree wide."@en ;skos:inScheme <https://linked.data.gov.au/def/geoadminfeatures> ;skos:broader geoad:MapSeries ;skos:notation "9548" ;skos:prefLabel "Waddy Point:9548"@en .
geoad:Yaluma6547 a skos:Concept ;skos:definition "Map sheet for Yaluma at 1:100 000 scale. The first two digits define a longitude band 0.5 degree wide and the second two digits a latitude band 0.5 degree wide."@en ;skos:inScheme <https://linked.data.gov.au/def/geoadminfeatures> ;skos:broader geoad:MapSeries ;skos:notation "6547" ;skos:prefLabel "Yaluma:6547"@en .
geoad:Muncoonie6647 a skos:Concept ;skos:definition "Map sheet for Muncoonie at 1:100 000 scale. The first two digits define a longitude band 0.5 degree wide and the second two digits a latitude band 0.5 degree wide."@en ;skos:inScheme <https://linked.data.gov.au/def/geoadminfeatures> ;skos:broader geoad:MapSeries ;skos:notation "6647" ;skos:prefLabel "Muncoonie:6647"@en .
geoad:Bygombo6747 a skos:Concept ;skos:definition "Map sheet for Bygombo at 1:100 000 scale. The first two digits define a longitude band 0.5 degree wide and the second two digits a latitude band 0.5 degree wide."@en ;skos:inScheme <https://linked.data.gov.au/def/geoadminfeatures> ;skos:broader geoad:MapSeries ;skos:notation "6747" ;skos:prefLabel "Bygombo:6747"@en .
geoad:Bilpamorea6847 a skos:Concept ;skos:definition "Map sheet for Bilpamorea at 1:100 000 scale. The first two digits define a longitude band 0.5 degree wide and the second two digits a latitude band 0.5 degree wide."@en ;skos:inScheme <https://linked.data.gov.au/def/geoadminfeatures> ;skos:broader geoad:MapSeries ;skos:notation "6847" ;skos:prefLabel "Bilpamorea:6847"@en .
geoad:Wantata6947 a skos:Concept ;skos:definition "Map sheet for Wantata at 1:100 000 scale. The first two digits define a longitude band 0.5 degree wide and the second two digits a latitude band 0.5 degree wide."@en ;skos:inScheme <https://linked.data.gov.au/def/geoadminfeatures> ;skos:broader geoad:MapSeries ;skos:notation "6947" ;skos:prefLabel "Wantata:6947"@en .
geoad:Mooraberree7047 a skos:Concept ;skos:definition "Map sheet for Mooraberree at 1:100 000 scale. The first two digits define a longitude band 0.5 degree wide and the second two digits a latitude band 0.5 degree wide."@en ;skos:inScheme <https://linked.data.gov.au/def/geoadminfeatures> ;skos:broader geoad:MapSeries ;skos:notation "7047" ;skos:prefLabel "Mooraberree:7047"@en .
geoad:Currawilla7147 a skos:Concept ;skos:definition "Map sheet for Currawilla at 1:100 000 scale. The first two digits define a longitude band 0.5 degree wide and the second two digits a latitude band 0.5 degree wide."@en ;skos:inScheme <https://linked.data.gov.au/def/geoadminfeatures> ;skos:broader geoad:MapSeries ;skos:notation "7147" ;skos:prefLabel "Currawilla:7147"@en .
geoad:Canterbury7247 a skos:Concept ;skos:definition "Map sheet for Canterbury at 1:100 000 scale. The first two digits define a longitude band 0.5 degree wide and the second two digits a latitude band 0.5 degree wide."@en ;skos:inScheme <https://linked.data.gov.au/def/geoadminfeatures> ;skos:broader geoad:MapSeries ;skos:notation "7247" ;skos:prefLabel "Canterbury:7247"@en .
geoad:Whitula7347 a skos:Concept ;skos:definition "Map sheet for Whitula at 1:100 000 scale. The first two digits define a longitude band 0.5 degree wide and the second two digits a latitude band 0.5 degree wide."@en ;skos:inScheme <https://linked.data.gov.au/def/geoadminfeatures> ;skos:broader geoad:MapSeries ;skos:notation "7347" ;skos:prefLabel "Whitula:7347"@en .
geoad:Windorah7447 a skos:Concept ;skos:definition "Map sheet for Windorah at 1:100 000 scale. The first two digits define a longitude band 0.5 degree wide and the second two digits a latitude band 0.5 degree wide."@en ;skos:inScheme <https://linked.data.gov.au/def/geoadminfeatures> ;skos:broader geoad:MapSeries ;skos:notation "7447" ;skos:prefLabel "Windorah:7447"@en .
geoad:Retreat7547 a skos:Concept ;skos:definition "Map sheet for Retreat at 1:100 000 scale. The first two digits define a longitude band 0.5 degree wide and the second two digits a latitude band 0.5 degree wide."@en ;skos:inScheme <https://linked.data.gov.au/def/geoadminfeatures> ;skos:broader geoad:MapSeries ;skos:notation "7547" ;skos:prefLabel "Retreat:7547"@en .
geoad:Budgerygar7647 a skos:Concept ;skos:definition "Map sheet for Budgerygar at 1:100 000 scale. The first two digits define a longitude band 0.5 degree wide and the second two digits a latitude band 0.5 degree wide."@en ;skos:inScheme <https://linked.data.gov.au/def/geoadminfeatures> ;skos:broader geoad:MapSeries ;skos:notation "7647" ;skos:prefLabel "Budgerygar:7647"@en .
geoad:Glenara7747 a skos:Concept ;skos:definition "Map sheet for Glenara at 1:100 000 scale. The first two digits define a longitude band 0.5 degree wide and the second two digits a latitude band 0.5 degree wide."@en ;skos:inScheme <https://linked.data.gov.au/def/geoadminfeatures> ;skos:broader geoad:MapSeries ;skos:notation "7747" ;skos:prefLabel "Glenara:7747"@en .
geoad:Collabara7847 a skos:Concept ;skos:definition "Map sheet for Collabara at 1:100 000 scale. The first two digits define a longitude band 0.5 degree wide and the second two digits a latitude band 0.5 degree wide."@en ;skos:inScheme <https://linked.data.gov.au/def/geoadminfeatures> ;skos:broader geoad:MapSeries ;skos:notation "7847" ;skos:prefLabel "Collabara:7847"@en .
geoad:ListowelDowns7947 a skos:Concept ;skos:definition "Map sheet for Listowel Downs at 1:100 000 scale. The first two digits define a longitude band 0.5 degree wide and the second two digits a latitude band 0.5 degree wide."@en ;skos:inScheme <https://linked.data.gov.au/def/geoadminfeatures> ;skos:broader geoad:MapSeries ;skos:notation "7947" ;skos:prefLabel "Listowel Downs:7947"@en .
geoad:Glanworth8047 a skos:Concept ;skos:definition "Map sheet for Glanworth at 1:100 000 scale. The first two digits define a longitude band 0.5 degree wide and the second two digits a latitude band 0.5 degree wide."@en ;skos:inScheme <https://linked.data.gov.au/def/geoadminfeatures> ;skos:broader geoad:MapSeries ;skos:notation "8047" ;skos:prefLabel "Glanworth:8047"@en .
geoad:Lansdowne8147 a skos:Concept ;skos:definition "Map sheet for Lansdowne at 1:100 000 scale. The first two digits define a longitude band 0.5 degree wide and the second two digits a latitude band 0.5 degree wide."@en ;skos:inScheme <https://linked.data.gov.au/def/geoadminfeatures> ;skos:broader geoad:MapSeries ;skos:notation "8147" ;skos:prefLabel "Lansdowne:8147"@en .
geoad:Caldervale8247 a skos:Concept ;skos:definition "Map sheet for Caldervale at 1:100 000 scale. The first two digits define a longitude band 0.5 degree wide and the second two digits a latitude band 0.5 degree wide."@en ;skos:inScheme <https://linked.data.gov.au/def/geoadminfeatures> ;skos:broader geoad:MapSeries ;skos:notation "8247" ;skos:prefLabel "Caldervale:8247"@en .
geoad:Chesterton8347 a skos:Concept ;skos:definition "Map sheet for Chesterton at 1:100 000 scale. The first two digits define a longitude band 0.5 degree wide and the second two digits a latitude band 0.5 degree wide."@en ;skos:inScheme <https://linked.data.gov.au/def/geoadminfeatures> ;skos:broader geoad:MapSeries ;skos:notation "8347" ;skos:prefLabel "Chesterton:8347"@en .
geoad:Warrong8447 a skos:Concept ;skos:definition "Map sheet for Warrong at 1:100 000 scale. The first two digits define a longitude band 0.5 degree wide and the second two digits a latitude band 0.5 degree wide."@en ;skos:inScheme <https://linked.data.gov.au/def/geoadminfeatures> ;skos:broader geoad:MapSeries ;skos:notation "8447" ;skos:prefLabel "Warrong:8447"@en .
geoad:MountHowe8547 a skos:Concept ;skos:definition "Map sheet for Mount Howe at 1:100 000 scale. The first two digits define a longitude band 0.5 degree wide and the second two digits a latitude band 0.5 degree wide."@en ;skos:inScheme <https://linked.data.gov.au/def/geoadminfeatures> ;skos:broader geoad:MapSeries ;skos:notation "8547" ;skos:prefLabel "Mount Howe:8547"@en .
geoad:Arcadia8647 a skos:Concept ;skos:definition "Map sheet for Arcadia at 1:100 000 scale. The first two digits define a longitude band 0.5 degree wide and the second two digits a latitude band 0.5 degree wide."@en ;skos:inScheme <https://linked.data.gov.au/def/geoadminfeatures> ;skos:broader geoad:MapSeries ;skos:notation "8647" ;skos:prefLabel "Arcadia:8647"@en .
geoad:Glenhaughton8747 a skos:Concept ;skos:definition "Map sheet for Glenhaughton at 1:100 000 scale. The first two digits define a longitude band 0.5 degree wide and the second two digits a latitude band 0.5 degree wide."@en ;skos:inScheme <https://linked.data.gov.au/def/geoadminfeatures> ;skos:broader geoad:MapSeries ;skos:notation "8747" ;skos:prefLabel "Glenhaughton:8747"@en .
geoad:Ghinghinda8847 a skos:Concept ;skos:definition "Map sheet for Ghinghinda at 1:100 000 scale. The first two digits define a longitude band 0.5 degree wide and the second two digits a latitude band 0.5 degree wide."@en ;skos:inScheme <https://linked.data.gov.au/def/geoadminfeatures> ;skos:broader geoad:MapSeries ;skos:notation "8847" ;skos:prefLabel "Ghinghinda:8847"@en .
geoad:Cracow8947 a skos:Concept ;skos:definition "Map sheet for Cracow at 1:100 000 scale. The first two digits define a longitude band 0.5 degree wide and the second two digits a latitude band 0.5 degree wide."@en ;skos:inScheme <https://linked.data.gov.au/def/geoadminfeatures> ;skos:broader geoad:MapSeries ;skos:notation "8947" ;skos:prefLabel "Cracow:8947"@en .
geoad:Rawbelle9047 a skos:Concept ;skos:definition "Map sheet for Rawbelle at 1:100 000 scale. The first two digits define a longitude band 0.5 degree wide and the second two digits a latitude band 0.5 degree wide."@en ;skos:inScheme <https://linked.data.gov.au/def/geoadminfeatures> ;skos:broader geoad:MapSeries ;skos:notation "9047" ;skos:prefLabel "Rawbelle:9047"@en .
geoad:Eidsvold9147 a skos:Concept ;skos:definition "Map sheet for Eidsvold at 1:100 000 scale. The first two digits define a longitude band 0.5 degree wide and the second two digits a latitude band 0.5 degree wide."@en ;skos:inScheme <https://linked.data.gov.au/def/geoadminfeatures> ;skos:broader geoad:MapSeries ;skos:notation "9147" ;skos:prefLabel "Eidsvold:9147"@en .
geoad:MountPerry9247 a skos:Concept ;skos:definition "Map sheet for Mount Perry at 1:100 000 scale. The first two digits define a longitude band 0.5 degree wide and the second two digits a latitude band 0.5 degree wide."@en ;skos:inScheme <https://linked.data.gov.au/def/geoadminfeatures> ;skos:broader geoad:MapSeries ;skos:notation "9247" ;skos:prefLabel "Mount Perry:9247"@en .
geoad:Childers9347 a skos:Concept ;skos:definition "Map sheet for Childers at 1:100 000 scale. The first two digits define a longitude band 0.5 degree wide and the second two digits a latitude band 0.5 degree wide."@en ;skos:inScheme <https://linked.data.gov.au/def/geoadminfeatures> ;skos:broader geoad:MapSeries ;skos:notation "9347" ;skos:prefLabel "Childers:9347"@en .
geoad:Pialba9447 a skos:Concept ;skos:definition "Map sheet for Pialba at 1:100 000 scale. The first two digits define a longitude band 0.5 degree wide and the second two digits a latitude band 0.5 degree wide."@en ;skos:inScheme <https://linked.data.gov.au/def/geoadminfeatures> ;skos:broader geoad:MapSeries ;skos:notation "9447" ;skos:prefLabel "Pialba:9447"@en .
geoad:HappyValley9547 a skos:Concept ;skos:definition "Map sheet for Happy Valley at 1:100 000 scale. The first two digits define a longitude band 0.5 degree wide and the second two digits a latitude band 0.5 degree wide."@en ;skos:inScheme <https://linked.data.gov.au/def/geoadminfeatures> ;skos:broader geoad:MapSeries ;skos:notation "9547" ;skos:prefLabel "Happy Valley:9547"@en .
geoad:PoeppelCorner6546 a skos:Concept ;skos:definition "Map sheet for Poeppel Corner at 1:100 000 scale. The first two digits define a longitude band 0.5 degree wide and the second two digits a latitude band 0.5 degree wide."@en ;skos:inScheme <https://linked.data.gov.au/def/geoadminfeatures> ;skos:broader geoad:MapSeries ;skos:notation "6546" ;skos:prefLabel "Poeppel Corner:6546"@en .
geoad:Goonamillera6646 a skos:Concept ;skos:definition "Map sheet for Goonamillera at 1:100 000 scale. The first two digits define a longitude band 0.5 degree wide and the second two digits a latitude band 0.5 degree wide."@en ;skos:inScheme <https://linked.data.gov.au/def/geoadminfeatures> ;skos:broader geoad:MapSeries ;skos:notation "6646" ;skos:prefLabel "Goonamillera:6646"@en .
geoad:Birdsville6746 a skos:Concept ;skos:definition "Map sheet for Birdsville at 1:100 000 scale. The first two digits define a longitude band 0.5 degree wide and the second two digits a latitude band 0.5 degree wide."@en ;skos:inScheme <https://linked.data.gov.au/def/geoadminfeatures> ;skos:broader geoad:MapSeries ;skos:notation "6746" ;skos:prefLabel "Birdsville:6746"@en .
geoad:Roseberth6846 a skos:Concept ;skos:definition "Map sheet for Roseberth at 1:100 000 scale. The first two digits define a longitude band 0.5 degree wide and the second two digits a latitude band 0.5 degree wide."@en ;skos:inScheme <https://linked.data.gov.au/def/geoadminfeatures> ;skos:broader geoad:MapSeries ;skos:notation "6846" ;skos:prefLabel "Roseberth:6846"@en .
geoad:Durrie6946 a skos:Concept ;skos:definition "Map sheet for Durrie at 1:100 000 scale. The first two digits define a longitude band 0.5 degree wide and the second two digits a latitude band 0.5 degree wide."@en ;skos:inScheme <https://linked.data.gov.au/def/geoadminfeatures> ;skos:broader geoad:MapSeries ;skos:notation "6946" ;skos:prefLabel "Durrie:6946"@en .
geoad:Betoota7046 a skos:Concept ;skos:definition "Map sheet for Betoota at 1:100 000 scale. The first two digits define a longitude band 0.5 degree wide and the second two digits a latitude band 0.5 degree wide."@en ;skos:inScheme <https://linked.data.gov.au/def/geoadminfeatures> ;skos:broader geoad:MapSeries ;skos:notation "7046" ;skos:prefLabel "Betoota:7046"@en .
geoad:HaddonCorner7146 a skos:Concept ;skos:definition "Map sheet for Haddon Corner at 1:100 000 scale. The first two digits define a longitude band 0.5 degree wide and the second two digits a latitude band 0.5 degree wide."@en ;skos:inScheme <https://linked.data.gov.au/def/geoadminfeatures> ;skos:broader geoad:MapSeries ;skos:notation "7146" ;skos:prefLabel "Haddon Corner:7146"@en .
geoad:Tanbar7246 a skos:Concept ;skos:definition "Map sheet for Tanbar at 1:100 000 scale. The first two digits define a longitude band 0.5 degree wide and the second two digits a latitude band 0.5 degree wide."@en ;skos:inScheme <https://linked.data.gov.au/def/geoadminfeatures> ;skos:broader geoad:MapSeries ;skos:notation "7246" ;skos:prefLabel "Tanbar:7246"@en .
geoad:SouthGalway7346 a skos:Concept ;skos:definition "Map sheet for South Galway at 1:100 000 scale. The first two digits define a longitude band 0.5 degree wide and the second two digits a latitude band 0.5 degree wide."@en ;skos:inScheme <https://linked.data.gov.au/def/geoadminfeatures> ;skos:broader geoad:MapSeries ;skos:notation "7346" ;skos:prefLabel "South Galway:7346"@en .
geoad:Keeroongooloo7446 a skos:Concept ;skos:definition "Map sheet for Keeroongooloo at 1:100 000 scale. The first two digits define a longitude band 0.5 degree wide and the second two digits a latitude band 0.5 degree wide."@en ;skos:inScheme <https://linked.data.gov.au/def/geoadminfeatures> ;skos:broader geoad:MapSeries ;skos:notation "7446" ;skos:prefLabel "Keeroongooloo:7446"@en .
geoad:Springfield7546 a skos:Concept ;skos:definition "Map sheet for Springfield at 1:100 000 scale. The first two digits define a longitude band 0.5 degree wide and the second two digits a latitude band 0.5 degree wide."@en ;skos:inScheme <https://linked.data.gov.au/def/geoadminfeatures> ;skos:broader geoad:MapSeries ;skos:notation "7546" ;skos:prefLabel "Springfield:7546"@en .
geoad:Bulgroo7646 a skos:Concept ;skos:definition "Map sheet for Bulgroo at 1:100 000 scale. The first two digits define a longitude band 0.5 degree wide and the second two digits a latitude band 0.5 degree wide."@en ;skos:inScheme <https://linked.data.gov.au/def/geoadminfeatures> ;skos:broader geoad:MapSeries ;skos:notation "7646" ;skos:prefLabel "Bulgroo:7646"@en .
geoad:Milo7746 a skos:Concept ;skos:definition "Map sheet for Milo at 1:100 000 scale. The first two digits define a longitude band 0.5 degree wide and the second two digits a latitude band 0.5 degree wide."@en ;skos:inScheme <https://linked.data.gov.au/def/geoadminfeatures> ;skos:broader geoad:MapSeries ;skos:notation "7746" ;skos:prefLabel "Milo:7746"@en .
geoad:Adavale7846 a skos:Concept ;skos:definition "Map sheet for Adavale at 1:100 000 scale. The first two digits define a longitude band 0.5 degree wide and the second two digits a latitude band 0.5 degree wide."@en ;skos:inScheme <https://linked.data.gov.au/def/geoadminfeatures> ;skos:broader geoad:MapSeries ;skos:notation "7846" ;skos:prefLabel "Adavale:7846"@en .
geoad:Ambathala7946 a skos:Concept ;skos:definition "Map sheet for Ambathala at 1:100 000 scale. The first two digits define a longitude band 0.5 degree wide and the second two digits a latitude band 0.5 degree wide."@en ;skos:inScheme <https://linked.data.gov.au/def/geoadminfeatures> ;skos:broader geoad:MapSeries ;skos:notation "7946" ;skos:prefLabel "Ambathala:7946"@en .
geoad:MountMorris8046 a skos:Concept ;skos:definition "Map sheet for Mount Morris at 1:100 000 scale. The first two digits define a longitude band 0.5 degree wide and the second two digits a latitude band 0.5 degree wide."@en ;skos:inScheme <https://linked.data.gov.au/def/geoadminfeatures> ;skos:broader geoad:MapSeries ;skos:notation "8046" ;skos:prefLabel "Mount Morris:8046"@en .
geoad:Oakwood8146 a skos:Concept ;skos:definition "Map sheet for Oakwood at 1:100 000 scale. The first two digits define a longitude band 0.5 degree wide and the second two digits a latitude band 0.5 degree wide."@en ;skos:inScheme <https://linked.data.gov.au/def/geoadminfeatures> ;skos:broader geoad:MapSeries ;skos:notation "8146" ;skos:prefLabel "Oakwood:8146"@en .
geoad:Augathella8246 a skos:Concept ;skos:definition "Map sheet for Augathella at 1:100 000 scale. The first two digits define a longitude band 0.5 degree wide and the second two digits a latitude band 0.5 degree wide."@en ;skos:inScheme <https://linked.data.gov.au/def/geoadminfeatures> ;skos:broader geoad:MapSeries ;skos:notation "8246" ;skos:prefLabel "Augathella:8246"@en .
geoad:Hoganthulla8346 a skos:Concept ;skos:definition "Map sheet for Hoganthulla at 1:100 000 scale. The first two digits define a longitude band 0.5 degree wide and the second two digits a latitude band 0.5 degree wide."@en ;skos:inScheme <https://linked.data.gov.au/def/geoadminfeatures> ;skos:broader geoad:MapSeries ;skos:notation "8346" ;skos:prefLabel "Hoganthulla:8346"@en .
geoad:ForestVale8446 a skos:Concept ;skos:definition "Map sheet for Forest Vale at 1:100 000 scale. The first two digits define a longitude band 0.5 degree wide and the second two digits a latitude band 0.5 degree wide."@en ;skos:inScheme <https://linked.data.gov.au/def/geoadminfeatures> ;skos:broader geoad:MapSeries ;skos:notation "8446" ;skos:prefLabel "Forest Vale:8446"@en .
geoad:Womblebank8546 a skos:Concept ;skos:definition "Map sheet for Womblebank at 1:100 000 scale. The first two digits define a longitude band 0.5 degree wide and the second two digits a latitude band 0.5 degree wide."@en ;skos:inScheme <https://linked.data.gov.au/def/geoadminfeatures> ;skos:broader geoad:MapSeries ;skos:notation "8546" ;skos:prefLabel "Womblebank:8546"@en .
geoad:Injune8646 a skos:Concept ;skos:definition "Map sheet for Injune at 1:100 000 scale. The first two digits define a longitude band 0.5 degree wide and the second two digits a latitude band 0.5 degree wide."@en ;skos:inScheme <https://linked.data.gov.au/def/geoadminfeatures> ;skos:broader geoad:MapSeries ;skos:notation "8646" ;skos:prefLabel "Injune:8646"@en .
geoad:HornetBank8746 a skos:Concept ;skos:definition "Map sheet for Hornet Bank at 1:100 000 scale. The first two digits define a longitude band 0.5 degree wide and the second two digits a latitude band 0.5 degree wide."@en ;skos:inScheme <https://linked.data.gov.au/def/geoadminfeatures> ;skos:broader geoad:MapSeries ;skos:notation "8746" ;skos:prefLabel "Hornet Bank:8746"@en .
geoad:Taroom8846 a skos:Concept ;skos:definition "Map sheet for Taroom at 1:100 000 scale. The first two digits define a longitude band 0.5 degree wide and the second two digits a latitude band 0.5 degree wide."@en ;skos:inScheme <https://linked.data.gov.au/def/geoadminfeatures> ;skos:broader geoad:MapSeries ;skos:notation "8846" ;skos:prefLabel "Taroom:8846"@en .
geoad:Bungaban8946 a skos:Concept ;skos:definition "Map sheet for Bungaban at 1:100 000 scale. The first two digits define a longitude band 0.5 degree wide and the second two digits a latitude band 0.5 degree wide."@en ;skos:inScheme <https://linked.data.gov.au/def/geoadminfeatures> ;skos:broader geoad:MapSeries ;skos:notation "8946" ;skos:prefLabel "Bungaban:8946"@en .
geoad:Auburn9046 a skos:Concept ;skos:definition "Map sheet for Auburn at 1:100 000 scale. The first two digits define a longitude band 0.5 degree wide and the second two digits a latitude band 0.5 degree wide."@en ;skos:inScheme <https://linked.data.gov.au/def/geoadminfeatures> ;skos:broader geoad:MapSeries ;skos:notation "9046" ;skos:prefLabel "Auburn:9046"@en .
geoad:Mundubbera9146 a skos:Concept ;skos:definition "Map sheet for Mundubbera at 1:100 000 scale. The first two digits define a longitude band 0.5 degree wide and the second two digits a latitude band 0.5 degree wide."@en ;skos:inScheme <https://linked.data.gov.au/def/geoadminfeatures> ;skos:broader geoad:MapSeries ;skos:notation "9146" ;skos:prefLabel "Mundubbera:9146"@en .
geoad:Gayndah9246 a skos:Concept ;skos:definition "Map sheet for Gayndah at 1:100 000 scale. The first two digits define a longitude band 0.5 degree wide and the second two digits a latitude band 0.5 degree wide."@en ;skos:inScheme <https://linked.data.gov.au/def/geoadminfeatures> ;skos:broader geoad:MapSeries ;skos:notation "9246" ;skos:prefLabel "Gayndah:9246"@en .
geoad:Biggenden9346 a skos:Concept ;skos:definition "Map sheet for Biggenden at 1:100 000 scale. The first two digits define a longitude band 0.5 degree wide and the second two digits a latitude band 0.5 degree wide."@en ;skos:inScheme <https://linked.data.gov.au/def/geoadminfeatures> ;skos:broader geoad:MapSeries ;skos:notation "9346" ;skos:prefLabel "Biggenden:9346"@en .
geoad:Maryborough9446 a skos:Concept ;skos:definition "Map sheet for Maryborough at 1:100 000 scale. The first two digits define a longitude band 0.5 degree wide and the second two digits a latitude band 0.5 degree wide."@en ;skos:inScheme <https://linked.data.gov.au/def/geoadminfeatures> ;skos:broader geoad:MapSeries ;skos:notation "9446" ;skos:prefLabel "Maryborough:9446"@en .
geoad:WideBay9546 a skos:Concept ;skos:definition "Map sheet for Wide Bay at 1:100 000 scale. The first two digits define a longitude band 0.5 degree wide and the second two digits a latitude band 0.5 degree wide."@en ;skos:inScheme <https://linked.data.gov.au/def/geoadminfeatures> ;skos:broader geoad:MapSeries ;skos:notation "9546" ;skos:prefLabel "Wide Bay:9546"@en .
geoad:LakePoeppel6545 a skos:Concept ;skos:definition "Map sheet for Lake Poeppel at 1:100 000 scale. The first two digits define a longitude band 0.5 degree wide and the second two digits a latitude band 0.5 degree wide."@en ;skos:inScheme <https://linked.data.gov.au/def/geoadminfeatures> ;skos:broader geoad:MapSeries ;skos:notation "6545" ;skos:prefLabel "Lake Poeppel:6545"@en .
geoad:AltonDowns6645 a skos:Concept ;skos:definition "Map sheet for Alton Downs at 1:100 000 scale. The first two digits define a longitude band 0.5 degree wide and the second two digits a latitude band 0.5 degree wide."@en ;skos:inScheme <https://linked.data.gov.au/def/geoadminfeatures> ;skos:broader geoad:MapSeries ;skos:notation "6645" ;skos:prefLabel "Alton Downs:6645"@en .
geoad:PandiePandie6745 a skos:Concept ;skos:definition "Map sheet for Pandie Pandie at 1:100 000 scale. The first two digits define a longitude band 0.5 degree wide and the second two digits a latitude band 0.5 degree wide."@en ;skos:inScheme <https://linked.data.gov.au/def/geoadminfeatures> ;skos:broader geoad:MapSeries ;skos:notation "6745" ;skos:prefLabel "Pandie Pandie:6745"@en .
geoad:Etamunbanie6845 a skos:Concept ;skos:definition "Map sheet for Etamunbanie at 1:100 000 scale. The first two digits define a longitude band 0.5 degree wide and the second two digits a latitude band 0.5 degree wide."@en ;skos:inScheme <https://linked.data.gov.au/def/geoadminfeatures> ;skos:broader geoad:MapSeries ;skos:notation "6845" ;skos:prefLabel "Etamunbanie:6845"@en .
geoad:Cadelga6945 a skos:Concept ;skos:definition "Map sheet for Cadelga at 1:100 000 scale. The first two digits define a longitude band 0.5 degree wide and the second two digits a latitude band 0.5 degree wide."@en ;skos:inScheme <https://linked.data.gov.au/def/geoadminfeatures> ;skos:broader geoad:MapSeries ;skos:notation "6945" ;skos:prefLabel "Cadelga:6945"@en .
geoad:Haddon7045 a skos:Concept ;skos:definition "Map sheet for Haddon at 1:100 000 scale. The first two digits define a longitude band 0.5 degree wide and the second two digits a latitude band 0.5 degree wide."@en ;skos:inScheme <https://linked.data.gov.au/def/geoadminfeatures> ;skos:broader geoad:MapSeries ;skos:notation "7045" ;skos:prefLabel "Haddon:7045"@en .
geoad:LakeYammaYamma7145 a skos:Concept ;skos:definition "Map sheet for Lake Yamma Yamma at 1:100 000 scale. The first two digits define a longitude band 0.5 degree wide and the second two digits a latitude band 0.5 degree wide."@en ;skos:inScheme <https://linked.data.gov.au/def/geoadminfeatures> ;skos:broader geoad:MapSeries ;skos:notation "7145" ;skos:prefLabel "Lake Yamma Yamma:7145"@en .
geoad:Barrolka7245 a skos:Concept ;skos:definition "Map sheet for Barrolka at 1:100 000 scale. The first two digits define a longitude band 0.5 degree wide and the second two digits a latitude band 0.5 degree wide."@en ;skos:inScheme <https://linked.data.gov.au/def/geoadminfeatures> ;skos:broader geoad:MapSeries ;skos:notation "7245" ;skos:prefLabel "Barrolka:7245"@en .
geoad:Malagarga7345 a skos:Concept ;skos:definition "Map sheet for Malagarga at 1:100 000 scale. The first two digits define a longitude band 0.5 degree wide and the second two digits a latitude band 0.5 degree wide."@en ;skos:inScheme <https://linked.data.gov.au/def/geoadminfeatures> ;skos:broader geoad:MapSeries ;skos:notation "7345" ;skos:prefLabel "Malagarga:7345"@en .
geoad:MountRouse7445 a skos:Concept ;skos:definition "Map sheet for Mount Rouse at 1:100 000 scale. The first two digits define a longitude band 0.5 degree wide and the second two digits a latitude band 0.5 degree wide."@en ;skos:inScheme <https://linked.data.gov.au/def/geoadminfeatures> ;skos:broader geoad:MapSeries ;skos:notation "7445" ;skos:prefLabel "Mount Rouse:7445"@en .
geoad:Thylungra7545 a skos:Concept ;skos:definition "Map sheet for Thylungra at 1:100 000 scale. The first two digits define a longitude band 0.5 degree wide and the second two digits a latitude band 0.5 degree wide."@en ;skos:inScheme <https://linked.data.gov.au/def/geoadminfeatures> ;skos:broader geoad:MapSeries ;skos:notation "7545" ;skos:prefLabel "Thylungra:7545"@en .
geoad:Ray7645 a skos:Concept ;skos:definition "Map sheet for Ray at 1:100 000 scale. The first two digits define a longitude band 0.5 degree wide and the second two digits a latitude band 0.5 degree wide."@en ;skos:inScheme <https://linked.data.gov.au/def/geoadminfeatures> ;skos:broader geoad:MapSeries ;skos:notation "7645" ;skos:prefLabel "Ray:7645"@en .
geoad:Nickavilla7745 a skos:Concept ;skos:definition "Map sheet for Nickavilla at 1:100 000 scale. The first two digits define a longitude band 0.5 degree wide and the second two digits a latitude band 0.5 degree wide."@en ;skos:inScheme <https://linked.data.gov.au/def/geoadminfeatures> ;skos:broader geoad:MapSeries ;skos:notation "7745" ;skos:prefLabel "Nickavilla:7745"@en .
geoad:Gumbardo7845 a skos:Concept ;skos:definition "Map sheet for Gumbardo at 1:100 000 scale. The first two digits define a longitude band 0.5 degree wide and the second two digits a latitude band 0.5 degree wide."@en ;skos:inScheme <https://linked.data.gov.au/def/geoadminfeatures> ;skos:broader geoad:MapSeries ;skos:notation "7845" ;skos:prefLabel "Gumbardo:7845"@en .
geoad:LakeDartmouth7945 a skos:Concept ;skos:definition "Map sheet for Lake Dartmouth at 1:100 000 scale. The first two digits define a longitude band 0.5 degree wide and the second two digits a latitude band 0.5 degree wide."@en ;skos:inScheme <https://linked.data.gov.au/def/geoadminfeatures> ;skos:broader geoad:MapSeries ;skos:notation "7945" ;skos:prefLabel "Lake Dartmouth:7945"@en .
geoad:LangloCrossing8045 a skos:Concept ;skos:definition "Map sheet for Langlo Crossing at 1:100 000 scale. The first two digits define a longitude band 0.5 degree wide and the second two digits a latitude band 0.5 degree wide."@en ;skos:inScheme <https://linked.data.gov.au/def/geoadminfeatures> ;skos:broader geoad:MapSeries ;skos:notation "8045" ;skos:prefLabel "Langlo Crossing:8045"@en .
geoad:Charleville8145 a skos:Concept ;skos:definition "Map sheet for Charleville at 1:100 000 scale. The first two digits define a longitude band 0.5 degree wide and the second two digits a latitude band 0.5 degree wide."@en ;skos:inScheme <https://linked.data.gov.au/def/geoadminfeatures> ;skos:broader geoad:MapSeries ;skos:notation "8145" ;skos:prefLabel "Charleville:8145"@en .
geoad:Angellala8245 a skos:Concept ;skos:definition "Map sheet for Angellala at 1:100 000 scale. The first two digits define a longitude band 0.5 degree wide and the second two digits a latitude band 0.5 degree wide."@en ;skos:inScheme <https://linked.data.gov.au/def/geoadminfeatures> ;skos:broader geoad:MapSeries ;skos:notation "8245" ;skos:prefLabel "Angellala:8245"@en .
geoad:Morven8345 a skos:Concept ;skos:definition "Map sheet for Morven at 1:100 000 scale. The first two digits define a longitude band 0.5 degree wide and the second two digits a latitude band 0.5 degree wide."@en ;skos:inScheme <https://linked.data.gov.au/def/geoadminfeatures> ;skos:broader geoad:MapSeries ;skos:notation "8345" ;skos:prefLabel "Morven:8345"@en .
geoad:Mitchell8445 a skos:Concept ;skos:definition "Map sheet for Mitchell at 1:100 000 scale. The first two digits define a longitude band 0.5 degree wide and the second two digits a latitude band 0.5 degree wide."@en ;skos:inScheme <https://linked.data.gov.au/def/geoadminfeatures> ;skos:broader geoad:MapSeries ;skos:notation "8445" ;skos:prefLabel "Mitchell:8445"@en .
geoad:Waroonga8545 a skos:Concept ;skos:definition "Map sheet for Waroonga at 1:100 000 scale. The first two digits define a longitude band 0.5 degree wide and the second two digits a latitude band 0.5 degree wide."@en ;skos:inScheme <https://linked.data.gov.au/def/geoadminfeatures> ;skos:broader geoad:MapSeries ;skos:notation "8545" ;skos:prefLabel "Waroonga:8545"@en .
geoad:Orallo8645 a skos:Concept ;skos:definition "Map sheet for Orallo at 1:100 000 scale. The first two digits define a longitude band 0.5 degree wide and the second two digits a latitude band 0.5 degree wide."@en ;skos:inScheme <https://linked.data.gov.au/def/geoadminfeatures> ;skos:broader geoad:MapSeries ;skos:notation "8645" ;skos:prefLabel "Orallo:8645"@en .
geoad:Muggleton8745 a skos:Concept ;skos:definition "Map sheet for Muggleton at 1:100 000 scale. The first two digits define a longitude band 0.5 degree wide and the second two digits a latitude band 0.5 degree wide."@en ;skos:inScheme <https://linked.data.gov.au/def/geoadminfeatures> ;skos:broader geoad:MapSeries ;skos:notation "8745" ;skos:prefLabel "Muggleton:8745"@en .
geoad:Wandoan8845 a skos:Concept ;skos:definition "Map sheet for Wandoan at 1:100 000 scale. The first two digits define a longitude band 0.5 degree wide and the second two digits a latitude band 0.5 degree wide."@en ;skos:inScheme <https://linked.data.gov.au/def/geoadminfeatures> ;skos:broader geoad:MapSeries ;skos:notation "8845" ;skos:prefLabel "Wandoan:8845"@en .
geoad:Guluguba8945 a skos:Concept ;skos:definition "Map sheet for Guluguba at 1:100 000 scale. The first two digits define a longitude band 0.5 degree wide and the second two digits a latitude band 0.5 degree wide."@en ;skos:inScheme <https://linked.data.gov.au/def/geoadminfeatures> ;skos:broader geoad:MapSeries ;skos:notation "8945" ;skos:prefLabel "Guluguba:8945"@en .
geoad:Barakula9045 a skos:Concept ;skos:definition "Map sheet for Barakula at 1:100 000 scale. The first two digits define a longitude band 0.5 degree wide and the second two digits a latitude band 0.5 degree wide."@en ;skos:inScheme <https://linked.data.gov.au/def/geoadminfeatures> ;skos:broader geoad:MapSeries ;skos:notation "9045" ;skos:prefLabel "Barakula:9045"@en .
geoad:Boondooma9145 a skos:Concept ;skos:definition "Map sheet for Boondooma at 1:100 000 scale. The first two digits define a longitude band 0.5 degree wide and the second two digits a latitude band 0.5 degree wide."@en ;skos:inScheme <https://linked.data.gov.au/def/geoadminfeatures> ;skos:broader geoad:MapSeries ;skos:notation "9145" ;skos:prefLabel "Boondooma:9145"@en .
geoad:Murgon9245 a skos:Concept ;skos:definition "Map sheet for Murgon at 1:100 000 scale. The first two digits define a longitude band 0.5 degree wide and the second two digits a latitude band 0.5 degree wide."@en ;skos:inScheme <https://linked.data.gov.au/def/geoadminfeatures> ;skos:broader geoad:MapSeries ;skos:notation "9245" ;skos:prefLabel "Murgon:9245"@en .
geoad:Goomeri9345 a skos:Concept ;skos:definition "Map sheet for Goomeri at 1:100 000 scale. The first two digits define a longitude band 0.5 degree wide and the second two digits a latitude band 0.5 degree wide."@en ;skos:inScheme <https://linked.data.gov.au/def/geoadminfeatures> ;skos:broader geoad:MapSeries ;skos:notation "9345" ;skos:prefLabel "Goomeri:9345"@en .
geoad:Gympie9445 a skos:Concept ;skos:definition "Map sheet for Gympie at 1:100 000 scale. The first two digits define a longitude band 0.5 degree wide and the second two digits a latitude band 0.5 degree wide."@en ;skos:inScheme <https://linked.data.gov.au/def/geoadminfeatures> ;skos:broader geoad:MapSeries ;skos:notation "9445" ;skos:prefLabel "Gympie:9445"@en .
geoad:LagunaBay9545 a skos:Concept ;skos:definition "Map sheet for Laguna Bay at 1:100 000 scale. The first two digits define a longitude band 0.5 degree wide and the second two digits a latitude band 0.5 degree wide."@en ;skos:inScheme <https://linked.data.gov.au/def/geoadminfeatures> ;skos:broader geoad:MapSeries ;skos:notation "9545" ;skos:prefLabel "Laguna Bay:9545"@en .
geoad:Koomarinna6544 a skos:Concept ;skos:definition "Map sheet for Koomarinna at 1:100 000 scale. The first two digits define a longitude band 0.5 degree wide and the second two digits a latitude band 0.5 degree wide."@en ;skos:inScheme <https://linked.data.gov.au/def/geoadminfeatures> ;skos:broader geoad:MapSeries ;skos:notation "6544" ;skos:prefLabel "Koomarinna:6544"@en .
geoad:Goyder6644 a skos:Concept ;skos:definition "Map sheet for Goyder at 1:100 000 scale. The first two digits define a longitude band 0.5 degree wide and the second two digits a latitude band 0.5 degree wide."@en ;skos:inScheme <https://linked.data.gov.au/def/geoadminfeatures> ;skos:broader geoad:MapSeries ;skos:notation "6644" ;skos:prefLabel "Goyder:6644"@en .
geoad:Diamantina6744 a skos:Concept ;skos:definition "Map sheet for Diamantina at 1:100 000 scale. The first two digits define a longitude band 0.5 degree wide and the second two digits a latitude band 0.5 degree wide."@en ;skos:inScheme <https://linked.data.gov.au/def/geoadminfeatures> ;skos:broader geoad:MapSeries ;skos:notation "6744" ;skos:prefLabel "Diamantina:6744"@en .
geoad:Yeriecoola6844 a skos:Concept ;skos:definition "Map sheet for Yeriecoola at 1:100 000 scale. The first two digits define a longitude band 0.5 degree wide and the second two digits a latitude band 0.5 degree wide."@en ;skos:inScheme <https://linked.data.gov.au/def/geoadminfeatures> ;skos:broader geoad:MapSeries ;skos:notation "6844" ;skos:prefLabel "Yeriecoola:6844"@en .
geoad:RainbowPlain6944 a skos:Concept ;skos:definition "Map sheet for Rainbow Plain at 1:100 000 scale. The first two digits define a longitude band 0.5 degree wide and the second two digits a latitude band 0.5 degree wide."@en ;skos:inScheme <https://linked.data.gov.au/def/geoadminfeatures> ;skos:broader geoad:MapSeries ;skos:notation "6944" ;skos:prefLabel "Rainbow Plain:6944"@en .
geoad:Cordillo7044 a skos:Concept ;skos:definition "Map sheet for Cordillo at 1:100 000 scale. The first two digits define a longitude band 0.5 degree wide and the second two digits a latitude band 0.5 degree wide."@en ;skos:inScheme <https://linked.data.gov.au/def/geoadminfeatures> ;skos:broader geoad:MapSeries ;skos:notation "7044" ;skos:prefLabel "Cordillo:7044"@en .
geoad:Arrabury7144 a skos:Concept ;skos:definition "Map sheet for Arrabury at 1:100 000 scale. The first two digits define a longitude band 0.5 degree wide and the second two digits a latitude band 0.5 degree wide."@en ;skos:inScheme <https://linked.data.gov.au/def/geoadminfeatures> ;skos:broader geoad:MapSeries ;skos:notation "7144" ;skos:prefLabel "Arrabury:7144"@en .
geoad:BuncheedaSwamp7244 a skos:Concept ;skos:definition "Map sheet for Buncheeda Swamp at 1:100 000 scale. The first two digits define a longitude band 0.5 degree wide and the second two digits a latitude band 0.5 degree wide."@en ;skos:inScheme <https://linked.data.gov.au/def/geoadminfeatures> ;skos:broader geoad:MapSeries ;skos:notation "7244" ;skos:prefLabel "Buncheeda Swamp:7244"@en .
geoad:MountHowitt7344 a skos:Concept ;skos:definition "Map sheet for Mount Howitt at 1:100 000 scale. The first two digits define a longitude band 0.5 degree wide and the second two digits a latitude band 0.5 degree wide."@en ;skos:inScheme <https://linked.data.gov.au/def/geoadminfeatures> ;skos:broader geoad:MapSeries ;skos:notation "7344" ;skos:prefLabel "Mount Howitt:7344"@en .
geoad:PlevnaDowns7444 a skos:Concept ;skos:definition "Map sheet for Plevna Downs at 1:100 000 scale. The first two digits define a longitude band 0.5 degree wide and the second two digits a latitude band 0.5 degree wide."@en ;skos:inScheme <https://linked.data.gov.au/def/geoadminfeatures> ;skos:broader geoad:MapSeries ;skos:notation "7444" ;skos:prefLabel "Plevna Downs:7444"@en .
geoad:Eromanga7544 a skos:Concept ;skos:definition "Map sheet for Eromanga at 1:100 000 scale. The first two digits define a longitude band 0.5 degree wide and the second two digits a latitude band 0.5 degree wide."@en ;skos:inScheme <https://linked.data.gov.au/def/geoadminfeatures> ;skos:broader geoad:MapSeries ;skos:notation "7544" ;skos:prefLabel "Eromanga:7544"@en .
geoad:Congie7644 a skos:Concept ;skos:definition "Map sheet for Congie at 1:100 000 scale. The first two digits define a longitude band 0.5 degree wide and the second two digits a latitude band 0.5 degree wide."@en ;skos:inScheme <https://linked.data.gov.au/def/geoadminfeatures> ;skos:broader geoad:MapSeries ;skos:notation "7644" ;skos:prefLabel "Congie:7644"@en .
geoad:Quilpie7744 a skos:Concept ;skos:definition "Map sheet for Quilpie at 1:100 000 scale. The first two digits define a longitude band 0.5 degree wide and the second two digits a latitude band 0.5 degree wide."@en ;skos:inScheme <https://linked.data.gov.au/def/geoadminfeatures> ;skos:broader geoad:MapSeries ;skos:notation "7744" ;skos:prefLabel "Quilpie:7744"@en .
geoad:Winbin7844 a skos:Concept ;skos:definition "Map sheet for Winbin at 1:100 000 scale. The first two digits define a longitude band 0.5 degree wide and the second two digits a latitude band 0.5 degree wide."@en ;skos:inScheme <https://linked.data.gov.au/def/geoadminfeatures> ;skos:broader geoad:MapSeries ;skos:notation "7844" ;skos:prefLabel "Winbin:7844"@en .
geoad:Cheepie7944 a skos:Concept ;skos:definition "Map sheet for Cheepie at 1:100 000 scale. The first two digits define a longitude band 0.5 degree wide and the second two digits a latitude band 0.5 degree wide."@en ;skos:inScheme <https://linked.data.gov.au/def/geoadminfeatures> ;skos:broader geoad:MapSeries ;skos:notation "7944" ;skos:prefLabel "Cheepie:7944"@en .
geoad:Loddon8044 a skos:Concept ;skos:definition "Map sheet for Loddon at 1:100 000 scale. The first two digits define a longitude band 0.5 degree wide and the second two digits a latitude band 0.5 degree wide."@en ;skos:inScheme <https://linked.data.gov.au/def/geoadminfeatures> ;skos:broader geoad:MapSeries ;skos:notation "8044" ;skos:prefLabel "Loddon:8044"@en .
geoad:Westgate8144 a skos:Concept ;skos:definition "Map sheet for Westgate at 1:100 000 scale. The first two digits define a longitude band 0.5 degree wide and the second two digits a latitude band 0.5 degree wide."@en ;skos:inScheme <https://linked.data.gov.au/def/geoadminfeatures> ;skos:broader geoad:MapSeries ;skos:notation "8144" ;skos:prefLabel "Westgate:8144"@en .
geoad:Authoringa8244 a skos:Concept ;skos:definition "Map sheet for Authoringa at 1:100 000 scale. The first two digits define a longitude band 0.5 degree wide and the second two digits a latitude band 0.5 degree wide."@en ;skos:inScheme <https://linked.data.gov.au/def/geoadminfeatures> ;skos:broader geoad:MapSeries ;skos:notation "8244" ;skos:prefLabel "Authoringa:8244"@en .
geoad:Ularunda8344 a skos:Concept ;skos:definition "Map sheet for Ularunda at 1:100 000 scale. The first two digits define a longitude band 0.5 degree wide and the second two digits a latitude band 0.5 degree wide."@en ;skos:inScheme <https://linked.data.gov.au/def/geoadminfeatures> ;skos:broader geoad:MapSeries ;skos:notation "8344" ;skos:prefLabel "Ularunda:8344"@en .
geoad:BonusDowns8444 a skos:Concept ;skos:definition "Map sheet for Bonus Downs at 1:100 000 scale. The first two digits define a longitude band 0.5 degree wide and the second two digits a latitude band 0.5 degree wide."@en ;skos:inScheme <https://linked.data.gov.au/def/geoadminfeatures> ;skos:broader geoad:MapSeries ;skos:notation "8444" ;skos:prefLabel "Bonus Downs:8444"@en .
geoad:Muckadilla8544 a skos:Concept ;skos:definition "Map sheet for Muckadilla at 1:100 000 scale. The first two digits define a longitude band 0.5 degree wide and the second two digits a latitude band 0.5 degree wide."@en ;skos:inScheme <https://linked.data.gov.au/def/geoadminfeatures> ;skos:broader geoad:MapSeries ;skos:notation "8544" ;skos:prefLabel "Muckadilla:8544"@en .
geoad:Roma8644 a skos:Concept ;skos:definition "Map sheet for Roma at 1:100 000 scale. The first two digits define a longitude band 0.5 degree wide and the second two digits a latitude band 0.5 degree wide."@en ;skos:inScheme <https://linked.data.gov.au/def/geoadminfeatures> ;skos:broader geoad:MapSeries ;skos:notation "8644" ;skos:prefLabel "Roma:8644"@en .
geoad:Yuleba8744 a skos:Concept ;skos:definition "Map sheet for Yuleba at 1:100 000 scale. The first two digits define a longitude band 0.5 degree wide and the second two digits a latitude band 0.5 degree wide."@en ;skos:inScheme <https://linked.data.gov.au/def/geoadminfeatures> ;skos:broader geoad:MapSeries ;skos:notation "8744" ;skos:prefLabel "Yuleba:8744"@en .
geoad:Dulacca8844 a skos:Concept ;skos:definition "Map sheet for Dulacca at 1:100 000 scale. The first two digits define a longitude band 0.5 degree wide and the second two digits a latitude band 0.5 degree wide."@en ;skos:inScheme <https://linked.data.gov.au/def/geoadminfeatures> ;skos:broader geoad:MapSeries ;skos:notation "8844" ;skos:prefLabel "Dulacca:8844"@en .
geoad:Miles8944 a skos:Concept ;skos:definition "Map sheet for Miles at 1:100 000 scale. The first two digits define a longitude band 0.5 degree wide and the second two digits a latitude band 0.5 degree wide."@en ;skos:inScheme <https://linked.data.gov.au/def/geoadminfeatures> ;skos:broader geoad:MapSeries ;skos:notation "8944" ;skos:prefLabel "Miles:8944"@en .
geoad:Chinchilla9044 a skos:Concept ;skos:definition "Map sheet for Chinchilla at 1:100 000 scale. The first two digits define a longitude band 0.5 degree wide and the second two digits a latitude band 0.5 degree wide."@en ;skos:inScheme <https://linked.data.gov.au/def/geoadminfeatures> ;skos:broader geoad:MapSeries ;skos:notation "9044" ;skos:prefLabel "Chinchilla:9044"@en .
geoad:Jandowae9144 a skos:Concept ;skos:definition "Map sheet for Jandowae at 1:100 000 scale. The first two digits define a longitude band 0.5 degree wide and the second two digits a latitude band 0.5 degree wide."@en ;skos:inScheme <https://linked.data.gov.au/def/geoadminfeatures> ;skos:broader geoad:MapSeries ;skos:notation "9144" ;skos:prefLabel "Jandowae:9144"@en .
geoad:Kingaroy9244 a skos:Concept ;skos:definition "Map sheet for Kingaroy at 1:100 000 scale. The first two digits define a longitude band 0.5 degree wide and the second two digits a latitude band 0.5 degree wide."@en ;skos:inScheme <https://linked.data.gov.au/def/geoadminfeatures> ;skos:broader geoad:MapSeries ;skos:notation "9244" ;skos:prefLabel "Kingaroy:9244"@en .
geoad:Nanango9344 a skos:Concept ;skos:definition "Map sheet for Nanango at 1:100 000 scale. The first two digits define a longitude band 0.5 degree wide and the second two digits a latitude band 0.5 degree wide."@en ;skos:inScheme <https://linked.data.gov.au/def/geoadminfeatures> ;skos:broader geoad:MapSeries ;skos:notation "9344" ;skos:prefLabel "Nanango:9344"@en .
geoad:Nambour9444 a skos:Concept ;skos:definition "Map sheet for Nambour at 1:100 000 scale. The first two digits define a longitude band 0.5 degree wide and the second two digits a latitude band 0.5 degree wide."@en ;skos:inScheme <https://linked.data.gov.au/def/geoadminfeatures> ;skos:broader geoad:MapSeries ;skos:notation "9444" ;skos:prefLabel "Nambour:9444"@en .
geoad:Caloundra9544 a skos:Concept ;skos:definition "Map sheet for Caloundra at 1:100 000 scale. The first two digits define a longitude band 0.5 degree wide and the second two digits a latitude band 0.5 degree wide."@en ;skos:inScheme <https://linked.data.gov.au/def/geoadminfeatures> ;skos:broader geoad:MapSeries ;skos:notation "9544" ;skos:prefLabel "Caloundra:9544"@en .
geoad:Pathraootara6543 a skos:Concept ;skos:definition "Map sheet for Pathraootara at 1:100 000 scale. The first two digits define a longitude band 0.5 degree wide and the second two digits a latitude band 0.5 degree wide."@en ;skos:inScheme <https://linked.data.gov.au/def/geoadminfeatures> ;skos:broader geoad:MapSeries ;skos:notation "6543" ;skos:prefLabel "Pathraootara:6543"@en .
geoad:Gason6643 a skos:Concept ;skos:definition "Map sheet for Gason at 1:100 000 scale. The first two digits define a longitude band 0.5 degree wide and the second two digits a latitude band 0.5 degree wide."@en ;skos:inScheme <https://linked.data.gov.au/def/geoadminfeatures> ;skos:broader geoad:MapSeries ;skos:notation "6643" ;skos:prefLabel "Gason:6643"@en .
geoad:Talleranie6743 a skos:Concept ;skos:definition "Map sheet for Talleranie at 1:100 000 scale. The first two digits define a longitude band 0.5 degree wide and the second two digits a latitude band 0.5 degree wide."@en ;skos:inScheme <https://linked.data.gov.au/def/geoadminfeatures> ;skos:broader geoad:MapSeries ;skos:notation "6743" ;skos:prefLabel "Talleranie:6743"@en .
geoad:ChristmasCreek6843 a skos:Concept ;skos:definition "Map sheet for Christmas Creek at 1:100 000 scale. The first two digits define a longitude band 0.5 degree wide and the second two digits a latitude band 0.5 degree wide."@en ;skos:inScheme <https://linked.data.gov.au/def/geoadminfeatures> ;skos:broader geoad:MapSeries ;skos:notation "6843" ;skos:prefLabel "Christmas Creek:6843"@en .
geoad:Coongie6943 a skos:Concept ;skos:definition "Map sheet for Coongie at 1:100 000 scale. The first two digits define a longitude band 0.5 degree wide and the second two digits a latitude band 0.5 degree wide."@en ;skos:inScheme <https://linked.data.gov.au/def/geoadminfeatures> ;skos:broader geoad:MapSeries ;skos:notation "6943" ;skos:prefLabel "Coongie:6943"@en .
geoad:Patchawara7043 a skos:Concept ;skos:definition "Map sheet for Patchawara at 1:100 000 scale. The first two digits define a longitude band 0.5 degree wide and the second two digits a latitude band 0.5 degree wide."@en ;skos:inScheme <https://linked.data.gov.au/def/geoadminfeatures> ;skos:broader geoad:MapSeries ;skos:notation "7043" ;skos:prefLabel "Patchawara:7043"@en .
geoad:LakePure7143 a skos:Concept ;skos:definition "Map sheet for Lake Pure at 1:100 000 scale. The first two digits define a longitude band 0.5 degree wide and the second two digits a latitude band 0.5 degree wide."@en ;skos:inScheme <https://linked.data.gov.au/def/geoadminfeatures> ;skos:broader geoad:MapSeries ;skos:notation "7143" ;skos:prefLabel "Lake Pure:7143"@en .
geoad:DurhamDowns7243 a skos:Concept ;skos:definition "Map sheet for Durham Downs at 1:100 000 scale. The first two digits define a longitude band 0.5 degree wide and the second two digits a latitude band 0.5 degree wide."@en ;skos:inScheme <https://linked.data.gov.au/def/geoadminfeatures> ;skos:broader geoad:MapSeries ;skos:notation "7243" ;skos:prefLabel "Durham Downs:7243"@en .
geoad:Woomanooka7343 a skos:Concept ;skos:definition "Map sheet for Woomanooka at 1:100 000 scale. The first two digits define a longitude band 0.5 degree wide and the second two digits a latitude band 0.5 degree wide."@en ;skos:inScheme <https://linked.data.gov.au/def/geoadminfeatures> ;skos:broader geoad:MapSeries ;skos:notation "7343" ;skos:prefLabel "Woomanooka:7343"@en .
geoad:Kihee7443 a skos:Concept ;skos:definition "Map sheet for Kihee at 1:100 000 scale. The first two digits define a longitude band 0.5 degree wide and the second two digits a latitude band 0.5 degree wide."@en ;skos:inScheme <https://linked.data.gov.au/def/geoadminfeatures> ;skos:broader geoad:MapSeries ;skos:notation "7443" ;skos:prefLabel "Kihee:7443"@en .
geoad:Barcoonia7543 a skos:Concept ;skos:definition "Map sheet for Barcoonia at 1:100 000 scale. The first two digits define a longitude band 0.5 degree wide and the second two digits a latitude band 0.5 degree wide."@en ;skos:inScheme <https://linked.data.gov.au/def/geoadminfeatures> ;skos:broader geoad:MapSeries ;skos:notation "7543" ;skos:prefLabel "Barcoonia:7543"@en .
geoad:Bowalli7643 a skos:Concept ;skos:definition "Map sheet for Bowalli at 1:100 000 scale. The first two digits define a longitude band 0.5 degree wide and the second two digits a latitude band 0.5 degree wide."@en ;skos:inScheme <https://linked.data.gov.au/def/geoadminfeatures> ;skos:broader geoad:MapSeries ;skos:notation "7643" ;skos:prefLabel "Bowalli:7643"@en .
geoad:Toompine7743 a skos:Concept ;skos:definition "Map sheet for Toompine at 1:100 000 scale. The first two digits define a longitude band 0.5 degree wide and the second two digits a latitude band 0.5 degree wide."@en ;skos:inScheme <https://linked.data.gov.au/def/geoadminfeatures> ;skos:broader geoad:MapSeries ;skos:notation "7743" ;skos:prefLabel "Toompine:7743"@en .
geoad:Beechal7843 a skos:Concept ;skos:definition "Map sheet for Beechal at 1:100 000 scale. The first two digits define a longitude band 0.5 degree wide and the second two digits a latitude band 0.5 degree wide."@en ;skos:inScheme <https://linked.data.gov.au/def/geoadminfeatures> ;skos:broader geoad:MapSeries ;skos:notation "7843" ;skos:prefLabel "Beechal:7843"@en .
geoad:Humeburn7943 a skos:Concept ;skos:definition "Map sheet for Humeburn at 1:100 000 scale. The first two digits define a longitude band 0.5 degree wide and the second two digits a latitude band 0.5 degree wide."@en ;skos:inScheme <https://linked.data.gov.au/def/geoadminfeatures> ;skos:broader geoad:MapSeries ;skos:notation "7943" ;skos:prefLabel "Humeburn:7943"@en .
geoad:Wyandra8043 a skos:Concept ;skos:definition "Map sheet for Wyandra at 1:100 000 scale. The first two digits define a longitude band 0.5 degree wide and the second two digits a latitude band 0.5 degree wide."@en ;skos:inScheme <https://linked.data.gov.au/def/geoadminfeatures> ;skos:broader geoad:MapSeries ;skos:notation "8043" ;skos:prefLabel "Wyandra:8043"@en .
geoad:Murweh8143 a skos:Concept ;skos:definition "Map sheet for Murweh at 1:100 000 scale. The first two digits define a longitude band 0.5 degree wide and the second two digits a latitude band 0.5 degree wide."@en ;skos:inScheme <https://linked.data.gov.au/def/geoadminfeatures> ;skos:broader geoad:MapSeries ;skos:notation "8143" ;skos:prefLabel "Murweh:8143"@en .
geoad:Elmina8243 a skos:Concept ;skos:definition "Map sheet for Elmina at 1:100 000 scale. The first two digits define a longitude band 0.5 degree wide and the second two digits a latitude band 0.5 degree wide."@en ;skos:inScheme <https://linked.data.gov.au/def/geoadminfeatures> ;skos:broader geoad:MapSeries ;skos:notation "8243" ;skos:prefLabel "Elmina:8243"@en .
geoad:Tongy8343 a skos:Concept ;skos:definition "Map sheet for Tongy at 1:100 000 scale. The first two digits define a longitude band 0.5 degree wide and the second two digits a latitude band 0.5 degree wide."@en ;skos:inScheme <https://linked.data.gov.au/def/geoadminfeatures> ;skos:broader geoad:MapSeries ;skos:notation "8343" ;skos:prefLabel "Tongy:8343"@en .
geoad:Abbieglassie8443 a skos:Concept ;skos:definition "Map sheet for Abbieglassie at 1:100 000 scale. The first two digits define a longitude band 0.5 degree wide and the second two digits a latitude band 0.5 degree wide."@en ;skos:inScheme <https://linked.data.gov.au/def/geoadminfeatures> ;skos:broader geoad:MapSeries ;skos:notation "8443" ;skos:prefLabel "Abbieglassie:8443"@en .
geoad:Struan8543 a skos:Concept ;skos:definition "Map sheet for Struan at 1:100 000 scale. The first two digits define a longitude band 0.5 degree wide and the second two digits a latitude band 0.5 degree wide."@en ;skos:inScheme <https://linked.data.gov.au/def/geoadminfeatures> ;skos:broader geoad:MapSeries ;skos:notation "8543" ;skos:prefLabel "Struan:8543"@en .
geoad:Cogoon8643 a skos:Concept ;skos:definition "Map sheet for Cogoon at 1:100 000 scale. The first two digits define a longitude band 0.5 degree wide and the second two digits a latitude band 0.5 degree wide."@en ;skos:inScheme <https://linked.data.gov.au/def/geoadminfeatures> ;skos:broader geoad:MapSeries ;skos:notation "8643" ;skos:prefLabel "Cogoon:8643"@en .
geoad:Surat8743 a skos:Concept ;skos:definition "Map sheet for Surat at 1:100 000 scale. The first two digits define a longitude band 0.5 degree wide and the second two digits a latitude band 0.5 degree wide."@en ;skos:inScheme <https://linked.data.gov.au/def/geoadminfeatures> ;skos:broader geoad:MapSeries ;skos:notation "8743" ;skos:prefLabel "Surat:8743"@en .
geoad:Meandarra8843 a skos:Concept ;skos:definition "Map sheet for Meandarra at 1:100 000 scale. The first two digits define a longitude band 0.5 degree wide and the second two digits a latitude band 0.5 degree wide."@en ;skos:inScheme <https://linked.data.gov.au/def/geoadminfeatures> ;skos:broader geoad:MapSeries ;skos:notation "8843" ;skos:prefLabel "Meandarra:8843"@en .
geoad:Tara8943 a skos:Concept ;skos:definition "Map sheet for Tara at 1:100 000 scale. The first two digits define a longitude band 0.5 degree wide and the second two digits a latitude band 0.5 degree wide."@en ;skos:inScheme <https://linked.data.gov.au/def/geoadminfeatures> ;skos:broader geoad:MapSeries ;skos:notation "8943" ;skos:prefLabel "Tara:8943"@en .
geoad:Kogan9043 a skos:Concept ;skos:definition "Map sheet for Kogan at 1:100 000 scale. The first two digits define a longitude band 0.5 degree wide and the second two digits a latitude band 0.5 degree wide."@en ;skos:inScheme <https://linked.data.gov.au/def/geoadminfeatures> ;skos:broader geoad:MapSeries ;skos:notation "9043" ;skos:prefLabel "Kogan:9043"@en .
geoad:Dalby9143 a skos:Concept ;skos:definition "Map sheet for Dalby at 1:100 000 scale. The first two digits define a longitude band 0.5 degree wide and the second two digits a latitude band 0.5 degree wide."@en ;skos:inScheme <https://linked.data.gov.au/def/geoadminfeatures> ;skos:broader geoad:MapSeries ;skos:notation "9143" ;skos:prefLabel "Dalby:9143"@en .
geoad:Oakey9243 a skos:Concept ;skos:definition "Map sheet for Oakey at 1:100 000 scale. The first two digits define a longitude band 0.5 degree wide and the second two digits a latitude band 0.5 degree wide."@en ;skos:inScheme <https://linked.data.gov.au/def/geoadminfeatures> ;skos:broader geoad:MapSeries ;skos:notation "9243" ;skos:prefLabel "Oakey:9243"@en .
geoad:Esk9343 a skos:Concept ;skos:definition "Map sheet for Esk at 1:100 000 scale. The first two digits define a longitude band 0.5 degree wide and the second two digits a latitude band 0.5 degree wide."@en ;skos:inScheme <https://linked.data.gov.au/def/geoadminfeatures> ;skos:broader geoad:MapSeries ;skos:notation "9343" ;skos:prefLabel "Esk:9343"@en .
geoad:Caboolture9443 a skos:Concept ;skos:definition "Map sheet for Caboolture at 1:100 000 scale. The first two digits define a longitude band 0.5 degree wide and the second two digits a latitude band 0.5 degree wide."@en ;skos:inScheme <https://linked.data.gov.au/def/geoadminfeatures> ;skos:broader geoad:MapSeries ;skos:notation "9443" ;skos:prefLabel "Caboolture:9443"@en .
geoad:Brisbane9543 a skos:Concept ;skos:definition "Map sheet for Brisbane at 1:100 000 scale. The first two digits define a longitude band 0.5 degree wide and the second two digits a latitude band 0.5 degree wide."@en ;skos:inScheme <https://linked.data.gov.au/def/geoadminfeatures> ;skos:broader geoad:MapSeries ;skos:notation "9543" ;skos:prefLabel "Brisbane:9543"@en .
geoad:PointLookout9643 a skos:Concept ;skos:definition "Map sheet for Point Lookout at 1:100 000 scale. The first two digits define a longitude band 0.5 degree wide and the second two digits a latitude band 0.5 degree wide."@en ;skos:inScheme <https://linked.data.gov.au/def/geoadminfeatures> ;skos:broader geoad:MapSeries ;skos:notation "9643" ;skos:prefLabel "Point Lookout:9643"@en .
geoad:Cowarie6542 a skos:Concept ;skos:definition "Map sheet for Cowarie at 1:100 000 scale. The first two digits define a longitude band 0.5 degree wide and the second two digits a latitude band 0.5 degree wide."@en ;skos:inScheme <https://linked.data.gov.au/def/geoadminfeatures> ;skos:broader geoad:MapSeries ;skos:notation "6542" ;skos:prefLabel "Cowarie:6542"@en .
geoad:MirraMitta6642 a skos:Concept ;skos:definition "Map sheet for Mirra Mitta at 1:100 000 scale. The first two digits define a longitude band 0.5 degree wide and the second two digits a latitude band 0.5 degree wide."@en ;skos:inScheme <https://linked.data.gov.au/def/geoadminfeatures> ;skos:broader geoad:MapSeries ;skos:notation "6642" ;skos:prefLabel "Mirra Mitta:6642"@en .
geoad:Perigundi6742 a skos:Concept ;skos:definition "Map sheet for Perigundi at 1:100 000 scale. The first two digits define a longitude band 0.5 degree wide and the second two digits a latitude band 0.5 degree wide."@en ;skos:inScheme <https://linked.data.gov.au/def/geoadminfeatures> ;skos:broader geoad:MapSeries ;skos:notation "6742" ;skos:prefLabel "Perigundi:6742"@en .
geoad:Kanowana6842 a skos:Concept ;skos:definition "Map sheet for Kanowana at 1:100 000 scale. The first two digits define a longitude band 0.5 degree wide and the second two digits a latitude band 0.5 degree wide."@en ;skos:inScheme <https://linked.data.gov.au/def/geoadminfeatures> ;skos:broader geoad:MapSeries ;skos:notation "6842" ;skos:prefLabel "Kanowana:6842"@en .
geoad:Gidgealpa6942 a skos:Concept ;skos:definition "Map sheet for Gidgealpa at 1:100 000 scale. The first two digits define a longitude band 0.5 degree wide and the second two digits a latitude band 0.5 degree wide."@en ;skos:inScheme <https://linked.data.gov.au/def/geoadminfeatures> ;skos:broader geoad:MapSeries ;skos:notation "6942" ;skos:prefLabel "Gidgealpa:6942"@en .
geoad:Innamincka7042 a skos:Concept ;skos:definition "Map sheet for Innamincka at 1:100 000 scale. The first two digits define a longitude band 0.5 degree wide and the second two digits a latitude band 0.5 degree wide."@en ;skos:inScheme <https://linked.data.gov.au/def/geoadminfeatures> ;skos:broader geoad:MapSeries ;skos:notation "7042" ;skos:prefLabel "Innamincka:7042"@en .
geoad:Nappamerry7142 a skos:Concept ;skos:definition "Map sheet for Nappamerry at 1:100 000 scale. The first two digits define a longitude band 0.5 degree wide and the second two digits a latitude band 0.5 degree wide."@en ;skos:inScheme <https://linked.data.gov.au/def/geoadminfeatures> ;skos:broader geoad:MapSeries ;skos:notation "7142" ;skos:prefLabel "Nappamerry:7142"@en .
geoad:Baryulah7242 a skos:Concept ;skos:definition "Map sheet for Baryulah at 1:100 000 scale. The first two digits define a longitude band 0.5 degree wide and the second two digits a latitude band 0.5 degree wide."@en ;skos:inScheme <https://linked.data.gov.au/def/geoadminfeatures> ;skos:broader geoad:MapSeries ;skos:notation "7242" ;skos:prefLabel "Baryulah:7242"@en .
geoad:Naccowlah7342 a skos:Concept ;skos:definition "Map sheet for Naccowlah at 1:100 000 scale. The first two digits define a longitude band 0.5 degree wide and the second two digits a latitude band 0.5 degree wide."@en ;skos:inScheme <https://linked.data.gov.au/def/geoadminfeatures> ;skos:broader geoad:MapSeries ;skos:notation "7342" ;skos:prefLabel "Naccowlah:7342"@en .
geoad:Noccundra7442 a skos:Concept ;skos:definition "Map sheet for Noccundra at 1:100 000 scale. The first two digits define a longitude band 0.5 degree wide and the second two digits a latitude band 0.5 degree wide."@en ;skos:inScheme <https://linked.data.gov.au/def/geoadminfeatures> ;skos:broader geoad:MapSeries ;skos:notation "7442" ;skos:prefLabel "Noccundra:7442"@en .
geoad:Pinidary7542 a skos:Concept ;skos:definition "Map sheet for Pinidary at 1:100 000 scale. The first two digits define a longitude band 0.5 degree wide and the second two digits a latitude band 0.5 degree wide."@en ;skos:inScheme <https://linked.data.gov.au/def/geoadminfeatures> ;skos:broader geoad:MapSeries ;skos:notation "7542" ;skos:prefLabel "Pinidary:7542"@en .
geoad:Thargomindah7642 a skos:Concept ;skos:definition "Map sheet for Thargomindah at 1:100 000 scale. The first two digits define a longitude band 0.5 degree wide and the second two digits a latitude band 0.5 degree wide."@en ;skos:inScheme <https://linked.data.gov.au/def/geoadminfeatures> ;skos:broader geoad:MapSeries ;skos:notation "7642" ;skos:prefLabel "Thargomindah:7642"@en .
geoad:WerieEla7742 a skos:Concept ;skos:definition "Map sheet for Werie Ela at 1:100 000 scale. The first two digits define a longitude band 0.5 degree wide and the second two digits a latitude band 0.5 degree wide."@en ;skos:inScheme <https://linked.data.gov.au/def/geoadminfeatures> ;skos:broader geoad:MapSeries ;skos:notation "7742" ;skos:prefLabel "Werie Ela:7742"@en .
geoad:Dundoo7842 a skos:Concept ;skos:definition "Map sheet for Dundoo at 1:100 000 scale. The first two digits define a longitude band 0.5 degree wide and the second two digits a latitude band 0.5 degree wide."@en ;skos:inScheme <https://linked.data.gov.au/def/geoadminfeatures> ;skos:broader geoad:MapSeries ;skos:notation "7842" ;skos:prefLabel "Dundoo:7842"@en .
geoad:Boobara7942 a skos:Concept ;skos:definition "Map sheet for Boobara at 1:100 000 scale. The first two digits define a longitude band 0.5 degree wide and the second two digits a latitude band 0.5 degree wide."@en ;skos:inScheme <https://linked.data.gov.au/def/geoadminfeatures> ;skos:broader geoad:MapSeries ;skos:notation "7942" ;skos:prefLabel "Boobara:7942"@en .
geoad:Coongoola8042 a skos:Concept ;skos:definition "Map sheet for Coongoola at 1:100 000 scale. The first two digits define a longitude band 0.5 degree wide and the second two digits a latitude band 0.5 degree wide."@en ;skos:inScheme <https://linked.data.gov.au/def/geoadminfeatures> ;skos:broader geoad:MapSeries ;skos:notation "8042" ;skos:prefLabel "Coongoola:8042"@en .
geoad:Yarmouth8142 a skos:Concept ;skos:definition "Map sheet for Yarmouth at 1:100 000 scale. The first two digits define a longitude band 0.5 degree wide and the second two digits a latitude band 0.5 degree wide."@en ;skos:inScheme <https://linked.data.gov.au/def/geoadminfeatures> ;skos:broader geoad:MapSeries ;skos:notation "8142" ;skos:prefLabel "Yarmouth:8142"@en .
geoad:Bendena8242 a skos:Concept ;skos:definition "Map sheet for Bendena at 1:100 000 scale. The first two digits define a longitude band 0.5 degree wide and the second two digits a latitude band 0.5 degree wide."@en ;skos:inScheme <https://linked.data.gov.au/def/geoadminfeatures> ;skos:broader geoad:MapSeries ;skos:notation "8242" ;skos:prefLabel "Bendena:8242"@en .
geoad:Homeboin8342 a skos:Concept ;skos:definition "Map sheet for Homeboin at 1:100 000 scale. The first two digits define a longitude band 0.5 degree wide and the second two digits a latitude band 0.5 degree wide."@en ;skos:inScheme <https://linked.data.gov.au/def/geoadminfeatures> ;skos:broader geoad:MapSeries ;skos:notation "8342" ;skos:prefLabel "Homeboin:8342"@en .
geoad:Wierbolla8442 a skos:Concept ;skos:definition "Map sheet for Wierbolla at 1:100 000 scale. The first two digits define a longitude band 0.5 degree wide and the second two digits a latitude band 0.5 degree wide."@en ;skos:inScheme <https://linked.data.gov.au/def/geoadminfeatures> ;skos:broader geoad:MapSeries ;skos:notation "8442" ;skos:prefLabel "Wierbolla:8442"@en .
geoad:Boolba8542 a skos:Concept ;skos:definition "Map sheet for Boolba at 1:100 000 scale. The first two digits define a longitude band 0.5 degree wide and the second two digits a latitude band 0.5 degree wide."@en ;skos:inScheme <https://linked.data.gov.au/def/geoadminfeatures> ;skos:broader geoad:MapSeries ;skos:notation "8542" ;skos:prefLabel "Boolba:8542"@en .
geoad:Burgorah8642 a skos:Concept ;skos:definition "Map sheet for Burgorah at 1:100 000 scale. The first two digits define a longitude band 0.5 degree wide and the second two digits a latitude band 0.5 degree wide."@en ;skos:inScheme <https://linked.data.gov.au/def/geoadminfeatures> ;skos:broader geoad:MapSeries ;skos:notation "8642" ;skos:prefLabel "Burgorah:8642"@en .
geoad:Bidgel8742 a skos:Concept ;skos:definition "Map sheet for Bidgel at 1:100 000 scale. The first two digits define a longitude band 0.5 degree wide and the second two digits a latitude band 0.5 degree wide."@en ;skos:inScheme <https://linked.data.gov.au/def/geoadminfeatures> ;skos:broader geoad:MapSeries ;skos:notation "8742" ;skos:prefLabel "Bidgel:8742"@en .
geoad:Flinton8842 a skos:Concept ;skos:definition "Map sheet for Flinton at 1:100 000 scale. The first two digits define a longitude band 0.5 degree wide and the second two digits a latitude band 0.5 degree wide."@en ;skos:inScheme <https://linked.data.gov.au/def/geoadminfeatures> ;skos:broader geoad:MapSeries ;skos:notation "8842" ;skos:prefLabel "Flinton:8842"@en .
geoad:Moonie8942 a skos:Concept ;skos:definition "Map sheet for Moonie at 1:100 000 scale. The first two digits define a longitude band 0.5 degree wide and the second two digits a latitude band 0.5 degree wide."@en ;skos:inScheme <https://linked.data.gov.au/def/geoadminfeatures> ;skos:broader geoad:MapSeries ;skos:notation "8942" ;skos:prefLabel "Moonie:8942"@en .
geoad:WaarWaar9042 a skos:Concept ;skos:definition "Map sheet for Waar Waar at 1:100 000 scale. The first two digits define a longitude band 0.5 degree wide and the second two digits a latitude band 0.5 degree wide."@en ;skos:inScheme <https://linked.data.gov.au/def/geoadminfeatures> ;skos:broader geoad:MapSeries ;skos:notation "9042" ;skos:prefLabel "Waar Waar:9042"@en .
geoad:Millmerran9142 a skos:Concept ;skos:definition "Map sheet for Millmerran at 1:100 000 scale. The first two digits define a longitude band 0.5 degree wide and the second two digits a latitude band 0.5 degree wide."@en ;skos:inScheme <https://linked.data.gov.au/def/geoadminfeatures> ;skos:broader geoad:MapSeries ;skos:notation "9142" ;skos:prefLabel "Millmerran:9142"@en .
geoad:Toowoomba9242 a skos:Concept ;skos:definition "Map sheet for Toowoomba at 1:100 000 scale. The first two digits define a longitude band 0.5 degree wide and the second two digits a latitude band 0.5 degree wide."@en ;skos:inScheme <https://linked.data.gov.au/def/geoadminfeatures> ;skos:broader geoad:MapSeries ;skos:notation "9242" ;skos:prefLabel "Toowoomba:9242"@en .
geoad:Helidon9342 a skos:Concept ;skos:definition "Map sheet for Helidon at 1:100 000 scale. The first two digits define a longitude band 0.5 degree wide and the second two digits a latitude band 0.5 degree wide."@en ;skos:inScheme <https://linked.data.gov.au/def/geoadminfeatures> ;skos:broader geoad:MapSeries ;skos:notation "9342" ;skos:prefLabel "Helidon:9342"@en .
geoad:Ipswich9442 a skos:Concept ;skos:definition "Map sheet for Ipswich at 1:100 000 scale. The first two digits define a longitude band 0.5 degree wide and the second two digits a latitude band 0.5 degree wide."@en ;skos:inScheme <https://linked.data.gov.au/def/geoadminfeatures> ;skos:broader geoad:MapSeries ;skos:notation "9442" ;skos:prefLabel "Ipswich:9442"@en .
geoad:Beenleigh9542 a skos:Concept ;skos:definition "Map sheet for Beenleigh at 1:100 000 scale. The first two digits define a longitude band 0.5 degree wide and the second two digits a latitude band 0.5 degree wide."@en ;skos:inScheme <https://linked.data.gov.au/def/geoadminfeatures> ;skos:broader geoad:MapSeries ;skos:notation "9542" ;skos:prefLabel "Beenleigh:9542"@en .
geoad:Kittakittaooloo6541 a skos:Concept ;skos:definition "Map sheet for Kittakittaooloo at 1:100 000 scale. The first two digits define a longitude band 0.5 degree wide and the second two digits a latitude band 0.5 degree wide."@en ;skos:inScheme <https://linked.data.gov.au/def/geoadminfeatures> ;skos:broader geoad:MapSeries ;skos:notation "6541" ;skos:prefLabel "Kittakittaooloo:6541"@en .
geoad:Mulka6641 a skos:Concept ;skos:definition "Map sheet for Mulka at 1:100 000 scale. The first two digits define a longitude band 0.5 degree wide and the second two digits a latitude band 0.5 degree wide."@en ;skos:inScheme <https://linked.data.gov.au/def/geoadminfeatures> ;skos:broader geoad:MapSeries ;skos:notation "6641" ;skos:prefLabel "Mulka:6641"@en .
geoad:LakeHope6741 a skos:Concept ;skos:definition "Map sheet for Lake Hope at 1:100 000 scale. The first two digits define a longitude band 0.5 degree wide and the second two digits a latitude band 0.5 degree wide."@en ;skos:inScheme <https://linked.data.gov.au/def/geoadminfeatures> ;skos:broader geoad:MapSeries ;skos:notation "6741" ;skos:prefLabel "Lake Hope:6741"@en .
geoad:DiamondBog6841 a skos:Concept ;skos:definition "Map sheet for Diamond Bog at 1:100 000 scale. The first two digits define a longitude band 0.5 degree wide and the second two digits a latitude band 0.5 degree wide."@en ;skos:inScheme <https://linked.data.gov.au/def/geoadminfeatures> ;skos:broader geoad:MapSeries ;skos:notation "6841" ;skos:prefLabel "Diamond Bog:6841"@en .
geoad:Daralingie6941 a skos:Concept ;skos:definition "Map sheet for Daralingie at 1:100 000 scale. The first two digits define a longitude band 0.5 degree wide and the second two digits a latitude band 0.5 degree wide."@en ;skos:inScheme <https://linked.data.gov.au/def/geoadminfeatures> ;skos:broader geoad:MapSeries ;skos:notation "6941" ;skos:prefLabel "Daralingie:6941"@en .
geoad:Dullingari7041 a skos:Concept ;skos:definition "Map sheet for Dullingari at 1:100 000 scale. The first two digits define a longitude band 0.5 degree wide and the second two digits a latitude band 0.5 degree wide."@en ;skos:inScheme <https://linked.data.gov.au/def/geoadminfeatures> ;skos:broader geoad:MapSeries ;skos:notation "7041" ;skos:prefLabel "Dullingari:7041"@en .
geoad:Epsilon7141 a skos:Concept ;skos:definition "Map sheet for Epsilon at 1:100 000 scale. The first two digits define a longitude band 0.5 degree wide and the second two digits a latitude band 0.5 degree wide."@en ;skos:inScheme <https://linked.data.gov.au/def/geoadminfeatures> ;skos:broader geoad:MapSeries ;skos:notation "7141" ;skos:prefLabel "Epsilon:7141"@en .
geoad:Orientos7241 a skos:Concept ;skos:definition "Map sheet for Orientos at 1:100 000 scale. The first two digits define a longitude band 0.5 degree wide and the second two digits a latitude band 0.5 degree wide."@en ;skos:inScheme <https://linked.data.gov.au/def/geoadminfeatures> ;skos:broader geoad:MapSeries ;skos:notation "7241" ;skos:prefLabel "Orientos:7241"@en .
geoad:Bransby7341 a skos:Concept ;skos:definition "Map sheet for Bransby at 1:100 000 scale. The first two digits define a longitude band 0.5 degree wide and the second two digits a latitude band 0.5 degree wide."@en ;skos:inScheme <https://linked.data.gov.au/def/geoadminfeatures> ;skos:broader geoad:MapSeries ;skos:notation "7341" ;skos:prefLabel "Bransby:7341"@en .
geoad:Pitteroo7441 a skos:Concept ;skos:definition "Map sheet for Pitteroo at 1:100 000 scale. The first two digits define a longitude band 0.5 degree wide and the second two digits a latitude band 0.5 degree wide."@en ;skos:inScheme <https://linked.data.gov.au/def/geoadminfeatures> ;skos:broader geoad:MapSeries ;skos:notation "7441" ;skos:prefLabel "Pitteroo:7441"@en .
geoad:Thuringowa7541 a skos:Concept ;skos:definition "Map sheet for Thuringowa at 1:100 000 scale. The first two digits define a longitude band 0.5 degree wide and the second two digits a latitude band 0.5 degree wide."@en ;skos:inScheme <https://linked.data.gov.au/def/geoadminfeatures> ;skos:broader geoad:MapSeries ;skos:notation "7541" ;skos:prefLabel "Thuringowa:7541"@en .
geoad:NooyeahDowns7641 a skos:Concept ;skos:definition "Map sheet for Nooyeah Downs at 1:100 000 scale. The first two digits define a longitude band 0.5 degree wide and the second two digits a latitude band 0.5 degree wide."@en ;skos:inScheme <https://linked.data.gov.au/def/geoadminfeatures> ;skos:broader geoad:MapSeries ;skos:notation "7641" ;skos:prefLabel "Nooyeah Downs:7641"@en .
geoad:DynevorDowns7741 a skos:Concept ;skos:definition "Map sheet for Dynevor Downs at 1:100 000 scale. The first two digits define a longitude band 0.5 degree wide and the second two digits a latitude band 0.5 degree wide."@en ;skos:inScheme <https://linked.data.gov.au/def/geoadminfeatures> ;skos:broader geoad:MapSeries ;skos:notation "7741" ;skos:prefLabel "Dynevor Downs:7741"@en .
geoad:Yowah7841 a skos:Concept ;skos:definition "Map sheet for Yowah at 1:100 000 scale. The first two digits define a longitude band 0.5 degree wide and the second two digits a latitude band 0.5 degree wide."@en ;skos:inScheme <https://linked.data.gov.au/def/geoadminfeatures> ;skos:broader geoad:MapSeries ;skos:notation "7841" ;skos:prefLabel "Yowah:7841"@en .
geoad:Eulo7941 a skos:Concept ;skos:definition "Map sheet for Eulo at 1:100 000 scale. The first two digits define a longitude band 0.5 degree wide and the second two digits a latitude band 0.5 degree wide."@en ;skos:inScheme <https://linked.data.gov.au/def/geoadminfeatures> ;skos:broader geoad:MapSeries ;skos:notation "7941" ;skos:prefLabel "Eulo:7941"@en .
geoad:Cunnamulla8041 a skos:Concept ;skos:definition "Map sheet for Cunnamulla at 1:100 000 scale. The first two digits define a longitude band 0.5 degree wide and the second two digits a latitude band 0.5 degree wide."@en ;skos:inScheme <https://linked.data.gov.au/def/geoadminfeatures> ;skos:broader geoad:MapSeries ;skos:notation "8041" ;skos:prefLabel "Cunnamulla:8041"@en .
geoad:Weelamurra8141 a skos:Concept ;skos:definition "Map sheet for Weelamurra at 1:100 000 scale. The first two digits define a longitude band 0.5 degree wide and the second two digits a latitude band 0.5 degree wide."@en ;skos:inScheme <https://linked.data.gov.au/def/geoadminfeatures> ;skos:broader geoad:MapSeries ;skos:notation "8141" ;skos:prefLabel "Weelamurra:8141"@en .
geoad:BonnaVonna8241 a skos:Concept ;skos:definition "Map sheet for Bonna Vonna at 1:100 000 scale. The first two digits define a longitude band 0.5 degree wide and the second two digits a latitude band 0.5 degree wide."@en ;skos:inScheme <https://linked.data.gov.au/def/geoadminfeatures> ;skos:broader geoad:MapSeries ;skos:notation "8241" ;skos:prefLabel "Bonna Vonna:8241"@en .
geoad:Bollon8341 a skos:Concept ;skos:definition "Map sheet for Bollon at 1:100 000 scale. The first two digits define a longitude band 0.5 degree wide and the second two digits a latitude band 0.5 degree wide."@en ;skos:inScheme <https://linked.data.gov.au/def/geoadminfeatures> ;skos:broader geoad:MapSeries ;skos:notation "8341" ;skos:prefLabel "Bollon:8341"@en .
geoad:Yamma8441 a skos:Concept ;skos:definition "Map sheet for Yamma at 1:100 000 scale. The first two digits define a longitude band 0.5 degree wide and the second two digits a latitude band 0.5 degree wide."@en ;skos:inScheme <https://linked.data.gov.au/def/geoadminfeatures> ;skos:broader geoad:MapSeries ;skos:notation "8441" ;skos:prefLabel "Yamma:8441"@en .
geoad:Whyenbah8541 a skos:Concept ;skos:definition "Map sheet for Whyenbah at 1:100 000 scale. The first two digits define a longitude band 0.5 degree wide and the second two digits a latitude band 0.5 degree wide."@en ;skos:inScheme <https://linked.data.gov.au/def/geoadminfeatures> ;skos:broader geoad:MapSeries ;skos:notation "8541" ;skos:prefLabel "Whyenbah:8541"@en .
geoad:StGeorge8641 a skos:Concept ;skos:definition "Map sheet for St George at 1:100 000 scale. The first two digits define a longitude band 0.5 degree wide and the second two digits a latitude band 0.5 degree wide."@en ;skos:inScheme <https://linked.data.gov.au/def/geoadminfeatures> ;skos:broader geoad:MapSeries ;skos:notation "8641" ;skos:prefLabel "St George:8641"@en .
geoad:Talwood8741 a skos:Concept ;skos:definition "Map sheet for Talwood at 1:100 000 scale. The first two digits define a longitude band 0.5 degree wide and the second two digits a latitude band 0.5 degree wide."@en ;skos:inScheme <https://linked.data.gov.au/def/geoadminfeatures> ;skos:broader geoad:MapSeries ;skos:notation "8741" ;skos:prefLabel "Talwood:8741"@en .
geoad:Bungunya8841 a skos:Concept ;skos:definition "Map sheet for Bungunya at 1:100 000 scale. The first two digits define a longitude band 0.5 degree wide and the second two digits a latitude band 0.5 degree wide."@en ;skos:inScheme <https://linked.data.gov.au/def/geoadminfeatures> ;skos:broader geoad:MapSeries ;skos:notation "8841" ;skos:prefLabel "Bungunya:8841"@en .
geoad:Goodar8941 a skos:Concept ;skos:definition "Map sheet for Goodar at 1:100 000 scale. The first two digits define a longitude band 0.5 degree wide and the second two digits a latitude band 0.5 degree wide."@en ;skos:inScheme <https://linked.data.gov.au/def/geoadminfeatures> ;skos:broader geoad:MapSeries ;skos:notation "8941" ;skos:prefLabel "Goodar:8941"@en .
geoad:Wyaga9041 a skos:Concept ;skos:definition "Map sheet for Wyaga at 1:100 000 scale. The first two digits define a longitude band 0.5 degree wide and the second two digits a latitude band 0.5 degree wide."@en ;skos:inScheme <https://linked.data.gov.au/def/geoadminfeatures> ;skos:broader geoad:MapSeries ;skos:notation "9041" ;skos:prefLabel "Wyaga:9041"@en .
geoad:Inglewood9141 a skos:Concept ;skos:definition "Map sheet for Inglewood at 1:100 000 scale. The first two digits define a longitude band 0.5 degree wide and the second two digits a latitude band 0.5 degree wide."@en ;skos:inScheme <https://linked.data.gov.au/def/geoadminfeatures> ;skos:broader geoad:MapSeries ;skos:notation "9141" ;skos:prefLabel "Inglewood:9141"@en .
geoad:Allora9241 a skos:Concept ;skos:definition "Map sheet for Allora at 1:100 000 scale. The first two digits define a longitude band 0.5 degree wide and the second two digits a latitude band 0.5 degree wide."@en ;skos:inScheme <https://linked.data.gov.au/def/geoadminfeatures> ;skos:broader geoad:MapSeries ;skos:notation "9241" ;skos:prefLabel "Allora:9241"@en .
geoad:Warwick9341 a skos:Concept ;skos:definition "Map sheet for Warwick at 1:100 000 scale. The first two digits define a longitude band 0.5 degree wide and the second two digits a latitude band 0.5 degree wide."@en ;skos:inScheme <https://linked.data.gov.au/def/geoadminfeatures> ;skos:broader geoad:MapSeries ;skos:notation "9341" ;skos:prefLabel "Warwick:9341"@en .
geoad:MountLindesay9441 a skos:Concept ;skos:definition "Map sheet for Mount Lindesay at 1:100 000 scale. The first two digits define a longitude band 0.5 degree wide and the second two digits a latitude band 0.5 degree wide."@en ;skos:inScheme <https://linked.data.gov.au/def/geoadminfeatures> ;skos:broader geoad:MapSeries ;skos:notation "9441" ;skos:prefLabel "Mount Lindesay:9441"@en .
geoad:Murwillumbah9541 a skos:Concept ;skos:definition "Map sheet for Murwillumbah at 1:100 000 scale. The first two digits define a longitude band 0.5 degree wide and the second two digits a latitude band 0.5 degree wide."@en ;skos:inScheme <https://linked.data.gov.au/def/geoadminfeatures> ;skos:broader geoad:MapSeries ;skos:notation "9541" ;skos:prefLabel "Murwillumbah:9541"@en .
geoad:TweedHeads9641 a skos:Concept ;skos:definition "Map sheet for Tweed Heads at 1:100 000 scale. The first two digits define a longitude band 0.5 degree wide and the second two digits a latitude band 0.5 degree wide."@en ;skos:inScheme <https://linked.data.gov.au/def/geoadminfeatures> ;skos:broader geoad:MapSeries ;skos:notation "9641" ;skos:prefLabel "Tweed Heads:9641"@en .
geoad:Palankarinna6540 a skos:Concept ;skos:definition "Map sheet for Palankarinna at 1:100 000 scale. The first two digits define a longitude band 0.5 degree wide and the second two digits a latitude band 0.5 degree wide."@en ;skos:inScheme <https://linked.data.gov.au/def/geoadminfeatures> ;skos:broader geoad:MapSeries ;skos:notation "6540" ;skos:prefLabel "Palankarinna:6540"@en .
geoad:Kopperamanna6640 a skos:Concept ;skos:definition "Map sheet for Kopperamanna at 1:100 000 scale. The first two digits define a longitude band 0.5 degree wide and the second two digits a latitude band 0.5 degree wide."@en ;skos:inScheme <https://linked.data.gov.au/def/geoadminfeatures> ;skos:broader geoad:MapSeries ;skos:notation "6640" ;skos:prefLabel "Kopperamanna:6640"@en .
geoad:Gregory6740 a skos:Concept ;skos:definition "Map sheet for Gregory at 1:100 000 scale. The first two digits define a longitude band 0.5 degree wide and the second two digits a latitude band 0.5 degree wide."@en ;skos:inScheme <https://linked.data.gov.au/def/geoadminfeatures> ;skos:broader geoad:MapSeries ;skos:notation "6740" ;skos:prefLabel "Gregory:6740"@en .
geoad:Boxwood6840 a skos:Concept ;skos:definition "Map sheet for Boxwood at 1:100 000 scale. The first two digits define a longitude band 0.5 degree wide and the second two digits a latitude band 0.5 degree wide."@en ;skos:inScheme <https://linked.data.gov.au/def/geoadminfeatures> ;skos:broader geoad:MapSeries ;skos:notation "6840" ;skos:prefLabel "Boxwood:6840"@en .
geoad:TingaTingana6940 a skos:Concept ;skos:definition "Map sheet for Tinga Tingana at 1:100 000 scale. The first two digits define a longitude band 0.5 degree wide and the second two digits a latitude band 0.5 degree wide."@en ;skos:inScheme <https://linked.data.gov.au/def/geoadminfeatures> ;skos:broader geoad:MapSeries ;skos:notation "6940" ;skos:prefLabel "Tinga Tingana:6940"@en .
geoad:Bollard7040 a skos:Concept ;skos:definition "Map sheet for Bollard at 1:100 000 scale. The first two digits define a longitude band 0.5 degree wide and the second two digits a latitude band 0.5 degree wide."@en ;skos:inScheme <https://linked.data.gov.au/def/geoadminfeatures> ;skos:broader geoad:MapSeries ;skos:notation "7040" ;skos:prefLabel "Bollard:7040"@en .
geoad:Tualta7140 a skos:Concept ;skos:definition "Map sheet for Tualta at 1:100 000 scale. The first two digits define a longitude band 0.5 degree wide and the second two digits a latitude band 0.5 degree wide."@en ;skos:inScheme <https://linked.data.gov.au/def/geoadminfeatures> ;skos:broader geoad:MapSeries ;skos:notation "7140" ;skos:prefLabel "Tualta:7140"@en .
geoad:Naryilco7240 a skos:Concept ;skos:definition "Map sheet for Naryilco at 1:100 000 scale. The first two digits define a longitude band 0.5 degree wide and the second two digits a latitude band 0.5 degree wide."@en ;skos:inScheme <https://linked.data.gov.au/def/geoadminfeatures> ;skos:broader geoad:MapSeries ;skos:notation "7240" ;skos:prefLabel "Naryilco:7240"@en .
geoad:Tickalara7340 a skos:Concept ;skos:definition "Map sheet for Tickalara at 1:100 000 scale. The first two digits define a longitude band 0.5 degree wide and the second two digits a latitude band 0.5 degree wide."@en ;skos:inScheme <https://linked.data.gov.au/def/geoadminfeatures> ;skos:broader geoad:MapSeries ;skos:notation "7340" ;skos:prefLabel "Tickalara:7340"@en .
geoad:Bulloo7440 a skos:Concept ;skos:definition "Map sheet for Bulloo at 1:100 000 scale. The first two digits define a longitude band 0.5 degree wide and the second two digits a latitude band 0.5 degree wide."@en ;skos:inScheme <https://linked.data.gov.au/def/geoadminfeatures> ;skos:broader geoad:MapSeries ;skos:notation "7440" ;skos:prefLabel "Bulloo:7440"@en .
geoad:TitherooCreek7540 a skos:Concept ;skos:definition "Map sheet for Titheroo Creek at 1:100 000 scale. The first two digits define a longitude band 0.5 degree wide and the second two digits a latitude band 0.5 degree wide."@en ;skos:inScheme <https://linked.data.gov.au/def/geoadminfeatures> ;skos:broader geoad:MapSeries ;skos:notation "7540" ;skos:prefLabel "Titheroo Creek:7540"@en .
geoad:Kilcowera7640 a skos:Concept ;skos:definition "Map sheet for Kilcowera at 1:100 000 scale. The first two digits define a longitude band 0.5 degree wide and the second two digits a latitude band 0.5 degree wide."@en ;skos:inScheme <https://linked.data.gov.au/def/geoadminfeatures> ;skos:broader geoad:MapSeries ;skos:notation "7640" ;skos:prefLabel "Kilcowera:7640"@en .
geoad:Hungerford7740 a skos:Concept ;skos:definition "Map sheet for Hungerford at 1:100 000 scale. The first two digits define a longitude band 0.5 degree wide and the second two digits a latitude band 0.5 degree wide."@en ;skos:inScheme <https://linked.data.gov.au/def/geoadminfeatures> ;skos:broader geoad:MapSeries ;skos:notation "7740" ;skos:prefLabel "Hungerford:7740"@en .
geoad:Caiwarro7840 a skos:Concept ;skos:definition "Map sheet for Caiwarro at 1:100 000 scale. The first two digits define a longitude band 0.5 degree wide and the second two digits a latitude band 0.5 degree wide."@en ;skos:inScheme <https://linked.data.gov.au/def/geoadminfeatures> ;skos:broader geoad:MapSeries ;skos:notation "7840" ;skos:prefLabel "Caiwarro:7840"@en .
geoad:Kungie7940 a skos:Concept ;skos:definition "Map sheet for Kungie at 1:100 000 scale. The first two digits define a longitude band 0.5 degree wide and the second two digits a latitude band 0.5 degree wide."@en ;skos:inScheme <https://linked.data.gov.au/def/geoadminfeatures> ;skos:broader geoad:MapSeries ;skos:notation "7940" ;skos:prefLabel "Kungie:7940"@en .
geoad:Tuen8040 a skos:Concept ;skos:definition "Map sheet for Tuen at 1:100 000 scale. The first two digits define a longitude band 0.5 degree wide and the second two digits a latitude band 0.5 degree wide."@en ;skos:inScheme <https://linked.data.gov.au/def/geoadminfeatures> ;skos:broader geoad:MapSeries ;skos:notation "8040" ;skos:prefLabel "Tuen:8040"@en .
geoad:Noorama8140 a skos:Concept ;skos:definition "Map sheet for Noorama at 1:100 000 scale. The first two digits define a longitude band 0.5 degree wide and the second two digits a latitude band 0.5 degree wide."@en ;skos:inScheme <https://linked.data.gov.au/def/geoadminfeatures> ;skos:broader geoad:MapSeries ;skos:notation "8140" ;skos:prefLabel "Noorama:8140"@en .
geoad:Bundaleer8240 a skos:Concept ;skos:definition "Map sheet for Bundaleer at 1:100 000 scale. The first two digits define a longitude band 0.5 degree wide and the second two digits a latitude band 0.5 degree wide."@en ;skos:inScheme <https://linked.data.gov.au/def/geoadminfeatures> ;skos:broader geoad:MapSeries ;skos:notation "8240" ;skos:prefLabel "Bundaleer:8240"@en .
geoad:Coomburra8340 a skos:Concept ;skos:definition "Map sheet for Coomburra at 1:100 000 scale. The first two digits define a longitude band 0.5 degree wide and the second two digits a latitude band 0.5 degree wide."@en ;skos:inScheme <https://linked.data.gov.au/def/geoadminfeatures> ;skos:broader geoad:MapSeries ;skos:notation "8340" ;skos:prefLabel "Coomburra:8340"@en .
geoad:Hebel8440 a skos:Concept ;skos:definition "Map sheet for Hebel at 1:100 000 scale. The first two digits define a longitude band 0.5 degree wide and the second two digits a latitude band 0.5 degree wide."@en ;skos:inScheme <https://linked.data.gov.au/def/geoadminfeatures> ;skos:broader geoad:MapSeries ;skos:notation "8440" ;skos:prefLabel "Hebel:8440"@en .
geoad:Dirranbandi8540 a skos:Concept ;skos:definition "Map sheet for Dirranbandi at 1:100 000 scale. The first two digits define a longitude band 0.5 degree wide and the second two digits a latitude band 0.5 degree wide."@en ;skos:inScheme <https://linked.data.gov.au/def/geoadminfeatures> ;skos:broader geoad:MapSeries ;skos:notation "8540" ;skos:prefLabel "Dirranbandi:8540"@en .
geoad:Thallon8640 a skos:Concept ;skos:definition "Map sheet for Thallon at 1:100 000 scale. The first two digits define a longitude band 0.5 degree wide and the second two digits a latitude band 0.5 degree wide."@en ;skos:inScheme <https://linked.data.gov.au/def/geoadminfeatures> ;skos:broader geoad:MapSeries ;skos:notation "8640" ;skos:prefLabel "Thallon:8640"@en .
geoad:Burrenbar8740 a skos:Concept ;skos:definition "Map sheet for Burrenbar at 1:100 000 scale. The first two digits define a longitude band 0.5 degree wide and the second two digits a latitude band 0.5 degree wide."@en ;skos:inScheme <https://linked.data.gov.au/def/geoadminfeatures> ;skos:broader geoad:MapSeries ;skos:notation "8740" ;skos:prefLabel "Burrenbar:8740"@en .
geoad:Boomi8840 a skos:Concept ;skos:definition "Map sheet for Boomi at 1:100 000 scale. The first two digits define a longitude band 0.5 degree wide and the second two digits a latitude band 0.5 degree wide."@en ;skos:inScheme <https://linked.data.gov.au/def/geoadminfeatures> ;skos:broader geoad:MapSeries ;skos:notation "8840" ;skos:prefLabel "Boomi:8840"@en .
geoad:Goondiwindi8940 a skos:Concept ;skos:definition "Map sheet for Goondiwindi at 1:100 000 scale. The first two digits define a longitude band 0.5 degree wide and the second two digits a latitude band 0.5 degree wide."@en ;skos:inScheme <https://linked.data.gov.au/def/geoadminfeatures> ;skos:broader geoad:MapSeries ;skos:notation "8940" ;skos:prefLabel "Goondiwindi:8940"@en .
geoad:Yetman9040 a skos:Concept ;skos:definition "Map sheet for Yetman at 1:100 000 scale. The first two digits define a longitude band 0.5 degree wide and the second two digits a latitude band 0.5 degree wide."@en ;skos:inScheme <https://linked.data.gov.au/def/geoadminfeatures> ;skos:broader geoad:MapSeries ;skos:notation "9040" ;skos:prefLabel "Yetman:9040"@en .
geoad:Texas9140 a skos:Concept ;skos:definition "Map sheet for Texas at 1:100 000 scale. The first two digits define a longitude band 0.5 degree wide and the second two digits a latitude band 0.5 degree wide."@en ;skos:inScheme <https://linked.data.gov.au/def/geoadminfeatures> ;skos:broader geoad:MapSeries ;skos:notation "9140" ;skos:prefLabel "Texas:9140"@en .
geoad:Stanthorpe9240 a skos:Concept ;skos:definition "Map sheet for Stanthorpe at 1:100 000 scale. The first two digits define a longitude band 0.5 degree wide and the second two digits a latitude band 0.5 degree wide."@en ;skos:inScheme <https://linked.data.gov.au/def/geoadminfeatures> ;skos:broader geoad:MapSeries ;skos:notation "9240" ;skos:prefLabel "Stanthorpe:9240"@en .
geoad:Drake9340 a skos:Concept ;skos:definition "Map sheet for Drake at 1:100 000 scale. The first two digits define a longitude band 0.5 degree wide and the second two digits a latitude band 0.5 degree wide."@en ;skos:inScheme <https://linked.data.gov.au/def/geoadminfeatures> ;skos:broader geoad:MapSeries ;skos:notation "9340" ;skos:prefLabel "Drake:9340"@en .
geoad:Bonalbo9440 a skos:Concept ;skos:definition "Map sheet for Bonalbo at 1:100 000 scale. The first two digits define a longitude band 0.5 degree wide and the second two digits a latitude band 0.5 degree wide."@en ;skos:inScheme <https://linked.data.gov.au/def/geoadminfeatures> ;skos:broader geoad:MapSeries ;skos:notation "9440" ;skos:prefLabel "Bonalbo:9440"@en .
geoad:Lismore9540 a skos:Concept ;skos:definition "Map sheet for Lismore at 1:100 000 scale. The first two digits define a longitude band 0.5 degree wide and the second two digits a latitude band 0.5 degree wide."@en ;skos:inScheme <https://linked.data.gov.au/def/geoadminfeatures> ;skos:broader geoad:MapSeries ;skos:notation "9540" ;skos:prefLabel "Lismore:9540"@en .
geoad:Ballina9640 a skos:Concept ;skos:definition "Map sheet for Ballina at 1:100 000 scale. The first two digits define a longitude band 0.5 degree wide and the second two digits a latitude band 0.5 degree wide."@en ;skos:inScheme <https://linked.data.gov.au/def/geoadminfeatures> ;skos:broader geoad:MapSeries ;skos:notation "9640" ;skos:prefLabel "Ballina:9640"@en .
geoad:Clayton6539 a skos:Concept ;skos:definition "Map sheet for Clayton at 1:100 000 scale. The first two digits define a longitude band 0.5 degree wide and the second two digits a latitude band 0.5 degree wide."@en ;skos:inScheme <https://linked.data.gov.au/def/geoadminfeatures> ;skos:broader geoad:MapSeries ;skos:notation "6539" ;skos:prefLabel "Clayton:6539"@en .
geoad:Cooryanna6639 a skos:Concept ;skos:definition "Map sheet for Cooryanna at 1:100 000 scale. The first two digits define a longitude band 0.5 degree wide and the second two digits a latitude band 0.5 degree wide."@en ;skos:inScheme <https://linked.data.gov.au/def/geoadminfeatures> ;skos:broader geoad:MapSeries ;skos:notation "6639" ;skos:prefLabel "Cooryanna:6639"@en .
geoad:Tooncatchyin6739 a skos:Concept ;skos:definition "Map sheet for Tooncatchyin at 1:100 000 scale. The first two digits define a longitude band 0.5 degree wide and the second two digits a latitude band 0.5 degree wide."@en ;skos:inScheme <https://linked.data.gov.au/def/geoadminfeatures> ;skos:broader geoad:MapSeries ;skos:notation "6739" ;skos:prefLabel "Tooncatchyin:6739"@en .
geoad:Montecollina6839 a skos:Concept ;skos:definition "Map sheet for Montecollina at 1:100 000 scale. The first two digits define a longitude band 0.5 degree wide and the second two digits a latitude band 0.5 degree wide."@en ;skos:inScheme <https://linked.data.gov.au/def/geoadminfeatures> ;skos:broader geoad:MapSeries ;skos:notation "6839" ;skos:prefLabel "Montecollina:6839"@en .
geoad:Artracoona6939 a skos:Concept ;skos:definition "Map sheet for Artracoona at 1:100 000 scale. The first two digits define a longitude band 0.5 degree wide and the second two digits a latitude band 0.5 degree wide."@en ;skos:inScheme <https://linked.data.gov.au/def/geoadminfeatures> ;skos:broader geoad:MapSeries ;skos:notation "6939" ;skos:prefLabel "Artracoona:6939"@en .
geoad:Burruna7039 a skos:Concept ;skos:definition "Map sheet for Burruna at 1:100 000 scale. The first two digits define a longitude band 0.5 degree wide and the second two digits a latitude band 0.5 degree wide."@en ;skos:inScheme <https://linked.data.gov.au/def/geoadminfeatures> ;skos:broader geoad:MapSeries ;skos:notation "7039" ;skos:prefLabel "Burruna:7039"@en .
geoad:FortGrey7139 a skos:Concept ;skos:definition "Map sheet for Fort Grey at 1:100 000 scale. The first two digits define a longitude band 0.5 degree wide and the second two digits a latitude band 0.5 degree wide."@en ;skos:inScheme <https://linked.data.gov.au/def/geoadminfeatures> ;skos:broader geoad:MapSeries ;skos:notation "7139" ;skos:prefLabel "Fort Grey:7139"@en .
geoad:OliveDowns7239 a skos:Concept ;skos:definition "Map sheet for Olive Downs at 1:100 000 scale. The first two digits define a longitude band 0.5 degree wide and the second two digits a latitude band 0.5 degree wide."@en ;skos:inScheme <https://linked.data.gov.au/def/geoadminfeatures> ;skos:broader geoad:MapSeries ;skos:notation "7239" ;skos:prefLabel "Olive Downs:7239"@en .
geoad:Tibooburra7339 a skos:Concept ;skos:definition "Map sheet for Tibooburra at 1:100 000 scale. The first two digits define a longitude band 0.5 degree wide and the second two digits a latitude band 0.5 degree wide."@en ;skos:inScheme <https://linked.data.gov.au/def/geoadminfeatures> ;skos:broader geoad:MapSeries ;skos:notation "7339" ;skos:prefLabel "Tibooburra:7339"@en .
geoad:Tongowoko7439 a skos:Concept ;skos:definition "Map sheet for Tongowoko at 1:100 000 scale. The first two digits define a longitude band 0.5 degree wide and the second two digits a latitude band 0.5 degree wide."@en ;skos:inScheme <https://linked.data.gov.au/def/geoadminfeatures> ;skos:broader geoad:MapSeries ;skos:notation "7439" ;skos:prefLabel "Tongowoko:7439"@en .
geoad:ThurlooDowns7539 a skos:Concept ;skos:definition "Map sheet for Thurloo Downs at 1:100 000 scale. The first two digits define a longitude band 0.5 degree wide and the second two digits a latitude band 0.5 degree wide."@en ;skos:inScheme <https://linked.data.gov.au/def/geoadminfeatures> ;skos:broader geoad:MapSeries ;skos:notation "7539" ;skos:prefLabel "Thurloo Downs:7539"@en .
geoad:BerawinniaDowns7639 a skos:Concept ;skos:definition "Map sheet for Berawinnia Downs at 1:100 000 scale. The first two digits define a longitude band 0.5 degree wide and the second two digits a latitude band 0.5 degree wide."@en ;skos:inScheme <https://linked.data.gov.au/def/geoadminfeatures> ;skos:broader geoad:MapSeries ;skos:notation "7639" ;skos:prefLabel "Berawinnia Downs:7639"@en .
geoad:Talyealye7739 a skos:Concept ;skos:definition "Map sheet for Talyealye at 1:100 000 scale. The first two digits define a longitude band 0.5 degree wide and the second two digits a latitude band 0.5 degree wide."@en ;skos:inScheme <https://linked.data.gov.au/def/geoadminfeatures> ;skos:broader geoad:MapSeries ;skos:notation "7739" ;skos:prefLabel "Talyealye:7739"@en .
geoad:Brindingabba7839 a skos:Concept ;skos:definition "Map sheet for Brindingabba at 1:100 000 scale. The first two digits define a longitude band 0.5 degree wide and the second two digits a latitude band 0.5 degree wide."@en ;skos:inScheme <https://linked.data.gov.au/def/geoadminfeatures> ;skos:broader geoad:MapSeries ;skos:notation "7839" ;skos:prefLabel "Brindingabba:7839"@en .
geoad:Yaniabulla7939 a skos:Concept ;skos:definition "Map sheet for Yaniabulla at 1:100 000 scale. The first two digits define a longitude band 0.5 degree wide and the second two digits a latitude band 0.5 degree wide."@en ;skos:inScheme <https://linked.data.gov.au/def/geoadminfeatures> ;skos:broader geoad:MapSeries ;skos:notation "7939" ;skos:prefLabel "Yaniabulla:7939"@en .
geoad:Enngonia8039 a skos:Concept ;skos:definition "Map sheet for Enngonia at 1:100 000 scale. The first two digits define a longitude band 0.5 degree wide and the second two digits a latitude band 0.5 degree wide."@en ;skos:inScheme <https://linked.data.gov.au/def/geoadminfeatures> ;skos:broader geoad:MapSeries ;skos:notation "8039" ;skos:prefLabel "Enngonia:8039"@en .
geoad:Gerara8139 a skos:Concept ;skos:definition "Map sheet for Gerara at 1:100 000 scale. The first two digits define a longitude band 0.5 degree wide and the second two digits a latitude band 0.5 degree wide."@en ;skos:inScheme <https://linked.data.gov.au/def/geoadminfeatures> ;skos:broader geoad:MapSeries ;skos:notation "8139" ;skos:prefLabel "Gerara:8139"@en .
geoad:Weilmoringle8239 a skos:Concept ;skos:definition "Map sheet for Weilmoringle at 1:100 000 scale. The first two digits define a longitude band 0.5 degree wide and the second two digits a latitude band 0.5 degree wide."@en ;skos:inScheme <https://linked.data.gov.au/def/geoadminfeatures> ;skos:broader geoad:MapSeries ;skos:notation "8239" ;skos:prefLabel "Weilmoringle:8239"@en .
geoad:Goodooga8339 a skos:Concept ;skos:definition "Map sheet for Goodooga at 1:100 000 scale. The first two digits define a longitude band 0.5 degree wide and the second two digits a latitude band 0.5 degree wide."@en ;skos:inScheme <https://linked.data.gov.au/def/geoadminfeatures> ;skos:broader geoad:MapSeries ;skos:notation "8339" ;skos:prefLabel "Goodooga:8339"@en .
geoad:LightningRidge8439 a skos:Concept ;skos:definition "Map sheet for Lightning Ridge at 1:100 000 scale. The first two digits define a longitude band 0.5 degree wide and the second two digits a latitude band 0.5 degree wide."@en ;skos:inScheme <https://linked.data.gov.au/def/geoadminfeatures> ;skos:broader geoad:MapSeries ;skos:notation "8439" ;skos:prefLabel "Lightning Ridge:8439"@en .
geoad:Dunumbral8539 a skos:Concept ;skos:definition "Map sheet for Dunumbral at 1:100 000 scale. The first two digits define a longitude band 0.5 degree wide and the second two digits a latitude band 0.5 degree wide."@en ;skos:inScheme <https://linked.data.gov.au/def/geoadminfeatures> ;skos:broader geoad:MapSeries ;skos:notation "8539" ;skos:prefLabel "Dunumbral:8539"@en .
geoad:MogilMogil8639 a skos:Concept ;skos:definition "Map sheet for Mogil Mogil at 1:100 000 scale. The first two digits define a longitude band 0.5 degree wide and the second two digits a latitude band 0.5 degree wide."@en ;skos:inScheme <https://linked.data.gov.au/def/geoadminfeatures> ;skos:broader geoad:MapSeries ;skos:notation "8639" ;skos:prefLabel "Mogil Mogil:8639"@en .
geoad:Bunarba8739 a skos:Concept ;skos:definition "Map sheet for Bunarba at 1:100 000 scale. The first two digits define a longitude band 0.5 degree wide and the second two digits a latitude band 0.5 degree wide."@en ;skos:inScheme <https://linked.data.gov.au/def/geoadminfeatures> ;skos:broader geoad:MapSeries ;skos:notation "8739" ;skos:prefLabel "Bunarba:8739"@en .
geoad:Moree8839 a skos:Concept ;skos:definition "Map sheet for Moree at 1:100 000 scale. The first two digits define a longitude band 0.5 degree wide and the second two digits a latitude band 0.5 degree wide."@en ;skos:inScheme <https://linked.data.gov.au/def/geoadminfeatures> ;skos:broader geoad:MapSeries ;skos:notation "8839" ;skos:prefLabel "Moree:8839"@en .
geoad:CroppaCreek8939 a skos:Concept ;skos:definition "Map sheet for Croppa Creek at 1:100 000 scale. The first two digits define a longitude band 0.5 degree wide and the second two digits a latitude band 0.5 degree wide."@en ;skos:inScheme <https://linked.data.gov.au/def/geoadminfeatures> ;skos:broader geoad:MapSeries ;skos:notation "8939" ;skos:prefLabel "Croppa Creek:8939"@en .
geoad:Yallaroi9039 a skos:Concept ;skos:definition "Map sheet for Yallaroi at 1:100 000 scale. The first two digits define a longitude band 0.5 degree wide and the second two digits a latitude band 0.5 degree wide."@en ;skos:inScheme <https://linked.data.gov.au/def/geoadminfeatures> ;skos:broader geoad:MapSeries ;skos:notation "9039" ;skos:prefLabel "Yallaroi:9039"@en .
geoad:Ashford9139 a skos:Concept ;skos:definition "Map sheet for Ashford at 1:100 000 scale. The first two digits define a longitude band 0.5 degree wide and the second two digits a latitude band 0.5 degree wide."@en ;skos:inScheme <https://linked.data.gov.au/def/geoadminfeatures> ;skos:broader geoad:MapSeries ;skos:notation "9139" ;skos:prefLabel "Ashford:9139"@en .
geoad:Clive9239 a skos:Concept ;skos:definition "Map sheet for Clive at 1:100 000 scale. The first two digits define a longitude band 0.5 degree wide and the second two digits a latitude band 0.5 degree wide."@en ;skos:inScheme <https://linked.data.gov.au/def/geoadminfeatures> ;skos:broader geoad:MapSeries ;skos:notation "9239" ;skos:prefLabel "Clive:9239"@en .
geoad:Tenterfield9339 a skos:Concept ;skos:definition "Map sheet for Tenterfield at 1:100 000 scale. The first two digits define a longitude band 0.5 degree wide and the second two digits a latitude band 0.5 degree wide."@en ;skos:inScheme <https://linked.data.gov.au/def/geoadminfeatures> ;skos:broader geoad:MapSeries ;skos:notation "9339" ;skos:prefLabel "Tenterfield:9339"@en .
geoad:Coaldale9439 a skos:Concept ;skos:definition "Map sheet for Coaldale at 1:100 000 scale. The first two digits define a longitude band 0.5 degree wide and the second two digits a latitude band 0.5 degree wide."@en ;skos:inScheme <https://linked.data.gov.au/def/geoadminfeatures> ;skos:broader geoad:MapSeries ;skos:notation "9439" ;skos:prefLabel "Coaldale:9439"@en .
geoad:Woodburn9539 a skos:Concept ;skos:definition "Map sheet for Woodburn at 1:100 000 scale. The first two digits define a longitude band 0.5 degree wide and the second two digits a latitude band 0.5 degree wide."@en ;skos:inScheme <https://linked.data.gov.au/def/geoadminfeatures> ;skos:broader geoad:MapSeries ;skos:notation "9539" ;skos:prefLabel "Woodburn:9539"@en .
geoad:Bensbach7179 a skos:Concept ;skos:definition "Map sheet for Bensbach at 1:100 000 scale. The first two digits define a longitude band 0.5 degree wide and the second two digits a latitude band 0.5 degree wide."@en ;skos:inScheme <https://linked.data.gov.au/def/geoadminfeatures> ;skos:broader geoad:MapSeries ;skos:notation "7179" ;skos:prefLabel "Bensbach:7179"@en .
geoad:Mari7279 a skos:Concept ;skos:definition "Map sheet for Mari at 1:100 000 scale. The first two digits define a longitude band 0.5 degree wide and the second two digits a latitude band 0.5 degree wide."@en ;skos:inScheme <https://linked.data.gov.au/def/geoadminfeatures> ;skos:broader geoad:MapSeries ;skos:notation "7279" ;skos:prefLabel "Mari:7279"@en .
geoad:Saibai7479 a skos:Concept ;skos:definition "Map sheet for Saibai at 1:100 000 scale. The first two digits define a longitude band 0.5 degree wide and the second two digits a latitude band 0.5 degree wide."@en ;skos:inScheme <https://linked.data.gov.au/def/geoadminfeatures> ;skos:broader geoad:MapSeries ;skos:notation "7479" ;skos:prefLabel "Saibai:7479"@en .
geoad:Boigu7379 a skos:Concept ;skos:definition "Map sheet for Boigu at 1:100 000 scale. The first two digits define a longitude band 0.5 degree wide and the second two digits a latitude band 0.5 degree wide."@en ;skos:inScheme <https://linked.data.gov.au/def/geoadminfeatures> ;skos:broader geoad:MapSeries ;skos:notation "7379" ;skos:prefLabel "Boigu:7379"@en .
geoad:Daru7579 a skos:Concept ;skos:definition "Map sheet for Daru at 1:100 000 scale. The first two digits define a longitude band 0.5 degree wide and the second two digits a latitude band 0.5 degree wide."@en ;skos:inScheme <https://linked.data.gov.au/def/geoadminfeatures> ;skos:broader geoad:MapSeries ;skos:notation "7579" ;skos:prefLabel "Daru:7579"@en .
geoad:OffshoreMap7277 a skos:Concept ;skos:definition "Map sheet for Offshore Map at 1:100 000 scale. The first two digits define a longitude band 0.5 degree wide and the second two digits a latitude band 0.5 degree wide."@en ;skos:inScheme <https://linked.data.gov.au/def/geoadminfeatures> ;skos:broader geoad:MapSeries ;skos:notation "7277" ;skos:prefLabel "Offshore Map:7277"@en .
geoad:OffshoreMap7673 a skos:Concept ;skos:definition "Map sheet for Offshore Map at 1:100 000 scale. The first two digits define a longitude band 0.5 degree wide and the second two digits a latitude band 0.5 degree wide."@en ;skos:inScheme <https://linked.data.gov.au/def/geoadminfeatures> ;skos:broader geoad:MapSeries ;skos:notation "7673" ;skos:prefLabel "Offshore Map:7673"@en .
geoad:OffshoreMap7674 a skos:Concept ;skos:definition "Map sheet for Offshore Map at 1:100 000 scale. The first two digits define a longitude band 0.5 degree wide and the second two digits a latitude band 0.5 degree wide."@en ;skos:inScheme <https://linked.data.gov.au/def/geoadminfeatures> ;skos:broader geoad:MapSeries ;skos:notation "7674" ;skos:prefLabel "Offshore Map:7674"@en .
geoad:OffshoreMap7675 a skos:Concept ;skos:definition "Map sheet for Offshore Map at 1:100 000 scale. The first two digits define a longitude band 0.5 degree wide and the second two digits a latitude band 0.5 degree wide."@en ;skos:inScheme <https://linked.data.gov.au/def/geoadminfeatures> ;skos:broader geoad:MapSeries ;skos:notation "7675" ;skos:prefLabel "Offshore Map:7675"@en .
geoad:OffshoreMap7676 a skos:Concept ;skos:definition "Map sheet for Offshore Map at 1:100 000 scale. The first two digits define a longitude band 0.5 degree wide and the second two digits a latitude band 0.5 degree wide."@en ;skos:inScheme <https://linked.data.gov.au/def/geoadminfeatures> ;skos:broader geoad:MapSeries ;skos:notation "7676" ;skos:prefLabel "Offshore Map:7676"@en .
geoad:OffshoreMap7677 a skos:Concept ;skos:definition "Map sheet for Offshore Map at 1:100 000 scale. The first two digits define a longitude band 0.5 degree wide and the second two digits a latitude band 0.5 degree wide."@en ;skos:inScheme <https://linked.data.gov.au/def/geoadminfeatures> ;skos:broader geoad:MapSeries ;skos:notation "7677" ;skos:prefLabel "Offshore Map:7677"@en .
geoad:OffshoreMap7770 a skos:Concept ;skos:definition "Map sheet for Offshore Map at 1:100 000 scale. The first two digits define a longitude band 0.5 degree wide and the second two digits a latitude band 0.5 degree wide."@en ;skos:inScheme <https://linked.data.gov.au/def/geoadminfeatures> ;skos:broader geoad:MapSeries ;skos:notation "7770" ;skos:prefLabel "Offshore Map:7770"@en .
geoad:OffshoreMap7771 a skos:Concept ;skos:definition "Map sheet for Offshore Map at 1:100 000 scale. The first two digits define a longitude band 0.5 degree wide and the second two digits a latitude band 0.5 degree wide."@en ;skos:inScheme <https://linked.data.gov.au/def/geoadminfeatures> ;skos:broader geoad:MapSeries ;skos:notation "7771" ;skos:prefLabel "Offshore Map:7771"@en .
geoad:OffshoreMap7773 a skos:Concept ;skos:definition "Map sheet for Offshore Map at 1:100 000 scale. The first two digits define a longitude band 0.5 degree wide and the second two digits a latitude band 0.5 degree wide."@en ;skos:inScheme <https://linked.data.gov.au/def/geoadminfeatures> ;skos:broader geoad:MapSeries ;skos:notation "7773" ;skos:prefLabel "Offshore Map:7773"@en .
geoad:OffshoreMap7774 a skos:Concept ;skos:definition "Map sheet for Offshore Map at 1:100 000 scale. The first two digits define a longitude band 0.5 degree wide and the second two digits a latitude band 0.5 degree wide."@en ;skos:inScheme <https://linked.data.gov.au/def/geoadminfeatures> ;skos:broader geoad:MapSeries ;skos:notation "7774" ;skos:prefLabel "Offshore Map:7774"@en .
geoad:OffshoreMap7775 a skos:Concept ;skos:definition "Map sheet for Offshore Map at 1:100 000 scale. The first two digits define a longitude band 0.5 degree wide and the second two digits a latitude band 0.5 degree wide."@en ;skos:inScheme <https://linked.data.gov.au/def/geoadminfeatures> ;skos:broader geoad:MapSeries ;skos:notation "7775" ;skos:prefLabel "Offshore Map:7775"@en .
geoad:OffshoreMap7777 a skos:Concept ;skos:definition "Map sheet for Offshore Map at 1:100 000 scale. The first two digits define a longitude band 0.5 degree wide and the second two digits a latitude band 0.5 degree wide."@en ;skos:inScheme <https://linked.data.gov.au/def/geoadminfeatures> ;skos:broader geoad:MapSeries ;skos:notation "7777" ;skos:prefLabel "Offshore Map:7777"@en .
geoad:OffshoreMap7779 a skos:Concept ;skos:definition "Map sheet for Offshore Map at 1:100 000 scale. The first two digits define a longitude band 0.5 degree wide and the second two digits a latitude band 0.5 degree wide."@en ;skos:inScheme <https://linked.data.gov.au/def/geoadminfeatures> ;skos:broader geoad:MapSeries ;skos:notation "7779" ;skos:prefLabel "Offshore Map:7779"@en .
geoad:OffshoreMap7870 a skos:Concept ;skos:definition "Map sheet for Offshore Map at 1:100 000 scale. The first two digits define a longitude band 0.5 degree wide and the second two digits a latitude band 0.5 degree wide."@en ;skos:inScheme <https://linked.data.gov.au/def/geoadminfeatures> ;skos:broader geoad:MapSeries ;skos:notation "7870" ;skos:prefLabel "Offshore Map:7870"@en .
geoad:OffshoreMap8068 a skos:Concept ;skos:definition "Map sheet for Offshore Map at 1:100 000 scale. The first two digits define a longitude band 0.5 degree wide and the second two digits a latitude band 0.5 degree wide."@en ;skos:inScheme <https://linked.data.gov.au/def/geoadminfeatures> ;skos:broader geoad:MapSeries ;skos:notation "8068" ;skos:prefLabel "Offshore Map:8068"@en .
geoad:OffshoreMap8956 a skos:Concept ;skos:definition "Map sheet for Offshore Map at 1:100 000 scale. The first two digits define a longitude band 0.5 degree wide and the second two digits a latitude band 0.5 degree wide."@en ;skos:inScheme <https://linked.data.gov.au/def/geoadminfeatures> ;skos:broader geoad:MapSeries ;skos:notation "8956" ;skos:prefLabel "Offshore Map:8956"@en .
geoad:OffshoreMap9448 a skos:Concept ;skos:definition "Map sheet for Offshore Map at 1:100 000 scale. The first two digits define a longitude band 0.5 degree wide and the second two digits a latitude band 0.5 degree wide."@en ;skos:inScheme <https://linked.data.gov.au/def/geoadminfeatures> ;skos:broader geoad:MapSeries ;skos:notation "9448" ;skos:prefLabel "Offshore Map:9448"@en .
