@prefix dcterms: <http://purl.org/dc/terms/> .
@prefix geof: <https://linked.data.gov.au/def/geofeatures/> .
@prefix owl: <http://www.w3.org/2002/07/owl#> .
@prefix prof: <http://www.w3.org/ns/dx/prof/> .
@prefix sdo: <https://schema.org/> .
@prefix skos: <http://www.w3.org/2004/02/skos/core#> .
@prefix rdfs: <http://www.w3.org/2000/01/rdf-schema#> .
@prefix xsd: <http://www.w3.org/2001/XMLSchema#> .

geof:AbundanceZone a skos:Concept ;
    dcterms:source <http://www.stratigraphy.org/index.php/ics-stratigraphicguide> ;
    skos:broader geof:BiostratigraphicUnit ;
    skos:definition "The body of strata in which the abundance of a particular taxon or specified group of taxa is significantly greater than is usual in the adjacent parts of the section. (ICS, Online, December 2019)"@en ;
    rdfs:isDefinedBy <https://linked.data.gov.au/def/geofeatures> ;
    skos:inScheme <https://linked.data.gov.au/def/geofeatures> ;
    skos:notation "gfabz" ;
    skos:prefLabel "abundance zone"@en .

geof:AncientContinent a skos:Concept ;
    skos:definition "A continent that has been recognised as being a distinct entity in the past and not as a supercontinent, and, is not recognised as a present-day continent, although it may form part of one or more (present-day continents). (Definition created here)"@en ;
    rdfs:isDefinedBy <https://linked.data.gov.au/def/geofeatures> ;
    skos:inScheme <https://linked.data.gov.au/def/geofeatures> ;
    skos:prefLabel "ancient continent"@en .

geof:Anticline a skos:Concept ;
    dcterms:source <http://www.glossaryofgeology.org> ;
    skos:broader geof:StructuralFeature ;
    skos:definition "A fold, generally convex upward, whose core contains the stratigraphically older rocks. (Neuendorf et al., 2011)"@en ;
    rdfs:isDefinedBy <https://linked.data.gov.au/def/geofeatures> ;
    skos:inScheme <https://linked.data.gov.au/def/geofeatures> ;
    skos:notation "gfann" ;
    skos:prefLabel "anticline"@en .

geof:Anticlinorium a skos:Concept ;
    dcterms:source <http://www.glossaryofgeology.org> ;
    skos:broader geof:StructuralFeature ;
    skos:definition "A composite anticlinal structure of regional extent composed of lesser folds. (Neuendorf et al., 2011)"@en ;
    rdfs:isDefinedBy <https://linked.data.gov.au/def/geofeatures> ;
    skos:inScheme <https://linked.data.gov.au/def/geofeatures> ;
    skos:notation "gfanm" ;
    skos:prefLabel "anticlinorium"@en .

geof:Antiform a skos:Concept ;
    dcterms:source <http://www.glossaryofgeology.org> ;
    skos:broader geof:StructuralFeature ;
    skos:definition "Any convex-upward, concave downward fold. The term is usually used when the folded layers do not possess a stratigraphic order, when the stratigraphic order of the folded layers is not known, or when the fold core also contains the stratigraphically younger rock. (Neuendorf et al., 2011)"@en ;
    rdfs:isDefinedBy <https://linked.data.gov.au/def/geofeatures> ;
    skos:inScheme <https://linked.data.gov.au/def/geofeatures> ;
    skos:notation "gfant" ;
    skos:prefLabel "antiform"@en .

geof:AntiformalStack a skos:Concept ;
    dcterms:source <http://www.glossaryofgeology.org> ;
    skos:broader geof:StructuralFeature ;
    skos:definition "A duplex in which the trailing branch lines coincide and the leading branch lines either nearly coincide or lie vertically above each other. This results in a stack of horses and leads to a local culmination in thrust sheet. (Neuendorf et al. (2011) citing Boyer & Elliott (1982))"@en ;
    rdfs:isDefinedBy <https://linked.data.gov.au/def/geofeatures> ;
    skos:inScheme <https://linked.data.gov.au/def/geofeatures> ;
    skos:notation "gfank" ;
    skos:prefLabel "antiformal stack"@en .

geof:Arch a skos:Concept ;
    dcterms:source <http://www.glossaryofgeology.org> ;
    skos:broader geof:StructuralFeature ;
    skos:definition "A broad, open anticlinal fold on a regional scale; it is usually a basement doming. (Neuendorf et al., 2011)"@en ;
    rdfs:isDefinedBy <https://linked.data.gov.au/def/geofeatures> ;
    skos:inScheme <https://linked.data.gov.au/def/geofeatures> ;
    skos:notation "gfarh" ;
    skos:prefLabel "arch"@en .

geof:AssemblageZone a skos:Concept ;
    dcterms:source <http://www.stratigraphy.org/index.php/ics-stratigraphicguide> ;
    skos:broader geof:BiostratigraphicUnit ;
    skos:definition "The body of strata characterized by an assemblage of three or more fossil taxa that, taken together, distinguishes it in biostratigraphic character from adjacent strata. (ICS, Online, December 2019)"@en ;
    rdfs:isDefinedBy <https://linked.data.gov.au/def/geofeatures> ;
    skos:inScheme <https://linked.data.gov.au/def/geofeatures> ;
    skos:notation "gfasz" ;
    skos:prefLabel "assemblage zone"@en .

geof:AssociationZone a skos:Concept ;
    dcterms:source <https://doi.org/10.1016/j.revpalbo.2014.04.002>,
        <https://doi.org/10.1080/01916122.2012.718609> ;
    skos:broader geof:BiostratigraphicUnit ;
    skos:definition "The body of strata between two designated biostratigraphical horizons, which represent the boundaries of the unit and separate it from any preceding or succeeding biozone. These bounding horizons may be delimited individually by: the level of the first stratigraphical appearance (lowermost or oldest occurrence) of a specified taxon (species, genus) in any one stratigraphical section; or another specified biostratigraphical feature considered to approximate a time horizon. The zone is further delimited by specified taxa (preferably, at least three), which have first appearances within the zone. (de Jersey & McKellar, 2013; Bomfleur et al., 2014)"@en ;
    rdfs:isDefinedBy <https://linked.data.gov.au/def/geofeatures> ;
    skos:inScheme <https://linked.data.gov.au/def/geofeatures> ;
    skos:notation "gfasn" ;
    skos:prefLabel "association zone"@en .

geof:Bed a skos:Concept ;
    dcterms:source <http://www.stratigraphy.org/index.php/ics-stratigraphicguide>,
        <https://doi.org/10.1080/08120098508729316>,
        <https://doi.org/10.1130/9780813774022> ;
    skos:broader geof:LithostratigraphicUnit ;
    skos:definition "Bed (Beds) is the smallest formal unit in the hierarchy of sedimentary lithostratigraphic units, e.g. a single stratum lithologically distinguishable from other layers above and below (Salvador, 2013; ICS Online, January 2020). Customarily, only distinctive beds (commonly known as marker beds), which are particularly useful for stratigraphic purposes, like correlation or reference, are given proper names and considered formal lithostratigraphic units (Staines, 1985)"@en ;
    rdfs:isDefinedBy <https://linked.data.gov.au/def/geofeatures> ;
    skos:inScheme <https://linked.data.gov.au/def/geofeatures> ;
    skos:notation "gfbed" ;
    skos:prefLabel "bed"@en .

geof:Beds a skos:Concept ;
    dcterms:source <https://doi.org/10.1080/08120098508729316> ;
    skos:broader geof:LithostratigraphicUnit ;
    skos:definition "beds (uncapitalised): an informal unit applied to a sequence of poorly known strata until further work is carried out, as advised in the Field Geologist’s Guide to Lithostratigraphic Nomenclature in Australia (Staines, 1985), and endorsed by the Stratigraphic Nomenclature Committee, Geological Society of Australia."@en ;
    rdfs:isDefinedBy <https://linked.data.gov.au/def/geofeatures> ;
    skos:inScheme <https://linked.data.gov.au/def/geofeatures> ;
    skos:notation "gfbds" ;
    skos:prefLabel "beds"@en .

geof:Block a skos:Concept ;
    dcterms:source <http://www.glossaryofgeology.org> ;
    skos:broader geof:StructuralFeature ;
    skos:definition "A block of the crust that has been displaced by movement on a fault. (Neuendorf et al., 2011)"@en ;
    rdfs:isDefinedBy <https://linked.data.gov.au/def/geofeatures> ;
    skos:inScheme <https://linked.data.gov.au/def/geofeatures> ;
    skos:notation "gfblk" ;
    skos:prefLabel "block"@en .

geof:ChronostratigraphicUnit a skos:Concept ;
    dcterms:source <http://www.stratigraphy.org/index.php/ics-stratigraphicguide>,
        <https://citeseerx.ist.psu.edu/viewdoc/summary?doi=10.1.1.605.7824>,
        <https://doi.org/10.1306/05230505015> ;
    skos:broader geof:StratigraphicUnit ;
    skos:definition """As the term implies, Chronostratigraphic Units are Time-Rock Units. They are bodies of rocks, layered or unlayered, that were formed during a specified interval of geologic time. [The units of geologic time during which chronostratigraphic units were formed are called geochronologic (geological-time) units.] (ICS, Online, December, 2019). NB: The North American Stratigraphic Code (2005) and Owen (2009) advise that geochronologic units should only be associated with "lithodemic" (i.e., non-stratigraphic) units."""@en ;
    rdfs:isDefinedBy <https://linked.data.gov.au/def/geofeatures> ;
    skos:inScheme <https://linked.data.gov.au/def/geofeatures> ;
    skos:notation "gfcht" ;
    skos:prefLabel "chronostratigraphic unit"@en .

geof:ComplexRockUnit a skos:Concept ; 
    skos:altLabel "complex unit"@en ;
    skos:altLabel "composite unit"@en ; 
    dcterms:references "After and compare: Murphy, M.A. & Salvador, A. (Editors; revised by W.E. Piller & M-P Aubry), Online: International Stratigraphic Guide — An abridged version. Accessed online 04.11.2021. <https://stratigraphy.org/guide/>"@en ;
    dcterms:references "After and compare: Salvador, A., 2013: International Stratigraphic Guide. Reprinted Second Edition, The International Union of Geological Sciences and The Geological Society of America, 214 pages. <https://doi.org/10.1130/9780813774022>"@en ;
    dcterms:references "After and compare: North American Stratigraphic Code, 2005: AAPG Bulletin, 89(11), 1547–1591. <https://doi.org/10.1306/05230505015>"@en ;
    dcterms:references "After and compare: Gillespie, M.R. & Leslie, A.G., 2021: BRUCS: a new system for classifying and naming mappable rock units. Journal of the Geological Society, 178(4), jgs2020-212. <https://jgs.lyellcollection.org/content/jgs/178/4/jgs2020-212.full.pdf>"@en ;
    dcterms:references "Compare: Kumpulainen (Editor), 2017: Guide for Geological Nomenclature in Sweden. GFF, 139:1, 3-20. <https://doi.org/10.1080/11035897.2016.1178666>"@en ;
    dcterms:references "After and compare: Subcommission on Quaternary Stratigraphy — Lithodemic Stratigraphy. Accessed online 04.11.2021. <http://quaternary.stratigraphy.org/stratigraphic-guide/lithodemic-stratigraphy/>"@en ;
    dcterms:references "See usage of: Jell, P.A. (Editor), 2013: Geology of Queensland. Geological Survey of Queensland, Brisbane, 1063 pages. <https://www.business.qld.gov.au/industries/mining-energy-water/resources/geoscience-information/reports-news/geology-queensland-book-map>"@en ;
    skos:broader <http://sweetontology.net/realmGeol/GeologicFeature> ;
    skos:definition "A rock unit that embraces a mixture composed of diverse types of any genetic (sedimentary, igneous, metamorphic) class of rocks or a mixture of two or more genetic classes, and characterised by irregularly-mixed lithology or by highly-complicated structural relations (Rephrased from: Salvador, 2013; Murphy & Salvador, Online)."@en ;
    rdfs:isDefinedBy <https://linked.data.gov.au/def/geofeatures> ;
    skos:inScheme <https://linked.data.gov.au/def/geofeatures> ;
    skos:notation "gfcru" ;
    skos:scopeNote "The ISG definition is followed, with minor rewording (and without any change of meaning), although a complex unit is not here classified as a lithostratigraphic unit (as per the ISG). The NASC (2005) and Kumpulainen (2017), together with other Scandinavian guides, preferably adhere to a more specific definition, restricting a complex to a mixture of two or more genetic classes, albeit regarding a complex as a non-ranked lithodemic unit (generally, a defined, nonstratiform/non-stratified body of predominantly intrusive or highly deformed and/or highly metamorphosed rock). However, as the ISG usage better suits the nomenclature applied to some complex rock units in Queensland, it is therefore provisionally followed. A complex, although unranked in the NASC, was considered to be ‘commonly comparable to suite or supersuite’, such that two or more associated complexes could be grouped in a supersuite. This problematical application of lithodemic nomenclature was addressed by the Subcommission on Quaternary Stratigraphy with their introduction of the term ‘supercomplex’ and attendant recommendation for a two-fold hierarchy of rank for lithodemic rock units: lithodeme, suite and supersuite; and complex and supercomplex. Here, complex rock units are separated from lithostratigraphic and other single-class units (e.g., intrusive rock units) and broadly treated as stand-alone, largely nonstratiform, mixed-class units, thus reflecting the approach of Gillespie & Leslie (2021) in their construction of the British Geological Survey’s rock classification system (BRUCS). [Also, following Gillespie & Leslie, the NASC lithodemic terminology is not followed, and ‘suite’ rankings are applied solely to intrusive rock units (not also to metamorphic units)]. However, as indicated, nomenclatural usage in Queensland is not true to the more restricted definition of rock complexes comprising more than one genetic class of rocks (e.g., Jell, 2013)."@en ; 
    skos:prefLabel "complex rock unit"@en .

geof:ConcurrentRangeZone a skos:Concept ;
    dcterms:source <http://www.stratigraphy.org/index.php/ics-stratigraphicguide> ;
    skos:broader geof:BiostratigraphicUnit ;
    skos:definition "The body of strata including the overlapping parts of the range zones of two specified taxa. (ICS, Online, December 2019)"@en ;
    rdfs:isDefinedBy <https://linked.data.gov.au/def/geofeatures> ;
    skos:inScheme <https://linked.data.gov.au/def/geofeatures> ;
    skos:notation "gfcrz" ;
    skos:prefLabel "concurrent range zone"@en .

geof:Continent a skos:Concept ;
    dcterms:source <http://doi.org/10.22459/SN.08.2012>,
        <http://www.glossaryofgeology.org> ;
    skos:broader geof:TectonicFeature ;
    skos:definition "One of Earth’s major landmasses (or former major landmasses), including continental shelves. (Neuendorf et al., 2011; Blewett, 2012). The Australian Continent, as an example, is divided into fundamental geological elements embracing geological provinces."@en ;
    rdfs:isDefinedBy <https://linked.data.gov.au/def/geofeatures> ;
    skos:inScheme <https://linked.data.gov.au/def/geofeatures> ;
    skos:notation "gfcnt" ;
    skos:prefLabel "continent"@en .

geof:Craton a skos:Concept ;
    dcterms:source <http://www.glossaryofgeology.org> ;
    skos:broader geof:TectonicFeature ;
    skos:definition "A craton is part of Earth's continental crust that has attained stability and has been little deformed for a prolonged period. Cratons include shield areas, where Precambrian rocks are exposed, and platform areas, where Precambrian rocks are overlain by a thin layer of Phanerozoic strata. (Neuendorf et al., 2011)"@en ;
    rdfs:isDefinedBy <https://linked.data.gov.au/def/geofeatures> ;
    skos:inScheme <https://linked.data.gov.au/def/geofeatures> ;
    skos:notation "gfcrn" ;
    skos:prefLabel "craton"@en .

geof:CrustalElement a skos:Concept ;
    dcterms:source <http://pid.geoscience.gov.au/dataset/ga/14909> ;
    skos:broader geof:GeophysicalDomain ;
    skos:definition "Crustal Elements are geophysical domains that represent upper-crustal segments showing some overall commonality of geophysical properties, primarily magnetic and gravity data sets. Crustal elements are not geologically defined features, such as basement provinces. The latter are defined on the basis of geological criteria and are three-dimensional bodies that have a definite thickness and represent time-rock units whose maximum and minimum ages are generally, but not always, well established. Some crustal elements could represent a set of overlying or overlapping basement provinces. (Shaw et al., 1996)"@en ;
    rdfs:isDefinedBy <https://linked.data.gov.au/def/geofeatures> ;
    skos:inScheme <https://linked.data.gov.au/def/geofeatures> ;
    skos:notation "gfcrt" ;
    skos:prefLabel "crustal element"@en .

geof:Depression a skos:Concept ;
    dcterms:source <http://www.glossaryofgeology.org> ;
    skos:broader geof:StructuralFeature ;
    skos:definition "A structurally low area formed in the crust, with various mechanisms of formation. (Modified from Neuendorf et al., 2011)"@en ;
    rdfs:isDefinedBy <https://linked.data.gov.au/def/geofeatures> ;
    skos:inScheme <https://linked.data.gov.au/def/geofeatures> ;
    skos:notation "gfdpn" ;
    skos:prefLabel "depression"@en .

geof:Dome a skos:Concept ;
    dcterms:source <http://www.glossaryofgeology.org> ;
    skos:broader geof:StructuralFeature ;
    skos:definition "An uplift or anticlinal structure, either circular or elliptical in outline, in which the rocks dip gently away in all directions. A dome may be small or many kilometers in diameter. Domes include diapirs, volcanic domes, and cratonic uplifts. (Neuendorf et al., 2011)"@en ;
    rdfs:isDefinedBy <https://linked.data.gov.au/def/geofeatures> ;
    skos:inScheme <https://linked.data.gov.au/def/geofeatures> ;
    skos:notation "gfdme" ;
    skos:prefLabel "dome"@en .

geof:Duplex a skos:Concept ;
    dcterms:source <http://www.glossaryofgeology.org> ;
    skos:broader geof:StructuralFeature ;
    skos:definition "A structural complex consisting of a roof thrust at the top and a floor thrust at the base, within which a suite of more steeply dipping imbricate thrust faults thicken and shorten the intervening panel of rock (Neuendorf et al. (2011) citing Dahlstrom (1970), Boyer (1976))"@en ;
    rdfs:isDefinedBy <https://linked.data.gov.au/def/geofeatures> ;
    skos:inScheme <https://linked.data.gov.au/def/geofeatures> ;
    skos:notation "gfdpx" ;
    skos:prefLabel "duplex"@en .

geof:Embayment a skos:Concept ;
    dcterms:source <http://www.glossaryofgeology.org> ;
    skos:broader geof:StructuralFeature ;
    skos:definition "A downwarped area containing stratified rocks, either sedimentary or volcanic or both, that extends into a terrain of other rocks. (Neuendorf et al., 2011)"@en ;
    rdfs:isDefinedBy <https://linked.data.gov.au/def/geofeatures> ;
    skos:inScheme <https://linked.data.gov.au/def/geofeatures> ;
    skos:notation "gfeby" ;
    skos:prefLabel "embayment"@en .

geof:Escarpment a skos:Concept ;
    dcterms:source <http://www.glossaryofgeology.org> ;
    skos:broader geof:StructuralFeature ;
    skos:definition "(a) A long, more or less continuous cliff or relatively steep slope facing in one general direction, breaking the continuity of the land by separating two levels of gently sloping surfaces, and produced by erosion or faulting. The term is often used synonymously with scarp, although escarpment is more often applied to a cliff formed by differential erosion;  (b) A steep, abrupt face of rock, often presented by the highest strata in a line of cliffs, and generally marking the outcrop of a resistant layer occurring in a series of gently dipping softer strata, specifically the steep face of a cuesta; (c) A term used loosely in Great Britain as a synonym of cuesta. (Neuendorf et al., 2011)"@en ;
    rdfs:isDefinedBy <https://linked.data.gov.au/def/geofeatures> ;
    skos:inScheme <https://linked.data.gov.au/def/geofeatures> ;
    skos:notation "gfecp" ;
    skos:prefLabel "escarpment"@en .

geof:ExtendedCrustProvince a skos:Concept ;
    dcterms:source <https://earthquake.usgs.gov/data/crust/definitions.html> ;
    skos:broader geof:TectonicFeature ;
    skos:definition "A province of thinned crust (>50 %) due to extension (e.g., the Basin and Range Province of the Western United States and northwestern Mexico."@en ;
    rdfs:isDefinedBy <https://linked.data.gov.au/def/geofeatures> ;
    skos:inScheme <https://linked.data.gov.au/def/geofeatures> ;
    skos:notation "gfxcp" ;
    skos:prefLabel "extended crust province"@en .

geof:Fault a skos:Concept ;
    dcterms:source <http://www.glossaryofgeology.org> ;
    skos:broader geof:StructuralFeature ;
    skos:definition "A discrete surface or zone of discrete surfaces separating two rock masses across which one mass has slid past the other. (Neuendorf et al., 2011)"@en ;
    rdfs:isDefinedBy <https://linked.data.gov.au/def/geofeatures> ;
    skos:inScheme <https://linked.data.gov.au/def/geofeatures> ;
    skos:notation "gfflt" ;
    skos:prefLabel "fault"@en .

geof:FaultScarp a skos:Concept ;
    dcterms:source <http://www.glossaryofgeology.org> ;
    skos:broader geof:StructuralFeature ;
    skos:definition "(a) A steep slope or cliff formed directly by movement along a fault and representing the exposed surface of the fault before modification by erosion and weathering. It is an initial landform; (b) A term used loosely in England for any scarp that is due to the presence of a fault, even though the relief may be erosional. (Neuendorf et al., 2011)"@en ;
    rdfs:isDefinedBy <https://linked.data.gov.au/def/geofeatures> ;
    skos:inScheme <https://linked.data.gov.au/def/geofeatures> ;
    skos:notation "gfflp" ;
    skos:prefLabel "fault scarp"@en .

geof:FaultSet a skos:Concept ;
    dcterms:source <http://www.glossaryofgeology.org> ;
    skos:broader geof:StructuralFeature ;
    skos:definition "A group of faults that are parallel or nearly so, and that are related to a particular deformational episode. (Neuendorf et al., 2011)"@en ;
    rdfs:isDefinedBy <https://linked.data.gov.au/def/geofeatures> ;
    skos:inScheme <https://linked.data.gov.au/def/geofeatures> ;
    skos:notation "gffts" ;
    skos:prefLabel "fault set"@en .

geof:FaultSystem a skos:Concept ;
    dcterms:source <http://www.glossaryofgeology.org> ;
    skos:broader geof:StructuralFeature ;
    skos:definition "(a) An array of interconnected and kinematically related faults; (b) Two or more geometrically related fault sets, e.g., a conjugate fault system. (Neuendorf et al., 2011)"@en ;
    rdfs:isDefinedBy <https://linked.data.gov.au/def/geofeatures> ;
    skos:inScheme <https://linked.data.gov.au/def/geofeatures> ;
    skos:notation "gfflm" ;
    skos:prefLabel "fault system"@en .

geof:FaultZone a skos:Concept ;
    dcterms:source <http://www.glossaryofgeology.org> ;
    skos:broader geof:StructuralFeature ;
    skos:definition "A fault that is expressed as a zone of numerous small fractures, breccia, and/or fault gouge. A fault zone may be as wide as hundreds of meters. (Neuendorf et al., 2011)"@en ;
    rdfs:isDefinedBy <https://linked.data.gov.au/def/geofeatures> ;
    skos:inScheme <https://linked.data.gov.au/def/geofeatures> ;
    skos:notation "gfflz" ;
    skos:prefLabel "fault zone"@en .

geof:Flow a skos:Concept ;
    dcterms:source <http://www.stratigraphy.org/index.php/ics-stratigraphicguide> ;
    skos:broader geof:LithostratigraphicUnit ;
    skos:definition "A discrete extrusive volcanic body distinguishable by texture, composition, or other objective criteria. (ICS, Online, December 2019)"@en ;
    rdfs:isDefinedBy <https://linked.data.gov.au/def/geofeatures> ;
    skos:inScheme <https://linked.data.gov.au/def/geofeatures> ;
    skos:notation "gfflw" ;
    skos:prefLabel "flow"@en .

geof:Fold a skos:Concept ;
    dcterms:source <http://www.glossaryofgeology.org> ;
    skos:broader geof:StructuralFeature ;
    skos:definition "A curve or bend of a planar structure, such as rock strata, bedding planes, foliation or cleavage. A fold is usually the product of deformation, involving the compression of strata, but may include primary structures, as its definition is descriptive, not genetic. (Neuendorf et al., 2011)"@en ;
    rdfs:isDefinedBy <https://linked.data.gov.au/def/geofeatures> ;
    skos:inScheme <https://linked.data.gov.au/def/geofeatures> ;
    skos:notation "gffld" ;
    skos:prefLabel "fold"@en .

geof:FoldBelt a skos:Concept ;
    dcterms:source <http://www.glossaryofgeology.org>,
        <https://doi.org/10.1093/acref/9780199653065.001.0001> ;
    skos:broader geof:StructuralFeature ;
    skos:definition "A region in Earth’s lithosphere characterised by compressional tectonics, involving folding (usually parellel) and thrusting (both causing crustal shortening). Fold belts generally develop in the foreland bordering an ogogenic zone that was initiated by convergence between two tectonic plates or major crustal blocks. (Modified from: Neuendorf et al., 2011; Allaby, 2013 (Oxford Dictionary of Geology and Earth Sciences))"@en ;
    rdfs:isDefinedBy <https://linked.data.gov.au/def/geofeatures> ;
    skos:inScheme <https://linked.data.gov.au/def/geofeatures> ;
    skos:notation "gffdb" ;
    skos:prefLabel "fold belt"@en .

geof:Formation a skos:Concept ;
    dcterms:source <http://www.stratigraphy.org/index.php/ics-stratigraphicguide> ;
    skos:broader geof:LithostratigraphicUnit ;
    skos:definition "The primary formal unit of lithostratigraphic classification. Formations are the only formal lithostratigraphic units into which the stratigraphic column everywhere should be divided completely on the basis of lithology. (ICS, Online, December 2019)"@en ;
    rdfs:isDefinedBy <https://linked.data.gov.au/def/geofeatures> ;
    skos:inScheme <https://linked.data.gov.au/def/geofeatures> ;
    skos:notation "gffrm" ;
    skos:prefLabel "formation"@en .

geof:GeoResourceAccumulation a skos:Concept ;
    skos:definition "Georesource accumulations are naturally occurring masses, volumes or concentrations of geological materials that have existing or potential economic value. These resources may include, but are not limited to, minerals (including coal), hydrocarbons, quarry resources and groundwater."@en ;
    rdfs:isDefinedBy <https://linked.data.gov.au/def/geofeatures> ;
    skos:inScheme <https://linked.data.gov.au/def/geofeatures> ;
    skos:prefLabel "georesource accumulation"@en .

geof:GeologicalHeritageSite a skos:Concept ;
    dcterms:source geof:ref01 ;
    skos:broader geof:GeologicallySignificantSite ;
    skos:definition "Geological Heritage Sites (formerly known as Geological Monuments) display geological features that are so outstanding or so rare that they form part of our natural heritage, requiring recognition, description and protection, for education, research and their geotourism potential. They show evidence of the geological processes that have occurred on Earth, and of the plants and animals that have lived on it. These sites include landforms, rock outcrops, river banks, sea cliffs and shore platforms, and are, in part, represented in road cuttings, mines, quarries and other excavations. (Geological Society of Australia)"@en ;
    rdfs:isDefinedBy <https://linked.data.gov.au/def/geofeatures> ;
    skos:inScheme <https://linked.data.gov.au/def/geofeatures> ;
    skos:notation "gfghs" ;
    skos:prefLabel "geological heritage site"@en .

geof:Geopark a skos:Concept ;
    dcterms:source <https://unesdoc.unesco.org/ark:/48223/pf0000150007> ;
    skos:broader geof:GeologicallySignificantSite ;
    skos:definition "A Geopark is a nationally protected area containing a number of geological heritage sites of particular importance, rarity or aesthetic appeal. These Earth heritage sites are part of an integrated concept of protection, education and sustainable development. (UNESCO; December 2019)"@en ;
    rdfs:isDefinedBy <https://linked.data.gov.au/def/geofeatures> ;
    skos:inScheme <https://linked.data.gov.au/def/geofeatures> ;
    skos:notation "gfgpk" ;
    skos:prefLabel "geopark"@en .

geof:Geotrail a skos:Concept ;
    dcterms:source geof:ref02 ;
    skos:broader geof:GeologicallySignificantSite ;
    skos:definition "Geotrails aim to provide a tourism experience linking an area’s geology and landscape (i.e., its geological heritage features, including mining heritage) to its biodiversity and cultural history. (Geological Society of Australia)"@en ;
    rdfs:isDefinedBy <https://linked.data.gov.au/def/geofeatures> ;
    skos:inScheme <https://linked.data.gov.au/def/geofeatures> ;
    skos:notation "gfgtl" ;
    skos:prefLabel "geotrail"@en .

geof:Graben a skos:Concept ;
    dcterms:source <http://www.glossaryofgeology.org> ;
    skos:broader geof:StructuralFeature ;
    skos:definition "An elongate trough or basin, bounded on both sides by high-angle normal faults that dip toward one another. It is a structural form that may or may not be geomorphologically expressed as a rift valley. (Neuendorf et al., 2011)"@en ;
    rdfs:isDefinedBy <https://linked.data.gov.au/def/geofeatures> ;
    skos:inScheme <https://linked.data.gov.au/def/geofeatures> ;
    skos:notation "gfgbn" ;
    skos:prefLabel "graben"@en .

geof:Group a skos:Concept ;
    dcterms:source <http://www.stratigraphy.org/index.php/ics-stratigraphicguide> ;
    skos:broader geof:LithostratigraphicUnit ;
    skos:definition "A succession of two or more contiguous or associated formations with significant and diagnostic lithologic properties in common. (ICS, Online, December 2019)"@en ;
    rdfs:isDefinedBy <https://linked.data.gov.au/def/geofeatures> ;
    skos:inScheme <https://linked.data.gov.au/def/geofeatures> ;
    skos:notation "gfgrp" ;
    skos:prefLabel "group"@en .

geof:HalfGraben a skos:Concept ;
    dcterms:source <http://www.glossaryofgeology.org> ;
    skos:broader geof:StructuralFeature ;
    skos:definition "An elongate, asymmetric trough or basin bounded on one side by a normal fault. (Neuendorf et al., 2011)"@en ;
    rdfs:isDefinedBy <https://linked.data.gov.au/def/geofeatures> ;
    skos:inScheme <https://linked.data.gov.au/def/geofeatures> ;
    skos:notation "gfhgn" ;
    skos:prefLabel "half graben"@en .

geof:Horst a skos:Concept ;
    dcterms:source <http://www.glossaryofgeology.org> ;
    skos:broader geof:StructuralFeature ;
    skos:definition "An elongate block that is bounded on both sides by normal faults that dip away from one another. It is a structural form and may or may not be expressed geomorphologically. (Neuendorf et al., 2011)"@en ;
    rdfs:isDefinedBy <https://linked.data.gov.au/def/geofeatures> ;
    skos:inScheme <https://linked.data.gov.au/def/geofeatures> ;
    skos:notation "gfhrt" ;
    skos:prefLabel "horst"@en .

geof:IgneousAssociation a skos:Concept ;
    dcterms:source "See usage of: Jell, P.A. (Editor), 2013: Geology of Queensland. Geological Survey of Queensland, Brisbane, 1063 pages. <https://www.business.qld.gov.au/industries/mining-energy-water/resources/geoscience-information/reports-news/geology-queensland-book-map>"@en ;
    skos:broader geof:TectonicFeature ;
    skos:definition "A term employed by Jell (2013: Geology of Queensland), essentially without definition, for an association of igneous rocks where their differentiation remained uncertain and the geodynamic environment of their magmatism remained not well understood. In such instances, the term replaced the previous use of igneous provinces for such ‘igneous associations’, although the latter were subdivided into the previously recognized igneous subprovinces, and not into redefined igneous sub-associations (if this is at all an issue)."@en ;
    rdfs:isDefinedBy <https://linked.data.gov.au/def/geofeatures> ;
    skos:inScheme <https://linked.data.gov.au/def/geofeatures> ;
    skos:notation "gfiga" ;
    skos:prefLabel "igneous association"@en .

geof:IgneousIntrusiveRockUnit a skos:Concept ;
    dcterms:references "After: Gillespie, M.R. & Leslie, A.G., 2021: BRUCS: a new system for classifying and naming mappable rock units. <https://jgs.lyellcollection.org/content/jgs/178/4/jgs2020-212.full.pdf>@en" ; 
    skos:broader geof:IntrusiveRockUnit ;
    skos:definition "A unit formed by the emplacement of magma which solodifies before reaching the Earth's surface (after Gillespie & Leslie, 2021)."@en ;
    rdfs:isDefinedBy <https://linked.data.gov.au/def/geofeatures> ;
    skos:inScheme <https://linked.data.gov.au/def/geofeatures> ;
    skos:notation "gfiir" ;
    skos:prefLabel "igneous intrusive rock unit"@en .

geof:IgneousProvince a skos:Concept ;
    dcterms:source <http://www.glossaryofgeology.org> ;
    skos:broader geof:TectonicFeature ;
    skos:definition "A broad area in which similar igneous rocks are considered to have been formed during the same period of (igneous) activity. (Neuendorf et al., 2011)"@en ;
    rdfs:isDefinedBy <https://linked.data.gov.au/def/geofeatures> ;
    skos:inScheme <https://linked.data.gov.au/def/geofeatures> ;
    skos:notation "gfigp" ;
    skos:prefLabel "igneous province"@en .

geof:IgneousSubprovince a skos:Concept ;
    skos:broader geof:TectonicFeature ;
    skos:definition "To be provided later, as there is an issue here with Igneous Associations and daughter subprovinces."@en ;
    rdfs:isDefinedBy <https://linked.data.gov.au/def/geofeatures> ;
    skos:inScheme <https://linked.data.gov.au/def/geofeatures> ;
    skos:notation "gfisp" ;
    skos:prefLabel "igneous subprovince"@en .

geof:Inlier a skos:Concept ;
    dcterms:source <http://www.glossaryofgeology.org> ;
    skos:broader geof:DenudationalFeature ;
    skos:definition "An area or group of rocks surrounded by younger rocks, e.g., an eroded anticlinal crest. (Neuendorf et al., 2011)"@en ;
    rdfs:isDefinedBy <https://linked.data.gov.au/def/geofeatures> ;
    skos:inScheme <https://linked.data.gov.au/def/geofeatures> ;
    skos:notation "gfinl" ;
    skos:prefLabel "inlier"@en .

geof:IntervalZone a skos:Concept ;
    dcterms:source <http://www.stratigraphy.org/index.php/ics-stratigraphicguide> ;
    skos:broader geof:BiostratigraphicUnit ;
    skos:definition "The body of fossiliferous strata between two specified biohorizons. (ICS, Online, December 2019)"@en ;
    rdfs:isDefinedBy <https://linked.data.gov.au/def/geofeatures> ;
    skos:inScheme <https://linked.data.gov.au/def/geofeatures> ;
    skos:notation "gfinz" ;
    skos:prefLabel "interval zone"@en .

geof:IntrusiveRockUnit a skos:Concept ;
    dcterms:references "This vocabulary"@en ;
    skos:broader <http://sweetontology.net/realmGeol/GeologicFeature> ;
    skos:definition "Includes: (1) Igneous intrusive rock-unit types (e.g., ranked under supersuite, suite, subsuite, etc. and, at lower rank levels, plutons, lopoliths, laccoliths, dykes, sills, etc.); and (2) Non-igneous intrusive rock-unit types (viz., salt domes, sediment-filled fractures, etc.)."@en ; 
    rdfs:isDefinedBy <https://linked.data.gov.au/def/geofeatures> ;
    skos:inScheme <https://linked.data.gov.au/def/geofeatures> ;
    skos:notation "gfiru" ;
    skos:prefLabel "intrusive rock unit"@en .
   
geof:Klippe a skos:Concept ;
    dcterms:source <http://www.glossaryofgeology.org> ;
    skos:broader geof:DenudationalFeature ;
    skos:definition "An isolated rock unit that is an erosional remnant or outlier of a nappe. Plural: klippen. (Neuendorf et al., 2011)"@en ;
    rdfs:isDefinedBy <https://linked.data.gov.au/def/geofeatures> ;
    skos:inScheme <https://linked.data.gov.au/def/geofeatures> ;
    skos:notation "gfklp" ;
    skos:prefLabel "klippe"@en .

geof:LargeIgneousProvince a skos:Concept ;
    dcterms:source <http://www.glossaryofgeology.org> ;
    skos:broader geof:TectonicFeature ;
    skos:definition "A region characterized by massive crustal emplacements of predominantly mafic (Mg- and Fe-rich) extrusive and intrusive rocks which originated through processes other than \"normal\" seafloor spreading (Coffin & Eldholm, 1994); includes continental flood basalt provinces (e.g., Deccan Traps), oceanic plateaus (e.g., Ontong & Java Oceanic Plateaus), and North Atlantic volcanic passive margins. Abbrev: LIP. (Neuendorf et al., 2011)"@en ;
    rdfs:isDefinedBy <https://linked.data.gov.au/def/geofeatures> ;
    skos:inScheme <https://linked.data.gov.au/def/geofeatures> ;
    skos:notation "gflip" ;
    skos:prefLabel "large igneous province"@en .

geof:LineageZone a skos:Concept ;
    dcterms:source <http://www.stratigraphy.org/index.php/ics-stratigraphicguide> ;
    skos:broader geof:BiostratigraphicUnit ;
    skos:definition "The body of strata containing specimens representing a specific segment of an evolutionary lineage. (ICS, Online, December 2019)"@en ;
    rdfs:isDefinedBy <https://linked.data.gov.au/def/geofeatures> ;
    skos:inScheme <https://linked.data.gov.au/def/geofeatures> ;
    skos:notation "gflnz" ;
    skos:prefLabel "lineage zone"@en .

geof:MagnetostratigraphicPolaritySubzone a skos:Concept ;
    dcterms:source <http://www.stratigraphy.org/index.php/ics-stratigraphicguide>,
        <https://doi.org/10.1130/9780813774022> ;
    skos:broader geof:MagnetostratigraphicUnit ;
    skos:definition "Polarity Zones may be subdivided into Polarity Suzones. The corresponding interval of geological time during which the rocks in the Polarity Subzone were deposited is referred to as its associated Polarity Subchron. (Salvador, 2013; ICS, Online, December, 2019)"@en ;
    rdfs:isDefinedBy <https://linked.data.gov.au/def/geofeatures> ;
    skos:inScheme <https://linked.data.gov.au/def/geofeatures> ;
    skos:notation "gfmpb" ;
    skos:prefLabel "magnetostratigraphic polarity subzone"@en .

geof:MagnetostratigraphicPolaritySuperzone a skos:Concept ;
    dcterms:source <http://pid.geoscience.gov.au/dataset/ga/70149>,
        <http://www.stratigraphy.org/index.php/ics-stratigraphicguide>,
        <https://doi.org/10.1130/9780813774022> ;
    skos:broader geof:MagnetostratigraphicUnit ;
    skos:definition "Polarity Zones may be grouped into Polarity Superzones (Hyperzones in Russian literature). The corresponding interval of geological time during which the rocks in the Polarity Superzone were deposited is referred to as its associated Polarity Superchron. As an example of the latter, the mid-Carboniferous – Middle Permian Kiaman Superchron is the longest known period of predominantly reversed polarity, which was terminated by the Illawarra Geomagnetic Polarity Reversal near the base of the Capitanian. (Salvador, 2013; ICS, Online, December, 2019; Gradstein et al., 2012)"@en ;
    rdfs:isDefinedBy <https://linked.data.gov.au/def/geofeatures> ;
    skos:inScheme <https://linked.data.gov.au/def/geofeatures> ;
    skos:notation "gfmpp" ;
    skos:prefLabel "magnetostratigraphic polarity superzone"@en .

geof:MagnetostratigraphicPolarityZone a skos:Concept ;
    dcterms:source <http://www.stratigraphy.org/index.php/ics-stratigraphicguide>,
        <https://doi.org/10.1130/9780813774022> ;
    skos:broader geof:MagnetostratigraphicUnit ;
    skos:definition "The basic formal unit in magnetostratigraphic polarity classification is the Magnetostratigraphic Polarity Zone (or Polarity Zone). The corresponding interval of geological time during which the rocks in the Polarity Zone were deposited is referred to as its associated Polarity Chron. (Salvador, 2013; ICS, Online, December, 2019)"@en ;
    rdfs:isDefinedBy <https://linked.data.gov.au/def/geofeatures> ;
    skos:inScheme <https://linked.data.gov.au/def/geofeatures> ;
    skos:notation "gfmpz" ;
    skos:prefLabel "magnetostratigraphic polarity zone"@en .

geof:Member a skos:Concept ;
    dcterms:source <http://www.stratigraphy.org/index.php/ics-stratigraphicguide> ;
    skos:broader geof:LithostratigraphicUnit ;
    skos:definition "The formal lithostratigraphic unit next in rank below a formation. (ICS, Online, December 2019)"@en ;
    rdfs:isDefinedBy <https://linked.data.gov.au/def/geofeatures> ;
    skos:inScheme <https://linked.data.gov.au/def/geofeatures> ;
    skos:notation "gfmbr" ;
    skos:prefLabel "member"@en .

geof:MineralProvince a skos:Concept ;
    dcterms:source <http://www.glossaryofgeology.org> ;
    skos:broader geof:TectonicFeature ;
    skos:definition "An area characterized by a particular assemblage of mineral deposits, or by one or more characteristic types of mineralization. A metallogenic province may have had more than one episode of mineralization.  (Neuendorf et al., 2011)"@en ;
    rdfs:isDefinedBy <https://linked.data.gov.au/def/geofeatures> ;
    skos:inScheme <https://linked.data.gov.au/def/geofeatures> ;
    skos:notation "gfmnp" ;
    skos:prefLabel "mineral province"@en .

geof:Monocline a skos:Concept ;
    dcterms:source <https://doi.org/10.1093/acref/9780199653065.001.0001> ;
    skos:broader geof:StructuralFeature ;
    skos:definition "A one-limbed flexure on either side of which the strata are horizontal or dip uniformly at low angles. (Allaby, 2013)"@en ;
    rdfs:isDefinedBy <https://linked.data.gov.au/def/geofeatures> ;
    skos:inScheme <https://linked.data.gov.au/def/geofeatures> ;
    skos:notation "gfmnc" ;
    skos:prefLabel "monocline"@en .

geof:MyloniteZone a skos:Concept ;
    dcterms:source <http://www.glossaryofgeology.org>,
        <https://doi.org/10.1093/acref/9780199653065.001.0001> ;
    skos:broader geof:StructuralFeature ;
    skos:definition "Usually found in narrow, planar zones of localised ductile deformation, although kilometre-scale zones exist. Mylonites form in shear zones by mechanical grinding, crushing and recrystallization of rock to produce a metamorphic rock that has foliation and is much finer grained than its precursor. (Modified from: Neuendorf et al., 2011; Allaby, 2013)"@en ;
    rdfs:isDefinedBy <https://linked.data.gov.au/def/geofeatures> ;
    skos:inScheme <https://linked.data.gov.au/def/geofeatures> ;
    skos:notation "gfmyz" ;
    skos:prefLabel "mylonite zone"@en .

geof:Nappe a skos:Concept ;
    dcterms:source <http://www.glossaryofgeology.org>,
        <https://doi.org/10.1093/acref/9780199653065.001.0001> ;
    skos:broader geof:TectonostratigraphicRockUnit ;
    skos:definition "A sheetlike, allochthonous rock unit, which has moved on a predominantly horizontal surface as a result of thrust faulting, recumbent folding, or both. Fold limbs and axes are approximately horizontal (After Neuendorf et al., 2011; Allaby, 2013)"@en ;
    rdfs:isDefinedBy <https://linked.data.gov.au/def/geofeatures> ;
    skos:inScheme <https://linked.data.gov.au/def/geofeatures> ;
    skos:notation "gfnpp" ;
    skos:prefLabel "nappe"@en .

geof:NappeComplex a skos:Concept ;
    dcterms:source <https://doi.org/10.1080/11035897.2016.1178666> ;
    skos:broader geof:TectonostratigraphicRockUnit ;
    skos:definition "A nappe complex consists of two or more distinct nappes that are stacked upon, and related to, one another in some significant respect, e.g., shared general environment of origin, similar metamorphism and/or deformation. (Kumpulainen, 2017)"@en ;
    rdfs:isDefinedBy <https://linked.data.gov.au/def/geofeatures> ;
    skos:inScheme <https://linked.data.gov.au/def/geofeatures> ;
    skos:notation "gfnpx" ;
    skos:prefLabel "nappe complex"@en .

geof:Non-IgneousIntrusiveRockUnit a skos:Concept ;
    dcterms:references "After: Gillespie et al., 2008: BGS classification of lithodemic units: Proposals for classifying units of intrusive rock. British Geological Survey Research Report RR/08/05. <http://nora.nerc.ac.uk/id/eprint/5226/1/RR08005.pdf>"@en ;
    skos:broader geof:IntrusiveRockUnit ;
    skos:definition "A non-igneous intrusive rock unit such as a salt dome or a sediment-filled fracture (after Gillespie & Leslie, 2008)."@en ;
    rdfs:isDefinedBy <https://linked.data.gov.au/def/geofeatures> ;
    skos:inScheme <https://linked.data.gov.au/def/geofeatures> ;
    skos:notation "gfnii" ;
    skos:prefLabel "non-igneous intrusive rock unit"@en ;
    skos:scopeNote "Note: As per Gillespie & Leslie (2021), the BGS no longer supports the lithodemic nomenclature of the North American Stratigraphic Code (2005), as also is the case here (see references and discussion elsewhere in this ontology)."@en .

geof:Orogen a skos:Concept ;
    dcterms:source <http://www.glossaryofgeology.org> ;
    skos:broader geof:TectonicFeature ;
    skos:definition "An orogen (orogenic system, orogenic zone, orogenic belt) is a region in Earth’s lithosphere where a mountain belt is created by tectonic processes involving deformation, regional metamorphism, and associated magmatism, usually caused by convergence (± accretion and/or collision) between two tectonic plates or major crustal blocks. (Alt obsolete term: geosyncline). (Modified from Neuendorf et al., 2011; Hoy, pers. comm.)"@en ;
    rdfs:isDefinedBy <https://linked.data.gov.au/def/geofeatures> ;
    skos:inScheme <https://linked.data.gov.au/def/geofeatures> ;
    skos:notation "gforn" ;
    skos:prefLabel "orogen"@en .

geof:OrogenicCollage a skos:Concept ;
    dcterms:source <http://www.glossaryofgeology.org>,
        <https://doi.org/10.1146/annurev-earth-082517-010146> ;
    skos:broader geof:TectonicFeature ;
    skos:definition "A patchwork-map pattern of accreted terranes, embracing a geotectonic assemblage of crustal blocks separated by major faults (Neuendorf et al., 2011). In eastern Australia, such a collage is represented by the Tasmanides, which is part of the larger-scale Terra Australis Orogen that developed along the southern Panthalassan (Paleo-Pacific) margin of Gondwana, and which comprises multiple metamorphic belts, fold-thrust belts, igneous provinces, and sedimentary basins that have been attributed to five Cambrian to Triassic subduction-related orogens: the Delamerian, Thomson, Lachlan, Mossman, and New England Orogens (Rosenbaum, 2018)"@en ;
    rdfs:isDefinedBy <https://linked.data.gov.au/def/geofeatures> ;
    skos:inScheme <https://linked.data.gov.au/def/geofeatures> ;
    skos:notation "gforg" ;
    skos:prefLabel "orogenic collage"@en .

geof:Outlier a skos:Concept ;
    dcterms:source <http://www.glossaryofgeology.org> ;
    skos:broader geof:DenudationalFeature ;
    skos:definition "An area or group of rocks surrounded by older rocks. (Neuendorf et al., 2011)"@en ;
    rdfs:isDefinedBy <https://linked.data.gov.au/def/geofeatures> ;
    skos:inScheme <https://linked.data.gov.au/def/geofeatures> ;
    skos:notation "gfout" ;
    skos:prefLabel "outlier"@en .

geof:OverturnedFold a skos:Concept ;
    dcterms:source <https://doi.org/10.1093/acref/9780199653065.001.0001> ;
    skos:broader geof:StructuralFeature ;
    skos:definition "A zone where folds in their axial planes are inclined so that the fold limbs dip in the same direction, although not necessarily by the same amount. For each fold, one limb is thus ‘overturned'. (Allaby, 2008)"@en ;
    rdfs:isDefinedBy <https://linked.data.gov.au/def/geofeatures> ;
    skos:inScheme <https://linked.data.gov.au/def/geofeatures> ;
    skos:notation "gfofz" ;
    skos:prefLabel "overturned fold"@en .

geof:PedostratigraphicUnit a skos:Concept ;
    dcterms:source <http://www.glossaryofgeology.org>,
        <https://doi.org/10.1306/05230505015> ;
    skos:broader geof:StratigraphicUnit ;
    skos:definition "A buried, traceable, three-dimensional body of rock (or sediment) that consists of one or more differentiated pedologic horizons developed in, and overlain by, one or more formally defined lithostratigraphic or allostratigraphic units. (NACSN, 2005; Neuendorf et al., 2011)"@en ;
    rdfs:isDefinedBy <https://linked.data.gov.au/def/geofeatures> ;
    skos:inScheme <https://linked.data.gov.au/def/geofeatures> ;
    skos:notation "pdu" ;
    skos:prefLabel "pedostratigraphic unit"@en .

geof:Peneplain a skos:Concept ;
    dcterms:source <http://www.glossaryofgeology.org>,
        <https://doi.org/10.1093/acref/9780199653065.001.0001> ;
    skos:broader geof:DenudationalFeature ;
    skos:definition "A low, nearly featureless, gently undulating land surface of considerable area, which has been produced by the processes of prolonged subaerial erosion almost to base level; it is the end product of a cycle of erosion. (Davis, 1889; Neuendorf et al., 2011; Allaby, 2013)"@en ;
    rdfs:isDefinedBy <https://linked.data.gov.au/def/geofeatures> ;
    skos:inScheme <https://linked.data.gov.au/def/geofeatures> ;
    skos:notation "gfpnn" ;
    skos:prefLabel "peneplain"@en .

geof:PresentContinent a skos:Concept ;
    skos:definition "A large, existing landmass, comprising continental crust and embracing exposed land above sea level (Zealandia being an exception), and, below sea level, based on major differences in the inclination of the bathymetric surface, the attendant continental shelf, continental slope, and, if present, the continental rise (Modified and compiled from: Burke & Drake, 1974, Sheriff, 2002; Mortimer et al., 2017; Wikipedia, March 2020)."@en ;
    rdfs:isDefinedBy <https://linked.data.gov.au/def/geofeatures> ;
    skos:inScheme <https://linked.data.gov.au/def/geofeatures> ;
    skos:prefLabel "present continent"@en .

geof:Province a skos:Concept ;
    skos:broader geof:TectonicFeature ;
    skos:definition "A geologic province is a spatial entity with common geologic attributes, comprising a large area or region, which, considered as a whole, is characterised by similar geologic features or by a geologic history differing significantly from that of adjacent areas. (Modified from: Neuendorf et al. 2011; Geoscience Australia, USGS & Wikipedia, all accessed 13.05.2020)."@en ;
    rdfs:isDefinedBy <https://linked.data.gov.au/def/geofeatures> ;
    skos:inScheme <https://linked.data.gov.au/def/geofeatures> ;
    skos:notation "gfprv" ;
    skos:prefLabel "Province"@en ;
    skos:scopeNote "A geologic province may include a single dominant tectonic/structural entity such as a sedimentary basin or an association of genetically-related basins, but otherwise craton (including shields and platforms) or orogen, as well as specified types of provinces (viz., mineral province, igneous province, large igneous province, tectonised/metamorphosed province, extended-crust province) that are individually defined by a complex history of tectonics, metamorphism, magmatism and/or metallogenesis. A province may be divided into two or more subprovinces that may be further divided into geologic domains."@en .

geof:RangeZone a skos:Concept ;
    dcterms:source <http://www.stratigraphy.org/index.php/ics-stratigraphicguide> ;
    skos:broader geof:BiostratigraphicUnit ;
    skos:definition "The body of strata representing the known stratigraphic and geographic range of occurrence of a particular taxon or combination of two taxa of any rank. There are two principal types: taxon-range zones and concurrent-range zones. (ICS, Online, December 2019)"@en ;
    rdfs:isDefinedBy <https://linked.data.gov.au/def/geofeatures> ;
    skos:inScheme <https://linked.data.gov.au/def/geofeatures> ;
    skos:notation "gfrnz" ;
    skos:prefLabel "range zone"@en .

geof:Ridge a skos:Concept ;
    dcterms:source <https://en.wikipedia.org/wiki/Ridge> ;
    skos:broader geof:StructuralFeature ;
    skos:definition "A ridge or a mountain ridge is a geographical feature consisting of a chain of mountains or hills that form a continuous elevated crest for some distance. The sides of the ridge slope away from narrow top on either side. The lines along the crest formed by the highest points, with the terrain dropping down on either sides, are called the ridgelines. Ridges are usually termed hills or mountains as well, depending on size. (Adapted from Wikipedia)"@en ;
    rdfs:isDefinedBy <https://linked.data.gov.au/def/geofeatures> ;
    skos:inScheme <https://linked.data.gov.au/def/geofeatures> ;
    skos:notation "gfrdg" ;
    skos:prefLabel "ridge"@en .

geof:SedimentaryBasin a skos:Concept ;
    dcterms:source <https://doi.org/10.1007/978-3-662-03999-1> ;
    skos:broader geof:TectonicFeature ;
    skos:definition "A low area in the Earth’s crust, of tectonic origin, in which sediments accumulate. Sedimentary basins range in size from small continental basins to large oceanic basins. The essential element of the concept is tectonic creation of relief, to provide both a source of sediment and a relatively low place for the deposition of that sediment. (After Miall, 2000)"@en ;
    rdfs:isDefinedBy <https://linked.data.gov.au/def/geofeatures> ;
    skos:inScheme <https://linked.data.gov.au/def/geofeatures> ;
    skos:notation "gfsdb" ;
    skos:prefLabel "sedimentary basin"@en .

geof:SeismicProvince a skos:Concept ;
    dcterms:source <http://pid.geoscience.gov.au/dataset/ga/70149>,
        <https://doi.org/10.1016/j.tecto.2012.02.022> ;
    skos:broader geof:GeophysicalDomain ;
    skos:definition "Representative of a discrete \"volume\" of middle to lower crust which cannot be traced to the surface, and whose crustal reflectivity is different to that of laterally or vertically adjoining provinces (in differing lithology, geological history, and/or structural architecture). A Seismic Province is a Geophysical Domain. In North Queensland, the Numil and Abingdon Seismic Provinces are two lower crustal sectors that have been interpreted to represent microcontinents that accreted to the eastern fringe of the North Australian Craton prior to the late Paleoproterozoic (Korsch et al., 2010, Korsch, 2012)"@en ;
    rdfs:isDefinedBy <https://linked.data.gov.au/def/geofeatures> ;
    skos:inScheme <https://linked.data.gov.au/def/geofeatures> ;
    skos:notation "gfssp" ;
    skos:prefLabel "seismic province"@en .

geof:Subprovince a skos:Concept ;
    skos:broader geof:TectonicFeature ;
    skos:definition "One of two or more divisions of a province, based on differences in geological character."@en ;
    rdfs:isDefinedBy <https://linked.data.gov.au/def/geofeatures> ;
    skos:inScheme <https://linked.data.gov.au/def/geofeatures> ;
    skos:notation "gfsbp" ;
    skos:prefLabel "Subprovince"@en .

geof:Superprovince a skos:Concept ;
    skos:broader geof:TectonicFeature ;
    skos:definition "A grouping of two or more like geologic provinces."@en ;
    rdfs:isDefinedBy <https://linked.data.gov.au/def/geofeatures> ;
    skos:inScheme <https://linked.data.gov.au/def/geofeatures> ;
    skos:notation "gfspp" ;
    skos:prefLabel "Superprovince"@en ;
    skos:scopeNote "This highest-level root term was introduced by Mortimer et al. (2014), as the Austral Superprovince, to encompass all rocks of New Zealand’s Eastern Province and Western Province basement (providing a single stratigraphic search term for basement rocks in digital databases). In Queensland, for example, the term has application with the Tasmanides Orogenic Collage, the Great Australian Superbasin, and the Centralian Superbasin."@en .

geof:SequenceStratigraphicUnit a skos:Concept ;
    dcterms:source <https://doi.org/10.1080/11035897.2016.1178666>,
        <https://doi.org/10.1127/0078-0421/2011/0011> ;
    skos:broader geof:StratigraphicUnit ;
    skos:definition "A Sequence Stratigraphic Unit is an extensive, depositional unit that may be bounded by subaerial unconformities and their correlative conformities, by transgressive surfaces or by surfaces of maximum marine flooding. It documents changes in relative sea level, which may have been the result of eustasy, regional or local tectonic movements, compaction, isostasy or the combination of two or more of these factors. (Kumpulainen, 2017; Catuneanu et al., 2011)"@en ;
    rdfs:isDefinedBy <https://linked.data.gov.au/def/geofeatures> ;
    skos:inScheme <https://linked.data.gov.au/def/geofeatures> ;
    skos:notation "gfsqu" ;
    skos:prefLabel "sequence stratigraphic unit"@en .

geof:ShearZone a skos:Concept ;
    dcterms:source <https://doi.org/10.1093/acref/9780199653065.001.0001> ;
    skos:broader geof:StructuralFeature ;
    skos:definition "A region, narrow compared to its length, within which rocks have undergone intense deformation: viz. brecciation. There are two end-members: brittle shear zones (faults), marked by a surface of rupture, which are a common feature of higher crustal levels; and ductile shear zones in which deformation is continuous and characterized by high ductile strain due to the rocks having formed under high temperatures and pressures at deeper crustal levels. Both brittle and ductile shear zones may occur as subparallel or conjugate sets. (after Allaby, 2013 (Oxford Dictionary of Geology and Earth Sciences))"@en ;
    rdfs:isDefinedBy <https://linked.data.gov.au/def/geofeatures> ;
    skos:inScheme <https://linked.data.gov.au/def/geofeatures> ;
    skos:notation "gfshz" ;
    skos:prefLabel "shear zone"@en .

geof:Shield a skos:Concept ;
    dcterms:source <http://www.glossaryofgeology.org> ;
    skos:broader geof:TectonicFeature ;
    skos:definition "A large area of exposed basement rock in a craton, commonly with a very gently convex surface, surrounded by sediment covered platforms. The rocks of virtually all shield areas are Precambrian. (Neuendorf et al., 2011)"@en ;
    rdfs:isDefinedBy <https://linked.data.gov.au/def/geofeatures> ;
    skos:inScheme <https://linked.data.gov.au/def/geofeatures> ;
    skos:notation "gfshd" ;
    skos:prefLabel "shield"@en .

geof:StratigraphicEvent a skos:Concept ;
    dcterms:source <https://doi.org/10.1080/11035897.2016.1178666> ;
    skos:broader geof:StratigraphicFeature ;
    skos:definition "Stratigraphic Events reflect physical, chemical and biological events that left identifiable, widespread, if not worldwide, traces or markers in the sedimentary or extrusive igneous record (Kumpulainen, 2017)"@en ;
    rdfs:isDefinedBy <https://linked.data.gov.au/def/geofeatures> ;
    skos:inScheme <https://linked.data.gov.au/def/geofeatures> ;
    skos:notation "gfste" ;
    skos:prefLabel "stratigraphic event"@en .

geof:Subbasin a skos:Concept ;
    skos:definition "A sedimentary basin may be subdivided into two or more subbasins that have separate depocentres and are separated from one another by some tectonic/structural element, such as a fault or basement high. (Definition created here: Paul Blake, John McKellar)"@en ;
    rdfs:isDefinedBy <https://linked.data.gov.au/def/geofeatures> ;
    skos:inScheme <https://linked.data.gov.au/def/geofeatures> ;
    skos:prefLabel "subbasin"@en .

geof:Subgroup a skos:Concept ;
    skos:definition "A Subgroup is a part of a Group. (Definition created here: Paul Blake, John McKellar)"@en ;
    rdfs:isDefinedBy <https://linked.data.gov.au/def/geofeatures> ;
    skos:inScheme <https://linked.data.gov.au/def/geofeatures> ;
    skos:prefLabel "subgroup"@en .

geof:Superbasin a skos:Concept ;
    skos:definition "A superbasin is a hierarchial term applied to  a group of largely interconnected or associated sedimentary basins of the same or similar age. Its component basins may be separated or partially separated by tectonic elements that define 'boundaries'  between them, or they may have been subjected to somewhat different geological influences. In the Australian Mesozoic, the Great Australian Superbasin, composed of the Nambour, Clarence-Moreton, Surat, Eromanga, Carpentaria and other basins, is a prime example, variously covering a geographically-extensive area in parts of Queensland, the Northern Territory, New South Wales and South Australia. (Definition created here)"@en ;
    rdfs:isDefinedBy <https://linked.data.gov.au/def/geofeatures> ;
    skos:inScheme <https://linked.data.gov.au/def/geofeatures> ;
    skos:prefLabel "superbasin"@en .

geof:Supercontinent a skos:Concept ;
    dcterms:source <http://doi.org/10.22459/SN.08.2012> ;
    skos:broader geof:TectonicFeature ;
    skos:definition """A large continent formed by the amalgamation of most or all of Earth’s continental landmasses. (Blewett, 2012)"""@en ;
    rdfs:isDefinedBy <https://linked.data.gov.au/def/geofeatures> ;
    skos:inScheme <https://linked.data.gov.au/def/geofeatures> ;
    skos:notation "gfspc" ;
    skos:prefLabel "supercontinent"@en .

geof:Supercraton a skos:Concept ;
    dcterms:source <http://doi.org/10.22459/SN.08.2012> ;
    skos:broader geof:TectonicFeature ;
    skos:definition "A large, ancestral (largely Archean) landmass consisting of two or more cratons. (Blewett, 2012)"@en ;
    rdfs:isDefinedBy <https://linked.data.gov.au/def/geofeatures> ;
    skos:inScheme <https://linked.data.gov.au/def/geofeatures> ;
    skos:notation "gfspn" ;
    skos:prefLabel "supercraton"@en .

geof:Syncline a skos:Concept ;
    dcterms:source <http://www.glossaryofgeology.org> ;
    skos:broader geof:StructuralFeature ;
    skos:definition "A fold of which the core contains the stratigraphically younger rocks; it is generally concave upward. (Neuendorf et al., 2011)"@en ;
    rdfs:isDefinedBy <https://linked.data.gov.au/def/geofeatures> ;
    skos:inScheme <https://linked.data.gov.au/def/geofeatures> ;
    skos:notation "gfsyn" ;
    skos:prefLabel "syncline"@en .

geof:Synclinorium a skos:Concept ;
    dcterms:source <http://www.glossaryofgeology.org> ;
    skos:broader geof:StructuralFeature ;
    skos:definition "A composite synclinal structure of regional extent composed of lesser folds. (Neuendorf et al., 2011)"@en ;
    rdfs:isDefinedBy <https://linked.data.gov.au/def/geofeatures> ;
    skos:inScheme <https://linked.data.gov.au/def/geofeatures> ;
    skos:notation "gfsyc" ;
    skos:prefLabel "synclinorium"@en .

geof:Synform a skos:Concept ;
    dcterms:source <http://www.glossaryofgeology.org> ;
    skos:broader geof:StructuralFeature ;
    skos:definition "Any fold whose limbs close at the bottom. The term is usually used when the folded layers do not possess a stratigraphic order, when the stratigraphic order of the folded layers is not known, or when the fold core also contains the stratigraphically older rock. (Neuendorf et al., 2011)"@en ;
    rdfs:isDefinedBy <https://linked.data.gov.au/def/geofeatures> ;
    skos:inScheme <https://linked.data.gov.au/def/geofeatures> ;
    skos:notation "gfsyf" ;
    skos:prefLabel "synform"@en .

geof:TaxonRangeZone a skos:Concept ;
    dcterms:source <http://www.stratigraphy.org/index.php/ics-stratigraphicguide> ;
    skos:broader geof:BiostratigraphicUnit ;
    skos:definition "The body of strata representing the known range of stratigraphic and geographic occurrence of specimens of a particular taxon. (ICS, Online, December 2019)"@en ;
    rdfs:isDefinedBy <https://linked.data.gov.au/def/geofeatures> ;
    skos:inScheme <https://linked.data.gov.au/def/geofeatures> ;
    skos:notation "gftrz" ;
    skos:prefLabel "taxon range zone"@en .

geof:TectonicPlate a skos:Concept ;
    dcterms:source <https://pubs.usgs.gov/gip/dynamic/tectonic.html> ;
    skos:broader geof:TectonicFeature ;
    skos:definition """The lithosphere is divided into a number of discrete tectonic plates each of which has motion relative to other plates. 

Tectonic plates vary significantly in size and thickness, with boundaries marked by seismic and volcanic activity. They move slowly relative to one another due to convection currents in the Upper Mantle, and may slide on a boundary with another along transform faults. A tectonic plate comprising oceanic lithosphere (entirely or partly thereof), can sink/subduct in a subduction zone below another, usually a lighter, continental plate. Along mid-ocean ridges and major rifts, tectonic plates separate and new crust is formed by the upwelling of basaltic magma.(Adapted from Sheriff, 2002; USGS, 1999)."""@en ;
    rdfs:isDefinedBy <https://linked.data.gov.au/def/geofeatures> ;
    skos:inScheme <https://linked.data.gov.au/def/geofeatures> ;
    skos:notation "gfplt" ;
    skos:prefLabel "tectonic plate"@en .

geof:TectonisedMetomorphosedProvince a skos:Concept ;
    skos:definition "A Tectonised and/or Metamorphosed Province is generally an old sedimentary basin that has been strongly tectonised and/or metamorphosed, so that its original basin extent and form are no longer preserved. Such provinces may have associated magmatism and metallogenesis. (Definition created here)"@en ;
    rdfs:isDefinedBy <https://linked.data.gov.au/def/geofeatures> ;
    skos:inScheme <https://linked.data.gov.au/def/geofeatures> ;
    skos:prefLabel "tectonised metomorphosed province"@en .
    
geof:TectonometamorphicRockUnit a skos:Concept ; 
    dcterms:references "Gillespie, M.R. & Leslie, A.G., 2021: BRUCS: a new system for classifying and naming mappable rock units. Journal of the Geological Society, 178(4), jgs2020-212. <https://jgs.lyellcollection.org/content/jgs/178/4/jgs2020-212.full.pdf>"@en ; 
    dcterms:references "See and compare: Nystuen, J.P. (Editor), 1989: Rules and recommendations of naming geological units in Norway. Norsk Geologisk Tidskrift 69 (Supplement 2), 1–111. <https://foreninger.uio.no/ngf/ngt/pdfs/NGT_69_supplement1.pdf>"@en ;
    dcterms:references "See and compare: Kumpulainen (Editor), 2017: Guide for Geological Nomenclature in Sweden. GFF, 139:1, 3-20. <https://doi.org/10.1080/11035897.2016.1178666>"@en ;
    skos:broader <http://sweetontology.net/realmGeol/GeologicFeature> ;
    skos:definition "Tectonometamorphic rock units are defined bodies of rock that cannot reliably be classified as accumulated (stratiform, lithostratigraphic) rock units or as intrusive rock units, as a result of superimposed deformation and/or metamorphism (Gillespie & Leslie, 2021)."@en ; 
    rdfs:isDefinedBy <https://linked.data.gov.au/def/geofeatures> ;
    skos:inScheme <https://linked.data.gov.au/def/geofeatures> ;
    skos:notation "gftme" ; 
    skos:scopeNote "Separated out from tectonometamorphic rock units are tectonostratigraphic rock units which embrace tectonically-displaced, allochthonous sheets (Nystuen, 1989; Kumpulainen, 2017; also see and compare: Gillespie & Leslie, 2021, pp. 16–17). In GSQ’s associated rock-unit-rank vocabulary, the terminology applied therein to tectonometamorphic rock units, as per Gillespie & Leslie (2021), in the development by these authors of the British Geological Survey’s new Rock Unit Classification System/BRUCS), is currently not well progressed, apart from application of the term ‘ophiolite’. The BRUCS tectonometamorphic nomenclature has merit but requires consideration for its potential in application in Queensland (and Australia) to tectonometamorphic bodies of rock, the nomenclature of which, in terms of rank, is presently assessed (here) as being in need of revision."@en ; 
    skos:prefLabel "tectonometamorphic rock unit"@en .

geof:Terrane a skos:Concept ;
    dcterms:source <http://www.glossaryofgeology.org> ;
    skos:broader geof:TectonicFeature ;
    skos:definition "A fault-bounded body of rock of regional extent, characterised by a geologic history different from that of contiguous terranes or bounding continents. A terrane is generally considered to be a discrete allochthonous fragment of oceanic or continental material added to a craton (or continental plate) at an active margin by accretion. (After  Neuendorf et al., 2011)"@en ;
    rdfs:isDefinedBy <https://linked.data.gov.au/def/geofeatures> ;
    skos:inScheme <https://linked.data.gov.au/def/geofeatures> ;
    skos:notation "gftrn" ;
    skos:prefLabel "terrane"@en .

geof:Trough a skos:Concept ;
    skos:definition "A trough (in the continental realm) is an elongate region of the lithosphere that has undergone subsidence because of faulting along one or both of its elongate margins, permitting the accumulation of sediments and the subsequent formation of sedimentary rocks. Troughs are generally grabens or half-grabens, sometimes associated with initial magmatism, that have formed under extensional or transtensional tectonic conditions and may be part of, or associated with, the formation, and subsequent evolution, of larger sedimentary-basin/rifting systems or basin-and-range (western-North-America) type settings. (Definition created here)"@en ;
    skos:notation "gftrh" ;
    rdfs:isDefinedBy <https://linked.data.gov.au/def/geofeatures> ;
    skos:inScheme <https://linked.data.gov.au/def/geofeatures> ;
    skos:prefLabel "trough"@en .

geof:Unconformity a skos:Concept ;
    dcterms:source <http://www.glossaryofgeology.org>,
        <https://doi.org/10.1093/acref/9780199653065.001.0001> ;
    skos:broader geof:DenudationalFeature ;
    skos:definition "The surface of contact between rock strata that represents a lack of continuity in deposition, encompassing a period of nondeposition or weathering/erosion prior to the deposition of younger rocks, sometimes, in the case of sedimentary rocks, marked by the absence of conformity between the dip and strike of underlying and overlying strata. (Modified from Neuendorf et al., 2011; Allaby, 2013)"@en ;
    rdfs:isDefinedBy <https://linked.data.gov.au/def/geofeatures> ;
    skos:inScheme <https://linked.data.gov.au/def/geofeatures> ;
    skos:notation "gfunc" ;
    skos:prefLabel "unconformity"@en .

geof:Window a skos:Concept ;
    dcterms:source <http://www.glossaryofgeology.org> ;
    skos:broader geof:DenudationalFeature ;
    skos:definition "An eroded area of a thrust sheet or nappe that displays the rocks beneath the thrust sheet. (Neuendorf et al., 2011)"@en ;
    rdfs:isDefinedBy <https://linked.data.gov.au/def/geofeatures> ;
    skos:inScheme <https://linked.data.gov.au/def/geofeatures> ;
    skos:notation "gfwnw" ;
    skos:prefLabel "window"@en .

<https://linked.data.gov.au/org/ga> a sdo:Organization ;
    sdo:name "Geoscience Australia" ;
    sdo:url "https://www.ga.gov.au"^^xsd:anyURI .

geof:GeophysicalFeature a skos:Concept ;
    dcterms:source <http://www.glossaryofgeology.org> ;
    skos:broader <http://sweetontology.net/realmGeol/GeologicFeature> ;
    skos:definition "A feature associated with, and interpreted from, the physical properties and processes of the Earth, e.g., seismology. (Neuendorf et al., 2011)"@en ;
    rdfs:isDefinedBy <https://linked.data.gov.au/def/geofeatures> ;
    skos:inScheme <https://linked.data.gov.au/def/geofeatures> ;
    skos:notation "gfgpf" ;
    skos:prefLabel "geophysical feature"@en .

<https://orcid.org/0000-0001-5489-9590> a owl:NamedIndividual,
        sdo:Person ;
    sdo:affiliation <https://linked.data.gov.au/org/gsq> ;
    sdo:email <mailto:john.mckellar@dnrme.qld.gov.au> ;
    sdo:name "John L. McKellar" ;
    sdo:identifier <https://orcid.org/0000-0001-5489-9590> .

<https://orcid.org/0000-0002-8742-7730> a owl:NamedIndividual,
        sdo:Person ;
    sdo:affiliation [ a sdo:Organization ;
            sdo:name "SURROUND Australia Pty Ltd" ;
            sdo:url "https://surroundaustralia.com"^^xsd:anyURI ] ;
    sdo:email <mailto:nicholas.car@surroundaustralia.com> ;
    sdo:name "Nicholas J. Car" ;
    sdo:identifier <https://orcid.org/0000-0002-8742-7730> .

geof:GeophysicalDomain a skos:Concept ;
    dcterms:source <http://pid.geoscience.gov.au/dataset/ga/14909>,
        <https://doi.org/10.1016/j.tecto.2012.02.022> ;
    skos:broader geof:GeophysicalFeature ;
    skos:definition "Geophysical Domains are Geologic Features delimited by their geophysical properties, primarily magnetic and gravity properties or, in the case of Seismic Provinces, their crustal reflectivity. They represent discrete \"volumes\" of middle to lower crust. (Terminology based on usage of Shaw et al., 1996; Korsch et al., 2012)"@en ;
    rdfs:isDefinedBy <https://linked.data.gov.au/def/geofeatures> ;
    skos:inScheme <https://linked.data.gov.au/def/geofeatures> ;
    skos:notation "gfgpd" ;
    skos:prefLabel "geophysical domain"@en .

geof:StratigraphicFeature a skos:Concept ;
    dcterms:source <http://www.stratigraphy.org/index.php/ics-stratigraphicguide>,
        <https://doi.org/10.1080/11035897.2016.1178666> ;
    skos:broader <http://sweetontology.net/realmGeol/GeologicFeature> ;
    skos:definition "Stratigraphic Features embrace Stratigraphic Units, which are units of rock and/or sediment that conform to the Law of Superposition (e.g. lithostratigraphic units, biostratigraphic units, chronostratigraphic units), and Stratigraphic Events which reflect physical, chemical and biological events that left identifiable, widespread, if not worldwide, traces or markers in the sedimentary or extrusive igneous record (ICS; Kumpulainen, R.A., 2016)"@en ;
    rdfs:isDefinedBy <https://linked.data.gov.au/def/geofeatures> ;
    skos:inScheme <https://linked.data.gov.au/def/geofeatures> ;
    skos:notation "gfstf" ;
    skos:prefLabel "stratigraphic feature"@en .

geof:TectonicFeature a skos:Concept ;
    dcterms:source <https://doi.org/10.1080/11035897.2016.1178666> ;
    skos:broader <http://sweetontology.net/realmGeol/GeologicFeature> ;
    skos:definition "Tectonic Features (Tectonic Units, Tectonic Entities) include the lithosphere, including the continental and oceanic crust, tectonic plates (that the lithosphere is subdivided into), mid-ocean ridges, orogens, subduction zones, volcanic arcs, continents, cratons/shields, extended crust provinces, tectonised and or metamorphosed provinces, metallogenic (mineral) provinces, igneous provinces (including large igneous provinces), and sedimentary basins; collectively, they include continents, past and present, and, when previously formed, supercontinents (modified and extended from Kumpulainen, 2017; Wikipedia, March 2022)."@en ;
    rdfs:isDefinedBy <https://linked.data.gov.au/def/geofeatures> ;
    skos:inScheme <https://linked.data.gov.au/def/geofeatures> ;
    skos:notation "gftcr" ;
    skos:prefLabel "tectonic feature"@en .

geof:GeologicallySignificantSite a skos:Concept ;
    dcterms:source <http://www.unesco.org/new/en/natural-sciences/environment/earth-sciences/unesco-global-geoparks/frequently-asked-questions/what-is-a-unesco-global-geopark/> ;
    skos:broader <http://sweetontology.net/realmGeol/GeologicFeature>,
        <http://www.opengis.net/ont/geosparql#Feature> ;
    skos:definition "Single, unified geographical areas where sites and landscapes of international geological significance are managed with a holistic concept of protection, education and sustainable development"@en ;
    rdfs:isDefinedBy <https://linked.data.gov.au/def/geofeatures> ;
    skos:inScheme <https://linked.data.gov.au/def/geofeatures> ;
    skos:notation "gfgss" ;
    skos:prefLabel "geologically significant site"@en .

geof:MagnetostratigraphicUnit a skos:Concept ;
    dcterms:source <http://www.stratigraphy.org/index.php/ics-stratigraphicguide>,
        <https://doi.org/10.1130/9780813774022> ;
    skos:broader geof:StratigraphicUnit ;
    skos:definition "A Magnetostratigraphic Unit (Magnetozone) is a body of rocks unified by similar magnetic characteristics which allow it to be differentiated from adjacent rock bodies.  The term is collectively applied to the different kinds of stratigraphic units that are identified by their measurable magnetic properties. (Salvador, 2013; ICS, Online, December, 2019)"@en ;
    rdfs:isDefinedBy <https://linked.data.gov.au/def/geofeatures> ;
    skos:inScheme <https://linked.data.gov.au/def/geofeatures> ;
    skos:notation "gfmsu" ;
    skos:prefLabel "magnetostratigraphic unit"@en .

geof:TectonostratigraphicRockUnit a skos:Concept ;
dcterms:references "Kumpulainen (Editor), 2017: Guide for Geological Nomenclature in Sweden. GFF, 139:1, 3-20. <https://doi.org/10.1080/11035897.2016.1178666>"@en ;
    skos:broader <http://sweetontology.net/realmGeol/GeologicFeature> ;
    skos:definition "Tectonostratigraphic rock units encompass generally flat-lying, scale-independent, tectonic rock units that are bounded by zones of high strain (ductile shear zone, deformation zone or belt, fault, fault zone, etc.). They include tectonically-displaced allochthonous sheets that are represented by nappes (thrust sheets) and nappe complexes (after Kumpulainen, 2017)."@en ; 
    rdfs:isDefinedBy <https://linked.data.gov.au/def/geofeatures> ;
    skos:inScheme <https://linked.data.gov.au/def/geofeatures> ;
    skos:notation "gftse" ;
    skos:prefLabel "tectonostratigraphic rock unit"@en .

<https://linked.data.gov.au/org/gsq> a owl:NamedIndividual,
        sdo:Organization ;
    sdo:email <mailto:geological_info@dnrme.qld.gov.au> ;
    sdo:name "Geological Survey of Queensland" ;
    sdo:url "https://www.business.qld.gov.au/industries/mining-energy-water/resources/geoscience-information/gsq"^^xsd:anyURI .

geof:DenudationalFeature a skos:Concept ;
    dcterms:source <https://doi.org/10.1080/11035897.2016.1178666> ;
    skos:broader geof:StructuralFeature ;
    skos:definition "Structures shaped by weathering and erosion; include inlier, outlier, window, klippe, unconformity and peneplain (Kumpulainen, 2017)"@en ;
    rdfs:isDefinedBy <https://linked.data.gov.au/def/geofeatures> ;
    skos:inScheme <https://linked.data.gov.au/def/geofeatures> ;
    skos:notation "gfdnf" ;
    skos:prefLabel "denudational feature"@en .

geof:StratigraphicUnit a skos:Concept ;
    dcterms:references "North American Stratigraphic Code (NASC), 2005: AAPG Bulletin, 89(11), 1547–1591. <https://doi.org/10.1306/05230505015>@en" ; 
    dcterms:references "Kumpulainen (Editor), 2017: Guide for Geological Nomenclature in Sweden. GFF, 139:1, 3-20. <https://doi.org/10.1080/11035897.2016.1178666>"@en ;
    dcterms:references "Gillespie, M.R. & Leslie, A.G., 2021: BRUCS: a new system for classifying and naming mappable rock units. Journal of the Geological Society, 178(4), jgs2020-212. <https://jgs.lyellcollection.org/content/jgs/178/4/jgs2020-212.full.pdf>"@en ;
    dcterms:references "Steno, N. 1669. De solido intra solidum naturaliter contento dissertationis prodromus. Florence, Italy, 144 pages. <https://archive.org/details/ita-bnc-mag-00001426-001/page/n50/mode/2up> @en" ;
    dcterms:references "Compare: Salvador, A., 2013: International Stratigraphic Guide. Reprinted Second Edition, The International Union of Geological Sciences and The Geological Society of America, 214 pages. <https://doi.org/10.1130/9780813774022> "@en ;
    dcterms:references "Compare: Murphy, M.A. & Salvador, A. (Editors; revised by W.E. Piller & M-P Aubry), Online: International Stratigraphic Guide — An abridged version. Accessed online 04.11.2021. < https://stratigraphy.org/guide/defs >"@en ;
    skos:broader geof:StratigraphicFeature ;
    skos:definition "A stratigraphic unit is a distinct and definable body of layered rock that conforms with the Law of Superposition (Steno, 1669) and is variously described and differentiated, in each case from the same unit type, by: its lithologic properties (lithostratigraphic unit); its fossil content (biostratigraphic unit); its magnetic properties (magnetostratigraphic unit); the time interval during which it was formed (chronostratigraphic unit); by its bounding subaerial unconformities and their correlative conformities (sequence stratigraphic unit); or by one or more pedologic horizons buried in one or more lithic units (pedostratigraphic unit) [modified variously from: NASC, 2005; Kumpulainen, 2017; cf.: Salvador, 2013; cf: Murphy & Salvador, Online]."@en ;
    rdfs:isDefinedBy <https://linked.data.gov.au/def/geofeatures> ;
    skos:inScheme <https://linked.data.gov.au/def/geofeatures> ;
    skos:notation "gfstu" ;
    skos:prefLabel "stratigraphic unit"@en ;
    skos:scopeNote "Followed here are the definitions applied to ‘stratigraphy’ and ‘stratigraphic unit’ by the North American Stratigraphic Code (NASC, 2005) and Kumpulainen (2017). This approach thus differs from that proffered by the International Commission on Stratigraphy in the ‘International Stratigraphic Guide’/ISG (e.g., Salvador, 2013; Murphy & Salvador, Online), which regards ‘stratigraphy’ as embracing the description of all classes of rocks (sedimentary, igneous, metamorphic) forming the Earth’s crust and their organisation/classification into distinctive, useful, mappable units based on their inherent properties or attributes, in order to establish their distribution and relationship in space and their succession in time. The NASC (2005) introduced the term ‘lithodemic unit’ to encompass (predominantly intrusive, highly metamorphosed, or intensely deformed) rocks that do not obey Steno’s (1669) Law of Superposition (as opposed to a ‘lithostratigraphic unit’ which encompasses rocks that conform to this Law). The NASC lithodemic classification for non-stratified (nonstratiform) rocks, employing the terms ‘Lithodeme’, ‘Suite’ and ‘Supersuite’, was accepted by Kumpulainen (2017), such that lithodemic (non-stratified/nonstratiform) rocks and lithostratigraphic (stratified/stratiform) rocks were considered to be different, requiring different approaches to their classification. But, lithodemic terminology, per se, has not been embraced here, as it was also used to incorporate a rock ‘complex’(as a non-ranked, lithodemic unit). Rock complexes are here separated from other rock types (and, in an associated rock-unit-rank ontology, accorded rank: supercomplex, complex, etc.), with a comparable approach being adopted by Gillespie & Leslie (2021) in the British Geological Survey’s Rock Unit Classification System (BRUCS). The rank terms ‘Suite’ and ‘Supersuite’ are applied to (nonstratiform) intrusive rock units, as per BRUCS, contrasting with the NASC (2005), which also applied these rankings to metamorphic rock types."@en .

geof:LithostratigraphicUnit a skos:Concept ;
    skos:altLabel "stratiform unit"@en ;
    skos:altLabel "accumulated unit"@en ;
    dcterms:references "North American Stratigraphic Code (NASC), 2005: AAPG Bulletin, 89(11), 1547–1591. <https://doi.org/10.1306/05230505015>@en" ; 
    dcterms:references "Kumpulainen (Editor), 2017: Guide for Geological Nomenclature in Sweden. GFF, 139:1, 3-20. <https://doi.org/10.1080/11035897.2016.1178666>"@en ;
    dcterms:references "Gillespie, M.R. & Leslie, A.G., 2021: BRUCS: a new system for classifying and naming mappable rock units. Journal of the Geological Society, 178(4), jgs2020-212. <https://jgs.lyellcollection.org/content/jgs/178/4/jgs2020-212.full.pdf>"@en ;
    dcterms:references "Steno, N. 1669. De solido intra solidum naturaliter contento dissertationis prodromus. Florence, Italy, 144 pages. <https://archive.org/details/ita-bnc-mag-00001426-001/page/n50/mode/2up> @en" ;
    dcterms:references "Compare: Salvador, A., 2013: International Stratigraphic Guide. Reprinted Second Edition, The International Union of Geological Sciences and The Geological Society of America, 214 pages. <https://doi.org/10.1130/9780813774022> "@en ;
    dcterms:references "Compare: Murphy, M.A. & Salvador, A. (Editors; revised by W.E. Piller & M-P Aubry), Online: International Stratigraphic Guide — An abridged version. Accessed online 04.11.2021. < https://stratigraphy.org/guide/defs >"@en ;
    skos:broader geof:StratigraphicUnit ;
    skos:definition "Lithostratigraphic units are bodies of rocks, bedded or unbedded, that are defined and characterized on the basis of their lithologic properties and their stratigraphic relations, but conforming to the Law of Superposition (Steno, 1669) [NASC, 2005, Kulpmainen, 2017; cf. Salvador, 2013; cf. Murphy & Salvador, Online]."@en ;
    rdfs:isDefinedBy <https://linked.data.gov.au/def/geofeatures> ;
    skos:inScheme <https://linked.data.gov.au/def/geofeatures> ;
    skos:notation "gflsu" ;
    skos:prefLabel "lithostratigraphic unit"@en .

<http://sweetontology.net/realmGeol/GeologicFeature> a skos:Concept ;
    skos:definition "A geologic feature is a conceptual feature a that is hypothesized to exist coherently in the Earth that results from geological processes"@en ;
    rdfs:isDefinedBy <https://linked.data.gov.au/def/geofeatures> ;
    skos:inScheme <https://linked.data.gov.au/def/geofeatures> ;
    skos:prefLabel "geologic feature"@en .

geof:BiostratigraphicUnit a skos:Concept ;
    dcterms:source <http://www.stratigraphy.org/index.php/ics-stratigraphicguide> ;
    skos:broader geof:StratigraphicUnit ;
    skos:definition "Biostratigraphic units/Biostratigraphic Zones (biozones) are bodies of strata that are defined or characterized on the basis of their contained fossils.  The different types have no hierarchical significance, and are not based on mutually exclusive criteria. (ICS, Online, December 2019)"@en ;
    rdfs:isDefinedBy <https://linked.data.gov.au/def/geofeatures> ;
    skos:inScheme <https://linked.data.gov.au/def/geofeatures> ;
    skos:notation "gfbst" ;
    skos:prefLabel "biostratigraphic unit"@en .

geof:StructuralFeature a skos:Concept ;
    dcterms:source <http://www.glossaryofgeology.org> ;
    skos:broader <http://sweetontology.net/realmGeol/GeologicFeature> ;
    skos:definition "A feature produced by deformation or displacement of rocks, such as a fold or fault (Neuendorf et al., 2011)."@en ;
    rdfs:isDefinedBy <https://linked.data.gov.au/def/geofeatures> ;
    skos:inScheme <https://linked.data.gov.au/def/geofeatures> ;
    skos:notation "gfstr" ;
    skos:prefLabel "structural feature"@en .

<https://linked.data.gov.au/def/geofeatures> a owl:NamedIndividual,
        owl:Ontology,
        skos:ConceptScheme,
        prof:Profile ;
    dcterms:contributor [ a owl:NamedIndividual,
                sdo:Person ;
            sdo:affiliation <https://linked.data.gov.au/org/gsq> ;
            sdo:email <mailto:derek.hoy@dnrme.qld.gov.au> ;
            sdo:identifier <mailto:derek.hoy@dnrme.qld.gov.au> ;
            sdo:name "Derek Hoy" ],
        <https://linked.data.gov.au/org/gsq> ;
    dcterms:created "2020-01-23"^^xsd:date ;
    dcterms:creator <https://orcid.org/0000-0001-5489-9590>,
        <https://orcid.org/0000-0002-8742-7730> ;
    dcterms:modified "2020-03-10"^^xsd:date ;
    dcterms:publisher <https://linked.data.gov.au/org/gsq> ;
    owl:imports <http://www.opengis.net/ont/geosparql>,
        <http://www.w3.org/2004/02/skos/core> ;
    owl:versionIRI <https://linked.data.gov.au/def/geofeatures/0.5> ;
    owl:versionInfo "Most ontology content but not complete diagrammatic coverage." ;
    skos:definition "This vocabulary lists types of geological features relevant to the duties of the Geological Survey of Queensland. It is automatically derived from GSQ's Geologic Features Ontology (https://linked.data.gov.au/def/geofeatures)"@en ;
    skos:hasTopConcept <http://sweetontology.net/realmGeol/GeologicFeature> ;
    skos:prefLabel "Geologic Feature Types"@en ;
    prof:isProfileOf <http://sweetontology.net/realmGeol> ;
    sdo:codeRepository <https://github.com/geological-survey-of-queensland/geologic-features-ont> .
