@prefix dc: <http://purl.org/dc/elements/1.1/> .
@prefix dct: <http://purl.org/dc/terms/> .
@prefix gsqst: <http://linked.data.gov.au/def/geological-sites/> .
@prefix owl: <http://www.w3.org/2002/07/owl#> .
@prefix rdf: <http://www.w3.org/1999/02/22-rdf-syntax-ns#> .
@prefix rdfs: <http://www.w3.org/2000/01/rdf-schema#> .
@prefix skos: <http://www.w3.org/2004/02/skos/core#> .
@prefix xml: <http://www.w3.org/XML/1998/namespace> .
@prefix xsd: <http://www.w3.org/2001/XMLSchema#> .

<http://linked.data.gov.au/def/geological-sites> a owl:Ontology , skos:ConceptScheme ;
    dct:created "2020-02-07T14:06:56"^^xsd:dateTime ;
    dct:creator "Geological Survey of Queensland" ;
    dct:modified "2020-02-07T14:06:56"^^xsd:dateTime ;
    dct:source "Compiled by the Geological Survey of Queensland" ;
    skos:definition "The proximate geological features and locations that may be sampled or observed to determine the geological properties of an ultimate feature of interest."@en ;
    skos:hasTopConcept gsqst:base-station,
        gsqst:borehole,
        gsqst:cutting,
        gsqst:field-site,
        gsqst:mine,
        gsqst:mineral-occurrence,
        gsqst:mineral-deposit,
        gsqst:pit,
        gsqst:survey-site,
        #gsqst:wellbore,
        gsqst:wellbore-interval ;
    skos:prefLabel "Geological Sites"@en .

gsqst:alluviual a skos:Concept ;
    skos:broader gsqst:field-site ;
    skos:definition "A field site from which a sediment sample transported by transport in a medium (air, water, ice) is taken or observation is made."@en ;
    skos:inScheme <http://linked.data.gov.au/def/geological-sites> ;
    skos:notation "av" ;
    skos:prefLabel "Alluvial Site"@en .

gsqst:colluvial a skos:Concept ;
    skos:altLabel "Float"@en,
        "Scree"@en,
        "Scree Slope"@en,
        "Talus"@en ;
    skos:broader gsqst:field-site ;
    skos:definition "A field site from which a sediment sample transported by gravity is taken or observation is made."@en ;
    skos:inScheme <http://linked.data.gov.au/def/geological-sites> ;
    skos:notation "cv" ;
    skos:prefLabel "Colluvial Site"@en .

gsqst:outcrop a skos:Concept ;
    skos:broader gsqst:field-site ;
    dct:source "Merriam-Webster Dictionary" ;
    skos:definition "The part of a rock formation that appears at the surface of the ground. "@en ;
    skos:inScheme <http://linked.data.gov.au/def/geological-sites> ;
    skos:notation "oc" ;
    skos:prefLabel "Outcrop"@en .

gsqst:soil-horizon a skos:Concept ;
    skos:broader gsqst:field-site ;
    skos:definition "A field site from which a soil sample is taken or observation is made."@en ;
    skos:inScheme <http://linked.data.gov.au/def/geological-sites> ;
    skos:notation "sh" ;
    skos:prefLabel "Soil Horizon"@en .

gsqst:tailings a skos:Concept ;
    skos:altLabel "Mine Dump"@en ;
    skos:broader gsqst:field-site ;
    skos:definition "An accumulation of material left over after the process of separating the valuable fraction from the uneconomic fraction (gangue) of an ore."@en ;
    skos:inScheme <http://linked.data.gov.au/def/geological-sites> ;
    skos:notation "tl" ;
    skos:prefLabel "Tailings"@en .

gsqst:waterbody a skos:Concept ;
    skos:broader gsqst:field-site ;
    dct:source "Source: Merriam-Webster Dictionary" ;
    skos:definition "Any significant accumulation of typically non-flowing water, generally on a planet's surface. The term most often refers to oceans, seas, and lakes, but it includes smaller pools of water such as ponds, wetlands, or more rarely, puddles."@en ;
    skos:inScheme <http://linked.data.gov.au/def/geological-sites> ;
    skos:notation "wb" ;
    skos:prefLabel "Waterbody"@en .

gsqst:watercourse a skos:Concept ;
    skos:altLabel "Brook"@en,
        "Canal"@en,
        "Creek"@en,
        "Drain"@en,
        "River"@en,
        "Stream"@en ;
    skos:broader gsqst:field-site ;
    skos:definition "The channel that a flowing body of water follows."@en ;
    skos:inScheme <http://linked.data.gov.au/def/geological-sites> ;
    skos:notation "wc" ;
    skos:prefLabel "Watercourse"@en .

gsqst:base-station a skos:Concept ;
    skos:definition "A site of known location for the samplng or measurement of a property or as a point with a known measurement of a property for the calibration of a larger survey."@en ;
    skos:inScheme <http://linked.data.gov.au/def/geological-sites> ;
    skos:notation "bs" ;
    skos:prefLabel "Base Station"@en ;
    skos:topConceptOf <http://linked.data.gov.au/def/geological-sites> .

gsqst:borehole a skos:Concept ;
    skos:altLabel "Auger Hole"@en,
        "Bore"@en,
        "Core Hole"@en,
        "Corehole"@en,
        "Drillhole"@en,
        "Well"@en ;
    skos:definition "A Borehole is a hole in the ground designed to exchange (or facilitate the exchange of) fluids between a subsurface reservoir and the surface (or another reservoir), or to enable the detection and measurement of rock properties.  Boreholes are the sites of extraction or rock samples, as core or cuttings, and fluid samples. A Borehole has a single Origin and all Wellbore(s) that extend from this Well Origin are parts of the Borehole. Sources: PPDM What Is A Well, GSQ."@en ;
    skos:scopeNote "In the context of administration by a regulatory body, a borehole exists as an entity once proposed-to-be-drilled, prior to drilling and having a tangible physical manifestation."@en ;
    skos:inScheme <http://linked.data.gov.au/def/geological-sites> ;
    skos:notation "bh" ;
    skos:prefLabel "Borehole"@en ;
    skos:topConceptOf <http://linked.data.gov.au/def/geological-sites> .

gsqst:cutting a skos:Concept ;
    skos:altLabel "Excavation"@en,
        "Tunnel"@en ;
    skos:definition "A man-made excavation through the earth typically for infrastucture and/or transport."@en ;
    skos:inScheme <http://linked.data.gov.au/def/geological-sites> ;
    skos:notation "ct" ;
    skos:prefLabel "Cutting"@en ;
    skos:topConceptOf <http://linked.data.gov.au/def/geological-sites> .

gsqst:mine a skos:Concept ;
    skos:altLabel "Quarry"@en ;
    dct:source "Source: Merriam-Webster Dictionary" ;
    skos:definition "A pit or excavation in the earth from which mineral substances are taken. Source: Merriam-Webster Dictionary"@en ;
    skos:inScheme <http://linked.data.gov.au/def/geological-sites> ;
    skos:notation "mi" ;
    skos:prefLabel "Mine"@en ;
    skos:topConceptOf <http://linked.data.gov.au/def/geological-sites> .

gsqst:mineral-occurrence a skos:Concept ;
    dct:source "Source: USGS" ;
    skos:definition "A concentration of a mineral (usually, but not necessarily, considered in terms of some commodity, such as copper, barite or gold) that is considered valuable by someone somewhere, or that is of scientific or technical interest."@en ;
    skos:inScheme <http://linked.data.gov.au/def/geological-sites> ;
    skos:notation "mo" ;
    skos:prefLabel "Mineral Occurrence"@en ;
    skos:topConceptOf <http://linked.data.gov.au/def/geological-sites> .

gsqst:mineral-deposit a skos:Concept ;
    skos:definition "A major mineral occurrence that has a defined resource, usually associated with a major exploration project."@en ;
    skos:inScheme <http://linked.data.gov.au/def/geological-sites> ;
    skos:notation "md" ;
    skos:prefLabel "Mineral Deposit"@en ;
    skos:topConceptOf <http://linked.data.gov.au/def/geological-sites> .

gsqst:pit a skos:Concept ;
    skos:altLabel "Box Cut"@en,
        "Costean"@en,
        "Trench"@en ;
    skos:definition "A type of excavation or depression in the ground used for analysis or sample collection."@en ;
    skos:inScheme <http://linked.data.gov.au/def/geological-sites> ;
    skos:notation "pt" ;
    skos:prefLabel "Pit"@en ;
    skos:topConceptOf <http://linked.data.gov.au/def/geological-sites> .

#gsqst:wellbore a skos:Concept ;
#    skos:altLabel "Branch"@en,
#        "Sidetrack"@en ;
#    skos:definition "A Wellbore is a path of drilled footage, from the Borehole Origin (top/start) to a terminating point (bottom/end). There are one or more Wellbores in a planned or drilled Borehole, namely the original Wellbore, and a Wellbore for each intended, actual or accidental sidetrack. Each Wellbore has a unique terminating point. A deepening of an existing Wellbore is considered a new Wellbore with the same Borehole Origin. Source: PPDM What Is A  Well."@en ;
#    skos:inScheme <http://linked.data.gov.au/def/geological-sites> ;
#    skos:notation "wl" ;
#    skos:prefLabel "Wellbore"@en ;
#    skos:topConceptOf <http://linked.data.gov.au/def/geological-sites> .

gsqst:wellbore-interval a skos:Concept ;
    skos:altLabel "Drilling Interval"@en,
        "Well Section"@en,
        "Well Segment"@en ;
    skos:definition "A Wellbore Segment is a unique drilled interval within the Well, either the original Wellbore from the Well Origin to the terminating point, or additional footage from a point in an existing Wellbore to a new terminating point. A Wellbore Segment is generally drilled in one continuous operation. The starting point of a new Wellbore Segment is a point in an existing Wellbore from which additional footage is drilled. This point may be a kick-off or sidetrack point or the original terminating point of the original Wellbore, as in a deepening. Wellbore Intervals typically are drilled with a constant diameter and may commonly be referred to by a functional name e.g. Conductor, Surface, Intermediate, Production. Sources: PPDM What is a Well, GSQ"@en ;
    skos:inScheme <http://linked.data.gov.au/def/geological-sites> ;
    skos:notation "wi" ;
    skos:prefLabel "Wellbore Interval"@en ;
    skos:topConceptOf <http://linked.data.gov.au/def/geological-sites> .

gsqst:survey-site a skos:Concept ;
    skos:altLabel "Project"@en ;
    skos:definition "The location of a survey."@en ;
    skos:inScheme <http://linked.data.gov.au/def/geological-sites> ;
    skos:notation "ss" ;
    skos:prefLabel "Survey Site"@en ;
    skos:topConceptOf <http://linked.data.gov.au/def/geological-sites> .

gsqst:field-site a skos:Concept ;
    skos:altLabel "Dig site"@en ;
    skos:definition "An area, transect, or point where samples are taken or observations are made directly from earth materials."@en ;
    skos:inScheme <http://linked.data.gov.au/def/geological-sites> ;
    skos:notation "fs" ;
    skos:prefLabel "Field Site"@en ;
    skos:topConceptOf <http://linked.data.gov.au/def/geological-sites> .
