@prefix dc: <http://purl.org/dc/elements/1.1/> .
@prefix dct: <http://purl.org/dc/terms/> .
@prefix owl: <http://www.w3.org/2002/07/owl#> .
@prefix rdf: <http://www.w3.org/1999/02/22-rdf-syntax-ns#> .
@prefix rdfs: <http://www.w3.org/2000/01/rdf-schema#> .
@prefix skos: <http://www.w3.org/2004/02/skos/core#> .
@prefix obst: <http://linked.data.gov.au/def/observation-type/> .
@prefix xml: <http://www.w3.org/XML/1998/namespace> .
@prefix xsd: <http://www.w3.org/2001/XMLSchema#> .

<http://linked.data.gov.au/def/observation-type> a owl:Ontology , skos:ConceptScheme ;
    dct:created "2020-02-05T13:54:52"^^xsd:dateTime ;
    dct:creator "Geological Survey of Queensland" ;
    dct:modified "2020-02-05T13:54:52"^^xsd:dateTime ;
    dct:source "Compiled by the Geological Survey of Queensland" ;
    skos:definition "The one-off event of examining a Feature. The observation performed may produce samples."@en ;
    skos:hasTopConcept obst:atmospheric,
        obst:directional,
        obst:electrical,
        obst:electromagnetic,
        obst:geochemistry,
        obst:geotechnical,
        obst:geothermics,
        obst:gravity,
        obst:hydrochemistry,
        obst:magnetic,
        obst:magnetotelluric,
        obst:petrophysical,
        obst:photographic,
        obst:physical-geology,
        obst:process,
        obst:radiometric,
        obst:seismic,
        obst:spectral,
        obst:spatial,
        obst:velocity ;
    skos:prefLabel "Observation Type"@en .

obst:airborne a skos:Collection ;
    skos:definition "Observations in which the observation equipment is mounted to an aircraft such as an airplane, helicopter, balloon, or aerial drone."@en ;
    skos:member obst:atmospheric,
        obst:electromagnetic,
        #obst:gravity-gradiometry,
        obst:magnetic,
        #obst:magnetic-gradiometry,
        obst:photographic,
        obst:radiometric,
        obst:spatial,
        obst:spectral ;     
    skos:prefLabel "Airborne"@en .

obst:downhole a skos:Collection ;
    skos:definition "Observations where equipment is conveyed down a borehole to record measurements of borehole, rock, or fluid attributes."@en ;
    skos:member obst:directional,
        obst:electrical,
        obst:electromagnetic,
        obst:geochemistry,
        obst:geotechnical,
        obst:gravity,
        #obst:gravity-gradiometry,
        obst:magnetic,
        #obst:magnetic-gradiometry,
        #obst:organic-geochemistry,
        obst:petrophysical,
        obst:photographic,
        obst:radiometric,
        obst:spectral,
        obst:velocity ;
    skos:prefLabel "Downhole"@en .

obst:ground a skos:Collection ;
    skos:definition "Observations undertaken at ground level or a solid subsurface level such as an underground mine floor. This may include surface collection of rocks, soil, water or other physical samples; geophysical observations from surface locations; handheld photography."@en ;
    skos:member obst:atmospheric,
        obst:electrical,
        obst:electromagnetic,
        obst:geochemistry,
        obst:geotechnical,
        obst:geothermics,
        obst:gravity,
        #obst:gravity-gradiometry,
        obst:hydrochemistry,
        obst:magnetic,
        #obst:magnetic-gradiometry,
        obst:magnetotelluric,
        #obst:organic-geochemistry,
        #obst:passive-seismic,
        obst:physical-geology,
        obst:radiometric,
        obst:seismic,
        obst:spatial ;
    skos:prefLabel "Ground"@en .

obst:procedural a skos:Collection ;
    skos:definition "Observations undertaken as part of an overall sampling procedure to modify existing samples, or create new sub-samples from existing samples."@en ;
    skos:member obst:process ;
    skos:prefLabel "Procedural"@en .

obst:satellite a skos:Collection ;
    skos:definition "Observations in which the observation equipment is mounted to a platform outside the earth's atmosphere. Typically in a stable orbit such as a satellite, space station, or shuttle."@en ;
    skos:member obst:gravity,
        obst:magnetic,
        obst:photographic,
        obst:spectral,
        obst:spatial ;
    skos:prefLabel "Satellite"@en .

#obst:passive-seismic a skos:Concept ;
#    skos:broader obst:seismic ;
#    skos:definition "A seismic observation using passive and natural noise sources. Typically capturing cumulative information over extended recording periods."@en ;
#    skos:inScheme <http://linked.data.gov.au/def/observation-type> ;
#    skos:notation "pv" ;
#    skos:prefLabel "Passive seismic"@en .

obst:directional a skos:Concept ;
    skos:definition "The process of recording the subsurface geometry of a borehole i.e. direction and position of a wellbore."@en ;
    skos:inScheme <http://linked.data.gov.au/def/observation-type> ;
    skos:notation "ds" ;
    skos:prefLabel "Directional"@en ;
    skos:topConceptOf <http://linked.data.gov.au/def/observation-type> .

obst:geothermics a skos:Concept ;
    skos:definition "A observation measuring variations of heat flow within the Earth."@en ;
    skos:inScheme <http://linked.data.gov.au/def/observation-type> ;
    skos:notation "ge" ;
    skos:prefLabel "Geothermics"@en ;
    skos:topConceptOf <http://linked.data.gov.au/def/observation-type> .

obst:hydrochemistry a skos:Concept ;
    skos:definition "A observation of the chemical and physical properties of surface or ground water."@en ;
    skos:inScheme <http://linked.data.gov.au/def/observation-type> ;
    skos:notation "hy" ;
    skos:prefLabel "Hydrochemistry"@en ;
    skos:topConceptOf <http://linked.data.gov.au/def/observation-type> .

obst:magnetotelluric a skos:Concept ;
    skos:altLabel "MT"@en,
        "MT Observation"@en ;
    skos:definition "A observation where recordings of the Earths electric and magnetic fields are taken concurrently to determine the subsurface electrical resistivity at a range of scales"@en ;
    skos:inScheme <http://linked.data.gov.au/def/observation-type> ;
    skos:notation "mt" ;
    skos:prefLabel "Magnetotelluric"@en ;
    skos:topConceptOf <http://linked.data.gov.au/def/observation-type> .

#obst:organic-geochemistry a skos:Concept ;
#    skos:broader obst:geochemistry ;
#    skos:definition "A geochemistry observation specifically determining organic chemical properties. Typically performed for material such as coal and oil."@en ;
#    skos:inScheme <http://linked.data.gov.au/def/observation-type> ;
#    skos:notation "og" ;
#    skos:prefLabel "Organic Geochemistry"@en .

obst:petrophysical a skos:Concept ;
    skos:altLabel "Wireline"@en ;
    skos:definition "The process of recording various physical, chemical, electrical, or other properties of the rock/fluid mixtures penetrated by a borehole."@en ;
    skos:inScheme <http://linked.data.gov.au/def/observation-type> ;
    skos:notation "pp" ;
    skos:prefLabel "Petrophysical"@en ;
    skos:topConceptOf <http://linked.data.gov.au/def/observation-type> .

obst:velocity a skos:Concept ;
    skos:altLabel "Checkshot"@en ;
    skos:definition "The process of recording the average sonic velocity with depth down a borehole."@en ;
    skos:inScheme <http://linked.data.gov.au/def/observation-type> ;
    skos:notation "vl" ;
    skos:prefLabel "Velocity"@en ;
    skos:topConceptOf <http://linked.data.gov.au/def/observation-type> .

obst:physical-geology a skos:Concept ;
    skos:altLabel "Field Mapping"@en ;
    skos:definition "A observation of physical geological features such as outcrop samples, structural measurements, sedimentological and stratigraphic observations."@en ;
    skos:inScheme <http://linked.data.gov.au/def/observation-type> ;
    skos:notation "pg" ;
    skos:prefLabel "Physical Geology"@en ;
    skos:topConceptOf <http://linked.data.gov.au/def/observation-type> .

obst:process a skos:Concept ;
    skos:altLabel "processing"@en,
        "reprocessing"@en,
        "resampling"@en ;
    skos:definition "A sampling procedure performed on an existing sample to alter the sample or generate a new sub-sample or set of sub-samples. This may include seismic processing and reprocessing."@en ;
    skos:inScheme <http://linked.data.gov.au/def/observation-type> ;
    skos:notation "ps" ;
    skos:prefLabel "Process"@en ;
    skos:topConceptOf <http://linked.data.gov.au/def/observation-type> .

obst:atmospheric a skos:Concept ;
    skos:definition "A observation measuring chemical and physical properties of the atmosphere."@en ;
    skos:inScheme <http://linked.data.gov.au/def/observation-type> ;
    skos:notation "at" ;
    skos:prefLabel "Atmospheric"@en ;
    skos:topConceptOf <http://linked.data.gov.au/def/observation-type> .

obst:electrical a skos:Concept ;
    skos:altLabel "Electrical Resistance"@en,
        "Electrical Sounding"@en,
        "IP"@en,
        "Induced Polarisation"@en,
        "MIMDAS"@en,
        "SP"@en,
        "Schlumberger Observation"@en,
        "Spontenous Pontential"@en,
        "Vertical Profiling"@en,
        "Wiener Observation"@en ;
    skos:definition "A observation measuring electrical currents as they travel through conductive pathways in the near surface."@en ;
    skos:inScheme <http://linked.data.gov.au/def/observation-type> ;
    skos:notation "es" ;
    skos:prefLabel "Electrical"@en ;
    skos:topConceptOf <http://linked.data.gov.au/def/observation-type> .

obst:geotechnical a skos:Concept ;
    skos:altLabel "Geomechanical"@en ;
    skos:definition "A observation measuring the physical and mechanical properties of rocks, soil and earth material with particular focus on rock strength and competence."@en ;
    skos:inScheme <http://linked.data.gov.au/def/observation-type> ;
    skos:notation "gt" ;
    skos:prefLabel "Geotechnical"@en ;
    skos:topConceptOf <http://linked.data.gov.au/def/observation-type> .

#obst:gravity-gradiometry a skos:Concept ;
#    skos:altLabel "Full tensor gravimetry"@en ;
#    skos:broader obst:gravity ;
#    skos:definition "A variation of gravity observation where the gradient of the gravity field is measured instead of the field directly."@en ;
#    skos:inScheme <http://linked.data.gov.au/def/observation-type> ;
#    skos:notation "gy" ;
#    skos:prefLabel "Gravity gradiometry"@en .

#obst:magnetic-gradiometry a skos:Concept ;
#    skos:broader obst:magnetic ;
#    skos:definition "A variation of magnetic observation which measured the gradient of the magnetic field instead of the field."@en ;
#    skos:inScheme <http://linked.data.gov.au/def/observation-type> ;
#    skos:notation "my" ;
#    skos:prefLabel "Magnetic gradiometry"@en .

obst:seismic a skos:Concept ;
    skos:definition "A observation using the interaction of seismic waves with sub-surface features of the earth to determine properties and morphology of those features."@en ;
    skos:inScheme <http://linked.data.gov.au/def/observation-type> ;
    skos:notation "ss" ;
    skos:prefLabel "Seismic"@en ;
    skos:topConceptOf <http://linked.data.gov.au/def/observation-type> .

obst:electromagnetic a skos:Concept ;
    skos:altLabel "EM"@en,
        "EM Observation"@en ;
    skos:definition "A observation measuring induced electromagnetic fields from the earth to determine the resistive/conductive structure of the earth."@en ;
    skos:inScheme <http://linked.data.gov.au/def/observation-type> ;
    skos:notation "em" ;
    skos:prefLabel "Electromagnetic"@en ;
    skos:topConceptOf <http://linked.data.gov.au/def/observation-type> .

obst:geochemistry a skos:Concept ;
    skos:definition "A observation where the chemical properties of rocks, soil, or other geological material is assessed to determine mineralogical and/or elemental composition."@en ;
    skos:inScheme <http://linked.data.gov.au/def/observation-type> ;
    skos:notation "gc" ;
    skos:prefLabel "Geochemistry"@en ;
    skos:topConceptOf <http://linked.data.gov.au/def/observation-type> .

obst:photographic a skos:Concept ;
    skos:definition "A observation using standard photographic equipment for image capture without intention for spectral analysis. Including land-based geological photography."@en ;
    skos:inScheme <http://linked.data.gov.au/def/observation-type> ;
    skos:notation "ph" ;
    skos:prefLabel "Photographic"@en ;
    skos:topConceptOf <http://linked.data.gov.au/def/observation-type> .

obst:radiometric a skos:Concept ;
    skos:altLabel "Gamma Logs"@en,
        "Gamma-Ray Spectrography"@en ;
    skos:definition "A observation where the emissions of natural gamma-rays are recorded to determine the quantity of radioelements (Potassium, Uranium, Thorium)."@en ;
    skos:inScheme <http://linked.data.gov.au/def/observation-type> ;
    skos:notation "rm" ;
    skos:prefLabel "Radiometric"@en ;
    skos:topConceptOf <http://linked.data.gov.au/def/observation-type> .

obst:spectral a skos:Concept ;
    skos:altLabel "hyperspectral"@en ;
    skos:definition "A observation capturing image information and intensity-per-wavelength-band to be used for spectral analysis e.g. ASTER, MODIS."@en ;
    skos:inScheme <http://linked.data.gov.au/def/observation-type> ;
    skos:notation "sp" ;
    skos:prefLabel "Spectral"@en ;
    skos:topConceptOf <http://linked.data.gov.au/def/observation-type> .

obst:spatial a skos:Concept ;
    skos:definition "A observation measuring the spatial characteristics of an object or region."@en ;
    skos:inScheme <http://linked.data.gov.au/def/observation-type> ;
    skos:notation "st" ;
    skos:prefLabel "Spatial"@en ;
    skos:topConceptOf <http://linked.data.gov.au/def/observation-type> .

obst:gravity a skos:Concept ;
    skos:definition "A observation where the variation of the Earth's gravity field in measured to determine the distribution of density in the region"@en ;
    skos:inScheme <http://linked.data.gov.au/def/observation-type> ;
    skos:notation "gv" ;
    skos:prefLabel "Gravity"@en ;
    skos:topConceptOf <http://linked.data.gov.au/def/observation-type> .

obst:magnetic a skos:Concept ;
    skos:altLabel "aeromagnetics"@en ;
    skos:definition "A observation where the variations of the Earth's magnetic field is measured to determine the distribution of magnetic minerals (predominately magnetite)"@en ;
    skos:inScheme <http://linked.data.gov.au/def/observation-type> ;
    skos:notation "mg" ;
    skos:prefLabel "Magnetic"@en ;
    skos:topConceptOf <http://linked.data.gov.au/def/observation-type> .
