#Version 0.3

@prefix dc: <http://purl.org/dc/elements/1.1/> .
@prefix dct: <http://purl.org/dc/terms/> .
@prefix owl: <http://www.w3.org/2002/07/owl#> .
@prefix rdf: <http://www.w3.org/1999/02/22-rdf-syntax-ns#> .
@prefix rdfs: <http://www.w3.org/2000/01/rdf-schema#> .
@prefix skos: <http://www.w3.org/2004/02/skos/core#> .
@prefix xml: <http://www.w3.org/XML/1998/namespace> .
@prefix xsd: <http://www.w3.org/2001/XMLSchema#> .
@prefix gmps: <http://linked.data.gov.au/def/qld-resource-permit-status/> .

<http://linked.data.gov.au/def/qld-resource-permit-status> a owl:Ontology .

gmps:conceptScheme a skos:ConceptScheme ;
    dct:created "2019-09-13"^^xsd:date ;
    dct:creator "Geological Survey of Queensland" ;
    dct:source "https://myminesonline.business.qld.gov.au" ;
    skos:definition "The stage in the life cycle of a Queensland Resource Permit."@en ;
    skos:hasTopConcept gmps:application,
        gmps:granted,
        gmps:non-current ;
    skos:prefLabel "Queensland Resource Permit Status"@en .

gmps:abandoned a skos:Concept ;
    skos:definition "The Resource Permit was not granted and the Application has been abandoned by the applicant."@en ;
    skos:broader gmps:application,
    skos:inScheme gmps:conceptScheme ;
    skos:prefLabel "Abandoned"@en .

gmps:competing-application a skos:Concept ;
    skos:definition "This application represents a competing application that was lodged on the same date for the same mineral."@en ;
    skos:broader gmps:application,
        gmps:granted ;
    skos:inScheme gmps:conceptScheme ;
    skos:prefLabel "Competing application"@en .

gmps:conditionally-surrendered a skos:Concept ;
    skos:definition "The Resource Permit has been surrendered in favour of a new Resource Permit."@en ;
    skos:broader gmps:application,
    skos:inScheme gmps:conceptScheme ;
    skos:prefLabel "Conditionally surrendered"@en .

gmps:conversion-of-ml-to-mc a skos:Concept ;
    skos:definition "The Mining Lease has been converted to a Mining Claim."@en ;
    skos:broader gmps:granted ;
    skos:inScheme gmps:conceptScheme ;
    skos:prefLabel "Conversion of ML to MC"@en .

gmps:finalised a skos:Concept ;
    skos:definition "The Resource Permit has no outstanding requirements."@en ;
    skos:broader gmps:non-current ;
    skos:inScheme gmps:conceptScheme ;
    skos:prefLabel "Finalised"@en .

gmps:preferred-tenderer a skos:Concept ;
    skos:definition "The applicant is the preferred tenderer."@en ;
    skos:broader gmps:application,
    skos:inScheme gmps:conceptScheme ;
    skos:prefLabel "Preferred Tenderer"@en .

gmps:priority-application a skos:Concept ;
    skos:definition "Priority Application substatus is accorded to the application of highest rank that has been determined by the Department from an assessment and ranking of competitive applications (generally for Exploration Permits Mineral) lodged on the same day for the same mineral and for the same area."@en ;
    skos:broader gmps:application ;
    skos:inScheme gmps:conceptScheme ;
    skos:prefLabel "Priority Applicant"@en .

gmps:ranked a skos:Concept ;
    skos:definition "The application for the Resource Permit is a Ranked Application, pending grant of a Priority Application."@en ;
    skos:broader gmps:application ;
    skos:inScheme gmps:conceptScheme ;
    skos:prefLabel "Ranked"@en .

gmps:renewal-lodged a skos:Concept ;
    skos:definition "The Application of Renewal for the Resource Permit has been lodged."@en ;
    skos:broader gmps:granted,
    skos:inScheme gmps:conceptScheme ;
    skos:prefLabel "Renewal lodged"@en .

gmps:renewal-withdrawn a skos:Concept ;
    skos:definition "The Application of Renewal for the Resource Permit has been withdrawn."@en ;
    skos:broader gmps:granted,
    skos:inScheme gmps:conceptScheme ;
    skos:prefLabel "Renewal withdrawn"@en .

gmps:replacement-permit-application a skos:Concept ;
    skos:definition "The application represents a Replacement Permit Application. Such applications relate to petroleum and gas permits for which a holder can replace a 1923 Act permit for a permit under the Petroleum and Gas Act 2004."@en ;
    skos:broader gmps:application,
        gmps:granted ;
    skos:inScheme gmps:conceptScheme ;
    skos:prefLabel "Replacement Permit Application"@en .

gmps:unfinalised a skos:Concept ;
    skos:definition "The Resource Permit has been terminated, but there are some outstanding requirements to be completed, to be compliant with the resources legislation."@en ;
    skos:broader gmps:non-current,
    skos:inScheme gmps:conceptScheme ;
    skos:prefLabel "Unfinalised"@en .

gmps:unsuccessful-application a skos:Concept ;
    skos:definition "The application represents an unsuccessful application."@en ;
    skos:broader gmps:application,
    skos:inScheme gmps:conceptScheme ;
    skos:prefLabel "Unsuccessful application"@en .

gmps:granted a skos:Concept ;
    skos:definition "The Resource Permit has been approved under the Resource Authority Legislation"@en ;
    skos:inScheme gmps:conceptScheme ;
    skos:prefLabel "Granted"@en ;
    skos:topConceptOf gmps:conceptScheme .

gmps:application a skos:Concept ;
    skos:definition "An application has been submitted and an outcome is pending."@en ;
    skos:inScheme gmps:conceptScheme ;
    skos:prefLabel "Application"@en ;
    skos:topConceptOf gmps:conceptScheme .

gmps:non-current a skos:Concept ;
    skos:definition "The Resource Permit has been terminated in the system and is longer current."@en ;
    skos:inScheme gmps:conceptScheme ;
    skos:prefLabel "Non-current"@en ;
    skos:topConceptOf gmps:conceptScheme .
