@prefix svymh: <http://linked.data.gov.au/def/survey-method/> .
@prefix dc: <http://purl.org/dc/elements/1.1/> .
@prefix dct: <http://purl.org/dc/terms/> .
@prefix owl: <http://www.w3.org/2002/07/owl#> .
@prefix rdf: <http://www.w3.org/1999/02/22-rdf-syntax-ns#> .
@prefix rdfs: <http://www.w3.org/2000/01/rdf-schema#> .
@prefix sdo: <https://schema.org/> .
@prefix skos: <http://www.w3.org/2004/02/skos/core#> .
@prefix xml: <http://www.w3.org/XML/1998/namespace> .
@prefix xsd: <http://www.w3.org/2001/XMLSchema#> .

<http://linked.data.gov.au/def/survey-method> a owl:Ontology, 
        skos:ConceptScheme ;
    dct:created "2020-02-10"^^xsd:date ;
    dct:creator <http://linked.data.gov.au/org/gsq> ;
    dct:modified "2020-05-14"^^xsd:date ;
    dct:publisher <http://linked.data.gov.au/org/gsq> ;
    dct:source "Compiled by the Geological Survey of Queensland" ;
    skos:definition "The method of collection used by a survey."@en ;
    skos:hasTopConcept svymh:airborne,
        svymh:downhole,
        svymh:ground,
        svymh:laboratory,
        svymh:marine,
        svymh:satellite ;
    skos:prefLabel "Survey Method"@en .

<http://linked.data.gov.au/org/gsq> a sdo:Organization ;
    sdo:name "Geological Survey of Queensland" .

svymh:airborne a skos:Concept ;
    skos:altLabel "Aerial"@en ;
    skos:definition "Surveys in which the surveying equipment is mounted to an aircraft such as an airplane, helicopter, balloon, or aerial drone."@en ;
    skos:inScheme <http://linked.data.gov.au/def/survey-method> ;
    skos:prefLabel "Airborne"@en ;
    skos:topConceptOf <http://linked.data.gov.au/def/survey-method> .
    
svymh:fixed-wing a skos:Concept ;
    skos:altLabel "Airplane"@en,
        "Aeroplane"@en,
        "Glider"@en ;
    skos:broader svymh:airborne ;
    skos:definition "A heavier-than-air flying machine that is capable of flight using wings that generate lift caused by the aircraft's forward airspeed and the shape of the wings. Source:Wikipedia"@en ;
    skos:inScheme <http://linked.data.gov.au/def/survey-method> ;
    skos:prefLabel "Fixed Wing"@en .

svymh:rotary-wing a skos:Concept ;
    skos:altLabel "Helicopter"@en,
        "Rotorcraft"@en,
        "Gyrodyne"@en,
        "Autogyro"@en ;
    skos:broader svymh:airborne ;
    skos:definition "A heavier-than-air flying machine that generates lift using rotary wings or rotor blades, which revolve around a mast."@en ;
    skos:inScheme <http://linked.data.gov.au/def/survey-method> ;
    skos:prefLabel "Rotary Wing"@en .
    
svymh:balloon a skos:Concept ;
    skos:altLabel "Hot Air Balloon"@en,
        "Gas Balloon"@en,
        "Hot-Air Balloon"@en ;
    skos:broader svymh:airborne ;
    skos:definition "A lighter-than-air flying machine that generates lift using buoyancy and lacks a means to propel and direct itself through the air. A balloon may be free, moving with the wind, or tethered to a fixed point. "@en ;
    skos:inScheme <http://linked.data.gov.au/def/survey-method> ;
    skos:prefLabel "Balloon"@en .
        
svymh:airship a skos:Concept ;
    skos:altLabel "Air-Ship"@en,
        "Air Ship"@en,
        "Dirigible"@en, 
        "Zeppelin"@en ;
    skos:broader svymh:airborne ;
    skos:definition "A lighter-than-air flying machine that generates lift using buoyancy and has a means to propel and direct itself through the air under its own power, such as a rotor."@en ;
    skos:inScheme <http://linked.data.gov.au/def/survey-method> ;
    skos:prefLabel "Airship"@en .

svymh:uav a skos:Concept ;
    skos:altLabel "UAV"@en,
        "Aerial Drone"@en,
        "Uncrewed aerial vehicle"@en ;
    skos:broader svymh:airborne ;
    skos:definition "An aircraft without a human pilot on board and a type of unmanned vehicle. UAVs may operate with various degrees of autonomy: either under remote control by a human operator or autonomously by onboard computers."@en ;
    skos:inScheme <http://linked.data.gov.au/def/survey-method> ;
    skos:prefLabel "Drone"@en .

svymh:downhole a skos:Concept ;
    skos:altLabel "Borehole"@en ;
    skos:definition "Surveys where equipment is conveyed down a borehole to record measurements of borehole, rock, or fluid attributes."@en ;
    skos:inScheme <http://linked.data.gov.au/def/survey-method> ;
    skos:prefLabel "Downhole"@en ;
    skos:topConceptOf <http://linked.data.gov.au/def/survey-method> .

svymh:mwd a skos:Concept ;
    skos:hiddenLabel "Logging While Drilling"@en,
        "LWD"@en,
        "L.W.D"@en,
        "L.W.D."@en ;
    skos:altLabel "MWD"@en,
        "M.W.D."@en,
        "M.W.D"@en ;
    skos:broader svymh:downhole ;
    skos:definition "A survey where data is acquired while the hole is being drilled, from sensors integrated within the drill string ."@en ;
    skos:inScheme <http://linked.data.gov.au/def/survey-method> ;
    skos:prefLabel "Measurement While Drilling"@en .

svymh:pipe-conveyed a skos:Concept ;
    skos:altLabel "on-pipe"@en,
        "on pipe"@en;
    skos:broader svymh:downhole ;
    skos:definition "A survey where data is acquired from logging tools attached to the drill string, while the well is not actively drilling."@en ;
    skos:inScheme <http://linked.data.gov.au/def/survey-method> ;
    skos:prefLabel "Pipe Conveyed"@en .

svymh:well-tractor a skos:Concept ;
    skos:altLabel "borehole tractor"@en;
    skos:broader svymh:downhole ;
    skos:definition "A survey where data is acquired from logging tools integrated in a Well Tractor, a device that moves through a wellbore using wheels or tracks pushed against the side of the borehole."@en ;
    skos:inScheme <http://linked.data.gov.au/def/survey-method> ;
    skos:prefLabel "Well Tractor"@en .

svymh:wireline a skos:Concept ;
    skos:altLabel "wireline logging"@en;
    skos:broader svymh:downhole ;
    skos:definition "A survey where data is acquired from logging tools lowered and raised within a borehole on a wireline or cable."@en ;
    skos:inScheme <http://linked.data.gov.au/def/survey-method> ;
    skos:prefLabel "Wireline"@en .

svymh:ground a skos:Concept ;
    skos:altLabel "Land"@en ;
    skos:definition "Surveys undertaken at ground level or a solid subsurface level such as an underground mine floor. This may include surface collection of rocks, soil, water or other physical samples; geophysical surveys from surface locations; handheld photography."@en ;
    skos:inScheme <http://linked.data.gov.au/def/survey-method> ;
    skos:prefLabel "Ground"@en ;
    skos:topConceptOf <http://linked.data.gov.au/def/survey-method> .

svymh:fixed-location a skos:Concept ;
    skos:altLabel "Permanent Location"@en ;
    skos:definition "Surveys undertaken at ground level from a set of fixed locations."@en ;
    skos:inScheme <http://linked.data.gov.au/def/survey-method> ;
    skos:prefLabel "Fixed location"@en ;
    skos:topConceptOf <http://linked.data.gov.au/def/survey-method> .

svymh:human a skos:Concept ;
    skos:altLabel "Manual"@en,
        "Field Work"@en,
        "In Person"@en ;
    skos:broader svymh:ground ;
    skos:definition "A ground based survey where data is acquired from a human conducting work on-foot."@en ;
    skos:inScheme <http://linked.data.gov.au/def/survey-method> ;
    skos:prefLabel "Human"@en .

svymh:vehicle a skos:Concept ;
    skos:altLabel "Car"@en,
        "Truck"@en,
        "Ute"@en,
        "Vehicle Conveyed"@en ;
    skos:broader svymh:ground ;
    skos:definition "A ground based survey where data is acquired from instruments mounted to a vehicle."@en ;
    skos:inScheme <http://linked.data.gov.au/def/survey-method> ;
    skos:prefLabel "Vehicle"@en .

svymh:laboratory a skos:Concept ;
    skos:altLabel "Rig Site"@en,
        "Mobile Lab"@en,
        "Lab"@en,
        "Mobile"@en ;
    skos:definition "Surveys undertaken on samples that are no-longer in-situ e.g. spectral surveys of core by hylogger in a laboratory, CoreScan in a rig site, XRF analysis of collected samples."@en ;
    skos:inScheme <http://linked.data.gov.au/def/survey-method> ;
    skos:prefLabel "Laboratory"@en ;
    skos:topConceptOf <http://linked.data.gov.au/def/survey-method> .

svymh:marine a skos:Concept ;
    skos:altLabel "Oceanic"@en,
        "Sea"@en,
        "On Water"@en;
    skos:definition "Surveys undertaken at or below the surface of a body of water such as an ocean, sea, or lake."@en ;
    skos:inScheme <http://linked.data.gov.au/def/survey-method> ;
    skos:prefLabel "Marine"@en ;
    skos:topConceptOf <http://linked.data.gov.au/def/survey-method> .

svymh:boat a skos:Concept ;
    skos:altLabel "Ship"@en,
        "Hovercraft"@en,
        "Sailboat"@en,
        "Motorboat"@en ;
    skos:broader svymh:marine ;
    skos:definition "A marine survey where data is acquired from instruments attached to a mobile water craft on the water's surface."@en ;
    skos:inScheme <http://linked.data.gov.au/def/survey-method> ;
    skos:prefLabel "Boat"@en .

svymh:diver a skos:Concept ;
    skos:altLabel "SCUBA"@en,
        "SCUBA Diver"@en;
    skos:broader svymh:marine ;
    skos:definition "A marine survey where data is acquired by a human conveying the instruments of measurement."@en ;
    skos:inScheme <http://linked.data.gov.au/def/survey-method> ;
    skos:prefLabel "Diver"@en .

svymh:float a skos:Concept ;
    skos:altLabel "Pontoon"@en,
        "Floating Dock"@en,
        "Floating Jetty"@en,
        "Floating Pier"@en ;
    skos:broader svymh:marine ;
    skos:definition "A marine survey where data is acquired from instruments operated from a fixed, buoyant, structure at the water's surface."@en ;
    skos:inScheme <http://linked.data.gov.au/def/survey-method> ;
    skos:prefLabel "Float"@en .

svymh:submarine a skos:Concept ;
    skos:altLabel "Sub"@en,
        "Submersible"@en,
        "Underwater"@en ;
    skos:broader svymh:marine ;
    skos:definition "A marine survey where data is acquired by a human piloted watercraft operating under the surface of the water. Surveys may be performed by submarines or submersibles."@en ;
    skos:inScheme <http://linked.data.gov.au/def/survey-method> ;
    skos:prefLabel "Submarine"@en .

svymh:uuv a skos:Concept ;
    skos:altLabel "UUV"@en,
        "Underwater Drone"@en,
        "AUV"@en,
        "Autonomous underwater vehicle"@en,
        "ROUV"@en,
        "remotely operated underwater vehicles"@en ;
    skos:broader svymh:marine ;
    skos:definition "A marine survey where data is acquired by a watercraft, without an onboard human pilot, operating under the surface of the water."@en ;
    skos:inScheme <http://linked.data.gov.au/def/survey-method> ;
    skos:prefLabel "Unmanned underwater vehicle"@en .

svymh:satellite a skos:Concept ;
    skos:definition "Surveys in which the surveying equipment is mounted to a platform outside the earth's atmosphere. Typically in a stable orbit such as a satellite, space station, or shuttle."@en ;
    skos:inScheme <http://linked.data.gov.au/def/survey-method> ;
    skos:prefLabel "Satellite"@en ;
    skos:topConceptOf <http://linked.data.gov.au/def/survey-method> .