 @prefix srt: <http://linked.data.gov.au/def/survey-relationship-type/> .


 @prefix dc: <http://purl.org/dc/elements/1.1/> .
 @prefix dct: <http://purl.org/dc/terms/> .
 @prefix owl: <http://www.w3.org/2002/07/owl#> .
 @prefix rdf: <http://www.w3.org/1999/02/22-rdf-syntax-ns#> .
 @prefix rdfs: <http://www.w3.org/2000/01/rdf-schema#> .
 @prefix skos: <http://www.w3.org/2004/02/skos/core#> .
 @prefix xsd: <http://www.w3.org/2001/XMLSchema#> .


<http://linked.data.gov.au/def/survey-relationship-type> a owl:Ontology .

srt:conceptScheme a skos:ConceptScheme ;
dct:created "2020-02-20T12:00:39+10:00"^^xsd:dateTime ;
dct:modified "2020-02-20T12:02:43+10:00"^^xsd:dateTime ;
dct:source "Developed by the Geological Survey of Queensland." ;
skos:definition "The relationships that exist between surveys. "@en ;
dct:creator "Geological Survey of Queensland" ;
skos:prefLabel "Survey relationship type"@en .

srt:infill a skos:Concept ; skos:broader :follow-up ; skos:definition "A follow-up survey designed to increase the spatial resolution of a pre-existing survey, usually using the same parameters to ensure data compatibility. "@en ; skos:inScheme srt:conceptScheme ; skos:prefLabel "Infill"@en  .
srt:reprocessing a skos:Concept ; skos:topConceptOf srt:conceptScheme ; skos:definition "Generating a new digital sample by reprocessing pre-existing raw data with a new algorithm or processing parameters."@en ; skos:inScheme srt:conceptScheme ; skos:prefLabel "Reprocessing"@en  .
srt:resampling a skos:Concept ; skos:topConceptOf srt:conceptScheme ; skos:definition "Generating new physical sample by changing the form of an existing sample. "@en ; skos:inScheme srt:conceptScheme ; skos:prefLabel "Resampling"@en  .
srt:extension a skos:Concept ; skos:broader :follow-up ; skos:definition "A follow-up survey designed to extend the coverage of an existing survey, usually using the same parameters to ensure data compatibility. "@en ; skos:inScheme srt:conceptScheme ; skos:prefLabel "Extension"@en  .
srt:repeat a skos:Concept ; skos:broader :follow-up ; skos:definition "A follow-up survey designed to replicate the coverage and parameters of an existing survey. A repeat survey may, for example, be needed to correct errors or to reproduce results from the initial survey. "@en ; skos:inScheme srt:conceptScheme ; skos:prefLabel "Repeat"@en  .
srt:follow-up a skos:Concept ; skos:topConceptOf srt:conceptScheme ; skos:definition "A survey that was designed on the basis of lessons learned from an initial survey. "@en ; skos:inScheme srt:conceptScheme ; skos:prefLabel "Follow-up"@en  .
srt:same-project a skos:Concept ; skos:topConceptOf srt:conceptScheme ; skos:definition "Surveys that were conducted, concurrently or otherwise, during the course of a single project. "@en ; skos:inScheme srt:conceptScheme ; skos:prefLabel "Same project"@en  .






