PREFIX bhse: <https://linked.data.gov.au/def/borehole-status-event/>
PREFIX dcterms: <http://purl.org/dc/terms/>
PREFIX owl: <http://www.w3.org/2002/07/owl#>
PREFIX rdfs: <http://www.w3.org/2000/01/rdf-schema#>
PREFIX sdo: <http://schema.org/>
PREFIX skos: <http://www.w3.org/2004/02/skos/core#>
PREFIX xsd: <http://www.w3.org/2001/XMLSchema#>

bhse:pggd-02
    a skos:Collection ;
    dcterms:provenance "Compiled by the Geological Survey of Queensland" ;
    skos:definition "The borehole events that may be reported via a PGGD-02 form to change the status of a borehole."@en ;
    skos:member
        bhse:abandonment ,
        bhse:alteration ,
        bhse:borehole-never-drilled ,
        bhse:completion ,
        bhse:petroleum-production-commencement ;
    skos:prefLabel "PGGD-02"@en ;
.

bhse:pggd-04
    a skos:Collection ;
    dcterms:provenance "Compiled by the Geological Survey of Queensland" ;
    skos:definition "The borehole events that may be reported via a PGGD-04 form to change the status of a borehole."@en ;
    skos:member
        bhse:hydraulic-fracturing-abandoned ,
        bhse:hydraulic-fracturing-altered ,
        bhse:hydraulic-fracturing-completed ,
        bhse:hydraulic-fracturing-partial ,
        bhse:hydraulic-fracturing-related ;
    skos:prefLabel "PGGD-04"@en ;
.

bhse:conversion-to-water-observation
    a skos:Concept ;
    dcterms:provenance "Compiled by the Geological Survey of Queensland" ;
    rdfs:isDefinedBy <https://linked.data.gov.au/def/borehole-status-event> ;
    skos:definition "A Notice of completion of conversion of petroleum well to water observation bore. Lodgement of Form WRA-05A. This event changes purpose from Petroleum, or narrower term, to Water and status to Monitoring."@en ;
    skos:inScheme <https://linked.data.gov.au/def/borehole-status-event> ;
    skos:prefLabel "Conversion to water observation borehole"@en ;
    skos:topConceptOf <https://linked.data.gov.au/def/borehole-status-event> ;
.

bhse:conversion-to-water-observation-on-notice
    a skos:Concept ;
    dcterms:provenance "Compiled by the Geological Survey of Queensland" ;
    rdfs:isDefinedBy <https://linked.data.gov.au/def/borehole-status-event> ;
    skos:definition "A Notice of intention to convert a petroleum well to a water observation bore. Lodgement of Form PA-42. This event is a recording of an intended activity which does not change the status."@en ;
    skos:inScheme <https://linked.data.gov.au/def/borehole-status-event> ;
    skos:prefLabel "Conversion to water observation borehole on notice"@en ;
    skos:topConceptOf <https://linked.data.gov.au/def/borehole-status-event> ;
.

bhse:conversion-to-water-supply
    a skos:Concept ;
    dcterms:provenance "Compiled by the Geological Survey of Queensland" ;
    rdfs:isDefinedBy <https://linked.data.gov.au/def/borehole-status-event> ;
    skos:definition "A Notice of completion of conversion of petroleum well to water supply bore. Lodgement of Form WRA-05A. The event changes the borehole purpose from Petroleum, or narrower term, to Water and the status to Water Supply."@en ;
    skos:inScheme <https://linked.data.gov.au/def/borehole-status-event> ;
    skos:prefLabel "Conversion to water supply borehole"@en ;
    skos:topConceptOf <https://linked.data.gov.au/def/borehole-status-event> ;
.

bhse:conversion-to-water-supply-on-notice
    a skos:Concept ;
    dcterms:provenance "Compiled by the Geological Survey of Queensland" ;
    rdfs:isDefinedBy <https://linked.data.gov.au/def/borehole-status-event> ;
    skos:definition "A Notice of intention to convert a petroleum well to a water supply bore. Lodgement of Form PA-42. This event is a recording of an intended activity that does not change the status."@en ;
    skos:inScheme <https://linked.data.gov.au/def/borehole-status-event> ;
    skos:prefLabel "Conversion to water supply borehole on notice"@en ;
    skos:topConceptOf <https://linked.data.gov.au/def/borehole-status-event> ;
.

bhse:decommissioning
    a skos:Concept ;
    dcterms:provenance "Compiled by the Geological Survey of Queensland" ;
    rdfs:isDefinedBy <https://linked.data.gov.au/def/borehole-status-event> ;
    skos:definition "A Notice of decommissioning a well, water observation bore, water monitoring bore or water supply bore. Lodgement of Form MMOL-44. Decommissioning refers to the act of permanently shutting-in and abandoning a borehole. This event changes the borehole status to Capped and Abandoned."@en ;
    skos:inScheme <https://linked.data.gov.au/def/borehole-status-event> ;
    skos:prefLabel "Decommissioning"@en ;
    skos:topConceptOf <https://linked.data.gov.au/def/borehole-status-event> ;
.

bhse:drilling-of-borehole-on-notice
    a skos:Concept ;
    dcterms:provenance "Compiled by the Geological Survey of Queensland" ;
    rdfs:isDefinedBy <https://linked.data.gov.au/def/borehole-status-event> ;
    skos:definition "A Notice of intention to drill a petroleum well or bore. Lodgement of Form PGGD-01. This event creates a borehole entity under the Proposed status."@en ;
    skos:inScheme <https://linked.data.gov.au/def/borehole-status-event> ;
    skos:prefLabel "Drilling of borehole on notice"@en ;
    skos:topConceptOf <https://linked.data.gov.au/def/borehole-status-event> ;
.

bhse:hydraulic-fracturing-on-notice
    a skos:Concept ;
    dcterms:provenance "Compiled by the Geological Survey of Queensland" ;
    rdfs:isDefinedBy <https://linked.data.gov.au/def/borehole-status-event> ;
    skos:definition "A Notice of intention to carry out hydraulic fracturing activities. Lodgement of Form PGGD-O3. This event is a recording of an intended activity that does not change the status."@en ;
    skos:inScheme <https://linked.data.gov.au/def/borehole-status-event> ;
    skos:prefLabel "Hydraulic fracturing on notice"@en ;
    skos:topConceptOf <https://linked.data.gov.au/def/borehole-status-event> ;
.

bhse:manual-update
    a skos:Concept ;
    dcterms:provenance "Compiled by the Geological Survey of Queensland" ;
    rdfs:isDefinedBy <https://linked.data.gov.au/def/borehole-status-event> ;
    skos:definition "A manual update to an existing borehole status or a manual creation of a new borehole status."@en ;
    skos:inScheme <https://linked.data.gov.au/def/borehole-status-event> ;
    skos:prefLabel "Manual Update or Creation"@en ;
    skos:topConceptOf <https://linked.data.gov.au/def/borehole-status-event> ;
.

bhse:abandonment
    a skos:Concept ;
    dcterms:provenance "Compiled by the Geological Survey of Queensland" ;
    rdfs:isDefinedBy <https://linked.data.gov.au/def/borehole-status-event> ;
    skos:definition "Notice of when a borehole is shut-in and permanently closed. Lodgement of Form PGGD-02. This event will change the borehole status to Capped and Abandoned."@en ;
    skos:inScheme <https://linked.data.gov.au/def/borehole-status-event> ;
    skos:prefLabel "Abandonment"@en ;
    skos:topConceptOf <https://linked.data.gov.au/def/borehole-status-event> ;
.

bhse:alteration
    a skos:Concept ;
    dcterms:provenance "Compiled by the Geological Survey of Queensland" ;
    rdfs:isDefinedBy <https://linked.data.gov.au/def/borehole-status-event> ;
    skos:definition "Notice of the activities that occur after completion of the initial drilling activities of the borehole. Lodgement of Form PGGD-02. This event is a recording of a reportable activity that does not change the status."@en ;
    skos:inScheme <https://linked.data.gov.au/def/borehole-status-event> ;
    skos:prefLabel "Alteration"@en ;
    skos:topConceptOf <https://linked.data.gov.au/def/borehole-status-event> ;
.

bhse:borehole-never-drilled
    a skos:Concept ;
    dcterms:provenance "Compiled by the Geological Survey of Queensland" ;
    rdfs:isDefinedBy <https://linked.data.gov.au/def/borehole-status-event> ;
    skos:altLabel "Drilling of borehole cancelled"@en ;
    skos:definition "Recording that the intended drilling of a borehole was cancelled and abandoned and drilling was never undertaken. This event changes the status to Never Used."@en ;
    skos:inScheme <https://linked.data.gov.au/def/borehole-status-event> ;
    skos:prefLabel "Never Drilled"@en ;
    skos:topConceptOf <https://linked.data.gov.au/def/borehole-status-event> ;
.

bhse:completion
    a skos:Concept ;
    dcterms:provenance "Compiled by the Geological Survey of Queensland" ;
    rdfs:isDefinedBy <https://linked.data.gov.au/def/borehole-status-event> ;
    skos:definition "Notice that the initial drilling activities of the borehole have been completed. Lodgement of Form PGGD-02. This event will change the borehole status from Proposed to Completed."@en ;
    skos:inScheme <https://linked.data.gov.au/def/borehole-status-event> ;
    skos:prefLabel "Completion"@en ;
    skos:topConceptOf <https://linked.data.gov.au/def/borehole-status-event> ;
.

bhse:hydraulic-fracturing-abandoned
    a skos:Concept ;
    dcterms:provenance "Compiled by the Geological Survey of Queensland" ;
    rdfs:isDefinedBy <https://linked.data.gov.au/def/borehole-status-event> ;
    skos:definition "A Notice that the intended hydraulic fracturing activity was cancelled and abandoned, the activity was never undertaken and no fluid injection occurred. Lodgement of Form PGGD-04. Borehole status does not change"@en ;
    skos:inScheme <https://linked.data.gov.au/def/borehole-status-event> ;
    skos:prefLabel "Hydraulic fracturing abandoned"@en ;
    skos:topConceptOf <https://linked.data.gov.au/def/borehole-status-event> ;
.

bhse:hydraulic-fracturing-altered
    a skos:Concept ;
    dcterms:provenance "Compiled by the Geological Survey of Queensland" ;
    rdfs:isDefinedBy <https://linked.data.gov.au/def/borehole-status-event> ;
    skos:definition "A Notice of completion of hydraulic fracturing activities, but with alteration. Lodgement of Form PGGD-04. The original well fracturing objectives were required to be changed due to unforeseen circumstances throughout the process, but the altered hydraulic fracturing activities were carried out and completed. This event is a recording of a reportable activity which does not change the status."@en ;
    skos:inScheme <https://linked.data.gov.au/def/borehole-status-event> ;
    skos:prefLabel "Hydraulic fracturing completed with alteration"@en ;
    skos:topConceptOf <https://linked.data.gov.au/def/borehole-status-event> ;
.

bhse:hydraulic-fracturing-completed
    a skos:Concept ;
    dcterms:provenance "Compiled by the Geological Survey of Queensland" ;
    rdfs:isDefinedBy <https://linked.data.gov.au/def/borehole-status-event> ;
    skos:definition "A Notice of completion of hydraulic fracturing activities. Lodgement of Form PGGD-04. This event is a recording of a reportable activity which does not change the status"@en ;
    skos:inScheme <https://linked.data.gov.au/def/borehole-status-event> ;
    skos:prefLabel "Hydraulic fracturing completed"@en ;
    skos:topConceptOf <https://linked.data.gov.au/def/borehole-status-event> ;
.

bhse:hydraulic-fracturing-partial
    a skos:Concept ;
    dcterms:provenance "Compiled by the Geological Survey of Queensland" ;
    rdfs:isDefinedBy <https://linked.data.gov.au/def/borehole-status-event> ;
    skos:definition "A Notice of a partial completion of hydraulic fracturing activities. The full well fracturing objectives were not acheived, but a portion of the planned hydraulic fracturing activities were carried out. Lodgement of Form PGGD-04. This event is a recording of a reportable activity which does not change the status"@en ;
    skos:inScheme <https://linked.data.gov.au/def/borehole-status-event> ;
    skos:prefLabel "Hydraulic fracturing partially completed"@en ;
    skos:topConceptOf <https://linked.data.gov.au/def/borehole-status-event> ;
.

bhse:hydraulic-fracturing-related
    a skos:Concept ;
    dcterms:provenance "Compiled by the Geological Survey of Queensland" ;
    rdfs:isDefinedBy <https://linked.data.gov.au/def/borehole-status-event> ;
    skos:definition "A Notice of other events or activities relating to hydraulic fracturing activities such as: industrial accident/s, adverse environmental condition/s (such as too wet, too hot, electrical storm etc.) at the wellsite, or concerns over workplace health and safety.  Lodgement of Form PGGD-04.  This event is a recording of a reportable activity which does not change the status."@en ;
    skos:inScheme <https://linked.data.gov.au/def/borehole-status-event> ;
    skos:prefLabel "Hydraulic fracturing related events"@en ;
    skos:topConceptOf <https://linked.data.gov.au/def/borehole-status-event> ;
.

bhse:petroleum-production-commencement
    a skos:Concept ;
    dcterms:provenance "Compiled by the Geological Survey of Queensland" ;
    rdfs:isDefinedBy <https://linked.data.gov.au/def/borehole-status-event> ;
    skos:definition "The production of petroleum from a well or bore has been confirmed by notice (PGGD-02) or through a Petroleum Production Report as defined under of the Petroleum and Gas (General Provisions) Regulation. This changes the borehole status to on-production."@en ;
    skos:inScheme <https://linked.data.gov.au/def/borehole-status-event> ;
    skos:prefLabel "Commencement of Production"@en ;
    skos:topConceptOf <https://linked.data.gov.au/def/borehole-status-event> ;
.

<https://linked.data.gov.au/org/gsq>
    a sdo:Organization ;
    sdo:name "Geological Survey of Queensland" ;
    sdo:url "http://www.business.qld.gov.au/industries/mining-energy-water/resources/geoscience-information/gsq"^^xsd:anyURI ;
.

<https://linked.data.gov.au/def/borehole-status-event>
    a
        owl:Ontology ,
        skos:ConceptScheme ;
    dcterms:created "2020-01-21"^^xsd:date ;
    dcterms:creator <https://linked.data.gov.au/org/gsq> ;
    dcterms:modified "2020-07-07"^^xsd:date ;
    dcterms:provenance "Compiled by the Geological Survey of Queensland" ;
    dcterms:publisher <https://linked.data.gov.au/org/gsq> ;
    skos:definition "Events that occur during the lifecycle a borehole that affect the status or history, or convert a borehole from one purpose to another."@en ;
    skos:hasTopConcept
        bhse:abandonment ,
        bhse:alteration ,
        bhse:borehole-never-drilled ,
        bhse:completion ,
        bhse:conversion-to-water-observation ,
        bhse:conversion-to-water-observation-on-notice ,
        bhse:conversion-to-water-supply ,
        bhse:conversion-to-water-supply-on-notice ,
        bhse:decommissioning ,
        bhse:drilling-of-borehole-on-notice ,
        bhse:hydraulic-fracturing-abandoned ,
        bhse:hydraulic-fracturing-altered ,
        bhse:hydraulic-fracturing-completed ,
        bhse:hydraulic-fracturing-on-notice ,
        bhse:hydraulic-fracturing-partial ,
        bhse:hydraulic-fracturing-related ,
        bhse:manual-update ,
        bhse:petroleum-production-commencement ;
    skos:prefLabel "Borehole Status Event"@en ;
.

