PREFIX : <https://linked.data.gov.au/def/core-size/>
PREFIX agldwgstatus: <https://linked.data.gov.au/def/reg-statuses/>
PREFIX cs: <https://linked.data.gov.au/def/core-size>
PREFIX dcterms: <http://purl.org/dc/terms/>
PREFIX reg: <http://purl.org/linked-data/registry#>
PREFIX rdfs: <http://www.w3.org/2000/01/rdf-schema#>
PREFIX sdo: <https://schema.org/>
PREFIX skos: <http://www.w3.org/2004/02/skos/core#>
PREFIX xsd: <http://www.w3.org/2001/XMLSchema#>

:AQ
    a skos:Concept ;
    rdfs:isDefinedBy cs: ;
    skos:definition "Standard Q sized bit with an outside diameter of 48mm and an inside diameter of 27mm."@en ;
    skos:historyNote "Created from the WIMS MIRO brainstorming session" ;
    skos:inScheme cs: ;
    skos:notation "AQ" ;
    skos:prefLabel "AQ"@en ;
    skos:topConceptOf cs: ;
.

:BQ
    a skos:Concept ;
    rdfs:isDefinedBy cs: ;
    skos:definition "Standard Q sized bit with an outside diameter of 60mm and an inside diameter of 36.5mm."@en ;
    skos:historyNote "Created from the WIMS MIRO brainstorming session" ;
    skos:inScheme cs: ;
    skos:notation "BQ" ;
    skos:prefLabel "BQ"@en ;
    skos:topConceptOf cs: ;
.

:NQ
    a skos:Concept ;
    rdfs:isDefinedBy cs: ;
    skos:definition "Standard Q sized bit with an outside diameter of 75.7mm and an inside diameter of 47.6mm."@en ;
    skos:historyNote "Created from the WIMS MIRO brainstorming session" ;
    skos:inScheme cs: ;
    skos:notation "NQ" ;
    skos:prefLabel "NQ"@en ;
    skos:topConceptOf cs: ;
.

:HQ
    a skos:Concept ;
    rdfs:isDefinedBy cs: ;
    skos:definition "Standard Q sized bit with an outside diameter of 96mm and an inside diameter of 63.5mm."@en ;
    skos:historyNote "Created from the WIMS MIRO brainstorming session" ;
    skos:inScheme cs: ;
    skos:notation "HQ" ;
    skos:prefLabel "HQ"@en ;
    skos:topConceptOf cs: ;
.

:HQ3
    a skos:Concept ;
    rdfs:isDefinedBy cs: ;
    skos:definition "Standard Q sized bit with an outside diameter of 96mm and an inside diameter of 61.1mm."@en ;
    skos:historyNote "Created from the WIMS MIRO brainstorming session" ;
    skos:inScheme cs: ;
    skos:notation "HQ3" ;
    skos:prefLabel "HQ3"@en ;
    skos:topConceptOf cs: ;
.

:PQ
    a skos:Concept ;
    rdfs:isDefinedBy cs: ;
    skos:definition "Standard Q sized bit with an outside diameter of 122.6mm and an inside diameter of 85mm."@en ;
    skos:historyNote "Created from the WIMS MIRO brainstorming session" ;
    skos:inScheme cs: ;
    skos:notation "PQ" ;
    skos:prefLabel "PQ"@en ;
    skos:topConceptOf cs: ;
.

:PQ3
    a skos:Concept ;
    rdfs:isDefinedBy cs: ;
    skos:definition "Standard Q sized bit with an outside diameter of 122.6mm and an inside diameter of 83mm."@en ;
    skos:historyNote "Created from the WIMS MIRO brainstorming session" ;
    skos:inScheme cs: ;
    skos:notation "PQ3" ;
    skos:prefLabel "PQ3"@en ;
    skos:topConceptOf cs: ;
.

:CHD76
    a skos:Concept ;
    rdfs:isDefinedBy cs: ;
    skos:definition "Standard Q sized bit with an outside diameter of 75.7mm and an inside diameter of 43.5mm."@en ;
    skos:historyNote "Created from the WIMS MIRO brainstorming session" ;
    skos:inScheme cs: ;
    skos:notation "CHD76" ;
    skos:prefLabel "CHD 76"@en ;
    skos:topConceptOf cs: ;
.

:CHD101
    a skos:Concept ;
    rdfs:isDefinedBy cs: ;
    skos:definition "Standard Q sized bit with an outside diameter of 101.3mm and an inside diameter of 63.5mm."@en ;
    skos:historyNote "Created from the WIMS MIRO brainstorming session" ;
    skos:inScheme cs: ;
    skos:notation "CHD101" ;
    skos:prefLabel "CHD 101"@en ;
    skos:topConceptOf cs: ;
.

:CHD134
    a skos:Concept ;
    rdfs:isDefinedBy cs: ;
    skos:definition "Standard Q sized bit with an outside diameter of 134.0mm and an inside diameter of 85mm."@en ;
    skos:historyNote "Created from the WIMS MIRO brainstorming session" ;
    skos:inScheme cs: ;
    skos:notation "CHD134" ;
    skos:prefLabel "CHD 134"@en ;
    skos:topConceptOf cs: ;
.

<https://linked.data.gov.au/org/gsq>
    a sdo:Organization ;
    sdo:name "Geological Survey of Queensland" ;
    sdo:url "https://www.business.qld.gov.au/industries/mining-energy-water/resources/geoscience-information/gsq"^^xsd:anyURI ;
.

cs:
    a skos:ConceptScheme ;
    sdo:keywords <http://linked.data.gov.au/def/earth-science-data-category/geology-not-elsewhere-classified> ;
    reg:status agldwgstatus:experimental ;
    skos:definition "Core Size"@en ;
    skos:hasTopConcept
        :AQ ,
        :BQ ,
        :NQ ,
        :HQ ,
        :HQ3 ,
        :PQ ,
        :PQ3 ,
        :CHD76 ,
        :CHD101 ,
        :CHD134 ;
    skos:historyNote "Created from the WIMS MIRO brainstorming session" ;
    skos:notation "core-size" ;
    skos:prefLabel "Core Size"@en ;
    sdo:copyrightNotice "(c) Geological Survey of Queensland, 2024" ;
    sdo:creator <https://linked.data.gov.au/org/gsq> ;
    dcterms:created "2024-08-07"^^xsd:date ;
    dcterms:modified "2024-08-16"^^xsd:date ;
    sdo:license <https://purl.org/NET/rdflicense/cc-by4.0> ;
    sdo:publisher <https://linked.data.gov.au/org/gsq> ;
.

