PREFIX : <http://linked.data.gov.au/def/geologic-feature-relationship/> # <<< To register #
PREFIX agldwg????: <https://linked.data.gov.au/def/?????/>
PREFIX cs: <http://linked.data.gov.au/def/geologic-feature-relationship>
PREFIX dcterms: <http://purl.org/dc/terms/>
PREFIX owl: <http://www.w3.org/2002/07/owl#>
PREFIX rdfs: <http://www.w3.org/2000/01/rdf-schema#>
PREFIX reg: <http://purl.org/linked-data/registry#>
PREFIX sdo: <https://schema.org/>
PREFIX skos: <http://www.w3.org/2004/02/skos/core#>
PREFIX xsd: <http://www.w3.org/2001/XMLSchema#>

:hasPart
    a skos:Concept ;
    skos:historyNote "Compiled by the Geological Survey of Queensland" ;
    rdfs:isDefinedBy cs: ;
    owl:inverseOf strel:partOf ;
    skos:definition "A Geologic Feature has a constituent part represented by another Feature."@en ;
    skos:example "The Evergreen Formation (Surat Basin) has a part represented by the Westgrove Ironstone Member."@en ;
    skos:inScheme cs: ;
    skos:prefLabel "Has Part"@en ;
    skos:topConceptOf cs: ;
.

:intertonguesWith
    a skos:Concept ;
    skos:historyNote "Compiled by the Geological Survey of Queensland" ;
    rdfs:isDefinedBy cs: ;
    skos:altLabel
        "Interdigitated with"@en ,
        "Interfingered with"@en ;
    skos:definition "Where the contact between laterally adjacent rock bodies breaks down into a series of wedges or tongues that penetrate the adjacent rock body and pinch out individually, essentially embracing the �disappearance� of both rock bodies (After: Gary et al., 1977; Wikipedia [Contact (geology)], accessed 07.09.2022)."@en ;
    skos:inScheme cs: ;
    skos:prefLabel "Intertongues with"@en ;
    skos:topConceptOf cs: ;
.

:intrudes
    a skos:Concept ;
    skos:historyNote "Compiled by the Geological Survey of Queensland" ;
    rdfs:isDefinedBy cs: ;
    skos:definition "Where the igneous or non-igneous intrusive rock unit intrudes/cross-cuts another lithologic rock unit, which may also be an (older) intrusive rock unit."@en ;
    skos:inScheme cs: ;
    skos:prefLabel "Intrudes"@en ;
    skos:topConceptOf cs: ;
.

:isAdjacentTo
    a skos:Concept ;
    skos:historyNote "Compiled by the Geological Survey of Queensland" ;
    rdfs:isDefinedBy cs: ;
    skos:definition "Describes a geologic feature that is next to or bordering another feature."@en ;
    skos:inScheme cs: ;
    skos:prefLabel "Is Adjacent To"@en ;
    skos:topConceptOf cs: ;
.

:isAssociatedWith
    a skos:Concept ;
    skos:historyNote "Compiled by the Geological Survey of Queensland" ;
    rdfs:isDefinedBy cs: ;
    skos:definition "Indicates a general relationship where two geologic features are commonly found together or have a related occurrence."@en ;
    skos:inScheme cs: ;
    skos:prefLabel "Is Associated With"@en ;
    skos:topConceptOf cs: ;
.

:isComagmaticWith
    a skos:Concept ;
    skos:historyNote "Compiled by the Geological Survey of Queensland" ;
    rdfs:isDefinedBy cs: ;
    skos:definition "Where the igneous rock unit, based on its chemistry and mineralogic features, is considered to have been derived from the same parent magma as another igneous rock unit (After: mindat.org; accessed 13.09.2022)."@en ;
    skos:inScheme cs: ;
    skos:prefLabel "Is Comagmatic With"@en ;
    skos:topConceptOf cs: ;
.

:isConformableWith
    a skos:Concept ;
    skos:historyNote "Compiled by the Geological Survey of Queensland" ;
    rdfs:isDefinedBy cs: ;
    skos:definition "The rock unit, including both lithologic rock units and non-lithologic rock units (such as biostratigraphic units/zones, magnetostratigraphic units, etc.) is conformable with the underlying rock unit, the overlying rock unit, or both, there being continuity of deposition between them, such that their contacts (boundaries, surfaces) are common to both and do not embrace hiatus."@en ;
    skos:inScheme cs: ;
    skos:prefLabel "Is Conformable With"@en ;
    skos:topConceptOf cs: ;
.

:isEquivalentTo
    a skos:Concept ;
    skos:historyNote "Compiled by the Geological Survey of Queensland" ;
    rdfs:isDefinedBy cs: ;
    skos:definition "Where the lithostratigraphic rock unit is laterally equivalent stratigraphically (lithostratigraphically) to another lithostratigraphic rock unit; or a biostratigraphic rock unit/zone is equivalent laterally to another such unit; or a biostratigraphic unit in one scheme/zonation is equivalent to another such unit in a different scheme/zonation that has either current or past application."@en ;
    skos:inScheme cs: ;
    skos:prefLabel "Is Equivalent To"@en ;
    skos:topConceptOf cs: ;
.

:isFaultedAgainst
    a skos:Concept ;
    skos:historyNote "Compiled by the Geological Survey of Queensland" ;
    rdfs:isDefinedBy cs: ;
    skos:definition "Where the lithologic rock unit is faulted against another lithologic rock unit."@en ;
    skos:inScheme cs: ;
    skos:prefLabel "Is Faulted Against"@en ;
    skos:topConceptOf cs: ;
.

:isGradationalInto
    a skos:Concept ;
    skos:historyNote "Compiled by the Geological Survey of Queensland" ;
    rdfs:isDefinedBy cs: ;
    skos:definition "Where the lithologic rock unit is gradational (lithologically) into a stratigraphically underlying or overlying rock unit, or gradational into a laterally adjacent (equivalent) rock unit."@en ;
    skos:inScheme cs: ;
    skos:prefLabel "Is Gradational Into"@en ;
    skos:topConceptOf cs: ;
.

:isIntrudedBy
    a skos:Concept ;
    skos:historyNote "Compiled by the Geological Survey of Queensland" ;
    rdfs:isDefinedBy cs: ;
    skos:definition "Where the lithologic rock unit (which may be an igneous or non-igneous intrusive rock unit) is intruded/cross-cut by an igneous or non-igneous intrusive rock unit."@en ;
    skos:inScheme cs: ;
    skos:prefLabel "Is Intruded By"@en ;
    skos:topConceptOf cs: ;
.

:isOverlappedStratigraphicallyBy
    a skos:Concept ;
    skos:historyNote "Compiled by the Geological Survey of Queensland" ;
    rdfs:isDefinedBy cs: ;
    skos:definition "Where the lithologic rock is overlapped stratigraphically by a younger, onlapping lithologic rock unit."@en ;
    skos:inScheme cs: ;
    skos:prefLabel "Is Overlapped Stratigraphically By"@en ;
    skos:topConceptOf cs: ;
.

:isPartOf
    a skos:Concept ;
    skos:historyNote "Compiled by the Geological Survey of Queensland" ;
    rdfs:isDefinedBy cs: ;
    owl:inverseOf strel:hasPart ;
    skos:definition "A geologic feature is part of another geologic feature."@en ;
    skos:example "The Westgrove Ironstone Member is part of the Evergreen Formation (Surat Basin)."@en ;
    skos:inScheme cs: ;
    skos:prefLabel "Is Part Of"@en ;
    skos:topConceptOf cs: ;
.

:isSimilarTo
    a skos:Concept ;
    skos:historyNote "Compiled by the Geological Survey of Queensland" ;
    rdfs:isDefinedBy cs: ;
    skos:definition "Specifies that two geologic features share similar properties or characteristics but are not identical."@en ;
    skos:inScheme cs: ;
    skos:prefLabel "Is Similar To"@en ;
    skos:topConceptOf cs: ;
.

:offsteps
    a skos:Concept ;
    skos:historyNote "Compiled by the Geological Survey of Queensland" ;
    rdfs:isDefinedBy cs: ;
    skos:definition "Where the lithologic rock unit sits unconformably on progressively older/underlying lithologic rock units."@en ;
    skos:inScheme cs: ;
    skos:prefLabel "Offsteps"@en ;
    skos:topConceptOf cs: ;
.

:overlapsStratigraphically
    a skos:Concept ;
    skos:historyNote "Compiled by the Geological Survey of Queensland" ;
    rdfs:isDefinedBy cs: ;
    skos:altLabel "Onlaps"@en ;
    skos:definition "Where the lithologic rock unit extends progressively across an erosion surface, stratigraphically overlapping/onlapping an older/underlying lithologic rock unit."@en ;
    skos:inScheme cs: ;
    skos:prefLabel "Overlaps Stratigraphically"@en ;
    skos:topConceptOf cs: ;
.

:overlies
    a skos:Concept ;
    skos:historyNote "Compiled by the Geological Survey of Queensland" ;
    rdfs:isDefinedBy cs: ;
    skos:altLabel "Underlain by"@en ;
    skos:definition "Where the rock unit (e.g., a lithostratigraphic rock unit, biostratigraphic rock unit/zone, etc.) overlies (is underlain by) another lithologic rock unit (of the same kind/type: lithologic, biostratigraphic, etc.)."@en ;
    skos:inScheme cs: ;
    skos:prefLabel "Overlies"@en ;
    skos:topConceptOf cs: ;
.

:underlies
    a skos:Concept ;
    skos:historyNote "Compiled by the Geological Survey of Queensland" ;
    rdfs:isDefinedBy cs: ;
    skos:altLabel "Overlain by"@en ;
    skos:definition "Where the rock unit (e.g., a lithostratigraphic rock unit, biostratigraphic rock unit/zone, etc.) underlies (is overlain by) another lithologic rock unit (of the same kind/type: lithologic, biostratigraphic, etc.)."@en ;
    skos:inScheme cs: ;
    skos:prefLabel "Underlies"@en ;
    skos:topConceptOf cs: ;
.

:unknown
    a skos:Concept ;
    skos:historyNote "Compiled by the Geological Survey of Queensland" ;
    rdfs:isDefinedBy cs: ;
    skos:definition "Where the relationship between two geological features is unknown."@en ;
    skos:inScheme cs: ;
    skos:prefLabel "Unknown"@en ;
    skos:topConceptOf cs: ;
.

:withIntercalationOf
    a skos:Concept ;
    skos:historyNote "Compiled by the Geological Survey of Queensland" ;
    rdfs:isDefinedBy cs: ;
    skos:definition "Where the lithologic rock unit at hand contains a rock layer or rock layers of a different character, especially where relatively thin strata of one kind of material alternate with thicker strata of some other kind of material, such being the case, for example, with lava flows, beds of shale, and concordant intrusive sills being �intercalated� in a large body of sandstone (thus with sedimentary/stratigraphic and intrusive intercalations). Also: The tectonic/structural insertion/intercalation of rock layers into a pre-existing body of rock (e.g., by thrusting); or the occurrence of a particular fossil horizon between fossil zones (biostratigraphic rock units) of a different character (the latter also representing a stratigraphic intercalation) [Modified from: Gary et al., 1977]."@en ;
    skos:inScheme cs: ;
    skos:prefLabel "With Intercalation Of"@en ;
    skos:topConceptOf cs: ;
.

cs:
    a
        owl:Ontology ,
        skos:ConceptScheme ;
    dcterms:created "2020-01-21"^^xsd:date ; <<<<<<<<<<<<<<<<<<<<<<<<<<<<<<<<<<<<<<<<<<<<<<
    dcterms:creator <https://linked.data.gov.au/org/gsq> ;
    dcterms:modified "2023-03-16"^^xsd:date ; <<<<<<<<<<<<<<<<<<<<<<<<<<<<<<<<<<<<<<
    skos:historyNote "Compiled by the Geological Survey of Queensland" ;
    dcterms:publisher <https://linked.data.gov.au/org/gsq> ;
    reg:status agldwgstatus:stable ; <<<<<<<<<<<<<<<<<<<<<<<<<<<<<< 
    skos:definition "The relationship between two geological features, for example: Stratigraphically (�vertically�) at a boundary in common between two rock units of the same type/kind (lithostratigraphic, biostratigraphic, etc.); laterally (geographically) between two lithologic rock units with a gradational change in lithology, or laterally between two rock units with an abrupt change in lithologic or biostratigraphic facies; and lithostratigraphically or biostratigraphically (both from a geographic perspective), based respectively on lithostratigraphic or biostratigraphic correlation. Not only included are relationships between any two types of lithologic rock units, such as between two stratiform (lithostratigraphic) units or between two nonstratiform (non-lithostratigraphic) units, but also between a stratiform unit and a nonstratiform unit, such as an intrusive rock unit."@en ;
     
   skos:hasTopConcept
    :hasPart ,
    :intertonguesWith ,
    :intrudes ,
    :isAdjacentTo ,
    :isAssociatedWith ,
    :isComagmaticWith ,
    :isConformableWith ,
    :isEquivalentTo ,
    :isFaultedAgainst ,
    :isGradationalInto ,
    :isIntrudedBy ,
    :isOverlappedStratigraphicallyBy ,
    :isPartOf ,
    :isSimilarTo ,
    :offsteps ,
    :overlapsStratigraphically ,
    :overlies ,
    :underlies ,
    :unknown ,
    :withIntercalationOf ;
skos:prefLabel "Geologic Feature Relationships"@en ;
.

<https://linked.data.gov.au/org/gsq>
    a sdo:Organization ;
    sdo:name "Geological Survey of Queensland" ;
    sdo:url "http://www.business.qld.gov.au/industries/mining-energy-water/resources/geoscience-information/gsq"^^xsd:anyURI ;
.
