PREFIX dcterms: <http://purl.org/dc/terms/>
PREFIX grt: <https://linked.data.gov.au/def/georesource-report/>
PREFIX owl: <http://www.w3.org/2002/07/owl#>
PREFIX rdfs: <http://www.w3.org/2000/01/rdf-schema#>
PREFIX sdo: <https://schema.org/>
PREFIX skos: <http://www.w3.org/2004/02/skos/core#>
PREFIX xsd: <http://www.w3.org/2001/XMLSchema#>

grt:activity-summary-reports
    a skos:Collection ;
    dcterms:provenance "Developed by the Geological Survey of Queensland." ;
    skos:definition "Reports mandated for submission by the Acts or Regulations governing granted resource permits in Queensland that aggregate the details of activities for the entire permit or project during a specific period. Reports are all-of-permit activity summary reports."@en ;
    skos:member
        grt:geothermal-report-annual-reserves ,
        grt:geothermal-report-production ,
        grt:mine-plan-lodgement ,
        grt:permit-report-annual ,
        grt:permit-report-final ,
        grt:permit-report-final-relinquishment ,
        grt:permit-report-mineral-associated-water ,
        grt:permit-report-other ,
        grt:permit-report-partial-relinquishment ,
        grt:permit-report-six-month ,
        grt:permit-report-surrender ,
        grt:petroleum-report-cumulative-water-production ,
        grt:petroleum-report-field-information ,
        grt:petroleum-report-infrastructure ,
        grt:petroleum-report-non-associated-water ,
        grt:petroleum-report-other ,
        grt:petroleum-report-production-information ,
        grt:petroleum-report-resource-and-reserves-information ,
        grt:production-petroleum ,
        grt:reserves-petroleum ;
    skos:prefLabel "Activity Summary Reports"@en ;
.

grt:departmental-reports
    a skos:Collection ;
    dcterms:provenance "Developed by the Geological Survey of Queensland." ;
    skos:definition "Non-Permit reports that were produced by Queensland's Department of Natural Resources, Mines and Energy."@en ;
    skos:member
        grt:annual-report ,
        grt:any-other-report ,
        grt:commissioned-industry-study-or-report ,
        grt:departmental-drilling ,
        grt:geological-survey-of-queensland-publication ,
        grt:geological-survey-of-queensland-record ,
        grt:industry-consultative-report ,
        grt:presentation ,
        grt:queensland-government-mining-journal ,
        grt:soil-and-land-resources ;
    skos:prefLabel "Departmental Reports"@en ;
.

grt:exploration-grants
    a skos:Collection ;
    dcterms:provenance "Developed by the Geological Survey of Queensland." ;
    skos:definition "Reports that were funded either fully or partially by a Queensland Government grant in aid of exploration."@en ;
    skos:member
        grt:collaborative-drilling-initiative-final ,
        grt:collaborative-drilling-initiative-proposals ,
        grt:collaborative-exploration-initiative-final ,
        grt:industry-network-initiative-final ;
    skos:prefLabel "Exploration Grants"@en ;
.

grt:external-reports
    a skos:Collection ;
    dcterms:provenance "Developed by the Geological Survey of Queensland." ;
    skos:definition "Non-Permit reports that were produced by sources external to Queensland's Department of Natural Resources, Mines and Energy."@en ;
    skos:member
        grt:any-other-report ,
        grt:article ,
        grt:presentation ,
        grt:technical-report ,
        grt:thesis ;
    skos:prefLabel "External Reports"@en ;
.

grt:geophysics-reports
    a skos:Collection ;
    dcterms:provenance "Developed by the Geological Survey of Queensland." ;
    skos:definition "Reports that detail the acquisition, results or processing of geophysical data."@en ;
    skos:member
        grt:geophysical-survey-report-acquisition ,
        grt:geophysical-survey-report-final ,
        grt:geophysical-survey-report-logistics ,
        grt:seismic-survey-report-final ,
        grt:seismic-survey-report-other ,
        grt:seismic-survey-report-reprocessing ;
    skos:prefLabel "Geophysics Reports"@en ;
.

grt:geothermal-reports
    a skos:Collection ;
    dcterms:provenance "Developed by the Geological Survey of Queensland." ;
    skos:definition "Reports governed by the Geothermal Energy Regulations."@en ;
    skos:member
        grt:geothermal-end-tenure ,
        grt:geothermal-report-annual-reserves ,
        grt:geothermal-report-injection ,
        grt:geothermal-report-injection-testing ,
        grt:geothermal-report-production ,
        grt:geothermal-report-production-testing ,
        grt:geothermal-report-relinquishment ,
        grt:geothermal-report-surrender ;
    skos:prefLabel "Geothermal Reports"@en ;
.

grt:greenhouse-gas-reports
    a skos:Collection ;
    dcterms:provenance "Developed by the Geological Survey of Queensland." ;
    skos:definition "Reports pertaining to Greenhouse Gas Storage permits."@en ;
    skos:member
        grt:greenhouse-gas-report-injection ,
        grt:greenhouse-gas-report-storage-capacity ,
        grt:greenhouse-gas-report-storage-injection ;
    skos:prefLabel "Greenhouse Gas Reports"@en ;
.

grt:lodgement-portal-internal
    a skos:Collection ;
    dcterms:provenance "Developed by the Geological Survey of Queensland." ;
    skos:definition "Reports accepted by the DNRME Geoscience Open Data Portal Lodgement site that can be accessed by internal DNRME users."@en ;
    skos:member
        grt:any-other-report ,
        grt:coal-quarterly-statistics ,
        grt:collaborative-drilling-initiative-final ,
        grt:collaborative-exploration-initiative-final ,
        grt:collaborative-exploration-initiative-proposals ,
        grt:commissioned-industry-study-or-report ,
        grt:departmental-drilling ,
        grt:extractives-annual-statistics ,
        grt:geological-survey-of-queensland-publication ,
        grt:geological-survey-of-queensland-record ,
        grt:geophysical-survey-report-final ,
        grt:geothermal-end-tenure ,
        grt:geothermal-report-annual ,
        grt:geothermal-report-annual-reserves ,
        grt:geothermal-report-injection ,
        grt:geothermal-report-injection-testing ,
        grt:geothermal-report-production ,
        grt:geothermal-report-production-testing ,
        grt:geothermal-report-relinquishment ,
        grt:geothermal-report-surrender ,
        grt:greenhouse-gas-report-injection ,
        grt:greenhouse-gas-report-storage-capacity ,
        grt:greenhouse-gas-report-storage-injection ,
        grt:hydraulic-fracturing-activity-report ,
        grt:mine-plan-lodgement ,
        grt:minerals-annual-statistics ,
        grt:mmol-44 ,
        grt:pa-21A ,
        grt:pa-22A ,
        grt:pa-42 ,
        grt:permit-report-annual ,
        grt:permit-report-annual-ml ,
        grt:permit-report-final ,
        grt:permit-report-final-higher-tenure ,
        grt:permit-report-final-relinquishment ,
        grt:permit-report-mineral-associated-water ,
        grt:permit-report-other ,
        grt:permit-report-partial-relinquishment ,
        grt:permit-report-partial-relinquishment-higher-tenure ,
        grt:permit-report-six-month ,
        grt:permit-report-surrender ,
        grt:permit-report-surrender-higher-tenure ,
        grt:petroleum-end-authority ,
        grt:petroleum-end-tenure ,
        grt:petroleum-report-annual ,
        grt:petroleum-report-cumulative-water-production ,
        grt:petroleum-report-field-information ,
        grt:petroleum-report-infrastructure ,
        grt:petroleum-report-non-associated-water ,
        grt:petroleum-report-other ,
        grt:petroleum-report-production-information ,
        grt:petroleum-report-relinquishment ,
        grt:petroleum-report-resource-and-reserves-information ,
        grt:petroleum-report-surrender ,
        grt:petroleum-report-transmission ,
        grt:pggd-01 ,
        grt:pggd-02 ,
        grt:pggd-03 ,
        grt:pggd-04 ,
        grt:pipeline-report-surrender ,
        grt:pm-1-2013 ,
        grt:presentation ,
        grt:production-petroleum ,
        grt:queensland-government-mining-journal ,
        grt:reserves-petroleum ,
        grt:scientific-or-technical-survey-report ,
        grt:seismic-survey-report-final ,
        grt:seismic-survey-report-other ,
        grt:seismic-survey-report-reprocessing ,
        grt:survey-plan ,
        grt:technical-report ,
        grt:water-report-other ,
        grt:water-report-performance-review ,
        grt:well-completion-report ,
        grt:well-or-bore-abandonment-report ,
        grt:well-production-testing-report ,
        grt:wra-05A ;
    skos:prefLabel "Internal Lodgement Portal"@en ;
.

grt:lodgement-portal-reports
    a skos:Collection ;
    dcterms:provenance "Developed by the Geological Survey of Queensland." ;
    skos:definition "Reports accepted by the DNRME Geoscience Open Data Portal Lodgement site."@en ;
    skos:member
        grt:coal-quarterly-statistics ,
        grt:extractives-annual-statistics ,
        grt:geophysical-survey-report-final ,
        grt:geothermal-end-tenure ,
        grt:geothermal-report-annual-reserves ,
        grt:geothermal-report-injection ,
        grt:geothermal-report-injection-testing ,
        grt:geothermal-report-production ,
        grt:geothermal-report-production-testing ,
        grt:geothermal-report-relinquishment ,
        grt:geothermal-report-surrender ,
        grt:greenhouse-gas-report-injection ,
        grt:greenhouse-gas-report-storage-capacity ,
        grt:greenhouse-gas-report-storage-injection ,
        grt:hydraulic-fracturing-activity-report ,
        grt:mine-plan-lodgement ,
        grt:minerals-annual-statistics ,
        grt:mmol-44 ,
        grt:pa-21A ,
        grt:pa-22A ,
        grt:pa-42 ,
        grt:permit-report-annual ,
        grt:permit-report-annual-ml ,
        grt:permit-report-final ,
        grt:permit-report-final-higher-tenure ,
        grt:permit-report-mineral-associated-water ,
        grt:permit-report-partial-relinquishment ,
        grt:permit-report-partial-relinquishment-higher-tenure ,
        grt:permit-report-surrender ,
        grt:permit-report-surrender-higher-tenure ,
        grt:petroleum-end-authority ,
        grt:petroleum-end-tenure ,
        grt:petroleum-report-annual ,
        grt:petroleum-report-non-associated-water ,
        grt:petroleum-report-production-information ,
        grt:petroleum-report-relinquishment ,
        grt:petroleum-report-resource-and-reserves-information ,
        grt:petroleum-report-surrender ,
        grt:pggd-01 ,
        grt:pggd-02 ,
        grt:pggd-03 ,
        grt:pggd-04 ,
        grt:pipeline-report-surrender ,
        grt:pm-1-2013 ,
        grt:scientific-or-technical-survey-report ,
        grt:seismic-survey-report-final ,
        grt:seismic-survey-report-other ,
        grt:seismic-survey-report-reprocessing ,
        grt:survey-plan ,
        grt:water-report-other ,
        grt:water-report-performance-review ,
        grt:well-completion-report ,
        grt:well-or-bore-abandonment-report ,
        grt:well-production-testing-report ,
        grt:wra-05A ;
    skos:prefLabel "Lodgement Portal Reports"@en ;
.

grt:non-current-reports
    a skos:Collection ;
    dcterms:provenance "Developed by the Geological Survey of Queensland." ;
    skos:definition "Reports that have been superceded or discontinued."@en ;
    skos:member
        grt:converted-from-qerd ,
        grt:permit-report-six-month ,
        grt:petroleum-report-field-information ,
        grt:petroleum-report-transmission ,
        grt:well-proposal ;
    skos:prefLabel "Non-Current Reports"@en ;
.

grt:non-permit-reports
    a skos:Collection ;
    dcterms:provenance "Developed by the Geological Survey of Queensland." ;
    skos:definition "Reports that are not required by Acts and/or Regulation in Queensland."@en ;
    skos:member
        grt:annual-report ,
        grt:any-other-report ,
        grt:article ,
        grt:commissioned-industry-study-or-report ,
        grt:departmental-drilling ,
        grt:geological-survey-of-queensland-publication ,
        grt:geological-survey-of-queensland-record ,
        grt:industry-consultative-report ,
        grt:presentation ,
        grt:queensland-government-mining-journal ,
        grt:soil-and-land-resources ,
        grt:technical-report ,
        grt:thesis ;
    skos:prefLabel "Non-Permit Reports"@en ;
.

grt:permit-reports
    a skos:Collection ;
    dcterms:provenance "Developed by the Geological Survey of Queensland." ;
    skos:definition "Reports mandated for submission by the Acts or Regulations governing granted resource permits in Queensland that detail any activities undertaken on that permit. Reports include all-of-permit activity summary reports and reports for single activities."@en ;
    skos:member
        grt:collaborative-drilling-initiative-final ,
        grt:collaborative-drilling-initiative-proposals ,
        grt:collaborative-exploration-initiative-final ,
        grt:converted-from-qerd ,
        grt:geophysical-survey-report-final ,
        grt:geothermal-end-tenure ,
        grt:geothermal-report-annual-reserves ,
        grt:geothermal-report-injection ,
        grt:geothermal-report-injection-testing ,
        grt:geothermal-report-production ,
        grt:geothermal-report-production-testing ,
        grt:geothermal-report-relinquishment ,
        grt:geothermal-report-surrender ,
        grt:greenhouse-gas-report-injection ,
        grt:greenhouse-gas-report-storage-capacity ,
        grt:greenhouse-gas-report-storage-injection ,
        grt:hydraulic-fracturing-activity-report ,
        grt:industry-network-initiative-final ,
        grt:mine-plan-lodgement ,
        grt:other-water-reports ,
        grt:permit-report-annual ,
        grt:permit-report-annual-ml ,
        grt:permit-report-final ,
        grt:permit-report-final-higher-tenure ,
        grt:permit-report-final-relinquishment ,
        grt:permit-report-mineral-associated-water ,
        grt:permit-report-other ,
        grt:permit-report-partial-relinquishment ,
        grt:permit-report-six-month ,
        grt:permit-report-surrender ,
        grt:permit-report-surrender-higher-tenure ,
        grt:petroleum-report-cumulative-water-production ,
        grt:petroleum-report-field-information ,
        grt:petroleum-report-infrastructure ,
        grt:petroleum-report-non-associated-water ,
        grt:petroleum-report-other ,
        grt:petroleum-report-production-information ,
        grt:petroleum-report-resource-and-reserves-information ,
        grt:petroleum-report-transmission ,
        grt:production-petroleum ,
        grt:reserves-petroleum ,
        grt:scientific-or-technical-survey-report ,
        grt:seismic-survey-report-final ,
        grt:seismic-survey-report-other ,
        grt:seismic-survey-report-reprocessing ,
        grt:water-report-performance-review ,
        grt:well-completion-report ,
        grt:well-or-bore-abandonment-report ,
        grt:well-production-testing-report ,
        grt:well-proposal ,
        grt:well-report-other ;
    skos:prefLabel "Permit Reports"@en ;
.

grt:petroleum-reports
    a skos:Collection ;
    dcterms:provenance "Developed by the Geological Survey of Queensland." ;
    skos:definition "Reports governed by the Petroleum and Gas Act of Queensland."@en ;
    skos:member
        grt:hydraulic-fracturing-activity-report ,
        grt:permit-report-surrender ,
        grt:petroleum-end-authority ,
        grt:petroleum-end-tenure ,
        grt:petroleum-report-annual ,
        grt:petroleum-report-cumulative-water-production ,
        grt:petroleum-report-infrastructure ,
        grt:petroleum-report-non-associated-water ,
        grt:petroleum-report-other ,
        grt:petroleum-report-production-information ,
        grt:petroleum-report-relinquishment ,
        grt:petroleum-report-resource-and-reserves-information ,
        grt:petroleum-report-surrender ,
        grt:petroleum-report-transmission ,
        grt:pipeline-report-surrender ,
        grt:production-petroleum ,
        grt:reserves-petroleum ,
        grt:scientific-or-technical-survey-report ,
        grt:well-completion-report ,
        grt:well-or-bore-abandonment-report ,
        grt:well-production-testing-report ,
        grt:well-report-other ;
    skos:prefLabel "Petroleum Reports"@en ;
.

grt:production-and-reserves-reports
    a skos:Collection ;
    dcterms:provenance "Developed by the Geological Survey of Queensland." ;
    skos:definition "Reports that describe the production and/or reserves of a permit or project."@en ;
    skos:member
        grt:geothermal-report-annual-reserves ,
        grt:geothermal-report-production ,
        grt:petroleum-report-cumulative-water-production ,
        grt:petroleum-report-production-information ,
        grt:petroleum-report-resource-and-reserves-information ,
        grt:production-petroleum ,
        grt:reserves-petroleum ;
    skos:prefLabel "Production and Reserves Reports"@en ;
.

grt:water-reports
    a skos:Collection ;
    dcterms:provenance "Developed by the Geological Survey of Queensland." ;
    skos:definition "Reports governed by the associated Acts of Queensland pertaining to water resources."@en ;
    skos:member
        grt:other-water-reports ,
        grt:permit-report-mineral-associated-water ,
        grt:petroleum-report-non-associated-water ,
        grt:water-report-performance-review ;
    skos:prefLabel "Water Reports"@en ;
.

grt:collaborative-exploration-initiative-proposals
    a skos:Concept ;
    dcterms:provenance "Developed by the Geological Survey of Queensland." ;
    rdfs:isDefinedBy <https://linked.data.gov.au/def/georesource-report> ;
    skos:definition "A proposal detailing the activities and results of a project that intend to receive support from the Collaborative Exploration Initiative. The details of which have been defined as a part of the terms and conditions of that initiative."@en ;
    skos:inScheme <https://linked.data.gov.au/def/georesource-report> ;
    skos:notation "CEIPRO" ;
    skos:prefLabel "Collaborative Exploration Initiative - Proposals"@en ;
    skos:topConceptOf <https://linked.data.gov.au/def/georesource-report> ;
.

grt:geophysical-survey-report-acquisition
    a skos:Concept ;
    dcterms:provenance "Developed by the Geological Survey of Queensland." ;
    rdfs:isDefinedBy <https://linked.data.gov.au/def/georesource-report> ;
    skos:altLabel "Acquisition Report"@en ;
    skos:definition "A report describing the acquisition of geophysics."@en ;
    skos:inScheme <https://linked.data.gov.au/def/georesource-report> ;
    skos:prefLabel "Geophysical Survey Report - Acquisition"@en ;
    skos:topConceptOf <https://linked.data.gov.au/def/georesource-report> ;
.

grt:geophysical-survey-report-logistics
    a skos:Concept ;
    dcterms:provenance "Developed by the Geological Survey of Queensland." ;
    rdfs:isDefinedBy <https://linked.data.gov.au/def/georesource-report> ;
    skos:definition "A report detailing the logistical requirements and procedures that were necessary to undertake an activity."@en ;
    skos:inScheme <https://linked.data.gov.au/def/georesource-report> ;
    skos:prefLabel "Geophysical Survey Report - Logistics"@en ;
    skos:topConceptOf <https://linked.data.gov.au/def/georesource-report> ;
.

grt:geothermal-report-annual
    a skos:Concept ;
    dcterms:provenance "Developed by the Geological Survey of Queensland." ;
    rdfs:isDefinedBy <https://linked.data.gov.au/def/georesource-report> ;
    skos:definition "A report detailing the activities that have occured on a geothermal authority such as an EPG for the 12 months ending on the anniversary day of the permit."@en ;
    skos:inScheme <https://linked.data.gov.au/def/georesource-report> ;
    skos:notation "GTHANN" ;
    skos:prefLabel "Geothermal Report - Annual"@en ;
    skos:topConceptOf <https://linked.data.gov.au/def/georesource-report> ;
.

<https://linked.data.gov.au/org/gsq>
    a sdo:Organization ;
    sdo:name "Geological Survey of Queensland" ;
    sdo:url "https://www.business.qld.gov.au/industries/mining-energy-water/resources/geoscience-information/gsq"^^xsd:anyURI ;
.

grt:annual-report
    a skos:Concept ;
    dcterms:provenance "Developed by the Geological Survey of Queensland." ;
    rdfs:isDefinedBy <https://linked.data.gov.au/def/georesource-report> ;
    skos:definition "A report that is not specifically linked to a permit that describes activities and/or the results of activities, market conditions etc. that occurred over a 12 month interval prior to the completion of that report."@en ;
    skos:inScheme <https://linked.data.gov.au/def/georesource-report> ;
    skos:prefLabel "Annual Report"@en ;
    skos:topConceptOf <https://linked.data.gov.au/def/georesource-report> ;
.

grt:article
    a skos:Concept ;
    dcterms:provenance "Developed by the Geological Survey of Queensland." ;
    rdfs:isDefinedBy <https://linked.data.gov.au/def/georesource-report> ;
    skos:definition "A piece of writing included with others in a newspaper, magazine, or other publication. Source: Oxford English Dictionary"@en ;
    skos:inScheme <https://linked.data.gov.au/def/georesource-report> ;
    skos:prefLabel "Article"@en ;
    skos:topConceptOf <https://linked.data.gov.au/def/georesource-report> ;
.

grt:coal-quarterly-statistics
    a skos:Concept ;
    dcterms:provenance "Developed by the Geological Survey of Queensland." ;
    rdfs:isDefinedBy <https://linked.data.gov.au/def/georesource-report> ;
    skos:definition "A report detailing the quarterly production and sales statistics for a coal mine."@en ;
    skos:inScheme <https://linked.data.gov.au/def/georesource-report> ;
    skos:notation "CQS" ;
    skos:prefLabel "Coal Quarterly Statistics"@en ;
    skos:topConceptOf <https://linked.data.gov.au/def/georesource-report> ;
.

grt:collaborative-drilling-initiative-proposals
    a skos:Concept ;
    dcterms:provenance "Developed by the Geological Survey of Queensland." ;
    rdfs:isDefinedBy <https://linked.data.gov.au/def/georesource-report> ;
    skos:definition "A propsal detailing the activities and results of a project that received support from the Collaborative Drilling Initiative. The details of which have been defined as a part of the terms and conditions of that initiative."@en ;
    skos:inScheme <https://linked.data.gov.au/def/georesource-report> ;
    skos:notation "CDIPRO" ;
    skos:prefLabel "Collaborative Drilling Initiative - Proposals"@en ;
    skos:topConceptOf <https://linked.data.gov.au/def/georesource-report> ;
.

grt:converted-from-qerd
    a skos:Concept ;
    dcterms:provenance "Developed by the Geological Survey of Queensland." ;
    rdfs:isDefinedBy <https://linked.data.gov.au/def/georesource-report> ;
    skos:definition "A report that was held in the Queensland Energy Resources Database and was subsequently converted into the Queensland Digital Exploration Reports database."@en ;
    skos:inScheme <https://linked.data.gov.au/def/georesource-report> ;
    skos:prefLabel "Converted from QERD"@en ;
    skos:topConceptOf <https://linked.data.gov.au/def/georesource-report> ;
.

grt:extractives-annual-statistics
    a skos:Concept ;
    dcterms:provenance "Developed by the Geological Survey of Queensland." ;
    rdfs:isDefinedBy <https://linked.data.gov.au/def/georesource-report> ;
    skos:definition "A report detailing the annual production and sales statistics for a quarry."@en ;
    skos:inScheme <https://linked.data.gov.au/def/georesource-report> ;
    skos:notation "EAS" ;
    skos:prefLabel "Extractives Annual Statistics"@en ;
    skos:topConceptOf <https://linked.data.gov.au/def/georesource-report> ;
.

grt:industry-consultative-report
    a skos:Concept ;
    dcterms:provenance "Developed by the Geological Survey of Queensland." ;
    rdfs:isDefinedBy <https://linked.data.gov.au/def/georesource-report> ;
    skos:definition "A report produced as the result of a consultative agreement between two agents, which does not directly fall under the Mineral Resource or Petroleum & Gas Acts."@en ;
    skos:inScheme <https://linked.data.gov.au/def/georesource-report> ;
    skos:prefLabel "Industry Consultative Report"@en ;
    skos:topConceptOf <https://linked.data.gov.au/def/georesource-report> ;
.

grt:industry-network-initiative-final
    a skos:Concept ;
    dcterms:provenance "Developed by the Geological Survey of Queensland." ;
    rdfs:isDefinedBy <https://linked.data.gov.au/def/georesource-report> ;
    skos:altLabel "Industry Network Initiative - Final (Completed)"@en ;
    skos:definition "A report detailing the activities and results of a project that received support from the Industry Network Initiative. The details of which have been defined as a part of the terms and conditions of that initiative."@en ;
    skos:inScheme <https://linked.data.gov.au/def/georesource-report> ;
    skos:notation "INIFIN" ;
    skos:prefLabel "Industry Network Initiative - Final"@en ;
    skos:topConceptOf <https://linked.data.gov.au/def/georesource-report> ;
.

grt:minerals-annual-statistics
    a skos:Concept ;
    dcterms:provenance "Developed by the Geological Survey of Queensland." ;
    rdfs:isDefinedBy <https://linked.data.gov.au/def/georesource-report> ;
    skos:definition "A report detailing the annual production and sales statistics for a mineral mine."@en ;
    skos:inScheme <https://linked.data.gov.au/def/georesource-report> ;
    skos:notation "MAS" ;
    skos:prefLabel "Minerals Annual Statistics"@en ;
    skos:topConceptOf <https://linked.data.gov.au/def/georesource-report> ;
.

grt:mmol-44
    a skos:Concept ;
    dcterms:provenance "Developed by the Geological Survey of Queensland." ;
    rdfs:isDefinedBy <https://linked.data.gov.au/def/georesource-report> ;
    skos:altLabel
        "Notice of decommissioning a well, water observation bore, water monitoring bore or water supply bore"@en ,
        "Notice of decommissioning petroleum wells, water observation bores or water supply bores"@en ;
    skos:definition "A notice to inform the Department that a well or water bore has been decommisioned."@en ;
    skos:historyNote "Form supersedes legacy form PA-40"@en ;
    skos:inScheme <https://linked.data.gov.au/def/georesource-report> ;
    skos:notation "MMOL-44"@en ;
    skos:prefLabel "MMOL-44 Notice of decommissioning petroleum wells, water observation bores or water supply bores"@en ;
    skos:topConceptOf <https://linked.data.gov.au/def/georesource-report> ;
.

grt:pa-21A
    a skos:Concept ;
    dcterms:provenance "Developed by the Geological Survey of Queensland." ;
    rdfs:isDefinedBy <https://linked.data.gov.au/def/georesource-report> ;
    skos:altLabel "Notice of Intention to carry out seismic survey or scientific or technical survey"@en ;
    skos:definition "A notice to inform the Department that a seismic survey or scientific or technical survey will be performed."@en ;
    skos:inScheme <https://linked.data.gov.au/def/georesource-report> ;
    skos:notation "PA-21A"@en ;
    skos:prefLabel "PA-21A Notice of Intention to carry out seismic survey or scientific or technical survey"@en ;
    skos:topConceptOf <https://linked.data.gov.au/def/georesource-report> ;
.

grt:pa-22A
    a skos:Concept ;
    dcterms:provenance "Developed by the Geological Survey of Queensland." ;
    rdfs:isDefinedBy <https://linked.data.gov.au/def/georesource-report> ;
    skos:altLabel "Notice of Completion of seismic survey or scientific or technical survey"@en ;
    skos:definition "A notice to inform the Department that a seismic survey or scientific or technical survey has been completed."@en ;
    skos:inScheme <https://linked.data.gov.au/def/georesource-report> ;
    skos:notation "PA-22A"@en ;
    skos:prefLabel "PA-22A Notice of Completion of seismic survey or scientific or technical survey"@en ;
    skos:topConceptOf <https://linked.data.gov.au/def/georesource-report> ;
.

grt:pa-42
    a skos:Concept ;
    dcterms:provenance "Developed by the Geological Survey of Queensland." ;
    rdfs:isDefinedBy <https://linked.data.gov.au/def/georesource-report> ;
    skos:altLabel "Notice of intention to convert a petroleum well to a water observation bore or water supply bore"@en ;
    skos:definition "A notice to inform the Department that a petroleum well is intended to be converted to a water bore."@en ;
    skos:inScheme <https://linked.data.gov.au/def/georesource-report> ;
    skos:notation "PA-42"@en ;
    skos:prefLabel "PA-42 Notice of intention to convert a petroleum well to a water observation bore or water supply bore"@en ;
    skos:topConceptOf <https://linked.data.gov.au/def/georesource-report> ;
.

grt:permit-report-partial-relinquishment-higher-tenure
    a skos:Concept ;
    dcterms:provenance "Developed by the Geological Survey of Queensland." ;
    rdfs:isDefinedBy <https://linked.data.gov.au/def/georesource-report> ;
    skos:definition "A report detailing all the activities a holder has undertaken on a specific region of an exploration permit that has been relinquished upon grant of a higher tenure. As required by the Mineral Resources Act and as defined by the Practice Direction. Required under the Queensland Mineral Resources Regulation 2013, s16 and s29B."@en ;
    skos:inScheme <https://linked.data.gov.au/def/georesource-report> ;
    skos:notation "RELINQHT" ;
    skos:prefLabel "Coal or Mineral Permit Report - Partial Relinquishment (Grant of higher tenure)"@en ;
    skos:topConceptOf <https://linked.data.gov.au/def/georesource-report> ;
.

grt:pggd-01
    a skos:Concept ;
    dcterms:provenance "Developed by the Geological Survey of Queensland." ;
    rdfs:isDefinedBy <https://linked.data.gov.au/def/georesource-report> ;
    skos:altLabel "Notice of intention to drill a petroleum well or bore"@en ;
    skos:definition "A notice to inform the Department that a petroleum well or bore will be drilled."@en ;
    skos:inScheme <https://linked.data.gov.au/def/georesource-report> ;
    skos:notation "PGGD-01"@en ;
    skos:prefLabel "PGGD-01 Notice of intention to drill a petroleum well or bore"@en ;
    skos:topConceptOf <https://linked.data.gov.au/def/georesource-report> ;
.

grt:pggd-02
    a skos:Concept ;
    dcterms:provenance "Developed by the Geological Survey of Queensland." ;
    rdfs:isDefinedBy <https://linked.data.gov.au/def/georesource-report> ;
    skos:altLabel "Notice of completion, alteration or abandonment of petroleum well or bore"@en ;
    skos:definition "A notice to inform the Department that a petroleum well or bore has been completed, altered, or abandoned."@en ;
    skos:inScheme <https://linked.data.gov.au/def/georesource-report> ;
    skos:notation "PGGD-02"@en ;
    skos:prefLabel "PGGD-02 Notice of completion, alteration or abandonment of petroleum well or bore"@en ;
    skos:topConceptOf <https://linked.data.gov.au/def/georesource-report> ;
.

grt:pggd-03
    a skos:Concept ;
    dcterms:provenance "Developed by the Geological Survey of Queensland." ;
    rdfs:isDefinedBy <https://linked.data.gov.au/def/georesource-report> ;
    skos:altLabel "Notice of intention to carry out hydraulic fracturing activities"@en ;
    skos:definition "A notice to inform the Department that hydraulic fracturing activities on a petroleum well or bore will performed."@en ;
    skos:inScheme <https://linked.data.gov.au/def/georesource-report> ;
    skos:notation "PGGD-03"@en ;
    skos:prefLabel "PGGD-03 Notice of intention to carry out hydraulic fracturing activities"@en ;
    skos:topConceptOf <https://linked.data.gov.au/def/georesource-report> ;
.

grt:pggd-04
    a skos:Concept ;
    dcterms:provenance "Developed by the Geological Survey of Queensland." ;
    rdfs:isDefinedBy <https://linked.data.gov.au/def/georesource-report> ;
    skos:altLabel "Notice of completion of hydraulic fracturing activities"@en ;
    skos:definition "A notice to inform the Department that hydraulic fracturing activities on a petroleum well or bore have been completed."@en ;
    skos:inScheme <https://linked.data.gov.au/def/georesource-report> ;
    skos:notation "PGGD-04"@en ;
    skos:prefLabel "PGGD-04 Notice of completion of hydraulic fracturing activities"@en ;
    skos:topConceptOf <https://linked.data.gov.au/def/georesource-report> ;
.

grt:pm-1-2013
    a skos:Concept ;
    dcterms:provenance "Developed by the Geological Survey of Queensland." ;
    rdfs:isDefinedBy <https://linked.data.gov.au/def/georesource-report> ;
    skos:altLabel "Notification of geophysical survey"@en ;
    skos:definition "A notice to inform the Department that a geophysical survey has been completed."@en ;
    skos:inScheme <https://linked.data.gov.au/def/georesource-report> ;
    skos:notation "PM 1/2013"@en ;
    skos:prefLabel "PM 1/2013 Notification of geophysical survey"@en ;
    skos:topConceptOf <https://linked.data.gov.au/def/georesource-report> ;
.

grt:soil-and-land-resources
    a skos:Concept ;
    dcterms:provenance "Developed by the Geological Survey of Queensland." ;
    rdfs:isDefinedBy <https://linked.data.gov.au/def/georesource-report> ;
    skos:altLabel "Soils & Land Resources"@en ;
    skos:definition "A series of historical reports detailing Soil and other studies conducted by the Natural Resources group of the Queensland Government. No longer managed in this system."@en ;
    skos:inScheme <https://linked.data.gov.au/def/georesource-report> ;
    skos:prefLabel "Soil and Land Resources"@en ;
    skos:topConceptOf <https://linked.data.gov.au/def/georesource-report> ;
.

grt:survey-plan
    a skos:Concept ;
    dcterms:provenance "Developed by the Geological Survey of Queensland." ;
    rdfs:isDefinedBy <https://linked.data.gov.au/def/georesource-report> ;
    skos:definition "A schematic or plan produces by certified surveyors detailing the location of site or feature."@en ;
    skos:inScheme <https://linked.data.gov.au/def/georesource-report> ;
    skos:prefLabel "Survey Plan"@en ;
    skos:topConceptOf <https://linked.data.gov.au/def/georesource-report> ;
.

grt:thesis
    a skos:Concept ;
    dcterms:provenance "Developed by the Geological Survey of Queensland." ;
    rdfs:isDefinedBy <https://linked.data.gov.au/def/georesource-report> ;
    skos:definition "A long essay or dissertation involving personal research, written by a candidate for a university degree. Source: Oxford English Dictionary"@en ;
    skos:inScheme <https://linked.data.gov.au/def/georesource-report> ;
    skos:prefLabel "Thesis"@en ;
    skos:topConceptOf <https://linked.data.gov.au/def/georesource-report> ;
.

grt:water-report-other
    a skos:Concept ;
    dcterms:provenance "Developed by the Geological Survey of Queensland." ;
    rdfs:isDefinedBy <https://linked.data.gov.au/def/georesource-report> ;
    skos:altLabel "Other Water Reports"@en ;
    skos:definition "A report detailing activities and results related to a water under the Queensland Water Act not described in other water reports."@en ;
    skos:inScheme <https://linked.data.gov.au/def/georesource-report> ;
    skos:notation "WATOTH" ;
    skos:prefLabel "Water Report - Other"@en ;
    skos:topConceptOf <https://linked.data.gov.au/def/georesource-report> ;
.

grt:well-proposal
    a skos:Concept ;
    dcterms:provenance "Developed by the Geological Survey of Queensland." ;
    rdfs:isDefinedBy <https://linked.data.gov.au/def/georesource-report> ;
    skos:definition "A report detailing the planning and purpose of a well or bore that is yet to be drilled."@en ;
    skos:inScheme <https://linked.data.gov.au/def/georesource-report> ;
    skos:notation "WELPRO" ;
    skos:prefLabel "Well proposal"@en ;
    skos:topConceptOf <https://linked.data.gov.au/def/georesource-report> ;
.

grt:well-report-other
    a skos:Concept ;
    dcterms:provenance "Developed by the Geological Survey of Queensland." ;
    rdfs:isDefinedBy <https://linked.data.gov.au/def/georesource-report> ;
    skos:definition "A report detailing the activities or results of a well not described in other well reports."@en ;
    skos:inScheme <https://linked.data.gov.au/def/georesource-report> ;
    skos:notation "WELOTH" ;
    skos:prefLabel "Well Report Other"@en ;
    skos:topConceptOf <https://linked.data.gov.au/def/georesource-report> ;
.

grt:wra-05A
    a skos:Concept ;
    dcterms:provenance "Developed by the Geological Survey of Queensland." ;
    rdfs:isDefinedBy <https://linked.data.gov.au/def/georesource-report> ;
    skos:altLabel "Notice of completion or conversion of petroleum well to water supply bore or water observation bore"@en ;
    skos:definition "A notice to inform the Department that a petroleum well has been converted to a water bore. Changes purpose from Petroleum, or narrower term, to Water. May trigger check for status change."@en ;
    skos:inScheme <https://linked.data.gov.au/def/georesource-report> ;
    skos:notation "WRA-05A"@en ;
    skos:prefLabel "WRA-05A Notice of completion or conversion of petroleum well to water supply bore or water observation bore"@en ;
    skos:topConceptOf <https://linked.data.gov.au/def/georesource-report> ;
.

grt:collaborative-drilling-initiative-final
    a skos:Concept ;
    dcterms:provenance "Developed by the Geological Survey of Queensland." ;
    rdfs:isDefinedBy <https://linked.data.gov.au/def/georesource-report> ;
    skos:altLabel "Collaborative Drilling Initiative - Final (Completed)"@en ;
    skos:definition "A report detailing the activities and results of a project that received support from the Collaborative Drilling Initiative. The details of which have been defined as a part of the terms and conditions of that initiative."@en ;
    skos:inScheme <https://linked.data.gov.au/def/georesource-report> ;
    skos:notation "CDIFIN" ;
    skos:prefLabel "Collaborative Drilling Initiative - Final"@en ;
    skos:topConceptOf <https://linked.data.gov.au/def/georesource-report> ;
.

grt:collaborative-exploration-initiative-final
    a skos:Concept ;
    dcterms:provenance "Developed by the Geological Survey of Queensland." ;
    rdfs:isDefinedBy <https://linked.data.gov.au/def/georesource-report> ;
    skos:altLabel "Collaborative Exploration Initiative - Final Report"@en ;
    skos:definition "A report detailing the activities and results of a project that received support from the Collaborative Exploration Initiative. The details of which have been defined as a part of the terms and conditions of that initiative."@en ;
    skos:inScheme <https://linked.data.gov.au/def/georesource-report> ;
    skos:notation "CEIFIN" ;
    skos:prefLabel "Collaborative Exploration Initiative - Final"@en ;
    skos:topConceptOf <https://linked.data.gov.au/def/georesource-report> ;
.

grt:commissioned-industry-study-or-report
    a skos:Concept ;
    dcterms:provenance "Developed by the Geological Survey of Queensland." ;
    rdfs:isDefinedBy <https://linked.data.gov.au/def/georesource-report> ;
    skos:definition "A report that was commissioned wholly or in part by a Queensland Government Department."@en ;
    skos:inScheme <https://linked.data.gov.au/def/georesource-report> ;
    skos:prefLabel "Commissioned Industry Study or Report"@en ;
    skos:topConceptOf <https://linked.data.gov.au/def/georesource-report> ;
.

grt:departmental-drilling
    a skos:Concept ;
    dcterms:provenance "Developed by the Geological Survey of Queensland." ;
    rdfs:isDefinedBy <https://linked.data.gov.au/def/georesource-report> ;
    skos:definition "A report detailing the activities and results of a project that was undertaken by one of Queensland's Government Departments and focussed on the activity of drilling."@en ;
    skos:inScheme <https://linked.data.gov.au/def/georesource-report> ;
    skos:prefLabel "Departmental Drilling"@en ;
    skos:topConceptOf <https://linked.data.gov.au/def/georesource-report> ;
.

grt:geological-survey-of-queensland-publication
    a skos:Concept ;
    dcterms:provenance "Developed by the Geological Survey of Queensland." ;
    rdfs:isDefinedBy <https://linked.data.gov.au/def/georesource-report> ;
    skos:definition "A publication that has been produced by the Geological Survey of Queensland. Potentially published in other systems, journals etc. Exclusive of the Geological Survey of Queensland Record series."@en ;
    skos:inScheme <https://linked.data.gov.au/def/georesource-report> ;
    skos:prefLabel "Geological Survey of Queensland Publication"@en ;
    skos:topConceptOf <https://linked.data.gov.au/def/georesource-report> ;
.

grt:geological-survey-of-queensland-record
    a skos:Concept ;
    dcterms:provenance "Developed by the Geological Survey of Queensland." ;
    rdfs:isDefinedBy <https://linked.data.gov.au/def/georesource-report> ;
    skos:definition "A publication that has been produced by the Geological Survey of Queensland and has been assigned a designation as a part of the Geological Survey of Queensland's Record series."@en ;
    skos:inScheme <https://linked.data.gov.au/def/georesource-report> ;
    skos:prefLabel "Geological Survey of Queensland Record"@en ;
    skos:topConceptOf <https://linked.data.gov.au/def/georesource-report> ;
.

grt:permit-report-annual-ml
    a skos:Concept ;
    dcterms:provenance "Developed by the Geological Survey of Queensland." ;
    rdfs:isDefinedBy <https://linked.data.gov.au/def/georesource-report> ;
    skos:altLabel
        "Activity Report (ML)"@en ,
        "Annual Report (ML)"@en ;
    skos:definition "A report that is required to be lodged annually as a part of the obligations of holding production tenure (ML) over a resource permit. Only applicable to Coal or Oil Shale Mining Leases in the Queensland Mineral Resources Regulation 2013, s29A."@en ;
    skos:inScheme <https://linked.data.gov.au/def/georesource-report> ;
    skos:notation "ANNML" ;
    skos:prefLabel "Coal or Mineral Permit Report - Activity Report (ML)"@en ;
    skos:topConceptOf <https://linked.data.gov.au/def/georesource-report> ;
.

grt:permit-report-final-higher-tenure
    a skos:Concept ;
    dcterms:provenance "Developed by the Geological Survey of Queensland." ;
    rdfs:isDefinedBy <https://linked.data.gov.au/def/georesource-report> ;
    skos:definition "A report that is required to be lodged when the tenure over a resource permit is superceded by grant of a higher tenure, detailing the work undertaken on the permit throughout the life of tenure. Required under the Queensland Mineral Resources Regulation 2013, s17."@en ;
    skos:inScheme <https://linked.data.gov.au/def/georesource-report> ;
    skos:notation "FINALHT" ;
    skos:prefLabel "Coal or Mineral Permit Report - Final (Grant of higher tenure)"@en ;
    skos:topConceptOf <https://linked.data.gov.au/def/georesource-report> ;
.

grt:permit-report-final-relinquishment
    a skos:Concept ;
    dcterms:provenance "Developed by the Geological Survey of Queensland." ;
    rdfs:isDefinedBy <https://linked.data.gov.au/def/georesource-report> ;
    skos:altLabel
        "Final Relinquishment (MDL)"@en ,
        "Permit Report - Final Relinquishment"@en ;
    skos:definition "A report that is required to be lodged when the tenure over a Mineral Development License ends, detailing the work undertaken on the permit throughout the life of tenure."@en ;
    skos:inScheme <https://linked.data.gov.au/def/georesource-report> ;
    skos:notation "FINREQ" ;
    skos:prefLabel "Coal or Mineral Permit Report - Final Relinquishment (MDL)"@en ;
    skos:topConceptOf <https://linked.data.gov.au/def/georesource-report> ;
.

grt:permit-report-other
    a skos:Concept ;
    dcterms:provenance "Developed by the Geological Survey of Queensland." ;
    rdfs:isDefinedBy <https://linked.data.gov.au/def/georesource-report> ;
    skos:altLabel
        "Any Other Resource Authority Report"@en ,
        "Permit Report - Other"@en ;
    skos:definition "A report that does not fall under any other category of permit reports."@en ;
    skos:inScheme <https://linked.data.gov.au/def/georesource-report> ;
    skos:prefLabel "Coal or Mineral Permit Report - Other"@en ;
    skos:topConceptOf <https://linked.data.gov.au/def/georesource-report> ;
.

grt:permit-report-surrender-higher-tenure
    a skos:Concept ;
    dcterms:provenance "Developed by the Geological Survey of Queensland." ;
    rdfs:isDefinedBy <https://linked.data.gov.au/def/georesource-report> ;
    skos:definition "A report that is required to be lodged as a part of the obligations of surrendering tenure over a Coal or Oil Shale Mining Lease or Mineral Development Licence upon grant of a higher tenure. Required under the Queensland Mineral Resources Regulation 2013, s16 and s29C"@en ;
    skos:inScheme <https://linked.data.gov.au/def/georesource-report> ;
    skos:notation "SURRHT" ;
    skos:prefLabel "Coal or Mineral Permit Report - Surrender (Grant of higher tenure)"@en ;
    skos:topConceptOf <https://linked.data.gov.au/def/georesource-report> ;
.

grt:petroleum-end-authority
    a skos:Concept ;
    dcterms:provenance "Developed by the Geological Survey of Queensland." ;
    rdfs:isDefinedBy <https://linked.data.gov.au/def/georesource-report> ;
    skos:altLabel
        "End of Authority Report (DAA)"@en ,
        "End of Authority Report (PSL)"@en ,
        "Petroleum Report - End of Authority Report"@en ;
    skos:definition "A report that is required to be lodged at the end of tenure over a Data Acquisition Authority or Petroleum Survey License, detailing the work undertaken on the authority throughout the life of tenure."@en ;
    skos:inScheme <https://linked.data.gov.au/def/georesource-report> ;
    skos:notation "PETAUT" ;
    skos:prefLabel "Petroleum Report - End of Authority (DAA/PSL)"@en ;
    skos:topConceptOf <https://linked.data.gov.au/def/georesource-report> ;
.

grt:petroleum-end-tenure
    a skos:Concept ;
    dcterms:provenance "Developed by the Geological Survey of Queensland." ;
    rdfs:isDefinedBy <https://linked.data.gov.au/def/georesource-report> ;
    skos:altLabel
        "End of Tenure Report (ATP)"@en ,
        "End of Tenure Report (PL)"@en ,
        "Petroleum Report - End of Tenure"@en ,
        "Petroleum Report - End of Tenure Report"@en ,
        "Petroleum Report - Final"@en ,
        "Petroleum Report - Final Report"@en ;
    skos:definition "A report that is required to be lodged at the end of tenure over a Petroleum Lease or Authority to Prospect, detailing the work undertaken on the permit throughout the life of tenure."@en ;
    skos:inScheme <https://linked.data.gov.au/def/georesource-report> ;
    skos:notation "PETEND" ;
    skos:prefLabel "Petroleum Report - End of Tenure (ATP/PL)"@en ;
    skos:topConceptOf <https://linked.data.gov.au/def/georesource-report> ;
.

grt:petroleum-report-annual
    a skos:Concept ;
    dcterms:provenance "Developed by the Geological Survey of Queensland." ;
    rdfs:isDefinedBy <https://linked.data.gov.au/def/georesource-report> ;
    skos:definition "A report detailing the activities that have occured on a petroleum authority such as a PL, ATP, PPL, or PFL for the 12 months ending on the last anniversary day, as mandatory in the Petroleum and Gas (Production and Safety) Act."@en ;
    skos:inScheme <https://linked.data.gov.au/def/georesource-report> ;
    skos:notation "PETANN" ;
    skos:prefLabel "Petroleum Report - Annual (ATP/PL/PPL/PFL)"@en ;
    skos:topConceptOf <https://linked.data.gov.au/def/georesource-report> ;
.

grt:petroleum-report-relinquishment
    a skos:Concept ;
    dcterms:provenance "Developed by the Geological Survey of Queensland." ;
    rdfs:isDefinedBy <https://linked.data.gov.au/def/georesource-report> ;
    skos:altLabel
        "Final Relinquishment (ATP)"@en ,
        "Final Relinquishment (PL)"@en ,
        "Petroleum Report - Final Relinquishment"@en ,
        "Petroleum Report - Relinquishment"@en ;
    skos:definition "A report that is required to be lodged with a partial or full relinquishment of a Petroleum Lease or Authority to Prospect, detailing the work undertaken on the relinquished portion of the permit throughout the life of tenure."@en ;
    skos:inScheme <https://linked.data.gov.au/def/georesource-report> ;
    skos:notation "PETREQ" ;
    skos:prefLabel "Petroleum Report - Relinquishment (ATP/PL)"@en ;
    skos:topConceptOf <https://linked.data.gov.au/def/georesource-report> ;
.

grt:petroleum-report-surrender
    a skos:Concept ;
    dcterms:provenance "Developed by the Geological Survey of Queensland." ;
    rdfs:isDefinedBy <https://linked.data.gov.au/def/georesource-report> ;
    skos:altLabel
        "Final Surrender (ATP)"@en ,
        "Final Surrender (PL)"@en ,
        "Petroleum Report - Final Surrender"@en ,
        "Petroleum Report - Surrender"@en ;
    skos:definition "A report that is required to be lodged with a partial or full surrender of a Petroleum Lease or Authority to Prospect, detailing the work undertaken on the surrendered portion of the permit throughout the life of tenure."@en ;
    skos:inScheme <https://linked.data.gov.au/def/georesource-report> ;
    skos:notation "PETSUR" ;
    skos:prefLabel "Petroleum Report - Surrender (ATP/PL)"@en ;
    skos:topConceptOf <https://linked.data.gov.au/def/georesource-report> ;
.

grt:pipeline-report-surrender
    a skos:Concept ;
    dcterms:provenance "Developed by the Geological Survey of Queensland." ;
    rdfs:isDefinedBy <https://linked.data.gov.au/def/georesource-report> ;
    skos:definition "A report that is required to be lodged with a partial or full surrender of a Petroleum Pipeline Lease, detailing the location of the pipeline and maintanence work undertaken throughout the life of tenure."@en ;
    skos:inScheme <https://linked.data.gov.au/def/georesource-report> ;
    skos:notation "PIPSUR" ;
    skos:prefLabel "Petroleum Report - Pipeline Surrender (PPL)"@en ;
    skos:topConceptOf <https://linked.data.gov.au/def/georesource-report> ;
.

grt:queensland-government-mining-journal
    a skos:Concept ;
    dcterms:provenance "Developed by the Geological Survey of Queensland." ;
    rdfs:isDefinedBy <https://linked.data.gov.au/def/georesource-report> ;
    skos:definition "The Queensland Government Mining Journal was a semi-annual publication that detailed the activities of the Geological Survey of Queensland and significant discoveries, mine openings or other geologically related happenings in the state or even globally."@en ;
    skos:inScheme <https://linked.data.gov.au/def/georesource-report> ;
    skos:prefLabel "Queensland Government Mining Journal"@en ;
    skos:topConceptOf <https://linked.data.gov.au/def/georesource-report> ;
.

grt:technical-report
    a skos:Concept ;
    dcterms:provenance "Developed by the Geological Survey of Queensland." ;
    rdfs:isDefinedBy <https://linked.data.gov.au/def/georesource-report> ;
    skos:definition "A report detailing activities of a highly technical nature that were not conducted as a part of a work programme for a resource permit."@en ;
    skos:inScheme <https://linked.data.gov.au/def/georesource-report> ;
    skos:prefLabel "Technical Report"@en ;
    skos:topConceptOf <https://linked.data.gov.au/def/georesource-report> ;
.

grt:any-other-report
    a skos:Concept ;
    dcterms:provenance "Developed by the Geological Survey of Queensland." ;
    rdfs:isDefinedBy <https://linked.data.gov.au/def/georesource-report> ;
    skos:definition "A report that does not fall under any other category of non-permit reports."@en ;
    skos:inScheme <https://linked.data.gov.au/def/georesource-report> ;
    skos:prefLabel "Any Other Report"@en ;
    skos:topConceptOf <https://linked.data.gov.au/def/georesource-report> ;
.

grt:geophysical-survey-report-final
    a skos:Concept ;
    dcterms:provenance "Developed by the Geological Survey of Queensland." ;
    rdfs:isDefinedBy <https://linked.data.gov.au/def/georesource-report> ;
    skos:definition "A report detailing the activities undertaken and their results, as a part of a geophysical survey."@en ;
    skos:inScheme <https://linked.data.gov.au/def/georesource-report> ;
    skos:notation "GEOPSR" ;
    skos:prefLabel "Geophysical Survey Report - Final"@en ;
    skos:topConceptOf <https://linked.data.gov.au/def/georesource-report> ;
.

grt:geothermal-end-tenure
    a skos:Concept ;
    dcterms:provenance "Developed by the Geological Survey of Queensland." ;
    rdfs:isDefinedBy <https://linked.data.gov.au/def/georesource-report> ;
    skos:altLabel
        "End of Tenure Report (EPG)"@en ,
        "End of Tenure Report (GL)"@en ,
        "Geothermal Report - End of Tenure"@en ,
        "Geothermal Report - End of Tenure Report"@en ,
        "Geothermal Report - Final"@en ,
        "Geothermal Report - Final Report"@en ;
    skos:definition "A report that is required to be lodged at the end of tenure over a Geothermal Lease or Exploration Permit Geothermal, detailing the work undertaken on the permit throughout the life of tenure."@en ;
    skos:inScheme <https://linked.data.gov.au/def/georesource-report> ;
    skos:notation "GEOEND" ;
    skos:prefLabel "Geothermal Report - End of Tenure (EPG/GL)"@en ;
    skos:topConceptOf <https://linked.data.gov.au/def/georesource-report> ;
.

grt:geothermal-report-injection
    a skos:Concept ;
    dcterms:provenance "Developed by the Geological Survey of Queensland." ;
    rdfs:isDefinedBy <https://linked.data.gov.au/def/georesource-report> ;
    skos:altLabel "Geothermal Injection Reports"@en ;
    skos:definition "A report detailing the performance and injected volumes of a geothermal injection well or wells."@en ;
    skos:inScheme <https://linked.data.gov.au/def/georesource-report> ;
    skos:notation "GTHIR" ;
    skos:prefLabel "Geothermal Report - Injection"@en ;
    skos:topConceptOf <https://linked.data.gov.au/def/georesource-report> ;
.

grt:geothermal-report-injection-testing
    a skos:Concept ;
    dcterms:provenance "Developed by the Geological Survey of Queensland." ;
    rdfs:isDefinedBy <https://linked.data.gov.au/def/georesource-report> ;
    skos:altLabel "Geothermal Injection Testing Reports"@en ;
    skos:definition "A report detailing the testing of the injection potential or performance of a geothermal injection well."@en ;
    skos:inScheme <https://linked.data.gov.au/def/georesource-report> ;
    skos:notation "GTHITR" ;
    skos:prefLabel "Geothermal Report - Injection Testing"@en ;
    skos:topConceptOf <https://linked.data.gov.au/def/georesource-report> ;
.

grt:geothermal-report-production-testing
    a skos:Concept ;
    dcterms:provenance "Developed by the Geological Survey of Queensland." ;
    rdfs:isDefinedBy <https://linked.data.gov.au/def/georesource-report> ;
    skos:altLabel "Geothermal Production Testing"@en ;
    skos:definition "A report detailing the testing of the production potential or performance of a geothermal well."@en ;
    skos:inScheme <https://linked.data.gov.au/def/georesource-report> ;
    skos:notation "GTHPT" ;
    skos:prefLabel "Geothermal Report - Production Testing"@en ;
    skos:topConceptOf <https://linked.data.gov.au/def/georesource-report> ;
.

grt:geothermal-report-relinquishment
    a skos:Concept ;
    dcterms:provenance "Developed by the Geological Survey of Queensland." ;
    rdfs:isDefinedBy <https://linked.data.gov.au/def/georesource-report> ;
    skos:altLabel
        "Final Relinquishment (EPG)"@en ,
        "Final Relinquishment (GL)"@en ,
        "Geothermal Report - Final Relinquishment"@en ,
        "Geothermal Report - Relinquishment"@en ;
    skos:definition "A report that is required to be lodged with a partial or full relinquishment of a Geothermal Lease or Exploration Permit Geothermal, detailing the work undertaken on the relinquished portion of the permit throughout the life of tenure."@en ;
    skos:inScheme <https://linked.data.gov.au/def/georesource-report> ;
    skos:notation "GEOREQ" ;
    skos:prefLabel "Geothermal Report - Relinquishment (EPG/GL)"@en ;
    skos:topConceptOf <https://linked.data.gov.au/def/georesource-report> ;
.

grt:geothermal-report-surrender
    a skos:Concept ;
    dcterms:provenance "Developed by the Geological Survey of Queensland." ;
    rdfs:isDefinedBy <https://linked.data.gov.au/def/georesource-report> ;
    skos:altLabel
        "Final Surrender (EPG)"@en ,
        "Final Surrender (GL)"@en ,
        "Geothermal Report - Final Surrender"@en ,
        "Geothermal Report - Surrender"@en ;
    skos:definition "A report that is required to be lodged with a partial or full surrender of a Geothermal Lease or Exploration Permit Geothermal, detailing the work undertaken on the surrendered portion of the permit throughout the life of tenure."@en ;
    skos:inScheme <https://linked.data.gov.au/def/georesource-report> ;
    skos:notation "GEOSUR" ;
    skos:prefLabel "Geothermal Report - Surrender (EPG/GL)"@en ;
    skos:topConceptOf <https://linked.data.gov.au/def/georesource-report> ;
.

grt:greenhouse-gas-report-injection
    a skos:Concept ;
    dcterms:provenance "Developed by the Geological Survey of Queensland." ;
    rdfs:isDefinedBy <https://linked.data.gov.au/def/georesource-report> ;
    skos:altLabel "Greenhouse Gas Injection Report"@en ;
    skos:definition "A report detailing the testing of greenhouse gas injection into a potential reservoir within a greenhouse gas storage permit."@en ;
    skos:inScheme <https://linked.data.gov.au/def/georesource-report> ;
    skos:notation "GHGIR" ;
    skos:prefLabel "Greenhouse Gas Report - Injection Testing"@en ;
    skos:topConceptOf <https://linked.data.gov.au/def/georesource-report> ;
.

grt:greenhouse-gas-report-storage-capacity
    a skos:Concept ;
    dcterms:provenance "Developed by the Geological Survey of Queensland." ;
    rdfs:isDefinedBy <https://linked.data.gov.au/def/georesource-report> ;
    skos:altLabel "Greenhouse Gas Stream Storage Capacity Report"@en ;
    skos:definition "A report detailing the potential greenhouse gas storage capacity within a greenhouse gas storage permit."@en ;
    skos:inScheme <https://linked.data.gov.au/def/georesource-report> ;
    skos:notation "GHGSSC" ;
    skos:prefLabel "Greenhouse Gas Report - Storage Capacity"@en ;
    skos:topConceptOf <https://linked.data.gov.au/def/georesource-report> ;
.

grt:greenhouse-gas-report-storage-injection
    a skos:Concept ;
    dcterms:provenance "Developed by the Geological Survey of Queensland." ;
    rdfs:isDefinedBy <https://linked.data.gov.au/def/georesource-report> ;
    skos:altLabel "Greenhouse Gas Storage Injection Report"@en ;
    skos:definition "A report detailing the performance and injected volumes of a greenhouse gas injection well or wells."@en ;
    skos:inScheme <https://linked.data.gov.au/def/georesource-report> ;
    skos:notation "GHGSIR" ;
    skos:prefLabel "Greenhouse Gas Report - Storage Injection"@en ;
    skos:topConceptOf <https://linked.data.gov.au/def/georesource-report> ;
.

grt:hydraulic-fracturing-activity-report
    a skos:Concept ;
    dcterms:provenance "Developed by the Geological Survey of Queensland." ;
    rdfs:isDefinedBy <https://linked.data.gov.au/def/georesource-report> ;
    skos:definition "A report detailing the activities and results of hydraulically fracturing activities conducted in a well."@en ;
    skos:inScheme <https://linked.data.gov.au/def/georesource-report> ;
    skos:notation "HFACR" ;
    skos:prefLabel "Hydraulic Fracturing Activity Report"@en ;
    skos:topConceptOf <https://linked.data.gov.au/def/georesource-report> ;
.

grt:mine-plan-lodgement
    a skos:Concept ;
    dcterms:provenance "Developed by the Geological Survey of Queensland." ;
    rdfs:isDefinedBy <https://linked.data.gov.au/def/georesource-report> ;
    skos:altLabel "Mine Plan Lodgement"@en ;
    skos:definition "A plan of the current and future workings and infrastructure of a mine, as required by the Mineral Resources Act."@en ;
    skos:inScheme <https://linked.data.gov.au/def/georesource-report> ;
    skos:notation "MPLODG" ;
    skos:prefLabel "Mine Working Plan"@en ;
    skos:topConceptOf <https://linked.data.gov.au/def/georesource-report> ;
.

grt:permit-report-annual
    a skos:Concept ;
    dcterms:provenance "Developed by the Geological Survey of Queensland." ;
    rdfs:isDefinedBy <https://linked.data.gov.au/def/georesource-report> ;
    skos:altLabel
        "Activity Report (EPC, EPM, MDL)"@en ,
        "Annual Report (EPC, EPM, MDL)"@en ,
        "Annual Resource Authority Report"@en ,
        "Permit Report - Annual"@en ;
    skos:definition "A report that is required to be lodged annually as a part of the obligations of holding exploration or development tenure (EPC, EPM, MDL) over a resource permit detailing activities performed. Required under the Queensland Mineral Resources Regulation 2013, s13."@en ;
    skos:inScheme <https://linked.data.gov.au/def/georesource-report> ;
    skos:notation "ANNUAL" ;
    skos:prefLabel "Coal or Mineral Permit Report - Activity Report (EPC, EPM, MDL)"@en ;
    skos:topConceptOf <https://linked.data.gov.au/def/georesource-report> ;
.

grt:permit-report-final
    a skos:Concept ;
    dcterms:provenance "Developed by the Geological Survey of Queensland." ;
    rdfs:isDefinedBy <https://linked.data.gov.au/def/georesource-report> ;
    skos:altLabel
        "Final or End of Tenure Report"@en ,
        "Permit Report - Final"@en ;
    skos:definition "A report that is required to be lodged when the tenure over a resource permit ends, detailing the work undertaken on the permit throughout the life of tenure. A final report may be combined with the last annual report into a single submission for the end of the tenure. Required under the Queensland Mineral Resources Regulation 2013, s17."@en ;
    skos:inScheme <https://linked.data.gov.au/def/georesource-report> ;
    skos:notation "FINAL" ;
    skos:prefLabel "Coal or Mineral Permit Report - Final (End of Tenure)"@en ;
    skos:topConceptOf <https://linked.data.gov.au/def/georesource-report> ;
.

grt:permit-report-partial-relinquishment
    a skos:Concept ;
    dcterms:provenance "Developed by the Geological Survey of Queensland." ;
    rdfs:isDefinedBy <https://linked.data.gov.au/def/georesource-report> ;
    skos:altLabel
        "Partial Relinquishment Report"@en ,
        "Permit Report - Partial Relinquishment"@en ;
    skos:definition "A report detailing all the activities a holder has undertaken on a specific region of an exploration permit that has been relinquished where a higher tenure over the same area has not been granted. As required by the Mineral Resources Act and as defined by the Practice Direction. Required under the Queensland Mineral Resources Regulation 2013, s16 and s29B."@en ;
    skos:inScheme <https://linked.data.gov.au/def/georesource-report> ;
    skos:notation "RELINQ" ;
    skos:prefLabel "Coal or Mineral Permit Report - Partial Relinquishment (End of Tenure)"@en ;
    skos:topConceptOf <https://linked.data.gov.au/def/georesource-report> ;
.

grt:permit-report-six-month
    a skos:Concept ;
    dcterms:provenance "Developed by the Geological Survey of Queensland." ;
    rdfs:isDefinedBy <https://linked.data.gov.au/def/georesource-report> ;
    skos:altLabel "Six Monthly Exploration Report"@en ;
    skos:definition "A report detailing the activities undertaken on an exploration permit in the six months prior to the submission of the report. Mostly deprecated in favour of annual reports."@en ;
    skos:inScheme <https://linked.data.gov.au/def/georesource-report> ;
    skos:notation "6MTH" ;
    skos:prefLabel "Permit Report - Six Month"@en ;
    skos:topConceptOf <https://linked.data.gov.au/def/georesource-report> ;
.

grt:petroleum-report-field-information
    a skos:Concept ;
    dcterms:provenance "Developed by the Geological Survey of Queensland." ;
    rdfs:isDefinedBy <https://linked.data.gov.au/def/georesource-report> ;
    skos:altLabel "Petroleum Field Reports"@en ;
    skos:definition "A report detailing the quantity, quality and other parameters of the reserves of petroleum and gas in a petroleum field that may cover one permit, multiple permits, and/or unpermitted areas."@en ;
    skos:inScheme <https://linked.data.gov.au/def/georesource-report> ;
    skos:notation "PETFLD" ;
    skos:prefLabel "Petroleum Report - Field Information"@en ;
    skos:topConceptOf <https://linked.data.gov.au/def/georesource-report> ;
.

grt:petroleum-report-infrastructure
    a skos:Concept ;
    dcterms:provenance "Developed by the Geological Survey of Queensland." ;
    rdfs:isDefinedBy <https://linked.data.gov.au/def/georesource-report> ;
    skos:altLabel "Petroleum Infrastructure Reports"@en ;
    skos:definition "A report detailing the infrastructure installed for the purpose of gathering, processing and storage of petroleum and gas on a permit or permits. Defined in detail as a part of the Petroleum and Gas (Production and Safety) Act."@en ;
    skos:inScheme <https://linked.data.gov.au/def/georesource-report> ;
    skos:notation "PETIR" ;
    skos:prefLabel "Petroleum Report - Infrastructure"@en ;
    skos:topConceptOf <https://linked.data.gov.au/def/georesource-report> ;
.

grt:petroleum-report-other
    a skos:Concept ;
    dcterms:provenance "Developed by the Geological Survey of Queensland." ;
    rdfs:isDefinedBy <https://linked.data.gov.au/def/georesource-report> ;
    skos:altLabel "ATP Other Report"@en ;
    skos:definition "A report that does not fall under any other category of Petroleum permit reports."@en ;
    skos:inScheme <https://linked.data.gov.au/def/georesource-report> ;
    skos:notation "EPPOTH" ;
    skos:prefLabel "Petroleum Report - Other"@en ;
    skos:topConceptOf <https://linked.data.gov.au/def/georesource-report> ;
.

grt:petroleum-report-transmission
    a skos:Concept ;
    dcterms:provenance "Developed by the Geological Survey of Queensland." ;
    rdfs:isDefinedBy <https://linked.data.gov.au/def/georesource-report> ;
    skos:altLabel "Transmission Report"@en ;
    skos:definition "A report that details the petroleum transmission for a Prospective Gas Production Land Reserve (PGPLR), including its number and the area of the lease, the entities who were supplied through the PGPLR and the volumes they were supplied."@en ;
    skos:inScheme <https://linked.data.gov.au/def/georesource-report> ;
    skos:notation "TRANS" ;
    skos:prefLabel "Petroleum Report - Transmission"@en ;
    skos:topConceptOf <https://linked.data.gov.au/def/georesource-report> ;
.

grt:presentation
    a skos:Concept ;
    dcterms:provenance "Developed by the Geological Survey of Queensland." ;
    rdfs:isDefinedBy <https://linked.data.gov.au/def/georesource-report> ;
    skos:definition "'A speech or talk in which a new product, idea, or piece of work is shown and explained to an audience. Source: Oxford English Dictionary. This includes speeches, talks, multimedia presentations, and posters.'"@en ;
    skos:inScheme <https://linked.data.gov.au/def/georesource-report> ;
    skos:prefLabel "Presentation"@en ;
    skos:topConceptOf <https://linked.data.gov.au/def/georesource-report> ;
.

grt:scientific-or-technical-survey-report
    a skos:Concept ;
    dcterms:provenance "Developed by the Geological Survey of Queensland." ;
    rdfs:isDefinedBy <https://linked.data.gov.au/def/georesource-report> ;
    skos:definition "A report detailing the activities undertaken and their results, as a part of a scientific or non-geophysical survey."@en ;
    skos:inScheme <https://linked.data.gov.au/def/georesource-report> ;
    skos:notation "STSURV" ;
    skos:prefLabel "Scientific or Technical Survey Report"@en ;
    skos:topConceptOf <https://linked.data.gov.au/def/georesource-report> ;
.

grt:seismic-survey-report-final
    a skos:Concept ;
    dcterms:provenance "Developed by the Geological Survey of Queensland." ;
    rdfs:isDefinedBy <https://linked.data.gov.au/def/georesource-report> ;
    skos:altLabel "Seismic Survey Final Report"@en ;
    skos:definition "A report detailing the acquisition, processing, and interpretation of a seismic survey."@en ;
    skos:inScheme <https://linked.data.gov.au/def/georesource-report> ;
    skos:notation "SSFINL" ;
    skos:prefLabel "Seismic Survey Report - Final"@en ;
    skos:topConceptOf <https://linked.data.gov.au/def/georesource-report> ;
.

grt:seismic-survey-report-other
    a skos:Concept ;
    dcterms:provenance "Developed by the Geological Survey of Queensland." ;
    rdfs:isDefinedBy <https://linked.data.gov.au/def/georesource-report> ;
    skos:altLabel "Seismic Survey Report Other"@en ;
    skos:definition "A report detailing activities related to a seismic survey not described in other seismic survey reports."@en ;
    skos:inScheme <https://linked.data.gov.au/def/georesource-report> ;
    skos:notation "SSOTHR" ;
    skos:prefLabel "Seismic Survey Report - Other"@en ;
    skos:topConceptOf <https://linked.data.gov.au/def/georesource-report> ;
.

grt:seismic-survey-report-reprocessing
    a skos:Concept ;
    dcterms:provenance "Developed by the Geological Survey of Queensland." ;
    rdfs:isDefinedBy <https://linked.data.gov.au/def/georesource-report> ;
    skos:altLabel "Seismic Reprocessing Report"@en ;
    skos:definition "A report detailing the reprocessing and interpretation of a previously reported seismic survey."@en ;
    skos:inScheme <https://linked.data.gov.au/def/georesource-report> ;
    skos:notation "SSREPR" ;
    skos:prefLabel "Seismic Survey Report - Reprocessing"@en ;
    skos:topConceptOf <https://linked.data.gov.au/def/georesource-report> ;
.

grt:water-report-performance-review
    a skos:Concept ;
    dcterms:provenance "Developed by the Geological Survey of Queensland." ;
    rdfs:isDefinedBy <https://linked.data.gov.au/def/georesource-report> ;
    skos:altLabel "Performance Review Report"@en ;
    skos:definition "A report detailing the study of the hydrological properties of a region and the effects of extractive activities."@en ;
    skos:inScheme <https://linked.data.gov.au/def/georesource-report> ;
    skos:notation "WATPRR" ;
    skos:prefLabel "Water Report - Performance Review"@en ;
    skos:topConceptOf <https://linked.data.gov.au/def/georesource-report> ;
.

grt:well-completion-report
    a skos:Concept ;
    dcterms:provenance "Developed by the Geological Survey of Queensland." ;
    rdfs:isDefinedBy <https://linked.data.gov.au/def/georesource-report> ;
    skos:altLabel "Well Completion Report"@en ;
    skos:definition "A report detailing the activities and results of drilling a well."@en ;
    skos:inScheme <https://linked.data.gov.au/def/georesource-report> ;
    skos:notation "WELCOM" ;
    skos:prefLabel "Well or Bore Completion Report"@en ;
    skos:topConceptOf <https://linked.data.gov.au/def/georesource-report> ;
.

grt:well-or-bore-abandonment-report
    a skos:Concept ;
    dcterms:provenance "Developed by the Geological Survey of Queensland." ;
    rdfs:isDefinedBy <https://linked.data.gov.au/def/georesource-report> ;
    skos:definition "A report detailing the activities and results of abandoning a well."@en ;
    skos:inScheme <https://linked.data.gov.au/def/georesource-report> ;
    skos:notation "WELAB" ;
    skos:prefLabel "Well or Bore Abandonment Report"@en ;
    skos:topConceptOf <https://linked.data.gov.au/def/georesource-report> ;
.

grt:well-production-testing-report
    a skos:Concept ;
    dcterms:provenance "Developed by the Geological Survey of Queensland." ;
    rdfs:isDefinedBy <https://linked.data.gov.au/def/georesource-report> ;
    skos:definition "A report detailing the testing of the production potential or performance of a petroleum well."@en ;
    skos:inScheme <https://linked.data.gov.au/def/georesource-report> ;
    skos:notation "WELTST" ;
    skos:prefLabel "Well Production Testing Report"@en ;
    skos:topConceptOf <https://linked.data.gov.au/def/georesource-report> ;
.

grt:permit-report-mineral-associated-water
    a skos:Concept ;
    dcterms:provenance "Developed by the Geological Survey of Queensland." ;
    rdfs:isDefinedBy <https://linked.data.gov.au/def/georesource-report> ;
    skos:altLabel
        "Coal or Mineral Permit Report - Mineral Associated Water"@en ,
        "Mineral Associated Water"@en ,
        "Permit Report - Mineral Associated Water"@en ;
    skos:definition "A report detailing the total water produced from a Mining Lease, defined as per the Mineral Resources Act."@en ;
    skos:inScheme <https://linked.data.gov.au/def/georesource-report> ;
    skos:notation "MINAW" ;
    skos:prefLabel "Water Report - Mineral Associated Water"@en ;
    skos:topConceptOf <https://linked.data.gov.au/def/georesource-report> ;
.

grt:permit-report-surrender
    a skos:Concept ;
    dcterms:provenance "Developed by the Geological Survey of Queensland." ;
    rdfs:isDefinedBy <https://linked.data.gov.au/def/georesource-report> ;
    skos:altLabel
        "Permit Report - Surrender"@en ,
        "Surrender Report"@en ;
    skos:definition "A report that is required to be lodged as a part of the obligations of surrendering tenure over a Coal or Oil Shale Mining Lease or Mineral Development Licence where a higher tenure over the same area has not been granted. Required under the Queensland Mineral Resources Regulation 2013, s16 and s29C."@en ;
    skos:inScheme <https://linked.data.gov.au/def/georesource-report> ;
    skos:notation "SURR" ;
    skos:prefLabel "Coal or Mineral Permit Report - Surrender (End of Tenure)"@en ;
    skos:topConceptOf <https://linked.data.gov.au/def/georesource-report> ;
.

grt:petroleum-report-cumulative-water-production
    a skos:Concept ;
    dcterms:provenance "Developed by the Geological Survey of Queensland." ;
    rdfs:isDefinedBy <https://linked.data.gov.au/def/georesource-report> ;
    skos:altLabel "Cumulative Prod/CSG Water Readings - Petroleum"@en ;
    skos:definition "A report detailing the cumulative total of water produced from a well, as mandatory in the Petroleum and Gas Act."@en ;
    skos:inScheme <https://linked.data.gov.au/def/georesource-report> ;
    skos:notation "CUMPRD" ;
    skos:prefLabel "Petroleum Report - Cumulative Water Production"@en ;
    skos:topConceptOf <https://linked.data.gov.au/def/georesource-report> ;
.

grt:production-petroleum
    a skos:Concept ;
    dcterms:provenance "Developed by the Geological Survey of Queensland." ;
    rdfs:isDefinedBy <https://linked.data.gov.au/def/georesource-report> ;
    skos:definition "A report detailing the quantity, quality and other parameters of the production of petroleum and gas products from an ATP as required by the Petroleum and Gas Act and General Provisions. Defined in greater detail as a part of the Petroleum and Gas Reporting Guideline. The legacy format of reporting prior to introduction of the data submission templates and GSQ Lodgement Portal."@en ;
    skos:inScheme <https://linked.data.gov.au/def/georesource-report> ;
    skos:notation "PROD" ;
    skos:prefLabel "Production (Petroleum) - Legacy Format"@en ;
    skos:topConceptOf <https://linked.data.gov.au/def/georesource-report> ;
.

grt:reserves-petroleum
    a skos:Concept ;
    dcterms:provenance "Developed by the Geological Survey of Queensland." ;
    rdfs:isDefinedBy <https://linked.data.gov.au/def/georesource-report> ;
    skos:definition "A report detailing the quantity, quality and other parameters of the reserves of petroleum and gas on an ATP, as required by the Petroleum and Gas Act and General Provisions. Defined in greater detail as a part of the Petroleum and Gas Reporting Guideline. The legacy format of reporting prior to introduction of the data submission templates and GSQ Lodgement Portal."@en ;
    skos:inScheme <https://linked.data.gov.au/def/georesource-report> ;
    skos:notation "RESERV" ;
    skos:prefLabel "Reserves (Petroleum) - Legacy Format"@en ;
    skos:topConceptOf <https://linked.data.gov.au/def/georesource-report> ;
.

grt:geothermal-report-annual-reserves
    a skos:Concept ;
    dcterms:provenance "Developed by the Geological Survey of Queensland." ;
    rdfs:isDefinedBy <https://linked.data.gov.au/def/georesource-report> ;
    skos:altLabel "Geothermal Annual Reserves Reports"@en ;
    skos:definition "A report detailing the quantity, quality and other parameters of the Geothermal reserves and resources on an Geothermal Permit."@en ;
    skos:inScheme <https://linked.data.gov.au/def/georesource-report> ;
    skos:notation "GTHARR" ;
    skos:prefLabel "Geothermal Report - Annual Reserves"@en ;
    skos:topConceptOf <https://linked.data.gov.au/def/georesource-report> ;
.

grt:geothermal-report-production
    a skos:Concept ;
    dcterms:provenance "Developed by the Geological Survey of Queensland." ;
    rdfs:isDefinedBy <https://linked.data.gov.au/def/georesource-report> ;
    skos:altLabel "Geothermal Production Reports"@en ;
    skos:definition "A report detailing the production performance of a geothermal well, wells, or field."@en ;
    skos:inScheme <https://linked.data.gov.au/def/georesource-report> ;
    skos:notation "GTHPR" ;
    skos:prefLabel "Geothermal Report - Production"@en ;
    skos:topConceptOf <https://linked.data.gov.au/def/georesource-report> ;
.

grt:petroleum-report-non-associated-water
    a skos:Concept ;
    dcterms:provenance "Developed by the Geological Survey of Queensland." ;
    rdfs:isDefinedBy <https://linked.data.gov.au/def/georesource-report> ;
    skos:altLabel "Petroleum Non-Associated Water"@en ;
    skos:definition "A report detailing the production of water by a permit holder that was not directly acquired from a petroleum well. Defined as per the Petroleum and Gas Act."@en ;
    skos:inScheme <https://linked.data.gov.au/def/georesource-report> ;
    skos:notation "PETNAW" ;
    skos:prefLabel "Petroleum Report - Non-Associated Water"@en ;
    skos:topConceptOf <https://linked.data.gov.au/def/georesource-report> ;
.

grt:petroleum-report-production-information
    a skos:Concept ;
    dcterms:provenance "Developed by the Geological Survey of Queensland." ;
    rdfs:isDefinedBy <https://linked.data.gov.au/def/georesource-report> ;
    skos:altLabel "Petroleum Production Information (Good Practice)"@en ;
    skos:definition "A report detailing the quantity, quality and other parameters of the production of petroleum and gas products from an ATP as required by the Petroleum and Gas Act and General Provisions. Defined in greater detail as a part of the Petroleum and Gas Reporting Guideline. These reports are submitted using the Queensland Government templates."@en ;
    skos:inScheme <https://linked.data.gov.au/def/georesource-report> ;
    skos:notation "PROINF" ;
    skos:prefLabel "Petroleum Report - Petroleum Production Report"@en ;
    skos:topConceptOf <https://linked.data.gov.au/def/georesource-report> ;
.

grt:petroleum-report-resource-and-reserves-information
    a skos:Concept ;
    dcterms:provenance "Developed by the Geological Survey of Queensland." ;
    rdfs:isDefinedBy <https://linked.data.gov.au/def/georesource-report> ;
    skos:altLabel "Petroleum Reserves and Resources Information (Good Practice)"@en ;
    skos:definition "A report detailing the quantity, quality and other parameters of the reserves of petroleum and gas on an ATP, as required by the Petroleum and Gas Act and General Provisions. Defined in greater detail as a part of the Petroleum and Gas Reporting Guideline. These reports are submitted using the Queensland Government templates."@en ;
    skos:inScheme <https://linked.data.gov.au/def/georesource-report> ;
    skos:notation "RESINF" ;
    skos:prefLabel "Petroleum Report - Petroleum Resources and Reserves Report"@en ;
    skos:topConceptOf <https://linked.data.gov.au/def/georesource-report> ;
.

<https://linked.data.gov.au/def/georesource-report>
    a
        owl:Ontology ,
        skos:ConceptScheme ;
    dcterms:created "2019-10-09"^^xsd:date ;
    dcterms:creator <https://linked.data.gov.au/org/gsq> ;
    dcterms:modified "2023-03-16"^^xsd:date ;
    dcterms:provenance "Developed by the Geological Survey of Queensland." ;
    dcterms:publisher <https://linked.data.gov.au/org/gsq> ;
    skos:definition "The types of reports administered by the GeoResources Division of the Department of Resources."@en ;
    skos:hasTopConcept
        grt:annual-report ,
        grt:any-other-report ,
        grt:article ,
        grt:coal-quarterly-statistics ,
        grt:collaborative-drilling-initiative-final ,
        grt:collaborative-drilling-initiative-proposals ,
        grt:collaborative-exploration-initiative-final ,
        grt:collaborative-exploration-initiative-proposals ,
        grt:commissioned-industry-study-or-report ,
        grt:converted-from-qerd ,
        grt:departmental-drilling ,
        grt:extractives-annual-statistics ,
        grt:geological-survey-of-queensland-publication ,
        grt:geological-survey-of-queensland-record ,
        grt:geophysical-survey-report-acquisition ,
        grt:geophysical-survey-report-final ,
        grt:geophysical-survey-report-logistics ,
        grt:geothermal-end-tenure ,
        grt:geothermal-report-annual ,
        grt:geothermal-report-annual-reserves ,
        grt:geothermal-report-injection ,
        grt:geothermal-report-injection-testing ,
        grt:geothermal-report-production ,
        grt:geothermal-report-production-testing ,
        grt:geothermal-report-relinquishment ,
        grt:geothermal-report-surrender ,
        grt:greenhouse-gas-report-injection ,
        grt:greenhouse-gas-report-storage-capacity ,
        grt:greenhouse-gas-report-storage-injection ,
        grt:hydraulic-fracturing-activity-report ,
        grt:industry-consultative-report ,
        grt:industry-network-initiative-final ,
        grt:mine-plan-lodgement ,
        grt:minerals-annual-statistics ,
        grt:mmol-44 ,
        grt:pa-21A ,
        grt:pa-22A ,
        grt:pa-42 ,
        grt:permit-report-annual ,
        grt:permit-report-annual-ml ,
        grt:permit-report-final ,
        grt:permit-report-final-higher-tenure ,
        grt:permit-report-final-relinquishment ,
        grt:permit-report-mineral-associated-water ,
        grt:permit-report-other ,
        grt:permit-report-partial-relinquishment ,
        grt:permit-report-partial-relinquishment-higher-tenure ,
        grt:permit-report-six-month ,
        grt:permit-report-surrender ,
        grt:permit-report-surrender-higher-tenure ,
        grt:petroleum-end-authority ,
        grt:petroleum-end-tenure ,
        grt:petroleum-report-annual ,
        grt:petroleum-report-cumulative-water-production ,
        grt:petroleum-report-field-information ,
        grt:petroleum-report-infrastructure ,
        grt:petroleum-report-non-associated-water ,
        grt:petroleum-report-other ,
        grt:petroleum-report-production-information ,
        grt:petroleum-report-relinquishment ,
        grt:petroleum-report-resource-and-reserves-information ,
        grt:petroleum-report-surrender ,
        grt:petroleum-report-transmission ,
        grt:pggd-01 ,
        grt:pggd-02 ,
        grt:pggd-03 ,
        grt:pggd-04 ,
        grt:pipeline-report-surrender ,
        grt:pm-1-2013 ,
        grt:presentation ,
        grt:production-petroleum ,
        grt:queensland-government-mining-journal ,
        grt:reserves-petroleum ,
        grt:scientific-or-technical-survey-report ,
        grt:seismic-survey-report-final ,
        grt:seismic-survey-report-other ,
        grt:seismic-survey-report-reprocessing ,
        grt:soil-and-land-resources ,
        grt:survey-plan ,
        grt:technical-report ,
        grt:thesis ,
        grt:water-report-other ,
        grt:water-report-performance-review ,
        grt:well-completion-report ,
        grt:well-or-bore-abandonment-report ,
        grt:well-production-testing-report ,
        grt:well-proposal ,
        grt:well-report-other ,
        grt:wra-05A ;
    skos:prefLabel "Georesource Report"@en ;
.

