PREFIX agldwgstatus: <https://linked.data.gov.au/def/reg-statuses/>
PREFIX als: <http://linked.data.gov.au/def/gsq-alias/>
PREFIX cs: <http://linked.data.gov.au/def/gsq-alias>
PREFIX dcterms: <http://purl.org/dc/terms/>
PREFIX owl: <http://www.w3.org/2002/07/owl#>
PREFIX rdfs: <http://www.w3.org/2000/01/rdf-schema#>
PREFIX reg: <http://purl.org/linked-data/registry#>
PREFIX sdo: <https://schema.org/>
PREFIX skos: <http://www.w3.org/2004/02/skos/core#>
PREFIX xsd: <http://www.w3.org/2001/XMLSchema#>

als:company
    a skos:Collection ;
    skos:historyNote "Compiled by the Geological Survey of Queensland" ;
    skos:definition "Aliases for entities or activities used by companies."@en ;
    skos:member
        als:operator ,
        als:service-provider ;
    skos:prefLabel "Company"@en ;
.

als:feature
    a skos:Collection ;
    skos:historyNote "Compiled by the Geological Survey of Queensland" ;
    skos:definition "Aliases and their sources used when describing geologic features."@en ;
    skos:member
        als:asud ,
        als:asud-indirect ,
        als:informal ,
        als:misspelt ,
        als:obsolete ,
        als:operator ,
        als:variation ;
    skos:prefLabel "Feature Alias"@en ;
.

als:government
    a skos:Collection ;
    skos:historyNote "Compiled by the Geological Survey of Queensland" ;
    skos:definition "Aliases used by other groups within the Department, other departments within Queensland Government, or other Government Agencies."@en ;
    skos:member
        als:des ,
        als:geoscience-australia ,
        als:mmol ,
        als:ogia ,
        als:treasury ;
        als:wims-sample-id ;
    skos:prefLabel "Government"@en ;
.

als:asud-indirect
    a skos:Concept ;
    skos:historyNote "Compiled by the Geological Survey of Queensland" ;
    rdfs:isDefinedBy cs: ;
    skos:altLabel "ASUD Indirect"@en ;
    skos:broader als:asud ;
    skos:definition "The Stratigraphic Number used in Geoscience Australia's Australian Stratigraphic Units Database where the match is to a unit listed in the ASUD as non-current, a variation, or an otherwise informal or obsolete unit."@en ;
    skos:inScheme cs: ;
    skos:prefLabel "Australian Stratigraphic Units Database (Indirect)"@en ;
.

als:colloquial
    a skos:Concept ;
    skos:historyNote "Compiled by the Geological Survey of Queensland" ;
    rdfs:isDefinedBy cs: ;
    skos:altLabel
        "Common"@en ,
        "Popular"@en ,
        "Public"@en ;
    skos:definition "An unofficial, informal, or colloquial name or reference used by the general public, industry, or government."@en ;
    skos:inScheme cs: ;
    skos:prefLabel "Colloquial"@en ;
    skos:topConceptOf cs: ;
.

als:firstNations
    a skos:Concept ;
    skos:historyNote "Compiled by the Geological Survey of Queensland" ;
    rdfs:isDefinedBy cs: ;
    skos:definition "The informal standing (in terms of an overriding code or protocol) that is attributed to the current First Nations name of a feature, such a lithologic rock unit, under the dual naming policy for Aboriginal and Torres Strait Islander place names, e.g., the Mount Warning Central Complex being named Wollumbin (fighting chief of the mountains)."@en ;
    skos:inScheme cs: ;
    skos:prefLabel "First Nations"@en ;
    skos:topConceptOf cs: ;
.

als:formal
    a skos:Concept ;
    skos:historyNote "Compiled by the Geological Survey of Queensland" ;
    rdfs:isDefinedBy cs: ;
    skos:altLabel "defined"@en ;
    skos:definition "The standing that is attributed to a formal name, with non-current usage, that has been formally replaced, if only partially, by another formal name, such as with the change in the ending of the name of a lithologic rock unit (e.g., from ‘Formation’ to Sandstone’ or similar) or a formal name has been replaced, if only partially, by an informal name (e.g., Stanwell Coal Measures to Stanwell 'Formation'/formation). This applies to other types of rock units, such as biostratigraphic units, which are rocks characterized by their fossil content, not their lithologic attributes."@en ;
    skos:inScheme cs: ;
    skos:prefLabel "Formal"@en ;
    skos:topConceptOf cs: ;
.

als:gsq-legacy
    a skos:Concept ;
    skos:historyNote "Compiled by the Geological Survey of Queensland" ;
    rdfs:isDefinedBy cs: ;
    skos:definition "Any superseded identifier, code, or name previously used by the Geological Survey of Queensland."@en ;
    skos:inScheme cs: ;
    skos:prefLabel "GSQ Legacy"@en ;
    skos:topConceptOf cs: ;
.

als:gsqr-number
    a skos:Concept ;
    skos:historyNote "Compiled by the Geological Survey of Queensland. The use of GSQR and GSQM numbers was separate up to about GSQR11000, from then (about 1997) they were synomymous (GSQR=GSQM) until the numbers where disused in about 2003." ;
    rdfs:isDefinedBy cs: ;
    skos:altLabel "GSQ Rock Number"@en ;
    skos:broader als:gsq-legacy ;
    skos:definition "A legacy unique identifier that links the rock sample with the petrological description reports. "@en ;
    skos:inScheme cs: ;
    skos:prefLabel "GSQR"@en ;
.

als:gsqm-number
    a skos:Concept ;
    skos:historyNote "Compiled by the Geological Survey of Queensland. The use of GSQR and GSQM numbers was separate up to about GSQR11000, from then (about 1997) they were synomymous (GSQR=GSQM) until the numbers where disused in about 2003. " ;
    rdfs:isDefinedBy cs: ;
    skos:altLabel "GSQ Microslide Number"@en ;
    skos:broader als:gsq-legacy ;
    skos:definition "A legacy unique identifier that links the microslide sample with the petrological description reports."@en ;
    skos:inScheme cs: ;
    skos:prefLabel "GSQM"@en ;
.

als:wims-sample-id
    a skos:Concept ;
    skos:historyNote "Generated by the Warehouse Inventory Management System" ;
    rdfs:isDefinedBy cs: ;
    skos:definition "A unique identifier for samples within the Warehouse Inventory Management System (WIMS)."@en ;
    skos:inScheme cs: ;
    skos:prefLabel "WIMS Sample Id"@en ;
    skos:topConceptOf cs: ;
.

als:igsn
    a skos:Concept ;
    skos:historyNote "Compiled by the Geological Survey of Queensland" ;
    rdfs:isDefinedBy cs: ;
    skos:altLabel "International Geo Sample Number"@en ;
    skos:definition "An identifier used as a globally unique and persistent identifier for material samples."@en ;
    skos:inScheme cs: ;
    skos:prefLabel "IGSN"@en ;
    skos:topConceptOf cs: ;
.

als:invalid
    a skos:Concept ;
    skos:historyNote "Compiled by the Geological Survey of Queensland" ;
    rdfs:isDefinedBy cs: ;
    skos:definition "The standing attributed to a rock unit the name and parameters of which have been published, but not in accordance with a national, international and/or other code or protocol that applies thereto (e.g., the International Stratigraphic Guide), rendering the unit with invalid status (as opposed to informal status). A yet-to-be corrected (replaced) rock unit example of this (as at 09.08.2022) is represented by the current name ‘Balfes Creek beds’, as the name ‘Balfes Creek Granodiorite’ has precedence (see ASUD Stratigraphic Number 36156). Upon replacement by a new name (with current status), the Balfes Creek beds will then be regarded as an alias (with invalid standing) of the new name of the rock unit that then has currency."@en ;
    skos:inScheme cs: ;
    skos:prefLabel "Invalid"@en ;
    skos:topConceptOf cs: ;
.

als:rshq
    a skos:Concept ;
    skos:historyNote "Compiled by the Geological Survey of Queensland" ;
    rdfs:isDefinedBy cs: ;
    skos:altLabel "Resources Safety and Health Queensland"@en ;
    skos:definition "An identifier used by Resources Safety and Health Queensland."@en ;
    skos:inScheme cs: ;
    skos:prefLabel "RSHQ"@en ;
    skos:topConceptOf cs: ;
.

als:unnamed
    a skos:Concept ;
    skos:historyNote "Compiled by the Geological Survey of Queensland" ;
    rdfs:isDefinedBy cs: ;
    skos:definition "The previous standing of a geological feature that was recorded in published or unpublished reports, records, maps, etc., and was not then named but now is named or part of it is named. The previously unnamed feature may have had a composite label, but not a true name, e.g., a complex rock unit that was comprised of multiple other rock units, one or more of which is now named."@en ;
    skos:inScheme cs: ;
    skos:prefLabel "Unnamed"@en ;
    skos:topConceptOf cs: ;
.

als:variation
    a skos:Concept ;
    skos:historyNote "Compiled by the Geological Survey of Queensland" ;
    rdfs:isDefinedBy cs: ;
    skos:altLabel "Alternate Name"@en ;
    skos:definition "An alternate term to refer to the same feature, that is recognised but not the official preferred name."@en ;
    skos:inScheme cs: ;
    skos:prefLabel "Variation"@en ;
    skos:topConceptOf cs: ;
.

als:asud
    a skos:Concept ;
    skos:historyNote "Compiled by the Geological Survey of Queensland" ;
    rdfs:isDefinedBy cs: ;
    skos:altLabel "ASUD"@en ;
    skos:broader als:geoscience-australia ;
    skos:definition "The Stratigraphic Number used in Geoscience Australia's Australian Stratigraphic Units Database. Used where the match is exact and direct."@en ;
    skos:inScheme cs: ;
    skos:prefLabel "Australian Stratigraphic Units Database"@en ;
.

als:des
    a skos:Concept ;
    skos:historyNote "Compiled by the Geological Survey of Queensland" ;
    rdfs:isDefinedBy cs: ;
    skos:altLabel "Department of Environment and Science"@en ;
    skos:definition "An identifier used by the Department of Environment and Science"@en ;
    skos:inScheme cs: ;
    skos:prefLabel "DES"@en ;
    skos:topConceptOf cs: ;
.

als:informal
    a skos:Concept ;
    skos:historyNote "Compiled by the Geological Survey of Queensland" ;
    rdfs:isDefinedBy cs: ;
    skos:definition "The standing that is attributed to a name that has not been formally instituted or recognized, such as under a national or international code or protocol (e.g., the International Stratigraphic Guide), and does not have current usage, as it has been replaced (superseded) by a formal name or another informal name. An example of the latter, in terms of lithologic rock units, embraces the name change from the ‘Taroom beds’ to the ‘Chong beds' (Hettangian/basal Jurassic), as the former name is preoccupied by the Taroom Coal Measures."@en ;
    skos:inScheme cs: ;
    skos:prefLabel "Informal"@en ;
    skos:topConceptOf cs: ;
.

als:misspelt
    a skos:Concept ;
    skos:historyNote "Compiled by the Geological Survey of Queensland" ;
    rdfs:isDefinedBy cs: ;
    skos:altLabel "Misspelt"@en ;
    skos:definition "The standing of a geologic feature, such as a lithologic rock unit, the name of which has been systematically misspelt or seemingly misspelt."@en ;
    skos:inScheme cs: ;
    skos:prefLabel "Misspelling"@en ;
    skos:topConceptOf cs: ;
.

als:mmol
    a skos:Concept ;
    skos:historyNote "Compiled by the Geological Survey of Queensland" ;
    rdfs:isDefinedBy cs: ;
    skos:altLabel "MyMinesOnline"@en ;
    skos:definition "An identifier used by the MyMinesOnline system administered by the Department."@en ;
    skos:inScheme cs: ;
    skos:prefLabel "MMOL"@en ;
    skos:topConceptOf cs: ;
.

als:obsolete
    a skos:Concept ;
    skos:historyNote "Compiled by the Geological Survey of Queensland" ;
    rdfs:isDefinedBy cs: ;
    skos:definition "The standing that is attributed to a name or term through lack of use and/or persistent change of use and that has been replaced by another name or term, either as a simple equal replacement or in a complicated, unequal (not one-to-one) process."@en ;
    skos:inScheme cs: ;
    skos:prefLabel "Obsolete"@en ;
    skos:topConceptOf cs: ;
.

als:ogia
    a skos:Concept ;
    skos:historyNote "Compiled by the Geological Survey of Queensland" ;
    rdfs:isDefinedBy cs: ;
    skos:altLabel
        "OGIA"@en ,
        "Office of Groundwater Impact Assessment"@en ;
    skos:definition "An identifier used by the Office of Groundwater Impact Assessment."@en ;
    skos:inScheme cs: ;
    skos:prefLabel "QWRC"@en ;
    skos:topConceptOf cs: ;
.

als:service-provider
    a skos:Concept ;
    skos:historyNote "Compiled by the Geological Survey of Queensland" ;
    rdfs:isDefinedBy cs: ;
    skos:altLabel "Contractor"@en ;
    skos:definition "An identifier used by the company who originally conducted activity on behalf of the operator."@en ;
    skos:inScheme cs: ;
    skos:prefLabel "Service Provider"@en ;
    skos:topConceptOf cs: ;
.

als:treasury
    a skos:Concept ;
    skos:historyNote "Compiled by the Geological Survey of Queensland" ;
    rdfs:isDefinedBy cs: ;
    skos:altLabel "Queensland Treasury"@en ;
    skos:definition "An identifier used by the Queensland Treasury."@en ;
    skos:inScheme cs: ;
    skos:prefLabel "Treasury"@en ;
    skos:topConceptOf cs: ;
.

<https://linked.data.gov.au/org/gsq>
    a sdo:Organization ;
    sdo:name "Geological Survey of Queensland" ;
    sdo:url "https://www.business.qld.gov.au/industries/mining-energy-water/resources/geoscience-information/gsq"^^xsd:anyURI ;
.

als:geoscience-australia
    a skos:Concept ;
    skos:historyNote "Compiled by the Geological Survey of Queensland" ;
    rdfs:isDefinedBy cs: ;
    skos:altLabel "GA"@en ;
    skos:definition "An identifier used by Geoscience Australia"@en ;
    skos:inScheme cs: ;
    skos:prefLabel "Geoscience Australia"@en ;
    skos:topConceptOf cs: ;
.

als:operator
    a skos:Concept ;
    skos:historyNote "Compiled by the Geological Survey of Queensland" ;
    rdfs:isDefinedBy cs: ;
    skos:definition "An identifier used by the company who originally owned or operated an asset or activity."@en ;
    skos:inScheme cs: ;
    skos:prefLabel "Operator"@en ;
    skos:topConceptOf cs: ;
.

cs:
    a
        owl:Ontology ,
        skos:ConceptScheme ;
    dcterms:created "2020-03-23"^^xsd:date ;
    dcterms:creator <https://linked.data.gov.au/org/gsq> ;
    dcterms:modified "2025-07-10"^^xsd:date ;
    skos:historyNote "Compiled by the Geological Survey of Queensland" ;
    dcterms:publisher <https://linked.data.gov.au/org/gsq> ;
    reg:status agldwgstatus:stable ;
    skos:definition "Sources for any alternate names for features, sites, surveys, or samples catalogued by the Geological Survey of Queensland."@en ;
    skos:hasTopConcept
        als:colloquial ,
        als:des ,
        als:firstNations ,
        als:formal ,
        als:geoscience-australia ,
        als:gsq-legacy ,
        als:igsn ,
        als:informal ,
        als:invalid ,
        als:misspelt ,
        als:mmol ,
        als:obsolete ,
        als:ogia ,
        als:operator ,
        als:rshq ,
        als:service-provider ,
        als:treasury ,
        als:wims-sample-id ,
        als:unnamed ;
    skos:prefLabel "GSQ Alias"@en ;
.

