PREFIX agldwgstatus: <http://linked.data.gov.au/def/reg-statuses/>
PREFIX cs: <http://linked.data.gov.au/def/gsq-feature-status>
PREFIX dcterms: <http://purl.org/dc/terms/>
PREFIX fst: <http://linked.data.gov.au/def/gsq-feature-status/>
PREFIX owl: <http://www.w3.org/2002/07/owl#>
PREFIX reg: <http://purl.org/linked-data/registry#>
PREFIX sdo: <https://schema.org/>
PREFIX skos: <http://www.w3.org/2004/02/skos/core#>
PREFIX xsd: <http://www.w3.org/2001/XMLSchema#>

fst:BrieflyDescribed
    a skos:Concept ;
    dcterms:provenance "Compiled by the Geological Survey of Queensland" ;
    skos:broader fst:Informal ;
    skos:definition "A geological feature that has been briefly described in a publication (e.g., in a table), a standard geological map series legend, or in a report, but not as a formal definition. A geological feature described by some, but minimal, defining information."@en ;
    skos:inScheme cs: ;
    skos:notation "fstibd" ;
    skos:prefLabel "Briefly described"@en ;
.

fst:Described
    a skos:Concept ;
    dcterms:provenance "Compiled by the Geological Survey of Queensland" ;
    skos:broader fst:Informal ;
    skos:definition "A geological feature that has been described in a publication, but not as a formal definition that conforms with the accepted standard, such as the International Stratigraphic Guide for rock units"@en ;
    skos:inScheme cs: ;
    skos:notation "fstide" ;
    skos:prefLabel "Described"@en ;
.

fst:Formal
    a skos:Concept ;
    dcterms:provenance "Compiled by the Geological Survey of Queensland" ;
    skos:altLabel "Defined"@en ;
    skos:definition "The status of a geological feature the name and parameters of which are in current use, and have been intentionally/formally defined and/or delineated by printed and/or digital publication (including Geoscience Australia's Australian Stratigraphic Units Database/ASUD) in accordance with a national, international and/or other code or protocol that applies thereto."@en ;
    skos:inScheme cs: ;
    skos:notation "fstfr" ;
    skos:prefLabel "Formal"@en ;
.

fst:FullyDescribed
    a skos:Concept ;
    dcterms:provenance "Compiled by the Geological Survey of Queensland" ;
    skos:broader fst:Informal ;
    skos:definition "A geological feature that has been described in full in a publication, but not as a formal definition that conforms with the accepted standard, such as the International Stratigraphic Guide for rock units, e.g., no type specified."@en ;
    skos:inScheme cs: ;
    skos:notation "fstifd" ;
    skos:prefLabel "Fully described"@en ;
.

fst:Invalid
    a skos:Concept ;
    dcterms:provenance "Compiled by the Geological Survey of Queensland" ;
    skos:definition "The status of a geological feature in which the name and parameters have been published, but not in accordance with a national, international and/or other code or protocol that applies thereto (e.g., the International Stratigraphic Guide), rendering the feature with invalid status as opposed to informal status."@en ;
    skos:inScheme cs: ;
    skos:notation "fstiv" ;
    skos:prefLabel "Invalid"@en ;
    skos:scopeNote "For example: The name Balfes Creek beds (ASUD Stratigraphic Number  36156) is invalid because the Balfes Creek Granodiorite has precedence as a reserved and defined rock unit in Queensland. There is also uncertainty as to whether the rocks associated with the Balfes Creek beds are representative of the Boonderoo beds in the northeastern Galilee Basin, occurring in a structurally-preserved remnant of this basin or occurring as equivalents of the Boonderoo beds in a separate basin."@en ;
.

fst:Mentioned
    a skos:Concept ;
    dcterms:provenance "Compiled by the Geological Survey of Queensland" ;
    skos:broader fst:Informal ;
    skos:definition "A geological feature that has been mentioned in a publication (e.g., in a table), a standard geological map series legend, or in a report, but not as a formal definition. A geological feature mentioned, but where no defining details have been given."@en ;
    skos:inScheme cs: ;
    skos:notation "fstime" ;
    skos:prefLabel "Mentioned"@en ;
.

fst:Obsolete
    a skos:Concept ;
    dcterms:provenance "Compiled by the Geological Survey of Queensland" ;
    skos:definition "A geological feature that has fallen into disuse (not used in the literature for at least 50 years)."@en ;
    skos:inScheme cs: ;
    skos:notation "fstob" ;
    skos:prefLabel "Obsolete"@en ;
    skos:scopeNote "An obsolete feature status indicates that the feature itself is no longer recognised or in use. This is in contrast to an obsolete or legacy name or alias for a feature that is still in use but whose name has changed."@en ;
.

fst:Reserved
    a skos:Concept ;
    dcterms:provenance "Compiled by the Geological Survey of Queensland" ;
    skos:altLabel "Reserved by GA"@en ;
    skos:definition "The status of a feature reserved for use with the relevant governing body or agency with authority over the subject domain. For example, a rock unit requested of, and accorded by, the Stratigraphic Index Officer of Geoscience Australia for the claim of a name for a rock unit (reserved for up to five years) prior to its hard-copy and/or digital publication."@en ;
    skos:inScheme cs: ;
    skos:notation "fstre" ;
    skos:prefLabel "Reserved"@en ;
    skos:scopeNote "For example: The 'Baga beds'[AUSD Stratigraphic No. 81555, 'Reserved by Geoscience Australia' at the request of Paul Blake (GSQ) on 20.08.2019] which superseded the 'Jim Crow beds' (AUSD Stratigraphic No. 74880) on 02.02.2021 (AUSD, Geoscience Australia, accessed on 08.02.2021)."@en ;
.

fst:Unconfirmed
    a skos:Concept ;
    dcterms:provenance "Compiled by the Geological Survey of Queensland" ;
    skos:definition "The status of a geological feature that is known to have been published, but the status of the publication was not known at the time the record was created; this incorporates features the status of which needs to be ascertained against the literature and, for lithologic rock units, also against Geoscience Australia’s ASUD."@en ;
    skos:inScheme cs: ;
    skos:notation "fstuc" ;
    skos:prefLabel "Unconfirmed"@en ;
    skos:scopeNote "Geoscience Australia definition supported here, additional to above: A distinctive area of rocks (polygon(s) in a dataset), where the rocks have been assigned a description, but not a name. Often used for subsurface units that are based on geophysical properties alone. Also used for very broad-scale maps where named units are too small to be displayed at the intended scale. ASUD does not have the resources to record all of these unnamed units created by all the State and Territory Surveys in any useful way, but this organisation’s current GIS dataset structure requires a 'stratno' for all geological polygons, so it does currently record any unnamed units used in its datasets."@en ;
.

fst:Unnamed
    a skos:Concept ;
    dcterms:provenance "Compiled by the Geological Survey of Queensland" ;
    skos:broader fst:Informal ;
    skos:definition "The status of a geological feature that has been recorded in published or unpublished reports, records, maps, etc., but has not been named. This may include features that have a composite label, but not a true name. For example a complex rock unit that is comprised of multiple other rock units and is only used within the scope of scale-dependent mapping"@en ;
    skos:inScheme cs: ;
    skos:notation "fstun" ;
    skos:prefLabel "Unnamed"@en ;
    skos:scopeNote "Geoscience Australia definition supported here, additional to above: A distinctive area of rocks (polygon(s) in a dataset), where the rocks have been assigned a description, but not a name. Often used for subsurface units that are based on geophysical properties alone. Also used for very broad-scale maps where named units are too small to be displayed at the intended scale. ASUD does not have the resources to record all of these unnamed units created by all the State and Territory Surveys in any useful way, but this organisation’s current GIS dataset structure requires a 'stratno' for all geological polygons, so it does currently record any unnamed units used in its datasets."@en ;
.

<https://linked.data.gov.au/org/gsq>
    a
        owl:NamedIndividual ,
        sdo:Organization ;
    sdo:email <mailto:geological_info@resources.qld.gov.au> ;
    sdo:name "Geological Survey of Queensland" ;
    sdo:url "https://www.business.qld.gov.au/industries/mining-energy-water/resources/geoscience-information/gsq"^^xsd:anyURI ;
.

fst:Informal
    a skos:Concept ;
    dcterms:provenance "Compiled by the Geological Survey of Queensland" ;
    skos:definition "The status of a geological feature the name and parameters of which are in current use, and have been informally defined and/or delineated, including mere mentioning, in printed and/or digital material, either published or unpublished (e.g., theses, company exploration reports, maps, etc.), and not in accordance with a national, international and/or other code or protocol for formal definition."@en ;
    skos:inScheme cs: ;
    skos:notation "fstir" ;
    skos:prefLabel "Informal"@en ;
    skos:scopeNote "Examples include the Eddystone beds (ASUD Stratigraphic Number 5953), the Chong beds (ASUD Stratigraphic Number 78567), and the Reids Dome beds (ASUD Stratigraphic Number 16012), all of which currently defy formal definition, because of a lack of detail to do so."@en ;
.

cs:
    a
        owl:Ontology ,
        skos:ConceptScheme ;
    dcterms:created "2022-08-08"^^xsd:date ;
    dcterms:creator <https://linked.data.gov.au/org/gsq> ;
    dcterms:modified "2023-03-16"^^xsd:date ;
    dcterms:provenance "Compiled by the Geological Survey of Queensland" ;
    dcterms:publisher <https://linked.data.gov.au/org/gsq> ;
    reg:status agldwgstatus:stable ;
    skos:definition "The status of a geologic feature, which in name (and definition) may embrace formal, informal, invalid, and other terms, is generally regulated variously (depending on the feature type) by a national, international and/or other code or protocol that applies thereto, and, where applicable, may be administered and/or reviewed by a relevant authority, such as the Geological Survey of Queensland or (for Australian rock units) by Geoscience Australia in collaboration with the Australian Stratigraphy Commission of the Geological Society of Australia."@en ;
    skos:hasTopConcept
        fst:BrieflyDescribed ,
        fst:Described ,
        fst:Formal ,
        fst:FullyDescribed ,
        fst:Informal ,
        fst:Invalid ,
        fst:Mentioned ,
        fst:Obsolete ,
        fst:Reserved ,
        fst:Unconfirmed ,
        fst:Unnamed ;
    skos:prefLabel "Geologic Feature Status"@en ;
.

