@prefix dc: <http://purl.org/dc/elements/1.1/> .
@prefix dcterms: <http://purl.org/dc/terms/> .
@prefix dcterms: <http://purl.org/dc/terms/> .
@prefix id: <http://linked.data.gov.au/def/party-identifier-type/> .
@prefix owl: <http://www.w3.org/2002/07/owl#> .
@prefix schema: <http://schema.org/> .
@prefix sdo: <http://schema.org/> .
@prefix skos: <http://www.w3.org/2004/02/skos/core#> .
@prefix rdfs: <http://www.w3.org/2000/01/rdf-schema#> .
@prefix xsd: <http://www.w3.org/2001/XMLSchema#> .

<http://linked.data.gov.au/def/party-identifier-type> a owl:Ontology,
        skos:ConceptScheme ;
    dcterms:created "2020-03-25"^^xsd:date ;
    dcterms:creator <http://linked.data.gov.au/org/gsq> ;
    dcterms:modified "2020-03-25"^^xsd:date ;
    dcterms:publisher <http://linked.data.gov.au/org/gsq> ;
    dcterms:provenance "Compiled by the Geological Survey of Queensland. From (QGOV)<http://account.qld.gov.au/help/faq.html#howDoIProvide100PointsOfIdentification> and (MyMinesOnline) <http://www.business.qld.gov.au/industries/mining-energy-water/resources/minerals-coal/online-services/myminesonline/register>" ;
    skos:definition "Types of Identification documents and numbers used in Queensland as acceptable proof of identity for individuals, businesses, and companies. Required and accepted documents by the QGOV and MyMinesOnline systems."@en ;
    skos:prefLabel "Party Identification Type"@en .

<http://linked.data.gov.au/org/gsq> a sdo:Organization ;
    sdo:name "Geological Survey of Queensland" ;
    sdo:url "http://www.business.qld.gov.au/industries/mining-energy-water/resources/geoscience-information/gsq"^^xsd:anyURI .

id:c-code a skos:Concept ;
 skos:definition "A locally relevant company code, commonly locally administered by an individual agency."@en ;
    rdfs:isDefinedBy <http://linked.data.gov.au/def/party-identifier-type> ;
 skos:inScheme <http://linked.data.gov.au/def/party-identifier-type> ;
 skos:prefLabel "Company Code"@en ;
 skos:topConceptOf <http://linked.data.gov.au/def/party-identifier-type> .

id:abn a skos:Concept ;
 skos:altLabel "Australian business number"@en ;
 skos:definition "The Australian Business Number (ABN) is a unique number used to identify business names and companies. The Australian Business Register (ABR) provides ABNs. Source:ASIC"@en ;
    rdfs:isDefinedBy <http://linked.data.gov.au/def/party-identifier-type> ;
 skos:inScheme <http://linked.data.gov.au/def/party-identifier-type> ;
 skos:prefLabel "ABN"@en ;
 skos:topConceptOf <http://linked.data.gov.au/def/party-identifier-type> .

id:acn a skos:Concept ;
 skos:altLabel "Australian company number"@en ;
 skos:definition "Every company in Australia is issued with a unique, nine-digit number when registered. This is an Australian Company Number (ACN) and must be displayed on all company documents. Source:ASIC"@en ;
    rdfs:isDefinedBy <http://linked.data.gov.au/def/party-identifier-type> ;
 skos:inScheme <http://linked.data.gov.au/def/party-identifier-type> ;
 skos:prefLabel "ACN"@en ;
 skos:topConceptOf <http://linked.data.gov.au/def/party-identifier-type> .

id:australian-university-id-card a skos:Concept ;
 skos:definition "An identification card issued by a recognised Australian tertiary education institute. Cards must be less than 1 year old to be valid."@en ;
    rdfs:isDefinedBy <http://linked.data.gov.au/def/party-identifier-type> ;
 skos:inScheme <http://linked.data.gov.au/def/party-identifier-type> ;
 skos:prefLabel "Australian university ID card"@en ;
 skos:topConceptOf <http://linked.data.gov.au/def/party-identifier-type> .

id:australian-visa a skos:Concept ;
 skos:definition "A conditional permit granted to a foreign national by the Australian Government conveying rights of entry, residence, or work within the country."@en ;
    rdfs:isDefinedBy <http://linked.data.gov.au/def/party-identifier-type> ;
 skos:inScheme <http://linked.data.gov.au/def/party-identifier-type> ;
 skos:prefLabel "Australian visa"@en ;
 skos:topConceptOf <http://linked.data.gov.au/def/party-identifier-type> .

id:bank-card a skos:Concept ;
 skos:altLabel "Bank passbook"@en,
 "Credit Card"@en,
 "Credit card, bank card or bank passbook"@en ;
 skos:definition "A card issued by a financial institution for the purpose of identity and account access."@en ;
    rdfs:isDefinedBy <http://linked.data.gov.au/def/party-identifier-type> ;
 skos:inScheme <http://linked.data.gov.au/def/party-identifier-type> ;
 skos:prefLabel "Bank Card"@en ;
 skos:topConceptOf <http://linked.data.gov.au/def/party-identifier-type> .

id:birth-certificate a skos:Concept ;
 skos:definition "A vital record that documents the birth of a child. Birth certificates may be the original document certifying the circumstances of the birth or to a certified copy or representation of the ensuing registration of that birth. "@en ;
    rdfs:isDefinedBy <http://linked.data.gov.au/def/party-identifier-type> ;
 skos:inScheme <http://linked.data.gov.au/def/party-identifier-type> ;
 skos:prefLabel "Birth certificate"@en ;
 skos:topConceptOf <http://linked.data.gov.au/def/party-identifier-type> .

id:centrelink-card a skos:Concept ;
 skos:definition "A card issued by the Australian social security agency Centrelink."@en ;
    rdfs:isDefinedBy <http://linked.data.gov.au/def/party-identifier-type> ;
 skos:inScheme <http://linked.data.gov.au/def/party-identifier-type> ;
 skos:prefLabel "Centrelink card"@en ;
 skos:topConceptOf <http://linked.data.gov.au/def/party-identifier-type> .

id:certificate-of-australian-citizenship a skos:Concept ;
 skos:definition "An Australian citizenship certificate is an official document issued by the Australian Government that shows that a person is an Australian."@en ;
    rdfs:isDefinedBy <http://linked.data.gov.au/def/party-identifier-type> ;
 skos:inScheme <http://linked.data.gov.au/def/party-identifier-type> ;
 skos:prefLabel "Certificate of Australian citizenship"@en ;
 skos:topConceptOf <http://linked.data.gov.au/def/party-identifier-type> .

id:council-rates-notice a skos:Concept ;
 skos:definition "A notice of council rates addressed to the owner of a property in Queensland."@en ;
    rdfs:isDefinedBy <http://linked.data.gov.au/def/party-identifier-type> ;
 skos:inScheme <http://linked.data.gov.au/def/party-identifier-type> ;
 skos:prefLabel "Council rates notice"@en ;
 skos:topConceptOf <http://linked.data.gov.au/def/party-identifier-type> .

id:electrol-roll-extract a skos:Concept ;
 skos:definition "An extract from the electoral roll administered by the Australian Electoral Commission. "@en ;
    rdfs:isDefinedBy <http://linked.data.gov.au/def/party-identifier-type> ;
 skos:inScheme <http://linked.data.gov.au/def/party-identifier-type> ;
 skos:prefLabel "Electrol roll extract"@en ;
 skos:topConceptOf <http://linked.data.gov.au/def/party-identifier-type> .

id:firearms-licence a skos:Concept ;
 skos:definition "A licence issued by the State of Queensland that allows ownership or use of a firearm."@en ;
    rdfs:isDefinedBy <http://linked.data.gov.au/def/party-identifier-type> ;
 skos:inScheme <http://linked.data.gov.au/def/party-identifier-type> ;
 skos:prefLabel "Firearms licence"@en ;
 skos:topConceptOf <http://linked.data.gov.au/def/party-identifier-type> .

id:foregin-passport a skos:Concept ;
 skos:definition "A foreign passport is a basic identity document accepted as valid for crossing international borders, issued by a government, other than Australia's, to its citizens. Source: The New Oxford Companion to Law"@en ;
    rdfs:isDefinedBy <http://linked.data.gov.au/def/party-identifier-type> ;
 skos:inScheme <http://linked.data.gov.au/def/party-identifier-type> ;
 skos:prefLabel "Foregin passport"@en ;
 skos:topConceptOf <http://linked.data.gov.au/def/party-identifier-type> .

id:letter-from-employer a skos:Concept ;
 skos:definition "A certified letter from the applicants employer."@en ;
    rdfs:isDefinedBy <http://linked.data.gov.au/def/party-identifier-type> ;
 skos:inScheme <http://linked.data.gov.au/def/party-identifier-type> ;
 skos:prefLabel "Letter from employer"@en ;
 skos:topConceptOf <http://linked.data.gov.au/def/party-identifier-type> .

id:public-service-photo-id a skos:Concept ;
 skos:altLabel "Government ID"@en ;
 skos:definition "An identification document or card issued by the Australian Government or one of the State or Territory government to a government employee."@en ;
    rdfs:isDefinedBy <http://linked.data.gov.au/def/party-identifier-type> ;
 skos:inScheme <http://linked.data.gov.au/def/party-identifier-type> ;
 skos:prefLabel "Public service photo ID"@en ;
 skos:topConceptOf <http://linked.data.gov.au/def/party-identifier-type> .

id:security-guard-licence a skos:Concept ;
 skos:altLabel "Security guard/crowd control licence"@en ;
 skos:definition "A licence issued by the State of Queensland that allows the bearer to perform duties pertaining to security and public safety."@en ;
    rdfs:isDefinedBy <http://linked.data.gov.au/def/party-identifier-type> ;
 skos:inScheme <http://linked.data.gov.au/def/party-identifier-type> ;
 skos:prefLabel "Security guard licence"@en ;
 skos:topConceptOf <http://linked.data.gov.au/def/party-identifier-type> .

id:veterans-affairs-card a skos:Concept ;
 skos:altLabel "Department of Veterans Affairs card"@en,
 "Veteran healthcare card"@en ;
 skos:definition "An identity card issued by the Australian Department of Veterans' Affairs that convey a range of benefits upon the bearer."@en ;
    rdfs:isDefinedBy <http://linked.data.gov.au/def/party-identifier-type> ;
 skos:inScheme <http://linked.data.gov.au/def/party-identifier-type> ;
 skos:prefLabel "Veterans affairs card"@en ;
 skos:topConceptOf <http://linked.data.gov.au/def/party-identifier-type> .

id:australian-passport a skos:Concept ;
 skos:definition "An Australian passport is a basic identity document accepted as valid for crossing international borders, issued by the Government of Australia to Australian citizens. Source: The New Oxford Companion to Law"@en ;
    rdfs:isDefinedBy <http://linked.data.gov.au/def/party-identifier-type> ;
 skos:inScheme <http://linked.data.gov.au/def/party-identifier-type> ;
 skos:prefLabel "Australian passport"@en ;
 skos:topConceptOf <http://linked.data.gov.au/def/party-identifier-type> .

id:change-of-name-certificate a skos:Concept ;
 skos:definition "A document issued by a a governing body registering a change of name."@en ;
    rdfs:isDefinedBy <http://linked.data.gov.au/def/party-identifier-type> ;
 skos:inScheme <http://linked.data.gov.au/def/party-identifier-type> ;
 skos:prefLabel "Change of name certificate"@en ;
 skos:topConceptOf <http://linked.data.gov.au/def/party-identifier-type> .

id:drivers-licence a skos:Concept ;
 skos:altLabel "Australian Drivers Licence"@en,
 "Australian Drivers License"@en,
 "Drivers License"@en ;
 skos:definition "The official permit required for a person to legally drive a motor vehicle in Australia. Issued by the States and Territories of Australia."@en ;
    rdfs:isDefinedBy <http://linked.data.gov.au/def/party-identifier-type> ;
 skos:inScheme <http://linked.data.gov.au/def/party-identifier-type> ;
 skos:prefLabel "Drivers licence"@en ;
 skos:topConceptOf <http://linked.data.gov.au/def/party-identifier-type> .

id:marriage-certificate a skos:Concept ;
 skos:definition "An official statement that two people are married. In most jurisdictions, a marriage certificate is issued by a government official only after the civil registration of the marriage. Source:Wikipedia"@en ;
    rdfs:isDefinedBy <http://linked.data.gov.au/def/party-identifier-type> ;
 skos:inScheme <http://linked.data.gov.au/def/party-identifier-type> ;
 skos:prefLabel "Marriage certificate"@en ;
 skos:topConceptOf <http://linked.data.gov.au/def/party-identifier-type> .

id:medicare-card a skos:Concept ;
 skos:definition "A card, issued to Australian citizens and permanent residents and their families. The card or the Medicare number enables the cardholder to receive a rebate of medical expenses under Australia's Medicare system, as well as subsidised medications under the Pharmaceutical Benefits Scheme (PBS). Source:Wikipedia"@en ;
    rdfs:isDefinedBy <http://linked.data.gov.au/def/party-identifier-type> ;
 skos:inScheme <http://linked.data.gov.au/def/party-identifier-type> ;
 skos:prefLabel "Medicare card"@en ;
 skos:topConceptOf <http://linked.data.gov.au/def/party-identifier-type> .
 
id:company-id a skos:Collection ;
 skos:definition "Identification numbers for businesses and companies within Australia."@en ;
 skos:member id:abn,
 id:acn,
 id:c-code ;
 skos:prefLabel "Company ID"@en .
 
id:mmol-list-a a skos:Collection ;
 skos:definition "Personal identification documents that act as primary proof-of-identity in the State of Queensland within MyMinesOnline. Identity checks must include at least one document from List A and one document from List B."@en ;
 skos:member id:australian-passport,
 id:drivers-licence,
 id:firearms-licence,
 id:foregin-passport,
 id:public-service-photo-id ;
 skos:prefLabel "MMOL list A"@en .

id:mmol-list-b a skos:Collection ;
 skos:definition "Personal identification documents that act as secondary proof-of-identity in the State of Queensland within MyMinesOnline. Identity checks must include at least one document from List A and one document from List B."@en ;
 skos:member id:australian-university-id-card,
 id:bank-card,
 id:centrelink-card,
 id:change-of-name-certificate,
 id:council-rates-notice,
 id:electrol-roll-extract,
 id:letter-from-employer,
 id:marriage-certificate,
 id:medicare-card,
 id:security-guard-licence,
 id:veterans-affairs-card ;
 skos:prefLabel "MMOL list B"@en .

id:personal-id a skos:Collection ;
 skos:definition "Australian or state-issued documents accepted as proof-of-identity for individuals by the Queensland Government."@en ;
 skos:member id:australian-passport,
 id:australian-university-id-card,
 id:australian-visa,
 id:bank-card,
 id:birth-certificate,
 id:centrelink-card,
 id:certificate-of-australian-citizenship,
 id:change-of-name-certificate,
 id:council-rates-notice,
 id:drivers-licence,
 id:electrol-roll-extract,
 id:firearms-licence,
 id:foregin-passport,
 id:letter-from-employer,
 id:marriage-certificate,
 id:medicare-card,
 id:public-service-photo-id,
 id:security-guard-licence,
 id:veterans-affairs-card ;
 skos:prefLabel "Personal ID"@en .

id:qgov-primary-documents a skos:Collection ;
 skos:definition "Personal identification documents that act as primary proof-of-identity in the State of Queensland within the QGOV identity brokerage system. Identity checks must make up 100 points and include at least one primary document."@en ;
 skos:member id:australian-passport,
 id:birth-certificate,
 id:drivers-licence ;
 skos:prefLabel "QGOV Primary Documents"@en .

id:qgov-secondary-documents a skos:Collection ;
 skos:definition "Personal identification documents that act as secondary proof-of-identity in the State of Queensland within the QGOV identity brokerage system. Identity checks must make up 100 points and include at least one primary document."@en ;
 skos:member id:australian-visa,
 id:certificate-of-australian-citizenship,
 id:change-of-name-certificate,
 id:marriage-certificate,
 id:medicare-card ;
 skos:prefLabel "QGOV Secondary Documents"@en .
