PREFIX : <https://linked.data.gov.au/def/object-condition/>
PREFIX agldwgstatus: <https://linked.data.gov.au/def/reg-statuses/>
PREFIX cs: <https://linked.data.gov.au/def/object-condition>
PREFIX dcterms: <http://purl.org/dc/terms/>
PREFIX reg: <http://purl.org/linked-data/registry#>
PREFIX rdfs: <http://www.w3.org/2000/01/rdf-schema#>
PREFIX sdo: <https://schema.org/>
PREFIX skos: <http://www.w3.org/2004/02/skos/core#>
PREFIX xsd: <http://www.w3.org/2001/XMLSchema#>

:pristine
    a skos:Concept ;
    rdfs:isDefinedBy cs: ;
    skos:definition "On a scale of 1-100 for condition, with 100 being the best, this object scores 100 points."@en ;
    skos:historyNote "Created from the WIMS MIRO brainstorming session" ;
    skos:inScheme cs: ;
    skos:notation "pristine" ;
    skos:prefLabel "Pristine"@en ;
    skos:topConceptOf cs: ;
.

:scuffed
    a skos:Concept ;
    rdfs:isDefinedBy cs: ;
    skos:definition "On a scale of 1-100 for condition, with 100 being the best, this object scores 90 points."@en ;
    skos:historyNote "Created from the WIMS MIRO brainstorming session" ;
    skos:inScheme cs: ;
    skos:notation "scuffed" ;
    skos:prefLabel "Scuffed"@en ;
    skos:topConceptOf cs: ;
.

:durable
    a skos:Concept ;
    rdfs:isDefinedBy cs: ;
    skos:definition "On a scale of 1-100 for condition, with 100 being the best, this object scores 80 points."@en ;
    skos:historyNote "Created from the WIMS MIRO brainstorming session" ;
    skos:inScheme cs: ;
    skos:notation "durable" ;
    skos:prefLabel "Durable"@en ;
    skos:topConceptOf cs: ;
.

:tested
    a skos:Concept ;
    rdfs:isDefinedBy cs: ;
    skos:definition "On a scale of 1-100 for condition, with 100 being the best, this object scores 70 points."@en ;
    skos:historyNote "Created from the WIMS MIRO brainstorming session" ;
    skos:inScheme cs: ;
    skos:notation "tested" ;
    skos:prefLabel "Tested"@en ;
    skos:topConceptOf cs: ;
.

:battered
    a skos:Concept ;
    rdfs:isDefinedBy cs: ;
    skos:definition "On a scale of 1-100 for condition, with 100 being the best, this object scores 60 points."@en ;
    skos:historyNote "Created from the WIMS MIRO brainstorming session" ;
    skos:inScheme cs: ;
    skos:notation "battered" ;
    skos:prefLabel "Battered"@en ;
    skos:topConceptOf cs: ;
.

:worn
    a skos:Concept ;
    rdfs:isDefinedBy cs: ;
    skos:definition "On a scale of 1-100 for condition, with 100 being the best, this object scores 50 points."@en ;
    skos:historyNote "Created from the WIMS MIRO brainstorming session" ;
    skos:inScheme cs: ;
    skos:notation "worn" ;
    skos:prefLabel "Worn"@en ;
    skos:topConceptOf cs: ;
.

:damaged
    a skos:Concept ;
    rdfs:isDefinedBy cs: ;
    skos:definition "On a scale of 1-100 for condition, with 100 being the best, this object scores 40 points."@en ;
    skos:historyNote "Created from the WIMS MIRO brainstorming session" ;
    skos:inScheme cs: ;
    skos:notation "damaged" ;
    skos:prefLabel "Damaged"@en ;
    skos:topConceptOf cs: ;
.

:weakened
    a skos:Concept ;
    rdfs:isDefinedBy cs: ;
    skos:definition "On a scale of 1-100 for condition, with 100 being the best, this object scores 30 points."@en ;
    skos:historyNote "Created from the WIMS MIRO brainstorming session" ;
    skos:inScheme cs: ;
    skos:notation "weakened" ;
    skos:prefLabel "Weakened"@en ;
    skos:topConceptOf cs: ;
.

:fragile
    a skos:Concept ;
    rdfs:isDefinedBy cs: ;
    skos:definition "On a scale of 1-100 for condition, with 100 being the best, this object scores 20 points."@en ;
    skos:historyNote "Created from the WIMS MIRO brainstorming session" ;
    skos:inScheme cs: ;
    skos:notation "fragile" ;
    skos:prefLabel "Fragile"@en ;
    skos:topConceptOf cs: ;
.

:compromised
    a skos:Concept ;
    rdfs:isDefinedBy cs: ;
    skos:definition "On a scale of 1-100 for condition, with 100 being the best, this object scores 10 points."@en ;
    skos:historyNote "Created from the WIMS MIRO brainstorming session" ;
    skos:inScheme cs: ;
    skos:notation "compromised" ;
    skos:prefLabel "Compromised"@en ;
    skos:topConceptOf cs: ;
.

:unusable
    a skos:Concept ;
    rdfs:isDefinedBy cs: ;
    skos:definition "On a scale of 1-100 for condition, with 100 being the best, this object scores 0 points."@en ;
    skos:historyNote "Created from the WIMS MIRO brainstorming session" ;
    skos:inScheme cs: ;
    skos:notation "unusable" ;
    skos:prefLabel "Unusable"@en ;
    skos:topConceptOf cs: ;
.

<https://linked.data.gov.au/org/gsq>
    a sdo:Organization ;
    sdo:name "Geological Survey of Queensland" ;
    sdo:url "https://www.business.qld.gov.au/industries/mining-energy-water/resources/geoscience-information/gsq"^^xsd:anyURI ;
.

cs:
    a skos:ConceptScheme ;
    sdo:keywords <http://linked.data.gov.au/def/earth-science-data-category/geology-not-elsewhere-classified> ;
    reg:status agldwgstatus:experimental ;
    skos:definition "Object Condition"@en ;
    skos:hasTopConcept
        :pristine ,
        :scuffed ,
        :durable ,
        :tested ,
        :battered ,
        :worn ,
        :damaged ,
        :weakened ,
        :fragile ,
        :compromised ,
        :unusable ;
    skos:historyNote "Created from the WIMS MIRO brainstorming session" ;
    skos:notation "Object Condition" ;
    skos:prefLabel "Object Condition"@en ;
    sdo:copyrightNotice "(c) Geological Survey of Queensland, 2024" ;
    sdo:creator <https://linked.data.gov.au/org/gsq> ;
    dcterms:created "2024-08-06"^^xsd:date ;
    dcterms:modified "2024-08-06"^^xsd:date ;
    sdo:license <https://purl.org/NET/rdflicense/cc-by4.0> ;
    sdo:publisher <https://linked.data.gov.au/org/gsq> ;
.

