PREFIX dcterms: <http://purl.org/dc/terms/>
PREFIX owl: <http://www.w3.org/2002/07/owl#>
PREFIX rdfs: <http://www.w3.org/2000/01/rdf-schema#>
PREFIX rslt: <https://linked.data.gov.au/def/result-type/>
PREFIX sdo: <https://schema.org/>
PREFIX skos: <http://www.w3.org/2004/02/skos/core#>
PREFIX xsd: <http://www.w3.org/2001/XMLSchema#>

rslt:azimuth
    a skos:Concept ;
    dcterms:provenance "Compiled by the Geological Survey of Queensland" ;
    rdfs:isDefinedBy <https://linked.data.gov.au/def/result-type> ;
    skos:broader rslt:angle ;
    skos:definition "An angle in the horizontal plane relative to North. By default azimuth is relative to True North, but may also be qualified as relative to Magnetic North or Grid North"@en ;
    skos:inScheme <https://linked.data.gov.au/def/result-type> ;
    skos:notation "razi" ;
    skos:prefLabel "Azimuth"@en ;
.

rslt:dip
    a skos:Concept ;
    dcterms:provenance "Compiled by the Geological Survey of Queensland" ;
    rdfs:isDefinedBy <https://linked.data.gov.au/def/result-type> ;
    skos:broader rslt:angle ;
    skos:definition "An angle in the vertrical plane relative to a horizontal reference. 90 degrees is vertical downwards, 0 degrees horizontal, -90 degrees is vertical upwards."@en ;
    skos:inScheme <https://linked.data.gov.au/def/result-type> ;
    skos:notation "rdip" ;
    skos:prefLabel "Dip"@en ;
.

rslt:inclination
    a skos:Concept ;
    dcterms:provenance "Compiled by the Geological Survey of Queensland" ;
    rdfs:isDefinedBy <https://linked.data.gov.au/def/result-type> ;
    skos:broader rslt:angle ;
    skos:definition "An angle in the vertrical plane relative to a reference vector parallel to the force of gravity, i.e. downwards. 0 degrees is vertical downwards, 90 degrees horizontal, 180 degrees is vertical upwards."@en ;
    skos:inScheme <https://linked.data.gov.au/def/result-type> ;
    skos:notation "rinc" ;
    skos:prefLabel "Inclination"@en ;
.

rslt:age
    a skos:Concept ;
    dcterms:provenance "Compiled by the Geological Survey of Queensland" ;
    rdfs:isDefinedBy <https://linked.data.gov.au/def/result-type> ;
    skos:definition "The time before a reference time. Commonly referenced to time before present (BP), before current era (BCE), or represented as Millions of Years Ago (Ma) in geological disciplines"@en ;
    skos:inScheme <https://linked.data.gov.au/def/result-type> ;
    skos:notation "rage" ;
    skos:prefLabel "Age"@en ;
    skos:topConceptOf <https://linked.data.gov.au/def/result-type> ;
.

rslt:api-gravity
    a skos:Concept ;
    dcterms:provenance "Compiled by the Geological Survey of Queensland" ;
    rdfs:isDefinedBy <https://linked.data.gov.au/def/result-type> ;
    skos:altLabel "Oil Gravity"@en ;
    skos:definition "A measure of how heavy or light a petroleum liquid is compared to water: if its API gravity is greater than 10, it is lighter and floats on water; if less than 10, it is heavier and sinks."@en ;
    skos:inScheme <https://linked.data.gov.au/def/result-type> ;
    skos:notation "rapi" ;
    skos:prefLabel "API Gravity"@en ;
    skos:topConceptOf <https://linked.data.gov.au/def/result-type> ;
.

rslt:area
    a skos:Concept ;
    dcterms:provenance "Compiled by the Geological Survey of Queensland" ;
    rdfs:isDefinedBy <https://linked.data.gov.au/def/result-type> ;
    skos:definition "The quantity that expresses the extent of a two-dimensional figure or shape or planar lamina, in the plane. Surface area is its analog on the two-dimensional surface of a three-dimensional object."@en ;
    skos:inScheme <https://linked.data.gov.au/def/result-type> ;
    skos:notation "rara" ;
    skos:prefLabel "Area"@en ;
    skos:topConceptOf <https://linked.data.gov.au/def/result-type> ;
.

rslt:capacitance
    a skos:Concept ;
    dcterms:provenance "Compiled by the Geological Survey of Queensland" ;
    rdfs:isDefinedBy <https://linked.data.gov.au/def/result-type> ;
    skos:altLabel "Chargeability"@en ;
    skos:definition "The ratio of the change in electric charge of a system, to the corresponding change in its electric potential."@en ;
    skos:inScheme <https://linked.data.gov.au/def/result-type> ;
    skos:notation "rcap" ;
    skos:prefLabel "Capacitance"@en ;
    skos:topConceptOf <https://linked.data.gov.au/def/result-type> ;
.

rslt:casing-weight
    a skos:Concept ;
    dcterms:provenance "Compiled by the Geological Survey of Queensland" ;
    rdfs:isDefinedBy <https://linked.data.gov.au/def/result-type> ;
    skos:definition "The mass per unit of length of a length of tubular installed in a borehole."@en ;
    skos:inScheme <https://linked.data.gov.au/def/result-type> ;
    skos:notation "rcsw" ;
    skos:prefLabel "Casing Weight"@en ;
    skos:topConceptOf <https://linked.data.gov.au/def/result-type> ;
.

rslt:colour
    a skos:Concept ;
    dcterms:provenance "Compiled by the Geological Survey of Queensland" ;
    rdfs:isDefinedBy <https://linked.data.gov.au/def/result-type> ;
    skos:definition "The qualitative description of the colour of an object."@en ;
    skos:inScheme <https://linked.data.gov.au/def/result-type> ;
    skos:notation "rcol" ;
    skos:prefLabel "Colour"@en ;
    skos:topConceptOf <https://linked.data.gov.au/def/result-type> ;
.

rslt:composition
    a skos:Concept ;
    dcterms:provenance "Compiled by the Geological Survey of Queensland" ;
    rdfs:isDefinedBy <https://linked.data.gov.au/def/result-type> ;
    skos:definition "A description of the component parts of a sample or object. Typically given as a component with its percentage or ratio within a bulk sample."@en ;
    skos:inScheme <https://linked.data.gov.au/def/result-type> ;
    skos:notation "rcmp" ;
    skos:prefLabel "Composition"@en ;
    skos:topConceptOf <https://linked.data.gov.au/def/result-type> ;
.

rslt:compressibility
    a skos:Concept ;
    dcterms:provenance "Compiled by the Geological Survey of Queensland" ;
    rdfs:isDefinedBy <https://linked.data.gov.au/def/result-type> ;
    skos:definition "A measure of the relative volume change of a fluid or solid as a response to a pressure (or mean stress) change."@en ;
    skos:inScheme <https://linked.data.gov.au/def/result-type> ;
    skos:notation "rcpb" ;
    skos:prefLabel "Compressibility"@en ;
    skos:topConceptOf <https://linked.data.gov.au/def/result-type> ;
.

rslt:compressive-strength
    a skos:Concept ;
    dcterms:provenance "Compiled by the Geological Survey of Queensland" ;
    rdfs:isDefinedBy <https://linked.data.gov.au/def/result-type> ;
    skos:definition "The capacity to withstand axially directed pushing forces"@en ;
    skos:inScheme <https://linked.data.gov.au/def/result-type> ;
    skos:notation "rcps" ;
    skos:prefLabel "Compressive Strength"@en ;
    skos:topConceptOf <https://linked.data.gov.au/def/result-type> ;
.

rslt:concentration
    a skos:Concept ;
    dcterms:provenance "Compiled by the Geological Survey of Queensland" ;
    rdfs:isDefinedBy <https://linked.data.gov.au/def/result-type> ;
    skos:definition "The abundance of a constituent divided by the total volume of a mixture."@en ;
    skos:inScheme <https://linked.data.gov.au/def/result-type> ;
    skos:notation "rctn" ;
    skos:prefLabel "Concentration"@en ;
    skos:topConceptOf <https://linked.data.gov.au/def/result-type> ;
.

rslt:cost
    a skos:Concept ;
    dcterms:provenance "Compiled by the Geological Survey of Queensland" ;
    rdfs:isDefinedBy <https://linked.data.gov.au/def/result-type> ;
    skos:definition "The monetary value, cost, or price (in a unit of currency) for goods, services, or items."@en ;
    skos:inScheme <https://linked.data.gov.au/def/result-type> ;
    skos:notation "rcst" ;
    skos:prefLabel "Cost"@en ;
    skos:topConceptOf <https://linked.data.gov.au/def/result-type> ;
.

rslt:count
    a skos:Concept ;
    dcterms:provenance "Compiled by the Geological Survey of Queensland" ;
    rdfs:isDefinedBy <https://linked.data.gov.au/def/result-type> ;
    skos:definition "A quanitifation of the absolute number of discrete objects, groups, or sets."@en ;
    skos:inScheme <https://linked.data.gov.au/def/result-type> ;
    skos:notation "rcnt" ;
    skos:prefLabel "Count"@en ;
    skos:topConceptOf <https://linked.data.gov.au/def/result-type> ;
.

rslt:curvature
    a skos:Concept ;
    dcterms:provenance "Compiled by the Geological Survey of Queensland" ;
    rdfs:isDefinedBy <https://linked.data.gov.au/def/result-type> ;
    skos:altLabel "Dog Leg Severity"@en ;
    skos:definition "The curvature of a line or length of material. The change in angle per unit of length. Used in oil and gas to describe the curvature of a wellbore."@en ;
    skos:inScheme <https://linked.data.gov.au/def/result-type> ;
    skos:notation "rdls" ;
    skos:prefLabel "Curvature"@en ;
    skos:topConceptOf <https://linked.data.gov.au/def/result-type> ;
.

rslt:data
    a skos:Concept ;
    dcterms:provenance "Compiled by the Geological Survey of Queensland" ;
    rdfs:isDefinedBy <https://linked.data.gov.au/def/result-type> ;
    skos:definition "The amount of data or information held by an electronic and measurable means. Typically reported in bytes or a derivative unit."@en ;
    skos:inScheme <https://linked.data.gov.au/def/result-type> ;
    skos:notation "rdat" ;
    skos:prefLabel "Data"@en ;
    skos:topConceptOf <https://linked.data.gov.au/def/result-type> ;
.

rslt:density
    a skos:Concept ;
    dcterms:provenance "Compiled by the Geological Survey of Queensland" ;
    rdfs:isDefinedBy <https://linked.data.gov.au/def/result-type> ;
    skos:definition "The density (more precisely, the volumetric mass density; also known as specific mass), of a substance is its mass per unit volume."@en ;
    skos:inScheme <https://linked.data.gov.au/def/result-type> ;
    skos:notation "rden" ;
    skos:prefLabel "Density"@en ;
    skos:topConceptOf <https://linked.data.gov.au/def/result-type> ;
.

rslt:descriptive
    a skos:Concept ;
    dcterms:provenance "Compiled by the Geological Survey of Queensland" ;
    rdfs:isDefinedBy <https://linked.data.gov.au/def/result-type> ;
    skos:definition "A decription of a subject or object of interest."@en ;
    skos:inScheme <https://linked.data.gov.au/def/result-type> ;
    skos:notation "rdsc" ;
    skos:prefLabel "Descriptive"@en ;
    skos:topConceptOf <https://linked.data.gov.au/def/result-type> ;
.

rslt:distance
    a skos:Concept ;
    dcterms:provenance "Compiled by the Geological Survey of Queensland" ;
    rdfs:isDefinedBy <https://linked.data.gov.au/def/result-type> ;
    skos:definition "The length of travel along a path that may be non-linear."@en ;
    skos:inScheme <https://linked.data.gov.au/def/result-type> ;
    skos:notation "rdis" ;
    skos:prefLabel "Distance"@en ;
    skos:topConceptOf <https://linked.data.gov.au/def/result-type> ;
.

rslt:drill-rate
    a skos:Concept ;
    dcterms:provenance "Compiled by the Geological Survey of Queensland" ;
    rdfs:isDefinedBy <https://linked.data.gov.au/def/result-type> ;
    skos:altLabel "Rate of Penetration"@en ;
    skos:definition "The rate that a drillbit penetrates the subsurface substrate and creates wellbore length."@en ;
    skos:inScheme <https://linked.data.gov.au/def/result-type> ;
    skos:notation "rdlr" ;
    skos:prefLabel "Drill Rate"@en ;
    skos:topConceptOf <https://linked.data.gov.au/def/result-type> ;
.

rslt:electric-charge
    a skos:Concept ;
    dcterms:provenance "Compiled by the Geological Survey of Queensland" ;
    rdfs:isDefinedBy <https://linked.data.gov.au/def/result-type> ;
    skos:altLabel "Electrical Charge"@en ;
    skos:definition "The physical property of matter that causes it to experience a force when placed in an electromagnetic field. There are two types of electric charge: positive and negative (commonly carried by protons and electrons respectively)."@en ;
    skos:inScheme <https://linked.data.gov.au/def/result-type> ;
    skos:notation "relc" ;
    skos:prefLabel "Electric Charge"@en ;
    skos:topConceptOf <https://linked.data.gov.au/def/result-type> ;
.

rslt:electric-current
    a skos:Concept ;
    dcterms:provenance "Compiled by the Geological Survey of Queensland" ;
    rdfs:isDefinedBy <https://linked.data.gov.au/def/result-type> ;
    skos:altLabel "Electrical Current"@en ;
    skos:definition "The rate of flow of electric charge past a point or region."@en ;
    skos:inScheme <https://linked.data.gov.au/def/result-type> ;
    skos:notation "relr" ;
    skos:prefLabel "Electric Current"@en ;
    skos:topConceptOf <https://linked.data.gov.au/def/result-type> ;
.

rslt:electrical-conductivity
    a skos:Concept ;
    dcterms:provenance "Compiled by the Geological Survey of Queensland" ;
    rdfs:isDefinedBy <https://linked.data.gov.au/def/result-type> ;
    skos:altLabel "Electrical Conductance"@en ;
    skos:definition "A measure of a material's ability to conduct an electric current."@en ;
    skos:inScheme <https://linked.data.gov.au/def/result-type> ;
    skos:notation "recd" ;
    skos:prefLabel "Conductivity"@en ;
    skos:topConceptOf <https://linked.data.gov.au/def/result-type> ;
.

rslt:elevation
    a skos:Concept ;
    dcterms:provenance "Compiled by the Geological Survey of Queensland" ;
    rdfs:isDefinedBy <https://linked.data.gov.au/def/result-type> ;
    skos:altLabel
        "Height" ,
        "Altitude"@en ;
    skos:definition "The distance vertically upward from a reference point, surface, or datum."@en ;
    skos:inScheme <https://linked.data.gov.au/def/result-type> ;
    skos:notation "relv" ;
    skos:prefLabel "Elevation"@en ;
    skos:topConceptOf <https://linked.data.gov.au/def/result-type> ;
.

rslt:energy
    a skos:Concept ;
    dcterms:provenance "Compiled by the Geological Survey of Queensland" ;
    rdfs:isDefinedBy <https://linked.data.gov.au/def/result-type> ;
    skos:definition "The quantitative property that must be transferred to an object in order to perform work on, or to heat, the object."@en ;
    skos:inScheme <https://linked.data.gov.au/def/result-type> ;
    skos:notation "reng" ;
    skos:prefLabel "Energy"@en ;
    skos:topConceptOf <https://linked.data.gov.au/def/result-type> ;
.

rslt:energy-density
    a skos:Concept ;
    dcterms:provenance "Compiled by the Geological Survey of Queensland" ;
    rdfs:isDefinedBy <https://linked.data.gov.au/def/result-type> ;
    skos:altLabel
        "Gas Quality"@en ,
        "Heat Content"@en ;
    skos:definition "The amount of energy stored in a given system or region of space per unit volume e.g. PJ/Mm3."@en ;
    skos:inScheme <https://linked.data.gov.au/def/result-type> ;
    skos:notation "rend" ;
    skos:prefLabel "Energy Density"@en ;
    skos:topConceptOf <https://linked.data.gov.au/def/result-type> ;
.

rslt:flow-rate
    a skos:Concept ;
    dcterms:provenance "Compiled by the Geological Survey of Queensland" ;
    rdfs:isDefinedBy <https://linked.data.gov.au/def/result-type> ;
    skos:altLabel "Volumetric Flow Rate"@en ;
    skos:definition "The volume of fluid which passes a point or region per unit time."@en ;
    skos:inScheme <https://linked.data.gov.au/def/result-type> ;
    skos:notation "rflr" ;
    skos:prefLabel "Flow Rate"@en ;
    skos:topConceptOf <https://linked.data.gov.au/def/result-type> ;
.

rslt:fluid-density
    a skos:Concept ;
    dcterms:provenance "Compiled by the Geological Survey of Queensland" ;
    rdfs:isDefinedBy <https://linked.data.gov.au/def/result-type> ;
    skos:altLabel "Mud Weight"@en ;
    skos:definition "The mass per unit volume of a fluid. Commonly used as a quantity for drilling fluids and cement in relation to boreholes."@en ;
    skos:inScheme <https://linked.data.gov.au/def/result-type> ;
    skos:notation "rfld" ;
    skos:prefLabel "Fluid Density"@en ;
    skos:topConceptOf <https://linked.data.gov.au/def/result-type> ;
.

rslt:force
    a skos:Concept ;
    dcterms:provenance "Compiled by the Geological Survey of Queensland" ;
    rdfs:isDefinedBy <https://linked.data.gov.au/def/result-type> ;
    skos:definition "Any interaction that, when unopposed, will change the motion of an object."@en ;
    skos:inScheme <https://linked.data.gov.au/def/result-type> ;
    skos:notation "rfrc" ;
    skos:prefLabel "Force"@en ;
    skos:topConceptOf <https://linked.data.gov.au/def/result-type> ;
.

rslt:frequency
    a skos:Concept ;
    dcterms:provenance "Compiled by the Geological Survey of Queensland" ;
    rdfs:isDefinedBy <https://linked.data.gov.au/def/result-type> ;
    skos:definition "The number of occurrences of a repeating event per unit of time."@en ;
    skos:inScheme <https://linked.data.gov.au/def/result-type> ;
    skos:notation "rfrq" ;
    skos:prefLabel "Frequency"@en ;
    skos:topConceptOf <https://linked.data.gov.au/def/result-type> ;
.

rslt:gas-content
    a skos:Concept ;
    dcterms:provenance "Compiled by the Geological Survey of Queensland" ;
    rdfs:isDefinedBy <https://linked.data.gov.au/def/result-type> ;
    skos:definition "The amount of gas, typically hydrocarbon, contained or within solid or liquid. Commonly used to describe to the amount of gas adsorbed to a mass of coal."@en ;
    skos:inScheme <https://linked.data.gov.au/def/result-type> ;
    skos:notation "rgsc" ;
    skos:prefLabel "Gas Content"@en ;
    skos:topConceptOf <https://linked.data.gov.au/def/result-type> ;
.

rslt:grain-shape
    a skos:Concept ;
    dcterms:provenance "Compiled by the Geological Survey of Queensland" ;
    rdfs:isDefinedBy <https://linked.data.gov.au/def/result-type> ;
    skos:altLabel "Roundness"@en ;
    skos:definition "The degree of smoothing due to abrasion of sedimentary particles i.e. well-rounded, rounded, sub-rounded, sub-angular, angular, very angular."@en ;
    skos:inScheme <https://linked.data.gov.au/def/result-type> ;
    skos:notation "rgrs" ;
    skos:prefLabel "Grain Shape"@en ;
    skos:topConceptOf <https://linked.data.gov.au/def/result-type> ;
.

rslt:grain-size
    a skos:Concept ;
    dcterms:provenance "Compiled by the Geological Survey of Queensland" ;
    rdfs:isDefinedBy <https://linked.data.gov.au/def/result-type> ;
    skos:definition "The diameter of individual grains of sediment, or the lithified particles in clastic rocks. The term may also be applied to other granular materials."@en ;
    skos:inScheme <https://linked.data.gov.au/def/result-type> ;
    skos:notation "rgrz" ;
    skos:prefLabel "Grain Size"@en ;
    skos:topConceptOf <https://linked.data.gov.au/def/result-type> ;
.

rslt:heat
    a skos:Concept ;
    dcterms:provenance "Compiled by the Geological Survey of Queensland" ;
    rdfs:isDefinedBy <https://linked.data.gov.au/def/result-type> ;
    skos:definition "Energy in transfer to or from a thermodynamic system, by mechanisms other than thermodynamic work or transfer of matter."@en ;
    skos:inScheme <https://linked.data.gov.au/def/result-type> ;
    skos:notation "rhet" ;
    skos:prefLabel "Heat"@en ;
    skos:topConceptOf <https://linked.data.gov.au/def/result-type> ;
.

rslt:illuminance
    a skos:Concept ;
    dcterms:provenance "Compiled by the Geological Survey of Queensland" ;
    rdfs:isDefinedBy <https://linked.data.gov.au/def/result-type> ;
    skos:definition "The total luminous flux incident on a surface, per unit area."@en ;
    skos:inScheme <https://linked.data.gov.au/def/result-type> ;
    skos:notation "rill" ;
    skos:prefLabel "Illuminance"@en ;
    skos:topConceptOf <https://linked.data.gov.au/def/result-type> ;
.

rslt:inductance
    a skos:Concept ;
    dcterms:provenance "Compiled by the Geological Survey of Queensland" ;
    rdfs:isDefinedBy <https://linked.data.gov.au/def/result-type> ;
    skos:definition "The tendency of an electrical conductor to oppose a change in the electric current flowing through it."@en ;
    skos:inScheme <https://linked.data.gov.au/def/result-type> ;
    skos:notation "rind" ;
    skos:prefLabel "Inductance"@en ;
    skos:topConceptOf <https://linked.data.gov.au/def/result-type> ;
.

rslt:length
    a skos:Concept ;
    dcterms:provenance "Compiled by the Geological Survey of Queensland" ;
    rdfs:isDefinedBy <https://linked.data.gov.au/def/result-type> ;
    skos:definition "A measure of distance in one dimension."@en ;
    skos:inScheme <https://linked.data.gov.au/def/result-type> ;
    skos:notation "rlen" ;
    skos:prefLabel "Length"@en ;
    skos:topConceptOf <https://linked.data.gov.au/def/result-type> ;
.

rslt:luminous-flux
    a skos:Concept ;
    dcterms:provenance "Compiled by the Geological Survey of Queensland" ;
    rdfs:isDefinedBy <https://linked.data.gov.au/def/result-type> ;
    skos:definition "The measure of the perceived power of light. It differs from radiant flux, the measure of the total power of electromagnetic radiation (including infrared, ultraviolet, and visible light), in that luminous flux is adjusted to reflect the varying sensitivity of the human eye to different wavelengths of light."@en ;
    skos:inScheme <https://linked.data.gov.au/def/result-type> ;
    skos:notation "rlfx" ;
    skos:prefLabel "Luminous Flux"@en ;
    skos:topConceptOf <https://linked.data.gov.au/def/result-type> ;
.

rslt:luminous-intensity
    a skos:Concept ;
    dcterms:provenance "Compiled by the Geological Survey of Queensland" ;
    rdfs:isDefinedBy <https://linked.data.gov.au/def/result-type> ;
    skos:definition "A measure of the wavelength-weighted power emitted by a light source in a particular direction per unit solid angle, based on the luminosity function, a standardized model of the sensitivity of the human eye."@en ;
    skos:inScheme <https://linked.data.gov.au/def/result-type> ;
    skos:notation "rlin" ;
    skos:prefLabel "Luminous Intensity"@en ;
    skos:topConceptOf <https://linked.data.gov.au/def/result-type> ;
.

rslt:magnetic-flux
    a skos:Concept ;
    dcterms:provenance "Compiled by the Geological Survey of Queensland" ;
    rdfs:isDefinedBy <https://linked.data.gov.au/def/result-type> ;
    skos:definition "The surface integral of the normal component of the magnetic field flux density B passing through that surface."@en ;
    skos:inScheme <https://linked.data.gov.au/def/result-type> ;
    skos:notation "rmfx" ;
    skos:prefLabel "Magnetic Flux"@en ;
    skos:topConceptOf <https://linked.data.gov.au/def/result-type> ;
.

rslt:magnetic-flux-density
    a skos:Concept ;
    dcterms:provenance "Compiled by the Geological Survey of Queensland" ;
    rdfs:isDefinedBy <https://linked.data.gov.au/def/result-type> ;
    skos:altLabel
        "B-Field"@en ,
        "Magnetic Field"@en ,
        "Magnetic Induction"@en ;
    skos:definition "The force a magnetic field exerts on a moving charged particle."@en ;
    skos:inScheme <https://linked.data.gov.au/def/result-type> ;
    skos:notation "rmfd" ;
    skos:prefLabel "Magnetic Flux Density"@en ;
    skos:topConceptOf <https://linked.data.gov.au/def/result-type> ;
.

rslt:magnetic-susceptibility
    a skos:Concept ;
    dcterms:provenance "Compiled by the Geological Survey of Queensland" ;
    rdfs:isDefinedBy <https://linked.data.gov.au/def/result-type> ;
    skos:definition "A measure of how much a material will become magnetized in an applied magnetic field. Mathematically, it is the ratio of magnetization M (magnetic moment per unit volume) to the applied magnetizing field intensity H."@en ;
    skos:inScheme <https://linked.data.gov.au/def/result-type> ;
    skos:notation "rmsc" ;
    skos:prefLabel "Magnetic Susceptibility"@en ;
    skos:topConceptOf <https://linked.data.gov.au/def/result-type> ;
.

rslt:mass
    a skos:Concept ;
    dcterms:provenance "Compiled by the Geological Survey of Queensland" ;
    rdfs:isDefinedBy <https://linked.data.gov.au/def/result-type> ;
    skos:definition "A property of a physical body and a measure of its resistance to acceleration (a change in its state of motion) when a net force is applied."@en ;
    skos:inScheme <https://linked.data.gov.au/def/result-type> ;
    skos:notation "rmss" ;
    skos:prefLabel "Mass"@en ;
    skos:topConceptOf <https://linked.data.gov.au/def/result-type> ;
.

rslt:measured-depth
    a skos:Concept ;
    dcterms:provenance "Compiled by the Geological Survey of Queensland" ;
    rdfs:isDefinedBy <https://linked.data.gov.au/def/result-type> ;
    skos:altLabel "MD" ;
    skos:definition "The depth below a reference point or reference datum along a defined path. Commonly used along the path of a wellbore."@en ;
    skos:inScheme <https://linked.data.gov.au/def/result-type> ;
    skos:notation "rmmd" ;
    skos:prefLabel "Measured Depth"@en ;
    skos:topConceptOf <https://linked.data.gov.au/def/result-type> ;
.

rslt:oil-quality
    a skos:Concept ;
    dcterms:provenance "Compiled by the Geological Survey of Queensland" ;
    rdfs:isDefinedBy <https://linked.data.gov.au/def/result-type> ;
    skos:definition "Value for the thermal quality of oil reported. This is often recorded in British Thermal Units (BTUs) and can be used to calculate the Barrel of Oil Equivalent (BOE)."@en ;
    skos:inScheme <https://linked.data.gov.au/def/result-type> ;
    skos:notation "rolq" ;
    skos:prefLabel "Oil Quality"@en ;
    skos:topConceptOf <https://linked.data.gov.au/def/result-type> ;
.

rslt:permeability
    a skos:Concept ;
    dcterms:provenance "Compiled by the Geological Survey of Queensland" ;
    rdfs:isDefinedBy <https://linked.data.gov.au/def/result-type> ;
    skos:definition "A measure of the ability of a material (such as rocks) to transmit fluids."@en ;
    skos:inScheme <https://linked.data.gov.au/def/result-type> ;
    skos:notation "rprm" ;
    skos:prefLabel "Permeability"@en ;
    skos:topConceptOf <https://linked.data.gov.au/def/result-type> ;
.

rslt:porosity
    a skos:Concept ;
    dcterms:provenance "Compiled by the Geological Survey of Queensland" ;
    rdfs:isDefinedBy <https://linked.data.gov.au/def/result-type> ;
    skos:definition "A measure of the void (i.e. 'empty') spaces in a material, and is a fraction of the volume of voids over the total volume, between 0 and 1, or as a percentage between 0% and 100%."@en ;
    skos:inScheme <https://linked.data.gov.au/def/result-type> ;
    skos:notation "rpor" ;
    skos:prefLabel "Porosity"@en ;
    skos:topConceptOf <https://linked.data.gov.au/def/result-type> ;
.

rslt:power
    a skos:Concept ;
    dcterms:provenance "Compiled by the Geological Survey of Queensland" ;
    rdfs:isDefinedBy <https://linked.data.gov.au/def/result-type> ;
    skos:definition "The rate of doing work or of transferring heat, i.e. the amount of energy transferred or converted per unit time."@en ;
    skos:inScheme <https://linked.data.gov.au/def/result-type> ;
    skos:notation "rpow" ;
    skos:prefLabel "Power"@en ;
    skos:topConceptOf <https://linked.data.gov.au/def/result-type> ;
.

rslt:pressure
    a skos:Concept ;
    dcterms:provenance "Compiled by the Geological Survey of Queensland" ;
    rdfs:isDefinedBy <https://linked.data.gov.au/def/result-type> ;
    skos:definition "The force applied perpendicular to the surface of an object per unit area over which that force is distributed."@en ;
    skos:inScheme <https://linked.data.gov.au/def/result-type> ;
    skos:notation "rprs" ;
    skos:prefLabel "Pressure"@en ;
    skos:topConceptOf <https://linked.data.gov.au/def/result-type> ;
.

rslt:radioactivity
    a skos:Concept ;
    dcterms:provenance "Compiled by the Geological Survey of Queensland" ;
    rdfs:isDefinedBy <https://linked.data.gov.au/def/result-type> ;
    skos:altLabel
        "nuclear decay"@en ,
        "nuclear disintegration"@en ,
        "radioactive decay"@en ,
        "radioactive disintegration"@en ;
    skos:definition "The process by which an unstable atomic nucleus loses energy by radiation. A material containing unstable nuclei is considered radioactive."@en ;
    skos:inScheme <https://linked.data.gov.au/def/result-type> ;
    skos:notation "rrad" ;
    skos:prefLabel "Radioactivity"@en ;
    skos:topConceptOf <https://linked.data.gov.au/def/result-type> ;
.

rslt:recovery
    a skos:Concept ;
    dcterms:provenance "Compiled by the Geological Survey of Queensland" ;
    rdfs:isDefinedBy <https://linked.data.gov.au/def/result-type> ;
    skos:definition "The amount of a target material recovered from an input mixture relative to the total amount of the target material initially present in the input. Expressed as a percentage."@en ;
    skos:inScheme <https://linked.data.gov.au/def/result-type> ;
    skos:notation "rrec" ;
    skos:prefLabel "Recovery"@en ;
    skos:topConceptOf <https://linked.data.gov.au/def/result-type> ;
.

rslt:resitivity
    a skos:Concept ;
    dcterms:provenance "Compiled by the Geological Survey of Queensland" ;
    rdfs:isDefinedBy <https://linked.data.gov.au/def/result-type> ;
    skos:altLabel "Resistance"@en ;
    skos:definition "The measure of the degree to which a conductor opposes an electric current through that conductor."@en ;
    skos:inScheme <https://linked.data.gov.au/def/result-type> ;
    skos:notation "rres" ;
    skos:prefLabel "Resitivity"@en ;
    skos:topConceptOf <https://linked.data.gov.au/def/result-type> ;
.

rslt:rotation
    a skos:Concept ;
    dcterms:provenance "Compiled by the Geological Survey of Queensland" ;
    rdfs:isDefinedBy <https://linked.data.gov.au/def/result-type> ;
    skos:altLabel "Rotation Rate"@en ;
    skos:definition "A measure of the rate of circular movement of an object around a center (or point) of rotation."@en ;
    skos:inScheme <https://linked.data.gov.au/def/result-type> ;
    skos:notation "rrtt" ;
    skos:prefLabel "Rotation"@en ;
    skos:topConceptOf <https://linked.data.gov.au/def/result-type> ;
.

rslt:sales-volumetric
    a skos:Concept ;
    dcterms:provenance "Compiled by the Geological Survey of Queensland" ;
    rdfs:isDefinedBy <https://linked.data.gov.au/def/result-type> ;
    skos:definition "A measure of the amount of a commodity in its unit of sale. A measure of a reserve or resource volume."@en ;
    skos:inScheme <https://linked.data.gov.au/def/result-type> ;
    skos:notation "rsal" ;
    skos:prefLabel "Sales Volumetric"@en ;
    skos:scopeNote "Sales volumes are represented by commodity specific units of measure that are internally inconsistent within a standard result type and refer specifically to the context of marketable quantities i.e. a sales quantity may be a volume, energy unit, mass, or other result type."@en ;
    skos:topConceptOf <https://linked.data.gov.au/def/result-type> ;
.

rslt:saturation
    a skos:Concept ;
    dcterms:provenance "Compiled by the Geological Survey of Queensland" ;
    rdfs:isDefinedBy <https://linked.data.gov.au/def/result-type> ;
    skos:definition "A measure of the amount of a substance contained within a volume or another material relative to the maximum theoretical amount of substance that could be contained under the same conditions."@en ;
    skos:inScheme <https://linked.data.gov.au/def/result-type> ;
    skos:notation "rsat" ;
    skos:prefLabel "Saturation"@en ;
    skos:topConceptOf <https://linked.data.gov.au/def/result-type> ;
.

rslt:shear-strength
    a skos:Concept ;
    dcterms:provenance "Compiled by the Geological Survey of Queensland" ;
    rdfs:isDefinedBy <https://linked.data.gov.au/def/result-type> ;
    skos:definition "The ability to withstand the strength of a material or component against the type of yield or structural failure when the material or component fails in shear. A shear load is a force that tends to produce a sliding failure on a material along a plane that is parallel to the direction of the force. When a paper is cut with scissors, the paper fails in shear.shearing"@en ;
    skos:inScheme <https://linked.data.gov.au/def/result-type> ;
    skos:notation "rshs" ;
    skos:prefLabel "Shear Strength"@en ;
    skos:topConceptOf <https://linked.data.gov.au/def/result-type> ;
.

rslt:sorting
    a skos:Concept ;
    dcterms:provenance "Compiled by the Geological Survey of Queensland" ;
    rdfs:isDefinedBy <https://linked.data.gov.au/def/result-type> ;
    skos:altLabel "Sedimentary Sorting"@en ;
    skos:definition "The distribution of grain size of sediments, either in unconsolidated deposits or in sedimentary rocks. Very poorly sorted indicates that the sediment sizes are mixed (large variance); whereas well sorted indicates that the sediment sizes are similar (low variance)."@en ;
    skos:inScheme <https://linked.data.gov.au/def/result-type> ;
    skos:notation "rsrt" ;
    skos:prefLabel "Sorting"@en ;
    skos:topConceptOf <https://linked.data.gov.au/def/result-type> ;
.

rslt:spacing
    a skos:Concept ;
    dcterms:provenance "Compiled by the Geological Survey of Queensland" ;
    rdfs:isDefinedBy <https://linked.data.gov.au/def/result-type> ;
    skos:definition "The regular, or average, distance between recurrences of a feature along a transect or across an object."@en ;
    skos:inScheme <https://linked.data.gov.au/def/result-type> ;
    skos:notation "rspc" ;
    skos:prefLabel "Spacing"@en ;
    skos:topConceptOf <https://linked.data.gov.au/def/result-type> ;
.

rslt:sphericity
    a skos:Concept ;
    dcterms:provenance "Compiled by the Geological Survey of Queensland" ;
    rdfs:isDefinedBy <https://linked.data.gov.au/def/result-type> ;
    skos:definition "A measure of how closely the shape of an object resembles that of a perfect sphere."@en ;
    skos:inScheme <https://linked.data.gov.au/def/result-type> ;
    skos:notation "rsph" ;
    skos:prefLabel "Sphericity"@en ;
    skos:topConceptOf <https://linked.data.gov.au/def/result-type> ;
.

rslt:stiffness
    a skos:Concept ;
    dcterms:provenance "Compiled by the Geological Survey of Queensland" ;
    rdfs:isDefinedBy <https://linked.data.gov.au/def/result-type> ;
    skos:definition "The extent to which an object resists deformation in response to an applied force."@en ;
    skos:inScheme <https://linked.data.gov.au/def/result-type> ;
    skos:notation "rstf" ;
    skos:prefLabel "Stiffness"@en ;
    skos:topConceptOf <https://linked.data.gov.au/def/result-type> ;
.

rslt:strain
    a skos:Concept ;
    dcterms:provenance "Compiled by the Geological Survey of Queensland" ;
    rdfs:isDefinedBy <https://linked.data.gov.au/def/result-type> ;
    skos:definition "Strain is a measure of deformation representing the displacement between particles in the body relative to a reference length."@en ;
    skos:inScheme <https://linked.data.gov.au/def/result-type> ;
    skos:notation "rstn" ;
    skos:prefLabel "Strain"@en ;
    skos:topConceptOf <https://linked.data.gov.au/def/result-type> ;
.

rslt:stress
    a skos:Concept ;
    dcterms:provenance "Compiled by the Geological Survey of Queensland" ;
    rdfs:isDefinedBy <https://linked.data.gov.au/def/result-type> ;
    skos:definition "A physical quantity that expresses the internal forces that neighbouring particles of a continuous material exert on each other, while strain is the measure of the deformation of the material."@en ;
    skos:inScheme <https://linked.data.gov.au/def/result-type> ;
    skos:notation "rsts" ;
    skos:prefLabel "Stress"@en ;
    skos:topConceptOf <https://linked.data.gov.au/def/result-type> ;
.

rslt:temperature
    a skos:Concept ;
    dcterms:provenance "Compiled by the Geological Survey of Queensland" ;
    rdfs:isDefinedBy <https://linked.data.gov.au/def/result-type> ;
    skos:definition "A physical property of matter that quantitatively expresses hot and cold. Temperature is the manifestation of thermal energy, present in all matter, which is the source of the occurrence of heat, a flow of energy, when a body is in contact with another that is colder."@en ;
    skos:inScheme <https://linked.data.gov.au/def/result-type> ;
    skos:notation "rtmp" ;
    skos:prefLabel "Temperature"@en ;
    skos:topConceptOf <https://linked.data.gov.au/def/result-type> ;
.

rslt:tensile-strength
    a skos:Concept ;
    dcterms:provenance "Compiled by the Geological Survey of Queensland" ;
    rdfs:isDefinedBy <https://linked.data.gov.au/def/result-type> ;
    skos:definition "The maximum stress that a material can withstand while being stretched or pulled before breaking."@en ;
    skos:inScheme <https://linked.data.gov.au/def/result-type> ;
    skos:notation "rtns" ;
    skos:prefLabel "Tensile Strength"@en ;
    skos:topConceptOf <https://linked.data.gov.au/def/result-type> ;
.

rslt:thermal-conductivity
    a skos:Concept ;
    dcterms:provenance "Compiled by the Geological Survey of Queensland" ;
    rdfs:isDefinedBy <https://linked.data.gov.au/def/result-type> ;
    skos:altLabel "Thermal Conductance"@en ;
    skos:definition "A measure of a material's ability to conduct an thermal energy."@en ;
    skos:inScheme <https://linked.data.gov.au/def/result-type> ;
    skos:notation "rtcd" ;
    skos:prefLabel "Thermal Conductivity"@en ;
    skos:topConceptOf <https://linked.data.gov.au/def/result-type> ;
.

rslt:time
    a skos:Concept ;
    dcterms:provenance "Compiled by the Geological Survey of Queensland" ;
    rdfs:isDefinedBy <https://linked.data.gov.au/def/result-type> ;
    skos:definition "The indefinite continued progress of existence and events that occur in an apparently irreversible succession from the past, through the present, into the future."@en ;
    skos:inScheme <https://linked.data.gov.au/def/result-type> ;
    skos:notation "rtme" ;
    skos:prefLabel "Time"@en ;
    skos:topConceptOf <https://linked.data.gov.au/def/result-type> ;
.

rslt:true-vertical-depth
    a skos:Concept ;
    dcterms:provenance "Compiled by the Geological Survey of Queensland" ;
    rdfs:isDefinedBy <https://linked.data.gov.au/def/result-type> ;
    skos:altLabel "TVD" ;
    skos:definition "The depth below a reference point or reference datum in a direct vertical direction."@en ;
    skos:inScheme <https://linked.data.gov.au/def/result-type> ;
    skos:notation "rtvd" ;
    skos:prefLabel "True Vertical Depth"@en ;
    skos:topConceptOf <https://linked.data.gov.au/def/result-type> ;
.

rslt:velocity
    a skos:Concept ;
    dcterms:provenance "Compiled by the Geological Survey of Queensland" ;
    rdfs:isDefinedBy <https://linked.data.gov.au/def/result-type> ;
    skos:definition "The rate of change of its position with respect to a frame of reference, and is a function of time."@en ;
    skos:inScheme <https://linked.data.gov.au/def/result-type> ;
    skos:notation "rvel" ;
    skos:prefLabel "Velocity"@en ;
    skos:topConceptOf <https://linked.data.gov.au/def/result-type> ;
.

rslt:viscosity
    a skos:Concept ;
    dcterms:provenance "Compiled by the Geological Survey of Queensland" ;
    rdfs:isDefinedBy <https://linked.data.gov.au/def/result-type> ;
    skos:definition "A measure of the resistance to deformation of a fluid at a given rate. For liquids, it corresponds to the informal concept of 'thickness': for example, syrup has a higher viscosity than water."@en ;
    skos:inScheme <https://linked.data.gov.au/def/result-type> ;
    skos:notation "rvis" ;
    skos:prefLabel "Viscosity"@en ;
    skos:topConceptOf <https://linked.data.gov.au/def/result-type> ;
.

rslt:voltage
    a skos:Concept ;
    dcterms:provenance "Compiled by the Geological Survey of Queensland" ;
    rdfs:isDefinedBy <https://linked.data.gov.au/def/result-type> ;
    skos:altLabel
        "electric potential difference"@en ,
        "electric pressure"@en ,
        "electric tension"@en ;
    skos:definition "The difference in electric potential between two points. The voltage in a static electric field is defined as the work needed per unit of charge to move a test charge between the two points."@en ;
    skos:inScheme <https://linked.data.gov.au/def/result-type> ;
    skos:notation "rvlt" ;
    skos:prefLabel "Voltage"@en ;
    skos:topConceptOf <https://linked.data.gov.au/def/result-type> ;
.

rslt:volume
    a skos:Concept ;
    dcterms:provenance "Compiled by the Geological Survey of Queensland" ;
    rdfs:isDefinedBy <https://linked.data.gov.au/def/result-type> ;
    skos:definition "The quantity of three-dimensional space enclosed by a closed surface, for example, the space that a substance (solid, liquid, gas, or plasma) or shape occupies or contains."@en ;
    skos:inScheme <https://linked.data.gov.au/def/result-type> ;
    skos:notation "rvol" ;
    skos:prefLabel "Volume"@en ;
    skos:topConceptOf <https://linked.data.gov.au/def/result-type> ;
.

rslt:wavelength
    a skos:Concept ;
    dcterms:provenance "Compiled by the Geological Survey of Queensland" ;
    rdfs:isDefinedBy <https://linked.data.gov.au/def/result-type> ;
    skos:definition "The wavelength is the spatial period of a periodic wave the distance over which the shape of a wave repeats."@en ;
    skos:inScheme <https://linked.data.gov.au/def/result-type> ;
    skos:notation "rwvl" ;
    skos:prefLabel "Wavelength"@en ;
    skos:topConceptOf <https://linked.data.gov.au/def/result-type> ;
.

rslt:weight
    a skos:Concept ;
    dcterms:provenance "Compiled by the Geological Survey of Queensland" ;
    rdfs:isDefinedBy <https://linked.data.gov.au/def/result-type> ;
    skos:definition "The weight of an object is related to the force acting on the object, either due to gravity or to a reaction force that holds it in place."@en ;
    skos:inScheme <https://linked.data.gov.au/def/result-type> ;
    skos:notation "rwgt" ;
    skos:prefLabel "Weight"@en ;
    skos:topConceptOf <https://linked.data.gov.au/def/result-type> ;
.

rslt:weight-on-bit
    a skos:Concept ;
    dcterms:provenance "Compiled by the Geological Survey of Queensland" ;
    rdfs:isDefinedBy <https://linked.data.gov.au/def/result-type> ;
    skos:definition "The weight or force applied to a drill bit in the process of drilling a borehole."@en ;
    skos:inScheme <https://linked.data.gov.au/def/result-type> ;
    skos:notation "rwob" ;
    skos:prefLabel "Weight on Bit"@en ;
    skos:topConceptOf <https://linked.data.gov.au/def/result-type> ;
.

rslt:width
    a skos:Concept ;
    dcterms:provenance "Compiled by the Geological Survey of Queensland" ;
    rdfs:isDefinedBy <https://linked.data.gov.au/def/result-type> ;
    skos:definition "The measurement or extent of something from side to side; the lesser of two or the least of three dimensions of a body."@en ;
    skos:inScheme <https://linked.data.gov.au/def/result-type> ;
    skos:notation "rwid" ;
    skos:prefLabel "Width"@en ;
    skos:topConceptOf <https://linked.data.gov.au/def/result-type> ;
.

rslt:work
    a skos:Concept ;
    dcterms:provenance "Compiled by the Geological Survey of Queensland" ;
    rdfs:isDefinedBy <https://linked.data.gov.au/def/result-type> ;
    skos:definition "The product of force and displacement. A force is said to do work if, when acting, there is a movement of the point of application in the direction of the force."@en ;
    skos:inScheme <https://linked.data.gov.au/def/result-type> ;
    skos:notation "rwrk" ;
    skos:prefLabel "Work"@en ;
    skos:topConceptOf <https://linked.data.gov.au/def/result-type> ;
.

rslt:yield-point
    a skos:Concept ;
    dcterms:provenance "Compiled by the Geological Survey of Queensland" ;
    rdfs:isDefinedBy <https://linked.data.gov.au/def/result-type> ;
    skos:definition "The point on a stress-strain curve that indicates the limit of elastic behavior and the beginning of plastic behavior."@en ;
    skos:inScheme <https://linked.data.gov.au/def/result-type> ;
    skos:notation "ryld" ;
    skos:prefLabel "Yield Point"@en ;
    skos:topConceptOf <https://linked.data.gov.au/def/result-type> ;
.

<https://linked.data.gov.au/org/gsq>
    a sdo:Organization ;
    sdo:name "Geological Survey of Queensland" ;
    sdo:url "https://www.business.qld.gov.au/industries/mining-energy-water/resources/geoscience-information/gsq"^^xsd:anyURI ;
.

rslt:angle
    a skos:Concept ;
    dcterms:provenance "Compiled by the Geological Survey of Queensland" ;
    rdfs:isDefinedBy <https://linked.data.gov.au/def/result-type> ;
    skos:definition "In plane geometry, an angle is the figure formed by two rays, called the sides of the angle, sharing a common endpoint, called the vertex of the angle."@en ;
    skos:inScheme <https://linked.data.gov.au/def/result-type> ;
    skos:notation "rang" ;
    skos:prefLabel "Angle"@en ;
    skos:topConceptOf <https://linked.data.gov.au/def/result-type> ;
.

<https://linked.data.gov.au/def/result-type>
    a
        owl:Ontology ,
        skos:ConceptScheme ;
    dcterms:created "2020-02-08"^^xsd:date ;
    dcterms:creator <https://linked.data.gov.au/org/gsq> ;
    dcterms:modified "2023-03-16"^^xsd:date ;
    dcterms:provenance "Compiled by the Geological Survey of Queensland" ;
    dcterms:publisher <https://linked.data.gov.au/org/gsq> ;
    skos:definition "The description and definition of the qualitative and quantitative results obtained through geoscience observations."@en ;
    skos:hasTopConcept
        rslt:age ,
        rslt:angle ,
        rslt:api-gravity ,
        rslt:area ,
        rslt:capacitance ,
        rslt:casing-weight ,
        rslt:colour ,
        rslt:composition ,
        rslt:compressibility ,
        rslt:compressive-strength ,
        rslt:concentration ,
        rslt:cost ,
        rslt:count ,
        rslt:curvature ,
        rslt:data ,
        rslt:density ,
        rslt:descriptive ,
        rslt:distance ,
        rslt:drill-rate ,
        rslt:electric-charge ,
        rslt:electric-current ,
        rslt:electrical-conductivity ,
        rslt:elevation ,
        rslt:energy ,
        rslt:energy-density ,
        rslt:flow-rate ,
        rslt:fluid-density ,
        rslt:force ,
        rslt:frequency ,
        rslt:gas-content ,
        rslt:grain-shape ,
        rslt:grain-size ,
        rslt:heat ,
        rslt:illuminance ,
        rslt:inductance ,
        rslt:length ,
        rslt:luminous-flux ,
        rslt:luminous-intensity ,
        rslt:magnetic-flux ,
        rslt:magnetic-flux-density ,
        rslt:magnetic-susceptibility ,
        rslt:mass ,
        rslt:measured-depth ,
        rslt:oil-quality ,
        rslt:permeability ,
        rslt:porosity ,
        rslt:power ,
        rslt:pressure ,
        rslt:radioactivity ,
        rslt:recovery ,
        rslt:resitivity ,
        rslt:rotation ,
        rslt:sales-volumetric ,
        rslt:saturation ,
        rslt:shear-strength ,
        rslt:sorting ,
        rslt:spacing ,
        rslt:sphericity ,
        rslt:stiffness ,
        rslt:strain ,
        rslt:stress ,
        rslt:temperature ,
        rslt:tensile-strength ,
        rslt:thermal-conductivity ,
        rslt:time ,
        rslt:true-vertical-depth ,
        rslt:velocity ,
        rslt:viscosity ,
        rslt:voltage ,
        rslt:volume ,
        rslt:wavelength ,
        rslt:weight ,
        rslt:weight-on-bit ,
        rslt:width ,
        rslt:work ,
        rslt:yield-point ;
    skos:prefLabel "Result Type"@en ;
.

