PREFIX retstat: <http://linked.data.gov.au/def/retention-status/>
PREFIX agldwgstatus: <https://linked.data.gov.au/def/reg-statuses/>
PREFIX cs: <http://linked.data.gov.au/def/retention-status/>
PREFIX dcterms: <http://purl.org/dc/terms/>
PREFIX owl: <http://www.w3.org/2002/07/owl#>
PREFIX rdfs: <http://www.w3.org/2000/01/rdf-schema#>
PREFIX reg: <http://purl.org/linked-data/registry#>
PREFIX sdo: <https://schema.org/>
PREFIX skos: <http://www.w3.org/2004/02/skos/core#>
PREFIX xsd: <http://www.w3.org/2001/XMLSchema#>

retstat:gsq-hold
    a skos:Concept ;
    skos:historyNote "Created from the WIMS MIRO brainstorming session" ;
    rdfs:isDefinedBy cs: ;
    skos:definition "To be held until the requesting officer or their director relinquishes the hold. Can be viewed and sampled, but not disposed."@en ;
    skos:inScheme cs: ;
    skos:notation "gsq-hold" ;
    skos:prefLabel "GSQ Hold"@en ;
    skos:topConceptOf cs: ;
.

retstat:type-section
    a skos:Concept ;
    skos:historyNote "Created from the WIMS MIRO brainstorming session" ;
    rdfs:isDefinedBy cs: ;
    skos:definition "To be held indefinitely or until replaced by a sample which meets the strict criteria set for type sections. Type sections are the part of the definition of a lithostratigraphic unit, without a type section the unit is considered invalid and has no official standing. Can be viewed and sampled (With approval), but not disposed. Refer to https://www.ga.gov.au/data-pubs/datastandards/stratigraphic-units/stratigraphic-type-sections"@en ;
    skos:inScheme cs: ;
    skos:notation "type-section" ;
    skos:prefLabel "Type Section"@en ;
    skos:topConceptOf cs: ;
.

retstat:reference-collection
    a skos:Concept ;
    skos:historyNote "Created from the WIMS MIRO brainstorming session" ;
    rdfs:isDefinedBy cs: ;
    skos:definition "To be held indefinitely or until replaced by a sample which meets the strict criteria set.  Can be viewed and sampled (With approval), but not disposed."@en ;
    skos:inScheme cs: ;
    skos:notation "reference-collection" ;
    skos:prefLabel "Reference Collection"@en ;
    skos:topConceptOf cs: ;
.

retstat:university-hold
    a skos:Concept ;
    skos:historyNote "Created from the WIMS MIRO brainstorming session" ;
    rdfs:isDefinedBy cs: ;
    skos:definition "Held by the Gelogical Survey of Queensland on behalf of a university. Not to be disposed of until the requesting acadameic relinquishes the hold, or the hold is released by a GSQ Director. Can be viewed and sampled, but not disposed."@en ;
    skos:inScheme cs: ;
    skos:notation "university-hold" ;
    skos:prefLabel "University Hold"@en ;
    skos:topConceptOf cs: ;
.

retstat:proposed-disposal
    a skos:Concept ;
    skos:historyNote "Created from the WIMS MIRO brainstorming session" ;
    rdfs:isDefinedBy cs: ;
    skos:definition "This sample has been proposed to be disposed. Can be viewed and sampled, but not disposed."@en ;
    skos:inScheme cs: ;
    skos:notation "proposed-disposal" ;
    skos:prefLabel "Proposed for Disposal"@en ;
    skos:topConceptOf cs: ;
.

retstat:approved-disposal
    a skos:Concept ;
    skos:historyNote "Created from the WIMS MIRO brainstorming session" ;
    rdfs:isDefinedBy cs: ;
    skos:definition "This sample has been approved for and is now pending disposal. Can be viewed and sampled and disposed."@en ;
    skos:inScheme cs: ;
    skos:notation "approved-disposal" ;
    skos:prefLabel "Awaiting Disposal"@en ;
    skos:topConceptOf cs: ;
.

retstat:disposed
    a skos:Concept ;
    skos:historyNote "Created from the WIMS MIRO brainstorming session" ;
    rdfs:isDefinedBy cs: ;
    skos:definition "This sample has been disposed of and no longer exists in the collection. Cannot be viewed, sampled or disposed."@en ;
    skos:inScheme cs: ;
    skos:notation "disposed" ;
    skos:prefLabel "Disposed"@en ;
    skos:topConceptOf cs: ;
.

retstat:permanent-collection
    a skos:Concept ;
    skos:historyNote "Created from the WIMS MIRO brainstorming session" ;
    rdfs:isDefinedBy cs: ;
    skos:definition "To be held indefinitely, or until a director approves its disposal. Can be viewed and sampled, but not disposed."@en ;
    skos:inScheme cs: ;
    skos:notation "permanent-collection" ;
    skos:prefLabel "Permanent Collection"@en ;
    skos:topConceptOf cs: ;
.

retstat:scientifically-significant 
    a skos:Concept ;
    skos:historyNote "Created from the WIMS MIRO brainstorming session" ;
    rdfs:isDefinedBy cs: ;
    skos:definition "A sample which has been identified as having a scientifically significant section contained within. To be held indefinitely, or until a director approves its disposal. Can be viewed and sampled, but not disposed."@en ;
    skos:inScheme cs: ;
    skos:notation "scientifically-significant " ;
    skos:prefLabel "Scientifically Significant "@en ;
    skos:topConceptOf cs: ;
.

<https://linked.data.gov.au/org/gsq>
    a sdo:Organization ;
    sdo:name "Geological Survey of Queensland" ;
    sdo:url "http://www.business.qld.gov.au/industries/mining-energy-water/resources/geoscience-information/gsq"^^xsd:anyURI ;
.

cs:
    a
        owl:Ontology ,
        skos:ConceptScheme ;
    dcterms:created "2024-08-06"^^xsd:date ;
    dcterms:creator <https://linked.data.gov.au/org/gsq> ;
    dcterms:modified "2025-11-10"^^xsd:date ;
    skos:historyNote "Created from the WIMS MIRO brainstorming session" ;
    dcterms:publisher <https://linked.data.gov.au/org/gsq> ;
    reg:status agldwgstatus:stable ;
    skos:definition "The role or use of the address in relation to a party. An address may have more than one purpose."@en ;
    skos:hasTopConcept
        retstat:gsq-hold ,
        retstat:type-section ,
        retstat:reference-collection ,
        retstat:university-hold ,
        retstat:proposed-disposal ,
        retstat:approved-disposal ,
        retstat:disposed ,
        retstat:scientifically-significant ,
        retstat:permanent-collection ;
    skos:prefLabel "Retention Status"@en ;
.
