PREFIX agldwgstatus: <https://linked.data.gov.au/def/reg-statuses/>
PREFIX cs: <http://linked.data.gov.au/def/sample-detail-type>
PREFIX dcterms: <http://purl.org/dc/terms/>
PREFIX owl: <http://www.w3.org/2002/07/owl#>
PREFIX rdfs: <http://www.w3.org/2000/01/rdf-schema#>
PREFIX reg: <http://purl.org/linked-data/registry#>
PREFIX sdo: <https://schema.org/>
PREFIX skos: <http://www.w3.org/2004/02/skos/core#>
PREFIX smpdt: <http://linked.data.gov.au/def/sample-detail-type/>
PREFIX xsd: <http://www.w3.org/2001/XMLSchema#>

smpdt:core-tray
    a skos:Concept ;
    skos:historyNote "Compiled by the Geological Survey of Queensland" ;
    rdfs:isDefinedBy cs: ;
    skos:definition "The range of plastic, cardboard or metal tray which holds samples of drill core on a pallet"@en ;
    skos:inScheme cs: ;
    skos:prefLabel "Core tray"@en ;
    skos:topConceptOf cs: ;
.

smpdt:retention-status
    a skos:Concept ;
    skos:historyNote "Compiled by the Geological Survey of Queensland" ;
    rdfs:isDefinedBy cs: ;
    skos:definition "The protections or lack thereof for a sample. For example, a core which is defined as a type section in its retention status, cannot be disposed. "@en ;
    skos:inScheme cs: ;
    skos:prefLabel "Retention Status"@en ;
    skos:topConceptOf cs: ;
.

smpdt:radiation-reading
    a skos:Concept ;
    skos:historyNote "Compiled by the Geological Survey of Queensland" ;
    rdfs:isDefinedBy cs: ;
    skos:definition "Radiation reading collected of each pallet, units recorded in microsievert per hour (Î¼Sv/hour)"@en ;
    skos:inScheme cs: ;
    skos:prefLabel "Radiation reading"@en ;
    skos:topConceptOf cs: ;
.

smpdt:stockpile-purpose
    a skos:Concept ;
    skos:historyNote "Compiled by the Geological Survey of Queensland" ;
    rdfs:isDefinedBy cs: ;
    skos:definition "The operational reason for which stockpiles created at a mine site "@en ;
    skos:inScheme cs: ;
    skos:prefLabel "Stockpile purpose"@en ;
    skos:topConceptOf cs: ;
.

smpdt:core-condition
    a skos:Concept ;
    skos:historyNote "Compiled by the Geological Survey of Queensland" ;
    rdfs:isDefinedBy cs: ;
    skos:definition "Condition of borehole core"@en ;
    skos:inScheme cs: ;
    skos:prefLabel "Core Condition"@en ;
    skos:topConceptOf cs: ;
.

smpdt:core-tray-condition
    a skos:Concept ;
    skos:historyNote "Compiled by the Geological Survey of Queensland" ;
    rdfs:isDefinedBy cs: ;
    skos:definition "Condition of tray used to store borehole core"@en ;
    skos:inScheme cs: ;
    skos:prefLabel "Core Tray Condition"@en ;
    skos:topConceptOf cs: ;
.

smpdt:pallet-condition
    a skos:Concept ;
    skos:historyNote "Compiled by the Geological Survey of Queensland" ;
    rdfs:isDefinedBy cs: ;
    skos:definition "Condition of a storage pallet"@en ;
    skos:inScheme cs: ;
    skos:prefLabel "Pallet Condition"@en ;
    skos:topConceptOf cs: ;
.

smpdt:pallet-weight
    a skos:Concept ;
    skos:historyNote "Compiled by the Geological Survey of Queensland" ;
    rdfs:isDefinedBy cs: ;
    skos:definition "Weight of pallet in kg"@en ;
    skos:inScheme cs: ;
    skos:prefLabel "Pallet Weight"@en ;
    skos:topConceptOf cs: ;
.

smpdt:processor
    a skos:Concept ;
    skos:historyNote "Compiled by the Geological Survey of Queensland" ;
    rdfs:isDefinedBy cs: ;
    skos:definition "An entity that performs any processing on the sample (Sampling Method), that is not the owner or final acquirer of the sample, e.g. a processing plant that generates a product from raw material on behalf of the reporting mine that acquires the sample."@en ;
    skos:inScheme cs: ;
    skos:prefLabel "Processor"@en ;
    skos:topConceptOf cs: ;
.

smpdt:sample-transactor
    a skos:Concept ;
    skos:historyNote "Compiled by the Geological Survey of Queensland" ;
    rdfs:isDefinedBy cs: ;
    skos:altLabel
        "Buyer"@en ,
        "Donor"@en ,
        "Giver"@en ,
        "Recipient"@en ,
        "Seller"@en ;
    skos:definition "The other party to a transaction with the party-of-interest in which a sample changes possession, ownership, or custodianship. The party who are the giver of a sample received or purchased by the party-of-interest.  The party who are the recipient of a sample given or sold by the party-of-interest."@en ;
    skos:inScheme cs: ;
    skos:prefLabel "Sample Transactor"@en ;
    skos:topConceptOf cs: ;
.

<https://linked.data.gov.au/org/gsq>
    a sdo:Organization ;
    sdo:name "Geological Survey of Queensland" ;
    sdo:url "https://www.business.qld.gov.au/industries/mining-energy-water/resources/geoscience-information/gsq"^^xsd:anyURI ;
.

cs:
    a
        owl:Ontology ,
        skos:ConceptScheme ;
    dcterms:created "2020-03-30"^^xsd:date ;
    dcterms:creator <https://linked.data.gov.au/org/gsq> ;
    dcterms:modified "2023-03-16"^^xsd:date ;
    skos:historyNote "Compiled by the Geological Survey of Queensland" ;
    dcterms:publisher <https://linked.data.gov.au/org/gsq> ;
    reg:status agldwgstatus:stable ;
    skos:definition "Miscellaneous details that describe samples that are outside the common core sample profile."@en ;
    skos:hasTopConcept
        smpdt:core-condition ,
        smpdt:core-tray-condition ,
        smpdt:pallet-condition ,
        smpdt:pallet-weight ,
        smpdt:processor ,
        smpdt:sample-transactor ;
    skos:prefLabel "Sample Detail Type"@en ;
.

