PREFIX agldwgstatus: <https://linked.data.gov.au/def/reg-statuses/>
PREFIX cs: <http://linked.data.gov.au/def/sample-type>
PREFIX dcterms: <http://purl.org/dc/terms/>
PREFIX owl: <http://www.w3.org/2002/07/owl#>
PREFIX rdfs: <http://www.w3.org/2000/01/rdf-schema#>
PREFIX reg: <http://purl.org/linked-data/registry#>
PREFIX sampty: <http://linked.data.gov.au/def/sample-type/>
PREFIX sdo: <https://schema.org/>
PREFIX skos: <http://www.w3.org/2004/02/skos/core#>
PREFIX xsd: <http://www.w3.org/2001/XMLSchema#>

sampty:hcore
    a skos:Concept ;
    skos:historyNote "Compiled by the Geological Survey of Queensland" ;
    rdfs:isDefinedBy cs: ;
    skos:broader sampty:core ;
    skos:definition "A core sample that has been cut in half parallel to its length."@en ;
    skos:inScheme cs: ;
    skos:notation "HCORE" ;
    skos:prefLabel "Half Core"@en ;
.

sampty:hydraulic-fracturing-fluid
    a skos:Concept ;
    skos:historyNote "Compiled by the Geological Survey of Queensland" ;
    rdfs:isDefinedBy cs: ;
    skos:definition "A sample of the fluid used in the hydraulic fracturing process."@en ;
    skos:inScheme cs: ;
    skos:prefLabel "Hydraulic Fracturing Fluid"@en ;
    skos:topConceptOf cs: ;
.

sampty:image-log
    a skos:Concept ;
    skos:historyNote "Compiled by the Geological Survey of Queensland" ;
    rdfs:isDefinedBy cs: ;
    skos:broader sampty:petrophysical-log ;
    skos:definition "A petrophysical log comprised of multiple directional measurements around the circumference of a wellbore to create an image detailing variation of properties around the borehole."@en ;
    skos:inScheme cs: ;
    skos:notation "IMLG" ;
    skos:prefLabel "Image Log"@en ;
.

sampty:qcore
    a skos:Concept ;
    skos:historyNote "Compiled by the Geological Survey of Queensland" ;
    rdfs:isDefinedBy cs: ;
    skos:broader sampty:core ;
    skos:definition "A core sample that has been cut in quarters parallel to its length."@en ;
    skos:inScheme cs: ;
    skos:notation "QCORE" ;
    skos:prefLabel "Quarter Core"@en ;

.
sampty:slab
    a skos:Concept ;
    skos:historyNote "Compiled by the Geological Survey of Queensland" ;
    rdfs:isDefinedBy cs: ;
    skos:broader sampty:core ;
    skos:definition "A thin, approximately 5mm slice, cut from the flat face of halved drill core."@en ;
    skos:inScheme cs: ;
    skos:notation "SLAB" ;
    skos:prefLabel "Slab"@en ;
.

sampty:blasted-sample
    a skos:Concept ;
    skos:historyNote "Compiled by the Geological Survey of Queensland" ;
    rdfs:isDefinedBy cs: ;
    skos:definition "Sample collected by drilling and blasting"@en ;
    skos:inScheme cs: ;
    skos:notation "BLSAMP" ;
    skos:prefLabel "Blasted Sample"@en ;
    skos:topConceptOf cs: ;
.

sampty:borehole-cement
    a skos:Concept ;
    skos:historyNote "Compiled by the Geological Survey of Queensland" ;
    rdfs:isDefinedBy cs: ;
    skos:definition "The cement used to bind casing to the wall of a well or bore, for borehole integrity."@en ;
    skos:inScheme cs: ;
    skos:notation "BHCM" ;
    skos:prefLabel "Borehole Cement"@en ;
    skos:topConceptOf cs: ;
.

sampty:boxed-core
    a skos:Concept ;
    skos:historyNote "Compiled by the Geological Survey of Queensland" ;
    rdfs:isDefinedBy cs: ;
    skos:altLabel
        "Core Box"@en ,
        "Core Tray"@en ;
    skos:definition "A part of a core sample which has been broken into shorter lengths and placed into boxes or trays for ease of storage."@en ;
    skos:inScheme cs: ;
    skos:notation "BOXCORE" ;
    skos:prefLabel "Boxed Core"@en ;
    skos:topConceptOf cs: ;
.

sampty:bulk-cyanide-leach-sample
    a skos:Concept ;
    skos:historyNote "Compiled by the Geological Survey of Queensland" ;
    rdfs:isDefinedBy cs: ;
    skos:definition "Sample collected to test for extraction by bulk cyanide leach process"@en ;
    skos:inScheme cs: ;
    skos:notation "BCL" ;
    skos:prefLabel "Bulk Cyanide Leach Sample"@en ;
    skos:topConceptOf cs: ;
.

sampty:channel-sample
    a skos:Concept ;
    skos:historyNote "Compiled by the Geological Survey of Queensland" ;
    rdfs:isDefinedBy cs: ;
    skos:definition "A sample composed of pieces of vein or mineral deposit that have been cut out of a small trench or channel, usually about 10 cm wide and 2 cm deep."@en ;
    skos:inScheme cs: ;
    skos:notation "CSAMP" ;
    skos:prefLabel "Channel Sample"@en ;
    skos:topConceptOf cs: ;
.

sampty:composited-core
    a skos:Concept ;
    skos:historyNote "Compiled by the Geological Survey of Queensland" ;
    rdfs:isDefinedBy cs: ;
    skos:definition "Core combined from various sources to create a representative sample."@en ;
    skos:inScheme cs: ;
    skos:notation "CCO" ;
    skos:prefLabel "Composited Core"@en ;
    skos:topConceptOf cs: ;
.

sampty:composited-cuttings
    a skos:Concept ;
    skos:historyNote "Compiled by the Geological Survey of Queensland" ;
    rdfs:isDefinedBy cs: ;
    skos:definition "Cuttings combined from various sources to create a representative sample."@en ;
    skos:inScheme cs: ;
    skos:notation "CCU" ;
    skos:prefLabel "Composited Cuttings"@en ;
    skos:topConceptOf cs: ;
.

sampty:continuous-channel-sample
    a skos:Concept ;
    skos:historyNote "Compiled by the Geological Survey of Queensland" ;
    rdfs:isDefinedBy cs: ;
    skos:definition "A composite channel sample taken from multiple points within a channel."@en ;
    skos:inScheme cs: ;
    skos:notation "CCSAMP" ;
    skos:prefLabel "Continuous Channel Sample"@en ;
    skos:topConceptOf cs: ;
.

sampty:core-plug
    a skos:Concept ;
    skos:historyNote "Compiled by the Geological Survey of Queensland" ;
    rdfs:isDefinedBy cs: ;
    skos:definition "A plug, or sample, taken from a core sample for analysis."@en ;
    skos:inScheme cs: ;
    skos:notation "PLUG" ;
    skos:prefLabel "Core Plug"@en ;
    skos:topConceptOf cs: ;
.

sampty:crushed-rock
    a skos:Concept ;
    skos:historyNote "Compiled by the Geological Survey of Queensland" ;
    rdfs:isDefinedBy cs: ;
    skos:altLabel
        "Ground Rock"@en ,
        "Milled rock"@en ;
    skos:definition "A sample of rock that has been artificially crushed, milled, or ground."@en ;
    skos:inScheme cs: ;
    skos:notation "CRUSH" ;
    skos:prefLabel "Crushed Rock"@en ;
    skos:topConceptOf cs: ;
.

sampty:cuttings
    a skos:Concept ;
    skos:historyNote "Compiled by the Geological Survey of Queensland" ;
    rdfs:isDefinedBy cs: ;
    skos:definition "Cuttings are the small pieces of rock that are chipped away by the bit while a well is being drilled."@en ;
    skos:inScheme cs: ;
    skos:notation "CUT" ;
    skos:prefLabel "Cuttings"@en ;
    skos:topConceptOf cs: ;
.

sampty:deviation-log
    a skos:Concept ;
    skos:historyNote "Compiled by the Geological Survey of Queensland" ;
    rdfs:isDefinedBy cs: ;
    skos:definition "A file containing information such as aziumth and inclination or positional offset to describe the downhole geometry of a borehole."@en ;
    skos:inScheme cs: ;
    skos:notation "DVLG" ;
    skos:prefLabel "Deviation Log"@en ;
    skos:topConceptOf cs: ;
.

sampty:drill-fluid
    a skos:Concept ;
    skos:historyNote "Compiled by the Geological Survey of Queensland" ;
    rdfs:isDefinedBy cs: ;
    skos:altLabel
        "Drill Mud"@en ,
        "Drilling Fluid"@en ,
        "Drilling Mud"@en ;
    skos:definition "Fluid used for drill bit lubrication and return of ground rock material from the drill bit."@en ;
    skos:inScheme cs: ;
    skos:notation "DLFD" ;
    skos:prefLabel "Drill Fluid"@en ;
    skos:topConceptOf cs: ;
.

sampty:drill-spoil
    a skos:Concept ;
    skos:historyNote "Compiled by the Geological Survey of Queensland" ;
    rdfs:isDefinedBy cs: ;
    skos:definition "Undifferentiated material generated during drilling."@en ;
    skos:inScheme cs: ;
    skos:notation "DSPOIN" ;
    skos:prefLabel "Drill Spoil"@en ;
    skos:topConceptOf cs: ;
.

sampty:drill-stem-test
    a skos:Concept ;
    skos:historyNote "Compiled by the Geological Survey of Queensland" ;
    rdfs:isDefinedBy cs: ;
    skos:definition "Test for pressure, permeability and production capabity of a reservoir"@en ;
    skos:inScheme cs: ;
    skos:notation "DSTEM" ;
    skos:prefLabel "Drill Stem Test"@en ;
    skos:topConceptOf cs: ;
.

sampty:feather-and-wedge-sample
    a skos:Concept ;
    skos:historyNote "Compiled by the Geological Survey of Queensland" ;
    rdfs:isDefinedBy cs: ;
    skos:definition "Sample collected by drilling and feathers and wedges."@en ;
    skos:inScheme cs: ;
    skos:notation "FWSAMP" ;
    skos:prefLabel "Feather & Wedge Sample"@en ;
    skos:topConceptOf cs: ;
.

sampty:float
    a skos:Concept ;
    skos:historyNote "Compiled by the Geological Survey of Queensland" ;
    rdfs:isDefinedBy cs: ;
    skos:definition "Loose rock collected at the surface"@en ;
    skos:inScheme cs: ;
    skos:notation "FLOAT" ;
    skos:prefLabel "Float"@en ;
    skos:topConceptOf cs: ;
.

sampty:georesource-process-input
    a skos:Concept ;
    skos:historyNote "Compiled by the Geological Survey of Queensland" ;
    rdfs:isDefinedBy cs: ;
    skos:altLabel "Mine Process Stock"@en ;
    skos:definition "Material feed for a mine processing plant or other refining facility that produced benefacted products. Feed may as mined or a blend of input materials with different attributes."@en ;
    skos:inScheme cs: ;
    skos:notation "GPM" ;
    skos:prefLabel "Georesource Process Material"@en ;
    skos:topConceptOf cs: ;
.

sampty:georesource-product
    a skos:Concept ;
    skos:historyNote "Compiled by the Geological Survey of Queensland" ;
    rdfs:isDefinedBy cs: ;
    skos:definition "The resource mined or material produced via a mine processing plant or other refining facility that is the final product."@en ;
    skos:inScheme cs: ;
    skos:notation "GP" ;
    skos:prefLabel "Georesource Product"@en ;
    skos:topConceptOf cs: ;
.

sampty:georesource-raw-material
    a skos:Concept ;
    skos:historyNote "Compiled by the Geological Survey of Queensland" ;
    rdfs:isDefinedBy cs: ;
    skos:definition "The raw resource of interest in mining or processing."@en ;
    skos:inScheme cs: ;
    skos:notation "GRM" ;
    skos:prefLabel "Georesource Raw Material"@en ;
    skos:topConceptOf cs: ;
.

sampty:hand-sample
    a skos:Concept ;
    skos:historyNote "Compiled by the Geological Survey of Queensland" ;
    rdfs:isDefinedBy cs: ;
    skos:definition "Representative sample collected from outcrop usually by geopick"@en ;
    skos:inScheme cs: ;
    skos:notation "HAND" ;
    skos:prefLabel "Hand Sample"@en ;
    skos:topConceptOf cs: ;
.

sampty:macrofossil
    a skos:Concept ;
    skos:historyNote "Compiled by the Geological Survey of Queensland" ;
    rdfs:isDefinedBy cs: ;
    skos:definition "Macrofossils collected for identification"@en ;
    skos:inScheme cs: ;
    skos:notation "MACFOS" ;
    skos:prefLabel "Macrofossil"@en ;
    skos:topConceptOf cs: ;
.

sampty:microfossil
    a skos:Concept ;
    skos:historyNote "Compiled by the Geological Survey of Queensland" ;
    rdfs:isDefinedBy cs: ;
    skos:definition "Sample collected to be processed for microfossil extraction"@en ;
    skos:inScheme cs: ;
    skos:notation "MICFOS" ;
    skos:prefLabel "Microfossil"@en ;
    skos:topConceptOf cs: ;
.

sampty:ore-sample
    a skos:Concept ;
    skos:historyNote "Compiled by the Geological Survey of Queensland" ;
    rdfs:isDefinedBy cs: ;
    skos:definition "Representative sample of ore sampled as a specimen or for analysis"@en ;
    skos:inScheme cs: ;
    skos:notation "ORE" ;
    skos:prefLabel "Ore Sample"@en ;
    skos:topConceptOf cs: ;
.

sampty:oriented-or-orientation-sample
    a skos:Concept ;
    skos:historyNote "Compiled by the Geological Survey of Queensland" ;
    rdfs:isDefinedBy cs: ;
    skos:definition "A sample collected as a known reference for the orientation of other samples."@en ;
    skos:inScheme cs: ;
    skos:notation "ORIENT" ;
    skos:prefLabel "Oriented Or Orientation Sample"@en ;
    skos:topConceptOf cs: ;
.

sampty:oriented-sample
    a skos:Concept ;
    skos:historyNote "Compiled by the Geological Survey of Queensland" ;
    rdfs:isDefinedBy cs: ;
    skos:altLabel "Oriented Section"@en ;
    skos:definition "Sample collected with orientation recorded for detailed structural geology analysis"@en ;
    skos:inScheme cs: ;
    skos:notation "OSAMP" ;
    skos:prefLabel "Oriented Sample"@en ;
    skos:topConceptOf cs: ;
.

sampty:paleomagnetic-sample
    a skos:Concept ;
    skos:historyNote "Compiled by the Geological Survey of Queensland" ;
    rdfs:isDefinedBy cs: ;
    skos:definition "Orientated hand-drill sample for paleomagnetic analysis"@en ;
    skos:inScheme cs: ;
    skos:notation "PMAG" ;
    skos:prefLabel "Paleomagnetic Sample"@en ;
    skos:topConceptOf cs: ;
.

sampty:pallet-core
    a skos:Concept ;
    skos:historyNote "Compiled by the Geological Survey of Queensland" ;
    rdfs:isDefinedBy cs: ;
    skos:altLabel
        "Core Pallet"@en ,
        "Pallet Core"@en ;
    skos:definition "A collection of core samples, typically boxed, placed on a pallet for the purpose of movement, storage, and logistics."@en ;
    skos:inScheme cs: ;
    skos:notation "PALCORE" ;
    skos:prefLabel "Palletised Core"@en ;
    skos:topConceptOf cs: ;
.

sampty:pan-concentrate
    a skos:Concept ;
    skos:historyNote "Compiled by the Geological Survey of Queensland" ;
    rdfs:isDefinedBy cs: ;
    skos:definition "Stream sediment that has been panned to concentrate heavy minerals"@en ;
    skos:inScheme cs: ;
    skos:notation "PCON" ;
    skos:prefLabel "Pan Concentrate"@en ;
    skos:topConceptOf cs: ;
.

sampty:photograph
    a skos:Concept ;
    skos:historyNote "Compiled by the Geological Survey of Queensland" ;
    rdfs:isDefinedBy cs: ;
    skos:definition "An image created by light falling on a photosensitive surface, usually photographic film or an electronic image sensor, such as a CCD or a CMOS chip."@en ;
    skos:inScheme cs: ;
    skos:notation "PHGR" ;
    skos:prefLabel "Photograph"@en ;
    skos:topConceptOf cs: ;
.

sampty:polished-block
    a skos:Concept ;
    skos:historyNote "Compiled by the Geological Survey of Queensland" ;
    rdfs:isDefinedBy cs: ;
    skos:definition "Rock samples that are bonded in epoxy and polished as small round blocks for reflected light microscopy."@en ;
    skos:inScheme cs: ;
    skos:notation "PBLK" ;
    skos:prefLabel "Polished Block"@en ;
    skos:topConceptOf cs: ;
.

sampty:powdered-chip
    a skos:Concept ;
    skos:historyNote "Compiled by the Geological Survey of Queensland" ;
    rdfs:isDefinedBy cs: ;
    skos:definition "A rock chip sample that has subsequently been powdered."@en ;
    skos:inScheme cs: ;
    skos:notation "PCHIP" ;
    skos:prefLabel "Powdered Chip"@en ;
    skos:topConceptOf cs: ;
.

sampty:pulp
    a skos:Concept ;
    skos:historyNote "Compiled by the Geological Survey of Queensland" ;
    rdfs:isDefinedBy cs: ;
    skos:definition "A rock sample that has been pulverised sample to a very fine powder and homogenised to be representative of a parent sample, or interval. "@en ;
    skos:inScheme cs: ;
    skos:notation "PULP" ;
    skos:prefLabel "Pulp"@en ;
    skos:topConceptOf cs: ;
.

sampty:random-dump-sample
    a skos:Concept ;
    skos:historyNote "Compiled by the Geological Survey of Queensland" ;
    rdfs:isDefinedBy cs: ;
    skos:definition "Sample collected from mine dump at random"@en ;
    skos:inScheme cs: ;
    skos:notation "RDSAMP" ;
    skos:prefLabel "Random Dump Sample"@en ;
    skos:topConceptOf cs: ;
.

sampty:random-sample
    a skos:Concept ;
    skos:historyNote "Compiled by the Geological Survey of Queensland" ;
    rdfs:isDefinedBy cs: ;
    skos:definition "A randomly collected sample"@en ;
    skos:inScheme cs: ;
    skos:notation "RSAMP" ;
    skos:prefLabel "Random Sample"@en ;
    skos:topConceptOf cs: ;
.

sampty:rock-chips
    a skos:Concept ;
    skos:historyNote "Compiled by the Geological Survey of Queensland" ;
    rdfs:isDefinedBy cs: ;
    skos:definition "Sample gathered as rock chips for geochemistry"@en ;
    skos:inScheme cs: ;
    skos:notation "CHIP" ;
    skos:prefLabel "Rock Chips"@en ;
    skos:topConceptOf cs: ;
.

sampty:scree
    a skos:Concept ;
    skos:historyNote "Compiled by the Geological Survey of Queensland" ;
    rdfs:isDefinedBy cs: ;
    skos:definition "Loose rock collected downslope from a ridge"@en ;
    skos:inScheme cs: ;
    skos:notation "SCREE" ;
    skos:prefLabel "Scree"@en ;
    skos:topConceptOf cs: ;
.

sampty:selected-dump-sample
    a skos:Concept ;
    skos:historyNote "Compiled by the Geological Survey of Queensland" ;
    rdfs:isDefinedBy cs: ;
    skos:definition "Sample collected from mine dump with suspected mineralisation"@en ;
    skos:inScheme cs: ;
    skos:notation "SDSAMP" ;
    skos:prefLabel "Selected Dump Sample"@en ;
    skos:topConceptOf cs: ;
.

sampty:selected-sample
    a skos:Concept ;
    skos:historyNote "Compiled by the Geological Survey of Queensland" ;
    rdfs:isDefinedBy cs: ;
    skos:definition "A sample that was specifically selected for analysis"@en ;
    skos:inScheme cs: ;
    skos:notation "SEL" ;
    skos:prefLabel "Selected Sample"@en ;
    skos:topConceptOf cs: ;
.

sampty:side-wall-core
    a skos:Concept ;
    skos:historyNote "Compiled by the Geological Survey of Queensland" ;
    rdfs:isDefinedBy cs: ;
    skos:definition "A core taken from the side of the borehole, usually by a wireline tool."@en ;
    skos:inScheme cs: ;
    skos:notation "SWC" ;
    skos:prefLabel "Side Wall Core"@en ;
    skos:topConceptOf cs: ;
.

sampty:sieved-stream-sediment-sample
    a skos:Concept ;
    skos:historyNote "Compiled by the Geological Survey of Queensland" ;
    rdfs:isDefinedBy cs: ;
    skos:definition "Stream sediment that has been sieved to break it up into different grainsize fractions"@en ;
    skos:inScheme cs: ;
    skos:notation "SSS" ;
    skos:prefLabel "Sieved Stream Sediment Sample"@en ;
    skos:topConceptOf cs: ;
.

sampty:sledge-hammer-sample
    a skos:Concept ;
    skos:historyNote "Compiled by the Geological Survey of Queensland" ;
    rdfs:isDefinedBy cs: ;
    skos:definition "Representative sample collected from outcrop by sledgehammer"@en ;
    skos:inScheme cs: ;
    skos:notation "SHSAMP" ;
    skos:prefLabel "Sledge Hammer Sample"@en ;
    skos:topConceptOf cs: ;
.

sampty:soil-sample
    a skos:Concept ;
    skos:historyNote "Compiled by the Geological Survey of Queensland" ;
    rdfs:isDefinedBy cs: ;
    skos:definition "Sample of soil taken from an exposure or auger sample"@en ;
    skos:inScheme cs: ;
    skos:notation "SOIL" ;
    skos:prefLabel "Soil Sample"@en ;
    skos:topConceptOf cs: ;
.

sampty:stream-sediment-sample
    a skos:Concept ;
    skos:historyNote "Compiled by the Geological Survey of Queensland" ;
    rdfs:isDefinedBy cs: ;
    skos:definition "Sample of sediment from active streams"@en ;
    skos:inScheme cs: ;
    skos:notation "STRSED" ;
    skos:prefLabel "Stream Sediment Sample"@en ;
    skos:topConceptOf cs: ;
.

sampty:suspended-silt-sample
    a skos:Concept ;
    skos:historyNote "Compiled by the Geological Survey of Queensland" ;
    rdfs:isDefinedBy cs: ;
    skos:definition "A water sample containing suspended sediment"@en ;
    skos:inScheme cs: ;
    skos:notation "SUSP" ;
    skos:prefLabel "Suspended Silt Sample"@en ;
    skos:topConceptOf cs: ;
.

sampty:termite-mound
    a skos:Concept ;
    skos:historyNote "Compiled by the Geological Survey of Queensland" ;
    rdfs:isDefinedBy cs: ;
    skos:definition "Sample collected from termite mounds"@en ;
    skos:inScheme cs: ;
    skos:notation "TMOUND" ;
    skos:prefLabel "Termite Mound"@en ;
    skos:topConceptOf cs: ;
.

sampty:thin-section
    a skos:Concept ;
    skos:historyNote "Compiled by the Geological Survey of Queensland" ;
    rdfs:isDefinedBy cs: ;
    skos:definition "A laboratory preparation of a rock, mineral, soil, pottery, bones, or even metal sample for use with a polarizing petrographic microscope, electron microscope and electron microprobe. A thin sliver of rock is cut from the sample with a diamond saw and ground optically flat. It is then mounted on a glass slide and then ground smooth using progressively finer abrasive grit until the sample is only 30 μm thick. "@en ;
    skos:inScheme cs: ;
    skos:notation "THINS" ;
    skos:prefLabel "Thin Section"@en ;
    skos:topConceptOf cs: ;
.

sampty:trench-spoil
    a skos:Concept ;
    skos:historyNote "Compiled by the Geological Survey of Queensland" ;
    rdfs:isDefinedBy cs: ;
    skos:definition "Undifferentiated material generated from sampling within a trench or pit."@en ;
    skos:inScheme cs: ;
    skos:notation "TSPOIL" ;
    skos:prefLabel "Trench Spoil"@en ;
    skos:topConceptOf cs: ;
.

sampty:unspecified
    a skos:Concept ;
    skos:historyNote "Compiled by the Geological Survey of Queensland" ;
    rdfs:isDefinedBy cs: ;
    skos:definition "An unknown or unspecified sample"@en ;
    skos:inScheme cs: ;
    skos:notation "UNSP" ;
    skos:prefLabel "Unspecified"@en ;
    skos:topConceptOf cs: ;
.

sampty:video
    a skos:Concept ;
    skos:historyNote "Compiled by the Geological Survey of Queensland" ;
    rdfs:isDefinedBy cs: ;
    skos:definition "An moving image created by light falling on a series of photosensitive surfaces, usually videographic film or an electronic image sensor, such as a CCD or a CMOS chip."@en ;
    skos:inScheme cs: ;
    skos:notation "VIDO" ;
    skos:prefLabel "video"@en ;
    skos:topConceptOf cs: ;
.

sampty:waste-rock
    a skos:Concept ;
    skos:historyNote "Compiled by the Geological Survey of Queensland" ;
    rdfs:isDefinedBy cs: ;
    skos:altLabel "Overburden"@en ;
    skos:definition "The rock removed during mining to reach resource."@en ;
    skos:inScheme cs: ;
    skos:notation "WR" ;
    skos:prefLabel "Waste Rock"@en ;
    skos:topConceptOf cs: ;
.

sampty:water-specimen
    a skos:Concept ;
    skos:historyNote "Compiled by the Geological Survey of Queensland" ;
    rdfs:isDefinedBy cs: ;
    skos:definition "A generic specimen of water of any type. Includes water specimen types collected by any method."@en ;
    skos:inScheme cs: ;
    skos:notation "WTRS" ;
    skos:prefLabel "Water specimen"@en ;
    skos:topConceptOf cs: ;
.

sampty:wellhead
    a skos:Concept ;
    skos:historyNote "Compiled by the Geological Survey of Queensland" ;
    rdfs:isDefinedBy cs: ;
    skos:definition "Component at surface that provides structural and pressure interface"@en ;
    skos:inScheme cs: ;
    skos:notation "WHEAD" ;
    skos:prefLabel "Wellhead"@en ;
    skos:topConceptOf cs: ;
.

sampty:petrophysical-log
    a skos:Concept ;
    skos:historyNote "Compiled by the Geological Survey of Queensland" ;
    rdfs:isDefinedBy cs: ;
    skos:definition "A digital file or image containing physical and chemical measurements from the logging of a borehole."@en ;
    skos:inScheme cs: ;
    skos:notation "PETL" ;
    skos:prefLabel "Petrophysical Log"@en ;
    skos:topConceptOf cs: ;
.

<https://linked.data.gov.au/org/gsq>
    a sdo:Organization ;
    sdo:name "Geological Survey of Queensland" ;
    sdo:url "https://www.business.qld.gov.au/industries/mining-energy-water/resources/geoscience-information/gsq"^^xsd:anyURI ;
.

sampty:core
    a skos:Concept ;
    skos:historyNote "Compiled by the Geological Survey of Queensland" ;
    rdfs:isDefinedBy cs: ;
    skos:definition "A core sample is a cylindrical section of (usually) a naturally occurring substance."@en ;
    skos:inScheme cs: ;
    skos:notation "CORE" ;
    skos:prefLabel "Core"@en ;
    skos:topConceptOf cs: ;
.

sampty:core-run
    a skos:Concept ;
    skos:historyNote "Compiled by the Geological Survey of Queensland" ;
    rdfs:isDefinedBy cs: ;
    skos:broader sampty:core ;
    skos:definition " A core run is a segment of a geological core sample that corresponds to the length of material recovered from a single core barrel during a coring operation."@en ;
    skos:inScheme cs: ;
    skos:notation "CORN" ;
    skos:prefLabel "Core Run"@en ;
    skos:topConceptOf cs: ;
.

cs:
    a
        owl:Ontology ,
        skos:ConceptScheme ;
    dcterms:created "2020-02-07"^^xsd:date ;
    dcterms:creator <https://linked.data.gov.au/org/gsq> ;
    dcterms:modified "2025-10-31"^^xsd:date ;
    skos:historyNote "Compiled by the Geological Survey of Queensland" ;
    dcterms:publisher <https://linked.data.gov.au/org/gsq> ;
    reg:status agldwgstatus:stable ;
    skos:definition "Types of sample used in Geoscience."@en ;
    skos:hasTopConcept
        sampty:blasted-sample ,
        sampty:borehole-cement ,
        sampty:boxed-core ,
        sampty:bulk-cyanide-leach-sample ,
        sampty:channel-sample ,
        sampty:composited-core ,
        sampty:composited-cuttings ,
        sampty:continuous-channel-sample ,
        sampty:core ,
        sampty:core-plug ,
        sampty:core-run ,
        sampty:crushed-rock ,
        sampty:cuttings ,
        sampty:deviation-log ,
        sampty:drill-fluid ,
        sampty:drill-spoil ,
        sampty:drill-stem-test ,
        sampty:feather-and-wedge-sample ,
        sampty:float ,
        sampty:georesource-process-input ,
        sampty:georesource-product ,
        sampty:georesource-raw-material ,
        sampty:hand-sample ,
        sampty:macrofossil ,
        sampty:microfossil ,
        sampty:ore-sample ,
        sampty:oriented-or-orientation-sample ,
        sampty:oriented-sample ,
        sampty:paleomagnetic-sample ,
        sampty:pallet-core ,
        sampty:pan-concentrate ,
        sampty:petrophysical-log ,
        sampty:photograph ,
        sampty:polished-block ,
        sampty:powdered-chip ,
        sampty:pulp ,
        sampty:random-dump-sample ,
        sampty:random-sample ,
        sampty:rock-chips ,
        sampty:scree ,
        sampty:selected-dump-sample ,
        sampty:selected-sample ,
        sampty:side-wall-core ,
        sampty:sieved-stream-sediment-sample ,
        sampty:slab ,
        sampty:sledge-hammer-sample ,
        sampty:soil-sample ,
        sampty:stream-sediment-sample ,
        sampty:suspended-silt-sample ,
        sampty:termite-mound ,
        sampty:thin-section ,
        sampty:trench-spoil ,
        sampty:unspecified ,
        sampty:video ,
        sampty:waste-rock ,
        sampty:water-specimen ,
        sampty:wellhead ;
    skos:prefLabel "Sample Type"@en ;
.

