@prefix dcterms: <http://purl.org/dc/terms/> .
@prefix owl: <http://www.w3.org/2002/07/owl#> .
@prefix ststs: <http://linked.data.gov.au/def/site-status/> .
@prefix sdo: <http://schema.org/> .
@prefix skos: <http://www.w3.org/2004/02/skos/core#> .
@prefix rdfs: <http://www.w3.org/2000/01/rdf-schema#> .
@prefix xsd: <http://www.w3.org/2001/XMLSchema#> .

<http://linked.data.gov.au/def/site-status> a owl:Ontology, skos:ConceptScheme ;
    dcterms:created "2020-02-28"^^xsd:date ;
    dcterms:creator <http://linked.data.gov.au/org/gsq> ;
    dcterms:modified "2022-05-12"^^xsd:date ;
    dcterms:publisher <http://linked.data.gov.au/org/gsq> ;
    dcterms:provenance "Compiled by the Geological Survey of Queensland. Mapped to GeoSciML Mine Status and amalgamation with Borehole status." ;
    skos:definition "The status of an individual site (e.g., mine, well) or single activity (e.g., survey) describing the current state within the lifecycle from proposed through operational through to abandonment. Lifecycle stages are commonly related to regulatory conditions administered by government agencies."@en ;
    skos:scopeNote "Site status describes the lifecycle of a single discrete activity, Whereas the resource project lifecycle describes the collective lifecycle status of a body of work that typically consists of multiple activities and sites"@en ;

    skos:hasTopConcept ststs:abandoned,
        ststs:active,
        ststs:construction,
        ststs:inactive,
        ststs:never-used,
        ststs:proposed,
        ststs:rehabilitation,
        ststs:unknown ;
    skos:altLabel  "Resource Project Status"@en ;
    skos:prefLabel "Site Status"@en .
    
<http://linked.data.gov.au/org/gsq> a sdo:Organization ;
    sdo:name "Geological Survey of Queensland" ;
    sdo:url "http://www.business.qld.gov.au/industries/mining-energy-water/resources/geoscience-information/gsq"^^xsd:anyURI .

ststs:cased-and-suspended a skos:Concept ;
    skos:broader ststs:inactive ;
    skos:definition "A well in which casing has been installed, but is suspended and inactive pending installation of completion, monitoring or other equipment."@en ;
    skos:inScheme <http://linked.data.gov.au/def/site-status> ;
    skos:prefLabel "Cased And Suspended"@en .

ststs:completed a skos:Concept ;
    skos:broader ststs:inactive ;
    skos:definition "A well that has had all relevant casing, tubing and completion equipment such as pumps installed, but is not in an active state of producing, injecting or monitoring."@en ;
    skos:inScheme <http://linked.data.gov.au/def/site-status> ;
    skos:prefLabel "Completed"@en .

ststs:monitoring a skos:Concept ;
    skos:broader ststs:active ;
    skos:definition "A well that is actively monitoring reservoir, aquifer or other geological parameters."@en ;
    skos:inScheme <http://linked.data.gov.au/def/site-status> ;
    skos:prefLabel "Monitoring"@en .

ststs:not-producing a skos:Concept ;
    skos:broader ststs:active ;
    skos:definition "A site that is part of a project or operation that is not currently contributing to production and is not conducting other operational activities. Such as a well undergoing routine maintenance that is not suspended, or a Mining Lease that is part of an active mine but is temporarily not contributing to mine production."@en ;
    skos:inScheme <http://linked.data.gov.au/def/site-status> ;
    skos:prefLabel "Not Producing"@en .

ststs:operational-non-prod a skos:Concept ;
    skos:altLabel "Operating But Not Producing"@en,
        "Non-Productive Operation"@en,
        "Excavation"@en,
        "Preparation"@en ;
    skos:broader ststs:active ;
    skos:definition "A site that is an active part of a project or operation that typically contributes to production but is not currently due to other activities, such as a well undergoing routine maintenance that is not suspended, or a Mining Lease in which excavation is occuring after construction, but prior to, or between, extraction phases."@en ;
    skos:inScheme <http://linked.data.gov.au/def/site-status> ;
    skos:prefLabel "Operating Not Producing"@en .

 ststs:secondary-operation a skos:Concept ;
    skos:altLabel "Other Purpose"@en,
        "Secondary Operations"@en;
    skos:broader ststs:active ;
    skos:definition "A site that is an active part of a project or operation, but is not involved in resource extraction, such as supporting secondary activities, including resoure processing, site access, adminstration or infrastructure. "@en ;
    skos:inScheme <http://linked.data.gov.au/def/site-status> ;
    skos:prefLabel "Supporting Operations"@en .

ststs:on-injection a skos:Concept ;
    skos:broader ststs:active ;
    skos:definition "A well that is injecting fluids, such as water or hydrocarbons into a reservoir for disposal or future production."@en ;
    skos:inScheme <http://linked.data.gov.au/def/site-status> ;
    skos:prefLabel "On Injection"@en .

ststs:on-production a skos:Concept ;
    skos:altLabel "Extraction"@en,
        "Mining"@en,
        "On Production"@en ;
    skos:broader ststs:active ;
    skos:definition "A well that is producing hydrocarbons or other non-water resources, or a mine or quarry that is actively extracting coal, minerals or other resources."@en ;
    skos:inScheme <http://linked.data.gov.au/def/site-status> ;
    skos:prefLabel "Producing"@en .

ststs:plugged-and-abandoned a skos:Concept ;
    skos:broader ststs:abandoned ;
    skos:definition "A borehole that has been abandoned without the intention and/or requirement to undertake further work. Petroleum wells must be abandoned as per the relevant Code of Practice. Petroleum wells are abandoned in two stages: sub-surface abandonment where the well is plugged with cement or another accepted plugging method, and surface abandonment where casing is cut and a vented plate or cap is installed at surface. Legislatively, a petroleum well is not abandoned until all aspects are completed including surface abandonment (cut and cap)."@en ;
    skos:inScheme <http://linked.data.gov.au/def/site-status> ;
    skos:altLabel "Capped and Abandoned"@en,
        "P&A"@en ;
    skos:prefLabel "Plugged And Abandoned"@en .

ststs:water-supply a skos:Concept ;
    skos:broader ststs:active ;
    skos:definition "A well that is primarily producing water"@en ;
    skos:inScheme <http://linked.data.gov.au/def/site-status> ;
    skos:prefLabel "Water Supply"@en .

ststs:care-and-maintenance a skos:Concept ;
    skos:broader ststs:inactive ;
    skos:definition "A non-operational mine site where production is stopped but the site is managed to ensure it remains in a safe and stable condition. Typically where there is potential to recommence works at a later date such as improved economic conditions."@en ;
    skos:exactMatch <http://resource.geosciml.org/classifier/cgi/mine-status/care-and-maintenance> ;
    skos:inScheme <http://linked.data.gov.au/def/site-status> ;
    skos:prefLabel "Care And Maintenance"@en .

ststs:on-hold a skos:Concept ;
    skos:altLabel "On Hold"@en ;
    skos:broader ststs:inactive ;
    skos:definition "A mine or project that has been closed but not abandoned and where there are no active and care-and-maintenance works."@en ;
    skos:exactMatch <http://resource.geosciml.org/classifier/cgi/mine-status/closed> ;
    skos:inScheme <http://linked.data.gov.au/def/site-status> ;
    skos:prefLabel "Closed"@en .

ststs:suspended a skos:Concept ;
    skos:altLabel "Drilled"@en,
        "Retention"@en ;
    skos:broader ststs:inactive ;
    skos:definition "A site such as a mine or quarry, project or activity that is temporarily not active, such as during the interval between construction and commencement of production or extraction."@en ;
    skos:exactMatch <http://resource.geosciml.org/classifier/cgi/mine-status/retention> ;
    skos:inScheme <http://linked.data.gov.au/def/site-status> ;
    skos:prefLabel "Suspended"@en .

ststs:never-used a skos:Concept ;
    skos:altLabel "Never Drilled"@en ;
    skos:definition "A project that was once proposed, but was never constructed and is no longer intended to be constructed."@en ;
    skos:inScheme <http://linked.data.gov.au/def/site-status> ;
    skos:prefLabel "Never Used"@en ;
    skos:topConceptOf <http://linked.data.gov.au/def/site-status> .

ststs:proposed a skos:Concept ;
    skos:definition "A mine, quarry or well that is intended, but has not yet been constructed."@en ;
    skos:inScheme <http://linked.data.gov.au/def/site-status> ;
    skos:prefLabel "Proposed"@en ;
    skos:topConceptOf <http://linked.data.gov.au/def/site-status> .

ststs:application a skos:Concept ;
    skos:definition "A mine, quarry, or well that is intended and has had an application for activity submitted to the governing authority that is pending assessment and outcome."@en ;
    skos:inScheme <http://linked.data.gov.au/def/site-status> ;
    skos:prefLabel "Application"@en ;
    skos:broader ststs:proposed .

ststs:approved a skos:Concept ;
    skos:definition "A mine, quarry or well that is intended and has had an application for activity approved, but has not yet commenced construction."@en ;
    skos:inScheme <http://linked.data.gov.au/def/site-status> ;
    skos:prefLabel "Approved"@en ;
    skos:broader ststs:proposed .

ststs:unknown a skos:Concept ;
    skos:definition "A mine, quarry, or well that has been constructed but whose further status is unknown."@en ;
    skos:inScheme <http://linked.data.gov.au/def/site-status> ;
    skos:prefLabel "Unknown"@en ;
    skos:topConceptOf <http://linked.data.gov.au/def/site-status> .

ststs:construction a skos:Concept ;
    skos:altLabel "Drilling"@en ;
    skos:definition "A mine, quarry or well that is being constructed or drilled, e.g. a well between spud date and rig release."@en ;
    skos:exactMatch <http://resource.geosciml.org/classifier/cgi/mine-status/construction> ;
    skos:inScheme <http://linked.data.gov.au/def/site-status> ;
    skos:prefLabel "Construction"@en ;
    skos:topConceptOf <http://linked.data.gov.au/def/site-status> .

ststs:abandoned a skos:Concept ;
    skos:altLabel "Concluded"@en ;
    skos:definition "A project or activity that has been abandoned without the intention and/or requirement to undertake further work."@en ;
    skos:exactMatch <http://resource.geosciml.org/classifier/cgi/mine-status/abandoned> ;
    skos:inScheme <http://linked.data.gov.au/def/site-status> ;
    skos:prefLabel "Abandoned"@en ;
    skos:topConceptOf <http://linked.data.gov.au/def/site-status> .

ststs:active a skos:Concept ;
    skos:altLabel "Active"@en ;
    skos:definition "A mine, quarry, or well that is in the active phase of resource exploitation as a direct extraction or associated activity i.e. producing, monitoring, injecting, mining, or processing."@en ;
    skos:exactMatch <http://resource.geosciml.org/classifier/cgi/mine-status/operating> ;
    skos:inScheme <http://linked.data.gov.au/def/site-status> ;
    skos:prefLabel "Operating"@en ;
    skos:topConceptOf <http://linked.data.gov.au/def/site-status> .

ststs:inactive a skos:Concept ;
    skos:altLabel "Not Operating"@en ;
    skos:definition "A project that has been constructed and not yet abandoned but is not in an active state."@en ;
    skos:exactMatch <http://resource.geosciml.org/classifier/cgi/mine-status/not-operating> ;
    skos:inScheme <http://linked.data.gov.au/def/site-status> ;
    skos:prefLabel "Inactive"@en ;
    skos:topConceptOf <http://linked.data.gov.au/def/site-status> .

ststs:rehabilitation a skos:Concept ;
    skos:definition "The stage in the life-cycle of a project or mine where the resources have been extracted and the site is being rehabilitated back to its original condition or an acceptable environmental standard."@en ;
    rdfs:isDefinedBy <http://linked.data.gov.au/def/site-status> ;
    skos:inScheme <http://linked.data.gov.au/def/site-status> ;
    skos:prefLabel "Rehabilitation"@en ;
    skos:topConceptOf <http://linked.data.gov.au/def/site-status> .

ststs:processing a skos:Concept ;
    skos:broader ststs:secondary-operation ;
    skos:definition "A site such as a mine or quarry which is processing but not mining raw material throughout the reporting period."@en ;
    skos:exactMatch <http://resource.geosciml.org/classifier/cgi/mine-status/retention> ;
    skos:inScheme <http://linked.data.gov.au/def/site-status> ;
    skos:prefLabel "Processing"@en .

ststs:approved a skos:Concept ;
    skos:broader ststs:active ;
    skos:definition "A site such as a mine or quarry which is approved for production."@en ;
    skos:inScheme <http://linked.data.gov.au/def/site-status> ;
    skos:prefLabel "Approved"@en .

ststs:borehole-status a skos:Collection ;
    skos:definition "Project statuses pertaining to the construction, usage, maintenance and abandonment of a well or bore."@en ;
    skos:member ststs:cased-and-suspended,
        ststs:completed,
        ststs:construction,
        ststs:monitoring,
        ststs:never-used,
        ststs:on-injection,
        ststs:on-production,
        ststs:plugged-and-abandoned,
        ststs:proposed,
        ststs:suspended,
        ststs:unknown,
        ststs:water-supply ;
    skos:prefLabel "Borehole Status"@en .

ststs:minocc a skos:Collection ;
    skos:definition "Project statuses pertaining to the operational lifecycle of a mineral occurence or mine."@en ;
    skos:member ststs:active,
        ststs:abandoned,
        ststs:application,
        ststs:approved,
        ststs:care-and-maintenance,
        ststs:construction,
        ststs:inactive,
        ststs:never-used,
        ststs:not-producing,
        ststs:on-hold,
        ststs:on-production,
        ststs:operational-non-prod,
        ststs:proposed,
        ststs:rehabilitation,
        ststs:secondary-operation,
        ststs:suspended,
        ststs:unknown ;
    skos:prefLabel "Minocc"@en .

ststs:minprodstat a skos:Collection ;
    skos:definition "The coarse status of a mineral mine as pertains to activity on a reporting basis. Such as the status of a mine sub-site, e.g. Mining Lease X is currently not producing and contributing to mine production within Mine A, which is still an active project."@en ;
    skos:member ststs:on-production,
        ststs:operational-non-prod,
        ststs:secondary-operation,
        ststs:not-producing ;
    skos:prefLabel "Mineral Production Sub-Site Status"@en .

ststs:prodstat a skos:Collection ;
    skos:definition "The coarse status of a coal mine as pertains to activity on a reporting basis. Such as the status of a mine sub-site, e.g. Mining Lease X is currently not producing and contributing to mine production within Mine A, which is still an active project."@en ;
    skos:member ststs:on-production,
        ststs:not-producing ;
    skos:prefLabel "Coal Production Sub-Site Status"@en .

ststs:quarry-status a skos:Collection ;
    skos:definition "The valid site statuses as applies to quarries in Queensland."@en ;
    skos:member ststs:active,
        ststs:application,
        ststs:approved,
        ststs:suspended,
        ststs:on-hold ;
    skos:prefLabel "Quarry Status"@en .
