@prefix strel: <http://linked.data.gov.au/def/site-relationships/> .
@prefix dc: <http://purl.org/dc/elements/1.1/> .
@prefix dcterms: <http://purl.org/dc/terms/> .
@prefix owl: <http://www.w3.org/2002/07/owl#> .
@prefix sdo: <http://schema.org/> .
@prefix skos: <http://www.w3.org/2004/02/skos/core#> .
@prefix rdfs: <http://www.w3.org/2000/01/rdf-schema#> .
@prefix xsd: <http://www.w3.org/2001/XMLSchema#> .

<http://linked.data.gov.au/def/site-relationships> a owl:Ontology , skos:ConceptScheme ;
    dcterms:creator <http://linked.data.gov.au/org/gsq> ;
    dcterms:created "2020-01-21"^^xsd:date ;
    dcterms:modified "2022-02-17"^^xsd:date ;
    dcterms:publisher <http://linked.data.gov.au/org/gsq> ;
    dcterms:provenance "Compiled by the Geological Survey of Queensland" ;
    skos:definition """The relationships between sites both topological and functional. See https://pro.arcgis.com/en/pro-app/latest/tool-reference/big-data-analytics/spatial-relationships-with-big-data.htm for visual representations of spatial relationships."""@en ;
    skos:hasTopConcept strel:above,
        strel:after,
        strel:before,
        strel:below,
        strel:boreholeIntersect,
        strel:contains,
        strel:covers,
        strel:crosses,
        strel:disjoint,
        strel:equals,
        strel:injectionExtractionPair,
        strel:hasPart,
        strel:touches,
        strel:observation,
        strel:overlaps,
        strel:intersects,
        strel:parent,
        strel:partOf,
        strel:permits,
        strel:hasPermit,
        strel:re-entry,
        strel:redrill,
        strel:supersedes,
        strel:twinned,
        strel:within,
        strel:wellPad ;
    skos:prefLabel "Site Relationships"@en .

<http://linked.data.gov.au/org/gsq>
    a sdo:Organization ;
    sdo:name "Geological Survey of Queensland" ;
    sdo:url "http://www.business.qld.gov.au/industries/mining-energy-water/resources/geoscience-information/gsq"^^xsd:anyURI .

 strel:geologicalFeature a skos:Collection ;
    skos:definition "The relationship between two geological features, for example: Stratigraphically (‘vertically’) at a boundary in common between two rock units of the same type/kind (lithostratigraphic, biostratigraphic, etc.); laterally (geographically) between two lithologic rock units with a gradational change in lithology, or laterally between two rock units with an abrupt change in lithologic or biostratigraphic facies; and lithostratigraphically or biostratigraphically (both from a geographic perspective), based respectively on lithostratigraphic or biostratigraphic correlation. Not only included are relationships between any two types of lithologic rock units, such as between two stratiform (lithostratigraphic) units or between two nonstratiform (non-lithostratigraphic) units, but also between a stratiform unit and a nonstratiform unit, such as an intrusive rock unit."@en ;
    #skos:member strel:hasPart, <<<<<<<<<<<<<<<<<<<<< NB#
        #strel:partOf,<<<<<<<<<<<<<<<<<< NB#
        #strel:??????,#
        #strel:??????,#
        #strel:??????,#
        #strel:??????,#
        #strel:??????,#
        #strel:??????,#
        #strel:?????? ;#

strel:intrudedBy a skos:Concept ;
    skos:definition "Where the lithologic rock unit (which may be an igneous or non-igneous intrusive rock unit) is intruded/cross-cut by an igneous or non-igneous intrusive rock unit."@en ;
    rdfs:isDefinedBy <http://linked.data.gov.au/def/site-relationships> ;
    skos:inScheme <http://linked.data.gov.au/def/site-relationships> ;
    skos:prefLabel "Intruded by"@en ;
    skos:topConceptOf <http://linked.data.gov.au/def/site-relationships> .

    strel:probablyIntrudedBy a skos:Concept ;
    skos:definition "Where the lithologic rock unit is probably intruded by an igneous or non-igneous intrusive rock unit."@en ;
    rdfs:isDefinedBy <http://linked.data.gov.au/def/site-relationships> ;
    skos:inScheme <http://linked.data.gov.au/def/site-relationships> ;
    skos:prefLabel "Probably intruded by"@en ;
    skos:topConceptOf <http://linked.data.gov.au/def/site-relationships> .

strel:intrudes a skos:Concept ;
    skos:definition "Where the igneous or non-igneous intrusive rock unit intrudes/cross-cuts another lithologic rock unit, which may also be an (older) intrusive rock unit."@en ;
    rdfs:isDefinedBy <http://linked.data.gov.au/def/site-relationships> ;
    skos:inScheme <http://linked.data.gov.au/def/site-relationships> ;
    skos:prefLabel "Intrudes"@en ;
    skos:topConceptOf <http://linked.data.gov.au/def/site-relationships> .

    strel:probablyIntrudes a skos:Concept ;
    skos:definition "Where an igneous or non-igneous intrusive rock unit probably intrudes/cross-cuts another lithologic rock unit."@en ;
    rdfs:isDefinedBy <http://linked.data.gov.au/def/site-relationships> ;
    skos:inScheme <http://linked.data.gov.au/def/site-relationships> ;
    skos:prefLabel "Probably intrudes"@en ;
    skos:topConceptOf <http://linked.data.gov.au/def/site-relationships> .

strel:underliesRegolith a skos:Concept ;
    skos:altLabel "Overlain by regolith"@en ;
    skos:definition "Where the lithologic rock unit directly underlies the regolith (i.e., the rock unit is directly overlain by the regolith), to which it may have contributed through the processes of weathering and erosion."@en ;
    rdfs:isDefinedBy <http://linked.data.gov.au/def/site-relationships> ;
    skos:inScheme <http://linked.data.gov.au/def/site-relationships> ;
    skos:prefLabel "Underlies regolith"@en ;
    skos:topConceptOf <http://linked.data.gov.au/def/site-relationships> .

    strel:overlainBy a skos:Concept ;
    skos:altLabel "Underlies"@en ;
    skos:definition "Where the rock unit (e.g., a lithostratigraphic rock unit, biostratigraphic rock unit/zone, etc.) underlies (is overlain by) another lithologic rock unit (of the same kind/type: lithologic, biostratigraphic, etc.) and where the rock units are in stratigraphic order of succession (have not been overturned), and have not been thrusted into their current position; also where there is no detailed assertion of conformity or unconformity between them, with conformity being unknown or uncertain."@en ;
    rdfs:isDefinedBy <http://linked.data.gov.au/def/site-relationships> ;
    skos:inScheme <http://linked.data.gov.au/def/site-relationships> ;
    skos:prefLabel "Overlain by"@en ;
    skos:topConceptOf <http://linked.data.gov.au/def/site-relationships> .

    strel:overlainUnconformablyBy a skos:Concept ;
    skos:altLabel "Unconformably underlies"@en ;
    skos:definition "Where the rock unit (e.g., a lithostratigraphic rock unit, biostratigraphic rock unit/zone, etc.) unconformably underlies (is overlain unconformably) by another rock unit (of the same kind/type: lithologic, biostratigraphic, etc.) and where, apart from hiatus, the rock units are in stratigraphic order of succession (have not been overturned), and have not been thrusted into their current position."@en ;
    rdfs:isDefinedBy <http://linked.data.gov.au/def/site-relationships> ;
    skos:inScheme <http://linked.data.gov.au/def/site-relationships> ;
    skos:prefLabel "Overlain unconformably by"@en ;
    skos:topConceptOf <http://linked.data.gov.au/def/site-relationships> .
    
    strel:overlainConformablyBy a skos:Concept ;
    skos:altLabel "Conformably underlies"@en ;
    skos:definition "Where the rock unit (lithostratigraphic rock unit, biostratigraphic rock unit/zone, etc.) conformably underlies (is conformably overlain by) another rock unit (of the same kind/type: lithologic, biostratigraphic, etc.) and where the rock units are in stratigraphic order of succession (have not been overturned), and have not been thrusted into their current position."@en ;
    rdfs:isDefinedBy <http://linked.data.gov.au/def/site-relationships> ;
    skos:inScheme <http://linked.data.gov.au/def/site-relationships> ;
    skos:prefLabel "Overlain conformably by"@en ;
    skos:topConceptOf <http://linked.data.gov.au/def/site-relationships> .
        
    strel:overlainGradationallyBy a skos:Concept ;
    skos:altLabel "Is gradational into overlying"@en,
    skos:altLabel "Is gradational into conformably overlying"@en ;
    skos:definition "Where the lithologic rock unit is lithologically gradational into the conformably overlying rock unit, and where the rock units are in stratigraphic order of succession (have not been overturned), and have not been thrusted into their current position."@en ;
    rdfs:isDefinedBy <http://linked.data.gov.au/def/site-relationships> ;
    skos:inScheme <http://linked.data.gov.au/def/site-relationships> ;
    skos:prefLabel "Overlain gradationally by"@en ;
    skos:topConceptOf <http://linked.data.gov.au/def/site-relationships> .

    strel:underlainGradationallyBy a skos:Concept ;
    skos:altLabel "Is gradational into underlying"@en,
    skos:altLabel "Is gradational into conformably underlying"@en ;
    skos:definition "Where the lithologic rock unit is lithologically gradational into the conformably underlying rock unit, and where the rock units are in stratigraphic order of succession (have not been overturned), and have not been thrusted into their current position."@en ;
    rdfs:isDefinedBy <http://linked.data.gov.au/def/site-relationships> ;
    skos:inScheme <http://linked.data.gov.au/def/site-relationships> ;
    skos:prefLabel "Overlain gradationally by"@en ;
    skos:topConceptOf <http://linked.data.gov.au/def/site-relationships> .
        
    strel:laterallyGradationalInto a skos:Concept ;
    skos:definition "Where the rock unit is laterally gradational lithologically into to another rock unit."@en ;
    rdfs:isDefinedBy <http://linked.data.gov.au/def/site-relationships> ;
    skos:inScheme <http://linked.data.gov.au/def/site-relationships> ;
    skos:prefLabel "Laterally gradational into"@en ;
    skos:topConceptOf <http://linked.data.gov.au/def/site-relationships> .

    strel:underlainConformablyBy a skos:Concept ;
    skos:altLabel "Conformably overlies"@en ;
    skos:definition "Where the rock unit (lithostratigraphic rock unit, biostratigraphic rock unit/zone, etc.) conformably overlies (is conformably underlain by) by another lithologic rock unit (of the same kind/type: lithologic, biostratigraphic, etc.) and where the rock units are in stratigraphic order of succession (have not been overturned), and have not been thrusted into their current position."@en ;
    rdfs:isDefinedBy <http://linked.data.gov.au/def/site-relationships> ;
    skos:inScheme <http://linked.data.gov.au/def/site-relationships> ;
    skos:prefLabel "Underlain conformably by"@en ;
    skos:topConceptOf <http://linked.data.gov.au/def/site-relationships> .
    
    strel:underlainUnconformablyBy a skos:Concept ;
    skos:altLabel "Unconformably overlies"@en ;
    skos:definition "Where the rock unit (lithostratigraphic rock unit, biostratigraphic rock unit/zone, etc.) unconformably overlies (is underlain unconformably by) another lithologic rock unit (of the same kind/type: lithologic, biostratigraphic, etc.) and where, apart from hiatus, the rock units are in stratigraphic order of succession (have not been overturned), and have not been thrusted into their current position."@en ;
    rdfs:isDefinedBy <http://linked.data.gov.au/def/site-relationships> ;
    skos:inScheme <http://linked.data.gov.au/def/site-relationships> ;
    skos:prefLabel "Underlain conformably by"@en ;
    skos:topConceptOf <http://linked.data.gov.au/def/site-relationships> .
 
    strel:underlainBy a skos:Concept ;
    skos:altLabel "Overlies"@en ;
    skos:definition "Where the rock unit (lithostratigraphic rock unit, biostratigraphic rock unit/zone, etc.) overlies (is underlain by) by another rock unit (of the same kind/type: lithologic, biostratigraphic, etc.) and where the rock units are in stratigraphic order of succession (have not been overturned), and have not been thrusted into their current position; also where there is no detailed assertion of conformity or unconformity between them, with conformity being unknown or uncertain."@en ;
    rdfs:isDefinedBy <http://linked.data.gov.au/def/site-relationships> ;
    skos:inScheme <http://linked.data.gov.au/def/site-relationships> ;
    skos:prefLabel "Underlain by"@en ;
    skos:topConceptOf <http://linked.data.gov.au/def/site-relationships> .

    strel:containsInterleavedThrustSheetsOf a skos:Concept ;
    skos:definition "Where the lithologic rock unit (or other geologic feature) contains thrust sheets of another lithologic rock unit that have been inserted tectonically."@en ;
    rdfs:isDefinedBy <http://linked.data.gov.au/def/site-relationships> ;
    skos:inScheme <http://linked.data.gov.au/def/site-relationships> ;
    skos:prefLabel "Contains interleaved thrust sheets of"@en ;
    skos:topConceptOf <http://linked.data.gov.au/def/site-relationships> .

    strel:interleavedThrustSheetsContainedIn a skos:Concept ;
    skos:definition "Where the interleaved thrust sheets of a lithologic rock unit have been tectonically inserted into another lithologic rock unit."@en ;
    rdfs:isDefinedBy <http://linked.data.gov.au/def/site-relationships> ;
    skos:inScheme <http://linked.data.gov.au/def/site-relationships> ;
    skos:prefLabel "Interleaved thrust sheets of"@en ;
    skos:topConceptOf <http://linked.data.gov.au/def/site-relationships> .

    strel:overlainByThrustNappe a skos:Concept ;
    skos:altLabel "Underlies thrust nappe"@en ;
    skos:definition "Where the lithologic rock unit underlies (is overlain by) an out-of-sequence thrust nappe."@en ;
    rdfs:isDefinedBy <http://linked.data.gov.au/def/site-relationships> ;
    skos:inScheme <http://linked.data.gov.au/def/site-relationships> ;
    skos:prefLabel "Overlain by thrust nappe"@en ;
    skos:topConceptOf <http://linked.data.gov.au/def/site-relationships> .

    strel:thrustNappeOverlying a skos:Concept ;
    skos:definition "Where the out-of-sequence thrust nappe overlies another lithologic rock unit."@en ;
    rdfs:isDefinedBy <http://linked.data.gov.au/def/site-relationships> ;
    skos:inScheme <http://linked.data.gov.au/def/site-relationships> ;
    skos:prefLabel "Thrust nappe overlying"@en ;
    skos:topConceptOf <http://linked.data.gov.au/def/site-relationships> .

    strel:equivalentTo a skos:Concept ;
    skos:definition "Where the lithostratigraphic rock unit is laterally equivalent stratigraphically (lithostratigraphically) to another lithostratigraphic rock unit."@en ;
    rdfs:isDefinedBy <http://linked.data.gov.au/def/site-relationships> ;
    skos:inScheme <http://linked.data.gov.au/def/site-relationships> ;
    skos:prefLabel "Equivalent to"@en ;
    skos:topConceptOf <http://linked.data.gov.au/def/site-relationships> .

    strel:equivalentPartlyTo a skos:Concept ;
    skos:definition "Where the lithostratigraphic rock unit, in part only, is laterally equivalent stratigraphically (lithostratigraphically) to another lithostratigraphic rock unit."@en ;
    rdfs:isDefinedBy <http://linked.data.gov.au/def/site-relationships> ;
    skos:inScheme <http://linked.data.gov.au/def/site-relationships> ;
    skos:prefLabel "Equivalent partly to"@en ;
    skos:topConceptOf <http://linked.data.gov.au/def/site-relationships> .

 strel:faultedAgainst a skos:Concept ;
    skos:definition "Where the lithologic rock unit is faulted against another lithologic rock unit."@en ;
    rdfs:isDefinedBy <http://linked.data.gov.au/def/site-relationships> ;
    skos:inScheme <http://linked.data.gov.au/def/site-relationships> ;
    skos:prefLabel "Faulted against"@en ;
    skos:topConceptOf <http://linked.data.gov.au/def/site-relationships> .

 strel:overlapsOlder a skos:Concept ;
    skos:altLabel "Onlaps"@en ;
    skos:definition "Where the lithologic rock unit extends progressively across an erosion surface, overlapping/onlapping an older/underlying lithologic rock unit."@en ;
    rdfs:isDefinedBy <http://linked.data.gov.au/def/site-relationships> ;
    skos:inScheme <http://linked.data.gov.au/def/site-relationships> ;
    skos:prefLabel "Overlaps older"@en ;
    skos:topConceptOf <http://linked.data.gov.au/def/site-relationships> .

 strel:overlappedBy a skos:Concept ;
    skos:definition "Where the lithologic rock is overlapped by a younger, onlapping lithologic rock unit."@en ;
    rdfs:isDefinedBy <http://linked.data.gov.au/def/site-relationships> ;
    skos:inScheme <http://linked.data.gov.au/def/site-relationships> ;
    skos:prefLabel "Overlapped by"@en ;
    skos:topConceptOf <http://linked.data.gov.au/def/site-relationships> .

 strel:offsteps a skos:Concept ;
    skos:definition "Where the lithologic rock unit sits unconformably on progressively older/underlying lithologic rock units."@en ;
    rdfs:isDefinedBy <http://linked.data.gov.au/def/site-relationships> ;
    skos:inScheme <http://linked.data.gov.au/def/site-relationships> ;
    skos:prefLabel "Offsteps"@en ;
    skos:topConceptOf <http://linked.data.gov.au/def/site-relationships> .

 strel:overliesBasement a skos:Concept ;
    skos:altLabel "Underlain by basement"@en ;
    skos:definition "Where the lithologic rock unit rests on a basement rock unit."@en ;
    rdfs:isDefinedBy <http://linked.data.gov.au/def/site-relationships> ;
    skos:inScheme <http://linked.data.gov.au/def/site-relationships> ;
    skos:prefLabel "Overlies basement"@en ;
    skos:topConceptOf <http://linked.data.gov.au/def/site-relationships> .

 strel:comagmaticWith a skos:Concept ;
    skos:definition "Where the igneous rock unit, based on its chemistry and mineralogic features, is considered to have been derived from the same parent magma as another igneous rock unit (After: mindat.org; accessed 13.09.2022)."@en ;
    rdfs:isDefinedBy <http://linked.data.gov.au/def/site-relationships> ;
    skos:inScheme <http://linked.data.gov.au/def/site-relationships> ;
    skos:prefLabel "Comagmatic with"@en ;
    skos:topConceptOf <http://linked.data.gov.au/def/site-relationships> .
    
strel:relationshipUnknown a skos:Concept ;
    skos:definition "Where the relationship between two geological features is unknown."@en ;
    rdfs:isDefinedBy <http://linked.data.gov.au/def/site-relationships> ;
    skos:inScheme <http://linked.data.gov.au/def/site-relationships> ;
    skos:prefLabel "Relationship unknown"@en ;
    skos:topConceptOf <http://linked.data.gov.au/def/site-relationships> .

strel:intercalatedWith a skos:Concept ;
    skos:definition "Where the lithologic rock unit contains a rock layer or rock layers of a different character, especially where relatively thin strata of one kind of material alternate with thicker strata of some other kind of material, such being the case, for example, with lava flows, beds of shale, and concordant intrusive sills being ‘intercalated’ in a large body of sandstone. Also: The insertion/intercalation by the tectonic thrusting of rock layers into a pre-existing body of stratified rock; or the occurrence of a particular fossil horizon between fossil zones (biostratigraphic rock units) of a different character (After: Gary et al., 1977)."@en ;
    rdfs:isDefinedBy <http://linked.data.gov.au/def/site-relationships> ;
    skos:inScheme <http://linked.data.gov.au/def/site-relationships> ;
    skos:prefLabel "Intercalated with"@en ;
    skos:topConceptOf <http://linked.data.gov.au/def/site-relationships> .

strel:intertonguedWith a skos:Concept ;
    skos:altLabel "Interfingered with"@en,
    skos:altLabel "Interdigitated with"@en ;
    skos:definition "Where the contact between laterally adjacent rock bodies breaks down into a series of wedges or tongues that penetrate the adjacent rock body and pinch out individually, essentially embracing the ‘disappearance’ of both rock bodies (After: Gary et al., 1977; Wikipedia [Contact (geology)], accessed 07.09.2022)."@en ;
    rdfs:isDefinedBy <http://linked.data.gov.au/def/site-relationships> ;
    skos:inScheme <http://linked.data.gov.au/def/site-relationships> ;
    skos:prefLabel "Intertongued with"@en ;
    skos:topConceptOf <http://linked.data.gov.au/def/site-relationships> .

strel:borehole a skos:Collection ;
    skos:definition "Relationships between associated boreholes and boreholes with other operational sites such as well pads, and hasPart relationships with constituent wellbores."@en ;
    skos:member strel:boreholeIntersect,
        strel:injectionExtractionPair,
        strel:observation,
        strel:re-entry,
        strel:redrill,
        strel:twinned,
        strel:wellPad,
        strel:hasPart ;
    skos:prefLabel "Borehole"@en .

strel:interval a skos:Collection ;
    skos:definition "Relationships between intervals where vertical offset is the defining factor. Typically used for within a well or bore."@en ;
    skos:member strel:above,
        strel:below,
        strel:contains,
        strel:overlaps,
        strel:covers,
        strel:disjoint,
        strel:equals,
        strel:touches,
        strel:intersects ;
    skos:prefLabel "Interval"@en .

strel:topological a skos:Collection ;
    skos:definition "Topology deals with spatial and structural properties of geometric objects, independent of their extension, type, or geometric form. Among the types of topological properties of objects there are: the number of dimensions an object has or the relationships that exist between objects."@en ;
    skos:member strel:contains,
        strel:covers,
        strel:crosses,
        strel:disjoint,
        strel:equals,
        strel:overlaps,
        strel:touches,
        strel:intersects,
        strel:within ;
    skos:prefLabel "Topological"@en .

strel:project a skos:Collection ;
    skos:definition "Spatial and temporal relationships between spatially bound project locations (sites)."@en ;
    skos:member strel:contains,
        strel:covers,
        strel:crosses,
        strel:disjoint,
        strel:equals,
        strel:touches,
        strel:intersects,
        strel:overlaps,
        strel:within,
        strel:hasPart,
        strel:partOf,
        strel:before,
        strel:after,
        strel:concurrent ;
    skos:prefLabel "Project"@en .

strel:temporal a skos:Collection ;
    skos:definition "Temporal relationships between projects and activities that are spatially bound as sites."@en ;
    skos:member strel:supersedes,
        strel:before,
        strel:after,
        strel:concurrent ;
    skos:prefLabel "Temporal"@en .

strel:wellbore a skos:Collection ;
    skos:definition "Defines the parent-child relationship of wellbores that constitute a borehole."@en ;
    skos:member strel:parent ;
    skos:prefLabel "Wellbore"@en .

strel:above a skos:Concept ;
    skos:definition "Object or interval A is above object or interval B."@en ;
    rdfs:isDefinedBy <http://linked.data.gov.au/def/site-relationships> ;
    skos:inScheme <http://linked.data.gov.au/def/site-relationships> ;
    skos:prefLabel "Above"@en ;
    skos:topConceptOf <http://linked.data.gov.au/def/site-relationships> .

strel:after a skos:Concept ;
    skos:definition "A spatially bound project follows or continues after the related project. Where times overlap used in conjunction with Concurrent relationship."@en ;
    rdfs:isDefinedBy <http://linked.data.gov.au/def/site-relationships> ;
    skos:inScheme <http://linked.data.gov.au/def/site-relationships> ;
    skos:prefLabel "After"@en ;
    skos:topConceptOf <http://linked.data.gov.au/def/site-relationships> .

strel:before a skos:Concept ;
    skos:definition "A spatially bound project precedes or begins prior to the related project. Where times overlap used in conjunction with Concurrent relationship."@en ;
    rdfs:isDefinedBy <http://linked.data.gov.au/def/site-relationships> ;
    skos:inScheme <http://linked.data.gov.au/def/site-relationships> ;
    skos:prefLabel "Before"@en ;
    skos:topConceptOf <http://linked.data.gov.au/def/site-relationships> .

strel:concurrent a skos:Concept ;
    skos:definition "A spatially bound project that occurs partially or fully at the same time as the related project."@en ;
    rdfs:isDefinedBy <http://linked.data.gov.au/def/site-relationships> ;
    skos:inScheme <http://linked.data.gov.au/def/site-relationships> ;
    skos:prefLabel "Concurrent"@en ;
    skos:topConceptOf <http://linked.data.gov.au/def/site-relationships> .

strel:below a skos:Concept ;
    skos:definition "Object or interval A is below object or interval B."@en ;
    rdfs:isDefinedBy <http://linked.data.gov.au/def/site-relationships> ;
    skos:inScheme <http://linked.data.gov.au/def/site-relationships> ;
    skos:prefLabel "Below"@en ;
    skos:topConceptOf <http://linked.data.gov.au/def/site-relationships> .

strel:crosses a skos:Concept ;
    skos:definition "Line A intersects Line B at points only. Or, Line A is partially inside and partially outside Polygon X"@en ;
    rdfs:isDefinedBy <http://linked.data.gov.au/def/site-relationships> ;
    skos:inScheme <http://linked.data.gov.au/def/site-relationships> ;
    skos:prefLabel "Crosses"@en ;
    skos:topConceptOf <http://linked.data.gov.au/def/site-relationships> .

strel:boreholeIntersect a skos:Concept ;
    skos:definition "A well that intersects the subject well."@en ;
    rdfs:isDefinedBy <http://linked.data.gov.au/def/site-relationships> ;
    skos:inScheme <http://linked.data.gov.au/def/site-relationships> ;
    skos:prefLabel "Borehole Intersect"@en ;
    skos:topConceptOf <http://linked.data.gov.au/def/site-relationships> .

strel:injectionExtractionPair a skos:Concept ;
    skos:definition "Wells that exist in a pair, or system, in which a well or wells inject fluids and one or more offset wells extract fluids. Such as stimulated production, enhanced geothermale etc."@en ;
    rdfs:isDefinedBy <http://linked.data.gov.au/def/site-relationships> ;
    skos:inScheme <http://linked.data.gov.au/def/site-relationships> ;
    skos:prefLabel "Injection-Extraction Pair"@en ;
    skos:topConceptOf <http://linked.data.gov.au/def/site-relationships> .

strel:observation a skos:Concept ;
    skos:altLabel "Monitoring"@en ;
    skos:definition "A borehole drilled for the observation or monitoring of the subject well or bore"@en ;
    rdfs:isDefinedBy <http://linked.data.gov.au/def/site-relationships> ;
    skos:inScheme <http://linked.data.gov.au/def/site-relationships> ;
    skos:prefLabel "Observation"@en ;
    skos:topConceptOf <http://linked.data.gov.au/def/site-relationships> .

strel:parent a skos:Concept ;
    skos:definition "The parent wellbore that the subject wellbore originated from."@en ;
    rdfs:isDefinedBy <http://linked.data.gov.au/def/site-relationships> ;
    skos:inScheme <http://linked.data.gov.au/def/site-relationships> ;
    skos:prefLabel "Has parent"@en ;
    skos:topConceptOf <http://linked.data.gov.au/def/site-relationships> .

strel:partOf a skos:Concept ;
    skos:definition "Entity A (the subject site) is a discrete object that forms part of the larger Entity B (the related site). Subject Site is partOf Related Site."@en ;
    skos:example "Suburb (subject site) partOf City (Related Site)"@en ;
    owl:inverseOf strel:hasPart ;
    rdfs:isDefinedBy <http://linked.data.gov.au/def/site-relationships> ;
    skos:inScheme <http://linked.data.gov.au/def/site-relationships> ;
    skos:prefLabel "Part Of"@en ;
    skos:topConceptOf <http://linked.data.gov.au/def/site-relationships> .

strel:hasPart a skos:Concept ;
    skos:definition "Entity A (the subject site) is a discrete object that has a consitutent part of Entity B (the related site). Subject Site hasPart Related Site."@en ;
    owl:inverseOf strel:partOf ;
    skos:example "City (subject site) hasPart Suburb (Related Site)"@en ;
    rdfs:isDefinedBy <http://linked.data.gov.au/def/site-relationships> ;
    skos:inScheme <http://linked.data.gov.au/def/site-relationships> ;
    skos:prefLabel "Has Part"@en ;
    skos:topConceptOf <http://linked.data.gov.au/def/site-relationships> .

strel:permits a skos:Concept ;
    skos:definition "The sites permitted to conduct activities under the license or authority issued under a legislation or regulation."@en ;
    rdfs:isDefinedBy <http://linked.data.gov.au/def/site-relationships> ;
    skos:inScheme <http://linked.data.gov.au/def/site-relationships> ;
    skos:scopeNote """This concept uses the verb 'permits'. The noun 'permit' is a GeoAdmin Feature concept defined at http://linked.data.gov.au/def/geoadminfeatures/permit"""@en ;
    skos:prefLabel "Permits"@en ;
    skos:topConceptOf <http://linked.data.gov.au/def/site-relationships> .

strel:hasPermit a skos:Concept ;
    skos:definition "Activities conducted at a site may be governed by a permit, license or authority issued under legislation or regulation. This concept is the inverse of Permits."@en ;
    rdfs:isDefinedBy <http://linked.data.gov.au/def/site-relationships> ;
    skos:inScheme <http://linked.data.gov.au/def/site-relationships> ;
    skos:prefLabel "Has permit"@en ;
    skos:topConceptOf <http://linked.data.gov.au/def/site-relationships> .

strel:re-entry a skos:Concept ;
    skos:definition "A previously abandoned well that the subject well drilled from within. A re-entry drills out or removes any abandonment plugs or equipment from the previously abandoned well."@en ;
    rdfs:isDefinedBy <http://linked.data.gov.au/def/site-relationships> ;
    skos:inScheme <http://linked.data.gov.au/def/site-relationships> ;
    skos:prefLabel "Re-Entry"@en ;
    skos:topConceptOf <http://linked.data.gov.au/def/site-relationships> .

strel:redrill a skos:Concept ;
    skos:altLabel "Offset"@en ;
    skos:definition "A well in which drilling was abandoned that the subject well is drilled at an offset position to as a direct replacement. A redrill is drilled with the same intended target(s) and commonly the same general design."@en ;
    rdfs:isDefinedBy <http://linked.data.gov.au/def/site-relationships> ;
    skos:inScheme <http://linked.data.gov.au/def/site-relationships> ;
    skos:prefLabel "Redrill"@en ;
    skos:topConceptOf <http://linked.data.gov.au/def/site-relationships> .

strel:twinned a skos:Concept ;
    skos:definition "A twin of the subject well. A hole drilled separate to but in support of the subject wells purpose and intent."@en ;
    rdfs:isDefinedBy <http://linked.data.gov.au/def/site-relationships> ;
    skos:inScheme <http://linked.data.gov.au/def/site-relationships> ;
    skos:prefLabel "Twinned"@en ;
    skos:topConceptOf <http://linked.data.gov.au/def/site-relationships> .

strel:wellPad a skos:Concept ;
    skos:definition "The well pad site from which a batch of wells or bores share a single operational area at surface but drill to different sub-surface targets."@en ;
    rdfs:isDefinedBy <http://linked.data.gov.au/def/site-relationships> ;
    skos:inScheme <http://linked.data.gov.au/def/site-relationships> ;
    skos:prefLabel "Well Pad"@en ;
    skos:topConceptOf <http://linked.data.gov.au/def/site-relationships> .

strel:contains a skos:Concept ;
    skos:definition "Object A contains Object B, and the boundaries do not intersect, i.e. Object A (the subject site), wholly encompasses Object B (the related site), in such a way that the boundary of Object A is outside-and-does-not-touch the boundary of Object B. The inverse of Within."@en ;
    rdfs:isDefinedBy <http://linked.data.gov.au/def/site-relationships> ;
    skos:inScheme <http://linked.data.gov.au/def/site-relationships> ;
    owl:inverseOf strel:within ;
    skos:prefLabel "Contains"@en ;
    skos:scopeNote "Use of strel:contains in a ternary relationship (A related_to B, related_to of type strel:contains) entails A geo:sfContains B"@en ;
    skos:topConceptOf <http://linked.data.gov.au/def/site-relationships> .

strel:within a skos:Concept ;
    skos:definition "Object A is within object B, and the boundaries do not intersect. The inverse of Contains."@en ;
    rdfs:isDefinedBy <http://linked.data.gov.au/def/site-relationships> ;
    skos:inScheme <http://linked.data.gov.au/def/site-relationships> ;
    owl:inverseOf strel:contains ;
    skos:prefLabel "Within"@en ;
    skos:topConceptOf <http://linked.data.gov.au/def/site-relationships> .

strel:covers a skos:Concept ;
    skos:definition "Object A covers object B, and the boundaries intersect."@en ;
    rdfs:isDefinedBy <http://linked.data.gov.au/def/site-relationships> ;
    skos:inScheme <http://linked.data.gov.au/def/site-relationships> ;
    skos:prefLabel "Covers"@en ;
    skos:topConceptOf <http://linked.data.gov.au/def/site-relationships> .

strel:disjoint a skos:Concept ;
    skos:definition "There is no intersection area between object A and object B."@en ;
    rdfs:isDefinedBy <http://linked.data.gov.au/def/site-relationships> ;
    skos:inScheme <http://linked.data.gov.au/def/site-relationships> ;
    skos:prefLabel "Disjoint"@en ;
    skos:scopeNote "Use of strel:disjoint in a ternary relationship (A related_to B, related_to of type strel:disjoint) entails A geo:sfDisjoint B"@en ;
    skos:topConceptOf <http://linked.data.gov.au/def/site-relationships> .

strel:equals a skos:Concept ;
    skos:definition "Object B and object A match."@en ;
    rdfs:isDefinedBy <http://linked.data.gov.au/def/site-relationships> ;
    skos:inScheme <http://linked.data.gov.au/def/site-relationships> ;
    skos:prefLabel "Equals"@en ;
    skos:scopeNote "Use of strel:equals in a ternary relationship (A related_to B, related_to of type strel:equals) entails A geo:sfEquals B"@en ;
    skos:topConceptOf <http://linked.data.gov.au/def/site-relationships> .

strel:touches a skos:Concept ;
    skos:altLabel "Meets"@en ;
    skos:definition "Object A and object B touch at the boundary."@en ;
    rdfs:isDefinedBy <http://linked.data.gov.au/def/site-relationships> ;
    skos:inScheme <http://linked.data.gov.au/def/site-relationships> ;
    skos:prefLabel "Touches"@en ;
    skos:scopeNote "Use of strel:touches in a ternary relationship (A related_to B, related_to of type strel:touches) entails A geo:sfTouches B"@en ;
    skos:topConceptOf <http://linked.data.gov.au/def/site-relationships> .

strel:intersects a skos:Concept ;
    skos:definition "Object A and B intersect spatially."@en ;
    rdfs:isDefinedBy <http://linked.data.gov.au/def/site-relationships> ;
    skos:inScheme <http://linked.data.gov.au/def/site-relationships> ;
    skos:prefLabel "Intersects"@en ;
    skos:scopeNote "Use of strel:intersects in a ternary relationship (A related_to B, related_to of type strel:intersects) entails A geo:sfIntersects B"@en ;
    skos:topConceptOf <http://linked.data.gov.au/def/site-relationships> .

strel:overlaps a skos:Concept ;
    skos:definition "Object A and B are the same geometry type (point, line, or polygon), the intersection is the same geometry type, and the intersection is distinct from each object."@en ;
    rdfs:isDefinedBy <http://linked.data.gov.au/def/site-relationships> ;
    skos:inScheme <http://linked.data.gov.au/def/site-relationships> ;
    skos:prefLabel "Overlaps"@en ;
    skos:topConceptOf <http://linked.data.gov.au/def/site-relationships> .

strel:supersedes a skos:Concept ;
    skos:definition "Object A supersedes object B. A temporal relationship whereby Object A follows, and is a direct result of the cessation of, Object B."@en ;
    rdfs:isDefinedBy <http://linked.data.gov.au/def/site-relationships> ;
    skos:inScheme <http://linked.data.gov.au/def/site-relationships> ;
    skos:prefLabel "Supersedes"@en ;
    skos:scopeNote """In the context of resource regulation, supersedes applies to the transition from an exploration permit to a 'higher tenure', such as a Mining Lease"""@en ;
    skos:topConceptOf <http://linked.data.gov.au/def/site-relationships> .
