PREFIX agldwgstatus: <https://linked.data.gov.au/def/reg-statuses/>
PREFIX cs: <http://linked.data.gov.au/def/site-detail-type>
PREFIX dcterms: <http://purl.org/dc/terms/>
PREFIX owl: <http://www.w3.org/2002/07/owl#>
PREFIX rdfs: <http://www.w3.org/2000/01/rdf-schema#>
PREFIX reg: <http://purl.org/linked-data/registry#>
PREFIX sdo: <https://schema.org/>
PREFIX skos: <http://www.w3.org/2004/02/skos/core#>
PREFIX stdt: <http://linked.data.gov.au/def/site-detail-type/>
PREFIX xsd: <http://www.w3.org/2001/XMLSchema#>

stdt:collaborative-drilling-initiative-well
    a skos:Concept ;
    skos:historyNote "Compiled by the Geological Survey of Queensland" ;
    rdfs:isDefinedBy cs: ;
    skos:altLabel "Collaborative Exploration Initiative Well"@en ;
    skos:definition "Whether the borehole was partly or wholly funded through the Collaborative Drilling Initiative."@en ;
    skos:inScheme cs: ;
    skos:prefLabel "Collaborative Drilling Initiative Well"@en ;
    skos:topConceptOf cs: ;
.

stdt:confidential
    a skos:Concept ;
    skos:historyNote "Compiled by the Geological Survey of Queensland" ;
    rdfs:isDefinedBy cs: ;
    skos:definition "Whether the details pertaining to the entity are confidential records."@en ;
    skos:inScheme cs: ;
    skos:prefLabel "Confidential"@en ;
    skos:topConceptOf cs: ;
.

stdt:critical-minerals-project-site
    a skos:Concept ;
    skos:historyNote "Compiled by the Geological Survey of Queensland" ;
    rdfs:isDefinedBy cs: ;
    skos:definition "A yes/no, Y/N, True/False flag indicating that a site is considered a critical minerals project. Used to indicate where a Project, mine complex, or site agglomeration, is used considered to be a Critical Mineral Project. For example where a mining project recovers as a primary or secondary product, any mineral considered to be critical in Schedule 4A of the Mineral Resources Regulation 2017 ."@en ;
    skos:inScheme cs: ;
    skos:prefLabel "Critical Minerals Project Site"@en ;
    skos:topConceptOf cs: ;
.
stdt:date-confidence
    a skos:Concept ;
    skos:historyNote "Compiled by the Geological Survey of Queensland" ;
    rdfs:isDefinedBy cs: ;
    skos:definition "The confidence in the accuracy of a recorded date or dates. Includes notes for where dates are estimated or calculated."@en ;
    skos:inScheme cs: ;
    skos:prefLabel "Date Confidence"@en ;
    skos:topConceptOf cs: ;
.

stdt:drill-result
    a skos:Concept ;
    skos:historyNote "Compiled by the Geological Survey of Queensland" ;
    rdfs:isDefinedBy cs: ;
    skos:definition "The result of hydrocarbon shows, presence of water, or presence of coal in a borehole."@en ;
    skos:inScheme cs: ;
    skos:prefLabel "Drill Result"@en ;
    skos:topConceptOf cs: ;
.

stdt:extent-of-workings
    a skos:Concept ;
    skos:historyNote "Compiled by the Geological Survey of Queensland" ;
    rdfs:isDefinedBy cs: ;
    skos:definition "The approximate spatial extent (length, width, and height) of mine works or diggings that exist at a site. "@en ;
    skos:inScheme cs: ;
    skos:prefLabel "Extent of workings"@en ;
    skos:scopeNote "May be an observation of a site, rather than a site attribute in future release."@en ;
    skos:topConceptOf cs: ;
.

stdt:locality
    a skos:Concept ;
    skos:historyNote "Compiled by the Geological Survey of Queensland" ;
    rdfs:isDefinedBy cs: ;
    skos:definition "Approximate location with respect to a nearby landmark or feature, be it a homestead, crossroads, town or city."@en ;
    skos:inScheme cs: ;
    skos:prefLabel "Locality"@en ;
    skos:topConceptOf cs: ;
.

stdt:location-accuracy
    a skos:Concept ;
    skos:historyNote "Compiled by the Geological Survey of Queensland" ;
    rdfs:isDefinedBy cs: ;
    skos:definition "The accuracy or uncertainty range for stated location i.e. the distance from which the stated location may diverge from the actual location."@en ;
    skos:inScheme cs: ;
    skos:prefLabel "Location Accuracy"@en ;
    skos:scopeNote "May be a spatial, rather than a site attribute in a future release."@en ;
    skos:topConceptOf cs: ;
.

stdt:location-method
    a skos:Concept ;
    skos:historyNote "Compiled by the Geological Survey of Queensland" ;
    rdfs:isDefinedBy cs: ;
    skos:definition "The survey or activity method that was used to locate the site."@en ;
    skos:inScheme cs: ;
    skos:prefLabel "Location Method"@en ;
    skos:scopeNote "May be a spatial, rather than a site attribute in a future release."@en ;
    skos:topConceptOf cs: ;
.

stdt:original-crs
    a skos:Concept ;
    skos:historyNote "Compiled by the Geological Survey of Queensland" ;
    rdfs:isDefinedBy cs: ;
    skos:definition "The original Coordinate Reference System of recorded location information."@en ;
    skos:inScheme cs: ;
    skos:prefLabel "Original CRS"@en ;
    skos:scopeNote "For use in data migration. Used for data previously stored in MERLIN that was converted to GDA94 in 2005."@en ;
    skos:topConceptOf cs: ;
.

stdt:reporting-site
    a skos:Concept ;
    skos:historyNote "Compiled by the Geological Survey of Queensland" ;
    rdfs:isDefinedBy cs: ;
    skos:definition "A yes/no, Y/N, True/False flag indicating that a site is considered a reporting entity. Used to indicate where a Project, mine complex, or site agglomeration, is used to report or refer to many sub-sites. For example where a mining project reports on multiple mines within and contributing to the project."@en ;
    skos:inScheme cs: ;
    skos:prefLabel "Reporting Site"@en ;
    skos:topConceptOf cs: ;
.

stdt:site-phone
    a skos:Concept ;
    skos:historyNote "Compiled by the Geological Survey of Queensland" ;
    rdfs:isDefinedBy cs: ;
    skos:definition "The contact phone number associated with a site, such as a mine or quarry, during operation."@en ;
    skos:inScheme cs: ;
    skos:prefLabel "Site Contact Phone"@en ;
    skos:topConceptOf cs: ;
.

<https://linked.data.gov.au/org/gsq>
    a sdo:Organization ;
    sdo:name "Geological Survey of Queensland" ;
    sdo:url "http://www.business.qld.gov.au/industries/mining-energy-water/resources/geoscience-information/gsq"^^xsd:anyURI ;
.

cs:
    a
        owl:Ontology ,
        skos:ConceptScheme ;
    dcterms:created "2020-03-30"^^xsd:date ;
    dcterms:creator <https://linked.data.gov.au/org/gsq> ;
    dcterms:modified "2023-03-16"^^xsd:date ;
    skos:historyNote "Compiled by the Geological Survey of Queensland" ;
    dcterms:publisher <https://linked.data.gov.au/org/gsq> ;
    reg:status agldwgstatus:stable ;
    skos:definition "Miscellaneous Site Details."@en ;
    skos:hasTopConcept
        stdt:collaborative-drilling-initiative-well ,
        stdt:confidential ,
        stdt:date-confidence ,
        stdt:drill-result ,
        stdt:extent-of-workings ,
        stdt:locality ,
        stdt:location-accuracy ,
        stdt:location-method ,
        stdt:original-crs ,
        stdt:reporting-site ,
        stdt:site-phone ;
    skos:prefLabel "Site Detail Type"@en ;
.

