PREFIX agldwgstatus: <https://linked.data.gov.au/def/reg-statuses/>
PREFIX cs: <http://linked.data.gov.au/def/survey-detail-type>
PREFIX dcterms: <http://purl.org/dc/terms/>
PREFIX owl: <http://www.w3.org/2002/07/owl#>
PREFIX rdfs: <http://www.w3.org/2000/01/rdf-schema#>
PREFIX reg: <http://purl.org/linked-data/registry#>
PREFIX sdo: <https://schema.org/>
PREFIX skos: <http://www.w3.org/2004/02/skos/core#>
PREFIX svydt: <http://linked.data.gov.au/def/survey-detail-type/>
PREFIX xsd: <http://www.w3.org/2001/XMLSchema#>

svydt:airborne-geophysics
    a skos:Collection ;
    skos:historyNote "Compiled by the Geological Survey of Queensland" ;
    skos:definition "Additional details that describe Airborne Geophysics surveys."@en ;
    skos:member
        svydt:ag-survey-type ,
        svydt:comments ,
        svydt:funding-program ,
        svydt:interval-m ,
        svydt:job-number ,
        svydt:line-direction-degrees ,
        svydt:survey-height-m ,
        svydt:tie-interval-m ,
        svydt:tie-line-direction-degrees ,
        svydt:total-area-square-kilometres,
        svydt:total-line-kilometres ,
        svydt:vessel-name ;
    skos:prefLabel "Airborne Geophysics"@en ;
.

svydt:airborne-spectral
    a skos:Collection ;
    skos:historyNote "Compiled by the Geological Survey of Queensland" ;
    skos:definition "Additional details that describe Airborne Spectral surveys."@en ;
    skos:member
        svydt:comments ,
        svydt:funding-program ,
        svydt:interval-m ,
        svydt:job-number ,
        svydt:line-direction-degrees ,
        svydt:survey-height-m ,
        svydt:tie-interval-m ,
        svydt:tie-line-direction-degrees ,
        svydt:total-area-square-kilometres,
        svydt:total-line-kilometres ,
        svydt:vessel-name ;
    skos:prefLabel "Airborne Spectral"@en ;
.

svydt:ground-geophysics
    a skos:Collection ;
    skos:historyNote "Compiled by the Geological Survey of Queensland" ;
    skos:definition "Additional details that describe Ground Geophysics surveys."@en ;
    skos:member
        svydt:comments ,
        svydt:funding-program ,
        svydt:interval-m ,
        svydt:job-number ,
        svydt:survey-line ,
        svydt:total-stations ;
    skos:prefLabel "Ground Geophysics"@en ;
.

svydt:seismic-surveys
    a skos:Collection ;
    skos:historyNote "Compiled by the Geological Survey of Queensland" ;
    skos:definition "Additional details that describe Seismic Surveys surveys."@en ;
    skos:member
        svydt:comments ,
        svydt:funding-program ,
        svydt:job-number ,
        svydt:survey-line ,
        svydt:total-area-square-kilometres,
        svydt:total-line-kilometres ;
    skos:prefLabel "Seismic Surveys"@en ;
.

svydt:survey-plans
    a skos:Collection ;
    skos:historyNote "Compiled by the Geological Survey of Queensland" ;
    skos:definition "Additional details that describe Survey Plans."@en ;
    skos:member
        svydt:comments ,
        svydt:historic-tenure ,
        svydt:historic-title ,
        svydt:locality ;
    skos:prefLabel "Survey Plans"@en ;
.

svydt:active-period
    a skos:Concept ;
    skos:historyNote "Compiled by the Geological Survey of Queensland" ;
    rdfs:isDefinedBy cs: ;
    skos:definition "The number of days during the reporting period (month) on which production occurred."@en ;
    skos:inScheme cs: ;
    skos:prefLabel "Active Period"@en ;
    skos:topConceptOf cs: ;
.

svydt:full-time-contractors
    a skos:Concept ;
    skos:historyNote "Compiled by the Geological Survey of Queensland" ;
    rdfs:isDefinedBy cs: ;
    skos:altLabel
        "FTE Contractors"@en ,
        "Full-Time (FTE) Equivalent Contractors"@en ,
        "Full-time equivalent contractors"@en ;
    skos:definition "The full-time equivalent (FTE) number of contract workers (contractors) working on a project throughout the reporting period."@en ;
    skos:inScheme cs: ;
    skos:prefLabel "Full-Time Equivalent Contractors"@en ;
    skos:topConceptOf cs: ;
.

svydt:full-time-employees
    a skos:Concept ;
    skos:historyNote "Compiled by the Geological Survey of Queensland" ;
    rdfs:isDefinedBy cs: ;
    skos:altLabel
        "FTE Employees"@en ,
        "Full-Time (FTE) Equivalent Employees"@en ,
        "Full-time equivalent employees"@en ;
    skos:definition "The full-time equivalent (FTE) number of employees working on a project throughout the reporting period."@en ;
    skos:inScheme cs: ;
    skos:prefLabel "Full-Time Equivalent Employees"@en ;
    skos:topConceptOf cs: ;
.

svydt:report-period-freight-cost
    a skos:Concept ;
    skos:historyNote "Compiled by the Geological Survey of Queensland" ;
    rdfs:isDefinedBy cs: ;
    skos:definition "The total freight charged to the reporting mine during the reporting period (AUD)"@en ;
    skos:inScheme cs: ;
    skos:prefLabel "Report Period Freight Cost"@en ;
    skos:topConceptOf cs: ;
.

svydt:ag-survey-type
    a skos:Concept ;
    skos:historyNote "Compiled by the Geological Survey of Queensland" ;
    rdfs:isDefinedBy cs: ;
    skos:definition "Airborne geophysical survey type (exploration, government, open range, multi-client or experimental)"@en ;
    skos:inScheme cs: ;
    skos:prefLabel "AG Survey Type"@en ;
    skos:topConceptOf cs: ;
.

svydt:historic-tenure
    a skos:Concept ;
    skos:historyNote "Compiled by the Geological Survey of Queensland" ;
    rdfs:isDefinedBy cs: ;
    skos:altLabel
        "Historic Permit"@en ,
        "Legacy Permit"@en ,
        "Legacy Tenure"@en ,
        "Previous System Tenure"@en ;
    skos:definition "A legacy tenure or permit identifier that is not in current usage."@en ;
    skos:inScheme cs: ;
    skos:prefLabel "Historic Tenure"@en ;
    skos:topConceptOf cs: ;
.

svydt:historic-title
    a skos:Concept ;
    skos:historyNote "Compiled by the Geological Survey of Queensland" ;
    rdfs:isDefinedBy cs: ;
    skos:altLabel
        "Former Plan Number"@en ,
        "Legacy Title"@en ;
    skos:definition "A previous title or reference to the survey or document that has been edited, amended, or replaced."@en ;
    skos:inScheme cs: ;
    skos:prefLabel "Historic Title"@en ;
    skos:topConceptOf cs: ;
.

svydt:locality
    a skos:Concept ;
    skos:historyNote "Compiled by the Geological Survey of Queensland" ;
    rdfs:isDefinedBy cs: ;
    skos:definition "A geographic subdivision or district used in rural and regional Australia. Localities are commonly based on a local feature or township, but some occurrences may be subjectively named."@en ;
    skos:inScheme cs: ;
    skos:prefLabel "Locality"@en ;
    skos:topConceptOf cs: ;
.

svydt:total-stations
    a skos:Concept ;
    skos:historyNote "Compiled by the Geological Survey of Queensland" ;
    rdfs:isDefinedBy cs: ;
    skos:definition "Number of stations included in survey"@en ;
    skos:inScheme cs: ;
    skos:prefLabel "Total Stations"@en ;
    skos:topConceptOf cs: ;
.

<https://linked.data.gov.au/org/gsq>
    a sdo:Organization ;
    sdo:name "Geological Survey of Queensland" ;
    sdo:url "https://www.business.qld.gov.au/industries/mining-energy-water/resources/geoscience-information/gsq"^^xsd:anyURI ;
.

svydt:line-direction-degrees
    a skos:Concept ;
    skos:historyNote "Compiled by the Geological Survey of Queensland" ;
    rdfs:isDefinedBy cs: ;
    skos:definition "Mean survey line direction (bearing) from true north.  Values between 000-359 degrees"@en ;
    skos:inScheme cs: ;
    skos:prefLabel "Line Direction (degrees)"@en ;
    skos:topConceptOf cs: ;
.

svydt:survey-height-m
    a skos:Concept ;
    skos:historyNote "Compiled by the Geological Survey of Queensland" ;
    rdfs:isDefinedBy cs: ;
    skos:altLabel "terrain clearance"@en ;
    skos:definition "Mean survey height above ground surface (values in metres relative to AHD)"@en ;
    skos:inScheme cs: ;
    skos:prefLabel "Survey Height (m)"@en ;
    skos:topConceptOf cs: ;
.

svydt:survey-line
    a skos:Concept ;
    skos:historyNote "Compiled by the Geological Survey of Queensland" ;
    rdfs:isDefinedBy cs: ;
    skos:definition "List of survey lines (comma deliminated) included in the survey"@en ;
    skos:inScheme cs: ;
    skos:prefLabel "Survey Line"@en ;
    skos:topConceptOf cs: ;
.

svydt:tie-interval-m
    a skos:Concept ;
    skos:historyNote "Compiled by the Geological Survey of Queensland" ;
    rdfs:isDefinedBy cs: ;
    skos:altLabel "tie line spacing"@en ;
    skos:definition "Mean distance in metres between survey tie lines (if used) in regularly spaced survey"@en ;
    skos:inScheme cs: ;
    skos:prefLabel "Tie Interval (m)"@en ;
    skos:topConceptOf cs: ;
.

svydt:tie-line-direction-degrees
    a skos:Concept ;
    skos:historyNote "Compiled by the Geological Survey of Queensland" ;
    rdfs:isDefinedBy cs: ;
    skos:definition "Mean survey tie line direction (bearing) from true north (often perpendicular to line direction).  Values between 000-359"@en ;
    skos:inScheme cs: ;
    skos:prefLabel "Tie Line Direction (degrees)"@en ;
    skos:topConceptOf cs: ;
.

svydt:vessel-name
    a skos:Concept ;
    skos:historyNote "Compiled by the Geological Survey of Queensland" ;
    rdfs:isDefinedBy cs: ;
    skos:definition "Name, or call sign, of survey vessel (plane, helicopter, boat).  Further information on vessel may also be added"@en ;
    skos:inScheme cs: ;
    skos:prefLabel "Vessel Name"@en ;
    skos:topConceptOf cs: ;
.

svydt:interval-m
    a skos:Concept ;
    skos:historyNote "Compiled by the Geological Survey of Queensland" ;
    rdfs:isDefinedBy cs: ;
    skos:altLabel
        "line spacing"@en ,
        "station spacing"@en ;
    skos:definition "Mean distance in metres between survey lines or stations for a regularly spaced survey"@en ;
    skos:inScheme cs: ;
    skos:prefLabel "Interval (m)"@en ;
    skos:topConceptOf cs: ;
.

svydt:total-area-square-kilometres
    a skos:Concept ;
    skos:historyNote "Compiled by the Geological Survey of Queensland" ;
    rdfs:isDefinedBy cs: ;
    skos:definition "Total surface areal coverage of the survey in square kilometres."@en ;
    skos:inScheme cs: ;
    skos:prefLabel "Total Area Square Kilometres"@en ;
    skos:topConceptOf cs: ;
.

svydt:total-line-kilometres
    a skos:Concept ;
    skos:historyNote "Compiled by the Geological Survey of Queensland" ;
    rdfs:isDefinedBy cs: ;
    skos:definition "Sum of the length of lines contained in the survey in kilometres."@en ;
    skos:inScheme cs: ;
    skos:prefLabel "Total Line Kilometres"@en ;
    skos:topConceptOf cs: ;
.

svydt:funding-program
    a skos:Concept ;
    skos:historyNote "Compiled by the Geological Survey of Queensland" ;
    rdfs:isDefinedBy cs: ;
    skos:definition "Government funding program that survey was conducted under"@en ;
    skos:inScheme cs: ;
    skos:prefLabel "Funding program"@en ;
    skos:topConceptOf cs: ;
.

svydt:job-number
    a skos:Concept ;
    skos:historyNote "Compiled by the Geological Survey of Queensland" ;
    rdfs:isDefinedBy cs: ;
    skos:definition "Survey contractors job number / job identification"@en ;
    skos:inScheme cs: ;
    skos:prefLabel "Job Number"@en ;
    skos:topConceptOf cs: ;
.

svydt:comments
    a skos:Concept ;
    skos:historyNote "Compiled by the Geological Survey of Queensland" ;
    rdfs:isDefinedBy cs: ;
    skos:definition "Free text comments or notes regarding survey"@en ;
    skos:inScheme cs: ;
    skos:prefLabel "Comments"@en ;
    skos:topConceptOf cs: ;
.

cs:
    a
        owl:Ontology ,
        skos:ConceptScheme ;
    dcterms:created "2020-03-30"^^xsd:date ;
    dcterms:creator <https://linked.data.gov.au/org/gsq> ;
    dcterms:modified "2025-06-17"^^xsd:date ;
    skos:historyNote "Compiled by the Geological Survey of Queensland" ;
    dcterms:publisher <https://linked.data.gov.au/org/gsq> ;
    reg:status agldwgstatus:stable ;
    skos:definition "Miscellaneous Survey Details."@en ;
    skos:hasTopConcept
        svydt:active-period ,
        svydt:ag-survey-type ,
        svydt:comments ,
        svydt:full-time-contractors ,
        svydt:full-time-employees ,
        svydt:funding-program ,
        svydt:historic-tenure ,
        svydt:historic-title ,
        svydt:interval-m ,
        svydt:job-number ,
        svydt:line-direction-degrees ,
        svydt:locality ,
        svydt:report-period-freight-cost ,
        svydt:survey-height-m ,
        svydt:survey-line ,
        svydt:tie-interval-m ,
        svydt:tie-line-direction-degrees ,
        svydt:total-area-square-kilometres,
        svydt:total-line-kilometres ,
        svydt:total-stations ,
        svydt:vessel-name ;
    skos:prefLabel "Survey Detail Type"@en ;
.

