PREFIX dcterms: <http://purl.org/dc/terms/>
PREFIX owl: <http://www.w3.org/2002/07/owl#>
PREFIX sdo: <http://schema.org/>
PREFIX skos: <http://www.w3.org/2004/02/skos/core#>
PREFIX svymh: <https://linked.data.gov.au/def/survey-method/>
PREFIX xsd: <http://www.w3.org/2001/XMLSchema#>

svymh:airship
    a skos:Concept ;
    dcterms:provenance "Compiled by the Geological Survey of Queensland" ;
    skos:altLabel
        "Air Ship"@en ,
        "Air-Ship"@en ,
        "Dirigible"@en ,
        "Zeppelin"@en ;
    skos:broader svymh:airborne ;
    skos:definition "A lighter-than-air flying machine that generates lift using buoyancy and has a means to propel and direct itself through the air under its own power, such as a rotor."@en ;
    skos:inScheme <https://linked.data.gov.au/def/survey-method> ;
    skos:prefLabel "Airship"@en ;
.

svymh:balloon
    a skos:Concept ;
    dcterms:provenance "Compiled by the Geological Survey of Queensland" ;
    skos:altLabel
        "Gas Balloon"@en ,
        "Hot Air Balloon"@en ,
        "Hot-Air Balloon"@en ;
    skos:broader svymh:airborne ;
    skos:definition "A lighter-than-air flying machine that generates lift using buoyancy and lacks a means to propel and direct itself through the air. A balloon may be free, moving with the wind, or tethered to a fixed point. "@en ;
    skos:inScheme <https://linked.data.gov.au/def/survey-method> ;
    skos:prefLabel "Balloon"@en ;
.

svymh:boat
    a skos:Concept ;
    dcterms:provenance "Compiled by the Geological Survey of Queensland" ;
    skos:altLabel
        "Hovercraft"@en ,
        "Motorboat"@en ,
        "Sailboat"@en ,
        "Ship"@en ;
    skos:broader svymh:marine ;
    skos:definition "A marine survey where data is acquired from instruments attached to a mobile water craft on the water's surface."@en ;
    skos:inScheme <https://linked.data.gov.au/def/survey-method> ;
    skos:prefLabel "Boat"@en ;
.

svymh:data-survey
    a skos:Concept ;
    dcterms:provenance "Compiled by the Geological Survey of Queensland" ;
    skos:altLabel
        "Desktop Study"@en ,
        "Desktop Survey"@en ;
    skos:definition "Any set of multiple observations or records that group together data from intangible activities and transactions such as: sales; analysis of pre-existing data; metanalyses; behavioural, personal and corporate interactions. A survey that examines activities that are not exclusively confined to primary data capture."@en ;
    skos:inScheme <https://linked.data.gov.au/def/survey-method> ;
    skos:prefLabel "Data Survey"@en ;
    skos:topConceptOf <https://linked.data.gov.au/def/survey-method> ;
.

svymh:diver
    a skos:Concept ;
    dcterms:provenance "Compiled by the Geological Survey of Queensland" ;
    skos:altLabel
        "SCUBA"@en ,
        "SCUBA Diver"@en ;
    skos:broader svymh:marine ;
    skos:definition "A marine survey where data is acquired by a human conveying the instruments of measurement."@en ;
    skos:inScheme <https://linked.data.gov.au/def/survey-method> ;
    skos:prefLabel "Diver"@en ;
.

svymh:fixed-location
    a skos:Concept ;
    dcterms:provenance "Compiled by the Geological Survey of Queensland" ;
    skos:altLabel "Permanent Location"@en ;
    skos:definition "Surveys undertaken at ground level from a set of fixed locations."@en ;
    skos:inScheme <https://linked.data.gov.au/def/survey-method> ;
    skos:prefLabel "Fixed location"@en ;
    skos:topConceptOf <https://linked.data.gov.au/def/survey-method> ;
.

svymh:fixed-wing
    a skos:Concept ;
    dcterms:provenance "Compiled by the Geological Survey of Queensland" ;
    skos:altLabel
        "Aeroplane"@en ,
        "Airplane"@en ,
        "Glider"@en ;
    skos:broader svymh:airborne ;
    skos:definition "A heavier-than-air flying machine that is capable of flight using wings that generate lift caused by the aircraft's forward airspeed and the shape of the wings. Source:Wikipedia"@en ;
    skos:inScheme <https://linked.data.gov.au/def/survey-method> ;
    skos:prefLabel "Fixed Wing"@en ;
.

svymh:float
    a skos:Concept ;
    dcterms:provenance "Compiled by the Geological Survey of Queensland" ;
    skos:altLabel
        "Floating Dock"@en ,
        "Floating Jetty"@en ,
        "Floating Pier"@en ,
        "Pontoon"@en ;
    skos:broader svymh:marine ;
    skos:definition "A marine survey where data is acquired from instruments operated from a fixed, buoyant, structure at the water's surface."@en ;
    skos:inScheme <https://linked.data.gov.au/def/survey-method> ;
    skos:prefLabel "Float"@en ;
.

svymh:human
    a skos:Concept ;
    dcterms:provenance "Compiled by the Geological Survey of Queensland" ;
    skos:altLabel
        "Field Work"@en ,
        "In Person"@en ,
        "Manual"@en ;
    skos:broader svymh:ground ;
    skos:definition "A ground based survey where data is acquired from a human conducting work on-foot."@en ;
    skos:inScheme <https://linked.data.gov.au/def/survey-method> ;
    skos:prefLabel "Human"@en ;
.

svymh:mwd
    a skos:Concept ;
    dcterms:provenance "Compiled by the Geological Survey of Queensland" ;
    skos:altLabel
        "M.W.D"@en ,
        "M.W.D."@en ,
        "MWD"@en ;
    skos:broader svymh:downhole ;
    skos:definition "A survey where data is acquired while the hole is being drilled, from sensors integrated within the drill string ."@en ;
    skos:hiddenLabel
        "L.W.D"@en ,
        "L.W.D."@en ,
        "LWD"@en ,
        "Logging While Drilling"@en ;
    skos:inScheme <https://linked.data.gov.au/def/survey-method> ;
    skos:prefLabel "Measurement While Drilling"@en ;
.

svymh:pipe-conveyed
    a skos:Concept ;
    dcterms:provenance "Compiled by the Geological Survey of Queensland" ;
    skos:altLabel
        "on pipe"@en ,
        "on-pipe"@en ;
    skos:broader svymh:downhole ;
    skos:definition "A survey where data is acquired from logging tools attached to the drill string, while the well is not actively drilling."@en ;
    skos:inScheme <https://linked.data.gov.au/def/survey-method> ;
    skos:prefLabel "Pipe Conveyed"@en ;
.

svymh:rotary-wing
    a skos:Concept ;
    dcterms:provenance "Compiled by the Geological Survey of Queensland" ;
    skos:altLabel
        "Autogyro"@en ,
        "Gyrodyne"@en ,
        "Helicopter"@en ,
        "Rotorcraft"@en ;
    skos:broader svymh:airborne ;
    skos:definition "A heavier-than-air flying machine that generates lift using rotary wings or rotor blades, which revolve around a mast."@en ;
    skos:inScheme <https://linked.data.gov.au/def/survey-method> ;
    skos:prefLabel "Rotary Wing"@en ;
.

svymh:submarine
    a skos:Concept ;
    dcterms:provenance "Compiled by the Geological Survey of Queensland" ;
    skos:altLabel
        "Sub"@en ,
        "Submersible"@en ,
        "Underwater"@en ;
    skos:broader svymh:marine ;
    skos:definition "A marine survey where data is acquired by a human piloted watercraft operating under the surface of the water. Surveys may be performed by submarines or submersibles."@en ;
    skos:inScheme <https://linked.data.gov.au/def/survey-method> ;
    skos:prefLabel "Submarine"@en ;
.

svymh:uav
    a skos:Concept ;
    dcterms:provenance "Compiled by the Geological Survey of Queensland" ;
    skos:altLabel
        "Aerial Drone"@en ,
        "UAV"@en ,
        "Uncrewed aerial vehicle"@en ;
    skos:broader svymh:airborne ;
    skos:definition "An aircraft without a human pilot on board and a type of unmanned vehicle. UAVs may operate with various degrees of autonomy: either under remote control by a human operator or autonomously by onboard computers."@en ;
    skos:inScheme <https://linked.data.gov.au/def/survey-method> ;
    skos:prefLabel "Drone"@en ;
.

svymh:uuv
    a skos:Concept ;
    dcterms:provenance "Compiled by the Geological Survey of Queensland" ;
    skos:altLabel
        "AUV"@en ,
        "Autonomous underwater vehicle"@en ,
        "ROUV"@en ,
        "UUV"@en ,
        "Underwater Drone"@en ,
        "remotely operated underwater vehicles"@en ;
    skos:broader svymh:marine ;
    skos:definition "A marine survey where data is acquired by a watercraft, without an onboard human pilot, operating under the surface of the water."@en ;
    skos:inScheme <https://linked.data.gov.au/def/survey-method> ;
    skos:prefLabel "Unmanned underwater vehicle"@en ;
.

svymh:vehicle
    a skos:Concept ;
    dcterms:provenance "Compiled by the Geological Survey of Queensland" ;
    skos:altLabel
        "Car"@en ,
        "Truck"@en ,
        "Ute"@en ,
        "Vehicle Conveyed"@en ;
    skos:broader svymh:ground ;
    skos:definition "A ground based survey where data is acquired from instruments mounted to a vehicle."@en ;
    skos:inScheme <https://linked.data.gov.au/def/survey-method> ;
    skos:prefLabel "Vehicle"@en ;
.

svymh:well-tractor
    a skos:Concept ;
    dcterms:provenance "Compiled by the Geological Survey of Queensland" ;
    skos:altLabel "borehole tractor"@en ;
    skos:broader svymh:downhole ;
    skos:definition "A survey where data is acquired from logging tools integrated in a Well Tractor, a device that moves through a wellbore using wheels or tracks pushed against the side of the borehole."@en ;
    skos:inScheme <https://linked.data.gov.au/def/survey-method> ;
    skos:prefLabel "Well Tractor"@en ;
.

svymh:wireline
    a skos:Concept ;
    dcterms:provenance "Compiled by the Geological Survey of Queensland" ;
    skos:altLabel "wireline logging"@en ;
    skos:broader svymh:downhole ;
    skos:definition "A survey where data is acquired from logging tools lowered and raised within a borehole on a wireline or cable."@en ;
    skos:inScheme <https://linked.data.gov.au/def/survey-method> ;
    skos:prefLabel "Wireline"@en ;
.

svymh:laboratory
    a skos:Concept ;
    dcterms:provenance "Compiled by the Geological Survey of Queensland" ;
    skos:altLabel
        "Lab"@en ,
        "Mobile"@en ,
        "Mobile Lab"@en ,
        "Rig Site"@en ;
    skos:definition "Surveys undertaken on samples that are no-longer in-situ e.g. spectral surveys of core by hylogger in a laboratory, CoreScan in a rig site, XRF analysis of collected samples."@en ;
    skos:inScheme <https://linked.data.gov.au/def/survey-method> ;
    skos:prefLabel "Laboratory"@en ;
    skos:topConceptOf <https://linked.data.gov.au/def/survey-method> ;
.

svymh:satellite
    a skos:Concept ;
    dcterms:provenance "Compiled by the Geological Survey of Queensland" ;
    skos:definition "Surveys in which the surveying equipment is mounted to a platform outside the earth's atmosphere. Typically in a stable orbit such as a satellite, space station, or shuttle."@en ;
    skos:inScheme <https://linked.data.gov.au/def/survey-method> ;
    skos:prefLabel "Satellite"@en ;
    skos:topConceptOf <https://linked.data.gov.au/def/survey-method> ;
.

<https://linked.data.gov.au/org/gsq>
    a sdo:Organization ;
    sdo:name "Geological Survey of Queensland" ;
    sdo:url "http://www.business.qld.gov.au/industries/mining-energy-water/resources/geoscience-information/gsq"^^xsd:anyURI ;
.

svymh:ground
    a skos:Concept ;
    dcterms:provenance "Compiled by the Geological Survey of Queensland" ;
    skos:altLabel "Land"@en ;
    skos:definition "Surveys undertaken at ground level or a solid subsurface level such as an underground mine floor. This may include surface collection of rocks, soil, water or other physical samples; geophysical surveys from surface locations; handheld photography."@en ;
    skos:inScheme <https://linked.data.gov.au/def/survey-method> ;
    skos:prefLabel "Ground"@en ;
    skos:topConceptOf <https://linked.data.gov.au/def/survey-method> ;
.

svymh:downhole
    a skos:Concept ;
    dcterms:provenance "Compiled by the Geological Survey of Queensland" ;
    skos:altLabel "Borehole"@en ;
    skos:definition "Surveys where equipment is conveyed down a borehole to record measurements of borehole, rock, or fluid attributes."@en ;
    skos:inScheme <https://linked.data.gov.au/def/survey-method> ;
    skos:prefLabel "Downhole"@en ;
    skos:topConceptOf <https://linked.data.gov.au/def/survey-method> ;
.

svymh:airborne
    a skos:Concept ;
    dcterms:provenance "Compiled by the Geological Survey of Queensland" ;
    skos:altLabel "Aerial"@en ;
    skos:definition "Surveys in which the surveying equipment is mounted to an aircraft such as an airplane, helicopter, balloon, or aerial drone."@en ;
    skos:inScheme <https://linked.data.gov.au/def/survey-method> ;
    skos:prefLabel "Airborne"@en ;
    skos:topConceptOf <https://linked.data.gov.au/def/survey-method> ;
.

svymh:marine
    a skos:Concept ;
    dcterms:provenance "Compiled by the Geological Survey of Queensland" ;
    skos:altLabel
        "Oceanic"@en ,
        "On Water"@en ,
        "Sea"@en ;
    skos:definition "Surveys undertaken at or below the surface of a body of water such as an ocean, sea, or lake."@en ;
    skos:inScheme <https://linked.data.gov.au/def/survey-method> ;
    skos:prefLabel "Marine"@en ;
    skos:topConceptOf <https://linked.data.gov.au/def/survey-method> ;
.

<https://linked.data.gov.au/def/survey-method>
    a
        owl:Ontology ,
        skos:ConceptScheme ;
    dcterms:created "2020-02-10"^^xsd:date ;
    dcterms:creator <https://linked.data.gov.au/org/gsq> ;
    dcterms:modified "2020-05-14"^^xsd:date ;
    dcterms:provenance "Compiled by the Geological Survey of Queensland" ;
    dcterms:publisher <https://linked.data.gov.au/org/gsq> ;
    skos:definition "The method of collection used by a survey."@en ;
    skos:hasTopConcept
        svymh:airborne ,
        svymh:downhole ,
        svymh:ground ,
        svymh:laboratory ,
        svymh:marine ,
        svymh:satellite ;
    skos:prefLabel "Survey Method"@en ;
.

